@prefix aat: <http://vocab.getty.edu/aat/> .
@prefix aat_contrib: <http://vocab.getty.edu/aat/contrib/> .
@prefix aat_rel: <http://vocab.getty.edu/aat/rel/> .
@prefix aat_rev: <http://vocab.getty.edu/aat/rev/> .
@prefix aat_scopeNote: <http://vocab.getty.edu/aat/scopeNote/> .
@prefix aat_source: <http://vocab.getty.edu/aat/source/> .
@prefix aat_source_rev: <http://vocab.getty.edu/aat/source/rev/> .
@prefix aat_term: <http://vocab.getty.edu/aat/term/> .
@prefix adms: <http://www.w3.org/ns/adms#> .
@prefix bibo: <http://purl.org/ontology/bibo/> .
@prefix bio: <http://purl.org/vocab/bio/0.1/> .
@prefix cc: <http://creativecommons.org/ns#> .
@prefix dc: <http://purl.org/dc/elements/1.1/> .
@prefix dcat: <http://www.w3.org/ns/dcat#> .
@prefix dct: <http://purl.org/dc/terms/> .
@prefix dctype: <http://purl.org/dc/dcmitype/> .
@prefix fmt: <http://www.w3.org/ns/formats/> .
@prefix foaf: <http://xmlns.com/foaf/0.1/> .
@prefix gvp: <http://vocab.getty.edu/ontology#> .
@prefix gvp_lang: <http://vocab.getty.edu/language/> .
@prefix iso: <http://purl.org/iso25964/skos-thes#> .
@prefix luc: <http://www.ontotext.com/owlim/lucene#> .
@prefix ontogeo: <http://www.ontotext.com/owlim/geo#> .
@prefix owl: <http://www.w3.org/2002/07/owl#> .
@prefix prov: <http://www.w3.org/ns/prov#> .
@prefix ptop: <http://www.ontotext.com/proton/protontop#> .
@prefix rdf: <http://www.w3.org/1999/02/22-rdf-syntax-ns#> .
@prefix rdfs: <http://www.w3.org/2000/01/rdf-schema#> .
@prefix rr: <http://www.w3.org/ns/r2rml#> .
@prefix rrx: <http://purl.org/r2rml-ext/> .
@prefix schema: <http://schema.org/> .
@prefix sd: <http://www.w3.org/ns/sparql-service-description#> .
@prefix sesame: <http://www.openrdf.org/schema/sesame#> .
@prefix skos: <http://www.w3.org/2004/02/skos/core#> .
@prefix skosxl: <http://www.w3.org/2008/05/skos-xl#> .
@prefix tgn: <http://vocab.getty.edu/tgn/> .
@prefix tgn_contrib: <http://vocab.getty.edu/tgn/contrib/> .
@prefix tgn_rel: <http://vocab.getty.edu/tgn/rel/> .
@prefix tgn_rev: <http://vocab.getty.edu/tgn/rev/> .
@prefix tgn_scopeNote: <http://vocab.getty.edu/tgn/scopeNote/> .
@prefix tgn_source: <http://vocab.getty.edu/tgn/source/> .
@prefix tgn_source_rev: <http://vocab.getty.edu/tgn/source/rev/> .
@prefix tgn_term: <http://vocab.getty.edu/tgn/term/> .
@prefix ulan: <http://vocab.getty.edu/ulan/> .
@prefix ulan_bio: <http://vocab.getty.edu/ulan/bio/> .
@prefix ulan_contrib: <http://vocab.getty.edu/ulan/contrib/> .
@prefix ulan_event: <http://vocab.getty.edu/ulan/event/> .
@prefix ulan_rel: <http://vocab.getty.edu/ulan/rel/> .
@prefix ulan_rev: <http://vocab.getty.edu/ulan/rev/> .
@prefix ulan_scopeNote: <http://vocab.getty.edu/ulan/scopeNote/> .
@prefix ulan_source: <http://vocab.getty.edu/ulan/source/> .
@prefix ulan_source_rev: <http://vocab.getty.edu/ulan/source/rev/> .
@prefix ulan_term: <http://vocab.getty.edu/ulan/term/> .
@prefix vaem: <http://www.linkedmodel.org/schema/vaem#> .
@prefix vann: <http://purl.org/vocab/vann/> .
@prefix vcard: <http://www.w3.org/2006/vcard/ns#> .
@prefix vdpp: <http://data.lirmm.fr/ontologies/vdpp#> .
@prefix voaf: <http://purl.org/vocommons/voaf#> .
@prefix voag: <http://voag.linkedmodel.org/voag#> .
@prefix void: <http://rdfs.org/ns/void#> .
@prefix wdrs: <http://www.w3.org/2007/05/powder-s#> .
@prefix wgs: <http://www.w3.org/2003/01/geo/wgs84_pos#> .
@prefix wv: <http://vocab.org/waiver/terms/> .
@prefix xml: <http://www.w3.org/XML/1998/namespace> .
@prefix xsd: <http://www.w3.org/2001/XMLSchema#> .

dct:isReplacedBy owl:inverseOf dct:replaces .

gvp:Infer_broaderNonConcept_PropChainType2 a ptop:PropChainType2 ;
    ptop:conclusion gvp:broaderNonConcept ;
    ptop:premise1 gvp:broaderNonConcept ;
    ptop:premise2 gvp:broader ;
    ptop:type2 gvp:GuideTerm .

gvp:Infer_broaderNonConcept_TypeRestr a ptop:TypeRestr ;
    ptop:conclusion gvp:broaderNonConcept ;
    ptop:premise gvp:broader ;
    ptop:type1 skos:Concept ;
    ptop:type2 gvp:GuideTerm .

gvp:Infer_broaderPreferredExtended a ptop:PropChainRestr ;
    ptop:conclusion gvp:broaderPreferredExtended ;
    ptop:premise1 gvp:broaderPreferredExtended ;
    ptop:premise2 gvp:broaderPreferred ;
    ptop:restriction gvp:broaderExtended .

gvp:Infer_isoBroaderGeneric a ptop:PropRestr ;
    ptop:conclusion iso:broaderGeneric ;
    ptop:premise gvp:broaderGenericExtended ;
    ptop:restriction skos:broader .

gvp:Infer_isoBroaderInstantial a ptop:PropRestr ;
    ptop:conclusion iso:broaderInstantial ;
    ptop:premise gvp:broaderInstantialExtended ;
    ptop:restriction skos:broader .

gvp:Infer_isoBroaderPartitive a ptop:PropRestr ;
    ptop:conclusion iso:broaderPartitive ;
    ptop:premise gvp:broaderPartitiveExtended ;
    ptop:restriction skos:broader .

gvp:Infer_skosBroader_PropChainType2 a ptop:PropChainType2 ;
    ptop:conclusion skos:broader ;
    ptop:premise1 gvp:broaderNonConcept ;
    ptop:premise2 gvp:broader ;
    ptop:type2 skos:Concept .

gvp:Infer_skosBroader_TypeRestr a ptop:TypeRestr ;
    ptop:conclusion skos:broader ;
    ptop:premise gvp:broader ;
    ptop:type1 skos:Concept ;
    ptop:type2 skos:Concept .

skos:altLabel owl:propertyChainAxiom ( skosxl:altLabel skosxl:literalForm ) .

skos:hiddenLabel owl:propertyChainAxiom ( skosxl:hiddenLabel skosxl:literalForm ) .

skos:prefLabel owl:propertyChainAxiom ( skosxl:prefLabel skosxl:literalForm ) .

<http://rdaregistry.info/termList/gender/1001> skos:exactMatch <http://vocab.getty.edu/aat/300189557> .

<http://rdaregistry.info/termList/gender/1002> skos:exactMatch <http://vocab.getty.edu/aat/300189559> .

schema:dissolutionLocation a owl:ObjectProperty,
        skos:Concept ;
    rdfs:label "dissolutionLocation"@en ;
    dct:description """The place where the Organization was dissolved.
Schema has properties foundationLocation and dissolutionDate but no dissolutionLocation. 
In contrast, for a person all 4 properties are present: birth/death place/date.
We posted issue https://github.com/schemaorg/schemaorg/issues/302, which looks like it will have a positive outcome in the far future.
And we define the property here""" ;
    rdfs:comment "The place where the Organization was dissolved" ;
    rdfs:domain schema:Organization ;
    rdfs:isDefinedBy <http://vocab.getty.edu/ontology> ;
    rdfs:range schema:Place ;
    rdfs:seeAlso <https://github.com/schemaorg/schemaorg/issues/302> ;
    skos:inScheme <http://vocab.getty.edu/ontology> ;
    skos:prefLabel "dissolutionLocation"@en ;
    skos:topConceptOf <http://vocab.getty.edu/ontology> .

<http://vocab.getty.edu/historic/current> a skos:Concept ;
    dct:description "Valid/used currently" ;
    skos:inScheme <http://vocab.getty.edu/historic/> ;
    skos:notation "C" ;
    skos:prefLabel "Current"@en ;
    skos:scopeNote "Valid/used currently" ;
    skos:topConceptOf <http://vocab.getty.edu/historic/> .

<http://vocab.getty.edu/historic/currentAndHistoric> a skos:Concept ;
    dct:description """Valid/used both in the past and currently.
Example: Saint Petersburg (TGN)""" ;
    skos:example "Saint Petersburg (TGN)" ;
    skos:inScheme <http://vocab.getty.edu/historic/> ;
    skos:notation "B" ;
    skos:prefLabel "Both Current and Historic"@en ;
    skos:scopeNote "Valid/used both in the past and currently" ;
    skos:topConceptOf <http://vocab.getty.edu/historic/> .

<http://vocab.getty.edu/historic/historic> a skos:Concept ;
    dct:description """Valid/used in the past but not currently.
Example: "Lutetia" is a historic name for "Paris" (TGN). "weyneschot" is a 16th-century spelling for "wainscoting" (AAT)""" ;
    skos:example "\"Lutetia\" is a historic name for \"Paris\" (TGN). \"weyneschot\" is a 16th-century spelling for \"wainscoting\" (AAT)" ;
    skos:inScheme <http://vocab.getty.edu/historic/> ;
    skos:notation "H" ;
    skos:prefLabel "Historic"@en ;
    skos:scopeNote "Valid/used in the past but not currently" ;
    skos:topConceptOf <http://vocab.getty.edu/historic/> .

<http://vocab.getty.edu/historic/localUse> a skos:Concept ;
    dct:description """Used locally for Unidentified Named People mentioned in some document (ULAN only).
Example: 500051176 Abinetti (ULAN) is an unknown artist mentioned in documentation of lot 209 of an auction held 29 Jan 1824 in London""" ;
    skos:example "500051176 Abinetti (ULAN) is an unknown artist mentioned in documentation of lot 209 of an auction held 29 Jan 1824 in London" ;
    skos:inScheme <http://vocab.getty.edu/historic/> ;
    skos:notation "LU" ;
    skos:prefLabel "Local Use"@en ;
    skos:scopeNote "Used locally for Unidentified Named People mentioned in some document (ULAN only)" ;
    skos:topConceptOf <http://vocab.getty.edu/historic/> .

gvp:ScopeNote a owl:Class,
        skos:Concept ;
    dct:description """Defines a GVP subject or provides usage information. Has fields:
- dc:identifier: numeric ID, also used in the URL.
- rdf:value: the note itself (as per SKOS Primer: 4.2 Advanced Documentation Features) with language tag
- dct:language: matches the language tag
- gvp:displayOrder, order of this note amongst others
- gvp:historicFlag, vp:estStart, gvp:estEnd, rdfs:comment: Historic Information about applicability
- dct:source or subproperties thereof 
- dct:contributor or subproperties thereof""" ;
    rdfs:comment """Defines a GVP subject or provides usage information. Has fields:
- dc:identifier: numeric ID, also used in the URL.
- rdf:value: the note itself (as per SKOS Primer: 4.2 Advanced Documentation Features) with language tag
- dct:language: matches the language tag
- gvp:displayOrder, order of this note amongst others
- gvp:historicFlag, gvp:estStart, gvp:estEnd, rdfs:comment: Historic Information about applicability
- dct:source or subproperties thereof 
- dct:contributor or subproperties thereof""" ;
    rdfs:isDefinedBy <http://vocab.getty.edu/ontology> ;
    skos:inScheme <http://vocab.getty.edu/ontology> ;
    skos:topConceptOf <http://vocab.getty.edu/ontology> .

gvp:displayOrder a owl:DatatypeProperty ;
    rdfs:label "displayOrder"@en ;
    dct:description """Display order of subject or term amongst its siblings.
If all are 1 then use alphabetical. Domain is gvp:Subject or skosxl:Label""" ;
    rdfs:comment """Display order of subject or term amongst its siblings.
If all are 1 then use alphabetical. Domain is gvp:Subject or skosxl:Label""" ;
    rdfs:isDefinedBy <http://vocab.getty.edu/ontology> ;
    rdfs:range xsd:positiveInteger ;
    skos:inScheme <http://vocab.getty.edu/ontology> ;
    skos:prefLabel "displayOrder"@en ;
    skos:topConceptOf <http://vocab.getty.edu/ontology> .

gvp:estEnd a owl:DatatypeProperty ;
    rdfs:label "estEnd"@en ;
    dct:description "Estimated end date of term, relation, type assignment, event, biography" ;
    rdfs:comment "Estimated end date of term, relation, type assignment, event, biography" ;
    rdfs:isDefinedBy <http://vocab.getty.edu/ontology> ;
    skos:inScheme <http://vocab.getty.edu/ontology> ;
    skos:prefLabel "estEnd"@en ;
    skos:topConceptOf <http://vocab.getty.edu/ontology> .

gvp:estStart a owl:DatatypeProperty ;
    rdfs:label "estStart"@en ;
    dct:description "Estimated start date of term, relation, type assignment, event, biography" ;
    rdfs:comment "Estimated start date of term, relation, type assignment, event, biography" ;
    rdfs:isDefinedBy <http://vocab.getty.edu/ontology> ;
    skos:inScheme <http://vocab.getty.edu/ontology> ;
    skos:prefLabel "estStart"@en ;
    skos:topConceptOf <http://vocab.getty.edu/ontology> .

gvp:historicFlag a owl:ObjectProperty,
        skos:Concept ;
    rdfs:label "historicFlag"@en ;
    dct:description "Historic Flag" ;
    rdfs:isDefinedBy <http://vocab.getty.edu/ontology> ;
    rdfs:range skos:Concept ;
    skos:inScheme <http://vocab.getty.edu/ontology> ;
    skos:prefLabel "historicFlag"@en ;
    skos:topConceptOf <http://vocab.getty.edu/ontology> .

gvp:isNoted a owl:DatatypeProperty ;
    rdfs:label "isNoted"@en ;
    dct:description """One amongst several homographic concepts may be especially noted so it's easier to find.
Example: tgn:7008038 Paris, France is noted but tgn:2106600 Paris, Texas is not (except if you're Fassbinder)""" ;
    rdfs:comment "One amongst several homographic concepts may be especially noted so it's easier to find" ;
    rdfs:domain gvp:Subject ;
    rdfs:isDefinedBy <http://vocab.getty.edu/ontology> ;
    rdfs:range xsd:boolean ;
    skos:example "tgn:7008038 Paris, France is noted but tgn:2106600 Paris, Texas is not (except if you're Fassbinder)" ;
    skos:inScheme <http://vocab.getty.edu/ontology> ;
    skos:prefLabel "isNoted"@en ;
    skos:topConceptOf <http://vocab.getty.edu/ontology> .

gvp:parentString a owl:DatatypeProperty ;
    rdfs:label "parentString"@en ;
    dct:description """Preferred labels of *all* of the subject's preferred ancestors, listed bottom up. Useful to show the subject's full context.
Display version of gvp:broaderPreferredExtended.
For aat:300226882 baking dishes: bakeware, <vessels for cooking food>, <containers for cooking food>, <culinary containers>, <containers by function or context>, containers (receptacles), Containers (Hierarchy Name), Furnishings and Equipment (Hierarchy Name), Objects Facet""" ;
    rdfs:comment "Preferred labels of *all* of the subject's preferred ancestors, listed bottom up. Useful to show the subject's full context" ;
    rdfs:domain gvp:Subject ;
    rdfs:isDefinedBy <http://vocab.getty.edu/ontology> ;
    rdfs:range rdf:Literal ;
    skos:example "For aat:300226882 baking dishes: bakeware, <vessels for cooking food>, <containers for cooking food>, <culinary containers>, <containers by function or context>, containers (receptacles), Containers (Hierarchy Name), Furnishings and Equipment (Hierarchy Name), Objects Facet" ;
    skos:inScheme <http://vocab.getty.edu/ontology> ;
    skos:note "Display version of gvp:broaderPreferredExtended" ;
    skos:prefLabel "parentString"@en ;
    skos:topConceptOf <http://vocab.getty.edu/ontology> .

gvp:parentStringAbbrev a owl:DatatypeProperty ;
    rdfs:label "parentStringAbbrev"@en ;
    dct:description """Preferred labels of *some* of the subject's preferred ancestors, listed bottom up. Useful to show the subject's context.
Shortened display version of gvp:broaderPreferredExtended.
Example for aat:300226882 baking dishes: bakeware, <vessels for cooking food>, ... Furnishings and Equipment (Hierarchy Name)""" ;
    rdfs:comment "Preferred labels of *some* of the subject's preferred ancestors, listed bottom up. Useful to show the subject's context" ;
    rdfs:domain gvp:Subject ;
    rdfs:isDefinedBy <http://vocab.getty.edu/ontology> ;
    rdfs:range rdf:Literal ;
    skos:example "For aat:300226882 baking dishes: bakeware, <vessels for cooking food>, ... Furnishings and Equipment (Hierarchy Name)" ;
    skos:inScheme <http://vocab.getty.edu/ontology> ;
    skos:note "Shortened display version of gvp:broaderPreferredExtended" ;
    skos:prefLabel "parentStringAbbrev"@en ;
    skos:topConceptOf <http://vocab.getty.edu/ontology> .

gvp:prefLabelGVP a owl:ObjectProperty,
        skos:Concept ;
    rdfs:label "prefLabelGVP"@en ;
    dct:description "Term preferred by the Getty Vocabulary Program. The language is usually English. Applicable to AAT, ULAN, TGN. Used with skosxl:prefLabel" ;
    rdfs:comment "Term preferred by the Getty Vocabulary Program. The language is usually English. Applicable to AAT, ULAN, TGN. Used with skosxl:prefLabel" ;
    rdfs:domain gvp:Subject ;
    rdfs:isDefinedBy <http://vocab.getty.edu/ontology> ;
    rdfs:range skosxl:Label ;
    skos:inScheme <http://vocab.getty.edu/ontology> ;
    skos:prefLabel "prefLabelGVP"@en ;
    skos:topConceptOf <http://vocab.getty.edu/ontology> .

gvp:prefLabelLoC a owl:ObjectProperty,
        skos:Concept ;
    rdfs:label "prefLabelLoC"@en ;
    dct:description "Term preferred by Library of Congress, thus used for cataloging according to AACR2. Applicable to AAT and ULAN. Used with skosxl:prefLabel" ;
    rdfs:comment "Term preferred by Library of Congress, thus used for cataloging according to AACR2. Applicable to AAT and ULAN. Used with skosxl:prefLabel" ;
    rdfs:domain gvp:Subject ;
    rdfs:isDefinedBy <http://vocab.getty.edu/ontology> ;
    rdfs:range skosxl:Label ;
    skos:inScheme <http://vocab.getty.edu/ontology> ;
    skos:prefLabel "prefLabelLoC"@en ;
    skos:topConceptOf <http://vocab.getty.edu/ontology> .

gvp:qualifier a owl:DatatypeProperty ;
    rdfs:label "qualifier"@en ;
    dct:description """Clarifies and disambiguates terms with the same spelling but different meaning.
Appended in parentheses to gvp:term, forming skosxsl:literalForm.
Every qualifier is in the same language as the term.
Example: "Rhea (vessels)"=rhyta (a kind of drinking vessel) vs "Rhea (species)"=Boehmeria nivea (Chinese grass)""" ;
    rdfs:comment """Clarifies and disambiguates terms with the same spelling but different meaning.
Appended in parentheses to gvp:term, forming skosxsl:literalForm.
Every qualifier is in the same language as the term""" ;
    rdfs:domain skosxl:Label ;
    rdfs:isDefinedBy <http://vocab.getty.edu/ontology> ;
    rdfs:range rdf:Literal ;
    skos:example "Rhea (vessels)=rhyta (a kind of drinking vessel) vs rhea (species)=Boehmeria nivea (Chinese grass)" ;
    skos:inScheme <http://vocab.getty.edu/ontology> ;
    skos:prefLabel "qualifier"@en ;
    skos:topConceptOf <http://vocab.getty.edu/ontology> .

gvp:term a owl:DatatypeProperty ;
    rdfs:label "term"@en ;
    dct:description "Term (label), used as the basic (prefix) part of skosxsl:literalForm" ;
    rdfs:comment "Term (label), used as the basic (prefix) part of skosxsl:literalForm" ;
    rdfs:domain skosxl:Label ;
    rdfs:isDefinedBy <http://vocab.getty.edu/ontology> ;
    rdfs:range rdf:Literal ;
    skos:inScheme <http://vocab.getty.edu/ontology> ;
    skos:prefLabel "term"@en ;
    skos:topConceptOf <http://vocab.getty.edu/ontology> .

gvp:termDisplay a owl:ObjectProperty,
        skos:Concept ;
    rdfs:label "termDisplay"@en ;
    dct:description "Term Display" ;
    rdfs:domain skosxl:Label ;
    rdfs:isDefinedBy <http://vocab.getty.edu/ontology> ;
    rdfs:range skos:Concept ;
    skos:inScheme <http://vocab.getty.edu/ontology> ;
    skos:prefLabel "termDisplay"@en ;
    skos:topConceptOf <http://vocab.getty.edu/ontology> .

gvp:termFlag a owl:ObjectProperty,
        skos:Concept ;
    rdfs:label "termFlag"@en ;
    dct:description "Term Flag" ;
    rdfs:domain skosxl:Label ;
    rdfs:isDefinedBy <http://vocab.getty.edu/ontology> ;
    rdfs:range skos:Concept ;
    skos:inScheme <http://vocab.getty.edu/ontology> ;
    skos:prefLabel "termFlag"@en ;
    skos:topConceptOf <http://vocab.getty.edu/ontology> .

gvp:termKind a owl:ObjectProperty,
        skos:Concept ;
    rdfs:label "termKind"@en ;
    dct:description "Term Kind" ;
    rdfs:domain skosxl:Label ;
    rdfs:isDefinedBy <http://vocab.getty.edu/ontology> ;
    rdfs:range skos:Concept ;
    skos:inScheme <http://vocab.getty.edu/ontology> ;
    skos:prefLabel "termKind"@en ;
    skos:topConceptOf <http://vocab.getty.edu/ontology> .

gvp:termPOS a owl:ObjectProperty,
        skos:Concept ;
    rdfs:label "termPOS"@en ;
    dct:description "Part of Speech" ;
    rdfs:domain skosxl:Label ;
    rdfs:isDefinedBy <http://vocab.getty.edu/ontology> ;
    rdfs:range skos:Concept ;
    skos:inScheme <http://vocab.getty.edu/ontology> ;
    skos:prefLabel "termPOS"@en ;
    skos:topConceptOf <http://vocab.getty.edu/ontology> .

gvp:termType a owl:ObjectProperty,
        skos:Concept ;
    rdfs:label "termType"@en ;
    dct:description "Term Type" ;
    rdfs:domain skosxl:Label ;
    rdfs:isDefinedBy <http://vocab.getty.edu/ontology> ;
    rdfs:range skos:Concept ;
    skos:inScheme <http://vocab.getty.edu/ontology> ;
    skos:prefLabel "termType"@en ;
    skos:topConceptOf <http://vocab.getty.edu/ontology> .

<http://vocab.getty.edu/term/POS/Adjectival> a skos:Concept ;
    dct:description """This term may be combined with others in post-coordinated compound terms.
Example: "Renaissance" (as in "Renaissance cathedral"), "painter's" (as in "painter's smock")""" ;
    skos:example "\"Renaissance\" (as in \"Renaissance cathedral\"), \"painter's\" (as in \"painter's smock\")" ;
    skos:inScheme <http://vocab.getty.edu/term/POS/> ;
    skos:notation "A" ;
    skos:prefLabel "Adjectival"@en ;
    skos:scopeNote "This term may be combined with others in post-coordinated compound terms" ;
    skos:topConceptOf <http://vocab.getty.edu/term/POS/> .

<http://vocab.getty.edu/term/POS/BothSingularAndPlural> a skos:Concept ;
    dct:description """A term that is used for both the singular and plural in the same language.
Example: "chassis" is both singular and plural in French""" ;
    skos:example "\"chassis\" is both singular and plural in French" ;
    skos:inScheme <http://vocab.getty.edu/term/POS/> ;
    skos:notation "B" ;
    skos:prefLabel "Both Singular and Plural"@en ;
    skos:scopeNote "A term that is used for both the singular and plural in the same language" ;
    skos:topConceptOf <http://vocab.getty.edu/term/POS/> .

<http://vocab.getty.edu/term/POS/Noun> a skos:Concept ;
    dct:description """Term is a noun but we are uncertain if it is plural or singular.
Example: Panthera leo""" ;
    skos:example "Panthera leo" ;
    skos:inScheme <http://vocab.getty.edu/term/POS/> ;
    skos:notation "N" ;
    skos:prefLabel "Noun"@en ;
    skos:scopeNote "Term is a noun but we are uncertain if it is plural or singular" ;
    skos:topConceptOf <http://vocab.getty.edu/term/POS/> .

<http://vocab.getty.edu/term/POS/PastParticiple> a skos:Concept ;
    dct:description """Rarely used but if at all, is most likely to apply in Attributes and Properties.
Example: hand-painted""" ;
    skos:example "hand-painted" ;
    skos:inScheme <http://vocab.getty.edu/term/POS/> ;
    skos:notation "PP" ;
    skos:prefLabel "Past Participle"@en ;
    skos:scopeNote "Rarely used but if at all, is most likely to apply in Attributes and Properties" ;
    skos:topConceptOf <http://vocab.getty.edu/term/POS/> .

<http://vocab.getty.edu/term/POS/PluralNoun> a skos:Concept ;
    dct:description """A term that is plural (the same word may be singular in another language).
Example: "filigrane" is the Italian plural for "watermarks\"""" ;
    skos:example "\"filigrane\" is the Italian plural for \"watermarks\"" ;
    skos:inScheme <http://vocab.getty.edu/term/POS/> ;
    skos:notation "PN" ;
    skos:prefLabel "Plural Noun"@en ;
    skos:scopeNote "A term that is plural (the same word may be singular in another language)" ;
    skos:topConceptOf <http://vocab.getty.edu/term/POS/> .

<http://vocab.getty.edu/term/POS/SingularNoun> a skos:Concept ;
    dct:description """A term that is singular (the same word may be plural in another language).
Example: "filigrane" is the French singular for "watermark\"""" ;
    skos:example "\"filigrane\" is the French singular for \"watermark\"" ;
    skos:inScheme <http://vocab.getty.edu/term/POS/> ;
    skos:notation "SN" ;
    skos:prefLabel "Singular Noun"@en ;
    skos:scopeNote "A term that is singular (the same word may be plural in another language)" ;
    skos:topConceptOf <http://vocab.getty.edu/term/POS/> .

<http://vocab.getty.edu/term/POS/VerbalNounGerund> a skos:Concept ;
    dct:description """Term is a verbal noun or gerund.
Example: polishing""" ;
    skos:example "polishing" ;
    skos:inScheme <http://vocab.getty.edu/term/POS/> ;
    skos:notation "VN" ;
    skos:prefLabel "Verbal Noun/Gerund"@en ;
    skos:scopeNote "Term is a verbal noun or gerund" ;
    skos:topConceptOf <http://vocab.getty.edu/term/POS/> .

<http://vocab.getty.edu/term/display/Display> a skos:Concept ;
    dct:description "Use in displays where natural order is appropriate" ;
    skos:inScheme <http://vocab.getty.edu/term/display/> ;
    skos:notation "D",
        "Y" ;
    skos:prefLabel "Use for Display"@en ;
    skos:scopeNote "Use in displays where natural order is appropriate" ;
    skos:topConceptOf <http://vocab.getty.edu/term/display/> .

<http://vocab.getty.edu/term/display/Indexing> a skos:Concept ;
    dct:description "Use in indexes or permuted lists where inverted order is appropriate" ;
    skos:inScheme <http://vocab.getty.edu/term/display/> ;
    skos:notation "I" ;
    skos:prefLabel "Use in Indexes/lists"@en ;
    skos:scopeNote "Use in indexes or permuted lists where inverted order is appropriate" ;
    skos:topConceptOf <http://vocab.getty.edu/term/display/> .

<http://vocab.getty.edu/term/flag/LiteralTranslation> a skos:Concept ;
    dct:description "Literal translation of a name.  Defined for ULAN, but currently there are no examples of this" ;
    skos:inScheme <http://vocab.getty.edu/term/flag/> ;
    skos:notation "T" ;
    skos:prefLabel "Literal Translation"@en ;
    skos:scopeNote "Literal translation of a name.  Defined for ULAN, but currently there are no examples of this" ;
    skos:topConceptOf <http://vocab.getty.edu/term/flag/> .

<http://vocab.getty.edu/term/flag/LoanTerm> a skos:Concept ;
    dct:description """Term borrowed from another language that has become naturalized in American English.
Example: papier mache""" ;
    skos:example "papier mache" ;
    skos:inScheme <http://vocab.getty.edu/term/flag/> ;
    skos:notation "L" ;
    skos:prefLabel "Loan Term"@en ;
    skos:scopeNote "Term borrowed from another language that has become naturalized in American English" ;
    skos:topConceptOf <http://vocab.getty.edu/term/flag/> .

<http://vocab.getty.edu/term/flag/Vernacular> a skos:Concept ;
    dct:description """Term is the vernacular for a certain place.
Example: "kachoga" is the Vernacular for 300266169 "bird-and-flower paintings" (AAT). "Firenze" is the vernacular in Italian (TGN)""" ;
    skos:example "\"kachoga\" is the Vernacular for 300266169 \"bird-and-flower paintings\" (AAT). \"Firenze\" is the vernacular in Italian (TGN)" ;
    skos:inScheme <http://vocab.getty.edu/term/flag/> ;
    skos:notation "V" ;
    skos:prefLabel "Vernacular"@en ;
    skos:scopeNote "Term is the vernacular for a certain place" ;
    skos:topConceptOf <http://vocab.getty.edu/term/flag/> .

<http://vocab.getty.edu/term/kind/Abbreviation> a skos:Concept ;
    dct:description """Term is an abbreviation, initialism, or acronym.
Example: "FLIM" is abbrevaition for "fluorescence lifetime imaging microscopy\"""" ;
    skos:example "\"FLIM\" is abbrevaition for \"fluorescence lifetime imaging microscopy\"" ;
    skos:inScheme <http://vocab.getty.edu/term/kind/> ;
    skos:notation "A" ;
    skos:prefLabel "Abbreviation"@en ;
    skos:scopeNote "Term is an abbreviation, initialism, or acronym" ;
    skos:topConceptOf <http://vocab.getty.edu/term/kind/> .

<http://vocab.getty.edu/term/kind/BirthName> a skos:Concept ;
    dct:description """Birth Name of an ULAN agent.
Example: TODO""" ;
    skos:example "TODO" ;
    skos:inScheme <http://vocab.getty.edu/term/kind/> ;
    skos:notation "BN" ;
    skos:prefLabel "Birth Name"@en ;
    skos:scopeNote "Birth Name of an ULAN agent" ;
    skos:topConceptOf <http://vocab.getty.edu/term/kind/> .

<http://vocab.getty.edu/term/kind/ChemicalName> a skos:Concept ;
    dct:description """Term is the chemical name for the descriptor. Used in AAT only.
Example: "sodium tetraborate decahydrate" is chemical name for "borax\"""" ;
    skos:example "\"sodium tetraborate decahydrate\" is chemical name for \"borax\"" ;
    skos:inScheme <http://vocab.getty.edu/term/kind/> ;
    skos:notation "CN" ;
    skos:prefLabel "Chemical Name"@en ;
    skos:scopeNote "Term is the chemical name for the descriptor. Used in AAT only" ;
    skos:topConceptOf <http://vocab.getty.edu/term/kind/> .

<http://vocab.getty.edu/term/kind/Code> a skos:Concept ;
    dct:description """Code, similar to Abbreviation.
Example: "sq yds", "m2\"""" ;
    skos:example "\"sq yds\", \"m2\"" ;
    skos:inScheme <http://vocab.getty.edu/term/kind/> ;
    skos:notation "79000" ;
    skos:prefLabel "Code"@en ;
    skos:scopeNote "Code, similar to Abbreviation" ;
    skos:topConceptOf <http://vocab.getty.edu/term/kind/> .

<http://vocab.getty.edu/term/kind/CommonName> a skos:Concept ;
    dct:description """Common Name of an ULAN agent.
Example: TODO""" ;
    skos:example "TODO" ;
    skos:inScheme <http://vocab.getty.edu/term/kind/> ;
    skos:notation "CN" ;
    skos:prefLabel "Common Name"@en ;
    skos:scopeNote "Common Name of an ULAN agent" ;
    skos:topConceptOf <http://vocab.getty.edu/term/kind/> .

<http://vocab.getty.edu/term/kind/CommonTerm> a skos:Concept ;
    dct:description """Preferred common language term. Used for subjects that also include a Scientific term. Used in AAT only.
Example: "frankincense" (species) is common term for "Boswellia sacra" (species)""" ;
    skos:example "\"frankincense\" (species) is common term for \"Boswellia sacra\" (species)" ;
    skos:inScheme <http://vocab.getty.edu/term/kind/> ;
    skos:notation "C" ;
    skos:prefLabel "Common term"@en ;
    skos:scopeNote "Preferred common language term. Used for subjects that also include a Scientific term. Used in AAT only" ;
    skos:topConceptOf <http://vocab.getty.edu/term/kind/> .

<http://vocab.getty.edu/term/kind/FIPSCode> a skos:Concept ;
    dct:description """FIPS region code. Used in TGN.
Example: "MX21" for Puebla, Mexico""" ;
    skos:example "\"MX21\" for Puebla, Mexico" ;
    skos:inScheme <http://vocab.getty.edu/term/kind/> ;
    skos:notation "FIPS" ;
    skos:prefLabel "FIPS Code"@en ;
    skos:scopeNote "FIPS region code. Used in TGN" ;
    skos:topConceptOf <http://vocab.getty.edu/term/kind/> .

<http://vocab.getty.edu/term/kind/FullName> a skos:Concept ;
    dct:description """Full Name of an ULAN agent.
Example: TODO""" ;
    skos:example "TODO" ;
    skos:inScheme <http://vocab.getty.edu/term/kind/> ;
    skos:notation "FN" ;
    skos:prefLabel "Full Name"@en ;
    skos:scopeNote "Full Name of an ULAN agent" ;
    skos:topConceptOf <http://vocab.getty.edu/term/kind/> .

<http://vocab.getty.edu/term/kind/FullTerm> a skos:Concept ;
    dct:description """Full-form term. Used when the descriptor is a shorter form, or the subject also includes an Abbreviation. Used in AAT only.
Example: "Extensible Markup Language" is the full term for "XML" (which is preferred)""" ;
    skos:example "\"Extensible Markup Language\" is the full term for \"XML\" (which is preferred)" ;
    skos:inScheme <http://vocab.getty.edu/term/kind/> ;
    skos:notation "F" ;
    skos:prefLabel "Full term"@en ;
    skos:scopeNote "Full-form term. Used when the descriptor is a shorter form, or the subject also includes an Abbreviation. Used in AAT only" ;
    skos:topConceptOf <http://vocab.getty.edu/term/kind/> .

<http://vocab.getty.edu/term/kind/ISOalpha2> a skos:Concept ;
    dct:description """ISO 3166-1 alpha-2 country code. Used in TGN.
Example: "AQ" for Antarctica""" ;
    skos:example "\"AQ\" for Antarctica" ;
    skos:inScheme <http://vocab.getty.edu/term/kind/> ;
    skos:notation "ISO2L" ;
    skos:prefLabel "ISO alpha-2 code"@en ;
    skos:scopeNote "ISO 3166-1 alpha-2 country code. Used in TGN" ;
    skos:topConceptOf <http://vocab.getty.edu/term/kind/> .

<http://vocab.getty.edu/term/kind/ISOalpha3> a skos:Concept ;
    dct:description """ISO 3166-1 alpha-3 country code. Used in TGN.
Example: "ATA" for Antarctica""" ;
    skos:example "\"ATA\" for Antarctica" ;
    skos:inScheme <http://vocab.getty.edu/term/kind/> ;
    skos:notation "ISO3L" ;
    skos:prefLabel "ISO alpha-3 code"@en ;
    skos:scopeNote "ISO 3166-1 alpha-3 country code. Used in TGN" ;
    skos:topConceptOf <http://vocab.getty.edu/term/kind/> .

<http://vocab.getty.edu/term/kind/ISOnumeric2> a skos:Concept ;
    dct:description "May be used in TGN, but no code of this kind is present" ;
    skos:inScheme <http://vocab.getty.edu/term/kind/> ;
    skos:notation "ISO2N" ;
    skos:prefLabel "ISO numeric-2 code"@en ;
    skos:scopeNote "May be used in TGN, but no code of this kind is present" ;
    skos:topConceptOf <http://vocab.getty.edu/term/kind/> .

<http://vocab.getty.edu/term/kind/ISOnumeric3> a skos:Concept ;
    dct:description """ISO 3166-1 numeric country code as "ISOnnn" (though ISO specifies only "nnn"). Used in TGN only.
Example: "ISO414" for Kuwait""" ;
    skos:example "\"ISO414\" for Kuwait" ;
    skos:inScheme <http://vocab.getty.edu/term/kind/> ;
    skos:notation "ISO3N" ;
    skos:prefLabel "ISO numeric-3 code"@en ;
    skos:scopeNote "ISO 3166-1 numeric country code as \"ISOnnn\" (though ISO specifies only \"nnn\"). Used in TGN only" ;
    skos:topConceptOf <http://vocab.getty.edu/term/kind/> .

<http://vocab.getty.edu/term/kind/JargonOrSlang> a skos:Concept ;
    dct:description """Slang or jargon term. Used in AAT only.
Example: "fool's gold" is slang for "pyrite\"""" ;
    skos:example "\"fool's gold\" is slang for \"pyrite\"" ;
    skos:inScheme <http://vocab.getty.edu/term/kind/> ;
    skos:notation "J" ;
    skos:prefLabel "Jargon or Slang"@en ;
    skos:scopeNote "Slang or jargon term. Used in AAT only" ;
    skos:topConceptOf <http://vocab.getty.edu/term/kind/> .

<http://vocab.getty.edu/term/kind/Neologism> a skos:Concept ;
    dct:description """Term that is new to the language, generally having been coined due to new technology. Used in AAT only..
Example: "folksonomy", "podcasting\"""" ;
    skos:example "\"folksonomy\", \"podcasting\"" ;
    skos:inScheme <http://vocab.getty.edu/term/kind/> ;
    skos:notation "N" ;
    skos:prefLabel "Neologism"@en ;
    skos:scopeNote "Term that is new to the language, generally having been coined due to new technology. Used in AAT only." ;
    skos:topConceptOf <http://vocab.getty.edu/term/kind/> .

<http://vocab.getty.edu/term/kind/OfficialName> a skos:Concept ;
    dct:description """Used in TGN and ULAN.
Example: "Noyen-sur-Seine" is official name of 7030197 "Noyen" (TGN)""" ;
    skos:example "\"Noyen-sur-Seine\" is official name of 7030197 \"Noyen\" (TGN)" ;
    skos:inScheme <http://vocab.getty.edu/term/kind/> ;
    skos:notation "O" ;
    skos:prefLabel "Official Name"@en ;
    skos:scopeNote "Used in TGN and ULAN" ;
    skos:topConceptOf <http://vocab.getty.edu/term/kind/> .

<http://vocab.getty.edu/term/kind/ProvisionalName> a skos:Concept ;
    dct:description """Used in TGN only.
Example: "Rockton" was provisional name considered before adoption of "Kent" (Ohio)""" ;
    skos:example "\"Rockton\" was provisional name considered before adoption of \"Kent\" (Ohio)" ;
    skos:inScheme <http://vocab.getty.edu/term/kind/> ;
    skos:notation "PN" ;
    skos:prefLabel "Provisional Name"@en ;
    skos:scopeNote "Used in TGN only" ;
    skos:topConceptOf <http://vocab.getty.edu/term/kind/> .

<http://vocab.getty.edu/term/kind/Pseudonym> a skos:Concept ;
    dct:description """Used in TGN and ULAN.
Example: "Frisco" is nickname for San Francisco (TGN)""" ;
    skos:example "\"Frisco\" is nickname for San Francisco (TGN)" ;
    skos:inScheme <http://vocab.getty.edu/term/kind/> ;
    skos:notation "P" ;
    skos:prefLabel "Pseudonym"@en ;
    skos:scopeNote "Used in TGN and ULAN" ;
    skos:topConceptOf <http://vocab.getty.edu/term/kind/> .

<http://vocab.getty.edu/term/kind/ScientificOrTechnical> a skos:Concept ;
    dct:description """Scientific taxon name (genus, species, etc). Used in AAT only. All such are emitted marked with English language, and most have the same string marked with Latin.
Example: "Boswellia sacra"@la, also emitted as "Boswellia sacra"@en, is scientific name of "frankincense\"""" ;
    skos:example "\"Boswellia sacra\"@la, also emitted as \"Boswellia sacra\"@en, is scientific name of \"frankincense\"" ;
    skos:inScheme <http://vocab.getty.edu/term/kind/> ;
    skos:notation "S" ;
    skos:prefLabel "Scientific or Technical term"@en ;
    skos:scopeNote "Scientific taxon name (genus, species, etc). Used in AAT only. All such are emitted marked with English language, and most have the same string marked with Latin" ;
    skos:topConceptOf <http://vocab.getty.edu/term/kind/> .

<http://vocab.getty.edu/term/kind/SiteName> a skos:Concept ;
    dct:description """Used in TGN only.
Example: "Flavia Solva", a deserted settlement and archaeological site (TGN)""" ;
    skos:example "\"Flavia Solva\", a deserted settlement and archaeological site (TGN)" ;
    skos:inScheme <http://vocab.getty.edu/term/kind/> ;
    skos:notation "S" ;
    skos:prefLabel "Site Name"@en ;
    skos:scopeNote "Used in TGN only" ;
    skos:topConceptOf <http://vocab.getty.edu/term/kind/> .

<http://vocab.getty.edu/term/kind/USPSCode> a skos:Concept ;
    dct:description """Used in TGN only.
Example: "CA" for California""" ;
    skos:example "\"CA\" for California" ;
    skos:inScheme <http://vocab.getty.edu/term/kind/> ;
    skos:notation "USPS" ;
    skos:prefLabel "US Postal Service Code"@en ;
    skos:scopeNote "Used in TGN only" ;
    skos:topConceptOf <http://vocab.getty.edu/term/kind/> .

<http://vocab.getty.edu/term/type/AlternateDescriptor> a skos:Concept ;
    dct:description """A lexical variant, eg singular.
Example: "manuscript" (English) instead of "manuscripts\"""" ;
    skos:example "\"manuscript\" (English) instead of \"manuscripts\"" ;
    skos:inScheme <http://vocab.getty.edu/term/type/> ;
    skos:notation "AD" ;
    skos:prefLabel "Alternate Descriptor"@en ;
    skos:scopeNote "A lexical variant, eg singular" ;
    skos:topConceptOf <http://vocab.getty.edu/term/type/> .

<http://vocab.getty.edu/term/type/Descriptor> a skos:Concept ;
    dct:description """Main term. Getty usually uses the plural.
Example: "manuscripts" (English)""" ;
    skos:example "\"manuscripts\" (English)" ;
    skos:inScheme <http://vocab.getty.edu/term/type/> ;
    skos:notation "D" ;
    skos:prefLabel "Descriptor"@en ;
    skos:scopeNote "Main term. Getty usually uses the plural" ;
    skos:topConceptOf <http://vocab.getty.edu/term/type/> .

<http://vocab.getty.edu/term/type/UsedForTerm> a skos:Concept ;
    dct:description """A synonym.
Example: "handschriften" (Dutch) instead of "manuscripten\"""" ;
    skos:example "\"handschriften\" (Dutch) instead of \"manuscripten\"" ;
    skos:inScheme <http://vocab.getty.edu/term/type/> ;
    skos:notation "UF" ;
    skos:prefLabel "Used for Term"@en ;
    skos:scopeNote "A synonym" ;
    skos:topConceptOf <http://vocab.getty.edu/term/type/> .

<http://www.wikidata.org/entity/Q6581072> skos:exactMatch <http://vocab.getty.edu/aat/300189557> .

<http://www.wikidata.org/entity/Q6581097> skos:exactMatch <http://vocab.getty.edu/aat/300189559> .

<http://vocab.getty.edu/aat/300189557> skos:exactMatch <http://rdaregistry.info/termList/gender/1001>,
        <http://www.wikidata.org/entity/Q6581072> .

<http://vocab.getty.edu/aat/300189559> skos:exactMatch <http://rdaregistry.info/termList/gender/1002>,
        <http://www.wikidata.org/entity/Q6581097> .

gvp:AdminPlaceConcept a owl:Class,
        skos:Concept ;
    rdfs:label "AdminPlaceConcept"@en ;
    dct:description """Place defined by administrative boundaries and conditions, including inhabited places, nations, and empires. Used in TGN only.
Example: Burgundy region in France (TGN)""" ;
    rdfs:comment "Place defined by administrative boundaries and conditions, including inhabited places, nations, and empires. Used in TGN only" ;
    rdfs:isDefinedBy <http://vocab.getty.edu/ontology> ;
    rdfs:subClassOf gvp:Subject,
        skos:Concept ;
    skos:broader gvp:Subject ;
    skos:example "Burgundy region in France (TGN)" ;
    skos:inScheme <http://vocab.getty.edu/ontology> ;
    skos:prefLabel "AdminPlaceConcept"@en ;
    skos:topConceptOf <http://vocab.getty.edu/ontology> .

gvp:Concept a owl:Class,
        skos:Concept ;
    rdfs:label "Concept"@en ;
    dct:description """Proper concept. Used in AAT only; TGN & ULAN have their own, e.g. gvp:PhysPlaceConcept & gvp:PersonConcept. Used for indexing and cataloguing.
Example: rhyta (AAT)""" ;
    rdfs:comment "Proper concept. Used in AAT only; TGN & ULAN have their own, e.g. gvp:PhysPlaceConcept & gvp:PersonConcept. Used for indexing and cataloguing" ;
    rdfs:isDefinedBy <http://vocab.getty.edu/ontology> ;
    rdfs:subClassOf gvp:Subject,
        skos:Concept ;
    skos:broader skos:Concept ;
    skos:example "rhyta (AAT)" ;
    skos:inScheme <http://vocab.getty.edu/ontology> ;
    skos:prefLabel "Concept"@en ;
    skos:topConceptOf <http://vocab.getty.edu/ontology> .

gvp:Facet a owl:Class,
        skos:Concept ;
    rdfs:label "Facet"@en ;
    dct:description """One of the major divisions of a vocabulary.
Example: Objects Facet (AAT), World (TGN), Artists (ULAN)""" ;
    rdfs:comment "One of the major divisions of a vocabulary" ;
    rdfs:isDefinedBy <http://vocab.getty.edu/ontology> ;
    rdfs:subClassOf iso:ThesaurusArray,
        gvp:Subject ;
    skos:broader gvp:Subject ;
    skos:example "Objects Facet (AAT), World (TGN), Artists (ULAN)" ;
    skos:inScheme <http://vocab.getty.edu/ontology> ;
    skos:prefLabel "Facet"@en ;
    skos:topConceptOf <http://vocab.getty.edu/ontology> .

gvp:GroupConcept a owl:Class,
        skos:Concept ;
    rdfs:label "GroupConcept"@en ;
    dct:description """Two or more people who generally worked together to collectively create art. Not necessarily legally incorporated. A family of artists may be considered a "corporate body". Corresponds to crm:E74_Group, not its subclass crm:E40_Legal_Body.
Example: 500356337 Albrecht Duerer Workshop (ULAN)""" ;
    rdfs:comment "Two or more people who generally worked together to collectively create art. Not necessarily legally incorporated. A family of artists may be considered a \"corporate body\". Corresponds to crm:E74_Group, not its subclass crm:E40_Legal_Body" ;
    rdfs:isDefinedBy <http://vocab.getty.edu/ontology> ;
    rdfs:subClassOf gvp:Subject,
        skos:Concept ;
    skos:broader skos:Concept ;
    skos:example "500356337 Albrecht Duerer Workshop (ULAN)" ;
    skos:inScheme <http://vocab.getty.edu/ontology> ;
    skos:prefLabel "GroupConcept"@en ;
    skos:topConceptOf <http://vocab.getty.edu/ontology> .

gvp:Hierarchy a owl:Class,
        skos:Concept ;
    rdfs:label "Hierarchy"@en ;
    dct:description """Top of a hierarchy. Used in AAT only. Not used for indexing or cataloguing.
Example: Containers (Hierarchy Name) (AAT)""" ;
    rdfs:comment "Top of a hierarchy. Used in AAT only. Not used for indexing or cataloguing" ;
    rdfs:isDefinedBy <http://vocab.getty.edu/ontology> ;
    rdfs:subClassOf iso:ThesaurusArray,
        gvp:Subject ;
    skos:broader iso:ThesaurusArray ;
    skos:example "Containers (Hierarchy Name) (AAT)" ;
    skos:inScheme <http://vocab.getty.edu/ontology> ;
    skos:prefLabel "Hierarchy"@en ;
    skos:topConceptOf <http://vocab.getty.edu/ontology> .

gvp:ObsoleteSubject a owl:Class,
        skos:Concept ;
    rdfs:label "ObsoleteSubject"@en ;
    dct:description """Obsolete subject: moved out of the publishable hierarchy, or merged to another (pointed by dct:isReplacedBy).
Example: 300375205 "shranks" (AAT) was merged to 300039264 "schranks" (AAT), so aat:300375205 dct:isReplacedBy aat:300039264""" ;
    rdfs:comment "Obsolete subject: moved out of the publishable hierarchy, or merged to another (pointed by dct:isReplacedBy)" ;
    rdfs:isDefinedBy <http://vocab.getty.edu/ontology> ;
    rdfs:subClassOf gvp:Subject ;
    skos:broader gvp:Subject ;
    skos:example "300375205 \"shranks\" (AAT) was merged to 300039264 \"schranks\" (AAT), so aat:300375205 dct:isReplacedBy aat:300039264" ;
    skos:inScheme <http://vocab.getty.edu/ontology> ;
    skos:prefLabel "ObsoleteSubject"@en ;
    skos:topConceptOf <http://vocab.getty.edu/ontology> .

gvp:PersonConcept a owl:Class,
        skos:Concept ;
    rdfs:label "PersonConcept"@en ;
    dct:description """A single individual. Usually people engaged in the design or creation of art or architecture ("Artists"); but may also include donors, patrons, rulers, sitters, art historians, etc ("Non-Artists").
Example: 500115493 Duerer, Albrecht (ULAN)""" ;
    rdfs:comment "A single individual. Usually people engaged in the design or creation of art or architecture (\"Artists\"); but may also include donors, patrons, rulers, sitters, art historians, etc (\"Non-Artists\")" ;
    rdfs:isDefinedBy <http://vocab.getty.edu/ontology> ;
    rdfs:subClassOf gvp:Subject,
        skos:Concept ;
    skos:broader skos:Concept ;
    skos:example "500115493 Duerer, Albrecht (ULAN)" ;
    skos:inScheme <http://vocab.getty.edu/ontology> ;
    skos:prefLabel "PersonConcept"@en ;
    skos:topConceptOf <http://vocab.getty.edu/ontology> .

gvp:PhysAdminPlaceConcept a owl:Class,
        skos:Concept ;
    rdfs:label "PhysAdminPlaceConcept"@en ;
    dct:description """Place that is both administrative and physical. Rarely used. Used in TGN only.
Example: 6003090 Kiik-Koba (TGN)""" ;
    rdfs:comment "Place that is both administrative and physical. Rarely used. Used in TGN only" ;
    rdfs:isDefinedBy <http://vocab.getty.edu/ontology> ;
    rdfs:subClassOf gvp:Subject,
        skos:Concept ;
    skos:broader gvp:Subject ;
    skos:example "6003090 Kiik-Koba (TGN)" ;
    skos:inScheme <http://vocab.getty.edu/ontology> ;
    skos:prefLabel "PhysAdminPlaceConcept"@en ;
    skos:topConceptOf <http://vocab.getty.edu/ontology> .

gvp:PhysPlaceConcept a owl:Class,
        skos:Concept ;
    rdfs:label "PhysPlaceConcept"@en ;
    dct:description """Physical feature, defined by its physical characteristics on planet Earth, including mountains, rivers, and oceans. Used in TGN only.
Example: Amazon River (TGN)""" ;
    rdfs:comment "Physical feature, defined by its physical characteristics on planet Earth, including mountains, rivers, and oceans. Used in TGN only" ;
    rdfs:isDefinedBy <http://vocab.getty.edu/ontology> ;
    rdfs:subClassOf gvp:Subject,
        skos:Concept ;
    skos:broader skos:Concept ;
    skos:example "Amazon River (TGN)" ;
    skos:inScheme <http://vocab.getty.edu/ontology> ;
    skos:prefLabel "PhysPlaceConcept"@en ;
    skos:topConceptOf <http://vocab.getty.edu/ontology> .

gvp:UnknownPersonConcept a owl:Class,
        skos:Concept ;
    rdfs:label "UnknownPersonConcept"@en ;
    dct:description """Unknown person representing a nationality/culture (the Unknown People by Culture facet).
Example: 500355202 Unknown Bulgarian (modern) (ULAN)""" ;
    rdfs:comment "Unknown person representing a nationality/culture (the Unknown People by Culture facet)" ;
    rdfs:isDefinedBy <http://vocab.getty.edu/ontology> ;
    rdfs:subClassOf gvp:Subject,
        skos:Concept ;
    skos:broader skos:Concept ;
    skos:example "500355202 Unknown Bulgarian (modern) (ULAN)" ;
    skos:inScheme <http://vocab.getty.edu/ontology> ;
    skos:prefLabel "UnknownPersonConcept"@en ;
    skos:topConceptOf <http://vocab.getty.edu/ontology> .

gvp:aat2001_formerly_referred_to a owl:ObjectProperty,
        owl:SymmetricProperty,
        skos:Concept ;
    dc:identifier "2001" ;
    dc:title "formerly referred to - any" ;
    dct:description """any - formerly referred - any.\r
Example: gigues formerly referred to fiddles""" ;
    rdfs:domain skos:Concept ;
    rdfs:isDefinedBy aat:,
        <http://vocab.getty.edu/ontology> ;
    rdfs:range skos:Concept ;
    rdfs:subPropertyOf skos:related ;
    skos:broader skos:related ;
    skos:example "gigues formerly referred to fiddles" ;
    skos:inScheme <http://vocab.getty.edu/ontology> ;
    skos:notation "2001" ;
    skos:prefLabel "aat2001_formerly_referred_to"@en ;
    skos:topConceptOf <http://vocab.getty.edu/ontology> .

gvp:aat2100_distinguished_from a owl:ObjectProperty,
        owl:SymmetricProperty,
        skos:Concept ;
    dc:identifier "2100" ;
    dc:title "distinguished from - any" ;
    dct:description """any - distinguished from - any.\r
Example: historic farms are distinguished from abandoned farms; naive art is distinguished from outsider art""" ;
    rdfs:domain skos:Concept ;
    rdfs:isDefinedBy aat:,
        <http://vocab.getty.edu/ontology> ;
    rdfs:range skos:Concept ;
    rdfs:subPropertyOf skos:related ;
    skos:broader skos:related ;
    skos:example "historic farms are distinguished from abandoned farms",
        "naive art is distinguished from outsider art" ;
    skos:inScheme <http://vocab.getty.edu/ontology> ;
    skos:notation "2100" ;
    skos:prefLabel "aat2100_distinguished_from"@en ;
    skos:topConceptOf <http://vocab.getty.edu/ontology> .

gvp:aat2205_causes-is_required a owl:ObjectProperty,
        skos:Concept ;
    dc:identifier "2205" ;
    dc:title "causes/is required - activity/event" ;
    dct:description """activity/event/[process/function] - causes/is required for - activity/event/[process/function].\r
Example: on-demand printing causes/is required for on-demand publishing;  preserving causes/is required for preservation""" ;
    rdfs:domain skos:Concept ;
    rdfs:isDefinedBy aat:,
        <http://vocab.getty.edu/ontology> ;
    rdfs:range skos:Concept ;
    rdfs:subPropertyOf skos:related ;
    owl:inverseOf gvp:aat2206_caused_by-requires ;
    skos:broader skos:related ;
    skos:example "on-demand printing causes/is required for on-demand publishing",
        "preserving causes/is required for preservation" ;
    skos:inScheme <http://vocab.getty.edu/ontology> ;
    skos:notation "2205" ;
    skos:prefLabel "aat2205_causes-is_required"@en ;
    skos:topConceptOf <http://vocab.getty.edu/ontology> .

gvp:aat2208_locus-setting_for a owl:ObjectProperty,
        skos:Concept ;
    dc:identifier "2208" ;
    dc:title "locus/setting for - things" ;
    dct:description """locus/setting - [is] locus/setting for - things.\r
Example: glassworks (buildings) are the locus/setting for glassware; caves are the locus/setting for cave paintings""" ;
    rdfs:domain skos:Concept ;
    rdfs:isDefinedBy aat:,
        <http://vocab.getty.edu/ontology> ;
    rdfs:range skos:Concept ;
    rdfs:subPropertyOf skos:related ;
    owl:inverseOf gvp:aat2209_used-located_in ;
    skos:broader skos:related ;
    skos:example "caves are the locus/setting for cave paintings",
        "glassworks (buildings) are the locus/setting for glassware" ;
    skos:inScheme <http://vocab.getty.edu/ontology> ;
    skos:notation "2208" ;
    skos:prefLabel "aat2208_locus-setting_for"@en ;
    skos:topConceptOf <http://vocab.getty.edu/ontology> .

gvp:aat2211_produce a owl:ObjectProperty,
        skos:Concept ;
    dc:identifier "2211" ;
    dc:title "produce - things" ;
    dct:description """things/[equipment] - produce - things.\r
Example: stereoscopic cameras produce stereoscopic photographs; punches (marking tools) produce punchwork""" ;
    rdfs:domain skos:Concept ;
    rdfs:isDefinedBy aat:,
        <http://vocab.getty.edu/ontology> ;
    rdfs:range skos:Concept ;
    rdfs:subPropertyOf skos:related ;
    owl:inverseOf gvp:aat2212_produced_by ;
    skos:broader skos:related ;
    skos:example "punches (marking tools) produce punchwork",
        "stereoscopic cameras produce stereoscopic photographs" ;
    skos:inScheme <http://vocab.getty.edu/ontology> ;
    skos:notation "2211" ;
    skos:prefLabel "aat2211_produce"@en ;
    skos:topConceptOf <http://vocab.getty.edu/ontology> .

gvp:aat2221_act_upon a owl:ObjectProperty,
        skos:Concept ;
    dc:identifier "2221" ;
    dc:title "act upon - genus/species" ;
    dct:description """[actors having] role - act upon - genus/species.\r
Example: jockeys act upon Equus caballus(species); tappers act upon Acer saccharum(species)""" ;
    rdfs:domain skos:Concept ;
    rdfs:isDefinedBy aat:,
        <http://vocab.getty.edu/ontology> ;
    rdfs:range skos:Concept ;
    rdfs:subPropertyOf skos:related ;
    owl:inverseOf gvp:aat2222_are_acted_upon ;
    skos:broader skos:related ;
    skos:example "jockeys act upon Equus caballus(species)",
        "tappers act upon Acer saccharum(species)" ;
    skos:inScheme <http://vocab.getty.edu/ontology> ;
    skos:notation "2221" ;
    skos:prefLabel "aat2221_act_upon"@en ;
    skos:topConceptOf <http://vocab.getty.edu/ontology> .

gvp:aat2281_have_counterpart a owl:ObjectProperty,
        owl:SymmetricProperty,
        skos:Concept ;
    dc:identifier "2281" ;
    dc:title "have counterpart - role" ;
    dct:description """role -[is] counterpart to - role.\r
Example: duchesses have counterpart dukes; godesses have counterpart gods""" ;
    rdfs:domain skos:Concept ;
    rdfs:isDefinedBy aat:,
        <http://vocab.getty.edu/ontology> ;
    rdfs:range skos:Concept ;
    rdfs:subPropertyOf skos:related ;
    skos:broader skos:related ;
    skos:example "duchesses have counterpart dukes",
        "godesses have counterpart gods" ;
    skos:inScheme <http://vocab.getty.edu/ontology> ;
    skos:notation "2281" ;
    skos:prefLabel "aat2281_have_counterpart"@en ;
    skos:topConceptOf <http://vocab.getty.edu/ontology> .

gvp:aat2285_practiced-studied_by a owl:ObjectProperty,
        skos:Concept ;
    dc:identifier "2285" ;
    dc:title "practiced/studied by - role" ;
    dct:description """field [of study, genre]/discipline - [is] practiced/studied by - a role.\r
Example: Egyptology is practiced/studied by Egyptologists; architectural history is practiced/studied by architectural historians""" ;
    rdfs:domain skos:Concept ;
    rdfs:isDefinedBy aat:,
        <http://vocab.getty.edu/ontology> ;
    rdfs:range skos:Concept ;
    rdfs:subPropertyOf skos:related ;
    owl:inverseOf gvp:aat2286_practice-study ;
    skos:broader skos:related ;
    skos:example "Egyptology is practiced/studied by Egyptologists",
        "architectural history is practiced/studied by architectural historians" ;
    skos:inScheme <http://vocab.getty.edu/ontology> ;
    skos:notation "2285" ;
    skos:prefLabel "aat2285_practiced-studied_by"@en ;
    skos:topConceptOf <http://vocab.getty.edu/ontology> .

gvp:aat2294_locus-setting_for a owl:ObjectProperty,
        skos:Concept ;
    dc:identifier "2294" ;
    dc:title "locus/setting for - locus/setting" ;
    dct:description """locus/setting - [is] locus setting for - locus/setting.\r
Example: nations are the locus/setting for national capitals; mountain ranges are the locus/setting for mountains""" ;
    rdfs:domain skos:Concept ;
    rdfs:isDefinedBy aat:,
        <http://vocab.getty.edu/ontology> ;
    rdfs:range skos:Concept ;
    rdfs:subPropertyOf skos:related ;
    owl:inverseOf gvp:aat2295_located_in ;
    skos:broader skos:related ;
    skos:example "mountain ranges are the locus/setting for mountains",
        "nations are the locus/setting for national capitals" ;
    skos:inScheme <http://vocab.getty.edu/ontology> ;
    skos:notation "2294" ;
    skos:prefLabel "aat2294_locus-setting_for"@en ;
    skos:topConceptOf <http://vocab.getty.edu/ontology> .

gvp:aat2311_performed_by a owl:ObjectProperty,
        skos:Concept ;
    dc:identifier "2311" ;
    dc:title "performed by - role" ;
    dct:description """activity/event/[process/function] - [is] performed by - [actors having] a role.\r
Example: clockmaking is performed by clockmakers; curating is performed by curators""" ;
    rdfs:domain skos:Concept ;
    rdfs:isDefinedBy aat:,
        <http://vocab.getty.edu/ontology> ;
    rdfs:range skos:Concept ;
    rdfs:subPropertyOf skos:related ;
    owl:inverseOf gvp:aat2312_perform ;
    skos:broader skos:related ;
    skos:example "clockmaking is performed by clockmakers",
        "curating is performed by curators" ;
    skos:inScheme <http://vocab.getty.edu/ontology> ;
    skos:notation "2311" ;
    skos:prefLabel "aat2311_performed_by"@en ;
    skos:topConceptOf <http://vocab.getty.edu/ontology> .

gvp:aat2318_involved_in a owl:ObjectProperty,
        skos:Concept ;
    dc:identifier "2318" ;
    dc:title "involved in - activity/event" ;
    dct:description """[actors having] role -[are] involved - activity/event.\r
Example: bridegrooms are involved in weddings; martyrs are involved in martyrdoms""" ;
    rdfs:domain skos:Concept ;
    rdfs:isDefinedBy aat:,
        <http://vocab.getty.edu/ontology> ;
    rdfs:range skos:Concept ;
    rdfs:subPropertyOf skos:related ;
    owl:inverseOf gvp:aat2319_involves ;
    skos:broader skos:related ;
    skos:example "bridegrooms are involved in weddings",
        "martyrs are involved in martyrdoms" ;
    skos:inScheme <http://vocab.getty.edu/ontology> ;
    skos:notation "2318" ;
    skos:prefLabel "aat2318_involved_in"@en ;
    skos:topConceptOf <http://vocab.getty.edu/ontology> .

gvp:aat2321_used_by a owl:ObjectProperty,
        skos:Concept ;
    dc:identifier "2321" ;
    dc:title "used by - role" ;
    dct:description """things/equipment - [are] used by - [actors having] role.\r
Example: violoncellos are used by violoncellists; surveying instruments are used by surveyors""" ;
    rdfs:domain skos:Concept ;
    rdfs:isDefinedBy aat:,
        <http://vocab.getty.edu/ontology> ;
    rdfs:range skos:Concept ;
    rdfs:subPropertyOf skos:related ;
    owl:inverseOf gvp:aat2322_use ;
    skos:broader skos:related ;
    skos:example "surveying instruments are used by surveyors",
        "violoncellos are used by violoncellists" ;
    skos:inScheme <http://vocab.getty.edu/ontology> ;
    skos:notation "2321" ;
    skos:prefLabel "aat2321_used_by"@en ;
    skos:topConceptOf <http://vocab.getty.edu/ontology> .

gvp:aat2332_affiliated_with a owl:ObjectProperty,
        skos:Concept ;
    dc:identifier "2332" ;
    dc:title "affiliated with - role" ;
    dct:description """[actors having] role - [are] affiliated with - role [organization].\r
Example: students are affiliated with schools (organizations); dukes are affiliated with duchies""" ;
    rdfs:domain skos:Concept ;
    rdfs:isDefinedBy aat:,
        <http://vocab.getty.edu/ontology> ;
    rdfs:range skos:Concept ;
    rdfs:subPropertyOf skos:related ;
    owl:inverseOf gvp:aat2333_have_affiliates ;
    skos:broader skos:related ;
    skos:example "dukes are affiliated with duchies",
        "students are affiliated with schools (organizations)" ;
    skos:inScheme <http://vocab.getty.edu/ontology> ;
    skos:notation "2332" ;
    skos:prefLabel "aat2332_affiliated_with"@en ;
    skos:topConceptOf <http://vocab.getty.edu/ontology> .

gvp:aat2335_associated_with a owl:ObjectProperty,
        skos:Concept ;
    dc:identifier "2335" ;
    dc:title "associated with - style/period/culture" ;
    dct:description """[actors having] role - [are] associated with - style/period/culture/[religion/ideology].\r
Example: abstract artists are associated with Abstract (fine arts style); popes are associated with Roman Catholicism""" ;
    rdfs:domain skos:Concept ;
    rdfs:isDefinedBy aat:,
        <http://vocab.getty.edu/ontology> ;
    rdfs:range skos:Concept ;
    rdfs:subPropertyOf skos:related ;
    owl:inverseOf gvp:aat2336_has_associates ;
    skos:broader skos:related ;
    skos:example "abstract artists are associated with Abstract (fine arts style)",
        "popes are associated with Roman Catholicism" ;
    skos:inScheme <http://vocab.getty.edu/ontology> ;
    skos:notation "2335" ;
    skos:prefLabel "aat2335_associated_with"@en ;
    skos:topConceptOf <http://vocab.getty.edu/ontology> .

gvp:aat2397_focus_of a owl:ObjectProperty,
        skos:Concept ;
    dc:identifier "2397" ;
    dc:title "focus of - field/discipline" ;
    dct:description """any - [is] focus of - field [of study]/discipline.\r
Example: manuscripts are the focus of codicology; music is the focus of musicology; Plantae (kingdom) is the focus of botany""" ;
    rdfs:domain skos:Concept ;
    rdfs:isDefinedBy aat:,
        <http://vocab.getty.edu/ontology> ;
    rdfs:range skos:Concept ;
    rdfs:subPropertyOf skos:related ;
    owl:inverseOf gvp:aat2398_focuses_on ;
    skos:broader skos:related ;
    skos:example "Plantae (kingdom) is the focus of botany",
        "manuscripts are the focus of codicology",
        "music is the focus of musicology" ;
    skos:inScheme <http://vocab.getty.edu/ontology> ;
    skos:notation "2397" ;
    skos:prefLabel "aat2397_focus_of"@en ;
    skos:topConceptOf <http://vocab.getty.edu/ontology> .

gvp:aat2415_required_for a owl:ObjectProperty,
        skos:Concept ;
    dc:identifier "2415" ;
    dc:title "required for - activity/event" ;
    dct:description """material - [is] required for - activity/event/[process/function].\r
Example: dye is required for dying; pewter is required for pewtersmithing""" ;
    rdfs:domain skos:Concept ;
    rdfs:isDefinedBy aat:,
        <http://vocab.getty.edu/ontology> ;
    rdfs:range skos:Concept ;
    rdfs:subPropertyOf skos:related ;
    owl:inverseOf gvp:aat2416_requires ;
    skos:broader skos:related ;
    skos:example "dye is required for dying",
        "pewter is required for pewtersmithing" ;
    skos:inScheme <http://vocab.getty.edu/ontology> ;
    skos:notation "2415" ;
    skos:prefLabel "aat2415_required_for"@en ;
    skos:topConceptOf <http://vocab.getty.edu/ontology> .

gvp:aat2427_produced_by a owl:ObjectProperty,
        skos:Concept ;
    dc:identifier "2427" ;
    dc:title "produced by - activity/event/process" ;
    dct:description """things - [are] produced by - activity/event/process.\r
Example: vase paintings (visual works) are produced by vase painting (image making); forgeries are produced by forging (copying)""" ;
    rdfs:domain skos:Concept ;
    rdfs:isDefinedBy aat:,
        <http://vocab.getty.edu/ontology> ;
    rdfs:range skos:Concept ;
    rdfs:subPropertyOf skos:related ;
    owl:inverseOf gvp:aat2428_produces ;
    skos:broader skos:related ;
    skos:example "forgeries are produced by forging (copying)",
        "vase paintings (visual works) are produced by vase painting (image making)" ;
    skos:inScheme <http://vocab.getty.edu/ontology> ;
    skos:notation "2427" ;
    skos:prefLabel "aat2427_produced_by"@en ;
    skos:topConceptOf <http://vocab.getty.edu/ontology> .

gvp:aat2434_contextualized_in a owl:ObjectProperty,
        skos:Concept ;
    dc:identifier "2434" ;
    dc:title "contextualized in - activity/event/process" ;
    dct:description """things - [are] context for - activity/event/process.\r
Example: funeral books are contextualized in funerals; Christmas trees are contextualized in Christmas""" ;
    rdfs:domain skos:Concept ;
    rdfs:isDefinedBy aat:,
        <http://vocab.getty.edu/ontology> ;
    rdfs:range skos:Concept ;
    rdfs:subPropertyOf skos:related ;
    owl:inverseOf gvp:aat2435_context_for ;
    skos:broader skos:related ;
    skos:example "Christmas trees are contextualized in Christmas",
        "funeral books are contextualized in funerals" ;
    skos:inScheme <http://vocab.getty.edu/ontology> ;
    skos:notation "2434" ;
    skos:prefLabel "aat2434_contextualized_in"@en ;
    skos:topConceptOf <http://vocab.getty.edu/ontology> .

gvp:aat2504_used-located_in a owl:ObjectProperty,
        skos:Concept ;
    dc:identifier "2504" ;
    dc:title "used/located in - locus/setting" ;
    dct:description """material - [is] used/located in - locus/setting.\r
Example: tephra is used/located in [at] volcanoes; brick (clay product) is used/located in brickworks (factories)""" ;
    rdfs:domain skos:Concept ;
    rdfs:isDefinedBy aat:,
        <http://vocab.getty.edu/ontology> ;
    rdfs:range skos:Concept ;
    rdfs:subPropertyOf skos:related ;
    owl:inverseOf gvp:aat2505_locus-setting_for ;
    skos:broader skos:related ;
    skos:example "brick (clay product) is used/located in brickworks (factories)",
        "tephra is used/located in [at] volcanoes" ;
    skos:inScheme <http://vocab.getty.edu/ontology> ;
    skos:notation "2504" ;
    skos:prefLabel "aat2504_used-located_in"@en ;
    skos:topConceptOf <http://vocab.getty.edu/ontology> .

gvp:aat2507_produce-process a owl:ObjectProperty,
        skos:Concept ;
    dc:identifier "2507" ;
    dc:title "produce/process - material" ;
    dct:description """things/[equipment] - produce/process - material.\r
Example: cotton (fiber) is produced/processed by cotton gins; groundwater is produced/processed by water wells""" ;
    rdfs:domain skos:Concept ;
    rdfs:isDefinedBy aat:,
        <http://vocab.getty.edu/ontology> ;
    rdfs:range skos:Concept ;
    rdfs:subPropertyOf skos:related ;
    owl:inverseOf gvp:aat2508_produced-processed_by ;
    skos:broader skos:related ;
    skos:example "cotton (fiber) is produced/processed by cotton gins",
        "groundwater is produced/processed by water wells" ;
    skos:inScheme <http://vocab.getty.edu/ontology> ;
    skos:notation "2507" ;
    skos:prefLabel "aat2507_produce-process"@en ;
    skos:topConceptOf <http://vocab.getty.edu/ontology> .

gvp:aat2562_locus-setting_for a owl:ObjectProperty,
        skos:Concept ;
    dc:identifier "2562" ;
    dc:title "locus/setting for - style/period/culture" ;
    dct:description """locus/setting - [is] locus/setting for - style/period/culture/[religion/ideology].\r
Example: First Nations reserves are the locus/setting for First Nations (culture); agraharas are the locus/setting for Brahmanism""" ;
    rdfs:domain skos:Concept ;
    rdfs:isDefinedBy aat:,
        <http://vocab.getty.edu/ontology> ;
    rdfs:range skos:Concept ;
    rdfs:subPropertyOf skos:related ;
    owl:inverseOf gvp:aat2563_located_in ;
    skos:broader skos:related ;
    skos:example "First Nations reserves are the locus/setting for First Nations (culture)",
        "agraharas are the locus/setting for Brahmanism" ;
    skos:inScheme <http://vocab.getty.edu/ontology> ;
    skos:notation "2562" ;
    skos:prefLabel "aat2562_locus-setting_for"@en ;
    skos:topConceptOf <http://vocab.getty.edu/ontology> .

gvp:aat2601_possessed_by-existing_in a owl:ObjectProperty,
        skos:Concept ;
    dc:identifier "2601" ;
    dc:title "possessed by/existing in - role" ;
    dct:description """attributes /associated concepts - [is] possessed by/existing in - role [of actors].\r
Example: adulthood is possessed by/existing in adults; nomadism is possessed by/existing in nomads""" ;
    rdfs:domain skos:Concept ;
    rdfs:isDefinedBy aat:,
        <http://vocab.getty.edu/ontology> ;
    rdfs:range skos:Concept ;
    rdfs:subPropertyOf skos:related ;
    owl:inverseOf gvp:aat2602_possess-exist_in ;
    skos:broader skos:related ;
    skos:example "adulthood is possessed by/existing in adults",
        "nomadism is possessed by/existing in nomads" ;
    skos:inScheme <http://vocab.getty.edu/ontology> ;
    skos:notation "2601" ;
    skos:prefLabel "aat2601_possessed_by-existing_in"@en ;
    skos:topConceptOf <http://vocab.getty.edu/ontology> .

gvp:aat2607_caused_by-requires a owl:ObjectProperty,
        skos:Concept ;
    dc:identifier "2607" ;
    dc:title "caused by/requires - activity/event" ;
    dct:description """attributes /associated concepts - [is] caused by/requires - an activity/event/[process/function].\r
Example: watertightness is caused by/requires waterproofing; creases (condition) is caused by/requires creasing (process)""" ;
    rdfs:domain skos:Concept ;
    rdfs:isDefinedBy aat:,
        <http://vocab.getty.edu/ontology> ;
    rdfs:range skos:Concept ;
    rdfs:subPropertyOf skos:related ;
    owl:inverseOf gvp:aat2608_causes-required_for ;
    skos:broader skos:related ;
    skos:example "creases (condition) is caused by/requires creasing (process)",
        "watertightness is caused by/requires waterproofing" ;
    skos:inScheme <http://vocab.getty.edu/ontology> ;
    skos:notation "2607" ;
    skos:prefLabel "aat2607_caused_by-requires"@en ;
    skos:topConceptOf <http://vocab.getty.edu/ontology> .

gvp:aat2801_conjuncted_with a owl:ObjectProperty,
        owl:SymmetricProperty,
        skos:Concept ;
    dc:identifier "2801" ;
    dc:title "conjuncted with - things" ;
    dct:description """things - [are] conjuncted with - things.\r
Example: cups are conjuncted with saucers; dining tables are conjuncted with dining chairs""" ;
    rdfs:domain skos:Concept ;
    rdfs:isDefinedBy aat:,
        <http://vocab.getty.edu/ontology> ;
    rdfs:range skos:Concept ;
    rdfs:subPropertyOf skos:related ;
    skos:broader skos:related ;
    skos:example "cups are conjuncted with saucers",
        "dining tables are conjuncted with dining chairs" ;
    skos:inScheme <http://vocab.getty.edu/ontology> ;
    skos:notation "2801" ;
    skos:prefLabel "aat2801_conjuncted_with"@en ;
    skos:topConceptOf <http://vocab.getty.edu/ontology> .

gvp:aat2807_derived_from_common_source a owl:ObjectProperty,
        owl:SymmetricProperty,
        skos:Concept ;
    dc:identifier "2807" ;
    dc:title "derived from common source - material" ;
    dct:description """material - [is] derived from common source [as] - material.\r
Example: malachite (mineral) is derived from common source with azurite (mineral); mustard(material) is derived from common source with mustard oil""" ;
    rdfs:domain skos:Concept ;
    rdfs:isDefinedBy aat:,
        <http://vocab.getty.edu/ontology> ;
    rdfs:range skos:Concept ;
    rdfs:subPropertyOf skos:related ;
    skos:broader skos:related ;
    skos:example "malachite (mineral) is derived from common source with azurite (mineral)",
        "mustard(material) is derived from common source with mustard oil" ;
    skos:inScheme <http://vocab.getty.edu/ontology> ;
    skos:notation "2807" ;
    skos:prefLabel "aat2807_derived_from_common_source"@en ;
    skos:topConceptOf <http://vocab.getty.edu/ontology> .

gvp:aat2809_coexisted_with a owl:ObjectProperty,
        owl:SymmetricProperty,
        skos:Concept ;
    dc:identifier "2809" ;
    dc:title "coexisted with - style/period/culture" ;
    dct:description """style/period/culture/[religion/ideology] - coexisted with -  style/period/culture/[religion/ideology].\r
Example: Sangoan coexisted with Fauresmith; Early Minoan coexisted with Prepalatial""" ;
    rdfs:domain skos:Concept ;
    rdfs:isDefinedBy aat:,
        <http://vocab.getty.edu/ontology> ;
    rdfs:range skos:Concept ;
    rdfs:subPropertyOf skos:related ;
    skos:broader skos:related ;
    skos:example "Early Minoan coexisted with Prepalatial",
        "Sangoan coexisted with Fauresmith" ;
    skos:inScheme <http://vocab.getty.edu/ontology> ;
    skos:notation "2809" ;
    skos:prefLabel "aat2809_coexisted_with"@en ;
    skos:topConceptOf <http://vocab.getty.edu/ontology> .

gvp:aat2811_preceded a owl:ObjectProperty,
        skos:Concept ;
    dc:identifier "2811" ;
    dc:title "preceded - style/period/culture" ;
    dct:description """style/period/culture/[religion/ideology] - preceded  - style/period/culture/[religion/ideology].\r
Example: Impressionist preceded Abstract Impressionist; Acheulian preceded Micoquian""" ;
    rdfs:domain skos:Concept ;
    rdfs:isDefinedBy aat:,
        <http://vocab.getty.edu/ontology> ;
    rdfs:range skos:Concept ;
    rdfs:subPropertyOf skos:related ;
    owl:inverseOf gvp:aat2812_followed ;
    skos:broader skos:related ;
    skos:example "Acheulian preceded Micoquian",
        "Impressionist preceded Abstract Impressionist" ;
    skos:inScheme <http://vocab.getty.edu/ontology> ;
    skos:notation "2811" ;
    skos:prefLabel "aat2811_preceded"@en ;
    skos:topConceptOf <http://vocab.getty.edu/ontology> .

gvp:aat2824_has_parallels_with a owl:ObjectProperty,
        owl:SymmetricProperty,
        skos:Concept ;
    dc:identifier "2824" ;
    dc:title "has parallels with - style/period/culture" ;
    dct:description """style/period/culture/[religion/ideology] - has parallels with - style/period/culture/[religion/ideology].\r
Example: Lagozza [culture] has parallels with Chasseen [culture];  Gnathian (pottery style) has parallels with West Slope (pottery style)""" ;
    rdfs:domain skos:Concept ;
    rdfs:isDefinedBy aat:,
        <http://vocab.getty.edu/ontology> ;
    rdfs:range skos:Concept ;
    rdfs:subPropertyOf skos:related ;
    skos:broader skos:related ;
    skos:example "Gnathian (pottery style) has parallels with West Slope (pottery style)",
        "Lagozza [culture] has parallels with Chasseen [culture]" ;
    skos:inScheme <http://vocab.getty.edu/ontology> ;
    skos:notation "2824" ;
    skos:prefLabel "aat2824_has_parallels_with"@en ;
    skos:topConceptOf <http://vocab.getty.edu/ontology> .

gvp:aat2831_associated_with a owl:ObjectProperty,
        owl:SymmetricProperty,
        skos:Concept ;
    dc:identifier "2831" ;
    dc:title "associated with - genus/species" ;
    dct:description """genus/species/[other living organism term] - [is] associated with - genus/species.\r
Example: Anthonomus grandis (species) [boll weevil] is associated with Gossypium (genus) [cotton]; Amphiprioninae (subfamily) [clown fish] is associated with Actiniaria (order) [sea anemone]""" ;
    rdfs:domain skos:Concept ;
    rdfs:isDefinedBy aat:,
        <http://vocab.getty.edu/ontology> ;
    rdfs:range skos:Concept ;
    rdfs:subPropertyOf skos:related ;
    skos:broader skos:related ;
    skos:example "Amphiprioninae (subfamily) [clown fish] is associated with Actiniaria (order) [sea anemone]",
        "Anthonomus grandis (species) [boll weevil] is associated with Gossypium (genus) [cotton]" ;
    skos:inScheme <http://vocab.getty.edu/ontology> ;
    skos:notation "2831" ;
    skos:prefLabel "aat2831_associated_with"@en ;
    skos:topConceptOf <http://vocab.getty.edu/ontology> .

gvp:aat2836_derived-made_from a owl:ObjectProperty,
        skos:Concept ;
    dc:identifier "2836" ;
    dc:title "derived/made from - genus/species" ;
    dct:description """things - [are] derived/made from - genus/species [or its parts].\r
Example: k?kaku are derived/made from Phormium tenax (species); ostrich-egg cups are derived/made from Struthio camelus (species)""" ;
    rdfs:domain skos:Concept ;
    rdfs:isDefinedBy aat:,
        <http://vocab.getty.edu/ontology> ;
    rdfs:range skos:Concept ;
    rdfs:subPropertyOf skos:related ;
    owl:inverseOf gvp:aat2837_source_for ;
    skos:broader skos:related ;
    skos:example "k?kaku are derived/made from Phormium tenax (species)",
        "ostrich-egg cups are derived/made from Struthio camelus (species)" ;
    skos:inScheme <http://vocab.getty.edu/ontology> ;
    skos:notation "2836" ;
    skos:prefLabel "aat2836_derived-made_from"@en ;
    skos:topConceptOf <http://vocab.getty.edu/ontology> .

gvp:aat2841_derived-made_from a owl:ObjectProperty,
        skos:Concept ;
    dc:identifier "2841" ;
    dc:title "derived/made from - genus/species" ;
    dct:description """material - [is] derived/made from - genus/species.\r
Example: alpaca (wool) is derived from Vicugna pacos (species); maple (wood) is derived from Acer (genus)""" ;
    rdfs:domain skos:Concept ;
    rdfs:isDefinedBy aat:,
        <http://vocab.getty.edu/ontology> ;
    rdfs:range skos:Concept ;
    rdfs:subPropertyOf skos:related ;
    owl:inverseOf gvp:aat2842_source_for ;
    skos:broader skos:related ;
    skos:example "alpaca (wool) is derived from Vicugna pacos (species)",
        "maple (wood) is derived from Acer (genus)" ;
    skos:inScheme <http://vocab.getty.edu/ontology> ;
    skos:notation "2841" ;
    skos:prefLabel "aat2841_derived-made_from"@en ;
    skos:topConceptOf <http://vocab.getty.edu/ontology> .

gvp:aat2845_used-located_in a owl:ObjectProperty,
        skos:Concept ;
    dc:identifier "2845" ;
    dc:title "used/located in - locus/setting" ;
    dct:description """genus/species - [is] used/located in -  locus/setting.\r
Example: Elephantidae(family) are used/located in elephant houses; Vitaceae (family) is used/located in vineyards""" ;
    rdfs:domain skos:Concept ;
    rdfs:isDefinedBy aat:,
        <http://vocab.getty.edu/ontology> ;
    rdfs:range skos:Concept ;
    rdfs:subPropertyOf skos:related ;
    owl:inverseOf gvp:aat2846_locus-setting_for ;
    skos:broader skos:related ;
    skos:example "Elephantidae(family) are used/located in elephant houses",
        "Vitaceae (family) is used/located in vineyards" ;
    skos:inScheme <http://vocab.getty.edu/ontology> ;
    skos:notation "2845" ;
    skos:prefLabel "aat2845_used-located_in"@en ;
    skos:topConceptOf <http://vocab.getty.edu/ontology> .

gvp:aat2848_involved_in a owl:ObjectProperty,
        skos:Concept ;
    dc:identifier "2848" ;
    dc:title "involved in - activity/event" ;
    dct:description """genus/species - is involved in - activity/event.\r
Example: bulls (animals) are involved in bullfighting; Equus caballus (species) is involved in polo(field sport)""" ;
    rdfs:domain skos:Concept ;
    rdfs:isDefinedBy aat:,
        <http://vocab.getty.edu/ontology> ;
    rdfs:range skos:Concept ;
    rdfs:subPropertyOf skos:related ;
    owl:inverseOf gvp:aat2849_involves ;
    skos:broader skos:related ;
    skos:example "Equus caballus (species) is involved in polo(field sport)",
        "bulls (animals) are involved in bullfighting" ;
    skos:inScheme <http://vocab.getty.edu/ontology> ;
    skos:notation "2848" ;
    skos:prefLabel "aat2848_involved_in"@en ;
    skos:topConceptOf <http://vocab.getty.edu/ontology> .

gvp:aat2852_involved_with a owl:ObjectProperty,
        skos:Concept ;
    dc:identifier "2852" ;
    dc:title "involved with - things" ;
    dct:description """genus/species - [is] involved with - things/[equipment].\r
Example: Rosa (genus) is involved with rose bowls; Camelus (genus) is involved with camel saddles""" ;
    rdfs:domain skos:Concept ;
    rdfs:isDefinedBy aat:,
        <http://vocab.getty.edu/ontology> ;
    rdfs:range skos:Concept ;
    rdfs:subPropertyOf skos:related ;
    owl:inverseOf gvp:aat2853_involve ;
    skos:broader skos:related ;
    skos:example "Camelus (genus) is involved with camel saddles",
        "Rosa (genus) is involved with rose bowls" ;
    skos:inScheme <http://vocab.getty.edu/ontology> ;
    skos:notation "2852" ;
    skos:prefLabel "aat2852_involved_with"@en ;
    skos:topConceptOf <http://vocab.getty.edu/ontology> .

gvp:aat2886_used-function_as a owl:ObjectProperty,
        skos:Concept ;
    dc:identifier "2886" ;
    dc:title "used/function as - material" ;
    dct:description """material - used/function as - material.\r
Example: carbon disulfide - is used/functions as - solvent""" ;
    rdfs:domain skos:Concept ;
    rdfs:isDefinedBy aat:,
        <http://vocab.getty.edu/ontology> ;
    rdfs:range skos:Concept ;
    rdfs:subPropertyOf skos:related ;
    owl:inverseOf gvp:aat2887_exemplified_by ;
    skos:broader skos:related ;
    skos:example "carbon disulfide - is used/functions as - solvent" ;
    skos:inScheme <http://vocab.getty.edu/ontology> ;
    skos:notation "2886" ;
    skos:prefLabel "aat2886_used-function_as"@en ;
    skos:topConceptOf <http://vocab.getty.edu/ontology> .

gvp:aat2900_miscellaneous_relationship a owl:ObjectProperty,
        owl:SymmetricProperty,
        skos:Concept ;
    dc:identifier "2900" ;
    dc:title "miscellaneous relationship - any" ;
    dct:description """any - [has] miscellaneous relationship [to] - any.\r
Example: Conditions and Effects has miscellaneous relationship with Processes and Techniques""" ;
    rdfs:domain skos:Concept ;
    rdfs:isDefinedBy aat:,
        <http://vocab.getty.edu/ontology> ;
    rdfs:range skos:Concept ;
    rdfs:subPropertyOf skos:related ;
    skos:broader skos:related ;
    skos:example "Conditions and Effects has miscellaneous relationship with Processes and Techniques" ;
    skos:inScheme <http://vocab.getty.edu/ontology> ;
    skos:notation "2900" ;
    skos:prefLabel "aat2900_miscellaneous_relationship"@en ;
    skos:topConceptOf <http://vocab.getty.edu/ontology> .

gvp:agentTypeNonPreferred a owl:ObjectProperty,
        skos:Concept ;
    rdfs:label "agentTypeNonPreferred"@en ;
    dct:description """A secondary type of a ULAN Person or Corporate body. Domain is ULAN concept, range is AAT concept.
Example: Non-preferred types of "Albrecht Duerer Workshop" (ULAN) include "printmakers" and painters" (AAT)""" ;
    rdfs:comment "A secondary type of a ULAN Person or Corporate body. Domain is ULAN concept, range is AAT concept" ;
    rdfs:domain gvp:Subject ;
    rdfs:isDefinedBy <http://vocab.getty.edu/ontology> ;
    rdfs:range gvp:Subject ;
    rdfs:subPropertyOf gvp:agentType ;
    skos:broader gvp:agentType ;
    skos:example "Non-preferred types of \"Albrecht Duerer Workshop\" (ULAN) include \"printmakers\" and painters\" (AAT)" ;
    skos:inScheme <http://vocab.getty.edu/ontology> ;
    skos:prefLabel "agentTypeNonPreferred"@en ;
    skos:topConceptOf <http://vocab.getty.edu/ontology> .

gvp:agentTypePreferred a owl:ObjectProperty,
        skos:Concept ;
    rdfs:label "agentTypePreferred"@en ;
    dct:description """The primary type of a ULAN Person or Corporate body. Domain is ULAN concept, range is AAT concept.
Example: The preferred type of "Albrecht Duerer Workshop" (ULAN) is "workshop" (AAT)""" ;
    rdfs:comment "The primary type of a ULAN Person or Corporate body. Domain is ULAN concept, range is AAT concept" ;
    rdfs:domain gvp:Subject ;
    rdfs:isDefinedBy <http://vocab.getty.edu/ontology> ;
    rdfs:range gvp:Subject ;
    rdfs:subPropertyOf gvp:agentType ;
    skos:broader gvp:agentType ;
    skos:example "The preferred type of \"Albrecht Duerer Workshop\" (ULAN) is \"workshop\" (AAT)" ;
    skos:inScheme <http://vocab.getty.edu/ontology> ;
    skos:prefLabel "agentTypePreferred"@en ;
    skos:topConceptOf <http://vocab.getty.edu/ontology> .

gvp:biographyNonPreferred a owl:ObjectProperty,
        skos:Concept ;
    rdfs:label "biographyNonPreferred"@en ;
    dct:description "Non-preferred biography of an ULAN agent. Domain is schema:Person/Organization, range is gvp:Biography" ;
    rdfs:comment "Non-preferred biography of an ULAN agent. Domain is schema:Person/Organization, range is gvp:Biography" ;
    rdfs:isDefinedBy <http://vocab.getty.edu/ontology> ;
    rdfs:range gvp:Biography ;
    rdfs:subPropertyOf gvp:biography ;
    skos:broader gvp:biography ;
    skos:inScheme <http://vocab.getty.edu/ontology> ;
    skos:prefLabel "biographyNonPreferred"@en ;
    skos:topConceptOf <http://vocab.getty.edu/ontology> .

gvp:biographyPreferred a owl:ObjectProperty,
        skos:Concept ;
    rdfs:label "biographyPreferred"@en ;
    dct:description "Preferred biography of an ULAN agent. Domain is schema:Person/Organization, range is gvp:Biography. The biography fields are also directly available in the Person/Organization" ;
    rdfs:comment "Preferred biography of an ULAN agent. Domain is schema:Person/Organization, range is gvp:Biography. The biography fields are also directly available in the Person/Organization" ;
    rdfs:isDefinedBy <http://vocab.getty.edu/ontology> ;
    rdfs:range gvp:Biography ;
    rdfs:subPropertyOf gvp:biography ;
    skos:broader gvp:biography ;
    skos:inScheme <http://vocab.getty.edu/ontology> ;
    skos:prefLabel "biographyPreferred"@en ;
    skos:topConceptOf <http://vocab.getty.edu/ontology> .

gvp:broaderInstantial a owl:ObjectProperty,
        skos:Concept ;
    rdfs:label "broaderInstantial"@en ;
    dct:description """BTI (Kind/Instance, "example of") relation. We also infer iso-thes:broaderInstantial, which goes only between Concepts.
Example: Rembrandt van Rijn BTI Persons/Artists (ULAN)""" ;
    rdfs:comment "BTI (Kind/Instance, \"example of\") relation. We also infer iso-thes:broaderInstantial, which goes only between Concepts" ;
    rdfs:domain gvp:Subject ;
    rdfs:isDefinedBy <http://vocab.getty.edu/ontology> ;
    rdfs:range gvp:Subject ;
    rdfs:subPropertyOf gvp:broader,
        gvp:broaderInstantialExtended ;
    skos:broader gvp:broaderInstantialExtended ;
    skos:example "Rembrandt van Rijn BTI Persons/Artists (ULAN)" ;
    skos:inScheme <http://vocab.getty.edu/ontology> ;
    skos:prefLabel "broaderInstantial"@en ;
    skos:topConceptOf <http://vocab.getty.edu/ontology> .

gvp:broaderNonPreferred a owl:ObjectProperty,
        skos:Concept ;
    rdfs:label "broaderNonPreferred"@en ;
    dct:description """Auxiliary parents of a subject. Very often there are several non-preferred parents (poly-hierarchy). Can use to mark such parents with [N] in displays .
Example: Non-preferred: "baking dishes" BTG "dishes (vessels)" (AAT)""" ;
    rdfs:comment "Auxiliary parents of a subject. Very often there are several non-preferred parents (poly-hierarchy). Can use to mark such parents with [N] in displays " ;
    rdfs:domain gvp:Subject ;
    rdfs:isDefinedBy <http://vocab.getty.edu/ontology> ;
    rdfs:range gvp:Subject ;
    rdfs:subPropertyOf gvp:broader ;
    skos:broader gvp:broader ;
    skos:example "Non-preferred: \"baking dishes\" BTG \"dishes (vessels)\" (AAT)" ;
    skos:inScheme <http://vocab.getty.edu/ontology> ;
    skos:prefLabel "broaderNonPreferred"@en ;
    skos:topConceptOf <http://vocab.getty.edu/ontology> .

gvp:contributorAlternatePreferred a owl:ObjectProperty,
        skos:Concept ;
    rdfs:label "contributorAlternatePreferred"@en ;
    dct:description "Contributor for which the term is Alternate Preferred. Range is foaf:Agent" ;
    rdfs:comment "Contributor for which the term is Alternate Preferred. Range is foaf:Agent" ;
    rdfs:domain skosxl:Label ;
    rdfs:isDefinedBy <http://vocab.getty.edu/ontology> ;
    rdfs:range foaf:Agent ;
    rdfs:subPropertyOf dct:contributor ;
    skos:broader dct:contributor ;
    skos:inScheme <http://vocab.getty.edu/ontology> ;
    skos:prefLabel "contributorAlternatePreferred"@en ;
    skos:topConceptOf <http://vocab.getty.edu/ontology> .

gvp:contributorNonPreferred a owl:ObjectProperty,
        skos:Concept ;
    rdfs:label "contributorNonPreferred"@en ;
    dct:description """Contributor for which the term is Non-preferred. Range is foaf:Agent.
Example: "Lycra" is non-preferred term for WHS""" ;
    rdfs:comment "Contributor for which the term is Non-preferred. Range is foaf:Agent" ;
    rdfs:domain skosxl:Label ;
    rdfs:isDefinedBy <http://vocab.getty.edu/ontology> ;
    rdfs:range foaf:Agent ;
    rdfs:subPropertyOf dct:contributor ;
    skos:broader dct:contributor ;
    skos:example "\"Lycra\" is non-preferred term for WHS" ;
    skos:inScheme <http://vocab.getty.edu/ontology> ;
    skos:prefLabel "contributorNonPreferred"@en ;
    skos:topConceptOf <http://vocab.getty.edu/ontology> .

gvp:contributorPreferred a owl:ObjectProperty,
        skos:Concept ;
    rdfs:label "contributorPreferred"@en ;
    dct:description """Contributor for which the term is Preferred. Range is foaf:Agent.
Example: "organza" is preferred term for WHS""" ;
    rdfs:comment "Contributor for which the term is Preferred. Range is foaf:Agent" ;
    rdfs:domain skosxl:Label ;
    rdfs:isDefinedBy <http://vocab.getty.edu/ontology> ;
    rdfs:range foaf:Agent ;
    rdfs:subPropertyOf dct:contributor ;
    skos:broader dct:contributor ;
    skos:example "\"organza\" is preferred term for WHS" ;
    skos:inScheme <http://vocab.getty.edu/ontology> ;
    skos:prefLabel "contributorPreferred"@en ;
    skos:topConceptOf <http://vocab.getty.edu/ontology> .

gvp:eventNonPreferred a owl:ObjectProperty,
        skos:Concept ;
    rdfs:label "eventNonPreferred"@en ;
    dct:description "Non-preferred life event of an ULAN agent. Domain is schema:Person/Organization, range is bio:Event" ;
    rdfs:comment "Non-preferred life event of an ULAN agent. Domain is schema:Person/Organization, range is bio:Event" ;
    rdfs:isDefinedBy <http://vocab.getty.edu/ontology> ;
    rdfs:range bio:Event ;
    rdfs:subPropertyOf bio:event ;
    skos:broader bio:event ;
    skos:inScheme <http://vocab.getty.edu/ontology> ;
    skos:prefLabel "eventNonPreferred"@en ;
    skos:topConceptOf <http://vocab.getty.edu/ontology> .

gvp:eventPreferred a owl:ObjectProperty,
        skos:Concept ;
    rdfs:label "eventPreferred"@en ;
    dct:description "Preferred life event of an ULAN agent. Domain is schema:Person/Organization, range is bio:Event" ;
    rdfs:comment "Preferred life event of an ULAN agent. Domain is schema:Person/Organization, range is bio:Event" ;
    rdfs:isDefinedBy <http://vocab.getty.edu/ontology> ;
    rdfs:range bio:Event ;
    rdfs:subPropertyOf bio:event ;
    skos:broader bio:event ;
    skos:inScheme <http://vocab.getty.edu/ontology> ;
    skos:prefLabel "eventPreferred"@en ;
    skos:topConceptOf <http://vocab.getty.edu/ontology> .

gvp:nationalityNonPreferred a owl:ObjectProperty,
        skos:Concept ;
    rdfs:label "nationalityNonPreferred"@en ;
    dct:description "Non-preferred nationality/culture/race/ethnicity/religion/sexual orientation of an ULAN agent. Domain is schema:Person/Organization, range is AAT concept" ;
    rdfs:comment "Non-preferred nationality/culture/race/ethnicity/religion/sexual orientation of an ULAN agent. Domain is schema:Person/Organization, range is AAT concept" ;
    rdfs:isDefinedBy <http://vocab.getty.edu/ontology> ;
    rdfs:range gvp:Subject ;
    rdfs:subPropertyOf schema:nationality ;
    skos:broader schema:nationality ;
    skos:inScheme <http://vocab.getty.edu/ontology> ;
    skos:prefLabel "nationalityNonPreferred"@en ;
    skos:topConceptOf <http://vocab.getty.edu/ontology> .

gvp:nationalityPreferred a owl:ObjectProperty,
        skos:Concept ;
    rdfs:label "nationalityPreferred"@en ;
    dct:description "Preferred nationality/culture/race/ethnicity/religion/sexual orientation of an ULAN agent. Domain is schema:Person/Organization, range is AAT concept" ;
    rdfs:comment "Preferred nationality/culture/race/ethnicity/religion/sexual orientation of an ULAN agent. Domain is schema:Person/Organization, range is AAT concept" ;
    rdfs:isDefinedBy <http://vocab.getty.edu/ontology> ;
    rdfs:range gvp:Subject ;
    rdfs:subPropertyOf schema:nationality ;
    skos:broader schema:nationality ;
    skos:inScheme <http://vocab.getty.edu/ontology> ;
    skos:prefLabel "nationalityPreferred"@en ;
    skos:topConceptOf <http://vocab.getty.edu/ontology> .

gvp:placeTypeNonPreferred a owl:ObjectProperty,
        skos:Concept ;
    rdfs:label "placeTypeNonPreferred"@en ;
    dct:description """A secondary type for a TGN Place. Domain is TGN concept, range is AAT concept.
Example: A non-preferred type of Machupicchu, Peru is "Inca center" (historical)""" ;
    rdfs:comment "A secondary type for a TGN Place. Domain is TGN concept, range is AAT concept" ;
    rdfs:domain gvp:Subject ;
    rdfs:isDefinedBy <http://vocab.getty.edu/ontology> ;
    rdfs:range gvp:Subject ;
    rdfs:subPropertyOf gvp:placeType ;
    skos:broader gvp:placeType ;
    skos:example "A non-preferred type of Machupicchu, Peru is \"Inca center\" (historical)" ;
    skos:inScheme <http://vocab.getty.edu/ontology> ;
    skos:prefLabel "placeTypeNonPreferred"@en ;
    skos:topConceptOf <http://vocab.getty.edu/ontology> .

gvp:placeTypePreferred a owl:ObjectProperty,
        skos:Concept ;
    rdfs:label "placeTypePreferred"@en ;
    dct:description """The primary type of a TGN Place. Domain is TGN concept, range is AAT concept.
Example: The preferred place type of Machupicchu, Peru is "deserted settlement" (current)""" ;
    rdfs:comment "The primary type of a TGN Place. Domain is TGN concept, range is AAT concept" ;
    rdfs:domain gvp:Subject ;
    rdfs:isDefinedBy <http://vocab.getty.edu/ontology> ;
    rdfs:range gvp:Subject ;
    rdfs:subPropertyOf gvp:placeType ;
    skos:broader gvp:placeType ;
    skos:example "The preferred place type of Machupicchu, Peru is \"deserted settlement\" (current)" ;
    skos:inScheme <http://vocab.getty.edu/ontology> ;
    skos:prefLabel "placeTypePreferred"@en ;
    skos:topConceptOf <http://vocab.getty.edu/ontology> .

gvp:sourceAlternatePreferred a owl:ObjectProperty,
        skos:Concept ;
    rdfs:label "sourceAlternatePreferred"@en ;
    dct:description """Source for which the term is Alternate Preferred. Range is bibo:Document or bibo:DocumentPart.
Example: "Kayseri" is alternate preferred in Webster's New Geographical Dictionary (1988)""" ;
    rdfs:comment "Source for which the term is Alternate Preferred. Range is bibo:Document or bibo:DocumentPart" ;
    rdfs:domain skosxl:Label ;
    rdfs:isDefinedBy <http://vocab.getty.edu/ontology> ;
    rdfs:range bibo:Document ;
    rdfs:subPropertyOf dct:source ;
    skos:broader dct:source ;
    skos:example "\"Kayseri\" is alternate preferred in Webster's New Geographical Dictionary (1988)" ;
    skos:inScheme <http://vocab.getty.edu/ontology> ;
    skos:prefLabel "sourceAlternatePreferred"@en ;
    skos:topConceptOf <http://vocab.getty.edu/ontology> .

gvp:sourceNonPreferred a owl:ObjectProperty,
        skos:Concept ;
    rdfs:label "sourceNonPreferred"@en ;
    dct:description """Source for which the term is Non-preferred. Range is bibo:Document or bibo:DocumentPart.
Example: "Panderma" is non-preferred in Webster's New Geographical Dictionary (1988)""" ;
    rdfs:comment "Source for which the term is Non-preferred. Range is bibo:Document or bibo:DocumentPart" ;
    rdfs:domain skosxl:Label ;
    rdfs:isDefinedBy <http://vocab.getty.edu/ontology> ;
    rdfs:range bibo:Document ;
    rdfs:subPropertyOf dct:source ;
    skos:broader dct:source ;
    skos:example "\"Panderma\" is non-preferred in Webster's New Geographical Dictionary (1988)" ;
    skos:inScheme <http://vocab.getty.edu/ontology> ;
    skos:prefLabel "sourceNonPreferred"@en ;
    skos:topConceptOf <http://vocab.getty.edu/ontology> .

gvp:sourcePreferred a owl:ObjectProperty,
        skos:Concept ;
    rdfs:label "sourcePreferred"@en ;
    dct:description """Source for which the term is Preferred. Range is bibo:Document or bibo:DocumentPart.
Example: "Isfahan" is preferred in Webster's New Geographical Dictionary (1988)""" ;
    rdfs:comment "Source for which the term is Preferred. Range is bibo:Document or bibo:DocumentPart" ;
    rdfs:domain skosxl:Label ;
    rdfs:isDefinedBy <http://vocab.getty.edu/ontology> ;
    rdfs:range bibo:Document ;
    rdfs:subPropertyOf dct:source ;
    skos:broader dct:source ;
    skos:example "\"Isfahan\" is preferred in Webster's New Geographical Dictionary (1988)" ;
    skos:inScheme <http://vocab.getty.edu/ontology> ;
    skos:prefLabel "sourcePreferred"@en ;
    skos:topConceptOf <http://vocab.getty.edu/ontology> .

gvp:tgn3001_distinguished_from a owl:ObjectProperty,
        owl:SymmetricProperty,
        skos:Concept ;
    dc:identifier "3001" ;
    dc:title "distinguished from - any" ;
    dct:description """any - distinguished from - any.\r
Example: The Ancient Mesopotamian Kingdom 'Assyria' is distinguished from the Roman Province of the same name""" ;
    rdfs:domain skos:Concept ;
    rdfs:isDefinedBy <http://vocab.getty.edu/ontology>,
        tgn: ;
    rdfs:range skos:Concept ;
    rdfs:subPropertyOf skos:related ;
    skos:broader skos:related ;
    skos:example "The Ancient Mesopotamian Kingdom 'Assyria' is distinguished from the Roman Province of the same name" ;
    skos:inScheme <http://vocab.getty.edu/ontology> ;
    skos:notation "3001" ;
    skos:prefLabel "tgn3001_distinguished_from"@en ;
    skos:topConceptOf <http://vocab.getty.edu/ontology> .

gvp:tgn3005_possibly_identified_as a owl:ObjectProperty,
        owl:SymmetricProperty,
        skos:Concept ;
    dc:identifier "3005" ;
    dc:title "possibly identified as - place" ;
    dct:description """place - possibly identified as - place.\r
Example: The lost settlement of Sharuhen is possibly identified as Tel el-Far'ah (As Suwayda', Syria) (deserted settlement)""" ;
    rdfs:domain skos:Concept ;
    rdfs:isDefinedBy <http://vocab.getty.edu/ontology>,
        tgn: ;
    rdfs:range skos:Concept ;
    rdfs:subPropertyOf skos:related ;
    skos:broader skos:related ;
    skos:example "The lost settlement of Sharuhen is possibly identified as Tel el-Far'ah (As Suwayda', Syria) (deserted settlement)" ;
    skos:inScheme <http://vocab.getty.edu/ontology> ;
    skos:notation "3005" ;
    skos:prefLabel "tgn3005_possibly_identified_as"@en ;
    skos:topConceptOf <http://vocab.getty.edu/ontology> .

gvp:tgn3201_capital_of a owl:ObjectProperty,
        skos:Concept ;
    dc:identifier "3201" ;
    dc:title "capital of - nation" ;
    dct:description """city - capital of - nation.\r
Example: Thecapital of Maxima Caesariensis from 296 to 800 CE was London""" ;
    rdfs:domain skos:Concept ;
    rdfs:isDefinedBy <http://vocab.getty.edu/ontology>,
        tgn: ;
    rdfs:range skos:Concept ;
    rdfs:subPropertyOf skos:related ;
    owl:inverseOf gvp:tgn3202_capital_is ;
    skos:broader skos:related ;
    skos:example "Thecapital of Maxima Caesariensis from 296 to 800 CE was London" ;
    skos:inScheme <http://vocab.getty.edu/ontology> ;
    skos:notation "3201" ;
    skos:prefLabel "tgn3201_capital_of"@en ;
    skos:topConceptOf <http://vocab.getty.edu/ontology> .

gvp:tgn3301_ally_of a owl:ObjectProperty,
        owl:SymmetricProperty,
        skos:Concept ;
    dc:identifier "3301" ;
    dc:title "ally of - nation" ;
    dct:description """nation - ally of - nation.\r
Example: Siena, Arezzo, Pisa, and Pistoia were Ghibeline allies during the 13th and 14th centuries.""" ;
    rdfs:domain skos:Concept ;
    rdfs:isDefinedBy <http://vocab.getty.edu/ontology>,
        tgn: ;
    rdfs:range skos:Concept ;
    rdfs:subPropertyOf skos:related ;
    skos:broader skos:related ;
    skos:example "Siena, Arezzo, Pisa, and Pistoia were Ghibeline allies during the 13th and 14th centuries." ;
    skos:inScheme <http://vocab.getty.edu/ontology> ;
    skos:notation "3301" ;
    skos:prefLabel "tgn3301_ally_of"@en ;
    skos:topConceptOf <http://vocab.getty.edu/ontology> .

gvp:tgn3401_moved_from a owl:ObjectProperty,
        skos:Concept ;
    dc:identifier "3401" ;
    dc:title "moved from - place" ;
    dct:description """place - moved from - place; Note: places that were physically moved from one location to another, often due to the threat or occurrence of natural disaster..\r
Example: Troupville, Georgia, USA was moved to Valdosta (Lowndes county, Georgia, USA)""" ;
    rdfs:domain skos:Concept ;
    rdfs:isDefinedBy <http://vocab.getty.edu/ontology>,
        tgn: ;
    rdfs:range skos:Concept ;
    rdfs:subPropertyOf skos:related ;
    owl:inverseOf gvp:tgn3402_moved_to ;
    skos:broader skos:related ;
    skos:example "Troupville, Georgia, USA was moved to Valdosta (Lowndes county, Georgia, USA)" ;
    skos:inScheme <http://vocab.getty.edu/ontology> ;
    skos:notation "3401" ;
    skos:prefLabel "tgn3401_moved_from"@en ;
    skos:scopeNote "Note: places that were physically moved from one location to another, often due to the threat or occurrence of natural disaster." ;
    skos:topConceptOf <http://vocab.getty.edu/ontology> .

gvp:ulan1000_related_to a owl:ObjectProperty,
        owl:SymmetricProperty,
        skos:Concept ;
    dc:identifier "1000" ;
    dc:title "related to - any" ;
    dct:description """any - related to - any.\r
Example: Frank Lloyd Wright is related to Francis Conroy Sullivan; Herman Miller, Inc. is related to Irving Harper; National Endowment for the Humanities is related to Connecticut Humanities Council""" ;
    rdfs:domain skos:Concept ;
    rdfs:isDefinedBy <http://vocab.getty.edu/ontology>,
        ulan: ;
    rdfs:range skos:Concept ;
    rdfs:subPropertyOf skos:related ;
    skos:broader skos:related ;
    skos:example "Frank Lloyd Wright is related to Francis Conroy Sullivan",
        "Herman Miller, Inc. is related to Irving Harper",
        "National Endowment for the Humanities is related to Connecticut Humanities Council" ;
    skos:inScheme <http://vocab.getty.edu/ontology> ;
    skos:notation "1000" ;
    skos:prefLabel "ulan1000_related_to"@en ;
    skos:topConceptOf <http://vocab.getty.edu/ontology> .

gvp:ulan1006_formerly_identified_with a owl:ObjectProperty,
        owl:SymmetricProperty,
        skos:Concept ;
    dc:identifier "1006" ;
    dc:title "formerly identified with - any" ;
    dct:description """any - formerly identified with - any.\r
Example: Tommaso is formerly identified with Tommaso di Stefano Lunetti; GreenWorks is formerly identified with Mike Faha & Associates""" ;
    rdfs:domain skos:Concept ;
    rdfs:isDefinedBy <http://vocab.getty.edu/ontology>,
        ulan: ;
    rdfs:range skos:Concept ;
    rdfs:subPropertyOf skos:related ;
    skos:broader skos:related ;
    skos:example "GreenWorks is formerly identified with Mike Faha & Associates",
        "Tommaso is formerly identified with Tommaso di Stefano Lunetti" ;
    skos:inScheme <http://vocab.getty.edu/ontology> ;
    skos:notation "1006" ;
    skos:prefLabel "ulan1006_formerly_identified_with"@en ;
    skos:topConceptOf <http://vocab.getty.edu/ontology> .

gvp:ulan1105_apprentice_of a owl:ObjectProperty,
        skos:Concept ;
    dc:identifier "1105" ;
    dc:title "apprentice of - person" ;
    dct:description """person - apprentice of - person.\r
Example: Nicolas Hawksmoor was the apprentice of Christopher Wren""" ;
    rdfs:domain skos:Concept ;
    rdfs:isDefinedBy <http://vocab.getty.edu/ontology>,
        ulan: ;
    rdfs:range skos:Concept ;
    rdfs:subPropertyOf skos:related ;
    owl:inverseOf gvp:ulan1106_apprentice_was ;
    skos:broader skos:related ;
    skos:example "Nicolas Hawksmoor was the apprentice of Christopher Wren" ;
    skos:inScheme <http://vocab.getty.edu/ontology> ;
    skos:notation "1105" ;
    skos:prefLabel "ulan1105_apprentice_of"@en ;
    skos:topConceptOf <http://vocab.getty.edu/ontology> .

gvp:ulan1111_master_of a owl:ObjectProperty,
        skos:Concept ;
    dc:identifier "1111" ;
    dc:title "master of - person" ;
    dct:description """person - master of - person.\r
Example: Peter Paul Rubens - master of Jan Thomas""" ;
    rdfs:domain skos:Concept ;
    rdfs:isDefinedBy <http://vocab.getty.edu/ontology>,
        ulan: ;
    rdfs:range skos:Concept ;
    rdfs:subPropertyOf skos:related ;
    owl:inverseOf gvp:ulan1112_master_was ;
    skos:broader skos:related ;
    skos:example "Peter Paul Rubens - master of Jan Thomas" ;
    skos:inScheme <http://vocab.getty.edu/ontology> ;
    skos:notation "1111" ;
    skos:prefLabel "ulan1111_master_of"@en ;
    skos:topConceptOf <http://vocab.getty.edu/ontology> .

gvp:ulan1113_fellow_student_of a owl:ObjectProperty,
        owl:SymmetricProperty,
        skos:Concept ;
    dc:identifier "1113" ;
    dc:title "fellow student of - person" ;
    dct:description """person - fellow student of - person.\r
Example: Alexander Calder was a fellow student of John Sloan; John Sloan was a fellow student of Thomas Hart Benton""" ;
    rdfs:domain skos:Concept ;
    rdfs:isDefinedBy <http://vocab.getty.edu/ontology>,
        ulan: ;
    rdfs:range skos:Concept ;
    rdfs:subPropertyOf skos:related ;
    skos:broader skos:related ;
    skos:example "Alexander Calder was a fellow student of John Sloan",
        "John Sloan was a fellow student of Thomas Hart Benton" ;
    skos:inScheme <http://vocab.getty.edu/ontology> ;
    skos:notation "1113" ;
    skos:prefLabel "ulan1113_fellow_student_of"@en ;
    skos:topConceptOf <http://vocab.getty.edu/ontology> .

gvp:ulan1203_donor_of a owl:ObjectProperty,
        skos:Concept ;
    dc:identifier "1203" ;
    dc:title "donor of - person/firm/family" ;
    dct:description """person/firm/family - donor of - person/firm/family.\r
Example: Andrew W. Mellon was a donor of National Gallery of Art""" ;
    rdfs:domain skos:Concept ;
    rdfs:isDefinedBy <http://vocab.getty.edu/ontology>,
        ulan: ;
    rdfs:range skos:Concept ;
    rdfs:subPropertyOf skos:related ;
    owl:inverseOf gvp:ulan1204_donor_was ;
    skos:broader skos:related ;
    skos:example "Andrew W. Mellon was a donor of National Gallery of Art" ;
    skos:inScheme <http://vocab.getty.edu/ontology> ;
    skos:notation "1203" ;
    skos:prefLabel "ulan1203_donor_of"@en ;
    skos:topConceptOf <http://vocab.getty.edu/ontology> .

gvp:ulan1205_client_of a owl:ObjectProperty,
        skos:Concept ;
    dc:identifier "1205" ;
    dc:title "client of - person/firm/family" ;
    dct:description """person/firm/family - client of - person/firm/family.\r
Example: The Chicago Herald was the client of Burnham and Root""" ;
    rdfs:domain skos:Concept ;
    rdfs:isDefinedBy <http://vocab.getty.edu/ontology>,
        ulan: ;
    rdfs:range skos:Concept ;
    rdfs:subPropertyOf skos:related ;
    owl:inverseOf gvp:ulan1206_client_was ;
    skos:broader skos:related ;
    skos:example "The Chicago Herald was the client of Burnham and Root" ;
    skos:inScheme <http://vocab.getty.edu/ontology> ;
    skos:notation "1205" ;
    skos:prefLabel "ulan1205_client_of"@en ;
    skos:topConceptOf <http://vocab.getty.edu/ontology> .

gvp:ulan1211_artist_to a owl:ObjectProperty,
        skos:Concept ;
    dc:identifier "1211" ;
    dc:title "artist to - person" ;
    dct:description """person - artist to - person.\r
Example: Artist to Louis XIV, King of France was Charles-Pierre Coustou""" ;
    rdfs:domain skos:Concept ;
    rdfs:isDefinedBy <http://vocab.getty.edu/ontology>,
        ulan: ;
    rdfs:range skos:Concept ;
    rdfs:subPropertyOf skos:related ;
    owl:inverseOf gvp:ulan1212_artist_was ;
    skos:broader skos:related ;
    skos:example "Artist to Louis XIV, King of France was Charles-Pierre Coustou" ;
    skos:inScheme <http://vocab.getty.edu/ontology> ;
    skos:notation "1211" ;
    skos:prefLabel "ulan1211_artist_to"@en ;
    skos:topConceptOf <http://vocab.getty.edu/ontology> .

gvp:ulan1213_court_artist_to a owl:ObjectProperty,
        skos:Concept ;
    dc:identifier "1213" ;
    dc:title "court artist to - person" ;
    dct:description """person - court artist to - person.\r
Example: Court artist to Gonzaga Vincenzo I, Duke of Mantua was Peter Paul Rubens; court artist to Charles IV, King of Spain was Francisco de Goya""" ;
    rdfs:domain skos:Concept ;
    rdfs:isDefinedBy <http://vocab.getty.edu/ontology>,
        ulan: ;
    rdfs:range skos:Concept ;
    rdfs:subPropertyOf skos:related ;
    owl:inverseOf gvp:ulan1214_court_artist_was ;
    skos:broader skos:related ;
    skos:example "Court artist to Gonzaga Vincenzo I, Duke of Mantua was Peter Paul Rubens",
        "court artist to Charles IV, King of Spain was Francisco de Goya" ;
    skos:inScheme <http://vocab.getty.edu/ontology> ;
    skos:notation "1213" ;
    skos:prefLabel "ulan1213_court_artist_to"@en ;
    skos:topConceptOf <http://vocab.getty.edu/ontology> .

gvp:ulan1217_employee_of a owl:ObjectProperty,
        skos:Concept ;
    dc:identifier "1217" ;
    dc:title "employee of - person" ;
    dct:description """person/firm - employee of - person.\r
Example: Employee of Christopher Wren was Jean Tijou""" ;
    rdfs:domain skos:Concept ;
    rdfs:isDefinedBy <http://vocab.getty.edu/ontology>,
        ulan: ;
    rdfs:range skos:Concept ;
    rdfs:subPropertyOf skos:related ;
    owl:inverseOf gvp:ulan1218_employee_was ;
    skos:broader skos:related ;
    skos:example "Employee of Christopher Wren was Jean Tijou" ;
    skos:inScheme <http://vocab.getty.edu/ontology> ;
    skos:notation "1217" ;
    skos:prefLabel "ulan1217_employee_of"@en ;
    skos:topConceptOf <http://vocab.getty.edu/ontology> .

gvp:ulan1301_colleague_of a owl:ObjectProperty,
        owl:SymmetricProperty,
        skos:Concept ;
    dc:identifier "1301" ;
    dc:title "colleague of - person" ;
    dct:description """person - colleague of - person.\r
Example: Titian was a colleague of Maria Giovanni Verdizotti""" ;
    rdfs:domain skos:Concept ;
    rdfs:isDefinedBy <http://vocab.getty.edu/ontology>,
        ulan: ;
    rdfs:range skos:Concept ;
    rdfs:subPropertyOf skos:related ;
    skos:broader skos:related ;
    skos:example "Titian was a colleague of Maria Giovanni Verdizotti" ;
    skos:inScheme <http://vocab.getty.edu/ontology> ;
    skos:notation "1301" ;
    skos:prefLabel "ulan1301_colleague_of"@en ;
    skos:topConceptOf <http://vocab.getty.edu/ontology> .

gvp:ulan1302_associate_of a owl:ObjectProperty,
        owl:SymmetricProperty,
        skos:Concept ;
    dc:identifier "1302" ;
    dc:title "associate of - person" ;
    dct:description """person - associate of - person.\r
Example: Frank Lloyd Wright was an associate of Giannini and Hilgart""" ;
    rdfs:domain skos:Concept ;
    rdfs:isDefinedBy <http://vocab.getty.edu/ontology>,
        ulan: ;
    rdfs:range skos:Concept ;
    rdfs:subPropertyOf skos:related ;
    skos:broader skos:related ;
    skos:example "Frank Lloyd Wright was an associate of Giannini and Hilgart" ;
    skos:inScheme <http://vocab.getty.edu/ontology> ;
    skos:notation "1302" ;
    skos:prefLabel "ulan1302_associate_of"@en ;
    skos:topConceptOf <http://vocab.getty.edu/ontology> .

gvp:ulan1306_performs_with a owl:ObjectProperty,
        owl:SymmetricProperty,
        skos:Concept ;
    dc:identifier "1306" ;
    dc:title "performs with - person" ;
    dct:description """person - performs with - person.\r
Example: Harry Kipper performs with Harry Kipper (as part of 'The Kipper Kids')""" ;
    rdfs:domain skos:Concept ;
    rdfs:isDefinedBy <http://vocab.getty.edu/ontology>,
        ulan: ;
    rdfs:range skos:Concept ;
    rdfs:subPropertyOf skos:related ;
    skos:broader skos:related ;
    skos:example "Harry Kipper performs with Harry Kipper (as part of 'The Kipper Kids')" ;
    skos:inScheme <http://vocab.getty.edu/ontology> ;
    skos:notation "1306" ;
    skos:prefLabel "ulan1306_performs_with"@en ;
    skos:topConceptOf <http://vocab.getty.edu/ontology> .

gvp:ulan1309_advisor_of a owl:ObjectProperty,
        skos:Concept ;
    dc:identifier "1309" ;
    dc:title "advisor of - person" ;
    dct:description """person - advisor of - person.\r
Example: Thomas Cromwell, Earl of Essex was the advisor of Henry VIII, King of England""" ;
    rdfs:domain skos:Concept ;
    rdfs:isDefinedBy <http://vocab.getty.edu/ontology>,
        ulan: ;
    rdfs:range skos:Concept ;
    rdfs:subPropertyOf skos:related ;
    owl:inverseOf gvp:ulan1310_advised_by ;
    skos:broader skos:related ;
    skos:example "Thomas Cromwell, Earl of Essex was the advisor of Henry VIII, King of England" ;
    skos:inScheme <http://vocab.getty.edu/ontology> ;
    skos:notation "1309" ;
    skos:prefLabel "ulan1309_advisor_of"@en ;
    skos:topConceptOf <http://vocab.getty.edu/ontology> .

gvp:ulan1313_partner_in a owl:ObjectProperty,
        skos:Concept ;
    dc:identifier "1313" ;
    dc:title "partner in - firm" ;
    dct:description """person - partner in - firm.\r
Example: Parners of Adler and Sullivan included Louis H. Sullivan and Dankmar Adler""" ;
    rdfs:domain skos:Concept ;
    rdfs:isDefinedBy <http://vocab.getty.edu/ontology>,
        ulan: ;
    rdfs:range skos:Concept ;
    rdfs:subPropertyOf skos:related ;
    owl:inverseOf gvp:ulan1314_partner_was ;
    skos:broader skos:related ;
    skos:example "Parners of Adler and Sullivan included Louis H. Sullivan and Dankmar Adler" ;
    skos:inScheme <http://vocab.getty.edu/ontology> ;
    skos:notation "1313" ;
    skos:prefLabel "ulan1313_partner_in"@en ;
    skos:topConceptOf <http://vocab.getty.edu/ontology> .

gvp:ulan1331_worked_with a owl:ObjectProperty,
        skos:Concept ;
    dc:identifier "1331" ;
    dc:title "worked with - person" ;
    dct:description """any - worked with - person.\r
Example: Scarsellino and Domenichino worked with the Carracci family""" ;
    rdfs:domain skos:Concept ;
    rdfs:isDefinedBy <http://vocab.getty.edu/ontology>,
        ulan: ;
    rdfs:range skos:Concept ;
    rdfs:subPropertyOf skos:related ;
    owl:inverseOf gvp:ulan1332_worker_was ;
    skos:broader skos:related ;
    skos:example "Scarsellino and Domenichino worked with the Carracci family" ;
    skos:inScheme <http://vocab.getty.edu/ontology> ;
    skos:notation "1331" ;
    skos:prefLabel "ulan1331_worked_with"@en ;
    skos:topConceptOf <http://vocab.getty.edu/ontology> .

gvp:ulan1411_successor_of a owl:ObjectProperty,
        skos:Concept ;
    dc:identifier "1411" ;
    dc:title "successor of - firm/group" ;
    dct:description """firm/group - successor of - firm/group.\r
Example: Richard Meier & Partners Architects LLP is the successor of Richard Meier & Associates""" ;
    rdfs:domain skos:Concept ;
    rdfs:isDefinedBy <http://vocab.getty.edu/ontology>,
        ulan: ;
    rdfs:range skos:Concept ;
    rdfs:subPropertyOf skos:related ;
    owl:inverseOf gvp:ulan1412_predecessor_of ;
    skos:broader skos:related ;
    skos:example "Richard Meier & Partners Architects LLP is the successor of Richard Meier & Associates" ;
    skos:inScheme <http://vocab.getty.edu/ontology> ;
    skos:notation "1411" ;
    skos:prefLabel "ulan1411_successor_of"@en ;
    skos:topConceptOf <http://vocab.getty.edu/ontology> .

gvp:ulan1414_joint_venture_with a owl:ObjectProperty,
        owl:SymmetricProperty,
        skos:Concept ;
    dc:identifier "1414" ;
    dc:title "joint venture with - firm/group" ;
    dct:description """firm/group - joint venture with - firm/group.\r
Example: Schwetye Luchini Architects is in a joint venture with ACME Architects""" ;
    rdfs:domain skos:Concept ;
    rdfs:isDefinedBy <http://vocab.getty.edu/ontology>,
        ulan: ;
    rdfs:range skos:Concept ;
    rdfs:subPropertyOf skos:related ;
    skos:broader skos:related ;
    skos:example "Schwetye Luchini Architects is in a joint venture with ACME Architects" ;
    skos:inScheme <http://vocab.getty.edu/ontology> ;
    skos:notation "1414" ;
    skos:prefLabel "ulan1414_joint_venture_with"@en ;
    skos:topConceptOf <http://vocab.getty.edu/ontology> .

gvp:ulan1513_grandchild_of a owl:ObjectProperty,
        skos:Concept ;
    dc:identifier "1513" ;
    dc:title "grandchild of - person" ;
    dct:description """person - grandchild of - person.\r
Example: Eric Lloyd Wright is the grandchild of Frank Lloyd Wright""" ;
    rdfs:domain skos:Concept ;
    rdfs:isDefinedBy <http://vocab.getty.edu/ontology>,
        ulan: ;
    rdfs:range skos:Concept ;
    rdfs:subPropertyOf skos:related ;
    owl:inverseOf gvp:ulan1514_gandparent_of ;
    skos:broader skos:related ;
    skos:example "Eric Lloyd Wright is the grandchild of Frank Lloyd Wright" ;
    skos:inScheme <http://vocab.getty.edu/ontology> ;
    skos:notation "1513" ;
    skos:prefLabel "ulan1513_grandchild_of"@en ;
    skos:topConceptOf <http://vocab.getty.edu/ontology> .

gvp:ulan1541_spouse_of a owl:ObjectProperty,
        owl:SymmetricProperty,
        skos:Concept ;
    dc:identifier "1541" ;
    dc:title "spouse of - person" ;
    dct:description """person - spouse of - person.\r
Example: Alfred Stieglitz and Georgia O'Keeffe were married to each other""" ;
    rdfs:domain skos:Concept ;
    rdfs:isDefinedBy <http://vocab.getty.edu/ontology>,
        ulan: ;
    rdfs:range skos:Concept ;
    rdfs:subPropertyOf skos:related ;
    skos:broader skos:related ;
    skos:example "Alfred Stieglitz and Georgia O'Keeffe were married to each other" ;
    skos:inScheme <http://vocab.getty.edu/ontology> ;
    skos:notation "1541" ;
    skos:prefLabel "ulan1541_spouse_of"@en ;
    skos:topConceptOf <http://vocab.getty.edu/ontology> .

gvp:ulan1550_relative_by_marriage a owl:ObjectProperty,
        owl:SymmetricProperty,
        skos:Concept ;
    dc:identifier "1550" ;
    dc:title "relative by marriage - person" ;
    dct:description """person - relative by marriage (in-law) - person.\r
Example: Juana Galarza d Goicoechea and Francisco de Goya are related by marriage""" ;
    rdfs:domain skos:Concept ;
    rdfs:isDefinedBy <http://vocab.getty.edu/ontology>,
        ulan: ;
    rdfs:range skos:Concept ;
    rdfs:subPropertyOf skos:related ;
    skos:broader skos:related ;
    skos:example "Juana Galarza d Goicoechea and Francisco de Goya are related by marriage" ;
    skos:inScheme <http://vocab.getty.edu/ontology> ;
    skos:notation "1550" ;
    skos:prefLabel "ulan1550_relative_by_marriage"@en ;
    skos:topConceptOf <http://vocab.getty.edu/ontology> .

gvp:ulan1552_parent_by_marriage_of a owl:ObjectProperty,
        skos:Concept ;
    dc:identifier "1552" ;
    dc:title "parent by marriage of - person" ;
    dct:description """person - parent by marriage (step parent) - person.\r
Example: Frans Hals is a parent by marriage of Pieter Gerritsz van Roestraten""" ;
    rdfs:domain skos:Concept ;
    rdfs:isDefinedBy <http://vocab.getty.edu/ontology>,
        ulan: ;
    rdfs:range skos:Concept ;
    rdfs:subPropertyOf skos:related ;
    owl:inverseOf gvp:ulan1553_child_by_marriage_of ;
    skos:broader skos:related ;
    skos:example "Frans Hals is a parent by marriage of Pieter Gerritsz van Roestraten" ;
    skos:inScheme <http://vocab.getty.edu/ontology> ;
    skos:notation "1552" ;
    skos:prefLabel "ulan1552_parent_by_marriage_of"@en ;
    skos:topConceptOf <http://vocab.getty.edu/ontology> .

gvp:ulan1556_half-sibling_of a owl:ObjectProperty,
        owl:SymmetricProperty,
        skos:Concept ;
    dc:identifier "1556" ;
    dc:title "half-sibling of - person" ;
    dct:description """person - half-sibling of - person.\r
Example: Juan Bautista Monegro and Luis de Carbajal are half siblings""" ;
    rdfs:domain skos:Concept ;
    rdfs:isDefinedBy <http://vocab.getty.edu/ontology>,
        ulan: ;
    rdfs:range skos:Concept ;
    rdfs:subPropertyOf skos:related ;
    skos:broader skos:related ;
    skos:example "Juan Bautista Monegro and Luis de Carbajal are half siblings" ;
    skos:inScheme <http://vocab.getty.edu/ontology> ;
    skos:notation "1556" ;
    skos:prefLabel "ulan1556_half-sibling_of"@en ;
    skos:topConceptOf <http://vocab.getty.edu/ontology> .

gvp:ulan1557_step-sibling_of a owl:ObjectProperty,
        owl:SymmetricProperty,
        skos:Concept ;
    dc:identifier "1557" ;
    dc:title "step-sibling of - person" ;
    dct:description """person - step-sibling of - person.\r
Example: W. L. Wyllie and Lionel Percy Smythe are step-siblings""" ;
    rdfs:domain skos:Concept ;
    rdfs:isDefinedBy <http://vocab.getty.edu/ontology>,
        ulan: ;
    rdfs:range skos:Concept ;
    rdfs:subPropertyOf skos:related ;
    skos:broader skos:related ;
    skos:example "W. L. Wyllie and Lionel Percy Smythe are step-siblings" ;
    skos:inScheme <http://vocab.getty.edu/ontology> ;
    skos:notation "1557" ;
    skos:prefLabel "ulan1557_step-sibling_of"@en ;
    skos:topConceptOf <http://vocab.getty.edu/ontology> .

gvp:ulan1574_godparent_of a owl:ObjectProperty,
        skos:Concept ;
    dc:identifier "1574" ;
    dc:title "godparent of - person" ;
    dct:description """person - godparent of - person.\r
Example: Jean-Baptiste Goy is godparent of Jean I Nocret""" ;
    rdfs:domain skos:Concept ;
    rdfs:isDefinedBy <http://vocab.getty.edu/ontology>,
        ulan: ;
    rdfs:range skos:Concept ;
    rdfs:subPropertyOf skos:related ;
    owl:inverseOf gvp:ulan1575_godchild_of ;
    skos:broader skos:related ;
    skos:example "Jean-Baptiste Goy is godparent of Jean I Nocret" ;
    skos:inScheme <http://vocab.getty.edu/ontology> ;
    skos:notation "1574" ;
    skos:prefLabel "ulan1574_godparent_of"@en ;
    skos:topConceptOf <http://vocab.getty.edu/ontology> .

gvp:ulan1581_descendant_of a owl:ObjectProperty,
        skos:Concept ;
    dc:identifier "1581" ;
    dc:title "descendant of - person" ;
    dct:description """person - descendant of - person.\r
Example: Paolo Caliari is the descendant of Paolo Veronese""" ;
    rdfs:domain skos:Concept ;
    rdfs:isDefinedBy <http://vocab.getty.edu/ontology>,
        ulan: ;
    rdfs:range skos:Concept ;
    rdfs:subPropertyOf skos:related ;
    owl:inverseOf gvp:ulan1582_ancestor_of ;
    skos:broader skos:related ;
    skos:example "Paolo Caliari is the descendant of Paolo Veronese" ;
    skos:inScheme <http://vocab.getty.edu/ontology> ;
    skos:notation "1581" ;
    skos:prefLabel "ulan1581_descendant_of"@en ;
    skos:topConceptOf <http://vocab.getty.edu/ontology> .

gvp:ulan1590_possibly_related_to a owl:ObjectProperty,
        owl:SymmetricProperty,
        skos:Concept ;
    dc:identifier "1590" ;
    dc:title "possibly related to - person" ;
    dct:description """person - possibly related to (familial relationship) - person.\r
Example: A familial relationship between Ramon Destorrents, the younger and Ramon Destorrents, the elder is possible""" ;
    rdfs:domain skos:Concept ;
    rdfs:isDefinedBy <http://vocab.getty.edu/ontology>,
        ulan: ;
    rdfs:range skos:Concept ;
    rdfs:subPropertyOf skos:related ;
    skos:broader skos:related ;
    skos:example "A familial relationship between Ramon Destorrents, the younger and Ramon Destorrents, the elder is possible" ;
    skos:inScheme <http://vocab.getty.edu/ontology> ;
    skos:notation "1590" ;
    skos:prefLabel "ulan1590_possibly_related_to"@en ;
    skos:topConceptOf <http://vocab.getty.edu/ontology> .

gvp:ulan2572_founder_of a owl:ObjectProperty,
        skos:Concept ;
    dc:identifier "2572" ;
    dc:title "founder of - institution" ;
    dct:description """person - founder of - institution.\r
Example: Louis Comfort Tiffany was the founder of Tiffany Glass & Decorating Company""" ;
    rdfs:domain skos:Concept ;
    rdfs:isDefinedBy <http://vocab.getty.edu/ontology>,
        ulan: ;
    rdfs:range skos:Concept ;
    rdfs:subPropertyOf skos:related ;
    owl:inverseOf gvp:ulan2573_founded_by ;
    skos:broader skos:related ;
    skos:example "Louis Comfort Tiffany was the founder of Tiffany Glass & Decorating Company" ;
    skos:inScheme <http://vocab.getty.edu/ontology> ;
    skos:notation "2572" ;
    skos:prefLabel "ulan2572_founder_of"@en ;
    skos:topConceptOf <http://vocab.getty.edu/ontology> .

gvp:ulan2574_director_of a owl:ObjectProperty,
        skos:Concept ;
    dc:identifier "2574" ;
    dc:title "director of - institution" ;
    dct:description """person - director of - institution.\r
Example: Jean Jans I directed Gobelins Tapestry Manufactory""" ;
    rdfs:domain skos:Concept ;
    rdfs:isDefinedBy <http://vocab.getty.edu/ontology>,
        ulan: ;
    rdfs:range skos:Concept ;
    rdfs:subPropertyOf skos:related ;
    owl:inverseOf gvp:ulan2575_directed_by ;
    skos:broader skos:related ;
    skos:example "Jean Jans I directed Gobelins Tapestry Manufactory" ;
    skos:inScheme <http://vocab.getty.edu/ontology> ;
    skos:notation "2574" ;
    skos:prefLabel "ulan2574_director_of"@en ;
    skos:topConceptOf <http://vocab.getty.edu/ontology> .

gvp:ulan2578_trustee_of a owl:ObjectProperty,
        skos:Concept ;
    dc:identifier "2578" ;
    dc:title "trustee of - institution" ;
    dct:description """person - trustee of - institution.\r
Example: George Douglas Haig was a trustee of the National Galleries of Scotland""" ;
    rdfs:domain skos:Concept ;
    rdfs:isDefinedBy <http://vocab.getty.edu/ontology>,
        ulan: ;
    rdfs:range skos:Concept ;
    rdfs:subPropertyOf skos:related ;
    owl:inverseOf gvp:ulan2579_trustee_was ;
    skos:broader skos:related ;
    skos:example "George Douglas Haig was a trustee of the National Galleries of Scotland" ;
    skos:inScheme <http://vocab.getty.edu/ontology> ;
    skos:notation "2578" ;
    skos:prefLabel "ulan2578_trustee_of"@en ;
    skos:topConceptOf <http://vocab.getty.edu/ontology> .

gvp:ulan2583_chairman_of a owl:ObjectProperty,
        skos:Concept ;
    dc:identifier "2583" ;
    dc:title "chairman of - institution" ;
    dct:description "person - chairman of - institution" ;
    rdfs:domain skos:Concept ;
    rdfs:isDefinedBy <http://vocab.getty.edu/ontology>,
        ulan: ;
    rdfs:range skos:Concept ;
    rdfs:subPropertyOf skos:related ;
    owl:inverseOf gvp:ulan2584_chaired_by ;
    skos:broader skos:related ;
    skos:inScheme <http://vocab.getty.edu/ontology> ;
    skos:notation "2583" ;
    skos:prefLabel "ulan2583_chairman_of"@en ;
    skos:topConceptOf <http://vocab.getty.edu/ontology> .

gvp:ulan2674_professor_at a owl:ObjectProperty,
        skos:Concept ;
    dc:identifier "2674" ;
    dc:title "professor at - institution" ;
    dct:description """person - professor at - institution.\r
Example: Paul Klee was a professor at Bauhaus""" ;
    rdfs:domain skos:Concept ;
    rdfs:isDefinedBy <http://vocab.getty.edu/ontology>,
        ulan: ;
    rdfs:range skos:Concept ;
    rdfs:subPropertyOf skos:related ;
    owl:inverseOf gvp:ulan2675_professor_was ;
    skos:broader skos:related ;
    skos:example "Paul Klee was a professor at Bauhaus" ;
    skos:inScheme <http://vocab.getty.edu/ontology> ;
    skos:notation "2674" ;
    skos:prefLabel "ulan2674_professor_at"@en ;
    skos:topConceptOf <http://vocab.getty.edu/ontology> .

gvp:ulan2696_leader_of a owl:ObjectProperty,
        skos:Concept ;
    dc:identifier "2696" ;
    dc:title "leader of - institution" ;
    dct:description """person - leader of - institution.\r
Example: Rush Harrison Kress was the leader of Samuel H. Kress Foundation""" ;
    rdfs:domain skos:Concept ;
    rdfs:isDefinedBy <http://vocab.getty.edu/ontology>,
        ulan: ;
    rdfs:range skos:Concept ;
    rdfs:subPropertyOf skos:related ;
    owl:inverseOf gvp:ulan2697_leader_was ;
    skos:broader skos:related ;
    skos:example "Rush Harrison Kress was the leader of Samuel H. Kress Foundation" ;
    skos:inScheme <http://vocab.getty.edu/ontology> ;
    skos:notation "2696" ;
    skos:prefLabel "ulan2696_leader_of"@en ;
    skos:topConceptOf <http://vocab.getty.edu/ontology> .

gvp:ulan2778_owner_of a owl:ObjectProperty,
        skos:Concept ;
    dc:identifier "2778" ;
    dc:title "owner of - person" ;
    dct:description """firm - owner of - person.\r
Example: Walter Scott Lenox was the owner of Lenox China Co.""" ;
    rdfs:domain skos:Concept ;
    rdfs:isDefinedBy <http://vocab.getty.edu/ontology>,
        ulan: ;
    rdfs:range skos:Concept ;
    rdfs:subPropertyOf skos:related ;
    owl:inverseOf gvp:ulan2779_owned_by ;
    skos:broader skos:related ;
    skos:example "Walter Scott Lenox was the owner of Lenox China Co." ;
    skos:inScheme <http://vocab.getty.edu/ontology> ;
    skos:notation "2778" ;
    skos:prefLabel "ulan2778_owner_of"@en ;
    skos:topConceptOf <http://vocab.getty.edu/ontology> .

gvp:ulan2781_dedicatee_of a owl:ObjectProperty,
        skos:Concept ;
    dc:identifier "2781" ;
    dc:title "dedicatee of - institution" ;
    dct:description """person - dedicatee of - institution.\r
Example: Auguste Rodin is the dedicatee of The Rodin Museum in Philadelphia""" ;
    rdfs:domain skos:Concept ;
    rdfs:isDefinedBy <http://vocab.getty.edu/ontology>,
        ulan: ;
    rdfs:range skos:Concept ;
    rdfs:subPropertyOf skos:related ;
    owl:inverseOf gvp:ulan2782_dedicated_to ;
    skos:broader skos:related ;
    skos:example "Auguste Rodin is the dedicatee of The Rodin Museum in Philadelphia" ;
    skos:inScheme <http://vocab.getty.edu/ontology> ;
    skos:notation "2781" ;
    skos:prefLabel "ulan2781_dedicatee_of"@en ;
    skos:topConceptOf <http://vocab.getty.edu/ontology> .

gvp:ulan2828_student_at a owl:ObjectProperty,
        skos:Concept ;
    dc:identifier "2828" ;
    dc:title "student at - institution" ;
    dct:description """person - student at - institution.\r
Example: Zdanek Rossman was a student at Bauhaus""" ;
    rdfs:domain skos:Concept ;
    rdfs:isDefinedBy <http://vocab.getty.edu/ontology>,
        ulan: ;
    rdfs:range skos:Concept ;
    rdfs:subPropertyOf skos:related ;
    owl:inverseOf gvp:ulan2829_student_was ;
    skos:broader skos:related ;
    skos:example "Zdanek Rossman was a student at Bauhaus" ;
    skos:inScheme <http://vocab.getty.edu/ontology> ;
    skos:notation "2828" ;
    skos:prefLabel "ulan2828_student_at"@en ;
    skos:topConceptOf <http://vocab.getty.edu/ontology> .

gvp:ulan2840_performer_with a owl:ObjectProperty,
        skos:Concept ;
    dc:identifier "2840" ;
    dc:title "performer with - group" ;
    dct:description "person - performer with - group" ;
    rdfs:domain skos:Concept ;
    rdfs:isDefinedBy <http://vocab.getty.edu/ontology>,
        ulan: ;
    rdfs:range skos:Concept ;
    rdfs:subPropertyOf skos:related ;
    owl:inverseOf gvp:ulan2841_performer_was ;
    skos:broader skos:related ;
    skos:inScheme <http://vocab.getty.edu/ontology> ;
    skos:notation "2840" ;
    skos:prefLabel "ulan2840_performer_with"@en ;
    skos:topConceptOf <http://vocab.getty.edu/ontology> .

gvp:aat2000_related_to a owl:ObjectProperty,
        owl:SymmetricProperty,
        skos:Concept ;
    dc:identifier "2000" ;
    dc:title "related to - any" ;
    dct:description """any - related to - any; generic relationship, not explained.\r
Example: gulf red is related to light red (pigment)""" ;
    rdfs:domain skos:Concept ;
    rdfs:isDefinedBy aat:,
        <http://vocab.getty.edu/ontology> ;
    rdfs:range skos:Concept ;
    rdfs:subPropertyOf skos:related ;
    skos:broader skos:related ;
    skos:example "gulf red is related to light red (pigment)" ;
    skos:inScheme aat:,
        <http://vocab.getty.edu/ontology> ;
    skos:notation "2000" ;
    skos:prefLabel "aat2000_related_to"@en ;
    skos:scopeNote "generic relationship, not explained" ;
    skos:topConceptOf aat:,
        <http://vocab.getty.edu/ontology> .

gvp:aat2110_meaning-usage_overlaps_with a owl:ObjectProperty,
        owl:SymmetricProperty,
        skos:Concept ;
    dc:identifier "2110" ;
    dc:title "meaning/usage overlaps with - any" ;
    dct:description """any - meaning/usage overlaps with - any.\r
Example: chimney hoods has meaning/usage that overlaps with chimney caps; scribes has meaning/usage that overlaps with copyists""" ;
    rdfs:domain skos:Concept ;
    rdfs:isDefinedBy aat:,
        <http://vocab.getty.edu/ontology> ;
    rdfs:range skos:Concept ;
    rdfs:subPropertyOf skos:related ;
    skos:broader skos:related ;
    skos:example "chimney hoods has meaning/usage that overlaps with chimney caps",
        "scribes has meaning/usage that overlaps with copyists" ;
    skos:inScheme aat:,
        <http://vocab.getty.edu/ontology> ;
    skos:notation "2110" ;
    skos:prefLabel "aat2110_meaning-usage_overlaps_with"@en ;
    skos:topConceptOf aat:,
        <http://vocab.getty.edu/ontology> .

gvp:aat2203_associated_with a owl:ObjectProperty,
        owl:SymmetricProperty,
        skos:Concept ;
    dc:identifier "2203" ;
    dc:title "associated with - activity/event" ;
    dct:description """activity/event/[process/function] - [is] associated with - activity/event/[process/function].\r
Example: Easter is associated with Lent; cavalry exercises are associated with dressage""" ;
    rdfs:domain skos:Concept ;
    rdfs:isDefinedBy aat:,
        <http://vocab.getty.edu/ontology> ;
    rdfs:range skos:Concept ;
    rdfs:subPropertyOf skos:related ;
    skos:broader skos:related ;
    skos:example "Easter is associated with Lent",
        "cavalry exercises are associated with dressage" ;
    skos:inScheme aat:,
        <http://vocab.getty.edu/ontology> ;
    skos:notation "2203" ;
    skos:prefLabel "aat2203_associated_with"@en ;
    skos:topConceptOf aat:,
        <http://vocab.getty.edu/ontology> .

gvp:aat2206_caused_by-requires a owl:ObjectProperty,
        skos:Concept ;
    dc:identifier "2206" ;
    dc:title "caused by/requires - activity/event" ;
    dct:description """activity/event/[process/function] - [is] caused by/dependent upon - activity/event/[process/function].\r
Example: on-demand publishing is caused by/requires on-demand printing; preservation is caused by/requires preserving""" ;
    rdfs:domain skos:Concept ;
    rdfs:isDefinedBy aat:,
        <http://vocab.getty.edu/ontology> ;
    rdfs:range skos:Concept ;
    rdfs:subPropertyOf skos:related ;
    skos:broader skos:related ;
    skos:example "on-demand publishing is caused by/requires on-demand printing",
        "preservation is caused by/requires preserving" ;
    skos:inScheme <http://vocab.getty.edu/ontology> ;
    skos:notation "2206" ;
    skos:prefLabel "aat2206_caused_by-requires"@en ;
    skos:topConceptOf <http://vocab.getty.edu/ontology> .

gvp:aat2215_required_for a owl:ObjectProperty,
        skos:Concept ;
    dc:identifier "2215" ;
    dc:title "required for - things" ;
    dct:description """things - [are] required for -  things.\r
Example: eyelets are required for broderie anglaise; compact discs are required for compact disc players""" ;
    rdfs:domain skos:Concept ;
    rdfs:isDefinedBy aat:,
        <http://vocab.getty.edu/ontology> ;
    rdfs:range skos:Concept ;
    rdfs:subPropertyOf skos:related ;
    owl:inverseOf gvp:aat2216_require ;
    skos:broader skos:related ;
    skos:example "compact discs are required for compact disc players",
        "eyelets are required for broderie anglaise" ;
    skos:inScheme aat:,
        <http://vocab.getty.edu/ontology> ;
    skos:notation "2215" ;
    skos:prefLabel "aat2215_required_for"@en ;
    skos:topConceptOf aat:,
        <http://vocab.getty.edu/ontology> .

gvp:aat2218_used-function_as a owl:ObjectProperty,
        skos:Concept ;
    dc:identifier "2218" ;
    dc:title "used/function as - things" ;
    dct:description """things - [are] used/function as - things.\r
Example: arc lamps are used/function as lighthouse lamps;  toile peinte is used/function as cartoons (working drawings)""" ;
    rdfs:domain skos:Concept ;
    rdfs:isDefinedBy aat:,
        <http://vocab.getty.edu/ontology> ;
    rdfs:range skos:Concept ;
    rdfs:subPropertyOf skos:related ;
    owl:inverseOf gvp:aat2219_have_form ;
    skos:broader skos:related ;
    skos:example "arc lamps are used/function as lighthouse lamps",
        "toile peinte is used/function as cartoons (working drawings)" ;
    skos:inScheme aat:,
        <http://vocab.getty.edu/ontology> ;
    skos:notation "2218" ;
    skos:prefLabel "aat2218_used-function_as"@en ;
    skos:topConceptOf aat:,
        <http://vocab.getty.edu/ontology> .

gvp:aat2219_have_form a owl:ObjectProperty,
        skos:Concept ;
    dc:identifier "2219" ;
    dc:title "have form - things" ;
    dct:description """things - have form [of] - things.\r
Example: lighthouse lamps have the form of arc lamps; cartoons (working drawings) have the form of toile peinte""" ;
    rdfs:domain skos:Concept ;
    rdfs:isDefinedBy aat:,
        <http://vocab.getty.edu/ontology> ;
    rdfs:range skos:Concept ;
    rdfs:subPropertyOf skos:related ;
    skos:broader skos:related ;
    skos:example "cartoons (working drawings) have the form of toile peinte",
        "lighthouse lamps have the form of arc lamps" ;
    skos:inScheme <http://vocab.getty.edu/ontology> ;
    skos:notation "2219" ;
    skos:prefLabel "aat2219_have_form"@en ;
    skos:topConceptOf <http://vocab.getty.edu/ontology> .

gvp:aat2222_are_acted_upon a owl:ObjectProperty,
        skos:Concept ;
    dc:identifier "2222" ;
    dc:title "are acted upon - role" ;
    dct:description """genus/species - is acted upon [by] - [actors having] role.\r
Example: Equus caballus(species) is acted upon by jockeys; Acer saccharum(species) is acted upon by tappers""" ;
    rdfs:domain skos:Concept ;
    rdfs:isDefinedBy aat:,
        <http://vocab.getty.edu/ontology> ;
    rdfs:range skos:Concept ;
    rdfs:subPropertyOf skos:related ;
    skos:broader skos:related ;
    skos:example "Acer saccharum(species) is acted upon by tappers",
        "Equus caballus(species) is acted upon by jockeys" ;
    skos:inScheme <http://vocab.getty.edu/ontology> ;
    skos:notation "2222" ;
    skos:prefLabel "aat2222_are_acted_upon"@en ;
    skos:topConceptOf <http://vocab.getty.edu/ontology> .

gvp:aat2291_locus-setting_for a owl:ObjectProperty,
        skos:Concept ;
    dc:identifier "2291" ;
    dc:title "locus/setting for - role" ;
    dct:description """locus/setting - [is] locus setting for - [actor or institution having] role.\r
Example: roperies are the locus/setting of rope-makers; convents (built complexes) are the locus/setting of nuns; libraries (buildings) are the locus/setting of libraries (institutions)""" ;
    rdfs:domain skos:Concept ;
    rdfs:isDefinedBy aat:,
        <http://vocab.getty.edu/ontology> ;
    rdfs:range skos:Concept ;
    rdfs:subPropertyOf skos:related ;
    owl:inverseOf gvp:aat2292_work-live_in ;
    skos:broader skos:related ;
    skos:example "convents (built complexes) are the locus/setting of nuns",
        "libraries (buildings) are the locus/setting of libraries (institutions)",
        "roperies are the locus/setting of rope-makers" ;
    skos:inScheme aat:,
        <http://vocab.getty.edu/ontology> ;
    skos:notation "2291" ;
    skos:prefLabel "aat2291_locus-setting_for"@en ;
    skos:topConceptOf aat:,
        <http://vocab.getty.edu/ontology> .

gvp:aat2292_work-live_in a owl:ObjectProperty,
        skos:Concept ;
    dc:identifier "2292" ;
    dc:title "work/live in - locus/setting" ;
    dct:description """[actor or institution having] role - work/live/[exist] in - locus/setting.\r
Example: rope-makers live/work in roperies; nuns live/work in convents (nunneries); libraries (institutions) live/work in libraries (buildings)""" ;
    rdfs:domain skos:Concept ;
    rdfs:isDefinedBy aat:,
        <http://vocab.getty.edu/ontology> ;
    rdfs:range skos:Concept ;
    rdfs:subPropertyOf skos:related ;
    skos:broader skos:related ;
    skos:example "libraries (institutions) live/work in libraries (buildings)",
        "nuns live/work in convents (nunneries)",
        "rope-makers live/work in roperies" ;
    skos:inScheme <http://vocab.getty.edu/ontology> ;
    skos:notation "2292" ;
    skos:prefLabel "aat2292_work-live_in"@en ;
    skos:topConceptOf <http://vocab.getty.edu/ontology> .

gvp:aat2295_located_in a owl:ObjectProperty,
        skos:Concept ;
    dc:identifier "2295" ;
    dc:title "located in - locus/setting" ;
    dct:description """locus/setting - [is] located in - locus/setting.\r
Example: national capitals are located in nations; mountains are located in mountain ranges""" ;
    rdfs:domain skos:Concept ;
    rdfs:isDefinedBy aat:,
        <http://vocab.getty.edu/ontology> ;
    rdfs:range skos:Concept ;
    rdfs:subPropertyOf skos:related ;
    skos:broader skos:related ;
    skos:example "mountains are located in mountain ranges",
        "national capitals are located in nations" ;
    skos:inScheme <http://vocab.getty.edu/ontology> ;
    skos:notation "2295" ;
    skos:prefLabel "aat2295_located_in"@en ;
    skos:topConceptOf <http://vocab.getty.edu/ontology> .

gvp:aat2312_perform a owl:ObjectProperty,
        skos:Concept ;
    dc:identifier "2312" ;
    dc:title "perform - activity/event" ;
    dct:description """[actors having] a role - perform - activity/event/process.\r
Example: clockmakers perform clockmaking; curators perform curating""" ;
    rdfs:domain skos:Concept ;
    rdfs:isDefinedBy aat:,
        <http://vocab.getty.edu/ontology> ;
    rdfs:range skos:Concept ;
    rdfs:subPropertyOf skos:related ;
    skos:broader skos:related ;
    skos:example "clockmakers perform clockmaking",
        "curators perform curating" ;
    skos:inScheme <http://vocab.getty.edu/ontology> ;
    skos:notation "2312" ;
    skos:prefLabel "aat2312_perform"@en ;
    skos:topConceptOf <http://vocab.getty.edu/ontology> .

gvp:aat2315_used_by a owl:ObjectProperty,
        skos:Concept ;
    dc:identifier "2315" ;
    dc:title "used by - role" ;
    dct:description """material - [is] used by - [actor having] role.\r
Example: precious stone is used by lapidiaries; brass (alloy) is used by braziers (metalworkers)""" ;
    rdfs:domain skos:Concept ;
    rdfs:isDefinedBy aat:,
        <http://vocab.getty.edu/ontology> ;
    rdfs:range skos:Concept ;
    rdfs:subPropertyOf skos:related ;
    owl:inverseOf gvp:aat2316_use ;
    skos:broader skos:related ;
    skos:example "brass (alloy) is used by braziers (metalworkers)",
        "precious stone is used by lapidiaries" ;
    skos:inScheme aat:,
        <http://vocab.getty.edu/ontology> ;
    skos:notation "2315" ;
    skos:prefLabel "aat2315_used_by"@en ;
    skos:topConceptOf aat:,
        <http://vocab.getty.edu/ontology> .

gvp:aat2319_involves a owl:ObjectProperty,
        skos:Concept ;
    dc:identifier "2319" ;
    dc:title "involves - role" ;
    dct:description """activity/event - involves - [actors having] role.\r
Example: weddings involve bridegrooms; martyrdoms involve martyrs""" ;
    rdfs:domain skos:Concept ;
    rdfs:isDefinedBy aat:,
        <http://vocab.getty.edu/ontology> ;
    rdfs:range skos:Concept ;
    rdfs:subPropertyOf skos:related ;
    skos:broader skos:related ;
    skos:example "martyrdoms involve martyrs",
        "weddings involve bridegrooms" ;
    skos:inScheme <http://vocab.getty.edu/ontology> ;
    skos:notation "2319" ;
    skos:prefLabel "aat2319_involves"@en ;
    skos:topConceptOf <http://vocab.getty.edu/ontology> .

gvp:aat2322_use a owl:ObjectProperty,
        skos:Concept ;
    dc:identifier "2322" ;
    dc:title "use - things" ;
    dct:description """[actors having] role - use - things/equipment.\r
Example: violoncellists use violoncellos; surveyors use surveying instruments""" ;
    rdfs:domain skos:Concept ;
    rdfs:isDefinedBy aat:,
        <http://vocab.getty.edu/ontology> ;
    rdfs:range skos:Concept ;
    rdfs:subPropertyOf skos:related ;
    skos:broader skos:related ;
    skos:example "surveyors use surveying instruments",
        "violoncellists use violoncellos" ;
    skos:inScheme <http://vocab.getty.edu/ontology> ;
    skos:notation "2322" ;
    skos:prefLabel "aat2322_use"@en ;
    skos:topConceptOf <http://vocab.getty.edu/ontology> .

gvp:aat2325_created_by a owl:ObjectProperty,
        skos:Concept ;
    dc:identifier "2325" ;
    dc:title "created by - role" ;
    dct:description """things - [are] created by - [actors having] role.\r
Example: drawings are created by draftsmen; poems are created by poets""" ;
    rdfs:domain skos:Concept ;
    rdfs:isDefinedBy aat:,
        <http://vocab.getty.edu/ontology> ;
    rdfs:range skos:Concept ;
    rdfs:subPropertyOf skos:related ;
    owl:inverseOf gvp:aat2326_create ;
    skos:broader skos:related ;
    skos:example "drawings are created by draftsmen",
        "poems are created by poets" ;
    skos:inScheme aat:,
        <http://vocab.getty.edu/ontology> ;
    skos:notation "2325" ;
    skos:prefLabel "aat2325_created_by"@en ;
    skos:topConceptOf aat:,
        <http://vocab.getty.edu/ontology> .

gvp:aat2326_create a owl:ObjectProperty,
        skos:Concept ;
    dc:identifier "2326" ;
    dc:title "create - things" ;
    dct:description """[actors having] role - create - things.\r
Example: draftsmen create drawings; poets create poems""" ;
    rdfs:domain skos:Concept ;
    rdfs:isDefinedBy aat:,
        <http://vocab.getty.edu/ontology> ;
    rdfs:range skos:Concept ;
    rdfs:subPropertyOf skos:related ;
    skos:broader skos:related ;
    skos:example "draftsmen create drawings",
        "poets create poems" ;
    skos:inScheme <http://vocab.getty.edu/ontology> ;
    skos:notation "2326" ;
    skos:prefLabel "aat2326_create"@en ;
    skos:topConceptOf <http://vocab.getty.edu/ontology> .

gvp:aat2328_involved_with a owl:ObjectProperty,
        skos:Concept ;
    dc:identifier "2328" ;
    dc:title "involved with - things" ;
    dct:description """[actors having] role - [are] involved in- things.\r
Example: sitters are involved with portraits; actors (performing artists) are involved with motion pictures (visual works)""" ;
    rdfs:domain skos:Concept ;
    rdfs:isDefinedBy aat:,
        <http://vocab.getty.edu/ontology> ;
    rdfs:range skos:Concept ;
    rdfs:subPropertyOf skos:related ;
    owl:inverseOf gvp:aat2329_involves ;
    skos:broader skos:related ;
    skos:example "actors (performing artists) are involved with motion pictures (visual works)",
        "sitters are involved with portraits" ;
    skos:inScheme aat:,
        <http://vocab.getty.edu/ontology> ;
    skos:notation "2328" ;
    skos:prefLabel "aat2328_involved_with"@en ;
    skos:topConceptOf aat:,
        <http://vocab.getty.edu/ontology> .

gvp:aat2329_involves a owl:ObjectProperty,
        skos:Concept ;
    dc:identifier "2329" ;
    dc:title "involves - role" ;
    dct:description """things - involve - [actors having] role.\r
Example: portraits involve sitters; motion pictures (visual works) involve actors (performing artists)""" ;
    rdfs:domain skos:Concept ;
    rdfs:isDefinedBy aat:,
        <http://vocab.getty.edu/ontology> ;
    rdfs:range skos:Concept ;
    rdfs:subPropertyOf skos:related ;
    skos:broader skos:related ;
    skos:example "motion pictures (visual works) involve actors (performing artists)",
        "portraits involve sitters" ;
    skos:inScheme <http://vocab.getty.edu/ontology> ;
    skos:notation "2329" ;
    skos:prefLabel "aat2329_involves"@en ;
    skos:topConceptOf <http://vocab.getty.edu/ontology> .

gvp:aat2336_has_associates a owl:ObjectProperty,
        skos:Concept ;
    dc:identifier "2336" ;
    dc:title "has associates - role" ;
    dct:description """style/period/culture/[relgion] - has associates - [actors having] role.\r
Example: Abstract (fine arts style) has associates abstract artists; Roman Catholicism has associates popes""" ;
    rdfs:domain skos:Concept ;
    rdfs:isDefinedBy aat:,
        <http://vocab.getty.edu/ontology> ;
    rdfs:range skos:Concept ;
    rdfs:subPropertyOf skos:related ;
    skos:broader skos:related ;
    skos:example "Abstract (fine arts style) has associates abstract artists",
        "Roman Catholicism has associates popes" ;
    skos:inScheme <http://vocab.getty.edu/ontology> ;
    skos:notation "2336" ;
    skos:prefLabel "aat2336_has_associates"@en ;
    skos:topConceptOf <http://vocab.getty.edu/ontology> .

gvp:aat2398_focuses_on a owl:ObjectProperty,
        skos:Concept ;
    dc:identifier "2398" ;
    dc:title "focuses on - any" ;
    dct:description """field [of study]/discipline - focuses on - any.\r
Example: codicology focuses on manuscripts; musicology focuses on music; bontany focuses on Plantae (kingdom)""" ;
    rdfs:domain skos:Concept ;
    rdfs:isDefinedBy aat:,
        <http://vocab.getty.edu/ontology> ;
    rdfs:range skos:Concept ;
    rdfs:subPropertyOf skos:related ;
    skos:broader skos:related ;
    skos:example "bontany focuses on Plantae (kingdom)",
        "codicology focuses on manuscripts",
        "musicology focuses on music" ;
    skos:inScheme <http://vocab.getty.edu/ontology> ;
    skos:notation "2398" ;
    skos:prefLabel "aat2398_focuses_on"@en ;
    skos:topConceptOf <http://vocab.getty.edu/ontology> .

gvp:aat2408_locus-setting_for a owl:ObjectProperty,
        skos:Concept ;
    dc:identifier "2408" ;
    dc:title "locus/setting for - field/discipline" ;
    dct:description """locus/setting - [is] locus/setting for - field of study/discipline.\r
Example: schools (buildings) are the locus/setting for education; hospitals (buildings) are the locus/setting for medicine (discipline)""" ;
    rdfs:domain skos:Concept ;
    rdfs:isDefinedBy aat:,
        <http://vocab.getty.edu/ontology> ;
    rdfs:range skos:Concept ;
    rdfs:subPropertyOf skos:related ;
    owl:inverseOf gvp:aat2409_takes_place_in ;
    skos:broader skos:related ;
    skos:example "hospitals (buildings) are the locus/setting for medicine (discipline)",
        "schools (buildings) are the locus/setting for education" ;
    skos:inScheme aat:,
        <http://vocab.getty.edu/ontology> ;
    skos:notation "2408" ;
    skos:prefLabel "aat2408_locus-setting_for"@en ;
    skos:topConceptOf aat:,
        <http://vocab.getty.edu/ontology> .

gvp:aat2409_takes_place_in a owl:ObjectProperty,
        skos:Concept ;
    dc:identifier "2409" ;
    dc:title "takes place in - locus/setting" ;
    dct:description """field of study/discipline - takes place in - locus/setting.\r
Example: education takes place in schools (buildings); medicine (discipline) takes place in hospitals (buildings)""" ;
    rdfs:domain skos:Concept ;
    rdfs:isDefinedBy aat:,
        <http://vocab.getty.edu/ontology> ;
    rdfs:range skos:Concept ;
    rdfs:subPropertyOf skos:related ;
    skos:broader skos:related ;
    skos:example "education takes place in schools (buildings)",
        "medicine (discipline) takes place in hospitals (buildings)" ;
    skos:inScheme <http://vocab.getty.edu/ontology> ;
    skos:notation "2409" ;
    skos:prefLabel "aat2409_takes_place_in"@en ;
    skos:topConceptOf <http://vocab.getty.edu/ontology> .

gvp:aat2411_involved_in a owl:ObjectProperty,
        skos:Concept ;
    dc:identifier "2411" ;
    dc:title "involved in - field/discipline" ;
    dct:description """activity/event/[process/function] - [is] involved in - field/discipline.\r
Example: journalistic photography is involved in photojournalism (discipline); gardening is involved in horticulture""" ;
    rdfs:domain skos:Concept ;
    rdfs:isDefinedBy aat:,
        <http://vocab.getty.edu/ontology> ;
    rdfs:range skos:Concept ;
    rdfs:subPropertyOf skos:related ;
    owl:inverseOf gvp:aat2412_involves ;
    skos:broader skos:related ;
    skos:example "gardening is involved in horticulture",
        "journalistic photography is involved in photojournalism (discipline)" ;
    skos:inScheme aat:,
        <http://vocab.getty.edu/ontology> ;
    skos:notation "2411" ;
    skos:prefLabel "aat2411_involved_in"@en ;
    skos:topConceptOf aat:,
        <http://vocab.getty.edu/ontology> .

gvp:aat2412_involves a owl:ObjectProperty,
        skos:Concept ;
    dc:identifier "2412" ;
    dc:title "involves - activity/event" ;
    dct:description """field/discipline - involves - activity/event/[process/function].\r
Example: photojournalism (discipline) involves journalistic photography; horticulture involves gardening""" ;
    rdfs:domain skos:Concept ;
    rdfs:isDefinedBy aat:,
        <http://vocab.getty.edu/ontology> ;
    rdfs:range skos:Concept ;
    rdfs:subPropertyOf skos:related ;
    skos:broader skos:related ;
    skos:example "horticulture involves gardening",
        "photojournalism (discipline) involves journalistic photography" ;
    skos:inScheme <http://vocab.getty.edu/ontology> ;
    skos:notation "2412" ;
    skos:prefLabel "aat2412_involves"@en ;
    skos:topConceptOf <http://vocab.getty.edu/ontology> .

gvp:aat2416_requires a owl:ObjectProperty,
        skos:Concept ;
    dc:identifier "2416" ;
    dc:title "requires - material" ;
    dct:description """activity/event/[process/function] - requires - material.\r
Example: dying requires dye; pewtersmithing requires pewter""" ;
    rdfs:domain skos:Concept ;
    rdfs:isDefinedBy aat:,
        <http://vocab.getty.edu/ontology> ;
    rdfs:range skos:Concept ;
    rdfs:subPropertyOf skos:related ;
    skos:broader skos:related ;
    skos:example "dying requires dye",
        "pewtersmithing requires pewter" ;
    skos:inScheme <http://vocab.getty.edu/ontology> ;
    skos:notation "2416" ;
    skos:prefLabel "aat2416_requires"@en ;
    skos:topConceptOf <http://vocab.getty.edu/ontology> .

gvp:aat2418_uses a owl:ObjectProperty,
        skos:Concept ;
    dc:identifier "2418" ;
    dc:title "uses - things" ;
    dct:description """field [of study]/discipline - uses - things/[equipment].\r
Example: astronomy uses astronomical instruments; divination [discipline] uses divination objects""" ;
    rdfs:domain skos:Concept ;
    rdfs:isDefinedBy aat:,
        <http://vocab.getty.edu/ontology> ;
    rdfs:range skos:Concept ;
    rdfs:subPropertyOf skos:related ;
    owl:inverseOf gvp:aat2419_used_for ;
    skos:broader skos:related ;
    skos:example "astronomy uses astronomical instruments",
        "divination [discipline] uses divination objects" ;
    skos:inScheme aat:,
        <http://vocab.getty.edu/ontology> ;
    skos:notation "2418" ;
    skos:prefLabel "aat2418_uses"@en ;
    skos:topConceptOf aat:,
        <http://vocab.getty.edu/ontology> .

gvp:aat2421_locus-setting_for a owl:ObjectProperty,
        skos:Concept ;
    dc:identifier "2421" ;
    dc:title "locus/setting for - activity/event" ;
    dct:description """locus/setting - [is] locus/setting for - activity/event/[process/function].\r
Example: smelters (metalworking plants) are the locus/setting for smelting; pilgrimage centers are the locus/setting for pilgrimages""" ;
    rdfs:domain skos:Concept ;
    rdfs:isDefinedBy aat:,
        <http://vocab.getty.edu/ontology> ;
    rdfs:range skos:Concept ;
    rdfs:subPropertyOf skos:related ;
    owl:inverseOf gvp:aat2422_takes_place_in ;
    skos:broader skos:related ;
    skos:example "pilgrimage centers are the locus/setting for pilgrimages",
        "smelters (metalworking plants) are the locus/setting for smelting" ;
    skos:inScheme aat:,
        <http://vocab.getty.edu/ontology> ;
    skos:notation "2421" ;
    skos:prefLabel "aat2421_locus-setting_for"@en ;
    skos:topConceptOf aat:,
        <http://vocab.getty.edu/ontology> .

gvp:aat2424_produced_by a owl:ObjectProperty,
        skos:Concept ;
    dc:identifier "2424" ;
    dc:title "produced by - activity/event/process" ;
    dct:description """material - [is] produced by - activity/event/process.\r
Example: wire is produced by wiredrawing; paper is produced by papermaking""" ;
    rdfs:domain skos:Concept ;
    rdfs:isDefinedBy aat:,
        <http://vocab.getty.edu/ontology> ;
    rdfs:range skos:Concept ;
    rdfs:subPropertyOf skos:related ;
    owl:inverseOf gvp:aat2425_produces ;
    skos:broader skos:related ;
    skos:example "paper is produced by papermaking",
        "wire is produced by wiredrawing" ;
    skos:inScheme aat:,
        <http://vocab.getty.edu/ontology> ;
    skos:notation "2424" ;
    skos:prefLabel "aat2424_produced_by"@en ;
    skos:topConceptOf aat:,
        <http://vocab.getty.edu/ontology> .

gvp:aat2425_produces a owl:ObjectProperty,
        skos:Concept ;
    dc:identifier "2425" ;
    dc:title "produces - material" ;
    dct:description """activity/event/process - produces - material.\r
Example: wiredrawing produces wire; papermaking produces paper""" ;
    rdfs:domain skos:Concept ;
    rdfs:isDefinedBy aat:,
        <http://vocab.getty.edu/ontology> ;
    rdfs:range skos:Concept ;
    rdfs:subPropertyOf skos:related ;
    skos:broader skos:related ;
    skos:example "papermaking produces paper",
        "wiredrawing produces wire" ;
    skos:inScheme <http://vocab.getty.edu/ontology> ;
    skos:notation "2425" ;
    skos:prefLabel "aat2425_produces"@en ;
    skos:topConceptOf <http://vocab.getty.edu/ontology> .

gvp:aat2431_required_for a owl:ObjectProperty,
        skos:Concept ;
    dc:identifier "2431" ;
    dc:title "required for - activity/event/process" ;
    dct:description """things/equipment - [are] required for - activity/event/process.\r
Example: painting equipment is required for painting (image making); dowels are required for doweling""" ;
    rdfs:domain skos:Concept ;
    rdfs:isDefinedBy aat:,
        <http://vocab.getty.edu/ontology> ;
    rdfs:range skos:Concept ;
    rdfs:subPropertyOf skos:related ;
    owl:inverseOf gvp:aat2432_requires ;
    skos:broader skos:related ;
    skos:example "dowels are required for doweling",
        "painting equipment is required for painting (image making)" ;
    skos:inScheme aat:,
        <http://vocab.getty.edu/ontology> ;
    skos:notation "2431" ;
    skos:prefLabel "aat2431_required_for"@en ;
    skos:topConceptOf aat:,
        <http://vocab.getty.edu/ontology> .

gvp:aat2435_context_for a owl:ObjectProperty,
        skos:Concept ;
    dc:identifier "2435" ;
    dc:title "context for - things" ;
    dct:description """activity/event/process - [is] contextualized in - thing.\r
Example: funerals are the context for funeral books; Christmas is the context for Christmas trees""" ;
    rdfs:domain skos:Concept ;
    rdfs:isDefinedBy aat:,
        <http://vocab.getty.edu/ontology> ;
    rdfs:range skos:Concept ;
    rdfs:subPropertyOf skos:related ;
    skos:broader skos:related ;
    skos:example "Christmas is the context for Christmas trees",
        "funerals are the context for funeral books" ;
    skos:inScheme <http://vocab.getty.edu/ontology> ;
    skos:notation "2435" ;
    skos:prefLabel "aat2435_context_for"@en ;
    skos:topConceptOf <http://vocab.getty.edu/ontology> .

gvp:aat2501_made_of-require a owl:ObjectProperty,
        skos:Concept ;
    dc:identifier "2501" ;
    dc:title "made of/require - material" ;
    dct:description """things - [are] made of/require - material.\r
Example: obsidian mirrors are made of/require obsidian; ivories (sculptures) are made of/require ivory""" ;
    rdfs:domain skos:Concept ;
    rdfs:isDefinedBy aat:,
        <http://vocab.getty.edu/ontology> ;
    rdfs:range skos:Concept ;
    rdfs:subPropertyOf skos:related ;
    owl:inverseOf gvp:aat2502_material_for ;
    skos:broader skos:related ;
    skos:example "ivories (sculptures) are made of/require ivory",
        "obsidian mirrors are made of/require obsidian" ;
    skos:inScheme aat:,
        <http://vocab.getty.edu/ontology> ;
    skos:notation "2501" ;
    skos:prefLabel "aat2501_made_of-require"@en ;
    skos:topConceptOf aat:,
        <http://vocab.getty.edu/ontology> .

gvp:aat2502_material_for a owl:ObjectProperty,
        skos:Concept ;
    dc:identifier "2502" ;
    dc:title "material for - things" ;
    dct:description """material - [is] material for - things.\r
Example: obsidian is material for obsidian mirrors; ivory is material for ivories (sculptures)""" ;
    rdfs:domain skos:Concept ;
    rdfs:isDefinedBy aat:,
        <http://vocab.getty.edu/ontology> ;
    rdfs:range skos:Concept ;
    rdfs:subPropertyOf skos:related ;
    skos:broader skos:related ;
    skos:example "ivory is material for ivories (sculptures)",
        "obsidian is material for obsidian mirrors" ;
    skos:inScheme <http://vocab.getty.edu/ontology> ;
    skos:notation "2502" ;
    skos:prefLabel "aat2502_material_for"@en ;
    skos:topConceptOf <http://vocab.getty.edu/ontology> .

gvp:aat2505_locus-setting_for a owl:ObjectProperty,
        skos:Concept ;
    dc:identifier "2505" ;
    dc:title "locus/setting for - material" ;
    dct:description """locus/setting - [is] locus/setting for - material.\r
Example: volcanoes are locus/setting for  tephra; brickworks (factories) are locus/setting for brick (clay product)""" ;
    rdfs:domain skos:Concept ;
    rdfs:isDefinedBy aat:,
        <http://vocab.getty.edu/ontology> ;
    rdfs:range skos:Concept ;
    rdfs:subPropertyOf skos:related ;
    skos:broader skos:related ;
    skos:example "brickworks (factories) are locus/setting for brick (clay product)",
        "volcanoes are locus/setting for  tephra" ;
    skos:inScheme <http://vocab.getty.edu/ontology> ;
    skos:notation "2505" ;
    skos:prefLabel "aat2505_locus-setting_for"@en ;
    skos:topConceptOf <http://vocab.getty.edu/ontology> .

gvp:aat2508_produced-processed_by a owl:ObjectProperty,
        skos:Concept ;
    dc:identifier "2508" ;
    dc:title "produced/processed by - things" ;
    dct:description """material - [is] produced/processed by - things/[equipment].\r
Example: cotton gins produce/process cotton (fiber); waterwells produce/process groundwater""" ;
    rdfs:domain skos:Concept ;
    rdfs:isDefinedBy aat:,
        <http://vocab.getty.edu/ontology> ;
    rdfs:range skos:Concept ;
    rdfs:subPropertyOf skos:related ;
    skos:broader skos:related ;
    skos:example "cotton gins produce/process cotton (fiber)",
        "waterwells produce/process groundwater" ;
    skos:inScheme <http://vocab.getty.edu/ontology> ;
    skos:notation "2508" ;
    skos:prefLabel "aat2508_produced-processed_by"@en ;
    skos:topConceptOf <http://vocab.getty.edu/ontology> .

gvp:aat2551_reflect-produced_by a owl:ObjectProperty,
        skos:Concept ;
    dc:identifier "2551" ;
    dc:title "reflect/produced by - style/period/culture" ;
    dct:description """things - reflect/[are] produced by - style/period/culture/[religion/ideology].\r
Example: Nasca lines reflect/are produced by Nasca [culture]; Judaica reflects/is produced by Judaism""" ;
    rdfs:domain skos:Concept ;
    rdfs:isDefinedBy aat:,
        <http://vocab.getty.edu/ontology> ;
    rdfs:range skos:Concept ;
    rdfs:subPropertyOf skos:related ;
    owl:inverseOf gvp:aat2552_reflected_in-produces ;
    skos:broader skos:related ;
    skos:example "Judaica reflects/is produced by Judaism",
        "Nasca lines reflect/are produced by Nasca [culture]" ;
    skos:inScheme aat:,
        <http://vocab.getty.edu/ontology> ;
    skos:notation "2551" ;
    skos:prefLabel "aat2551_reflect-produced_by"@en ;
    skos:topConceptOf aat:,
        <http://vocab.getty.edu/ontology> .

gvp:aat2552_reflected_in-produces a owl:ObjectProperty,
        skos:Concept ;
    dc:identifier "2552" ;
    dc:title "reflected in/produces - things" ;
    dct:description """style/period/culture/[religion/ideology] - [is] reflected in/produces - things.\r
Example: Nasca [culture] produces/is reflected in Nasca lines; Judaism produces/is reflected in Judaica""" ;
    rdfs:domain skos:Concept ;
    rdfs:isDefinedBy aat:,
        <http://vocab.getty.edu/ontology> ;
    rdfs:range skos:Concept ;
    rdfs:subPropertyOf skos:related ;
    skos:broader skos:related ;
    skos:example "Judaism produces/is reflected in Judaica",
        "Nasca [culture] produces/is reflected in Nasca lines" ;
    skos:inScheme <http://vocab.getty.edu/ontology> ;
    skos:notation "2552" ;
    skos:prefLabel "aat2552_reflected_in-produces"@en ;
    skos:topConceptOf <http://vocab.getty.edu/ontology> .

gvp:aat2554_reflects a owl:ObjectProperty,
        skos:Concept ;
    dc:identifier "2554" ;
    dc:title "reflects - style/period/culture" ;
    dct:description """activity/event - reflects - style/period/culture /[religion/ideology].\r
Example: dhokra (casting technique) reflects Dhokra (culture); red-figure vase painting reflects Red-figure [style]""" ;
    rdfs:domain skos:Concept ;
    rdfs:isDefinedBy aat:,
        <http://vocab.getty.edu/ontology> ;
    rdfs:range skos:Concept ;
    rdfs:subPropertyOf skos:related ;
    owl:inverseOf gvp:aat2555_reflected_in ;
    skos:broader skos:related ;
    skos:example "dhokra (casting technique) reflects Dhokra (culture)",
        "red-figure vase painting reflects Red-figure [style]" ;
    skos:inScheme aat:,
        <http://vocab.getty.edu/ontology> ;
    skos:notation "2554" ;
    skos:prefLabel "aat2554_reflects"@en ;
    skos:topConceptOf aat:,
        <http://vocab.getty.edu/ontology> .

gvp:aat2557_reflects a owl:ObjectProperty,
        skos:Concept ;
    dc:identifier "2557" ;
    dc:title "reflects - style/period/culture" ;
    dct:description """field/discipline - reflects - style/period/culture /[religion/ideology].\r
Example: bugatu [dance discipline] reflects Buddhism; church history reflects Christianity; classics (discipline) reflects Ancient Greek [culture]""" ;
    rdfs:domain skos:Concept ;
    rdfs:isDefinedBy aat:,
        <http://vocab.getty.edu/ontology> ;
    rdfs:range skos:Concept ;
    rdfs:subPropertyOf skos:related ;
    owl:inverseOf gvp:aat2558_reflected_in ;
    skos:broader skos:related ;
    skos:example "bugatu [dance discipline] reflects Buddhism",
        "church history reflects Christianity",
        "classics (discipline) reflects Ancient Greek [culture]" ;
    skos:inScheme aat:,
        <http://vocab.getty.edu/ontology> ;
    skos:notation "2557" ;
    skos:prefLabel "aat2557_reflects"@en ;
    skos:topConceptOf aat:,
        <http://vocab.getty.edu/ontology> .

gvp:aat2563_located_in a owl:ObjectProperty,
        skos:Concept ;
    dc:identifier "2563" ;
    dc:title "located in - locus/setting" ;
    dct:description """style/period/culture/[religion/ideology] - is located/[reflected] in - locus/setting.\r
Example: First Nations (culture) is located/reflected in First Nations reserves; Brahmanism is located/reflected in agraharas""" ;
    rdfs:domain skos:Concept ;
    rdfs:isDefinedBy aat:,
        <http://vocab.getty.edu/ontology> ;
    rdfs:range skos:Concept ;
    rdfs:subPropertyOf skos:related ;
    skos:broader skos:related ;
    skos:example "Brahmanism is located/reflected in agraharas",
        "First Nations (culture) is located/reflected in First Nations reserves" ;
    skos:inScheme <http://vocab.getty.edu/ontology> ;
    skos:notation "2563" ;
    skos:prefLabel "aat2563_located_in"@en ;
    skos:topConceptOf <http://vocab.getty.edu/ontology> .

gvp:aat2604_possessed_by-existing_in a owl:ObjectProperty,
        skos:Concept ;
    dc:identifier "2604" ;
    dc:title "possessed by/existing in - things" ;
    dct:description """attributes /associated concepts - [is] possessed by/existing in - things.\r
Example: boudoir (photograph size) is possessed by/existing in boudoir photographs; ruined [condition] is possessed by/existing in ruins""" ;
    rdfs:domain skos:Concept ;
    rdfs:isDefinedBy aat:,
        <http://vocab.getty.edu/ontology> ;
    rdfs:range skos:Concept ;
    rdfs:subPropertyOf skos:related ;
    owl:inverseOf gvp:aat2605_possess-exist_in ;
    skos:broader skos:related ;
    skos:example "boudoir (photograph size) is possessed by/existing in boudoir photographs",
        "ruined [condition] is possessed by/existing in ruins" ;
    skos:inScheme aat:,
        <http://vocab.getty.edu/ontology> ;
    skos:notation "2604" ;
    skos:prefLabel "aat2604_possessed_by-existing_in"@en ;
    skos:topConceptOf aat:,
        <http://vocab.getty.edu/ontology> .

gvp:aat2605_possess-exist_in a owl:ObjectProperty,
        skos:Concept ;
    dc:identifier "2605" ;
    dc:title "possess/exist in - attributes /associated concepts" ;
    dct:description """things - possess/exist in - attributes /associated concepts.\r
Example: boudoir photographs possess/exist in boudoir (photograph size); ruins possess/exist in ruined [contition]""" ;
    rdfs:domain skos:Concept ;
    rdfs:isDefinedBy aat:,
        <http://vocab.getty.edu/ontology> ;
    rdfs:range skos:Concept ;
    rdfs:subPropertyOf skos:related ;
    skos:broader skos:related ;
    skos:example "boudoir photographs possess/exist in boudoir (photograph size)",
        "ruins possess/exist in ruined [contition]" ;
    skos:inScheme <http://vocab.getty.edu/ontology> ;
    skos:notation "2605" ;
    skos:prefLabel "aat2605_possess-exist_in"@en ;
    skos:topConceptOf <http://vocab.getty.edu/ontology> .

gvp:aat2608_causes-required_for a owl:ObjectProperty,
        skos:Concept ;
    dc:identifier "2608" ;
    dc:title "causes/required for - attributes /associated concepts" ;
    dct:description """activity/event/[process/function] - causes/[is] required for - [a] state/condition/attributes.\r
Example: waterproofing causes/is required for watertighness; creasing (process) causes/is required for creases (condition)""" ;
    rdfs:domain skos:Concept ;
    rdfs:isDefinedBy aat:,
        <http://vocab.getty.edu/ontology> ;
    rdfs:range skos:Concept ;
    rdfs:subPropertyOf skos:related ;
    skos:broader skos:related ;
    skos:example "creasing (process) causes/is required for creases (condition)",
        "waterproofing causes/is required for watertighness" ;
    skos:inScheme <http://vocab.getty.edu/ontology> ;
    skos:notation "2608" ;
    skos:prefLabel "aat2608_causes-required_for"@en ;
    skos:topConceptOf <http://vocab.getty.edu/ontology> .

gvp:aat2612_possessed_by-existing_in a owl:ObjectProperty,
        skos:Concept ;
    dc:identifier "2612" ;
    dc:title "possessed by/existing in - material" ;
    dct:description """attributes /associated concepts - is possessed by/existing in - material.\r
Example: dry rot is possessed by/existing in wood(plant material); dielectric properties are possessed by/existing in dielectric (material)""" ;
    rdfs:domain skos:Concept ;
    rdfs:isDefinedBy aat:,
        <http://vocab.getty.edu/ontology> ;
    rdfs:range skos:Concept ;
    rdfs:subPropertyOf skos:related ;
    owl:inverseOf gvp:aat2613_possess-exist_in ;
    skos:broader skos:related ;
    skos:example "dielectric properties are possessed by/existing in dielectric (material)",
        "dry rot is possessed by/existing in wood(plant material)" ;
    skos:inScheme aat:,
        <http://vocab.getty.edu/ontology> ;
    skos:notation "2612" ;
    skos:prefLabel "aat2612_possessed_by-existing_in"@en ;
    skos:topConceptOf aat:,
        <http://vocab.getty.edu/ontology> .

gvp:aat2802_exemplified_by a owl:ObjectProperty,
        skos:Concept ;
    dc:identifier "2802" ;
    dc:title "exemplified by - brand name" ;
    dct:description """material - [is] exemplified by - brand name.\r
Example: petrolium jelly is exemplified by Vaseline (TM); polytetrafluoroethyelene is exemplified by Teflon (TM)""" ;
    rdfs:domain skos:Concept ;
    rdfs:isDefinedBy aat:,
        <http://vocab.getty.edu/ontology> ;
    rdfs:range skos:Concept ;
    rdfs:subPropertyOf skos:related ;
    owl:inverseOf gvp:aat2803_example_of ;
    skos:broader skos:related ;
    skos:example "petrolium jelly is exemplified by Vaseline (TM)",
        "polytetrafluoroethyelene is exemplified by Teflon (TM)" ;
    skos:inScheme aat:,
        <http://vocab.getty.edu/ontology> ;
    skos:notation "2802" ;
    skos:prefLabel "aat2802_exemplified_by"@en ;
    skos:topConceptOf aat:,
        <http://vocab.getty.edu/ontology> .

gvp:aat2803_example_of a owl:ObjectProperty,
        skos:Concept ;
    dc:identifier "2803" ;
    dc:title "example of - material" ;
    dct:description """brand name - [is] example of - material.\r
Example: Vaseline (TM) is an example of petrolium jelly; Teflon (TM) is an example of polytetrafluoroethyelene""" ;
    rdfs:domain skos:Concept ;
    rdfs:isDefinedBy aat:,
        <http://vocab.getty.edu/ontology> ;
    rdfs:range skos:Concept ;
    rdfs:subPropertyOf skos:related ;
    skos:broader skos:related ;
    skos:example "Teflon (TM) is an example of polytetrafluoroethyelene",
        "Vaseline (TM) is an example of petrolium jelly" ;
    skos:inScheme <http://vocab.getty.edu/ontology> ;
    skos:notation "2803" ;
    skos:prefLabel "aat2803_example_of"@en ;
    skos:topConceptOf <http://vocab.getty.edu/ontology> .

gvp:aat2805_contextualized_in a owl:ObjectProperty,
        skos:Concept ;
    dc:identifier "2805" ;
    dc:title "contextualized in - things" ;
    dct:description """[smaller] things - [are] contextualized in - [larger] things.\r
Example: predellas are contextualized in altarpieces; chapters are contextualized in books""" ;
    rdfs:domain skos:Concept ;
    rdfs:isDefinedBy aat:,
        <http://vocab.getty.edu/ontology> ;
    rdfs:range skos:Concept ;
    rdfs:subPropertyOf skos:related ;
    owl:inverseOf gvp:aat2806_provide_context ;
    skos:broader skos:related ;
    skos:example "chapters are contextualized in books",
        "predellas are contextualized in altarpieces" ;
    skos:inScheme aat:,
        <http://vocab.getty.edu/ontology> ;
    skos:notation "2805" ;
    skos:prefLabel "aat2805_contextualized_in"@en ;
    skos:topConceptOf aat:,
        <http://vocab.getty.edu/ontology> .

gvp:aat2814_constituent_of a owl:ObjectProperty,
        skos:Concept ;
    dc:identifier "2814" ;
    dc:title "constituent of - material" ;
    dct:description """material - [is] constituent of - material.\r
Example: titanium white is a constituent of composite white; iron oxide is a constituent of desert varnish""" ;
    rdfs:domain skos:Concept ;
    rdfs:isDefinedBy aat:,
        <http://vocab.getty.edu/ontology> ;
    rdfs:range skos:Concept ;
    rdfs:subPropertyOf skos:related ;
    owl:inverseOf gvp:aat2815_composed_of ;
    skos:broader skos:related ;
    skos:example "iron oxide is a constituent of desert varnish",
        "titanium white is a constituent of composite white" ;
    skos:inScheme aat:,
        <http://vocab.getty.edu/ontology> ;
    skos:notation "2814" ;
    skos:prefLabel "aat2814_constituent_of"@en ;
    skos:topConceptOf aat:,
        <http://vocab.getty.edu/ontology> .

gvp:aat2817_derived-made_from a owl:ObjectProperty,
        skos:Concept ;
    dc:identifier "2817" ;
    dc:title "derived/made from - material" ;
    dct:description """material - [is] derived/made from - material.\r
Example: gypsum is derived/made from from anhydrite; wood board is derived/made from timber (lumber)""" ;
    rdfs:domain skos:Concept ;
    rdfs:isDefinedBy aat:,
        <http://vocab.getty.edu/ontology> ;
    rdfs:range skos:Concept ;
    rdfs:subPropertyOf skos:related ;
    owl:inverseOf gvp:aat2818_source_for ;
    skos:broader skos:related ;
    skos:example "gypsum is derived/made from from anhydrite",
        "wood board is derived/made from timber (lumber)" ;
    skos:inScheme aat:,
        <http://vocab.getty.edu/ontology> ;
    skos:notation "2817" ;
    skos:prefLabel "aat2817_derived-made_from"@en ;
    skos:topConceptOf aat:,
        <http://vocab.getty.edu/ontology> .

gvp:aat2818_source_for a owl:ObjectProperty,
        skos:Concept ;
    dc:identifier "2818" ;
    dc:title "source for - material" ;
    dct:description """material - [is] source for - material.\r
Example: anhydrite is the source for gypsum; timber (lumber) is the source for wood board""" ;
    rdfs:domain skos:Concept ;
    rdfs:isDefinedBy aat:,
        <http://vocab.getty.edu/ontology> ;
    rdfs:range skos:Concept ;
    rdfs:subPropertyOf skos:related ;
    skos:broader skos:related ;
    skos:example "anhydrite is the source for gypsum",
        "timber (lumber) is the source for wood board" ;
    skos:inScheme <http://vocab.getty.edu/ontology> ;
    skos:notation "2818" ;
    skos:prefLabel "aat2818_source_for"@en ;
    skos:topConceptOf <http://vocab.getty.edu/ontology> .

gvp:aat2821_based_on a owl:ObjectProperty,
        skos:Concept ;
    dc:identifier "2821" ;
    dc:title "based on - any" ;
    dct:description """any - [is] based on - any.\r
Example: Neo-Gothic is based on Gothic (Medieval); curved [form attribute] is based on curves (geometric figures); pencils are based on plummets""" ;
    rdfs:domain skos:Concept ;
    rdfs:isDefinedBy aat:,
        <http://vocab.getty.edu/ontology> ;
    rdfs:range skos:Concept ;
    rdfs:subPropertyOf skos:related ;
    owl:inverseOf gvp:aat2822_basis_of ;
    skos:broader skos:related ;
    skos:example "Neo-Gothic is based on Gothic (Medieval)",
        "curved [form attribute] is based on curves (geometric figures)",
        "pencils are based on plummets" ;
    skos:inScheme aat:,
        <http://vocab.getty.edu/ontology> ;
    skos:notation "2821" ;
    skos:prefLabel "aat2821_based_on"@en ;
    skos:topConceptOf aat:,
        <http://vocab.getty.edu/ontology> .

gvp:aat2822_basis_of a owl:ObjectProperty,
        skos:Concept ;
    dc:identifier "2822" ;
    dc:title "basis of - any" ;
    dct:description """any - [is] basis of - any.\r
Example: Gothic (Medieval) is the basis of Neo-Gothic; curves (geometric figures) are the basis of curved [form attribute]; plummets are the basis of pencils""" ;
    rdfs:domain skos:Concept ;
    rdfs:isDefinedBy aat:,
        <http://vocab.getty.edu/ontology> ;
    rdfs:range skos:Concept ;
    rdfs:subPropertyOf skos:related ;
    skos:broader skos:related ;
    skos:example "Gothic (Medieval) is the basis of Neo-Gothic",
        "curves (geometric figures) are the basis of curved [form attribute]",
        "plummets are the basis of pencils" ;
    skos:inScheme <http://vocab.getty.edu/ontology> ;
    skos:notation "2822" ;
    skos:prefLabel "aat2822_basis_of"@en ;
    skos:topConceptOf <http://vocab.getty.edu/ontology> .

gvp:aat2826_used_with a owl:ObjectProperty,
        owl:SymmetricProperty,
        skos:Concept ;
    dc:identifier "2826" ;
    dc:title "used with - material" ;
    dct:description """material - [is] used with - material.\r
Example: watercolor paper is used with watercolor (paint); arriccio is used with intonaco""" ;
    rdfs:domain skos:Concept ;
    rdfs:isDefinedBy aat:,
        <http://vocab.getty.edu/ontology> ;
    rdfs:range skos:Concept ;
    rdfs:subPropertyOf skos:related ;
    skos:broader skos:related ;
    skos:example "arriccio is used with intonaco",
        "watercolor paper is used with watercolor (paint)" ;
    skos:inScheme aat:,
        <http://vocab.getty.edu/ontology> ;
    skos:notation "2826" ;
    skos:prefLabel "aat2826_used_with"@en ;
    skos:topConceptOf aat:,
        <http://vocab.getty.edu/ontology> .

gvp:aat2828_use-require a owl:ObjectProperty,
        skos:Concept ;
    dc:identifier "2828" ;
    dc:title "use/require - material" ;
    dct:description """things - use/require - material.\r
Example: oil paintings use/require varnish; wine glasses use/require wine""" ;
    rdfs:domain skos:Concept ;
    rdfs:isDefinedBy aat:,
        <http://vocab.getty.edu/ontology> ;
    rdfs:range skos:Concept ;
    rdfs:subPropertyOf skos:related ;
    owl:inverseOf gvp:aat2829_used-required_for ;
    skos:broader skos:related ;
    skos:example "oil paintings use/require varnish",
        "wine glasses use/require wine" ;
    skos:inScheme aat:,
        <http://vocab.getty.edu/ontology> ;
    skos:notation "2828" ;
    skos:prefLabel "aat2828_use-require"@en ;
    skos:topConceptOf aat:,
        <http://vocab.getty.edu/ontology> .

gvp:aat2833_ancestor_of a owl:ObjectProperty,
        skos:Concept ;
    dc:identifier "2833" ;
    dc:title "ancestor of - genus/species" ;
    dct:description """genus/species - is ancestor of -  another genus/species.\r
Example: Canis lupus is the ancestor of Canis familiaris; Equus asinus is the ancestor of donkeys""" ;
    rdfs:domain skos:Concept ;
    rdfs:isDefinedBy aat:,
        <http://vocab.getty.edu/ontology> ;
    rdfs:range skos:Concept ;
    rdfs:subPropertyOf skos:related ;
    owl:inverseOf gvp:aat2834_decendant_of ;
    skos:broader skos:related ;
    skos:example "Canis lupus is the ancestor of Canis familiaris",
        "Equus asinus is the ancestor of donkeys" ;
    skos:inScheme aat:,
        <http://vocab.getty.edu/ontology> ;
    skos:notation "2833" ;
    skos:prefLabel "aat2833_ancestor_of"@en ;
    skos:topConceptOf aat:,
        <http://vocab.getty.edu/ontology> .

gvp:aat2834_decendant_of a owl:ObjectProperty,
        skos:Concept ;
    dc:identifier "2834" ;
    dc:title "decendant of - genus/species" ;
    dct:description """genus/species - is decendant of -  genus/species.\r
Example: Canis familiaris is the descendant of Canis lupus; donkeys are the descendents of Equus asinus""" ;
    rdfs:domain skos:Concept ;
    rdfs:isDefinedBy aat:,
        <http://vocab.getty.edu/ontology> ;
    rdfs:range skos:Concept ;
    rdfs:subPropertyOf skos:related ;
    skos:broader skos:related ;
    skos:example "Canis familiaris is the descendant of Canis lupus",
        "donkeys are the descendents of Equus asinus" ;
    skos:inScheme <http://vocab.getty.edu/ontology> ;
    skos:notation "2834" ;
    skos:prefLabel "aat2834_decendant_of"@en ;
    skos:topConceptOf <http://vocab.getty.edu/ontology> .

gvp:aat2846_locus-setting_for a owl:ObjectProperty,
        skos:Concept ;
    dc:identifier "2846" ;
    dc:title "locus/setting for - genus/species" ;
    dct:description """locus/setting - [is] locus/setting for - genus/species.\r
Example: elephant houses are the locus/setting for Elephantidae(family); vineyards are the locus/setting of Vitaceae (family)""" ;
    rdfs:domain skos:Concept ;
    rdfs:isDefinedBy aat:,
        <http://vocab.getty.edu/ontology> ;
    rdfs:range skos:Concept ;
    rdfs:subPropertyOf skos:related ;
    skos:broader skos:related ;
    skos:example "elephant houses are the locus/setting for Elephantidae(family)",
        "vineyards are the locus/setting of Vitaceae (family)" ;
    skos:inScheme <http://vocab.getty.edu/ontology> ;
    skos:notation "2846" ;
    skos:prefLabel "aat2846_locus-setting_for"@en ;
    skos:topConceptOf <http://vocab.getty.edu/ontology> .

gvp:aat2853_involve a owl:ObjectProperty,
        skos:Concept ;
    dc:identifier "2853" ;
    dc:title "involve - genus/species" ;
    dct:description """things/[equipment] - involve - genus/species.\r
Example: rose bowls involve Rosa (genus); camel saddles involve Camelus (genus)""" ;
    rdfs:domain skos:Concept ;
    rdfs:isDefinedBy aat:,
        <http://vocab.getty.edu/ontology> ;
    rdfs:range skos:Concept ;
    rdfs:subPropertyOf skos:related ;
    skos:broader skos:related ;
    skos:example "camel saddles involve Camelus (genus)",
        "rose bowls involve Rosa (genus)" ;
    skos:inScheme <http://vocab.getty.edu/ontology> ;
    skos:notation "2853" ;
    skos:prefLabel "aat2853_involve"@en ;
    skos:topConceptOf <http://vocab.getty.edu/ontology> .

gvp:aat2875_characteristic_of a owl:ObjectProperty,
        skos:Concept ;
    dc:identifier "2875" ;
    dc:title "characteristic of - style/period/culture" ;
    dct:description """language - [is] characteristic of - style/period/culture.\r
Example: Afar (language) is characteristic of Afar (culture); Celtic (language) was characteristic of Celtic (culture)""" ;
    rdfs:domain skos:Concept ;
    rdfs:isDefinedBy aat:,
        <http://vocab.getty.edu/ontology> ;
    rdfs:range skos:Concept ;
    rdfs:subPropertyOf skos:related ;
    owl:inverseOf gvp:aat2876_characterized_by ;
    skos:broader skos:related ;
    skos:example "Afar (language) is characteristic of Afar (culture)",
        "Celtic (language) was characteristic of Celtic (culture)" ;
    skos:inScheme aat:,
        <http://vocab.getty.edu/ontology> ;
    skos:notation "2875" ;
    skos:prefLabel "aat2875_characteristic_of"@en ;
    skos:topConceptOf aat:,
        <http://vocab.getty.edu/ontology> .

gvp:aat2878_preceded-source_for a owl:ObjectProperty,
        skos:Concept ;
    dc:identifier "2878" ;
    dc:title "preceded/source for - language" ;
    dct:description """language - preceded/[is] source for - language.\r
Example: Ancient Greek (language) preceded/is source for Greek (modern language); Ancient Egyptian (language) preceded/is source for Egyptian, Coptic (language)""" ;
    rdfs:domain skos:Concept ;
    rdfs:isDefinedBy aat:,
        <http://vocab.getty.edu/ontology> ;
    rdfs:range skos:Concept ;
    rdfs:subPropertyOf skos:related ;
    owl:inverseOf gvp:aat2879_followed-developed_from ;
    skos:broader skos:related ;
    skos:example "Ancient Egyptian (language) preceded/is source for Egyptian, Coptic (language)",
        "Ancient Greek (language) preceded/is source for Greek (modern language)" ;
    skos:inScheme aat:,
        <http://vocab.getty.edu/ontology> ;
    skos:notation "2878" ;
    skos:prefLabel "aat2878_preceded-source_for"@en ;
    skos:topConceptOf aat:,
        <http://vocab.getty.edu/ontology> .

gvp:aat2879_followed-developed_from a owl:ObjectProperty,
        skos:Concept ;
    dc:identifier "2879" ;
    dc:title "followed/developed from - language" ;
    dct:description """language - followed/developed from - language.\r
Example: Greek (modern language) followed/developed from Ancient Greek (language); Egyptian, Coptic (language) followed/developed from Ancient Egyptian (language)""" ;
    rdfs:domain skos:Concept ;
    rdfs:isDefinedBy aat:,
        <http://vocab.getty.edu/ontology> ;
    rdfs:range skos:Concept ;
    rdfs:subPropertyOf skos:related ;
    skos:broader skos:related ;
    skos:example "Egyptian, Coptic (language) followed/developed from Ancient Egyptian (language)",
        "Greek (modern language) followed/developed from Ancient Greek (language)" ;
    skos:inScheme <http://vocab.getty.edu/ontology> ;
    skos:notation "2879" ;
    skos:prefLabel "aat2879_followed-developed_from"@en ;
    skos:topConceptOf <http://vocab.getty.edu/ontology> .

gvp:aat2881_reflected_in a owl:ObjectProperty,
        skos:Concept ;
    dc:identifier "2881" ;
    dc:title "reflected in - things" ;
    dct:description """language - [is] reflected in - things.\r
Example: Greek (language) is reflected in Greek alphabet; Sanskrit is reflected in Vedas""" ;
    rdfs:domain skos:Concept ;
    rdfs:isDefinedBy aat:,
        <http://vocab.getty.edu/ontology> ;
    rdfs:range skos:Concept ;
    rdfs:subPropertyOf skos:related ;
    owl:inverseOf gvp:aat2882_reflect ;
    skos:broader skos:related ;
    skos:example "Greek (language) is reflected in Greek alphabet",
        "Sanskrit is reflected in Vedas" ;
    skos:inScheme aat:,
        <http://vocab.getty.edu/ontology> ;
    skos:notation "2881" ;
    skos:prefLabel "aat2881_reflected_in"@en ;
    skos:topConceptOf aat:,
        <http://vocab.getty.edu/ontology> .

gvp:aat2884_involved_with a owl:ObjectProperty,
        skos:Concept ;
    dc:identifier "2884" ;
    dc:title "involved with - any" ;
    dct:description """attributes /associated concepts - [are] involved with - any.\r
Example: climate is involved with climate change; insect damage is involved with infestation; Celtic crosses (design motif) are involved with Celtic culture""" ;
    rdfs:domain skos:Concept ;
    rdfs:isDefinedBy aat:,
        <http://vocab.getty.edu/ontology> ;
    rdfs:range skos:Concept ;
    rdfs:subPropertyOf skos:related ;
    owl:inverseOf gvp:aat2885_involves ;
    skos:broader skos:related ;
    skos:example "Celtic crosses (design motif) are involved with Celtic culture",
        "climate is involved with climate change",
        "insect damage is involved with infestation" ;
    skos:inScheme aat:,
        <http://vocab.getty.edu/ontology> ;
    skos:notation "2884" ;
    skos:prefLabel "aat2884_involved_with"@en ;
    skos:topConceptOf aat:,
        <http://vocab.getty.edu/ontology> .

gvp:aat2887_exemplified_by a owl:ObjectProperty,
        skos:Concept ;
    dc:identifier "2887" ;
    dc:title "exemplified by - material" ;
    dct:description """material - exemplified by - material.\r
Example: solvent - exemplified by - carbon disulfide""" ;
    rdfs:domain skos:Concept ;
    rdfs:isDefinedBy aat:,
        <http://vocab.getty.edu/ontology> ;
    rdfs:range skos:Concept ;
    rdfs:subPropertyOf skos:related ;
    skos:broader skos:related ;
    skos:example "solvent - exemplified by - carbon disulfide" ;
    skos:inScheme <http://vocab.getty.edu/ontology> ;
    skos:notation "2887" ;
    skos:prefLabel "aat2887_exemplified_by"@en ;
    skos:topConceptOf <http://vocab.getty.edu/ontology> .

gvp:aat2891_exemplified_by a owl:ObjectProperty,
        skos:Concept ;
    dc:identifier "2891" ;
    dc:title "exemplified by - brand name" ;
    dct:description """things - [are] exemplied by - brand name.\r
Example: photothermographic transfer prints are exemplified by Pictrography (TM) prints""" ;
    rdfs:domain skos:Concept ;
    rdfs:isDefinedBy aat:,
        <http://vocab.getty.edu/ontology> ;
    rdfs:range skos:Concept ;
    rdfs:subPropertyOf skos:related ;
    owl:inverseOf gvp:aat2892_example_of ;
    skos:broader skos:related ;
    skos:example "photothermographic transfer prints are exemplified by Pictrography (TM) prints" ;
    skos:inScheme aat:,
        <http://vocab.getty.edu/ontology> ;
    skos:notation "2891" ;
    skos:prefLabel "aat2891_exemplified_by"@en ;
    skos:topConceptOf aat:,
        <http://vocab.getty.edu/ontology> .

gvp:aat2894_exemplified_by a owl:ObjectProperty,
        skos:Concept ;
    dc:identifier "2894" ;
    dc:title "exemplified by - brand name" ;
    dct:description """activity/event/[process/function] - [is] exemplified by - brand name.\r
Example: deacidification [process/function] is exemplified by Papersave Process (TM)""" ;
    rdfs:domain skos:Concept ;
    rdfs:isDefinedBy aat:,
        <http://vocab.getty.edu/ontology> ;
    rdfs:range skos:Concept ;
    rdfs:subPropertyOf skos:related ;
    owl:inverseOf gvp:aat2895_example_of ;
    skos:broader skos:related ;
    skos:example "deacidification [process/function] is exemplified by Papersave Process (TM)" ;
    skos:inScheme aat:,
        <http://vocab.getty.edu/ontology> ;
    skos:notation "2894" ;
    skos:prefLabel "aat2894_exemplified_by"@en ;
    skos:topConceptOf aat:,
        <http://vocab.getty.edu/ontology> .

gvp:aat2895_example_of a owl:ObjectProperty,
        skos:Concept ;
    dc:identifier "2895" ;
    dc:title "example of - activity/event" ;
    dct:description """brand name - [is] example of - activity/event/[process/function].\r
Example: Papersave Process (TM) is example of deacidification [process/function]""" ;
    rdfs:domain skos:Concept ;
    rdfs:isDefinedBy aat:,
        <http://vocab.getty.edu/ontology> ;
    rdfs:range skos:Concept ;
    rdfs:subPropertyOf skos:related ;
    skos:broader skos:related ;
    skos:example "Papersave Process (TM) is example of deacidification [process/function]" ;
    skos:inScheme <http://vocab.getty.edu/ontology> ;
    skos:notation "2895" ;
    skos:prefLabel "aat2895_example_of"@en ;
    skos:topConceptOf <http://vocab.getty.edu/ontology> .

gvp:broaderPartitive a owl:ObjectProperty,
        skos:Concept ;
    rdfs:label "broaderPartitive"@en ;
    dct:description """BTP (Part/Whole, "part of") relation. We also infer iso-thes:broaderPartitive, which goes only between Concepts.
Example: Tuscany (TGN) BTP Italy (TGN)""" ;
    rdfs:comment "BTP (Part/Whole, \"part of\") relation. We also infer iso-thes:broaderPartitive, which goes only between Concepts" ;
    rdfs:domain gvp:Subject ;
    rdfs:isDefinedBy <http://vocab.getty.edu/ontology> ;
    rdfs:range gvp:Subject ;
    rdfs:subPropertyOf gvp:broader,
        gvp:broaderPartitiveExtended ;
    skos:broader gvp:broader ;
    skos:example "Tuscany (TGN) BTP Italy (TGN)" ;
    skos:inScheme <http://vocab.getty.edu/ontology> ;
    skos:prefLabel "broaderPartitive"@en ;
    skos:topConceptOf <http://vocab.getty.edu/ontology> .

gvp:broaderPreferred a owl:ObjectProperty,
        skos:Concept ;
    rdfs:label "broaderPreferred"@en ;
    dct:description """Main parent of a subject. Needed to display the hierarchy.
Example: Preferred: "baking dishes" (AAT) BTG "bakeware" (AAT); Sofia (TGN) BTP Bulgaria (TGN)""" ;
    rdfs:comment "Main parent of a subject. Needed to display the hierarchy" ;
    rdfs:domain gvp:Subject ;
    rdfs:isDefinedBy <http://vocab.getty.edu/ontology> ;
    rdfs:range gvp:Subject ;
    rdfs:subPropertyOf gvp:broader,
        gvp:broaderPreferredExtended ;
    skos:broader gvp:broaderPreferredExtended ;
    skos:example "Preferred: \"baking dishes\" (AAT) BTG \"bakeware\" (AAT); Sofia (TGN) BTP Bulgaria (TGN)" ;
    skos:inScheme <http://vocab.getty.edu/ontology> ;
    skos:prefLabel "broaderPreferred"@en ;
    skos:topConceptOf <http://vocab.getty.edu/ontology> .

gvp:tgn3000_related_to a owl:ObjectProperty,
        owl:SymmetricProperty,
        skos:Concept ;
    dc:identifier "3000" ;
    dc:title "related to - any" ;
    dct:description """any - related to - any.\r
Example: Fountains Abbey is related to Studley Royal; Austria-Hungary is related to Magyarorszag""" ;
    rdfs:domain skos:Concept ;
    rdfs:isDefinedBy <http://vocab.getty.edu/ontology>,
        tgn: ;
    rdfs:range skos:Concept ;
    rdfs:subPropertyOf skos:related ;
    skos:broader skos:related ;
    skos:example "Austria-Hungary is related to Magyarorszag",
        "Fountains Abbey is related to Studley Royal" ;
    skos:inScheme <http://vocab.getty.edu/ontology>,
        tgn: ;
    skos:notation "3000" ;
    skos:prefLabel "tgn3000_related_to"@en ;
    skos:topConceptOf <http://vocab.getty.edu/ontology>,
        tgn: .

gvp:tgn3006_formerly_identified_as a owl:ObjectProperty,
        owl:SymmetricProperty,
        skos:Concept ;
    dc:identifier "3006" ;
    dc:title "formerly identified as - place" ;
    dct:description """place - formerly identified as - place; New.\r
Example: The deserted settlement of Machupicchu was formerly identified as Tampu Tocco""" ;
    rdfs:domain skos:Concept ;
    rdfs:isDefinedBy <http://vocab.getty.edu/ontology>,
        tgn: ;
    rdfs:range skos:Concept ;
    rdfs:subPropertyOf skos:related ;
    skos:broader skos:related ;
    skos:example "The deserted settlement of Machupicchu was formerly identified as Tampu Tocco" ;
    skos:inScheme <http://vocab.getty.edu/ontology>,
        tgn: ;
    skos:notation "3006" ;
    skos:prefLabel "tgn3006_formerly_identified_as"@en ;
    skos:scopeNote "New" ;
    skos:topConceptOf <http://vocab.getty.edu/ontology>,
        tgn: .

gvp:tgn3101_near-adjacent_to a owl:ObjectProperty,
        owl:SymmetricProperty,
        skos:Concept ;
    dc:identifier "3101" ;
    dc:title "near/adjacent to - any" ;
    dct:description """any - near/adjacent to - any.\r
Example: Saint Paul (Minnesota, USA), is linked to its 'Twin City' Minneapolis (Hennepin county, Minnesota, USA)""" ;
    rdfs:domain skos:Concept ;
    rdfs:isDefinedBy <http://vocab.getty.edu/ontology>,
        tgn: ;
    rdfs:range skos:Concept ;
    rdfs:subPropertyOf skos:related ;
    skos:broader skos:related ;
    skos:example "Saint Paul (Minnesota, USA), is linked to its 'Twin City' Minneapolis (Hennepin county, Minnesota, USA)" ;
    skos:inScheme <http://vocab.getty.edu/ontology>,
        tgn: ;
    skos:notation "3101" ;
    skos:prefLabel "tgn3101_near-adjacent_to"@en ;
    skos:topConceptOf <http://vocab.getty.edu/ontology>,
        tgn: .

gvp:tgn3102_coextensive_with a owl:ObjectProperty,
        owl:SymmetricProperty,
        skos:Concept ;
    dc:identifier "3102" ;
    dc:title "coextensive with - place" ;
    dct:description """place - coextensive with - place.\r
Example: Kings county (New York, USA) is coextensive with Brooklyn (New York, USA)""" ;
    rdfs:domain skos:Concept ;
    rdfs:isDefinedBy <http://vocab.getty.edu/ontology>,
        tgn: ;
    rdfs:range skos:Concept ;
    rdfs:subPropertyOf skos:related ;
    skos:broader skos:related ;
    skos:example "Kings county (New York, USA) is coextensive with Brooklyn (New York, USA)" ;
    skos:inScheme <http://vocab.getty.edu/ontology>,
        tgn: ;
    skos:notation "3102" ;
    skos:prefLabel "tgn3102_coextensive_with"@en ;
    skos:topConceptOf <http://vocab.getty.edu/ontology>,
        tgn: .

gvp:tgn3103_located_on a owl:ObjectProperty,
        skos:Concept ;
    dc:identifier "3103" ;
    dc:title "located on - place" ;
    dct:description """place - located on - place.\r
Example: tgn:7018835 Palmyra is located on tgn:7031416 Silk Road""" ;
    rdfs:domain skos:Concept ;
    rdfs:isDefinedBy <http://vocab.getty.edu/ontology>,
        tgn: ;
    rdfs:range skos:Concept ;
    rdfs:subPropertyOf skos:related ;
    owl:inverseOf gvp:tgn3104_is_location_of ;
    skos:broader skos:related ;
    skos:example "tgn:7018835 Palmyra is located on tgn:7031416 Silk Road" ;
    skos:inScheme <http://vocab.getty.edu/ontology>,
        tgn: ;
    skos:notation "3103" ;
    skos:prefLabel "tgn3103_located_on"@en ;
    skos:topConceptOf <http://vocab.getty.edu/ontology>,
        tgn: .

gvp:tgn3110_meaning-usage_overlaps_with a owl:ObjectProperty,
        owl:SymmetricProperty,
        skos:Concept ;
    dc:identifier "3110" ;
    dc:title "meaning/usage overlaps with - any" ;
    dct:description """any - meaning/usage overlaps with - any.\r
Example: Judaea (Israel) (historical region) meaning/usage overlaps with Holy Land (Asia) (historical region)""" ;
    rdfs:domain skos:Concept ;
    rdfs:isDefinedBy <http://vocab.getty.edu/ontology>,
        tgn: ;
    rdfs:range skos:Concept ;
    rdfs:subPropertyOf skos:related ;
    skos:broader skos:related ;
    skos:example "Judaea (Israel) (historical region) meaning/usage overlaps with Holy Land (Asia) (historical region)" ;
    skos:inScheme <http://vocab.getty.edu/ontology>,
        tgn: ;
    skos:notation "3110" ;
    skos:prefLabel "tgn3110_meaning-usage_overlaps_with"@en ;
    skos:topConceptOf <http://vocab.getty.edu/ontology>,
        tgn: .

gvp:tgn3202_capital_is a owl:ObjectProperty,
        skos:Concept ;
    dc:identifier "3202" ;
    dc:title "capital is - city" ;
    dct:description """nation - capital is - city.\r
Example: London was the capital of Maxima Caesariensis from 296 to 800 CE""" ;
    rdfs:domain skos:Concept ;
    rdfs:isDefinedBy <http://vocab.getty.edu/ontology>,
        tgn: ;
    rdfs:range skos:Concept ;
    rdfs:subPropertyOf skos:related ;
    skos:broader skos:related ;
    skos:example "London was the capital of Maxima Caesariensis from 296 to 800 CE" ;
    skos:inScheme <http://vocab.getty.edu/ontology> ;
    skos:notation "3202" ;
    skos:prefLabel "tgn3202_capital_is"@en ;
    skos:topConceptOf <http://vocab.getty.edu/ontology> .

gvp:tgn3317_member_of a owl:ObjectProperty,
        skos:Concept ;
    dc:identifier "3317" ;
    dc:title "member of - union" ;
    dct:description """nation - member of - union.\r
Example: Austria is a member of the European Union since 1915; Belgium is a member of the European Union since 1958""" ;
    rdfs:domain skos:Concept ;
    rdfs:isDefinedBy <http://vocab.getty.edu/ontology>,
        tgn: ;
    rdfs:range skos:Concept ;
    rdfs:subPropertyOf skos:related ;
    owl:inverseOf gvp:tgn3318_member_is ;
    skos:broader skos:related ;
    skos:example "Austria is a member of the European Union since 1915",
        "Belgium is a member of the European Union since 1958" ;
    skos:inScheme <http://vocab.getty.edu/ontology>,
        tgn: ;
    skos:notation "3317" ;
    skos:prefLabel "tgn3317_member_of"@en ;
    skos:topConceptOf <http://vocab.getty.edu/ontology>,
        tgn: .

gvp:tgn3411_successor_of a owl:ObjectProperty,
        skos:Concept ;
    dc:identifier "3411" ;
    dc:title "successor of - nation" ;
    dct:description """nation - successor of - nation.\r
Example: Iran (nation) is the successor of Persia""" ;
    rdfs:domain skos:Concept ;
    rdfs:isDefinedBy <http://vocab.getty.edu/ontology>,
        tgn: ;
    rdfs:range skos:Concept ;
    rdfs:subPropertyOf skos:related ;
    owl:inverseOf gvp:tgn3412_predecessor_of ;
    skos:broader skos:related ;
    skos:example "Iran (nation) is the successor of Persia" ;
    skos:inScheme <http://vocab.getty.edu/ontology>,
        tgn: ;
    skos:notation "3411" ;
    skos:prefLabel "tgn3411_successor_of"@en ;
    skos:topConceptOf <http://vocab.getty.edu/ontology>,
        tgn: .

gvp:tgn3412_predecessor_of a owl:ObjectProperty,
        skos:Concept ;
    dc:identifier "3412" ;
    dc:title "predecessor of - nation" ;
    dct:description """nation - predecessor of - nation.\r
Example: Persia is the predecessor of Iran (nation)""" ;
    rdfs:domain skos:Concept ;
    rdfs:isDefinedBy <http://vocab.getty.edu/ontology>,
        tgn: ;
    rdfs:range skos:Concept ;
    rdfs:subPropertyOf skos:related ;
    skos:broader skos:related ;
    skos:example "Persia is the predecessor of Iran (nation)" ;
    skos:inScheme <http://vocab.getty.edu/ontology> ;
    skos:notation "3412" ;
    skos:prefLabel "tgn3412_predecessor_of"@en ;
    skos:topConceptOf <http://vocab.getty.edu/ontology> .

gvp:tgn3510_historical_connection a owl:ObjectProperty,
        owl:SymmetricProperty,
        skos:Concept ;
    dc:identifier "3510" ;
    dc:title "historical connection - any" ;
    dct:description """any - historical connection - any.\r
Example: Guyenne, France (historical region) has a historical connection to Gascogne (France) (historical region)""" ;
    rdfs:domain skos:Concept ;
    rdfs:isDefinedBy <http://vocab.getty.edu/ontology>,
        tgn: ;
    rdfs:range skos:Concept ;
    rdfs:subPropertyOf skos:related ;
    skos:broader skos:related ;
    skos:example "Guyenne, France (historical region) has a historical connection to Gascogne (France) (historical region)" ;
    skos:inScheme <http://vocab.getty.edu/ontology>,
        tgn: ;
    skos:notation "3510" ;
    skos:prefLabel "tgn3510_historical_connection"@en ;
    skos:topConceptOf <http://vocab.getty.edu/ontology>,
        tgn: .

gvp:tgn3611_administrative_dependent_of a owl:ObjectProperty,
        skos:Concept ;
    dc:identifier "3611" ;
    dc:title "administrative dependent of - place" ;
    dct:description """place - administrative dependent of - place; New.\r
Example: Luni (La Spezia province, Liguria, Italy) is the admisistrative dependent of Ortonovo (Massa-Carrara province, Tuscany, Italy)""" ;
    rdfs:domain skos:Concept ;
    rdfs:isDefinedBy <http://vocab.getty.edu/ontology>,
        tgn: ;
    rdfs:range skos:Concept ;
    rdfs:subPropertyOf skos:related ;
    owl:inverseOf gvp:tgn3612_administrative_entity_for ;
    skos:broader skos:related ;
    skos:example "Luni (La Spezia province, Liguria, Italy) is the admisistrative dependent of Ortonovo (Massa-Carrara province, Tuscany, Italy)" ;
    skos:inScheme <http://vocab.getty.edu/ontology>,
        tgn: ;
    skos:notation "3611" ;
    skos:prefLabel "tgn3611_administrative_dependent_of"@en ;
    skos:scopeNote "New" ;
    skos:topConceptOf <http://vocab.getty.edu/ontology>,
        tgn: .

gvp:ulan1003_associated_with a owl:ObjectProperty,
        owl:SymmetricProperty,
        skos:Concept ;
    dc:identifier "1003" ;
    dc:title "associated with - any" ;
    dct:description """any - associated with - any.\r
Example: Richard Meier is associated with Renny B.Saltzman; United Nations is associated with World Bank""" ;
    rdfs:domain skos:Concept ;
    rdfs:isDefinedBy <http://vocab.getty.edu/ontology>,
        ulan: ;
    rdfs:range skos:Concept ;
    rdfs:subPropertyOf skos:related ;
    skos:broader skos:related ;
    skos:example "Richard Meier is associated with Renny B.Saltzman",
        "United Nations is associated with World Bank" ;
    skos:inScheme <http://vocab.getty.edu/ontology>,
        ulan: ;
    skos:notation "1003" ;
    skos:prefLabel "ulan1003_associated_with"@en ;
    skos:topConceptOf <http://vocab.getty.edu/ontology>,
        ulan: .

gvp:ulan1005_possibly_identified_with a owl:ObjectProperty,
        owl:SymmetricProperty,
        skos:Concept ;
    dc:identifier "1005" ;
    dc:title "possibly identified with - any" ;
    dct:description """any - possibly identified with - any.\r
Example: Master of the Saint John Altarpiece is possibly identified with Hughe Jacobsz; Bauart is possibly identified with Gruppe BAUart""" ;
    rdfs:domain skos:Concept ;
    rdfs:isDefinedBy <http://vocab.getty.edu/ontology>,
        ulan: ;
    rdfs:range skos:Concept ;
    rdfs:subPropertyOf skos:related ;
    skos:broader skos:related ;
    skos:example "Bauart is possibly identified with Gruppe BAUart",
        "Master of the Saint John Altarpiece is possibly identified with Hughe Jacobsz" ;
    skos:inScheme <http://vocab.getty.edu/ontology>,
        ulan: ;
    skos:notation "1005" ;
    skos:prefLabel "ulan1005_possibly_identified_with"@en ;
    skos:topConceptOf <http://vocab.getty.edu/ontology>,
        ulan: .

gvp:ulan1007_distinguished_from a owl:ObjectProperty,
        owl:SymmetricProperty,
        skos:Concept ;
    dc:identifier "1007" ;
    dc:title "distinguished from - any" ;
    dct:description """any - distinguished from - any.\r
Example: Laura Theresa Alma-Tadema is distinguished from Lawrence Alma-Tadema; The Noguchi Museum is distinguished form Isamu Noguchi Garden Museum Japan""" ;
    rdfs:domain skos:Concept ;
    rdfs:isDefinedBy <http://vocab.getty.edu/ontology>,
        ulan: ;
    rdfs:range skos:Concept ;
    rdfs:subPropertyOf skos:related ;
    skos:broader skos:related ;
    skos:example "Laura Theresa Alma-Tadema is distinguished from Lawrence Alma-Tadema",
        "The Noguchi Museum is distinguished form Isamu Noguchi Garden Museum Japan" ;
    skos:inScheme <http://vocab.getty.edu/ontology>,
        ulan: ;
    skos:notation "1007" ;
    skos:prefLabel "ulan1007_distinguished_from"@en ;
    skos:topConceptOf <http://vocab.getty.edu/ontology>,
        ulan: .

gvp:ulan1008_meaning_-usage_overlaps_with a owl:ObjectProperty,
        owl:SymmetricProperty,
        skos:Concept ;
    dc:identifier "1008" ;
    dc:title "meaning /usage overlaps with - any" ;
    dct:description """any - meaning /usage overlaps with - any.\r
Example: The meaning or usage of unknown Zimbabwean overlaps with unknown Rodesian""" ;
    rdfs:domain skos:Concept ;
    rdfs:isDefinedBy <http://vocab.getty.edu/ontology>,
        ulan: ;
    rdfs:range skos:Concept ;
    rdfs:subPropertyOf skos:related ;
    skos:broader skos:related ;
    skos:example "The meaning or usage of unknown Zimbabwean overlaps with unknown Rodesian" ;
    skos:inScheme <http://vocab.getty.edu/ontology>,
        ulan: ;
    skos:notation "1008" ;
    skos:prefLabel "ulan1008_meaning_-usage_overlaps_with"@en ;
    skos:topConceptOf <http://vocab.getty.edu/ontology>,
        ulan: .

gvp:ulan1101_teacher_of a owl:ObjectProperty,
        skos:Concept ;
    dc:identifier "1101" ;
    dc:title "teacher of - person" ;
    dct:description """person - teacher of - person.\r
Example: Rivalz, Antoine was the teacher of Pierre Subleyras""" ;
    rdfs:domain skos:Concept ;
    rdfs:isDefinedBy <http://vocab.getty.edu/ontology>,
        ulan: ;
    rdfs:range skos:Concept ;
    rdfs:subPropertyOf skos:related ;
    owl:inverseOf gvp:ulan1102_student_of ;
    skos:broader skos:related ;
    skos:example "Rivalz, Antoine was the teacher of Pierre Subleyras" ;
    skos:inScheme <http://vocab.getty.edu/ontology>,
        ulan: ;
    skos:notation "1101" ;
    skos:prefLabel "ulan1101_teacher_of"@en ;
    skos:topConceptOf <http://vocab.getty.edu/ontology>,
        ulan: .

gvp:ulan1107_influenced a owl:ObjectProperty,
        skos:Concept ;
    dc:identifier "1107" ;
    dc:title "influenced - person" ;
    dct:description """person - influenced - person.\r
Example: Rembrandt van Rijn influenced Salomon Koninck""" ;
    rdfs:domain skos:Concept ;
    rdfs:isDefinedBy <http://vocab.getty.edu/ontology>,
        ulan: ;
    rdfs:range skos:Concept ;
    rdfs:subPropertyOf skos:related ;
    owl:inverseOf gvp:ulan1108_influenced_by ;
    skos:broader skos:related ;
    skos:example "Rembrandt van Rijn influenced Salomon Koninck" ;
    skos:inScheme <http://vocab.getty.edu/ontology>,
        ulan: ;
    skos:notation "1107" ;
    skos:prefLabel "ulan1107_influenced"@en ;
    skos:topConceptOf <http://vocab.getty.edu/ontology>,
        ulan: .

gvp:ulan1201_patron_of a owl:ObjectProperty,
        skos:Concept ;
    dc:identifier "1201" ;
    dc:title "patron of - person/firm/family" ;
    dct:description """person - patron of - person/firm/family.\r
Example: Cosimo I, Grand-Duke of Tuscany was the patron of Donatello""" ;
    rdfs:domain skos:Concept ;
    rdfs:isDefinedBy <http://vocab.getty.edu/ontology>,
        ulan: ;
    rdfs:range skos:Concept ;
    rdfs:subPropertyOf skos:related ;
    owl:inverseOf gvp:ulan1202_patron_was ;
    skos:broader skos:related ;
    skos:example "Cosimo I, Grand-Duke of Tuscany was the patron of Donatello" ;
    skos:inScheme <http://vocab.getty.edu/ontology>,
        ulan: ;
    skos:notation "1201" ;
    skos:prefLabel "ulan1201_patron_of"@en ;
    skos:topConceptOf <http://vocab.getty.edu/ontology>,
        ulan: .

gvp:ulan1202_patron_was a owl:ObjectProperty,
        skos:Concept ;
    dc:identifier "1202" ;
    dc:title "patron was - person" ;
    dct:description """person/firm/family - patron was - person.\r
Example: The patron of Donatello was Cosimo I, Grand-Duke of Tuscany""" ;
    rdfs:domain skos:Concept ;
    rdfs:isDefinedBy <http://vocab.getty.edu/ontology>,
        ulan: ;
    rdfs:range skos:Concept ;
    rdfs:subPropertyOf skos:related ;
    skos:broader skos:related ;
    skos:example "The patron of Donatello was Cosimo I, Grand-Duke of Tuscany" ;
    skos:inScheme <http://vocab.getty.edu/ontology> ;
    skos:notation "1202" ;
    skos:prefLabel "ulan1202_patron_was"@en ;
    skos:topConceptOf <http://vocab.getty.edu/ontology> .

gvp:ulan1204_donor_was a owl:ObjectProperty,
        skos:Concept ;
    dc:identifier "1204" ;
    dc:title "donor was - person/firm/family" ;
    dct:description """person/firm/family - donor was - person/firm/family.\r
Example: Donor to the National Gallery of Art was Andrew W. Mellon""" ;
    rdfs:domain skos:Concept ;
    rdfs:isDefinedBy <http://vocab.getty.edu/ontology>,
        ulan: ;
    rdfs:range skos:Concept ;
    rdfs:subPropertyOf skos:related ;
    skos:broader skos:related ;
    skos:example "Donor to the National Gallery of Art was Andrew W. Mellon" ;
    skos:inScheme <http://vocab.getty.edu/ontology> ;
    skos:notation "1204" ;
    skos:prefLabel "ulan1204_donor_was"@en ;
    skos:topConceptOf <http://vocab.getty.edu/ontology> .

gvp:ulan1206_client_was a owl:ObjectProperty,
        skos:Concept ;
    dc:identifier "1206" ;
    dc:title "client was - person/firm/family" ;
    dct:description """person/firm/family - client was - person/firm/family.\r
Example: Burnham and Root's client was the Chicago Herald""" ;
    rdfs:domain skos:Concept ;
    rdfs:isDefinedBy <http://vocab.getty.edu/ontology>,
        ulan: ;
    rdfs:range skos:Concept ;
    rdfs:subPropertyOf skos:related ;
    skos:broader skos:related ;
    skos:example "Burnham and Root's client was the Chicago Herald" ;
    skos:inScheme <http://vocab.getty.edu/ontology> ;
    skos:notation "1206" ;
    skos:prefLabel "ulan1206_client_was"@en ;
    skos:topConceptOf <http://vocab.getty.edu/ontology> .

gvp:ulan1212_artist_was a owl:ObjectProperty,
        skos:Concept ;
    dc:identifier "1212" ;
    dc:title "artist was - person" ;
    dct:description """person - artist was - person.\r
Example: Charles-Pierre Coustou was artist to Louis XIV, King of France""" ;
    rdfs:domain skos:Concept ;
    rdfs:isDefinedBy <http://vocab.getty.edu/ontology>,
        ulan: ;
    rdfs:range skos:Concept ;
    rdfs:subPropertyOf skos:related ;
    skos:broader skos:related ;
    skos:example "Charles-Pierre Coustou was artist to Louis XIV, King of France" ;
    skos:inScheme <http://vocab.getty.edu/ontology> ;
    skos:notation "1212" ;
    skos:prefLabel "ulan1212_artist_was"@en ;
    skos:topConceptOf <http://vocab.getty.edu/ontology> .

gvp:ulan1214_court_artist_was a owl:ObjectProperty,
        skos:Concept ;
    dc:identifier "1214" ;
    dc:title "court artist was - person" ;
    dct:description """person - court artist was - person.\r
Example: Peter Paul Rubens was court artist to Gonzaga Vincenzo I, Duke of Mantua; Francisco de Goya was court artist to Charles IV, King of Spain""" ;
    rdfs:domain skos:Concept ;
    rdfs:isDefinedBy <http://vocab.getty.edu/ontology>,
        ulan: ;
    rdfs:range skos:Concept ;
    rdfs:subPropertyOf skos:related ;
    skos:broader skos:related ;
    skos:example "Francisco de Goya was court artist to Charles IV, King of Spain",
        "Peter Paul Rubens was court artist to Gonzaga Vincenzo I, Duke of Mantua" ;
    skos:inScheme <http://vocab.getty.edu/ontology> ;
    skos:notation "1214" ;
    skos:prefLabel "ulan1214_court_artist_was"@en ;
    skos:topConceptOf <http://vocab.getty.edu/ontology> .

gvp:ulan1218_employee_was a owl:ObjectProperty,
        skos:Concept ;
    dc:identifier "1218" ;
    dc:title "employee was - person/firm" ;
    dct:description """person - employee was - person/firm.\r
Example: Jean Tijou was an employee of Christopher Wren""" ;
    rdfs:domain skos:Concept ;
    rdfs:isDefinedBy <http://vocab.getty.edu/ontology>,
        ulan: ;
    rdfs:range skos:Concept ;
    rdfs:subPropertyOf skos:related ;
    skos:broader skos:related ;
    skos:example "Jean Tijou was an employee of Christopher Wren" ;
    skos:inScheme <http://vocab.getty.edu/ontology> ;
    skos:notation "1218" ;
    skos:prefLabel "ulan1218_employee_was"@en ;
    skos:topConceptOf <http://vocab.getty.edu/ontology> .

gvp:ulan1221_appointed_by a owl:ObjectProperty,
        skos:Concept ;
    dc:identifier "1221" ;
    dc:title "appointed by - person" ;
    dct:description """person - appointed by - person.\r
Example: Pope Urban VIII appointed Virginio Cesarini""" ;
    rdfs:domain skos:Concept ;
    rdfs:isDefinedBy <http://vocab.getty.edu/ontology>,
        ulan: ;
    rdfs:range skos:Concept ;
    rdfs:subPropertyOf skos:related ;
    owl:inverseOf gvp:ulan1222_appointee_of ;
    skos:broader skos:related ;
    skos:example "Pope Urban VIII appointed Virginio Cesarini" ;
    skos:inScheme <http://vocab.getty.edu/ontology>,
        ulan: ;
    skos:notation "1221" ;
    skos:prefLabel "ulan1221_appointed_by"@en ;
    skos:topConceptOf <http://vocab.getty.edu/ontology>,
        ulan: .

gvp:ulan1223_crowned_by a owl:ObjectProperty,
        skos:Concept ;
    dc:identifier "1223" ;
    dc:title "crowned by - person" ;
    dct:description """person - crowned by - person.\r
Example: Pope Leo III crowned Emperor Charlemagne""" ;
    rdfs:domain skos:Concept ;
    rdfs:isDefinedBy <http://vocab.getty.edu/ontology>,
        ulan: ;
    rdfs:range skos:Concept ;
    rdfs:subPropertyOf skos:related ;
    owl:inverseOf gvp:ulan1224_crowned ;
    skos:broader skos:related ;
    skos:example "Pope Leo III crowned Emperor Charlemagne" ;
    skos:inScheme <http://vocab.getty.edu/ontology>,
        ulan: ;
    skos:notation "1223" ;
    skos:prefLabel "ulan1223_crowned_by"@en ;
    skos:topConceptOf <http://vocab.getty.edu/ontology>,
        ulan: .

gvp:ulan1303_collaborated_with a owl:ObjectProperty,
        owl:SymmetricProperty,
        skos:Concept ;
    dc:identifier "1303" ;
    dc:title "collaborated with - person" ;
    dct:description """person - collaborated with - person.\r
Example: Pablo Picasso collaborated with Georges Braque""" ;
    rdfs:domain skos:Concept ;
    rdfs:isDefinedBy <http://vocab.getty.edu/ontology>,
        ulan: ;
    rdfs:range skos:Concept ;
    rdfs:subPropertyOf skos:related ;
    skos:broader skos:related ;
    skos:example "Pablo Picasso collaborated with Georges Braque" ;
    skos:inScheme <http://vocab.getty.edu/ontology>,
        ulan: ;
    skos:notation "1303" ;
    skos:prefLabel "ulan1303_collaborated_with"@en ;
    skos:topConceptOf <http://vocab.getty.edu/ontology>,
        ulan: .

gvp:ulan1305_worked_with a owl:ObjectProperty,
        owl:SymmetricProperty,
        skos:Concept ;
    dc:identifier "1305" ;
    dc:title "worked with - person" ;
    dct:description """person - worked with - person.\r
Example: William Cleare worked with Christopher Wren; Frank Lloyd Wright work with Aaron G. Green""" ;
    rdfs:domain skos:Concept ;
    rdfs:isDefinedBy <http://vocab.getty.edu/ontology>,
        ulan: ;
    rdfs:range skos:Concept ;
    rdfs:subPropertyOf skos:related ;
    skos:broader skos:related ;
    skos:example "Frank Lloyd Wright work with Aaron G. Green",
        "William Cleare worked with Christopher Wren" ;
    skos:inScheme <http://vocab.getty.edu/ontology>,
        ulan: ;
    skos:notation "1305" ;
    skos:prefLabel "ulan1305_worked_with"@en ;
    skos:topConceptOf <http://vocab.getty.edu/ontology>,
        ulan: .

gvp:ulan1307_assistant_of a owl:ObjectProperty,
        skos:Concept ;
    dc:identifier "1307" ;
    dc:title "assistant of - person" ;
    dct:description """person - assistant of - person.\r
Example: Bernard Castelli was assistant of Pablo Picasso""" ;
    rdfs:domain skos:Concept ;
    rdfs:isDefinedBy <http://vocab.getty.edu/ontology>,
        ulan: ;
    rdfs:range skos:Concept ;
    rdfs:subPropertyOf skos:related ;
    owl:inverseOf gvp:ulan1308_assisted_by ;
    skos:broader skos:related ;
    skos:example "Bernard Castelli was assistant of Pablo Picasso" ;
    skos:inScheme <http://vocab.getty.edu/ontology>,
        ulan: ;
    skos:notation "1307" ;
    skos:prefLabel "ulan1307_assistant_of"@en ;
    skos:topConceptOf <http://vocab.getty.edu/ontology>,
        ulan: .

gvp:ulan1308_assisted_by a owl:ObjectProperty,
        skos:Concept ;
    dc:identifier "1308" ;
    dc:title "assisted by - person" ;
    dct:description """person - assisted by - person.\r
Example: Pablo Picasso was assisted by Bernard Castelli""" ;
    rdfs:domain skos:Concept ;
    rdfs:isDefinedBy <http://vocab.getty.edu/ontology>,
        ulan: ;
    rdfs:range skos:Concept ;
    rdfs:subPropertyOf skos:related ;
    skos:broader skos:related ;
    skos:example "Pablo Picasso was assisted by Bernard Castelli" ;
    skos:inScheme <http://vocab.getty.edu/ontology> ;
    skos:notation "1308" ;
    skos:prefLabel "ulan1308_assisted_by"@en ;
    skos:topConceptOf <http://vocab.getty.edu/ontology> .

gvp:ulan1310_advised_by a owl:ObjectProperty,
        skos:Concept ;
    dc:identifier "1310" ;
    dc:title "advised by - person" ;
    dct:description """person - advised by - person.\r
Example: Henry VIII, King of England was advised by Thomas Cromwell, Earl of Essex""" ;
    rdfs:domain skos:Concept ;
    rdfs:isDefinedBy <http://vocab.getty.edu/ontology>,
        ulan: ;
    rdfs:range skos:Concept ;
    rdfs:subPropertyOf skos:related ;
    skos:broader skos:related ;
    skos:example "Henry VIII, King of England was advised by Thomas Cromwell, Earl of Essex" ;
    skos:inScheme <http://vocab.getty.edu/ontology> ;
    skos:notation "1310" ;
    skos:prefLabel "ulan1310_advised_by"@en ;
    skos:topConceptOf <http://vocab.getty.edu/ontology> .

gvp:ulan1311_partner_of a owl:ObjectProperty,
        owl:SymmetricProperty,
        skos:Concept ;
    dc:identifier "1311" ;
    dc:title "partner of - person" ;
    dct:description """person - partner of - person.\r
Example: Frank Gehry and James Glymph are partners""" ;
    rdfs:domain skos:Concept ;
    rdfs:isDefinedBy <http://vocab.getty.edu/ontology>,
        ulan: ;
    rdfs:range skos:Concept ;
    rdfs:subPropertyOf skos:related ;
    skos:broader skos:related ;
    skos:example "Frank Gehry and James Glymph are partners" ;
    skos:inScheme <http://vocab.getty.edu/ontology>,
        ulan: ;
    skos:notation "1311" ;
    skos:prefLabel "ulan1311_partner_of"@en ;
    skos:topConceptOf <http://vocab.getty.edu/ontology>,
        ulan: .

gvp:ulan1314_partner_was a owl:ObjectProperty,
        skos:Concept ;
    dc:identifier "1314" ;
    dc:title "partner was - person" ;
    dct:description """firm - partner was - person.\r
Example: Louis H. Sullivan and Dankmar Adler were partners in Adler and Sullivan""" ;
    rdfs:domain skos:Concept ;
    rdfs:isDefinedBy <http://vocab.getty.edu/ontology>,
        ulan: ;
    rdfs:range skos:Concept ;
    rdfs:subPropertyOf skos:related ;
    skos:broader skos:related ;
    skos:example "Louis H. Sullivan and Dankmar Adler were partners in Adler and Sullivan" ;
    skos:inScheme <http://vocab.getty.edu/ontology> ;
    skos:notation "1314" ;
    skos:prefLabel "ulan1314_partner_was"@en ;
    skos:topConceptOf <http://vocab.getty.edu/ontology> .

gvp:ulan1315_principal_in a owl:ObjectProperty,
        skos:Concept ;
    dc:identifier "1315" ;
    dc:title "principal in - firm" ;
    dct:description """person - principal in - firm.\r
Example: Principal in Fontana Workshop was Orazio Fontana""" ;
    rdfs:domain skos:Concept ;
    rdfs:isDefinedBy <http://vocab.getty.edu/ontology>,
        ulan: ;
    rdfs:range skos:Concept ;
    rdfs:subPropertyOf skos:related ;
    owl:inverseOf gvp:ulan1316_principal_was ;
    skos:broader skos:related ;
    skos:example "Principal in Fontana Workshop was Orazio Fontana" ;
    skos:inScheme <http://vocab.getty.edu/ontology>,
        ulan: ;
    skos:notation "1315" ;
    skos:prefLabel "ulan1315_principal_in"@en ;
    skos:topConceptOf <http://vocab.getty.edu/ontology>,
        ulan: .

gvp:ulan1317_member_of a owl:ObjectProperty,
        skos:Concept ;
    dc:identifier "1317" ;
    dc:title "member of - person/firm/group" ;
    dct:description """firm/group - member of - person/firm/group.\r
Example: A member of the Foundation of Documents of Architecture is the National Gallery of Art""" ;
    rdfs:domain skos:Concept ;
    rdfs:isDefinedBy <http://vocab.getty.edu/ontology>,
        ulan: ;
    rdfs:range skos:Concept ;
    rdfs:subPropertyOf skos:related ;
    owl:inverseOf gvp:ulan1318_member_was ;
    skos:broader skos:related ;
    skos:example "A member of the Foundation of Documents of Architecture is the National Gallery of Art" ;
    skos:inScheme <http://vocab.getty.edu/ontology>,
        ulan: ;
    skos:notation "1317" ;
    skos:prefLabel "ulan1317_member_of"@en ;
    skos:topConceptOf <http://vocab.getty.edu/ontology>,
        ulan: .

gvp:ulan1321_school_of a owl:ObjectProperty,
        skos:Concept ;
    dc:identifier "1321" ;
    dc:title "school of - firm/group" ;
    dct:description """person - school of - firm/group.\r
Example: The school of Pierre Saalburg was the Architectural Association. School of Architecture""" ;
    rdfs:domain skos:Concept ;
    rdfs:isDefinedBy <http://vocab.getty.edu/ontology>,
        ulan: ;
    rdfs:range skos:Concept ;
    rdfs:subPropertyOf skos:related ;
    owl:inverseOf gvp:ulan1322_school_was ;
    skos:broader skos:related ;
    skos:example "The school of Pierre Saalburg was the Architectural Association. School of Architecture" ;
    skos:inScheme <http://vocab.getty.edu/ontology>,
        ulan: ;
    skos:notation "1321" ;
    skos:prefLabel "ulan1321_school_of"@en ;
    skos:topConceptOf <http://vocab.getty.edu/ontology>,
        ulan: .

gvp:ulan1412_predecessor_of a owl:ObjectProperty,
        skos:Concept ;
    dc:identifier "1412" ;
    dc:title "predecessor of - firm/group" ;
    dct:description """firm/group - predecessor of - firm/group.\r
Example: Richard Meier & Associates is the predecessor of Richard Meier & Partners Architects LLP""" ;
    rdfs:domain skos:Concept ;
    rdfs:isDefinedBy <http://vocab.getty.edu/ontology>,
        ulan: ;
    rdfs:range skos:Concept ;
    rdfs:subPropertyOf skos:related ;
    skos:broader skos:related ;
    skos:example "Richard Meier & Associates is the predecessor of Richard Meier & Partners Architects LLP" ;
    skos:inScheme <http://vocab.getty.edu/ontology> ;
    skos:notation "1412" ;
    skos:prefLabel "ulan1412_predecessor_of"@en ;
    skos:topConceptOf <http://vocab.getty.edu/ontology> .

gvp:ulan1413_administration_overlaps_with a owl:ObjectProperty,
        owl:SymmetricProperty,
        skos:Concept ;
    dc:identifier "1413" ;
    dc:title "administration overlaps with - firm/group" ;
    dct:description """firm/group - administration overlaps with - firm/group.\r
Example: The administration of the Numismatic Collection overlaps with Bode Museum""" ;
    rdfs:domain skos:Concept ;
    rdfs:isDefinedBy <http://vocab.getty.edu/ontology>,
        ulan: ;
    rdfs:range skos:Concept ;
    rdfs:subPropertyOf skos:related ;
    skos:broader skos:related ;
    skos:example "The administration of the Numismatic Collection overlaps with Bode Museum" ;
    skos:inScheme <http://vocab.getty.edu/ontology>,
        ulan: ;
    skos:notation "1413" ;
    skos:prefLabel "ulan1413_administration_overlaps_with"@en ;
    skos:topConceptOf <http://vocab.getty.edu/ontology>,
        ulan: .

gvp:ulan1421_founded_by a owl:ObjectProperty,
        skos:Concept ;
    dc:identifier "1421" ;
    dc:title "founded by - firm/group" ;
    dct:description """firm/group - founded by - firm/group.\r
Example: National Gallery of Art was founded by United States Congress""" ;
    rdfs:domain skos:Concept ;
    rdfs:isDefinedBy <http://vocab.getty.edu/ontology>,
        ulan: ;
    rdfs:range skos:Concept ;
    rdfs:subPropertyOf skos:related ;
    owl:inverseOf gvp:ulan1422_founded ;
    skos:broader skos:related ;
    skos:example "National Gallery of Art was founded by United States Congress" ;
    skos:inScheme <http://vocab.getty.edu/ontology>,
        ulan: ;
    skos:notation "1421" ;
    skos:prefLabel "ulan1421_founded_by"@en ;
    skos:topConceptOf <http://vocab.getty.edu/ontology>,
        ulan: .

gvp:ulan1500_related_to a owl:ObjectProperty,
        owl:SymmetricProperty,
        skos:Concept ;
    dc:identifier "1500" ;
    dc:title "related to - person" ;
    dct:description """person - related to (familial relationship) - person.\r
Example: Titian and Tizianello have a familial relationship with each other""" ;
    rdfs:domain skos:Concept ;
    rdfs:isDefinedBy <http://vocab.getty.edu/ontology>,
        ulan: ;
    rdfs:range skos:Concept ;
    rdfs:subPropertyOf skos:related ;
    skos:broader skos:related ;
    skos:example "Titian and Tizianello have a familial relationship with each other" ;
    skos:inScheme <http://vocab.getty.edu/ontology>,
        ulan: ;
    skos:notation "1500" ;
    skos:prefLabel "ulan1500_related_to"@en ;
    skos:topConceptOf <http://vocab.getty.edu/ontology>,
        ulan: .

gvp:ulan1501_sibling_of a owl:ObjectProperty,
        owl:SymmetricProperty,
        skos:Concept ;
    dc:identifier "1501" ;
    dc:title "sibling of - person" ;
    dct:description """person - sibling of - person.\r
Example: Philippe Rubens is the sibling of Peter Paul Rubens""" ;
    rdfs:domain skos:Concept ;
    rdfs:isDefinedBy <http://vocab.getty.edu/ontology>,
        ulan: ;
    rdfs:range skos:Concept ;
    rdfs:subPropertyOf skos:related ;
    skos:broader skos:related ;
    skos:example "Philippe Rubens is the sibling of Peter Paul Rubens" ;
    skos:inScheme <http://vocab.getty.edu/ontology>,
        ulan: ;
    skos:notation "1501" ;
    skos:prefLabel "ulan1501_sibling_of"@en ;
    skos:topConceptOf <http://vocab.getty.edu/ontology>,
        ulan: .

gvp:ulan1511_child_of a owl:ObjectProperty,
        skos:Concept ;
    dc:identifier "1511" ;
    dc:title "child of - person" ;
    dct:description """person - child of - person.\r
Example: Rembrandt van Rijn is the child of Neeltgen Willemsdr van Zuydtbroeck""" ;
    rdfs:domain skos:Concept ;
    rdfs:isDefinedBy <http://vocab.getty.edu/ontology>,
        ulan: ;
    rdfs:range skos:Concept ;
    rdfs:subPropertyOf skos:related ;
    owl:inverseOf gvp:ulan1512_parent_of ;
    skos:broader skos:related ;
    skos:example "Rembrandt van Rijn is the child of Neeltgen Willemsdr van Zuydtbroeck" ;
    skos:inScheme <http://vocab.getty.edu/ontology>,
        ulan: ;
    skos:notation "1511" ;
    skos:prefLabel "ulan1511_child_of"@en ;
    skos:topConceptOf <http://vocab.getty.edu/ontology>,
        ulan: .

gvp:ulan1512_parent_of a owl:ObjectProperty,
        skos:Concept ;
    dc:identifier "1512" ;
    dc:title "parent of - person" ;
    dct:description """person - parent of - person.\r
Example: Rembrandt van Rijn is the parent of Rumbertus van Rijn""" ;
    rdfs:domain skos:Concept ;
    rdfs:isDefinedBy <http://vocab.getty.edu/ontology>,
        ulan: ;
    rdfs:range skos:Concept ;
    rdfs:subPropertyOf skos:related ;
    skos:broader skos:related ;
    skos:example "Rembrandt van Rijn is the parent of Rumbertus van Rijn" ;
    skos:inScheme <http://vocab.getty.edu/ontology> ;
    skos:notation "1512" ;
    skos:prefLabel "ulan1512_parent_of"@en ;
    skos:topConceptOf <http://vocab.getty.edu/ontology> .

gvp:ulan1514_gandparent_of a owl:ObjectProperty,
        skos:Concept ;
    dc:identifier "1514" ;
    dc:title "gandparent of - person" ;
    dct:description """person - gandparent of - person.\r
Example: Frank Lloyd Wright is the grandparent of Eric Lloyd Wright""" ;
    rdfs:domain skos:Concept ;
    rdfs:isDefinedBy <http://vocab.getty.edu/ontology>,
        ulan: ;
    rdfs:range skos:Concept ;
    rdfs:subPropertyOf skos:related ;
    skos:broader skos:related ;
    skos:example "Frank Lloyd Wright is the grandparent of Eric Lloyd Wright" ;
    skos:inScheme <http://vocab.getty.edu/ontology> ;
    skos:notation "1514" ;
    skos:prefLabel "ulan1514_gandparent_of"@en ;
    skos:topConceptOf <http://vocab.getty.edu/ontology> .

gvp:ulan1515_great-grandparent_of a owl:ObjectProperty,
        skos:Concept ;
    dc:identifier "1515" ;
    dc:title "great-grandparent of - person" ;
    dct:description """person - great-grandparent of - person.\r
Example: Albrecht Adam is the great-grandparent of Richard Benno Adam""" ;
    rdfs:domain skos:Concept ;
    rdfs:isDefinedBy <http://vocab.getty.edu/ontology>,
        ulan: ;
    rdfs:range skos:Concept ;
    rdfs:subPropertyOf skos:related ;
    owl:inverseOf gvp:ulan1516_great-grandchild_of ;
    skos:broader skos:related ;
    skos:example "Albrecht Adam is the great-grandparent of Richard Benno Adam" ;
    skos:inScheme <http://vocab.getty.edu/ontology>,
        ulan: ;
    skos:notation "1515" ;
    skos:prefLabel "ulan1515_great-grandparent_of"@en ;
    skos:topConceptOf <http://vocab.getty.edu/ontology>,
        ulan: .

gvp:ulan1521_cousin_of a owl:ObjectProperty,
        owl:SymmetricProperty,
        skos:Concept ;
    dc:identifier "1521" ;
    dc:title "cousin of - person" ;
    dct:description """person - cousin of - person.\r
Example: Richard Meier and Frank Gehry are cousins""" ;
    rdfs:domain skos:Concept ;
    rdfs:isDefinedBy <http://vocab.getty.edu/ontology>,
        ulan: ;
    rdfs:range skos:Concept ;
    rdfs:subPropertyOf skos:related ;
    skos:broader skos:related ;
    skos:example "Richard Meier and Frank Gehry are cousins" ;
    skos:inScheme <http://vocab.getty.edu/ontology>,
        ulan: ;
    skos:notation "1521" ;
    skos:prefLabel "ulan1521_cousin_of"@en ;
    skos:topConceptOf <http://vocab.getty.edu/ontology>,
        ulan: .

gvp:ulan1531_nephew-niece_of a owl:ObjectProperty,
        skos:Concept ;
    dc:identifier "1531" ;
    dc:title "nephew/niece of - person" ;
    dct:description """person - nephew/niece of - person.\r
Example: Jan Brueghel, the elder is the nephew/neice of  Pieter Coecke van Aeist, the younger""" ;
    rdfs:domain skos:Concept ;
    rdfs:isDefinedBy <http://vocab.getty.edu/ontology>,
        ulan: ;
    rdfs:range skos:Concept ;
    rdfs:subPropertyOf skos:related ;
    owl:inverseOf gvp:ulan1532_uncle-aunt_of ;
    skos:broader skos:related ;
    skos:example "Jan Brueghel, the elder is the nephew/neice of  Pieter Coecke van Aeist, the younger" ;
    skos:inScheme <http://vocab.getty.edu/ontology>,
        ulan: ;
    skos:notation "1531" ;
    skos:prefLabel "ulan1531_nephew-niece_of"@en ;
    skos:topConceptOf <http://vocab.getty.edu/ontology>,
        ulan: .

gvp:ulan1542_consort_of a owl:ObjectProperty,
        skos:Concept ;
    dc:identifier "1542" ;
    dc:title "consort of - person" ;
    dct:description """person - consort of - person.\r
Example: Empress Livia was the consort of Augustus, Emperor of Rome""" ;
    rdfs:domain skos:Concept ;
    rdfs:isDefinedBy <http://vocab.getty.edu/ontology>,
        ulan: ;
    rdfs:range skos:Concept ;
    rdfs:subPropertyOf skos:related ;
    owl:inverseOf gvp:ulan1543_consort_was ;
    skos:broader skos:related ;
    skos:example "Empress Livia was the consort of Augustus, Emperor of Rome" ;
    skos:inScheme <http://vocab.getty.edu/ontology>,
        ulan: ;
    skos:notation "1542" ;
    skos:prefLabel "ulan1542_consort_of"@en ;
    skos:topConceptOf <http://vocab.getty.edu/ontology>,
        ulan: .

gvp:ulan1543_consort_was a owl:ObjectProperty,
        skos:Concept ;
    dc:identifier "1543" ;
    dc:title "consort was - person" ;
    dct:description """person - consort was - person.\r
Example: Augustus, Emperor of Rome's consort was Empress Livia""" ;
    rdfs:domain skos:Concept ;
    rdfs:isDefinedBy <http://vocab.getty.edu/ontology>,
        ulan: ;
    rdfs:range skos:Concept ;
    rdfs:subPropertyOf skos:related ;
    skos:broader skos:related ;
    skos:example "Augustus, Emperor of Rome's consort was Empress Livia" ;
    skos:inScheme <http://vocab.getty.edu/ontology> ;
    skos:notation "1543" ;
    skos:prefLabel "ulan1543_consort_was"@en ;
    skos:topConceptOf <http://vocab.getty.edu/ontology> .

gvp:ulan1544_significant_other_of a owl:ObjectProperty,
        owl:SymmetricProperty,
        skos:Concept ;
    dc:identifier "1544" ;
    dc:title "significant other of - person" ;
    dct:description """person - significant other of - person.\r
Example: Jeanne Hebuterne was the significant other of Amedeo Modigliani""" ;
    rdfs:domain skos:Concept ;
    rdfs:isDefinedBy <http://vocab.getty.edu/ontology>,
        ulan: ;
    rdfs:range skos:Concept ;
    rdfs:subPropertyOf skos:related ;
    skos:broader skos:related ;
    skos:example "Jeanne Hebuterne was the significant other of Amedeo Modigliani" ;
    skos:inScheme <http://vocab.getty.edu/ontology>,
        ulan: ;
    skos:notation "1544" ;
    skos:prefLabel "ulan1544_significant_other_of"@en ;
    skos:topConceptOf <http://vocab.getty.edu/ontology>,
        ulan: .

gvp:ulan1547_romantic_partner_of a owl:ObjectProperty,
        owl:SymmetricProperty,
        skos:Concept ;
    dc:identifier "1547" ;
    dc:title "romantic partner of - person" ;
    dct:description """person - romantic partner of - person.\r
Example: Pablo Picasso and Gaby Lespinasse were romantic partners; Vincent van Gogh and Clasina Hoornik were romantic partners""" ;
    rdfs:domain skos:Concept ;
    rdfs:isDefinedBy <http://vocab.getty.edu/ontology>,
        ulan: ;
    rdfs:range skos:Concept ;
    rdfs:subPropertyOf skos:related ;
    skos:broader skos:related ;
    skos:example "Pablo Picasso and Gaby Lespinasse were romantic partners",
        "Vincent van Gogh and Clasina Hoornik were romantic partners" ;
    skos:inScheme <http://vocab.getty.edu/ontology>,
        ulan: ;
    skos:notation "1547" ;
    skos:prefLabel "ulan1547_romantic_partner_of"@en ;
    skos:topConceptOf <http://vocab.getty.edu/ontology>,
        ulan: .

gvp:ulan1548_domestic_partner_of a owl:ObjectProperty,
        owl:SymmetricProperty,
        skos:Concept ;
    dc:identifier "1548" ;
    dc:title "domestic partner of - person" ;
    dct:description "person - domestic partner of - person" ;
    rdfs:domain skos:Concept ;
    rdfs:isDefinedBy <http://vocab.getty.edu/ontology>,
        ulan: ;
    rdfs:range skos:Concept ;
    rdfs:subPropertyOf skos:related ;
    skos:broader skos:related ;
    skos:inScheme <http://vocab.getty.edu/ontology>,
        ulan: ;
    skos:notation "1548" ;
    skos:prefLabel "ulan1548_domestic_partner_of"@en ;
    skos:topConceptOf <http://vocab.getty.edu/ontology>,
        ulan: .

gvp:ulan1551_sibling_by_marriage_of a owl:ObjectProperty,
        owl:SymmetricProperty,
        skos:Concept ;
    dc:identifier "1551" ;
    dc:title "sibling by marriage of - person" ;
    dct:description """person - sibling by marriage (step sibling) - person.\r
Example: Peter Paul Rubens and Susanne Fourment are siblings by marriage""" ;
    rdfs:domain skos:Concept ;
    rdfs:isDefinedBy <http://vocab.getty.edu/ontology>,
        ulan: ;
    rdfs:range skos:Concept ;
    rdfs:subPropertyOf skos:related ;
    skos:broader skos:related ;
    skos:example "Peter Paul Rubens and Susanne Fourment are siblings by marriage" ;
    skos:inScheme <http://vocab.getty.edu/ontology>,
        ulan: ;
    skos:notation "1551" ;
    skos:prefLabel "ulan1551_sibling_by_marriage_of"@en ;
    skos:topConceptOf <http://vocab.getty.edu/ontology>,
        ulan: .

gvp:ulan1554_adoptive_parent_of a owl:ObjectProperty,
        skos:Concept ;
    dc:identifier "1554" ;
    dc:title "adoptive parent of - person" ;
    dct:description """person - adoptive parent of - person.\r
Example: Julius Caesar is the adoptive parent of Augustus, Emperor of Rome""" ;
    rdfs:domain skos:Concept ;
    rdfs:isDefinedBy <http://vocab.getty.edu/ontology>,
        ulan: ;
    rdfs:range skos:Concept ;
    rdfs:subPropertyOf skos:related ;
    owl:inverseOf gvp:ulan1555_adopted_child_of ;
    skos:broader skos:related ;
    skos:example "Julius Caesar is the adoptive parent of Augustus, Emperor of Rome" ;
    skos:inScheme <http://vocab.getty.edu/ontology>,
        ulan: ;
    skos:notation "1554" ;
    skos:prefLabel "ulan1554_adoptive_parent_of"@en ;
    skos:topConceptOf <http://vocab.getty.edu/ontology>,
        ulan: .

gvp:ulan1555_adopted_child_of a owl:ObjectProperty,
        skos:Concept ;
    dc:identifier "1555" ;
    dc:title "adopted child of - person" ;
    dct:description """person - adopted child of - person.\r
Example: Augusts, Emperor of Rome is the adopted child of Julius Caesar""" ;
    rdfs:domain skos:Concept ;
    rdfs:isDefinedBy <http://vocab.getty.edu/ontology>,
        ulan: ;
    rdfs:range skos:Concept ;
    rdfs:subPropertyOf skos:related ;
    skos:broader skos:related ;
    skos:example "Augusts, Emperor of Rome is the adopted child of Julius Caesar" ;
    skos:inScheme <http://vocab.getty.edu/ontology> ;
    skos:notation "1555" ;
    skos:prefLabel "ulan1555_adopted_child_of"@en ;
    skos:topConceptOf <http://vocab.getty.edu/ontology> .

gvp:ulan1561_step-child_of a owl:ObjectProperty,
        skos:Concept ;
    dc:identifier "1561" ;
    dc:title "step-child of - person" ;
    dct:description """person - step-child of - person.\r
Example: Hortense, Quene consort of Louis Bonaparte is the step-child of Napoleon I, Emperor of the French""" ;
    rdfs:domain skos:Concept ;
    rdfs:isDefinedBy <http://vocab.getty.edu/ontology>,
        ulan: ;
    rdfs:range skos:Concept ;
    rdfs:subPropertyOf skos:related ;
    owl:inverseOf gvp:ulan1562_step-parent_of ;
    skos:broader skos:related ;
    skos:example "Hortense, Quene consort of Louis Bonaparte is the step-child of Napoleon I, Emperor of the French" ;
    skos:inScheme <http://vocab.getty.edu/ontology>,
        ulan: ;
    skos:notation "1561" ;
    skos:prefLabel "ulan1561_step-child_of"@en ;
    skos:topConceptOf <http://vocab.getty.edu/ontology>,
        ulan: .

gvp:ulan1562_step-parent_of a owl:ObjectProperty,
        skos:Concept ;
    dc:identifier "1562" ;
    dc:title "step-parent of - person" ;
    dct:description """person - step-parent of - person.\r
Example: Napoleon I, Emperor of the French is the step-parent of Hortense, Quene consort of Louis Bonaparte""" ;
    rdfs:domain skos:Concept ;
    rdfs:isDefinedBy <http://vocab.getty.edu/ontology>,
        ulan: ;
    rdfs:range skos:Concept ;
    rdfs:subPropertyOf skos:related ;
    skos:broader skos:related ;
    skos:example "Napoleon I, Emperor of the French is the step-parent of Hortense, Quene consort of Louis Bonaparte" ;
    skos:inScheme <http://vocab.getty.edu/ontology> ;
    skos:notation "1562" ;
    skos:prefLabel "ulan1562_step-parent_of"@en ;
    skos:topConceptOf <http://vocab.getty.edu/ontology> .

gvp:ulan1571_guardian_of a owl:ObjectProperty,
        skos:Concept ;
    dc:identifier "1571" ;
    dc:title "guardian of - person" ;
    dct:description """person - guardian of - person.\r
Example: John Hoskins, the elder was the guardian of Samuel Cooper""" ;
    rdfs:domain skos:Concept ;
    rdfs:isDefinedBy <http://vocab.getty.edu/ontology>,
        ulan: ;
    rdfs:range skos:Concept ;
    rdfs:subPropertyOf skos:related ;
    owl:inverseOf gvp:ulan1573_ward_of ;
    skos:broader skos:related ;
    skos:example "John Hoskins, the elder was the guardian of Samuel Cooper" ;
    skos:inScheme <http://vocab.getty.edu/ontology>,
        ulan: ;
    skos:notation "1571" ;
    skos:prefLabel "ulan1571_guardian_of"@en ;
    skos:topConceptOf <http://vocab.getty.edu/ontology>,
        ulan: .

gvp:ulan2550_friend_of a owl:ObjectProperty,
        owl:SymmetricProperty,
        skos:Concept ;
    dc:identifier "2550" ;
    dc:title "friend of - person" ;
    dct:description """person - friend of (personal relationship) - person.\r
Example: Alfred Stieglitz and Frank Simon Herrmann were friends""" ;
    rdfs:domain skos:Concept ;
    rdfs:isDefinedBy <http://vocab.getty.edu/ontology>,
        ulan: ;
    rdfs:range skos:Concept ;
    rdfs:subPropertyOf skos:related ;
    skos:broader skos:related ;
    skos:example "Alfred Stieglitz and Frank Simon Herrmann were friends" ;
    skos:inScheme <http://vocab.getty.edu/ontology>,
        ulan: ;
    skos:notation "2550" ;
    skos:prefLabel "ulan2550_friend_of"@en ;
    skos:topConceptOf <http://vocab.getty.edu/ontology>,
        ulan: .

gvp:ulan2573_founded_by a owl:ObjectProperty,
        skos:Concept ;
    dc:identifier "2573" ;
    dc:title "founded by - person" ;
    dct:description """institution - founded by - person.\r
Example: Tiffany Glass & Decorating Company was founded by Louis Comfort Tiffany""" ;
    rdfs:domain skos:Concept ;
    rdfs:isDefinedBy <http://vocab.getty.edu/ontology>,
        ulan: ;
    rdfs:range skos:Concept ;
    rdfs:subPropertyOf skos:related ;
    skos:broader skos:related ;
    skos:example "Tiffany Glass & Decorating Company was founded by Louis Comfort Tiffany" ;
    skos:inScheme <http://vocab.getty.edu/ontology> ;
    skos:notation "2573" ;
    skos:prefLabel "ulan2573_founded_by"@en ;
    skos:topConceptOf <http://vocab.getty.edu/ontology> .

gvp:ulan2576_patron_of a owl:ObjectProperty,
        skos:Concept ;
    dc:identifier "2576" ;
    dc:title "patron of - person" ;
    dct:description """person - patron of - person.\r
Example: The patron of William Chambers was James Caulfiel, Earl of Charlemont""" ;
    rdfs:domain skos:Concept ;
    rdfs:isDefinedBy <http://vocab.getty.edu/ontology>,
        ulan: ;
    rdfs:range skos:Concept ;
    rdfs:subPropertyOf skos:related ;
    owl:inverseOf gvp:ulan2577_patron_was ;
    skos:broader skos:related ;
    skos:example "The patron of William Chambers was James Caulfiel, Earl of Charlemont" ;
    skos:inScheme <http://vocab.getty.edu/ontology>,
        ulan: ;
    skos:notation "2576" ;
    skos:prefLabel "ulan2576_patron_of"@en ;
    skos:topConceptOf <http://vocab.getty.edu/ontology>,
        ulan: .

gvp:ulan2579_trustee_was a owl:ObjectProperty,
        skos:Concept ;
    dc:identifier "2579" ;
    dc:title "trustee was - person" ;
    dct:description """institution - trustee was - person.\r
Example: National Galleries of Scotland trustee was George Douglas Haig""" ;
    rdfs:domain skos:Concept ;
    rdfs:isDefinedBy <http://vocab.getty.edu/ontology>,
        ulan: ;
    rdfs:range skos:Concept ;
    rdfs:subPropertyOf skos:related ;
    skos:broader skos:related ;
    skos:example "National Galleries of Scotland trustee was George Douglas Haig" ;
    skos:inScheme <http://vocab.getty.edu/ontology> ;
    skos:notation "2579" ;
    skos:prefLabel "ulan2579_trustee_was"@en ;
    skos:topConceptOf <http://vocab.getty.edu/ontology> .

gvp:ulan2581_administrator_of a owl:ObjectProperty,
        skos:Concept ;
    dc:identifier "2581" ;
    dc:title "administrator of - institution" ;
    dct:description """person - administrator of - institution.\r
Example: Georges Mathieu was the administrator of Societe nationale des chemins de fer Francais. Agence des gares""" ;
    rdfs:domain skos:Concept ;
    rdfs:isDefinedBy <http://vocab.getty.edu/ontology>,
        ulan: ;
    rdfs:range skos:Concept ;
    rdfs:subPropertyOf skos:related ;
    owl:inverseOf gvp:ulan2582_administered_by ;
    skos:broader skos:related ;
    skos:example "Georges Mathieu was the administrator of Societe nationale des chemins de fer Francais. Agence des gares" ;
    skos:inScheme <http://vocab.getty.edu/ontology>,
        ulan: ;
    skos:notation "2581" ;
    skos:prefLabel "ulan2581_administrator_of"@en ;
    skos:topConceptOf <http://vocab.getty.edu/ontology>,
        ulan: .

gvp:ulan2582_administered_by a owl:ObjectProperty,
        skos:Concept ;
    dc:identifier "2582" ;
    dc:title "administered by - person" ;
    dct:description """institution - administered by - person.\r
Example: Societe nationale des chemins de fer Francais. Agence des gares was administered by Georges Mathieu""" ;
    rdfs:domain skos:Concept ;
    rdfs:isDefinedBy <http://vocab.getty.edu/ontology>,
        ulan: ;
    rdfs:range skos:Concept ;
    rdfs:subPropertyOf skos:related ;
    skos:broader skos:related ;
    skos:example "Societe nationale des chemins de fer Francais. Agence des gares was administered by Georges Mathieu" ;
    skos:inScheme <http://vocab.getty.edu/ontology> ;
    skos:notation "2582" ;
    skos:prefLabel "ulan2582_administered_by"@en ;
    skos:topConceptOf <http://vocab.getty.edu/ontology> .

gvp:ulan2584_chaired_by a owl:ObjectProperty,
        skos:Concept ;
    dc:identifier "2584" ;
    dc:title "chaired by - person" ;
    dct:description "institution - chaired by - person" ;
    rdfs:domain skos:Concept ;
    rdfs:isDefinedBy <http://vocab.getty.edu/ontology>,
        ulan: ;
    rdfs:range skos:Concept ;
    rdfs:subPropertyOf skos:related ;
    skos:broader skos:related ;
    skos:inScheme <http://vocab.getty.edu/ontology> ;
    skos:notation "2584" ;
    skos:prefLabel "ulan2584_chaired_by"@en ;
    skos:topConceptOf <http://vocab.getty.edu/ontology> .

gvp:ulan2650_publisher_was a owl:ObjectProperty,
        skos:Concept ;
    dc:identifier "2650" ;
    dc:title "publisher was - firm" ;
    dct:description """person - publisher was - firm.\r
Example: The publisher for Pierre Joseph Rossier was Negretti and Zambra""" ;
    rdfs:domain skos:Concept ;
    rdfs:isDefinedBy <http://vocab.getty.edu/ontology>,
        ulan: ;
    rdfs:range skos:Concept ;
    rdfs:subPropertyOf skos:related ;
    owl:inverseOf gvp:ulan2651_publisher_of ;
    skos:broader skos:related ;
    skos:example "The publisher for Pierre Joseph Rossier was Negretti and Zambra" ;
    skos:inScheme <http://vocab.getty.edu/ontology>,
        ulan: ;
    skos:notation "2650" ;
    skos:prefLabel "ulan2650_publisher_was"@en ;
    skos:topConceptOf <http://vocab.getty.edu/ontology>,
        ulan: .

gvp:ulan2676_teacher_at a owl:ObjectProperty,
        skos:Concept ;
    dc:identifier "2676" ;
    dc:title "teacher at - institution" ;
    dct:description """person - teacher at - institution.\r
Example: Willem De Kooning was a teacher at Black Mountain College""" ;
    rdfs:domain skos:Concept ;
    rdfs:isDefinedBy <http://vocab.getty.edu/ontology>,
        ulan: ;
    rdfs:range skos:Concept ;
    rdfs:subPropertyOf skos:related ;
    owl:inverseOf gvp:ulan2677_teacher_was ;
    skos:broader skos:related ;
    skos:example "Willem De Kooning was a teacher at Black Mountain College" ;
    skos:inScheme <http://vocab.getty.edu/ontology>,
        ulan: ;
    skos:notation "2676" ;
    skos:prefLabel "ulan2676_teacher_at"@en ;
    skos:topConceptOf <http://vocab.getty.edu/ontology>,
        ulan: .

gvp:ulan2677_teacher_was a owl:ObjectProperty,
        skos:Concept ;
    dc:identifier "2677" ;
    dc:title "teacher was - person" ;
    dct:description """institution - teacher was - person.\r
Example: A teacher at Black Mountain College was Willem De Kooning""" ;
    rdfs:domain skos:Concept ;
    rdfs:isDefinedBy <http://vocab.getty.edu/ontology>,
        ulan: ;
    rdfs:range skos:Concept ;
    rdfs:subPropertyOf skos:related ;
    skos:broader skos:related ;
    skos:example "A teacher at Black Mountain College was Willem De Kooning" ;
    skos:inScheme <http://vocab.getty.edu/ontology> ;
    skos:notation "2677" ;
    skos:prefLabel "ulan2677_teacher_was"@en ;
    skos:topConceptOf <http://vocab.getty.edu/ontology> .

gvp:ulan2692_president_of a owl:ObjectProperty,
        skos:Concept ;
    dc:identifier "2692" ;
    dc:title "president of - institution" ;
    dct:description """person - president of - institution.\r
Example: David K. E. Bruce was president of National Gallery of Art""" ;
    rdfs:domain skos:Concept ;
    rdfs:isDefinedBy <http://vocab.getty.edu/ontology>,
        ulan: ;
    rdfs:range skos:Concept ;
    rdfs:subPropertyOf skos:related ;
    owl:inverseOf gvp:ulan2693_president_was ;
    skos:broader skos:related ;
    skos:example "David K. E. Bruce was president of National Gallery of Art" ;
    skos:inScheme <http://vocab.getty.edu/ontology>,
        ulan: ;
    skos:notation "2692" ;
    skos:prefLabel "ulan2692_president_of"@en ;
    skos:topConceptOf <http://vocab.getty.edu/ontology>,
        ulan: .

gvp:ulan2693_president_was a owl:ObjectProperty,
        skos:Concept ;
    dc:identifier "2693" ;
    dc:title "president was - person" ;
    dct:description """institution - president was - person.\r
Example: A president of National Gallery of Art was David K. E. Bruce""" ;
    rdfs:domain skos:Concept ;
    rdfs:isDefinedBy <http://vocab.getty.edu/ontology>,
        ulan: ;
    rdfs:range skos:Concept ;
    rdfs:subPropertyOf skos:related ;
    skos:broader skos:related ;
    skos:example "A president of National Gallery of Art was David K. E. Bruce" ;
    skos:inScheme <http://vocab.getty.edu/ontology> ;
    skos:notation "2693" ;
    skos:prefLabel "ulan2693_president_was"@en ;
    skos:topConceptOf <http://vocab.getty.edu/ontology> .

gvp:ulan2697_leader_was a owl:ObjectProperty,
        skos:Concept ;
    dc:identifier "2697" ;
    dc:title "leader was - person" ;
    dct:description """institution - leader was - person.\r
Example: The leader of Samuel H. Kress Foundation was Rush Harrison Kress""" ;
    rdfs:domain skos:Concept ;
    rdfs:isDefinedBy <http://vocab.getty.edu/ontology>,
        ulan: ;
    rdfs:range skos:Concept ;
    rdfs:subPropertyOf skos:related ;
    skos:broader skos:related ;
    skos:example "The leader of Samuel H. Kress Foundation was Rush Harrison Kress" ;
    skos:inScheme <http://vocab.getty.edu/ontology> ;
    skos:notation "2697" ;
    skos:prefLabel "ulan2697_leader_was"@en ;
    skos:topConceptOf <http://vocab.getty.edu/ontology> .

gvp:ulan2779_owned_by a owl:ObjectProperty,
        skos:Concept ;
    dc:identifier "2779" ;
    dc:title "owned by - firm" ;
    dct:description """person - owned by - firm.\r
Example: Walter Scott Lenox was owned by Lenox China Co.""" ;
    rdfs:domain skos:Concept ;
    rdfs:isDefinedBy <http://vocab.getty.edu/ontology>,
        ulan: ;
    rdfs:range skos:Concept ;
    rdfs:subPropertyOf skos:related ;
    skos:broader skos:related ;
    skos:example "Walter Scott Lenox was owned by Lenox China Co." ;
    skos:inScheme <http://vocab.getty.edu/ontology> ;
    skos:notation "2779" ;
    skos:prefLabel "ulan2779_owned_by"@en ;
    skos:topConceptOf <http://vocab.getty.edu/ontology> .

gvp:ulan2794_representative_of a owl:ObjectProperty,
        skos:Concept ;
    dc:identifier "2794" ;
    dc:title "representative of - institution" ;
    dct:description """person - representative of - institution.\r
Example: The Noguch Museum - representative was Isamu Noguchi""" ;
    rdfs:domain skos:Concept ;
    rdfs:isDefinedBy <http://vocab.getty.edu/ontology>,
        ulan: ;
    rdfs:range skos:Concept ;
    rdfs:subPropertyOf skos:related ;
    owl:inverseOf gvp:ulan2795_representative_was ;
    skos:broader skos:related ;
    skos:example "The Noguch Museum - representative was Isamu Noguchi" ;
    skos:inScheme <http://vocab.getty.edu/ontology>,
        ulan: ;
    skos:notation "2794" ;
    skos:prefLabel "ulan2794_representative_of"@en ;
    skos:topConceptOf <http://vocab.getty.edu/ontology>,
        ulan: .

gvp:ulan2795_representative_was a owl:ObjectProperty,
        skos:Concept ;
    dc:identifier "2795" ;
    dc:title "representative was - person" ;
    dct:description """institution - representative was - person.\r
Example: The Noguch Museum - representative was Isamu Noguchi""" ;
    rdfs:domain skos:Concept ;
    rdfs:isDefinedBy <http://vocab.getty.edu/ontology>,
        ulan: ;
    rdfs:range skos:Concept ;
    rdfs:subPropertyOf skos:related ;
    skos:broader skos:related ;
    skos:example "The Noguch Museum - representative was Isamu Noguchi" ;
    skos:inScheme <http://vocab.getty.edu/ontology> ;
    skos:notation "2795" ;
    skos:prefLabel "ulan2795_representative_was"@en ;
    skos:topConceptOf <http://vocab.getty.edu/ontology> .

iso:ThesaurusArray skos:narrower gvp:Hierarchy .

bio:event skos:narrower gvp:eventNonPreferred,
        gvp:eventPreferred .

schema:nationality skos:narrower gvp:nationalityNonPreferred,
        gvp:nationalityPreferred .

gvp:Biography a owl:Class,
        skos:Concept ;
    rdfs:comment """Biography of a ULAN agent (schema:Person|Organization). Depending on the agent, has these fields:
- schema:description: one-line-biography
- gvp:estStart
- schema:birthPlace | foundationLocation, pointing to TGN
- gvp:estEnd
- schema:deathPlace | dissolutionLocation, pointing to TGN
- schema:gender, pointing to AAT (male, female, other)
- dct:contributor
The fields of the preferred biogrpahy are also available in the agent.""" ;
    rdfs:isDefinedBy <http://vocab.getty.edu/ontology> ;
    skos:inScheme <http://vocab.getty.edu/ontology> ;
    skos:topConceptOf <http://vocab.getty.edu/ontology> .

gvp:aat2209_used-located_in a owl:ObjectProperty,
        skos:Concept ;
    dc:identifier "2209" ;
    dc:title "used/located in - locus/setting" ;
    dct:description """things -used/located in -  locus/setting.\r
Example: glassware is used/located in glassworks (buildings); cave paintings are located in caves""" ;
    rdfs:domain skos:Concept ;
    rdfs:isDefinedBy aat:,
        <http://vocab.getty.edu/ontology> ;
    rdfs:range skos:Concept ;
    rdfs:subPropertyOf skos:related ;
    skos:broader skos:related ;
    skos:example "cave paintings are located in caves",
        "glassware is used/located in glassworks (buildings)" ;
    skos:inScheme aat:,
        <http://vocab.getty.edu/ontology> ;
    skos:notation "2209" ;
    skos:prefLabel "aat2209_used-located_in"@en ;
    skos:topConceptOf aat:,
        <http://vocab.getty.edu/ontology> .

gvp:aat2212_produced_by a owl:ObjectProperty,
        skos:Concept ;
    dc:identifier "2212" ;
    dc:title "produced by - things" ;
    dct:description """things - [are] produced by - things/[equipment].\r
Example: stereoscopic photographs are produced by stereoscopic cameras; punchwork is produced by punches (marking tools)""" ;
    rdfs:domain skos:Concept ;
    rdfs:isDefinedBy aat:,
        <http://vocab.getty.edu/ontology> ;
    rdfs:range skos:Concept ;
    rdfs:subPropertyOf skos:related ;
    skos:broader skos:related ;
    skos:example "punchwork is produced by punches (marking tools)",
        "stereoscopic photographs are produced by stereoscopic cameras" ;
    skos:inScheme aat:,
        <http://vocab.getty.edu/ontology> ;
    skos:notation "2212" ;
    skos:prefLabel "aat2212_produced_by"@en ;
    skos:topConceptOf aat:,
        <http://vocab.getty.edu/ontology> .

gvp:aat2216_require a owl:ObjectProperty,
        skos:Concept ;
    dc:identifier "2216" ;
    dc:title "require - things" ;
    dct:description """things - require - things [in order to exist or work].\r
Example: broderie anglaise requires eyelets; compact disc players require compact discs""" ;
    rdfs:domain skos:Concept ;
    rdfs:isDefinedBy aat:,
        <http://vocab.getty.edu/ontology> ;
    rdfs:range skos:Concept ;
    rdfs:subPropertyOf skos:related ;
    skos:broader skos:related ;
    skos:example "broderie anglaise requires eyelets",
        "compact disc players require compact discs" ;
    skos:inScheme aat:,
        <http://vocab.getty.edu/ontology> ;
    skos:notation "2216" ;
    skos:prefLabel "aat2216_require"@en ;
    skos:topConceptOf aat:,
        <http://vocab.getty.edu/ontology> .

gvp:aat2286_practice-study a owl:ObjectProperty,
        skos:Concept ;
    dc:identifier "2286" ;
    dc:title "practice/study - field/discipline" ;
    dct:description """[actor having] role - practice/study - field [of study, genre]/discipline.\r
Example: Egyptologists practice/study Egyptology; architectural historians practice/study architectural history""" ;
    rdfs:domain skos:Concept ;
    rdfs:isDefinedBy aat:,
        <http://vocab.getty.edu/ontology> ;
    rdfs:range skos:Concept ;
    rdfs:subPropertyOf skos:related ;
    skos:broader skos:related ;
    skos:example "Egyptologists practice/study Egyptology",
        "architectural historians practice/study architectural history" ;
    skos:inScheme aat:,
        <http://vocab.getty.edu/ontology> ;
    skos:notation "2286" ;
    skos:prefLabel "aat2286_practice-study"@en ;
    skos:topConceptOf aat:,
        <http://vocab.getty.edu/ontology> .

gvp:aat2316_use a owl:ObjectProperty,
        skos:Concept ;
    dc:identifier "2316" ;
    dc:title "use - material" ;
    dct:description """[actors having] role - use - material.\r
Example: lapidaries use precious stone; braziers (metalworkers) use brass (alloy)""" ;
    rdfs:domain skos:Concept ;
    rdfs:isDefinedBy aat:,
        <http://vocab.getty.edu/ontology> ;
    rdfs:range skos:Concept ;
    rdfs:subPropertyOf skos:related ;
    skos:broader skos:related ;
    skos:example "braziers (metalworkers) use brass (alloy)",
        "lapidaries use precious stone" ;
    skos:inScheme aat:,
        <http://vocab.getty.edu/ontology> ;
    skos:notation "2316" ;
    skos:prefLabel "aat2316_use"@en ;
    skos:topConceptOf aat:,
        <http://vocab.getty.edu/ontology> .

gvp:aat2333_have_affiliates a owl:ObjectProperty,
        skos:Concept ;
    dc:identifier "2333" ;
    dc:title "have affiliates - role" ;
    dct:description """role [organizations] - have affiliates - [actors having] role.\r
Example: schools (organizations) have as affiliates students; duchies have as affiliates dukes""" ;
    rdfs:domain skos:Concept ;
    rdfs:isDefinedBy aat:,
        <http://vocab.getty.edu/ontology> ;
    rdfs:range skos:Concept ;
    rdfs:subPropertyOf skos:related ;
    skos:broader skos:related ;
    skos:example "duchies have as affiliates dukes",
        "schools (organizations) have as affiliates students" ;
    skos:inScheme aat:,
        <http://vocab.getty.edu/ontology> ;
    skos:notation "2333" ;
    skos:prefLabel "aat2333_have_affiliates"@en ;
    skos:topConceptOf aat:,
        <http://vocab.getty.edu/ontology> .

gvp:aat2419_used_for a owl:ObjectProperty,
        skos:Concept ;
    dc:identifier "2419" ;
    dc:title "used for - field/discipline" ;
    dct:description """things/[equipment] - [are] used for - field [of study]/discipline.\r
Example: astronomical instruments are used for astronomy; divination objects are used for divination [discipline]""" ;
    rdfs:domain skos:Concept ;
    rdfs:isDefinedBy aat:,
        <http://vocab.getty.edu/ontology> ;
    rdfs:range skos:Concept ;
    rdfs:subPropertyOf skos:related ;
    skos:broader skos:related ;
    skos:example "astronomical instruments are used for astronomy",
        "divination objects are used for divination [discipline]" ;
    skos:inScheme aat:,
        <http://vocab.getty.edu/ontology> ;
    skos:notation "2419" ;
    skos:prefLabel "aat2419_used_for"@en ;
    skos:topConceptOf aat:,
        <http://vocab.getty.edu/ontology> .

gvp:aat2422_takes_place_in a owl:ObjectProperty,
        skos:Concept ;
    dc:identifier "2422" ;
    dc:title "takes place in - locus/setting" ;
    dct:description """activity/event/[process/function] - takes place in - locus/setting.\r
Example: smelting takes place in smelters (metalworking plants); pilgrimages take place in pilgrimage centers""" ;
    rdfs:domain skos:Concept ;
    rdfs:isDefinedBy aat:,
        <http://vocab.getty.edu/ontology> ;
    rdfs:range skos:Concept ;
    rdfs:subPropertyOf skos:related ;
    skos:broader skos:related ;
    skos:example "pilgrimages take place in pilgrimage centers",
        "smelting takes place in smelters (metalworking plants)" ;
    skos:inScheme aat:,
        <http://vocab.getty.edu/ontology> ;
    skos:notation "2422" ;
    skos:prefLabel "aat2422_takes_place_in"@en ;
    skos:topConceptOf aat:,
        <http://vocab.getty.edu/ontology> .

gvp:aat2428_produces a owl:ObjectProperty,
        skos:Concept ;
    dc:identifier "2428" ;
    dc:title "produces - things" ;
    dct:description """activity/event/process - produces - things.\r
Example: vase painting (image making) produces vase paintings (visual works); forging (copying) produces forgeries""" ;
    rdfs:domain skos:Concept ;
    rdfs:isDefinedBy aat:,
        <http://vocab.getty.edu/ontology> ;
    rdfs:range skos:Concept ;
    rdfs:subPropertyOf skos:related ;
    skos:broader skos:related ;
    skos:example "forging (copying) produces forgeries",
        "vase painting (image making) produces vase paintings (visual works)" ;
    skos:inScheme aat:,
        <http://vocab.getty.edu/ontology> ;
    skos:notation "2428" ;
    skos:prefLabel "aat2428_produces"@en ;
    skos:topConceptOf aat:,
        <http://vocab.getty.edu/ontology> .

gvp:aat2432_requires a owl:ObjectProperty,
        skos:Concept ;
    dc:identifier "2432" ;
    dc:title "requires - things" ;
    dct:description """activity/event/process - requires - things/equipment.\r
Example: painting (image making) requires painting equipment; doweling requires dowels""" ;
    rdfs:domain skos:Concept ;
    rdfs:isDefinedBy aat:,
        <http://vocab.getty.edu/ontology> ;
    rdfs:range skos:Concept ;
    rdfs:subPropertyOf skos:related ;
    skos:broader skos:related ;
    skos:example "doweling requires dowels",
        "painting (image making) requires painting equipment" ;
    skos:inScheme aat:,
        <http://vocab.getty.edu/ontology> ;
    skos:notation "2432" ;
    skos:prefLabel "aat2432_requires"@en ;
    skos:topConceptOf aat:,
        <http://vocab.getty.edu/ontology> .

gvp:aat2555_reflected_in a owl:ObjectProperty,
        skos:Concept ;
    dc:identifier "2555" ;
    dc:title "reflected in - activity/event" ;
    dct:description """style/period/culture /[religion/ideology] - [is] reflected in activity/event.\r
Example: Dhokra (culture) is reflected in dhokra (casting technique); Red-figure [style] is reflected in red-figure vase painting""" ;
    rdfs:domain skos:Concept ;
    rdfs:isDefinedBy aat:,
        <http://vocab.getty.edu/ontology> ;
    rdfs:range skos:Concept ;
    rdfs:subPropertyOf skos:related ;
    skos:broader skos:related ;
    skos:example "Dhokra (culture) is reflected in dhokra (casting technique)",
        "Red-figure [style] is reflected in red-figure vase painting" ;
    skos:inScheme aat:,
        <http://vocab.getty.edu/ontology> ;
    skos:notation "2555" ;
    skos:prefLabel "aat2555_reflected_in"@en ;
    skos:topConceptOf aat:,
        <http://vocab.getty.edu/ontology> .

gvp:aat2558_reflected_in a owl:ObjectProperty,
        skos:Concept ;
    dc:identifier "2558" ;
    dc:title "reflected in - field/discipline" ;
    dct:description """style/period/culture /[religion/ideology] - [is] reflected in field/discipline.\r
Example: Buddhism is reflected in bugatu [dance discipline]; Christianity is reflected in church history; Ancient Greek [culture] is reflected in classics (discipline)""" ;
    rdfs:domain skos:Concept ;
    rdfs:isDefinedBy aat:,
        <http://vocab.getty.edu/ontology> ;
    rdfs:range skos:Concept ;
    rdfs:subPropertyOf skos:related ;
    skos:broader skos:related ;
    skos:example "Ancient Greek [culture] is reflected in classics (discipline)",
        "Buddhism is reflected in bugatu [dance discipline]",
        "Christianity is reflected in church history" ;
    skos:inScheme aat:,
        <http://vocab.getty.edu/ontology> ;
    skos:notation "2558" ;
    skos:prefLabel "aat2558_reflected_in"@en ;
    skos:topConceptOf aat:,
        <http://vocab.getty.edu/ontology> .

gvp:aat2602_possess-exist_in a owl:ObjectProperty,
        skos:Concept ;
    dc:identifier "2602" ;
    dc:title "possess/exist in - attributes /associated concepts" ;
    dct:description """role [of actors] - possess/exist in - attributes /associated concepts.\r
Example: adults possess/exist in adulthood; nomads possess/exist in [state of] nomadism""" ;
    rdfs:domain skos:Concept ;
    rdfs:isDefinedBy aat:,
        <http://vocab.getty.edu/ontology> ;
    rdfs:range skos:Concept ;
    rdfs:subPropertyOf skos:related ;
    skos:broader skos:related ;
    skos:example "adults possess/exist in adulthood",
        "nomads possess/exist in [state of] nomadism" ;
    skos:inScheme aat:,
        <http://vocab.getty.edu/ontology> ;
    skos:notation "2602" ;
    skos:prefLabel "aat2602_possess-exist_in"@en ;
    skos:topConceptOf aat:,
        <http://vocab.getty.edu/ontology> .

gvp:aat2613_possess-exist_in a owl:ObjectProperty,
        skos:Concept ;
    dc:identifier "2613" ;
    dc:title "possess/exist in - attributes /associated concepts" ;
    dct:description """material - possesses/exists in - condition/state/[property].\r
Example: wood(plant material) possesses/exists in [condition of] dry rot; dielectric (material) possesses/exists in dielectric properties""" ;
    rdfs:domain skos:Concept ;
    rdfs:isDefinedBy aat:,
        <http://vocab.getty.edu/ontology> ;
    rdfs:range skos:Concept ;
    rdfs:subPropertyOf skos:related ;
    skos:broader skos:related ;
    skos:example "dielectric (material) possesses/exists in dielectric properties",
        "wood(plant material) possesses/exists in [condition of] dry rot" ;
    skos:inScheme aat:,
        <http://vocab.getty.edu/ontology> ;
    skos:notation "2613" ;
    skos:prefLabel "aat2613_possess-exist_in"@en ;
    skos:topConceptOf aat:,
        <http://vocab.getty.edu/ontology> .

gvp:aat2806_provide_context a owl:ObjectProperty,
        skos:Concept ;
    dc:identifier "2806" ;
    dc:title "provide context - things" ;
    dct:description """[larger] things - provide context [for] - [smaller] things.\r
Example: altarpieces provide context for predellas; books provide context for chapters""" ;
    rdfs:domain skos:Concept ;
    rdfs:isDefinedBy aat:,
        <http://vocab.getty.edu/ontology> ;
    rdfs:range skos:Concept ;
    rdfs:subPropertyOf skos:related ;
    skos:broader skos:related ;
    skos:example "altarpieces provide context for predellas",
        "books provide context for chapters" ;
    skos:inScheme aat:,
        <http://vocab.getty.edu/ontology> ;
    skos:notation "2806" ;
    skos:prefLabel "aat2806_provide_context"@en ;
    skos:topConceptOf aat:,
        <http://vocab.getty.edu/ontology> .

gvp:aat2812_followed a owl:ObjectProperty,
        skos:Concept ;
    dc:identifier "2812" ;
    dc:title "followed - style/period/culture" ;
    dct:description """style/period/culture/[religion/ideology] - followed  - style/period/culture/[religion/ideology].\r
Example: Abstract Impressionism followed Impressionist; Micoquian followed Acheulian""" ;
    rdfs:domain skos:Concept ;
    rdfs:isDefinedBy aat:,
        <http://vocab.getty.edu/ontology> ;
    rdfs:range skos:Concept ;
    rdfs:subPropertyOf skos:related ;
    skos:broader skos:related ;
    skos:example "Abstract Impressionism followed Impressionist",
        "Micoquian followed Acheulian" ;
    skos:inScheme aat:,
        <http://vocab.getty.edu/ontology> ;
    skos:notation "2812" ;
    skos:prefLabel "aat2812_followed"@en ;
    skos:topConceptOf aat:,
        <http://vocab.getty.edu/ontology> .

gvp:aat2815_composed_of a owl:ObjectProperty,
        skos:Concept ;
    dc:identifier "2815" ;
    dc:title "composed of - material" ;
    dct:description """material - [is] composed of - material.\r
Example: composite white is composed of titanium white; desert varnish is composed of iron oxide""" ;
    rdfs:domain skos:Concept ;
    rdfs:isDefinedBy aat:,
        <http://vocab.getty.edu/ontology> ;
    rdfs:range skos:Concept ;
    rdfs:subPropertyOf skos:related ;
    skos:broader skos:related ;
    skos:example "composite white is composed of titanium white",
        "desert varnish is composed of iron oxide" ;
    skos:inScheme aat:,
        <http://vocab.getty.edu/ontology> ;
    skos:notation "2815" ;
    skos:prefLabel "aat2815_composed_of"@en ;
    skos:topConceptOf aat:,
        <http://vocab.getty.edu/ontology> .

gvp:aat2829_used-required_for a owl:ObjectProperty,
        skos:Concept ;
    dc:identifier "2829" ;
    dc:title "used/required for - things" ;
    dct:description """material - [is] required/used for - things.\r
Example: varnish is used/required for oil paintings; wine is required/used for wine glasses""" ;
    rdfs:domain skos:Concept ;
    rdfs:isDefinedBy aat:,
        <http://vocab.getty.edu/ontology> ;
    rdfs:range skos:Concept ;
    rdfs:subPropertyOf skos:related ;
    skos:broader skos:related ;
    skos:example "varnish is used/required for oil paintings",
        "wine is required/used for wine glasses" ;
    skos:inScheme aat:,
        <http://vocab.getty.edu/ontology> ;
    skos:notation "2829" ;
    skos:prefLabel "aat2829_used-required_for"@en ;
    skos:topConceptOf aat:,
        <http://vocab.getty.edu/ontology> .

gvp:aat2837_source_for a owl:ObjectProperty,
        skos:Concept ;
    dc:identifier "2837" ;
    dc:title "source for - things" ;
    dct:description """genus/species [or its parts] - [is] source for - things.\r
Example: Phormium tenax (species) is the source for k?kaku; Struthio camelus(species) is the source for ostrich-egg cups""" ;
    rdfs:domain skos:Concept ;
    rdfs:isDefinedBy aat:,
        <http://vocab.getty.edu/ontology> ;
    rdfs:range skos:Concept ;
    rdfs:subPropertyOf skos:related ;
    skos:broader skos:related ;
    skos:example "Phormium tenax (species) is the source for k?kaku",
        "Struthio camelus(species) is the source for ostrich-egg cups" ;
    skos:inScheme aat:,
        <http://vocab.getty.edu/ontology> ;
    skos:notation "2837" ;
    skos:prefLabel "aat2837_source_for"@en ;
    skos:topConceptOf aat:,
        <http://vocab.getty.edu/ontology> .

gvp:aat2842_source_for a owl:ObjectProperty,
        skos:Concept ;
    dc:identifier "2842" ;
    dc:title "source for - material" ;
    dct:description """genus/species - [is] source for - material.\r
Example: Vicugna pacos (species) is the source for alpaca (wool); Acer (genus) is the source for maple (wood)""" ;
    rdfs:domain skos:Concept ;
    rdfs:isDefinedBy aat:,
        <http://vocab.getty.edu/ontology> ;
    rdfs:range skos:Concept ;
    rdfs:subPropertyOf skos:related ;
    skos:broader skos:related ;
    skos:example "Acer (genus) is the source for maple (wood)",
        "Vicugna pacos (species) is the source for alpaca (wool)" ;
    skos:inScheme aat:,
        <http://vocab.getty.edu/ontology> ;
    skos:notation "2842" ;
    skos:prefLabel "aat2842_source_for"@en ;
    skos:topConceptOf aat:,
        <http://vocab.getty.edu/ontology> .

gvp:aat2849_involves a owl:ObjectProperty,
        skos:Concept ;
    dc:identifier "2849" ;
    dc:title "involves - genus/species" ;
    dct:description """activity/event - involves - genus/species.\r
Example: bullfighting involves bulls (animals); polo (field sport) involves Equus caballus (species)""" ;
    rdfs:domain skos:Concept ;
    rdfs:isDefinedBy aat:,
        <http://vocab.getty.edu/ontology> ;
    rdfs:range skos:Concept ;
    rdfs:subPropertyOf skos:related ;
    skos:broader skos:related ;
    skos:example "bullfighting involves bulls (animals)",
        "polo (field sport) involves Equus caballus (species)" ;
    skos:inScheme aat:,
        <http://vocab.getty.edu/ontology> ;
    skos:notation "2849" ;
    skos:prefLabel "aat2849_involves"@en ;
    skos:topConceptOf aat:,
        <http://vocab.getty.edu/ontology> .

gvp:aat2876_characterized_by a owl:ObjectProperty,
        skos:Concept ;
    dc:identifier "2876" ;
    dc:title "characterized by - language" ;
    dct:description """style/period/culture - [is] characterized by - language.\r
Example: Afar (culture) is characterized by Afar (language); Celtic (culture) is characterized by Celtic (language)""" ;
    rdfs:domain skos:Concept ;
    rdfs:isDefinedBy aat:,
        <http://vocab.getty.edu/ontology> ;
    rdfs:range skos:Concept ;
    rdfs:subPropertyOf skos:related ;
    skos:broader skos:related ;
    skos:example "Afar (culture) is characterized by Afar (language)",
        "Celtic (culture) is characterized by Celtic (language)" ;
    skos:inScheme aat:,
        <http://vocab.getty.edu/ontology> ;
    skos:notation "2876" ;
    skos:prefLabel "aat2876_characterized_by"@en ;
    skos:topConceptOf aat:,
        <http://vocab.getty.edu/ontology> .

gvp:aat2882_reflect a owl:ObjectProperty,
        skos:Concept ;
    dc:identifier "2882" ;
    dc:title "reflect - language" ;
    dct:description """things - reflect - language.\r
Example: Greek alphabet reflects Greek (language); Vedas reflect Sanskrit""" ;
    rdfs:domain skos:Concept ;
    rdfs:isDefinedBy aat:,
        <http://vocab.getty.edu/ontology> ;
    rdfs:range skos:Concept ;
    rdfs:subPropertyOf skos:related ;
    skos:broader skos:related ;
    skos:example "Greek alphabet reflects Greek (language)",
        "Vedas reflect Sanskrit" ;
    skos:inScheme aat:,
        <http://vocab.getty.edu/ontology> ;
    skos:notation "2882" ;
    skos:prefLabel "aat2882_reflect"@en ;
    skos:topConceptOf aat:,
        <http://vocab.getty.edu/ontology> .

gvp:aat2885_involves a owl:ObjectProperty,
        skos:Concept ;
    dc:identifier "2885" ;
    dc:title "involves - attributes /associated concepts" ;
    dct:description """any - involves - attributes /associated concepts.\r
Example: climate change involves climate;  infestation involves insect damage; Celtic culture involves Celtic crosses (design motif)""" ;
    rdfs:domain skos:Concept ;
    rdfs:isDefinedBy aat:,
        <http://vocab.getty.edu/ontology> ;
    rdfs:range skos:Concept ;
    rdfs:subPropertyOf skos:related ;
    skos:broader skos:related ;
    skos:example "Celtic culture involves Celtic crosses (design motif)",
        "climate change involves climate",
        "infestation involves insect damage" ;
    skos:inScheme aat:,
        <http://vocab.getty.edu/ontology> ;
    skos:notation "2885" ;
    skos:prefLabel "aat2885_involves"@en ;
    skos:topConceptOf aat:,
        <http://vocab.getty.edu/ontology> .

gvp:aat2892_example_of a owl:ObjectProperty,
        skos:Concept ;
    dc:identifier "2892" ;
    dc:title "example of - things" ;
    dct:description """brand name - [is] example of - things.\r
Example: Pictrography (TM) prints are examples of photothermographic transfer prints""" ;
    rdfs:domain skos:Concept ;
    rdfs:isDefinedBy aat:,
        <http://vocab.getty.edu/ontology> ;
    rdfs:range skos:Concept ;
    rdfs:subPropertyOf skos:related ;
    skos:broader skos:related ;
    skos:example "Pictrography (TM) prints are examples of photothermographic transfer prints" ;
    skos:inScheme aat:,
        <http://vocab.getty.edu/ontology> ;
    skos:notation "2892" ;
    skos:prefLabel "aat2892_example_of"@en ;
    skos:topConceptOf aat:,
        <http://vocab.getty.edu/ontology> .

gvp:tgn3104_is_location_of a owl:ObjectProperty,
        skos:Concept ;
    dc:identifier "3104" ;
    dc:title "is location of - place" ;
    dct:description """place - is location of - place.\r
Example: tgn:7031416 Silk Road is location of tgn:7018835 Palmyra""" ;
    rdfs:domain skos:Concept ;
    rdfs:isDefinedBy <http://vocab.getty.edu/ontology>,
        tgn: ;
    rdfs:range skos:Concept ;
    rdfs:subPropertyOf skos:related ;
    skos:broader skos:related ;
    skos:example "tgn:7031416 Silk Road is location of tgn:7018835 Palmyra" ;
    skos:inScheme <http://vocab.getty.edu/ontology>,
        tgn: ;
    skos:notation "3104" ;
    skos:prefLabel "tgn3104_is_location_of"@en ;
    skos:topConceptOf <http://vocab.getty.edu/ontology>,
        tgn: .

gvp:tgn3318_member_is a owl:ObjectProperty,
        skos:Concept ;
    dc:identifier "3318" ;
    dc:title "member is - nation" ;
    dct:description """union - member is - nation.\r
Example: Austria is a member of the European Union since 1915; Belgium is a member of the European Union since 1958""" ;
    rdfs:domain skos:Concept ;
    rdfs:isDefinedBy <http://vocab.getty.edu/ontology>,
        tgn: ;
    rdfs:range skos:Concept ;
    rdfs:subPropertyOf skos:related ;
    skos:broader skos:related ;
    skos:example "Austria is a member of the European Union since 1915",
        "Belgium is a member of the European Union since 1958" ;
    skos:inScheme <http://vocab.getty.edu/ontology>,
        tgn: ;
    skos:notation "3318" ;
    skos:prefLabel "tgn3318_member_is"@en ;
    skos:topConceptOf <http://vocab.getty.edu/ontology>,
        tgn: .

gvp:tgn3402_moved_to a owl:ObjectProperty,
        skos:Concept ;
    dc:identifier "3402" ;
    dc:title "moved to - place" ;
    dct:description """place - moved to - place.\r
Example: Valdosta (Lowndes county, Georgia, USA) moved from Troupville (Georgia, USA)""" ;
    rdfs:domain skos:Concept ;
    rdfs:isDefinedBy <http://vocab.getty.edu/ontology>,
        tgn: ;
    rdfs:range skos:Concept ;
    rdfs:subPropertyOf skos:related ;
    skos:broader skos:related ;
    skos:example "Valdosta (Lowndes county, Georgia, USA) moved from Troupville (Georgia, USA)" ;
    skos:inScheme <http://vocab.getty.edu/ontology>,
        tgn: ;
    skos:notation "3402" ;
    skos:prefLabel "tgn3402_moved_to"@en ;
    skos:topConceptOf <http://vocab.getty.edu/ontology>,
        tgn: .

gvp:tgn3612_administrative_entity_for a owl:ObjectProperty,
        skos:Concept ;
    dc:identifier "3612" ;
    dc:title "administrative entity for - place" ;
    dct:description """place - administrative entity for - place.\r
Example: Ortonovo (Massa-Carra province, Tuscany, Italy) is the administrative entity for Luni (La Spezia province, Liguria, Italy)""" ;
    rdfs:domain skos:Concept ;
    rdfs:isDefinedBy <http://vocab.getty.edu/ontology>,
        tgn: ;
    rdfs:range skos:Concept ;
    rdfs:subPropertyOf skos:related ;
    skos:broader skos:related ;
    skos:example "Ortonovo (Massa-Carra province, Tuscany, Italy) is the administrative entity for Luni (La Spezia province, Liguria, Italy)" ;
    skos:inScheme <http://vocab.getty.edu/ontology>,
        tgn: ;
    skos:notation "3612" ;
    skos:prefLabel "tgn3612_administrative_entity_for"@en ;
    skos:topConceptOf <http://vocab.getty.edu/ontology>,
        tgn: .

gvp:ulan1102_student_of a owl:ObjectProperty,
        skos:Concept ;
    dc:identifier "1102" ;
    dc:title "student of - person" ;
    dct:description """person - student of - person.\r
Example: Pierre Subleyras was the student of Rivalz, Antoine""" ;
    rdfs:domain skos:Concept ;
    rdfs:isDefinedBy <http://vocab.getty.edu/ontology>,
        ulan: ;
    rdfs:range skos:Concept ;
    rdfs:subPropertyOf skos:related ;
    skos:broader skos:related ;
    skos:example "Pierre Subleyras was the student of Rivalz, Antoine" ;
    skos:inScheme <http://vocab.getty.edu/ontology>,
        ulan: ;
    skos:notation "1102" ;
    skos:prefLabel "ulan1102_student_of"@en ;
    skos:topConceptOf <http://vocab.getty.edu/ontology>,
        ulan: .

gvp:ulan1106_apprentice_was a owl:ObjectProperty,
        skos:Concept ;
    dc:identifier "1106" ;
    dc:title "apprentice was - person" ;
    dct:description """person - apprentice was - person.\r
Example: Nicolas Hawksmoor was the apprentice of Christopher Wren""" ;
    rdfs:domain skos:Concept ;
    rdfs:isDefinedBy <http://vocab.getty.edu/ontology>,
        ulan: ;
    rdfs:range skos:Concept ;
    rdfs:subPropertyOf skos:related ;
    skos:broader skos:related ;
    skos:example "Nicolas Hawksmoor was the apprentice of Christopher Wren" ;
    skos:inScheme <http://vocab.getty.edu/ontology>,
        ulan: ;
    skos:notation "1106" ;
    skos:prefLabel "ulan1106_apprentice_was"@en ;
    skos:topConceptOf <http://vocab.getty.edu/ontology>,
        ulan: .

gvp:ulan1108_influenced_by a owl:ObjectProperty,
        skos:Concept ;
    dc:identifier "1108" ;
    dc:title "influenced by - person" ;
    dct:description """person - influenced by - person.\r
Example: Salomon Koninck was influenced by Rembrandt van Rijn""" ;
    rdfs:domain skos:Concept ;
    rdfs:isDefinedBy <http://vocab.getty.edu/ontology>,
        ulan: ;
    rdfs:range skos:Concept ;
    rdfs:subPropertyOf skos:related ;
    skos:broader skos:related ;
    skos:example "Salomon Koninck was influenced by Rembrandt van Rijn" ;
    skos:inScheme <http://vocab.getty.edu/ontology>,
        ulan: ;
    skos:notation "1108" ;
    skos:prefLabel "ulan1108_influenced_by"@en ;
    skos:topConceptOf <http://vocab.getty.edu/ontology>,
        ulan: .

gvp:ulan1112_master_was a owl:ObjectProperty,
        skos:Concept ;
    dc:identifier "1112" ;
    dc:title "master was - person" ;
    dct:description """person - master was - person.\r
Example: Peter Paul Rubens - master of Jan Thomas""" ;
    rdfs:domain skos:Concept ;
    rdfs:isDefinedBy <http://vocab.getty.edu/ontology>,
        ulan: ;
    rdfs:range skos:Concept ;
    rdfs:subPropertyOf skos:related ;
    skos:broader skos:related ;
    skos:example "Peter Paul Rubens - master of Jan Thomas" ;
    skos:inScheme <http://vocab.getty.edu/ontology>,
        ulan: ;
    skos:notation "1112" ;
    skos:prefLabel "ulan1112_master_was"@en ;
    skos:topConceptOf <http://vocab.getty.edu/ontology>,
        ulan: .

gvp:ulan1222_appointee_of a owl:ObjectProperty,
        skos:Concept ;
    dc:identifier "1222" ;
    dc:title "appointee of - person" ;
    dct:description """person - appointee of - person.\r
Example: Virginio Cesarini was appointee by Pope Urban VIII""" ;
    rdfs:domain skos:Concept ;
    rdfs:isDefinedBy <http://vocab.getty.edu/ontology>,
        ulan: ;
    rdfs:range skos:Concept ;
    rdfs:subPropertyOf skos:related ;
    skos:broader skos:related ;
    skos:example "Virginio Cesarini was appointee by Pope Urban VIII" ;
    skos:inScheme <http://vocab.getty.edu/ontology>,
        ulan: ;
    skos:notation "1222" ;
    skos:prefLabel "ulan1222_appointee_of"@en ;
    skos:topConceptOf <http://vocab.getty.edu/ontology>,
        ulan: .

gvp:ulan1224_crowned a owl:ObjectProperty,
        skos:Concept ;
    dc:identifier "1224" ;
    dc:title "crowned - person" ;
    dct:description """person - crowned - person.\r
Example: Emperor Charlemagne was crowned by Pope Leo III""" ;
    rdfs:domain skos:Concept ;
    rdfs:isDefinedBy <http://vocab.getty.edu/ontology>,
        ulan: ;
    rdfs:range skos:Concept ;
    rdfs:subPropertyOf skos:related ;
    skos:broader skos:related ;
    skos:example "Emperor Charlemagne was crowned by Pope Leo III" ;
    skos:inScheme <http://vocab.getty.edu/ontology>,
        ulan: ;
    skos:notation "1224" ;
    skos:prefLabel "ulan1224_crowned"@en ;
    skos:topConceptOf <http://vocab.getty.edu/ontology>,
        ulan: .

gvp:ulan1316_principal_was a owl:ObjectProperty,
        skos:Concept ;
    dc:identifier "1316" ;
    dc:title "principal was - person" ;
    dct:description """firm - principal was - person.\r
Example: Orazio Fontana was principal in Fontana Workshop""" ;
    rdfs:domain skos:Concept ;
    rdfs:isDefinedBy <http://vocab.getty.edu/ontology>,
        ulan: ;
    rdfs:range skos:Concept ;
    rdfs:subPropertyOf skos:related ;
    skos:broader skos:related ;
    skos:example "Orazio Fontana was principal in Fontana Workshop" ;
    skos:inScheme <http://vocab.getty.edu/ontology>,
        ulan: ;
    skos:notation "1316" ;
    skos:prefLabel "ulan1316_principal_was"@en ;
    skos:topConceptOf <http://vocab.getty.edu/ontology>,
        ulan: .

gvp:ulan1318_member_was a owl:ObjectProperty,
        skos:Concept ;
    dc:identifier "1318" ;
    dc:title "member was - firm/group" ;
    dct:description """person/firm/group - member was - firm/group.\r
Example: The National Gallery of Art was/is a member of the Foundation of Documentation of Architecture""" ;
    rdfs:domain skos:Concept ;
    rdfs:isDefinedBy <http://vocab.getty.edu/ontology>,
        ulan: ;
    rdfs:range skos:Concept ;
    rdfs:subPropertyOf skos:related ;
    skos:broader skos:related ;
    skos:example "The National Gallery of Art was/is a member of the Foundation of Documentation of Architecture" ;
    skos:inScheme <http://vocab.getty.edu/ontology>,
        ulan: ;
    skos:notation "1318" ;
    skos:prefLabel "ulan1318_member_was"@en ;
    skos:topConceptOf <http://vocab.getty.edu/ontology>,
        ulan: .

gvp:ulan1322_school_was a owl:ObjectProperty,
        skos:Concept ;
    dc:identifier "1322" ;
    dc:title "school was - person" ;
    dct:description """firm/group - school was - person.\r
Example: Pierre Saalburg attended Architectural Association. School of Architecture""" ;
    rdfs:domain skos:Concept ;
    rdfs:isDefinedBy <http://vocab.getty.edu/ontology>,
        ulan: ;
    rdfs:range skos:Concept ;
    rdfs:subPropertyOf skos:related ;
    skos:broader skos:related ;
    skos:example "Pierre Saalburg attended Architectural Association. School of Architecture" ;
    skos:inScheme <http://vocab.getty.edu/ontology>,
        ulan: ;
    skos:notation "1322" ;
    skos:prefLabel "ulan1322_school_was"@en ;
    skos:topConceptOf <http://vocab.getty.edu/ontology>,
        ulan: .

gvp:ulan1332_worker_was a owl:ObjectProperty,
        skos:Concept ;
    dc:identifier "1332" ;
    dc:title "worker was - any" ;
    dct:description """person - worker was - any.\r
Example: Workers for the Carracci family included Scarsellino and Domenichino""" ;
    rdfs:domain skos:Concept ;
    rdfs:isDefinedBy <http://vocab.getty.edu/ontology>,
        ulan: ;
    rdfs:range skos:Concept ;
    rdfs:subPropertyOf skos:related ;
    skos:broader skos:related ;
    skos:example "Workers for the Carracci family included Scarsellino and Domenichino" ;
    skos:inScheme <http://vocab.getty.edu/ontology>,
        ulan: ;
    skos:notation "1332" ;
    skos:prefLabel "ulan1332_worker_was"@en ;
    skos:topConceptOf <http://vocab.getty.edu/ontology>,
        ulan: .

gvp:ulan1422_founded a owl:ObjectProperty,
        skos:Concept ;
    dc:identifier "1422" ;
    dc:title "founded - firm/group" ;
    dct:description """firm/group - founded - firm/group.\r
Example: The United States Congress founded the National Gallery of Art""" ;
    rdfs:domain skos:Concept ;
    rdfs:isDefinedBy <http://vocab.getty.edu/ontology>,
        ulan: ;
    rdfs:range skos:Concept ;
    rdfs:subPropertyOf skos:related ;
    skos:broader skos:related ;
    skos:example "The United States Congress founded the National Gallery of Art" ;
    skos:inScheme <http://vocab.getty.edu/ontology>,
        ulan: ;
    skos:notation "1422" ;
    skos:prefLabel "ulan1422_founded"@en ;
    skos:topConceptOf <http://vocab.getty.edu/ontology>,
        ulan: .

gvp:ulan1516_great-grandchild_of a owl:ObjectProperty,
        skos:Concept ;
    dc:identifier "1516" ;
    dc:title "great-grandchild of - person" ;
    dct:description """person - great-grandchild of - person.\r
Example: Richard Benno Adam is the great-grandchild of Albrecht Adam""" ;
    rdfs:domain skos:Concept ;
    rdfs:isDefinedBy <http://vocab.getty.edu/ontology>,
        ulan: ;
    rdfs:range skos:Concept ;
    rdfs:subPropertyOf skos:related ;
    skos:broader skos:related ;
    skos:example "Richard Benno Adam is the great-grandchild of Albrecht Adam" ;
    skos:inScheme <http://vocab.getty.edu/ontology>,
        ulan: ;
    skos:notation "1516" ;
    skos:prefLabel "ulan1516_great-grandchild_of"@en ;
    skos:topConceptOf <http://vocab.getty.edu/ontology>,
        ulan: .

gvp:ulan1532_uncle-aunt_of a owl:ObjectProperty,
        skos:Concept ;
    dc:identifier "1532" ;
    dc:title "uncle/aunt of - person" ;
    dct:description """person - uncle/aunt of - person.\r
Example: Edouard Manet is the uncle/aunt of Julie Manet""" ;
    rdfs:domain skos:Concept ;
    rdfs:isDefinedBy <http://vocab.getty.edu/ontology>,
        ulan: ;
    rdfs:range skos:Concept ;
    rdfs:subPropertyOf skos:related ;
    skos:broader skos:related ;
    skos:example "Edouard Manet is the uncle/aunt of Julie Manet" ;
    skos:inScheme <http://vocab.getty.edu/ontology>,
        ulan: ;
    skos:notation "1532" ;
    skos:prefLabel "ulan1532_uncle-aunt_of"@en ;
    skos:topConceptOf <http://vocab.getty.edu/ontology>,
        ulan: .

gvp:ulan1553_child_by_marriage_of a owl:ObjectProperty,
        skos:Concept ;
    dc:identifier "1553" ;
    dc:title "child by marriage of - person" ;
    dct:description """person - child by marriage (step child) - person.\r
Example: Pieter Gerritsz van Roestraten is the child by marriage of Frans Hals""" ;
    rdfs:domain skos:Concept ;
    rdfs:isDefinedBy <http://vocab.getty.edu/ontology>,
        ulan: ;
    rdfs:range skos:Concept ;
    rdfs:subPropertyOf skos:related ;
    skos:broader skos:related ;
    skos:example "Pieter Gerritsz van Roestraten is the child by marriage of Frans Hals" ;
    skos:inScheme <http://vocab.getty.edu/ontology>,
        ulan: ;
    skos:notation "1553" ;
    skos:prefLabel "ulan1553_child_by_marriage_of"@en ;
    skos:topConceptOf <http://vocab.getty.edu/ontology>,
        ulan: .

gvp:ulan1573_ward_of a owl:ObjectProperty,
        skos:Concept ;
    dc:identifier "1573" ;
    dc:title "ward of - person" ;
    dct:description """person - ward of - person.\r
Example: Samuel Cooper was a ward of John Hoskins, the elder""" ;
    rdfs:domain skos:Concept ;
    rdfs:isDefinedBy <http://vocab.getty.edu/ontology>,
        ulan: ;
    rdfs:range skos:Concept ;
    rdfs:subPropertyOf skos:related ;
    skos:broader skos:related ;
    skos:example "Samuel Cooper was a ward of John Hoskins, the elder" ;
    skos:inScheme <http://vocab.getty.edu/ontology>,
        ulan: ;
    skos:notation "1573" ;
    skos:prefLabel "ulan1573_ward_of"@en ;
    skos:topConceptOf <http://vocab.getty.edu/ontology>,
        ulan: .

gvp:ulan1575_godchild_of a owl:ObjectProperty,
        skos:Concept ;
    dc:identifier "1575" ;
    dc:title "godchild of - person" ;
    dct:description """person - godchild of - person.\r
Example: Jean I Nocret is the godchild of Jean-Baptiste Goy""" ;
    rdfs:domain skos:Concept ;
    rdfs:isDefinedBy <http://vocab.getty.edu/ontology>,
        ulan: ;
    rdfs:range skos:Concept ;
    rdfs:subPropertyOf skos:related ;
    skos:broader skos:related ;
    skos:example "Jean I Nocret is the godchild of Jean-Baptiste Goy" ;
    skos:inScheme <http://vocab.getty.edu/ontology>,
        ulan: ;
    skos:notation "1575" ;
    skos:prefLabel "ulan1575_godchild_of"@en ;
    skos:topConceptOf <http://vocab.getty.edu/ontology>,
        ulan: .

gvp:ulan1582_ancestor_of a owl:ObjectProperty,
        skos:Concept ;
    dc:identifier "1582" ;
    dc:title "ancestor of - person" ;
    dct:description """person - ancestor of - person.\r
Example: Paolo Veronese is the ancestor of Paolo Caliari""" ;
    rdfs:domain skos:Concept ;
    rdfs:isDefinedBy <http://vocab.getty.edu/ontology>,
        ulan: ;
    rdfs:range skos:Concept ;
    rdfs:subPropertyOf skos:related ;
    skos:broader skos:related ;
    skos:example "Paolo Veronese is the ancestor of Paolo Caliari" ;
    skos:inScheme <http://vocab.getty.edu/ontology>,
        ulan: ;
    skos:notation "1582" ;
    skos:prefLabel "ulan1582_ancestor_of"@en ;
    skos:topConceptOf <http://vocab.getty.edu/ontology>,
        ulan: .

gvp:ulan2575_directed_by a owl:ObjectProperty,
        skos:Concept ;
    dc:identifier "2575" ;
    dc:title "directed by - person" ;
    dct:description """institution - directed by - person.\r
Example: Gobelins Tapestry Manufactory was directed by Jean Jans I""" ;
    rdfs:domain skos:Concept ;
    rdfs:isDefinedBy <http://vocab.getty.edu/ontology>,
        ulan: ;
    rdfs:range skos:Concept ;
    rdfs:subPropertyOf skos:related ;
    skos:broader skos:related ;
    skos:example "Gobelins Tapestry Manufactory was directed by Jean Jans I" ;
    skos:inScheme <http://vocab.getty.edu/ontology>,
        ulan: ;
    skos:notation "2575" ;
    skos:prefLabel "ulan2575_directed_by"@en ;
    skos:topConceptOf <http://vocab.getty.edu/ontology>,
        ulan: .

gvp:ulan2577_patron_was a owl:ObjectProperty,
        skos:Concept ;
    dc:identifier "2577" ;
    dc:title "patron was - person" ;
    dct:description """person - patron was - person.\r
Example: James Caulfiel, Earl of Charlemont was the patron of William Chambers""" ;
    rdfs:domain skos:Concept ;
    rdfs:isDefinedBy <http://vocab.getty.edu/ontology>,
        ulan: ;
    rdfs:range skos:Concept ;
    rdfs:subPropertyOf skos:related ;
    skos:broader skos:related ;
    skos:example "James Caulfiel, Earl of Charlemont was the patron of William Chambers" ;
    skos:inScheme <http://vocab.getty.edu/ontology>,
        ulan: ;
    skos:notation "2577" ;
    skos:prefLabel "ulan2577_patron_was"@en ;
    skos:topConceptOf <http://vocab.getty.edu/ontology>,
        ulan: .

gvp:ulan2651_publisher_of a owl:ObjectProperty,
        skos:Concept ;
    dc:identifier "2651" ;
    dc:title "publisher of - person" ;
    dct:description """firm - publisher of - person.\r
Example: Negretti and Zambra was the publisher of Pierre Joseph Rossier""" ;
    rdfs:domain skos:Concept ;
    rdfs:isDefinedBy <http://vocab.getty.edu/ontology>,
        ulan: ;
    rdfs:range skos:Concept ;
    rdfs:subPropertyOf skos:related ;
    skos:broader skos:related ;
    skos:example "Negretti and Zambra was the publisher of Pierre Joseph Rossier" ;
    skos:inScheme <http://vocab.getty.edu/ontology>,
        ulan: ;
    skos:notation "2651" ;
    skos:prefLabel "ulan2651_publisher_of"@en ;
    skos:topConceptOf <http://vocab.getty.edu/ontology>,
        ulan: .

gvp:ulan2675_professor_was a owl:ObjectProperty,
        skos:Concept ;
    dc:identifier "2675" ;
    dc:title "professor was - person" ;
    dct:description """institution - professor was - person.\r
Example: A professor at Bauhaus was Paul Klee""" ;
    rdfs:domain skos:Concept ;
    rdfs:isDefinedBy <http://vocab.getty.edu/ontology>,
        ulan: ;
    rdfs:range skos:Concept ;
    rdfs:subPropertyOf skos:related ;
    skos:broader skos:related ;
    skos:example "A professor at Bauhaus was Paul Klee" ;
    skos:inScheme <http://vocab.getty.edu/ontology>,
        ulan: ;
    skos:notation "2675" ;
    skos:prefLabel "ulan2675_professor_was"@en ;
    skos:topConceptOf <http://vocab.getty.edu/ontology>,
        ulan: .

gvp:ulan2782_dedicated_to a owl:ObjectProperty,
        skos:Concept ;
    dc:identifier "2782" ;
    dc:title "dedicated to - person" ;
    dct:description """institution - dedicated to - person.\r
Example: The Rodin Museum in Philadelphia is didicated to Auguste Rodin""" ;
    rdfs:domain skos:Concept ;
    rdfs:isDefinedBy <http://vocab.getty.edu/ontology>,
        ulan: ;
    rdfs:range skos:Concept ;
    rdfs:subPropertyOf skos:related ;
    skos:broader skos:related ;
    skos:example "The Rodin Museum in Philadelphia is didicated to Auguste Rodin" ;
    skos:inScheme <http://vocab.getty.edu/ontology>,
        ulan: ;
    skos:notation "2782" ;
    skos:prefLabel "ulan2782_dedicated_to"@en ;
    skos:topConceptOf <http://vocab.getty.edu/ontology>,
        ulan: .

gvp:ulan2829_student_was a owl:ObjectProperty,
        skos:Concept ;
    dc:identifier "2829" ;
    dc:title "student was - person" ;
    dct:description """institution - student was - person.\r
Example: Bauhaus student was Zdanek Rossman""" ;
    rdfs:domain skos:Concept ;
    rdfs:isDefinedBy <http://vocab.getty.edu/ontology>,
        ulan: ;
    rdfs:range skos:Concept ;
    rdfs:subPropertyOf skos:related ;
    skos:broader skos:related ;
    skos:example "Bauhaus student was Zdanek Rossman" ;
    skos:inScheme <http://vocab.getty.edu/ontology>,
        ulan: ;
    skos:notation "2829" ;
    skos:prefLabel "ulan2829_student_was"@en ;
    skos:topConceptOf <http://vocab.getty.edu/ontology>,
        ulan: .

gvp:ulan2841_performer_was a owl:ObjectProperty,
        skos:Concept ;
    dc:identifier "2841" ;
    dc:title "performer was - person" ;
    dct:description "group - performer was - person" ;
    rdfs:domain skos:Concept ;
    rdfs:isDefinedBy <http://vocab.getty.edu/ontology>,
        ulan: ;
    rdfs:range skos:Concept ;
    rdfs:subPropertyOf skos:related ;
    skos:broader skos:related ;
    skos:inScheme <http://vocab.getty.edu/ontology>,
        ulan: ;
    skos:notation "2841" ;
    skos:prefLabel "ulan2841_performer_was"@en ;
    skos:topConceptOf <http://vocab.getty.edu/ontology>,
        ulan: .

<http://www.getty.edu/research/> a foaf:Organization ;
    rdfs:label "Getty Research Institute"@en ;
    skos:prefLabel "Getty Research Institute"@en ;
    foaf:name "Getty Research Institute" .

<http://www.ontotext.com> a foaf:Organization ;
    rdfs:label "Ontotext Corp"@en ;
    skos:prefLabel "Ontotext Corp"@en ;
    foaf:name "Ontotext Corp" .

gvp:GuideTerm a owl:Class,
        skos:Concept ;
    rdfs:label "GuideTerm"@en ;
    dct:description """Guide Term: place holder to create a level in the hierarchy. Used in AAT and ULAN. Not used for indexing or cataloguing..
Example: <vessels for serving and consuming food> (AAT), ulan:500353455 <named animals> under facet Non-Artists (ULAN)""" ;
    rdfs:comment "Guide Term: place holder to create a level in the hierarchy. Used in AAT and ULAN. Not used for indexing or cataloguing." ;
    rdfs:isDefinedBy <http://vocab.getty.edu/ontology> ;
    rdfs:subClassOf iso:ThesaurusArray,
        gvp:Subject ;
    skos:broader gvp:Subject ;
    skos:example "<vessels for serving and consuming food> (AAT), ulan:500353455 <named animals> under facet Non-Artists (ULAN)" ;
    skos:inScheme <http://vocab.getty.edu/ontology> ;
    skos:prefLabel "GuideTerm"@en ;
    skos:topConceptOf <http://vocab.getty.edu/ontology> .

gvp:agentType a owl:ObjectProperty,
        skos:Concept ;
    rdfs:label "agentType"@en ;
    dct:description "Type of a ULAN PersonConcept or GroupConcept. Domain is ULAN concept, range is AAT concept" ;
    rdfs:comment "Type of a ULAN PersonConcept or GroupConcept. Domain is ULAN concept, range is AAT concept" ;
    rdfs:domain gvp:Subject ;
    rdfs:isDefinedBy <http://vocab.getty.edu/ontology> ;
    rdfs:range gvp:Subject ;
    skos:inScheme <http://vocab.getty.edu/ontology> ;
    skos:narrower gvp:agentTypeNonPreferred,
        gvp:agentTypePreferred ;
    skos:prefLabel "agentType"@en ;
    skos:topConceptOf <http://vocab.getty.edu/ontology> .

gvp:broaderNonConcept a owl:ObjectProperty,
        skos:Concept ;
    rdfs:label "broaderNonConcept"@en ;
    dct:description "Chain of gvp:broader from Concept to GuideTerms, without intervening Concept" ;
    rdfs:comment "Chain of gvp:broader from Concept to GuideTerms, without intervening Concept" ;
    rdfs:domain skos:Concept ;
    rdfs:isDefinedBy <http://vocab.getty.edu/ontology> ;
    rdfs:range gvp:GuideTerm ;
    skos:inScheme <http://vocab.getty.edu/ontology> ;
    skos:prefLabel "broaderNonConcept"@en ;
    skos:topConceptOf <http://vocab.getty.edu/ontology> .

gvp:broaderPreferredExtended a owl:ObjectProperty,
        skos:Concept ;
    rdfs:label "broaderPreferredExtended"@en ;
    dct:description """Preferred Ancestors. Meaningful closure of gvp:broaderPreferred. Needed to display the hierarchy.
Example: Mt Athos has preferred ancestor places (BTPE) World, Europe, Greece, Macedonia, Pangaíon Óros regional division;
and prefererd place type (BTIE) inhabited place""" ;
    rdfs:comment "Preferred Ancestors. Meaningful closure of gvp:broaderPreferred. Needed to display the hierarchy" ;
    rdfs:domain gvp:Subject ;
    rdfs:isDefinedBy <http://vocab.getty.edu/ontology> ;
    rdfs:range gvp:Subject ;
    skos:example """Mt Athos has preferred ancestor places (BTPE) World, Europe, Greece, Macedonia, Pangaíon Óros regional division;
and prefererd place type (BTIE) inhabited place""" ;
    skos:inScheme <http://vocab.getty.edu/ontology> ;
    skos:narrower gvp:broaderPreferred ;
    skos:prefLabel "broaderPreferredExtended"@en ;
    skos:topConceptOf <http://vocab.getty.edu/ontology> .

gvp:placeType a owl:ObjectProperty,
        skos:Concept ;
    rdfs:label "placeType"@en ;
    dct:description """Type for a TGN place. Domain is TGN concept (AdminPlaceConcept or PhysPlaceConcept), range is AAT Concept.
Example: Machupicchu, Peru has preferred type "deserted settlement" (current) and non-preferred type "Inca center" (historic)""" ;
    rdfs:comment "Type for a TGN place. Domain is TGN concept (AdminPlaceConcept or PhysPlaceConcept), range is AAT Concept" ;
    rdfs:domain gvp:Subject ;
    rdfs:isDefinedBy <http://vocab.getty.edu/ontology> ;
    rdfs:range gvp:Subject ;
    skos:example "Machupicchu, Peru has preferred type \"deserted settlement\" (current) and non-preferred type \"Inca center\" (historic)" ;
    skos:inScheme <http://vocab.getty.edu/ontology> ;
    skos:narrower gvp:placeTypeNonPreferred,
        gvp:placeTypePreferred ;
    skos:prefLabel "placeType"@en ;
    skos:topConceptOf <http://vocab.getty.edu/ontology> .

<http://vocab.getty.edu/term/display/> a skos:ConceptScheme ;
    rdfs:label "Term Display concept scheme"@en ;
    dct:description "Term Display concept scheme" ;
    rdfs:isDefinedBy <http://vocab.getty.edu/ontology> ;
    skos:hasTopConcept <http://vocab.getty.edu/term/display/Display>,
        <http://vocab.getty.edu/term/display/Indexing> ;
    skos:inScheme <http://vocab.getty.edu/ontology> ;
    skos:prefLabel "Term Display concept scheme"@en ;
    skos:topConceptOf <http://vocab.getty.edu/ontology> .

dct:contributor skos:narrower gvp:contributorAlternatePreferred,
        gvp:contributorNonPreferred,
        gvp:contributorPreferred .

dct:source skos:narrower gvp:sourceAlternatePreferred,
        gvp:sourceNonPreferred,
        gvp:sourcePreferred .

gvp:broaderGeneric a owl:ObjectProperty,
        skos:Concept ;
    rdfs:label "broaderGeneric"@en ;
    dct:description """BTG (Genus/Species, "is a") relation. We also infer iso-thes:broaderGeneric, which goes only between Concepts.
Example: calcite (AAT) BTG mineral (AAT)""" ;
    rdfs:comment "BTG (Genus/Species, \"is a\") relation. We also infer iso-thes:broaderGeneric, which goes only between Concepts" ;
    rdfs:domain gvp:Subject ;
    rdfs:isDefinedBy <http://vocab.getty.edu/ontology> ;
    rdfs:range gvp:Subject ;
    rdfs:subPropertyOf gvp:broader,
        gvp:broaderGenericExtended ;
    skos:broader gvp:broaderGenericExtended ;
    skos:example "calcite (AAT) BTG mineral (AAT)" ;
    skos:inScheme <http://vocab.getty.edu/ontology> ;
    skos:prefLabel "broaderGeneric"@en ;
    skos:topConceptOf <http://vocab.getty.edu/ontology> .

gvp:broaderGenericExtended a owl:ObjectProperty,
        skos:Concept ;
    rdfs:label "broaderGenericExtended"@en ;
    dct:description """Ancestors (Generic). Meaningful closure of gvp:broaderGeneric. Infers iso:broaderGeneric for pairs of directly related skos:Concepts.
Example: <anvils and anvil accessories> BTG <forging and metal-shaping tools> BTG <forging and metal-shaping equipment>,
so <anvils and anvil accessories> BTGE <forging and metal-shaping equipment>""" ;
    rdfs:comment "Ancestors (Generic). Meaningful closure of gvp:broaderGeneric. Infers iso:broaderGeneric for pairs of directly related skos:Concepts" ;
    rdfs:domain gvp:Subject ;
    rdfs:isDefinedBy <http://vocab.getty.edu/ontology> ;
    rdfs:range gvp:Subject ;
    rdfs:subPropertyOf gvp:broaderExtended ;
    owl:propertyChainAxiom ( gvp:broaderGenericExtended gvp:broaderGeneric ) ;
    skos:broader gvp:broaderExtended ;
    skos:example """<anvils and anvil accessories> BTG <forging and metal-shaping tools> BTG <forging and metal-shaping equipment>,
so <anvils and anvil accessories> BTGE <forging and metal-shaping equipment>""" ;
    skos:inScheme <http://vocab.getty.edu/ontology> ;
    skos:narrower gvp:broaderGeneric ;
    skos:prefLabel "broaderGenericExtended"@en ;
    skos:topConceptOf <http://vocab.getty.edu/ontology> .

gvp:broaderInstantialExtended a owl:ObjectProperty,
        skos:Concept ;
    rdfs:label "broaderInstantialExtended"@en ;
    dct:description "Ancestors (Instantial). Meaningful closure of gvp:broaderInstantial. Infers iso:broaderInstantial for pairs of directly related skos:Concepts." ;
    rdfs:domain gvp:Subject ;
    rdfs:isDefinedBy <http://vocab.getty.edu/ontology> ;
    rdfs:range gvp:Subject ;
    rdfs:subPropertyOf gvp:broaderExtended ;
    owl:propertyChainAxiom ( gvp:broaderInstantialExtended gvp:broaderGeneric ) ;
    skos:broader gvp:broaderExtended ;
    skos:example """Mt Athos (TGN) BTI orthodox religious center (AAT) BTG Christian religious center (AAT),
so Mt Athos (TGN) BTIE Christian religious center (AAT)""" ;
    skos:inScheme <http://vocab.getty.edu/ontology> ;
    skos:narrower gvp:broaderInstantial ;
    skos:prefLabel "broaderInstantialExtended"@en ;
    skos:topConceptOf <http://vocab.getty.edu/ontology> .

gvp:broaderPartitiveExtended a owl:ObjectProperty,
        skos:Concept ;
    rdfs:label "broaderPartitiveExtended"@en ;
    dct:description """Ancestors (Partitive). Meaningful closure of gvp:broaderPartitive. Infers iso:broaderPartitive for pairs of directly related skos:Concepts.
Example: anvil components BTP <anvils and anvil accessories> BTG <forging and metal-shaping tools>,
so anvil components BTPE <forging and metal-shaping tools>""" ;
    rdfs:comment "Ancestors (Partitive). Meaningful closure of gvp:broaderPartitive. Infers iso:broaderPartitive for pairs of directly related skos:Concepts" ;
    rdfs:domain gvp:Subject ;
    rdfs:isDefinedBy <http://vocab.getty.edu/ontology> ;
    rdfs:range gvp:Subject ;
    rdfs:subPropertyOf gvp:broaderExtended ;
    owl:propertyChainAxiom ( gvp:broaderPartitiveExtended gvp:broaderGeneric ),
        ( gvp:broaderPartitiveExtended gvp:broaderPartitive ),
        ( gvp:broaderGeneric gvp:broaderPartitiveExtended ) ;
    skos:broader gvp:broaderExtended ;
    skos:example """anvil components BTP <anvils and anvil accessories> BTG <forging and metal-shaping tools>,
so anvil components BTPE <forging and metal-shaping tools>""" ;
    skos:inScheme <http://vocab.getty.edu/ontology> ;
    skos:prefLabel "broaderPartitiveExtended"@en ;
    skos:topConceptOf <http://vocab.getty.edu/ontology> .

<http://vocab.getty.edu/term/flag/> a skos:ConceptScheme ;
    rdfs:label "Term Flag concept scheme"@en ;
    dct:description "Term Flag concept scheme" ;
    rdfs:isDefinedBy <http://vocab.getty.edu/ontology> ;
    skos:hasTopConcept <http://vocab.getty.edu/term/flag/LiteralTranslation>,
        <http://vocab.getty.edu/term/flag/LoanTerm>,
        <http://vocab.getty.edu/term/flag/Vernacular> ;
    skos:inScheme <http://vocab.getty.edu/ontology> ;
    skos:prefLabel "Term Flag concept scheme"@en ;
    skos:topConceptOf <http://vocab.getty.edu/ontology> .

<http://vocab.getty.edu/term/type/> a skos:ConceptScheme ;
    rdfs:label "Term Type concept scheme"@en ;
    dct:description "Term Type concept scheme" ;
    rdfs:isDefinedBy <http://vocab.getty.edu/ontology> ;
    skos:hasTopConcept <http://vocab.getty.edu/term/type/AlternateDescriptor>,
        <http://vocab.getty.edu/term/type/Descriptor>,
        <http://vocab.getty.edu/term/type/UsedForTerm> ;
    skos:inScheme <http://vocab.getty.edu/ontology> ;
    skos:prefLabel "Term Type concept scheme"@en ;
    skos:topConceptOf <http://vocab.getty.edu/ontology> .

gvp:biography a owl:ObjectProperty,
        skos:Concept ;
    rdfs:label "biography"@en ;
    dct:description "Biography of an ULAN agent. Domain is schema:Person/Organization, range is gvp:Biography. The preferred biography fields are also directly available in the Person/Organization" ;
    rdfs:comment "Biography of an ULAN agent. Domain is schema:Person/Organization, range is gvp:Biography. The preferred biography fields are also directly available in the Person/Organization" ;
    rdfs:isDefinedBy <http://vocab.getty.edu/ontology> ;
    rdfs:range gvp:Biography ;
    rdfs:subPropertyOf gvp:biography ;
    skos:broader gvp:biography ;
    skos:inScheme <http://vocab.getty.edu/ontology> ;
    skos:narrower gvp:biography,
        gvp:biographyNonPreferred,
        gvp:biographyPreferred ;
    skos:prefLabel "biography"@en ;
    skos:topConceptOf <http://vocab.getty.edu/ontology> .

gvp:broaderExtended a owl:ObjectProperty,
        skos:Concept ;
    rdfs:label "broaderExtended"@en ;
    dct:description """Appropriate ancestors. Meaningful closure of gvp:broader for query expansion. Use this, not skos:broaderTransitive.
Example: Mt Athos has ancestor places (BTPE) World, Europe, Greece, Macedonia, Pangaíon Óros regional division;
and place types (BTIE) inhabited place; and orthodox religious center, Christian religious center, religious center""" ;
    rdfs:comment "Appropriate ancestors. Meaningful closure of gvp:broader for query expansion. Use this, not skos:broaderTransitive" ;
    rdfs:domain gvp:Subject ;
    rdfs:isDefinedBy <http://vocab.getty.edu/ontology> ;
    rdfs:range gvp:Subject ;
    skos:example """Mt Athos has ancestor places (BTPE) World, Europe, Greece, Macedonia, Pangaíon Óros regional division;
and place types (BTIE) inhabited place; and orthodox religious center, Christian religious center, religious center""" ;
    skos:inScheme <http://vocab.getty.edu/ontology> ;
    skos:narrower gvp:broaderGenericExtended,
        gvp:broaderInstantialExtended,
        gvp:broaderPartitiveExtended ;
    skos:prefLabel "broaderExtended"@en ;
    skos:topConceptOf <http://vocab.getty.edu/ontology> .

<http://vocab.getty.edu/historic/> a skos:ConceptScheme ;
    rdfs:label "Historic Flag concept scheme"@en ;
    dct:description "Historic Flag concept scheme" ;
    rdfs:isDefinedBy <http://vocab.getty.edu/ontology> ;
    skos:hasTopConcept <http://vocab.getty.edu/historic/current>,
        <http://vocab.getty.edu/historic/currentAndHistoric>,
        <http://vocab.getty.edu/historic/historic>,
        <http://vocab.getty.edu/historic/localUse> ;
    skos:inScheme <http://vocab.getty.edu/ontology> ;
    skos:prefLabel "Historic Flag concept scheme"@en ;
    skos:topConceptOf <http://vocab.getty.edu/ontology> .

gvp:broader a owl:ObjectProperty,
        skos:Concept ;
    rdfs:label "broader"@en ;
    dct:description "Parents of a subject. Each broader is also Preferred|NonPreferred and Partitive|Instantial|Generic" ;
    rdfs:comment "Parents of a subject. Each broader is also Preferred|NonPreferred and Partitive|Instantial|Generic" ;
    rdfs:domain gvp:Subject ;
    rdfs:isDefinedBy <http://vocab.getty.edu/ontology> ;
    rdfs:range gvp:Subject ;
    skos:inScheme <http://vocab.getty.edu/ontology> ;
    skos:narrower gvp:broaderNonPreferred,
        gvp:broaderPartitive ;
    skos:prefLabel "broader"@en ;
    skos:topConceptOf <http://vocab.getty.edu/ontology> .

<http://vocab.getty.edu/term/POS/> a skos:ConceptScheme ;
    rdfs:label "Part of Speech concept scheme"@en ;
    dct:description "Part of Speech concept scheme" ;
    rdfs:isDefinedBy <http://vocab.getty.edu/ontology> ;
    skos:hasTopConcept <http://vocab.getty.edu/term/POS/Adjectival>,
        <http://vocab.getty.edu/term/POS/BothSingularAndPlural>,
        <http://vocab.getty.edu/term/POS/Noun>,
        <http://vocab.getty.edu/term/POS/PastParticiple>,
        <http://vocab.getty.edu/term/POS/PluralNoun>,
        <http://vocab.getty.edu/term/POS/SingularNoun>,
        <http://vocab.getty.edu/term/POS/VerbalNounGerund> ;
    skos:inScheme <http://vocab.getty.edu/ontology> ;
    skos:prefLabel "Part of Speech concept scheme"@en ;
    skos:topConceptOf <http://vocab.getty.edu/ontology> .

<http://vocab.getty.edu/term/kind/> a skos:ConceptScheme ;
    rdfs:label "Term Kind concept scheme"@en ;
    dct:description "Term Kind concept scheme" ;
    rdfs:isDefinedBy <http://vocab.getty.edu/ontology> ;
    skos:hasTopConcept <http://vocab.getty.edu/term/kind/Abbreviation>,
        <http://vocab.getty.edu/term/kind/BirthName>,
        <http://vocab.getty.edu/term/kind/ChemicalName>,
        <http://vocab.getty.edu/term/kind/Code>,
        <http://vocab.getty.edu/term/kind/CommonName>,
        <http://vocab.getty.edu/term/kind/CommonTerm>,
        <http://vocab.getty.edu/term/kind/FIPSCode>,
        <http://vocab.getty.edu/term/kind/FullName>,
        <http://vocab.getty.edu/term/kind/FullTerm>,
        <http://vocab.getty.edu/term/kind/ISOalpha2>,
        <http://vocab.getty.edu/term/kind/ISOalpha3>,
        <http://vocab.getty.edu/term/kind/ISOnumeric2>,
        <http://vocab.getty.edu/term/kind/ISOnumeric3>,
        <http://vocab.getty.edu/term/kind/JargonOrSlang>,
        <http://vocab.getty.edu/term/kind/Neologism>,
        <http://vocab.getty.edu/term/kind/OfficialName>,
        <http://vocab.getty.edu/term/kind/ProvisionalName>,
        <http://vocab.getty.edu/term/kind/Pseudonym>,
        <http://vocab.getty.edu/term/kind/ScientificOrTechnical>,
        <http://vocab.getty.edu/term/kind/SiteName>,
        <http://vocab.getty.edu/term/kind/USPSCode> ;
    skos:inScheme <http://vocab.getty.edu/ontology> ;
    skos:prefLabel "Term Kind concept scheme"@en ;
    skos:topConceptOf <http://vocab.getty.edu/ontology> .

tgn: a skos:ConceptScheme ;
    rdfs:label "Thesaurus of Geographic Names"@en ;
    dct:created "2014-06-15"^^xsd:date ;
    dct:creator <http://www.getty.edu/research/>,
        <http://www.ontotext.com> ;
    vann:preferredNamespacePrefix "tgn" ;
    vann:preferredNamespaceUri "http://vocab.getty.edu/tgn/" ;
    rdfs:comment "The Thesaurus of Geographic Names concept scheme" ;
    rdfs:seeAlso <http://vocab.getty.edu/>,
        <http://vocab.getty.edu/.well-known/void>,
        <http://www.getty.edu/research/tools/vocabularies/lod/> ;
    skos:hasTopConcept gvp:tgn3000_related_to,
        gvp:tgn3006_formerly_identified_as,
        gvp:tgn3101_near-adjacent_to,
        gvp:tgn3102_coextensive_with,
        gvp:tgn3103_located_on,
        gvp:tgn3104_is_location_of,
        gvp:tgn3110_meaning-usage_overlaps_with,
        gvp:tgn3317_member_of,
        gvp:tgn3318_member_is,
        gvp:tgn3402_moved_to,
        gvp:tgn3411_successor_of,
        gvp:tgn3510_historical_connection,
        gvp:tgn3611_administrative_dependent_of,
        gvp:tgn3612_administrative_entity_for ;
    skos:prefLabel "Thesaurus of Geographic Names"@en ;
    foaf:homepage <http://www.getty.edu/research/tools/vocabularies/tgn/> .

gvp:Subject a owl:Class,
        skos:Concept ;
    rdfs:label "Subject"@en ;
    dct:description """Node in a GVP vocabulary hierarchy. 
May be Facet, GuideTerm, Hierarchy, Concept, AdminPlaceConcept, PhysPlaceConcept, PhysAdminPlaceConcept, or ObsoleteSubject.
Implemented as skos:Concept or iso:ThesaurusArray and skos:Collection""" ;
    rdfs:comment """Node in a GVP vocabulary hierarchy. 
May be Facet, GuideTerm, Hierarchy, Concept, AdminPlaceConcept, PhysPlaceConcept, PhysAdminPlaceConcept, or ObsoleteSubject.
Implemented as skos:Concept or iso:ThesaurusArray and skos:Collection""" ;
    rdfs:isDefinedBy <http://vocab.getty.edu/ontology> ;
    skos:inScheme <http://vocab.getty.edu/ontology> ;
    skos:narrower gvp:AdminPlaceConcept,
        gvp:Facet,
        gvp:GuideTerm,
        gvp:ObsoleteSubject,
        gvp:PhysAdminPlaceConcept ;
    skos:prefLabel "Subject"@en ;
    skos:topConceptOf <http://vocab.getty.edu/ontology> .

aat: a skos:ConceptScheme ;
    rdfs:label "Art and Architecture Thesaurus"@en ;
    dct:created "2014-02-20"^^xsd:date ;
    dct:creator <http://www.getty.edu/research/>,
        <http://www.ontotext.com> ;
    vann:preferredNamespacePrefix "aat" ;
    vann:preferredNamespaceUri "http://vocab.getty.edu/aat/" ;
    rdfs:comment "The Art and Architecture Thesaurus concept scheme" ;
    rdfs:seeAlso <http://vocab.getty.edu/>,
        <http://vocab.getty.edu/.well-known/void>,
        <http://www.getty.edu/research/tools/vocabularies/lod/> ;
    skos:hasTopConcept gvp:aat2000_related_to,
        gvp:aat2110_meaning-usage_overlaps_with,
        gvp:aat2203_associated_with,
        gvp:aat2209_used-located_in,
        gvp:aat2212_produced_by,
        gvp:aat2215_required_for,
        gvp:aat2216_require,
        gvp:aat2218_used-function_as,
        gvp:aat2286_practice-study,
        gvp:aat2291_locus-setting_for,
        gvp:aat2315_used_by,
        gvp:aat2316_use,
        gvp:aat2325_created_by,
        gvp:aat2328_involved_with,
        gvp:aat2333_have_affiliates,
        gvp:aat2408_locus-setting_for,
        gvp:aat2411_involved_in,
        gvp:aat2418_uses,
        gvp:aat2419_used_for,
        gvp:aat2421_locus-setting_for,
        gvp:aat2422_takes_place_in,
        gvp:aat2424_produced_by,
        gvp:aat2428_produces,
        gvp:aat2431_required_for,
        gvp:aat2432_requires,
        gvp:aat2501_made_of-require,
        gvp:aat2551_reflect-produced_by,
        gvp:aat2554_reflects,
        gvp:aat2555_reflected_in,
        gvp:aat2557_reflects,
        gvp:aat2558_reflected_in,
        gvp:aat2602_possess-exist_in,
        gvp:aat2604_possessed_by-existing_in,
        gvp:aat2612_possessed_by-existing_in,
        gvp:aat2613_possess-exist_in,
        gvp:aat2802_exemplified_by,
        gvp:aat2805_contextualized_in,
        gvp:aat2806_provide_context,
        gvp:aat2812_followed,
        gvp:aat2814_constituent_of,
        gvp:aat2815_composed_of,
        gvp:aat2817_derived-made_from,
        gvp:aat2821_based_on,
        gvp:aat2826_used_with,
        gvp:aat2828_use-require,
        gvp:aat2829_used-required_for,
        gvp:aat2833_ancestor_of,
        gvp:aat2837_source_for,
        gvp:aat2842_source_for,
        gvp:aat2849_involves,
        gvp:aat2875_characteristic_of,
        gvp:aat2876_characterized_by,
        gvp:aat2878_preceded-source_for,
        gvp:aat2881_reflected_in,
        gvp:aat2882_reflect,
        gvp:aat2884_involved_with,
        gvp:aat2885_involves,
        gvp:aat2891_exemplified_by,
        gvp:aat2892_example_of,
        gvp:aat2894_exemplified_by ;
    skos:prefLabel "Art and Architecture Thesaurus"@en ;
    foaf:homepage <http://www.getty.edu/research/tools/vocabularies/aat/> .

ulan: a skos:ConceptScheme ;
    rdfs:label "Union List of Artist Names"@en ;
    dct:created "2015-03-25"^^xsd:date ;
    dct:creator <http://www.getty.edu/research/>,
        <http://www.ontotext.com> ;
    vann:preferredNamespacePrefix "ulan" ;
    vann:preferredNamespaceUri "http://vocab.getty.edu/ulan/" ;
    rdfs:comment "The Union List of Artist Names concept scheme" ;
    rdfs:seeAlso <http://vocab.getty.edu/>,
        <http://vocab.getty.edu/.well-known/void>,
        <http://www.getty.edu/research/tools/vocabularies/lod/> ;
    skos:hasTopConcept gvp:ulan1003_associated_with,
        gvp:ulan1005_possibly_identified_with,
        gvp:ulan1007_distinguished_from,
        gvp:ulan1008_meaning_-usage_overlaps_with,
        gvp:ulan1101_teacher_of,
        gvp:ulan1102_student_of,
        gvp:ulan1106_apprentice_was,
        gvp:ulan1107_influenced,
        gvp:ulan1108_influenced_by,
        gvp:ulan1112_master_was,
        gvp:ulan1201_patron_of,
        gvp:ulan1221_appointed_by,
        gvp:ulan1222_appointee_of,
        gvp:ulan1223_crowned_by,
        gvp:ulan1224_crowned,
        gvp:ulan1303_collaborated_with,
        gvp:ulan1305_worked_with,
        gvp:ulan1307_assistant_of,
        gvp:ulan1311_partner_of,
        gvp:ulan1315_principal_in,
        gvp:ulan1316_principal_was,
        gvp:ulan1317_member_of,
        gvp:ulan1318_member_was,
        gvp:ulan1321_school_of,
        gvp:ulan1322_school_was,
        gvp:ulan1332_worker_was,
        gvp:ulan1413_administration_overlaps_with,
        gvp:ulan1421_founded_by,
        gvp:ulan1422_founded,
        gvp:ulan1500_related_to,
        gvp:ulan1501_sibling_of,
        gvp:ulan1511_child_of,
        gvp:ulan1515_great-grandparent_of,
        gvp:ulan1516_great-grandchild_of,
        gvp:ulan1521_cousin_of,
        gvp:ulan1531_nephew-niece_of,
        gvp:ulan1532_uncle-aunt_of,
        gvp:ulan1542_consort_of,
        gvp:ulan1544_significant_other_of,
        gvp:ulan1547_romantic_partner_of,
        gvp:ulan1548_domestic_partner_of,
        gvp:ulan1551_sibling_by_marriage_of,
        gvp:ulan1553_child_by_marriage_of,
        gvp:ulan1554_adoptive_parent_of,
        gvp:ulan1561_step-child_of,
        gvp:ulan1571_guardian_of,
        gvp:ulan1573_ward_of,
        gvp:ulan1575_godchild_of,
        gvp:ulan1582_ancestor_of,
        gvp:ulan2550_friend_of,
        gvp:ulan2575_directed_by,
        gvp:ulan2576_patron_of,
        gvp:ulan2577_patron_was,
        gvp:ulan2581_administrator_of,
        gvp:ulan2650_publisher_was,
        gvp:ulan2651_publisher_of,
        gvp:ulan2675_professor_was,
        gvp:ulan2676_teacher_at,
        gvp:ulan2692_president_of,
        gvp:ulan2782_dedicated_to,
        gvp:ulan2794_representative_of,
        gvp:ulan2829_student_was,
        gvp:ulan2841_performer_was ;
    skos:prefLabel "Union List of Artist Names"@en ;
    foaf:homepage <http://www.getty.edu/research/tools/vocabularies/ulan/> .

skos:related skos:narrower gvp:aat2000_related_to,
        gvp:aat2001_formerly_referred_to,
        gvp:aat2100_distinguished_from,
        gvp:aat2110_meaning-usage_overlaps_with,
        gvp:aat2203_associated_with,
        gvp:aat2205_causes-is_required,
        gvp:aat2206_caused_by-requires,
        gvp:aat2208_locus-setting_for,
        gvp:aat2209_used-located_in,
        gvp:aat2211_produce,
        gvp:aat2212_produced_by,
        gvp:aat2215_required_for,
        gvp:aat2216_require,
        gvp:aat2218_used-function_as,
        gvp:aat2219_have_form,
        gvp:aat2221_act_upon,
        gvp:aat2222_are_acted_upon,
        gvp:aat2281_have_counterpart,
        gvp:aat2285_practiced-studied_by,
        gvp:aat2286_practice-study,
        gvp:aat2291_locus-setting_for,
        gvp:aat2292_work-live_in,
        gvp:aat2294_locus-setting_for,
        gvp:aat2295_located_in,
        gvp:aat2311_performed_by,
        gvp:aat2312_perform,
        gvp:aat2315_used_by,
        gvp:aat2316_use,
        gvp:aat2318_involved_in,
        gvp:aat2319_involves,
        gvp:aat2321_used_by,
        gvp:aat2322_use,
        gvp:aat2325_created_by,
        gvp:aat2326_create,
        gvp:aat2328_involved_with,
        gvp:aat2329_involves,
        gvp:aat2332_affiliated_with,
        gvp:aat2333_have_affiliates,
        gvp:aat2335_associated_with,
        gvp:aat2336_has_associates,
        gvp:aat2397_focus_of,
        gvp:aat2398_focuses_on,
        gvp:aat2408_locus-setting_for,
        gvp:aat2409_takes_place_in,
        gvp:aat2411_involved_in,
        gvp:aat2412_involves,
        gvp:aat2415_required_for,
        gvp:aat2416_requires,
        gvp:aat2418_uses,
        gvp:aat2419_used_for,
        gvp:aat2421_locus-setting_for,
        gvp:aat2422_takes_place_in,
        gvp:aat2424_produced_by,
        gvp:aat2425_produces,
        gvp:aat2427_produced_by,
        gvp:aat2428_produces,
        gvp:aat2431_required_for,
        gvp:aat2432_requires,
        gvp:aat2434_contextualized_in,
        gvp:aat2435_context_for,
        gvp:aat2501_made_of-require,
        gvp:aat2502_material_for,
        gvp:aat2504_used-located_in,
        gvp:aat2505_locus-setting_for,
        gvp:aat2507_produce-process,
        gvp:aat2508_produced-processed_by,
        gvp:aat2551_reflect-produced_by,
        gvp:aat2552_reflected_in-produces,
        gvp:aat2554_reflects,
        gvp:aat2555_reflected_in,
        gvp:aat2557_reflects,
        gvp:aat2558_reflected_in,
        gvp:aat2562_locus-setting_for,
        gvp:aat2563_located_in,
        gvp:aat2601_possessed_by-existing_in,
        gvp:aat2602_possess-exist_in,
        gvp:aat2604_possessed_by-existing_in,
        gvp:aat2605_possess-exist_in,
        gvp:aat2607_caused_by-requires,
        gvp:aat2608_causes-required_for,
        gvp:aat2612_possessed_by-existing_in,
        gvp:aat2613_possess-exist_in,
        gvp:aat2801_conjuncted_with,
        gvp:aat2802_exemplified_by,
        gvp:aat2803_example_of,
        gvp:aat2805_contextualized_in,
        gvp:aat2806_provide_context,
        gvp:aat2807_derived_from_common_source,
        gvp:aat2809_coexisted_with,
        gvp:aat2811_preceded,
        gvp:aat2812_followed,
        gvp:aat2814_constituent_of,
        gvp:aat2815_composed_of,
        gvp:aat2817_derived-made_from,
        gvp:aat2818_source_for,
        gvp:aat2821_based_on,
        gvp:aat2822_basis_of,
        gvp:aat2824_has_parallels_with,
        gvp:aat2826_used_with,
        gvp:aat2828_use-require,
        gvp:aat2829_used-required_for,
        gvp:aat2831_associated_with,
        gvp:aat2833_ancestor_of,
        gvp:aat2834_decendant_of,
        gvp:aat2836_derived-made_from,
        gvp:aat2837_source_for,
        gvp:aat2841_derived-made_from,
        gvp:aat2842_source_for,
        gvp:aat2845_used-located_in,
        gvp:aat2846_locus-setting_for,
        gvp:aat2848_involved_in,
        gvp:aat2849_involves,
        gvp:aat2852_involved_with,
        gvp:aat2853_involve,
        gvp:aat2875_characteristic_of,
        gvp:aat2876_characterized_by,
        gvp:aat2878_preceded-source_for,
        gvp:aat2879_followed-developed_from,
        gvp:aat2881_reflected_in,
        gvp:aat2882_reflect,
        gvp:aat2884_involved_with,
        gvp:aat2885_involves,
        gvp:aat2886_used-function_as,
        gvp:aat2887_exemplified_by,
        gvp:aat2891_exemplified_by,
        gvp:aat2892_example_of,
        gvp:aat2894_exemplified_by,
        gvp:aat2895_example_of,
        gvp:aat2900_miscellaneous_relationship,
        gvp:tgn3000_related_to,
        gvp:tgn3001_distinguished_from,
        gvp:tgn3005_possibly_identified_as,
        gvp:tgn3006_formerly_identified_as,
        gvp:tgn3101_near-adjacent_to,
        gvp:tgn3102_coextensive_with,
        gvp:tgn3103_located_on,
        gvp:tgn3104_is_location_of,
        gvp:tgn3110_meaning-usage_overlaps_with,
        gvp:tgn3201_capital_of,
        gvp:tgn3202_capital_is,
        gvp:tgn3301_ally_of,
        gvp:tgn3317_member_of,
        gvp:tgn3318_member_is,
        gvp:tgn3401_moved_from,
        gvp:tgn3402_moved_to,
        gvp:tgn3411_successor_of,
        gvp:tgn3412_predecessor_of,
        gvp:tgn3510_historical_connection,
        gvp:tgn3611_administrative_dependent_of,
        gvp:tgn3612_administrative_entity_for,
        gvp:ulan1000_related_to,
        gvp:ulan1003_associated_with,
        gvp:ulan1005_possibly_identified_with,
        gvp:ulan1006_formerly_identified_with,
        gvp:ulan1007_distinguished_from,
        gvp:ulan1008_meaning_-usage_overlaps_with,
        gvp:ulan1101_teacher_of,
        gvp:ulan1102_student_of,
        gvp:ulan1105_apprentice_of,
        gvp:ulan1106_apprentice_was,
        gvp:ulan1107_influenced,
        gvp:ulan1108_influenced_by,
        gvp:ulan1111_master_of,
        gvp:ulan1112_master_was,
        gvp:ulan1113_fellow_student_of,
        gvp:ulan1201_patron_of,
        gvp:ulan1202_patron_was,
        gvp:ulan1203_donor_of,
        gvp:ulan1204_donor_was,
        gvp:ulan1205_client_of,
        gvp:ulan1206_client_was,
        gvp:ulan1211_artist_to,
        gvp:ulan1212_artist_was,
        gvp:ulan1213_court_artist_to,
        gvp:ulan1214_court_artist_was,
        gvp:ulan1217_employee_of,
        gvp:ulan1218_employee_was,
        gvp:ulan1221_appointed_by,
        gvp:ulan1222_appointee_of,
        gvp:ulan1223_crowned_by,
        gvp:ulan1224_crowned,
        gvp:ulan1301_colleague_of,
        gvp:ulan1302_associate_of,
        gvp:ulan1303_collaborated_with,
        gvp:ulan1305_worked_with,
        gvp:ulan1306_performs_with,
        gvp:ulan1307_assistant_of,
        gvp:ulan1308_assisted_by,
        gvp:ulan1309_advisor_of,
        gvp:ulan1310_advised_by,
        gvp:ulan1311_partner_of,
        gvp:ulan1313_partner_in,
        gvp:ulan1314_partner_was,
        gvp:ulan1315_principal_in,
        gvp:ulan1316_principal_was,
        gvp:ulan1317_member_of,
        gvp:ulan1318_member_was,
        gvp:ulan1321_school_of,
        gvp:ulan1322_school_was,
        gvp:ulan1331_worked_with,
        gvp:ulan1332_worker_was,
        gvp:ulan1411_successor_of,
        gvp:ulan1412_predecessor_of,
        gvp:ulan1413_administration_overlaps_with,
        gvp:ulan1414_joint_venture_with,
        gvp:ulan1421_founded_by,
        gvp:ulan1422_founded,
        gvp:ulan1500_related_to,
        gvp:ulan1501_sibling_of,
        gvp:ulan1511_child_of,
        gvp:ulan1512_parent_of,
        gvp:ulan1513_grandchild_of,
        gvp:ulan1514_gandparent_of,
        gvp:ulan1515_great-grandparent_of,
        gvp:ulan1516_great-grandchild_of,
        gvp:ulan1521_cousin_of,
        gvp:ulan1531_nephew-niece_of,
        gvp:ulan1532_uncle-aunt_of,
        gvp:ulan1541_spouse_of,
        gvp:ulan1542_consort_of,
        gvp:ulan1543_consort_was,
        gvp:ulan1544_significant_other_of,
        gvp:ulan1547_romantic_partner_of,
        gvp:ulan1548_domestic_partner_of,
        gvp:ulan1550_relative_by_marriage,
        gvp:ulan1551_sibling_by_marriage_of,
        gvp:ulan1552_parent_by_marriage_of,
        gvp:ulan1553_child_by_marriage_of,
        gvp:ulan1554_adoptive_parent_of,
        gvp:ulan1555_adopted_child_of,
        gvp:ulan1556_half-sibling_of,
        gvp:ulan1557_step-sibling_of,
        gvp:ulan1561_step-child_of,
        gvp:ulan1562_step-parent_of,
        gvp:ulan1571_guardian_of,
        gvp:ulan1573_ward_of,
        gvp:ulan1574_godparent_of,
        gvp:ulan1575_godchild_of,
        gvp:ulan1581_descendant_of,
        gvp:ulan1582_ancestor_of,
        gvp:ulan1590_possibly_related_to,
        gvp:ulan2550_friend_of,
        gvp:ulan2572_founder_of,
        gvp:ulan2573_founded_by,
        gvp:ulan2574_director_of,
        gvp:ulan2575_directed_by,
        gvp:ulan2576_patron_of,
        gvp:ulan2577_patron_was,
        gvp:ulan2578_trustee_of,
        gvp:ulan2579_trustee_was,
        gvp:ulan2581_administrator_of,
        gvp:ulan2582_administered_by,
        gvp:ulan2583_chairman_of,
        gvp:ulan2584_chaired_by,
        gvp:ulan2650_publisher_was,
        gvp:ulan2651_publisher_of,
        gvp:ulan2674_professor_at,
        gvp:ulan2675_professor_was,
        gvp:ulan2676_teacher_at,
        gvp:ulan2677_teacher_was,
        gvp:ulan2692_president_of,
        gvp:ulan2693_president_was,
        gvp:ulan2696_leader_of,
        gvp:ulan2697_leader_was,
        gvp:ulan2778_owner_of,
        gvp:ulan2779_owned_by,
        gvp:ulan2781_dedicatee_of,
        gvp:ulan2782_dedicated_to,
        gvp:ulan2794_representative_of,
        gvp:ulan2795_representative_was,
        gvp:ulan2828_student_at,
        gvp:ulan2829_student_was,
        gvp:ulan2840_performer_with,
        gvp:ulan2841_performer_was .

skos:Concept skos:narrower gvp:Concept,
        gvp:GroupConcept,
        gvp:PersonConcept,
        gvp:PhysPlaceConcept,
        gvp:UnknownPersonConcept .

<http://vocab.getty.edu/ontology> a voaf:Vocabulary,
        owl:Ontology,
        skos:ConceptScheme ;
    rdfs:label "Getty Vocabulary Program ontology"@en ;
    dc:format "meta/rdf-schema" ;
    dct:created "2014-02-15"^^xsd:date ;
    dct:creator <http://www.getty.edu/research/>,
        <http://www.ontotext.com> ;
    dct:issued "2014-02-20"^^xsd:date ;
    dct:modified "2016-04-25"^^xsd:date ;
    vann:preferredNamespacePrefix "gvp" ;
    vann:preferredNamespaceUri "http://vocab.getty.edu/ontology#" ;
    rdfs:comment """The GVP Ontology defines classes, properties and values (skos:Concepts) used in GVP LOD.
As of version 3.0, it is complete regarding AAT, TGN and ULAN, and will be extended in time with more elements needed for other GVP vocabularies (CONA).
It uses the SKOS, SKOS-XL, ISO 25964; DC, DCT, BIBO, FOAF, BIO, Schema, PROV, WGS84 ontologies, but we import only the first 3""" ;
    rdfs:seeAlso <http://lov.okfn.org/dataset/lov/details/vocabulary_gvp.html>,
        <http://vocab.getty.edu/.well-known/void>,
        <http://vocab.getty.edu/doc>,
        <http://vocab.getty.edu/doc/queries>,
        <http://www.getty.edu/research/tools/vocabularies/lod/> ;
    owl:imports <http://purl.org/iso25964/skos-thes>,
        <http://www.w3.org/2004/02/skos/core>,
        <http://www.w3.org/2008/05/skos-xl> ;
    owl:versionInfo "3.3" ;
    skos:changeNote <http://vocab.getty.edu/doc#Version_2.0>,
        <http://vocab.getty.edu/doc#Version_3.0>,
        <http://vocab.getty.edu/doc#Version_3.3>,
        """2.0 changes: replaced gvp:broaderTransitive with gvp:broaderExtended.
3.0 changes: replaced schema:startDate, endDate with gvp:estStart, estEnd; added ULAN). See details in referenced links.
3.1 & 3.2: no changes.
3.3: added 6 associative relations: gvp:aat2886_used-function_as - gvp:aat2887_exemplified_by, gvp:tgn3103_located_on - gvp:tgn3104_is_location_of, and gvp:ulan2583_chairman_of - gvp:ulan2584_chaired_by""" ;
    skos:hasTopConcept schema:dissolutionLocation,
        <http://vocab.getty.edu/historic/>,
        gvp:AdminPlaceConcept,
        gvp:Biography,
        gvp:Concept,
        gvp:Facet,
        gvp:GroupConcept,
        gvp:GuideTerm,
        gvp:Hierarchy,
        gvp:ObsoleteSubject,
        gvp:PersonConcept,
        gvp:PhysAdminPlaceConcept,
        gvp:PhysPlaceConcept,
        gvp:ScopeNote,
        gvp:Subject,
        gvp:UnknownPersonConcept,
        gvp:aat2000_related_to,
        gvp:aat2001_formerly_referred_to,
        gvp:aat2100_distinguished_from,
        gvp:aat2110_meaning-usage_overlaps_with,
        gvp:aat2203_associated_with,
        gvp:aat2205_causes-is_required,
        gvp:aat2206_caused_by-requires,
        gvp:aat2208_locus-setting_for,
        gvp:aat2209_used-located_in,
        gvp:aat2211_produce,
        gvp:aat2212_produced_by,
        gvp:aat2215_required_for,
        gvp:aat2216_require,
        gvp:aat2218_used-function_as,
        gvp:aat2219_have_form,
        gvp:aat2221_act_upon,
        gvp:aat2222_are_acted_upon,
        gvp:aat2281_have_counterpart,
        gvp:aat2285_practiced-studied_by,
        gvp:aat2286_practice-study,
        gvp:aat2291_locus-setting_for,
        gvp:aat2292_work-live_in,
        gvp:aat2294_locus-setting_for,
        gvp:aat2295_located_in,
        gvp:aat2311_performed_by,
        gvp:aat2312_perform,
        gvp:aat2315_used_by,
        gvp:aat2316_use,
        gvp:aat2318_involved_in,
        gvp:aat2319_involves,
        gvp:aat2321_used_by,
        gvp:aat2322_use,
        gvp:aat2325_created_by,
        gvp:aat2326_create,
        gvp:aat2328_involved_with,
        gvp:aat2329_involves,
        gvp:aat2332_affiliated_with,
        gvp:aat2333_have_affiliates,
        gvp:aat2335_associated_with,
        gvp:aat2336_has_associates,
        gvp:aat2397_focus_of,
        gvp:aat2398_focuses_on,
        gvp:aat2408_locus-setting_for,
        gvp:aat2409_takes_place_in,
        gvp:aat2411_involved_in,
        gvp:aat2412_involves,
        gvp:aat2415_required_for,
        gvp:aat2416_requires,
        gvp:aat2418_uses,
        gvp:aat2419_used_for,
        gvp:aat2421_locus-setting_for,
        gvp:aat2422_takes_place_in,
        gvp:aat2424_produced_by,
        gvp:aat2425_produces,
        gvp:aat2427_produced_by,
        gvp:aat2428_produces,
        gvp:aat2431_required_for,
        gvp:aat2432_requires,
        gvp:aat2434_contextualized_in,
        gvp:aat2435_context_for,
        gvp:aat2501_made_of-require,
        gvp:aat2502_material_for,
        gvp:aat2504_used-located_in,
        gvp:aat2505_locus-setting_for,
        gvp:aat2507_produce-process,
        gvp:aat2508_produced-processed_by,
        gvp:aat2551_reflect-produced_by,
        gvp:aat2552_reflected_in-produces,
        gvp:aat2554_reflects,
        gvp:aat2555_reflected_in,
        gvp:aat2557_reflects,
        gvp:aat2558_reflected_in,
        gvp:aat2562_locus-setting_for,
        gvp:aat2563_located_in,
        gvp:aat2601_possessed_by-existing_in,
        gvp:aat2602_possess-exist_in,
        gvp:aat2604_possessed_by-existing_in,
        gvp:aat2605_possess-exist_in,
        gvp:aat2607_caused_by-requires,
        gvp:aat2608_causes-required_for,
        gvp:aat2612_possessed_by-existing_in,
        gvp:aat2613_possess-exist_in,
        gvp:aat2801_conjuncted_with,
        gvp:aat2802_exemplified_by,
        gvp:aat2803_example_of,
        gvp:aat2805_contextualized_in,
        gvp:aat2806_provide_context,
        gvp:aat2807_derived_from_common_source,
        gvp:aat2809_coexisted_with,
        gvp:aat2811_preceded,
        gvp:aat2812_followed,
        gvp:aat2814_constituent_of,
        gvp:aat2815_composed_of,
        gvp:aat2817_derived-made_from,
        gvp:aat2818_source_for,
        gvp:aat2821_based_on,
        gvp:aat2822_basis_of,
        gvp:aat2824_has_parallels_with,
        gvp:aat2826_used_with,
        gvp:aat2828_use-require,
        gvp:aat2829_used-required_for,
        gvp:aat2831_associated_with,
        gvp:aat2833_ancestor_of,
        gvp:aat2834_decendant_of,
        gvp:aat2836_derived-made_from,
        gvp:aat2837_source_for,
        gvp:aat2841_derived-made_from,
        gvp:aat2842_source_for,
        gvp:aat2845_used-located_in,
        gvp:aat2846_locus-setting_for,
        gvp:aat2848_involved_in,
        gvp:aat2849_involves,
        gvp:aat2852_involved_with,
        gvp:aat2853_involve,
        gvp:aat2875_characteristic_of,
        gvp:aat2876_characterized_by,
        gvp:aat2878_preceded-source_for,
        gvp:aat2879_followed-developed_from,
        gvp:aat2881_reflected_in,
        gvp:aat2882_reflect,
        gvp:aat2884_involved_with,
        gvp:aat2885_involves,
        gvp:aat2886_used-function_as,
        gvp:aat2887_exemplified_by,
        gvp:aat2891_exemplified_by,
        gvp:aat2892_example_of,
        gvp:aat2894_exemplified_by,
        gvp:aat2895_example_of,
        gvp:aat2900_miscellaneous_relationship,
        gvp:agentType,
        gvp:agentTypeNonPreferred,
        gvp:agentTypePreferred,
        gvp:biography,
        gvp:biographyNonPreferred,
        gvp:biographyPreferred,
        gvp:broader,
        gvp:broaderExtended,
        gvp:broaderGeneric,
        gvp:broaderGenericExtended,
        gvp:broaderInstantial,
        gvp:broaderInstantialExtended,
        gvp:broaderNonConcept,
        gvp:broaderNonPreferred,
        gvp:broaderPartitive,
        gvp:broaderPartitiveExtended,
        gvp:broaderPreferred,
        gvp:broaderPreferredExtended,
        gvp:contributorAlternatePreferred,
        gvp:contributorNonPreferred,
        gvp:contributorPreferred,
        gvp:displayOrder,
        gvp:estEnd,
        gvp:estStart,
        gvp:eventNonPreferred,
        gvp:eventPreferred,
        gvp:historicFlag,
        gvp:isNoted,
        gvp:nationalityNonPreferred,
        gvp:nationalityPreferred,
        gvp:parentString,
        gvp:parentStringAbbrev,
        gvp:placeType,
        gvp:placeTypeNonPreferred,
        gvp:placeTypePreferred,
        gvp:prefLabelGVP,
        gvp:prefLabelLoC,
        gvp:qualifier,
        gvp:sourceAlternatePreferred,
        gvp:sourceNonPreferred,
        gvp:sourcePreferred,
        gvp:term,
        gvp:termDisplay,
        gvp:termFlag,
        gvp:termKind,
        gvp:termPOS,
        gvp:termType,
        gvp:tgn3000_related_to,
        gvp:tgn3001_distinguished_from,
        gvp:tgn3005_possibly_identified_as,
        gvp:tgn3006_formerly_identified_as,
        gvp:tgn3101_near-adjacent_to,
        gvp:tgn3102_coextensive_with,
        gvp:tgn3103_located_on,
        gvp:tgn3104_is_location_of,
        gvp:tgn3110_meaning-usage_overlaps_with,
        gvp:tgn3201_capital_of,
        gvp:tgn3202_capital_is,
        gvp:tgn3301_ally_of,
        gvp:tgn3317_member_of,
        gvp:tgn3318_member_is,
        gvp:tgn3401_moved_from,
        gvp:tgn3402_moved_to,
        gvp:tgn3411_successor_of,
        gvp:tgn3412_predecessor_of,
        gvp:tgn3510_historical_connection,
        gvp:tgn3611_administrative_dependent_of,
        gvp:tgn3612_administrative_entity_for,
        gvp:ulan1000_related_to,
        gvp:ulan1003_associated_with,
        gvp:ulan1005_possibly_identified_with,
        gvp:ulan1006_formerly_identified_with,
        gvp:ulan1007_distinguished_from,
        gvp:ulan1008_meaning_-usage_overlaps_with,
        gvp:ulan1101_teacher_of,
        gvp:ulan1102_student_of,
        gvp:ulan1105_apprentice_of,
        gvp:ulan1106_apprentice_was,
        gvp:ulan1107_influenced,
        gvp:ulan1108_influenced_by,
        gvp:ulan1111_master_of,
        gvp:ulan1112_master_was,
        gvp:ulan1113_fellow_student_of,
        gvp:ulan1201_patron_of,
        gvp:ulan1202_patron_was,
        gvp:ulan1203_donor_of,
        gvp:ulan1204_donor_was,
        gvp:ulan1205_client_of,
        gvp:ulan1206_client_was,
        gvp:ulan1211_artist_to,
        gvp:ulan1212_artist_was,
        gvp:ulan1213_court_artist_to,
        gvp:ulan1214_court_artist_was,
        gvp:ulan1217_employee_of,
        gvp:ulan1218_employee_was,
        gvp:ulan1221_appointed_by,
        gvp:ulan1222_appointee_of,
        gvp:ulan1223_crowned_by,
        gvp:ulan1224_crowned,
        gvp:ulan1301_colleague_of,
        gvp:ulan1302_associate_of,
        gvp:ulan1303_collaborated_with,
        gvp:ulan1305_worked_with,
        gvp:ulan1306_performs_with,
        gvp:ulan1307_assistant_of,
        gvp:ulan1308_assisted_by,
        gvp:ulan1309_advisor_of,
        gvp:ulan1310_advised_by,
        gvp:ulan1311_partner_of,
        gvp:ulan1313_partner_in,
        gvp:ulan1314_partner_was,
        gvp:ulan1315_principal_in,
        gvp:ulan1316_principal_was,
        gvp:ulan1317_member_of,
        gvp:ulan1318_member_was,
        gvp:ulan1321_school_of,
        gvp:ulan1322_school_was,
        gvp:ulan1331_worked_with,
        gvp:ulan1332_worker_was,
        gvp:ulan1411_successor_of,
        gvp:ulan1412_predecessor_of,
        gvp:ulan1413_administration_overlaps_with,
        gvp:ulan1414_joint_venture_with,
        gvp:ulan1421_founded_by,
        gvp:ulan1422_founded,
        gvp:ulan1500_related_to,
        gvp:ulan1501_sibling_of,
        gvp:ulan1511_child_of,
        gvp:ulan1512_parent_of,
        gvp:ulan1513_grandchild_of,
        gvp:ulan1514_gandparent_of,
        gvp:ulan1515_great-grandparent_of,
        gvp:ulan1516_great-grandchild_of,
        gvp:ulan1521_cousin_of,
        gvp:ulan1531_nephew-niece_of,
        gvp:ulan1532_uncle-aunt_of,
        gvp:ulan1541_spouse_of,
        gvp:ulan1542_consort_of,
        gvp:ulan1543_consort_was,
        gvp:ulan1544_significant_other_of,
        gvp:ulan1547_romantic_partner_of,
        gvp:ulan1548_domestic_partner_of,
        gvp:ulan1550_relative_by_marriage,
        gvp:ulan1551_sibling_by_marriage_of,
        gvp:ulan1552_parent_by_marriage_of,
        gvp:ulan1553_child_by_marriage_of,
        gvp:ulan1554_adoptive_parent_of,
        gvp:ulan1555_adopted_child_of,
        gvp:ulan1556_half-sibling_of,
        gvp:ulan1557_step-sibling_of,
        gvp:ulan1561_step-child_of,
        gvp:ulan1562_step-parent_of,
        gvp:ulan1571_guardian_of,
        gvp:ulan1573_ward_of,
        gvp:ulan1574_godparent_of,
        gvp:ulan1575_godchild_of,
        gvp:ulan1581_descendant_of,
        gvp:ulan1582_ancestor_of,
        gvp:ulan1590_possibly_related_to,
        gvp:ulan2550_friend_of,
        gvp:ulan2572_founder_of,
        gvp:ulan2573_founded_by,
        gvp:ulan2574_director_of,
        gvp:ulan2575_directed_by,
        gvp:ulan2576_patron_of,
        gvp:ulan2577_patron_was,
        gvp:ulan2578_trustee_of,
        gvp:ulan2579_trustee_was,
        gvp:ulan2581_administrator_of,
        gvp:ulan2582_administered_by,
        gvp:ulan2583_chairman_of,
        gvp:ulan2584_chaired_by,
        gvp:ulan2650_publisher_was,
        gvp:ulan2651_publisher_of,
        gvp:ulan2674_professor_at,
        gvp:ulan2675_professor_was,
        gvp:ulan2676_teacher_at,
        gvp:ulan2677_teacher_was,
        gvp:ulan2692_president_of,
        gvp:ulan2693_president_was,
        gvp:ulan2696_leader_of,
        gvp:ulan2697_leader_was,
        gvp:ulan2778_owner_of,
        gvp:ulan2779_owned_by,
        gvp:ulan2781_dedicatee_of,
        gvp:ulan2782_dedicated_to,
        gvp:ulan2794_representative_of,
        gvp:ulan2795_representative_was,
        gvp:ulan2828_student_at,
        gvp:ulan2829_student_was,
        gvp:ulan2840_performer_with,
        gvp:ulan2841_performer_was,
        <http://vocab.getty.edu/term/POS/>,
        <http://vocab.getty.edu/term/display/>,
        <http://vocab.getty.edu/term/flag/>,
        <http://vocab.getty.edu/term/kind/>,
        <http://vocab.getty.edu/term/type/> ;
    skos:prefLabel "Getty Vocabulary Program ontology"@en .

