<?xml version="1.0" encoding="UTF-8"?>
<rdf:RDF
   xmlns:dc="http://purl.org/dc/elements/1.1/"
   xmlns:dct="http://purl.org/dc/terms/"
   xmlns:foaf="http://xmlns.com/foaf/0.1/"
   xmlns:owl="http://www.w3.org/2002/07/owl#"
   xmlns:ptop="http://www.ontotext.com/proton/protontop#"
   xmlns:rdf="http://www.w3.org/1999/02/22-rdf-syntax-ns#"
   xmlns:rdfs="http://www.w3.org/2000/01/rdf-schema#"
   xmlns:skos="http://www.w3.org/2004/02/skos/core#"
   xmlns:vann="http://purl.org/vocab/vann/"
>
  <rdf:Description rdf:about="http://vocab.getty.edu/ontology#aat2216_require">
    <skos:example>broderie anglaise requires eyelets</skos:example>
    <dc:title>require - things</dc:title>
    <rdfs:isDefinedBy rdf:resource="http://vocab.getty.edu/ontology"/>
    <rdfs:subPropertyOf rdf:resource="http://www.w3.org/2004/02/skos/core#related"/>
    <skos:example>compact disc players require compact discs</skos:example>
    <dc:identifier>2216</dc:identifier>
    <rdf:type rdf:resource="http://www.w3.org/2002/07/owl#ObjectProperty"/>
    <rdfs:isDefinedBy rdf:resource="http://vocab.getty.edu/aat/"/>
    <skos:prefLabel>aat2216_require</skos:prefLabel>
    <rdfs:range rdf:resource="http://www.w3.org/2004/02/skos/core#Concept"/>
    <dct:description>things - require - things [in order to exist or work].&#13;
Example: broderie anglaise requires eyelets; compact disc players require compact discs</dct:description>
    <rdfs:domain rdf:resource="http://www.w3.org/2004/02/skos/core#Concept"/>
  </rdf:Description>
  <rdf:Description rdf:about="http://vocab.getty.edu/ontology#aat2818_source_for">
    <rdfs:subPropertyOf rdf:resource="http://www.w3.org/2004/02/skos/core#related"/>
    <rdfs:range rdf:resource="http://www.w3.org/2004/02/skos/core#Concept"/>
    <rdfs:isDefinedBy rdf:resource="http://vocab.getty.edu/ontology"/>
    <dc:identifier>2818</dc:identifier>
    <skos:example>timber (lumber) is the source for wood board</skos:example>
    <rdfs:domain rdf:resource="http://www.w3.org/2004/02/skos/core#Concept"/>
    <skos:prefLabel>aat2818_source_for</skos:prefLabel>
    <dc:title>source for - material</dc:title>
    <skos:example>anhydrite is the source for gypsum</skos:example>
    <dct:description>material - [is] source for - material.&#13;
Example: anhydrite is the source for gypsum; timber (lumber) is the source for wood board</dct:description>
    <rdf:type rdf:resource="http://www.w3.org/2002/07/owl#ObjectProperty"/>
    <rdfs:isDefinedBy rdf:resource="http://vocab.getty.edu/aat/"/>
  </rdf:Description>
  <rdf:Description rdf:about="http://vocab.getty.edu/ontology#Infer_isoBroaderGeneric">
    <ptop:premise rdf:resource="http://vocab.getty.edu/ontology#broaderGenericExtended"/>
    <rdf:type rdf:resource="http://www.ontotext.com/proton/protontop#PropRestr"/>
    <ptop:conclusion rdf:resource="http://purl.org/iso25964/skos-thes#broaderGeneric"/>
    <ptop:restriction rdf:resource="http://www.w3.org/2004/02/skos/core#broader"/>
  </rdf:Description>
  <rdf:Description rdf:about="http://vocab.getty.edu/ontology#aat2412_involves">
    <skos:prefLabel>aat2412_involves</skos:prefLabel>
    <rdfs:domain rdf:resource="http://www.w3.org/2004/02/skos/core#Concept"/>
    <dc:identifier>2412</dc:identifier>
    <rdfs:range rdf:resource="http://www.w3.org/2004/02/skos/core#Concept"/>
    <rdfs:isDefinedBy rdf:resource="http://vocab.getty.edu/ontology"/>
    <skos:example>photojournalism (discipline) involves journalistic photography</skos:example>
    <dct:description>field/discipline - involves - activity/event/[process/function].&#13;
Example: photojournalism (discipline) involves journalistic photography; horticulture involves gardening</dct:description>
    <skos:example>horticulture involves gardening</skos:example>
    <rdfs:isDefinedBy rdf:resource="http://vocab.getty.edu/aat/"/>
    <rdf:type rdf:resource="http://www.w3.org/2002/07/owl#ObjectProperty"/>
    <dc:title>involves - activity/event</dc:title>
    <rdfs:subPropertyOf rdf:resource="http://www.w3.org/2004/02/skos/core#related"/>
  </rdf:Description>
  <rdf:Description rdf:about="http://vocab.getty.edu/ontology#aat2608_causes-required_for">
    <rdfs:domain rdf:resource="http://www.w3.org/2004/02/skos/core#Concept"/>
    <rdfs:subPropertyOf rdf:resource="http://www.w3.org/2004/02/skos/core#related"/>
    <rdfs:isDefinedBy rdf:resource="http://vocab.getty.edu/ontology"/>
    <skos:prefLabel>aat2608_causes-required_for</skos:prefLabel>
    <rdfs:isDefinedBy rdf:resource="http://vocab.getty.edu/aat/"/>
    <dct:description>activity/event/[process/function] - causes/[is] required for - [a] state/condition/attributes.&#13;
Example: waterproofing causes/is required for watertighness; creasing (process) causes/is required for creases (condition)</dct:description>
    <rdf:type rdf:resource="http://www.w3.org/2002/07/owl#ObjectProperty"/>
    <dc:identifier>2608</dc:identifier>
    <skos:example>creasing (process) causes/is required for creases (condition)</skos:example>
    <rdfs:range rdf:resource="http://www.w3.org/2004/02/skos/core#Concept"/>
    <dc:title>causes/required for - attributes /associated concepts</dc:title>
    <skos:example>waterproofing causes/is required for watertighness</skos:example>
  </rdf:Description>
  <rdf:Description rdf:about="http://vocab.getty.edu/ontology#ulan2781_dedicatee_of">
    <rdfs:domain rdf:resource="http://www.w3.org/2004/02/skos/core#Concept"/>
    <rdfs:subPropertyOf rdf:resource="http://www.w3.org/2004/02/skos/core#related"/>
    <rdfs:isDefinedBy rdf:resource="http://vocab.getty.edu/ontology"/>
    <skos:prefLabel>ulan2781_dedicatee_of</skos:prefLabel>
    <owl:inverseOf rdf:resource="http://vocab.getty.edu/ontology#ulan2782_dedicated_to"/>
    <rdfs:isDefinedBy rdf:resource="http://vocab.getty.edu/ulan/"/>
    <rdf:type rdf:resource="http://www.w3.org/2002/07/owl#ObjectProperty"/>
    <rdfs:range rdf:resource="http://www.w3.org/2004/02/skos/core#Concept"/>
    <dc:identifier>2781</dc:identifier>
    <dc:title>dedicatee of - institution</dc:title>
    <dct:description>person - dedicatee of - institution.&#13;
Example: Auguste Rodin is the dedicatee of The Rodin Museum in Philadelphia</dct:description>
    <skos:example>Auguste Rodin is the dedicatee of The Rodin Museum in Philadelphia</skos:example>
  </rdf:Description>
  <rdf:Description rdf:about="http://vocab.getty.edu/ontology#ulan1581_descendant_of">
    <rdf:type rdf:resource="http://www.w3.org/2002/07/owl#ObjectProperty"/>
    <dct:description>person - descendant of - person.&#13;
Example: Paolo Caliari is the descendant of Paolo Veronese</dct:description>
    <rdfs:range rdf:resource="http://www.w3.org/2004/02/skos/core#Concept"/>
    <dc:title>descendant of - person</dc:title>
    <rdfs:isDefinedBy rdf:resource="http://vocab.getty.edu/ontology"/>
    <rdfs:domain rdf:resource="http://www.w3.org/2004/02/skos/core#Concept"/>
    <dc:identifier>1581</dc:identifier>
    <skos:example>Paolo Caliari is the descendant of Paolo Veronese</skos:example>
    <skos:prefLabel>ulan1581_descendant_of</skos:prefLabel>
    <rdfs:isDefinedBy rdf:resource="http://vocab.getty.edu/ulan/"/>
    <rdfs:subPropertyOf rdf:resource="http://www.w3.org/2004/02/skos/core#related"/>
    <owl:inverseOf rdf:resource="http://vocab.getty.edu/ontology#ulan1582_ancestor_of"/>
  </rdf:Description>
  <rdf:Description rdf:about="http://vocab.getty.edu/ontology#ulan1555_adopted_child_of">
    <skos:prefLabel>ulan1555_adopted_child_of</skos:prefLabel>
    <rdf:type rdf:resource="http://www.w3.org/2002/07/owl#ObjectProperty"/>
    <dc:identifier>1555</dc:identifier>
    <dc:title>adopted child of - person</dc:title>
    <rdfs:isDefinedBy rdf:resource="http://vocab.getty.edu/ulan/"/>
    <dct:description>person - adopted child of - person.&#13;
Example: Augusts, Emperor of Rome is the adopted child of Julius Caesar</dct:description>
    <rdfs:isDefinedBy rdf:resource="http://vocab.getty.edu/ontology"/>
    <rdfs:subPropertyOf rdf:resource="http://www.w3.org/2004/02/skos/core#related"/>
    <rdfs:domain rdf:resource="http://www.w3.org/2004/02/skos/core#Concept"/>
    <rdfs:range rdf:resource="http://www.w3.org/2004/02/skos/core#Concept"/>
    <skos:example>Augusts, Emperor of Rome is the adopted child of Julius Caesar</skos:example>
  </rdf:Description>
  <rdf:Description rdf:about="http://vocab.getty.edu/ontology#aat2291_locus-setting_for">
    <skos:prefLabel>aat2291_locus-setting_for</skos:prefLabel>
    <rdfs:subPropertyOf rdf:resource="http://www.w3.org/2004/02/skos/core#related"/>
    <skos:example>libraries (buildings) are the locus/setting of libraries (institutions)</skos:example>
    <dc:identifier>2291</dc:identifier>
    <rdfs:domain rdf:resource="http://www.w3.org/2004/02/skos/core#Concept"/>
    <skos:example>roperies are the locus/setting of rope-makers</skos:example>
    <rdfs:isDefinedBy rdf:resource="http://vocab.getty.edu/ontology"/>
    <dc:title>locus/setting for - role</dc:title>
    <rdfs:range rdf:resource="http://www.w3.org/2004/02/skos/core#Concept"/>
    <owl:inverseOf rdf:resource="http://vocab.getty.edu/ontology#aat2292_work-live_in"/>
    <dct:description>locus/setting - [is] locus setting for - [actor or institution having] role.&#13;
Example: roperies are the locus/setting of rope-makers; convents (built complexes) are the locus/setting of nuns; libraries (buildings) are the locus/setting of libraries (institutions)</dct:description>
    <rdf:type rdf:resource="http://www.w3.org/2002/07/owl#ObjectProperty"/>
    <rdfs:isDefinedBy rdf:resource="http://vocab.getty.edu/aat/"/>
    <skos:example>convents (built complexes) are the locus/setting of nuns</skos:example>
  </rdf:Description>
  <rdf:Description rdf:nodeID="N8c1a90bd131243c0ae4503ccea2e2fb7">
    <rdf:rest rdf:nodeID="N902632d785fc4cb0b1919bc211810e50"/>
    <rdf:first rdf:resource="http://www.w3.org/2008/05/skos-xl#hiddenLabel"/>
  </rdf:Description>
  <rdf:Description rdf:about="http://vocab.getty.edu/ontology#ulan1217_employee_of">
    <rdf:type rdf:resource="http://www.w3.org/2002/07/owl#ObjectProperty"/>
    <rdfs:range rdf:resource="http://www.w3.org/2004/02/skos/core#Concept"/>
    <dct:description>person/firm - employee of - person.&#13;
Example: Employee of Christopher Wren was Jean Tijou</dct:description>
    <rdfs:isDefinedBy rdf:resource="http://vocab.getty.edu/ontology"/>
    <skos:prefLabel>ulan1217_employee_of</skos:prefLabel>
    <rdfs:domain rdf:resource="http://www.w3.org/2004/02/skos/core#Concept"/>
    <skos:example>Employee of Christopher Wren was Jean Tijou</skos:example>
    <dc:title>employee of - person</dc:title>
    <rdfs:isDefinedBy rdf:resource="http://vocab.getty.edu/ulan/"/>
    <owl:inverseOf rdf:resource="http://vocab.getty.edu/ontology#ulan1218_employee_was"/>
    <dc:identifier>1217</dc:identifier>
    <rdfs:subPropertyOf rdf:resource="http://www.w3.org/2004/02/skos/core#related"/>
  </rdf:Description>
  <rdf:Description rdf:about="http://vocab.getty.edu/ontology#aat2424_produced_by">
    <rdfs:isDefinedBy rdf:resource="http://vocab.getty.edu/ontology"/>
    <dct:description>material - [is] produced by - activity/event/process.&#13;
Example: wire is produced by wiredrawing; paper is produced by papermaking</dct:description>
    <skos:example>paper is produced by papermaking</skos:example>
    <rdfs:domain rdf:resource="http://www.w3.org/2004/02/skos/core#Concept"/>
    <rdfs:subPropertyOf rdf:resource="http://www.w3.org/2004/02/skos/core#related"/>
    <skos:prefLabel>aat2424_produced_by</skos:prefLabel>
    <rdfs:range rdf:resource="http://www.w3.org/2004/02/skos/core#Concept"/>
    <skos:example>wire is produced by wiredrawing</skos:example>
    <dc:identifier>2424</dc:identifier>
    <rdf:type rdf:resource="http://www.w3.org/2002/07/owl#ObjectProperty"/>
    <rdfs:isDefinedBy rdf:resource="http://vocab.getty.edu/aat/"/>
    <dc:title>produced by - activity/event/process</dc:title>
    <owl:inverseOf rdf:resource="http://vocab.getty.edu/ontology#aat2425_produces"/>
  </rdf:Description>
  <rdf:Description rdf:about="http://vocab.getty.edu/ontology#ulan1548_domestic_partner_of">
    <rdf:type rdf:resource="http://www.w3.org/2002/07/owl#SymmetricProperty"/>
    <rdfs:subPropertyOf rdf:resource="http://www.w3.org/2004/02/skos/core#related"/>
    <rdfs:isDefinedBy rdf:resource="http://vocab.getty.edu/ontology"/>
    <dc:title>domestic partner of - person</dc:title>
    <dct:description>person - domestic partner of - person</dct:description>
    <rdfs:isDefinedBy rdf:resource="http://vocab.getty.edu/ulan/"/>
    <rdf:type rdf:resource="http://www.w3.org/2002/07/owl#ObjectProperty"/>
    <skos:prefLabel>ulan1548_domestic_partner_of</skos:prefLabel>
    <rdfs:range rdf:resource="http://www.w3.org/2004/02/skos/core#Concept"/>
    <rdfs:domain rdf:resource="http://www.w3.org/2004/02/skos/core#Concept"/>
    <dc:identifier>1548</dc:identifier>
  </rdf:Description>
  <rdf:Description rdf:about="http://vocab.getty.edu/ontology#ulan1553_child_by_marriage_of">
    <rdf:type rdf:resource="http://www.w3.org/2002/07/owl#ObjectProperty"/>
    <skos:example>Pieter Gerritsz van Roestraten is the child by marriage of Frans Hals</skos:example>
    <rdfs:range rdf:resource="http://www.w3.org/2004/02/skos/core#Concept"/>
    <dct:description>person - child by marriage (step child) - person.&#13;
Example: Pieter Gerritsz van Roestraten is the child by marriage of Frans Hals</dct:description>
    <dc:identifier>1553</dc:identifier>
    <skos:prefLabel>ulan1553_child_by_marriage_of</skos:prefLabel>
    <rdfs:domain rdf:resource="http://www.w3.org/2004/02/skos/core#Concept"/>
    <rdfs:isDefinedBy rdf:resource="http://vocab.getty.edu/ontology"/>
    <rdfs:isDefinedBy rdf:resource="http://vocab.getty.edu/ulan/"/>
    <rdfs:subPropertyOf rdf:resource="http://www.w3.org/2004/02/skos/core#related"/>
    <dc:title>child by marriage of - person</dc:title>
  </rdf:Description>
  <rdf:Description rdf:about="http://vocab.getty.edu/ontology#ulan1315_principal_in">
    <rdfs:isDefinedBy rdf:resource="http://vocab.getty.edu/ulan/"/>
    <rdfs:subPropertyOf rdf:resource="http://www.w3.org/2004/02/skos/core#related"/>
    <rdfs:domain rdf:resource="http://www.w3.org/2004/02/skos/core#Concept"/>
    <dct:description>person - principal in - firm.&#13;
Example: Principal in Fontana Workshop was Orazio Fontana</dct:description>
    <skos:example>Principal in Fontana Workshop was Orazio Fontana</skos:example>
    <dc:identifier>1315</dc:identifier>
    <rdfs:isDefinedBy rdf:resource="http://vocab.getty.edu/ontology"/>
    <owl:inverseOf rdf:resource="http://vocab.getty.edu/ontology#ulan1316_principal_was"/>
    <rdfs:range rdf:resource="http://www.w3.org/2004/02/skos/core#Concept"/>
    <rdf:type rdf:resource="http://www.w3.org/2002/07/owl#ObjectProperty"/>
    <skos:prefLabel>ulan1315_principal_in</skos:prefLabel>
    <dc:title>principal in - firm</dc:title>
  </rdf:Description>
  <rdf:Description rdf:about="http://vocab.getty.edu/term/display/Indexing">
    <skos:notation>I</skos:notation>
    <dct:description>Use in indexes or permuted lists where inverted order is appropriate</dct:description>
    <skos:scopeNote>Use in indexes or permuted lists where inverted order is appropriate</skos:scopeNote>
    <rdf:type rdf:resource="http://www.w3.org/2004/02/skos/core#Concept"/>
    <skos:prefLabel>Use in Indexes/lists</skos:prefLabel>
    <skos:inScheme rdf:resource="http://vocab.getty.edu/term/display/"/>
  </rdf:Description>
  <rdf:Description rdf:about="http://vocab.getty.edu/term/kind/FullTerm">
    <rdf:type rdf:resource="http://www.w3.org/2004/02/skos/core#Concept"/>
    <dct:description>Full-form term. Used when the descriptor is a shorter form, or the subject also includes an Abbreviation. Used in AAT only.
Example: "Extensible Markup Language" is the full term for "XML" (which is preferred)</dct:description>
    <skos:scopeNote>Full-form term. Used when the descriptor is a shorter form, or the subject also includes an Abbreviation. Used in AAT only</skos:scopeNote>
    <skos:example>"Extensible Markup Language" is the full term for "XML" (which is preferred)</skos:example>
    <skos:notation>F</skos:notation>
    <skos:inScheme rdf:resource="http://vocab.getty.edu/term/kind/"/>
    <skos:prefLabel>Full term</skos:prefLabel>
  </rdf:Description>
  <rdf:Description rdf:about="http://vocab.getty.edu/ontology#aat2828_use-require">
    <skos:example>oil paintings use/require varnish</skos:example>
    <owl:inverseOf rdf:resource="http://vocab.getty.edu/ontology#aat2829_used-required_for"/>
    <rdfs:domain rdf:resource="http://www.w3.org/2004/02/skos/core#Concept"/>
    <dct:description>things - use/require - material.&#13;
Example: oil paintings use/require varnish; wine glasses use/require wine</dct:description>
    <dc:identifier>2828</dc:identifier>
    <skos:example>wine glasses use/require wine</skos:example>
    <rdfs:isDefinedBy rdf:resource="http://vocab.getty.edu/ontology"/>
    <skos:prefLabel>aat2828_use-require</skos:prefLabel>
    <dc:title>use/require - material</dc:title>
    <rdfs:range rdf:resource="http://www.w3.org/2004/02/skos/core#Concept"/>
    <rdfs:isDefinedBy rdf:resource="http://vocab.getty.edu/aat/"/>
    <rdfs:subPropertyOf rdf:resource="http://www.w3.org/2004/02/skos/core#related"/>
    <rdf:type rdf:resource="http://www.w3.org/2002/07/owl#ObjectProperty"/>
  </rdf:Description>
  <rdf:Description rdf:about="http://vocab.getty.edu/ontology#placeTypePreferred">
    <rdfs:range rdf:resource="http://vocab.getty.edu/ontology#Subject"/>
    <rdfs:domain rdf:resource="http://vocab.getty.edu/ontology#Subject"/>
    <skos:example>The preferred place type of Machupicchu, Peru is "deserted settlement" (current)</skos:example>
    <rdfs:isDefinedBy rdf:resource="http://vocab.getty.edu/ontology"/>
    <skos:prefLabel>placeTypePreferred</skos:prefLabel>
    <rdfs:subPropertyOf rdf:resource="http://vocab.getty.edu/ontology#placeType"/>
    <rdfs:comment>The primary type of a TGN Place. Domain is TGN concept, range is AAT concept</rdfs:comment>
    <rdf:type rdf:resource="http://www.w3.org/2002/07/owl#ObjectProperty"/>
    <dct:description>The primary type of a TGN Place. Domain is TGN concept, range is AAT concept.
Example: The preferred place type of Machupicchu, Peru is "deserted settlement" (current)</dct:description>
    <rdfs:label>placeTypePreferred</rdfs:label>
  </rdf:Description>
  <rdf:Description rdf:about="http://vocab.getty.edu/ontology#GuideTerm">
    <rdfs:isDefinedBy rdf:resource="http://vocab.getty.edu/ontology"/>
    <skos:example>&lt;vessels for serving and consuming food&gt; (AAT), ulan:500353455 &lt;named animals&gt; under facet Non-Artists (ULAN)</skos:example>
    <skos:prefLabel>GuideTerm</skos:prefLabel>
    <rdfs:comment>Guide Term: place holder to create a level in the hierarchy. Used in AAT and ULAN. Not used for indexing or cataloguing.</rdfs:comment>
    <rdfs:label>GuideTerm</rdfs:label>
    <rdfs:subClassOf rdf:resource="http://vocab.getty.edu/ontology#Subject"/>
    <rdfs:subClassOf rdf:resource="http://purl.org/iso25964/skos-thes#ThesaurusArray"/>
    <rdf:type rdf:resource="http://www.w3.org/2002/07/owl#Class"/>
    <dct:description>Guide Term: place holder to create a level in the hierarchy. Used in AAT and ULAN. Not used for indexing or cataloguing..
Example: &lt;vessels for serving and consuming food&gt; (AAT), ulan:500353455 &lt;named animals&gt; under facet Non-Artists (ULAN)</dct:description>
  </rdf:Description>
  <rdf:Description rdf:about="http://vocab.getty.edu/ontology#tgn3005_possibly_identified_as">
    <dct:description>place - possibly identified as - place.&#13;
Example: The lost settlement of Sharuhen is possibly identified as Tel el-Far'ah (As Suwayda', Syria) (deserted settlement)</dct:description>
    <rdfs:subPropertyOf rdf:resource="http://www.w3.org/2004/02/skos/core#related"/>
    <skos:example>The lost settlement of Sharuhen is possibly identified as Tel el-Far'ah (As Suwayda', Syria) (deserted settlement)</skos:example>
    <rdfs:domain rdf:resource="http://www.w3.org/2004/02/skos/core#Concept"/>
    <rdf:type rdf:resource="http://www.w3.org/2002/07/owl#SymmetricProperty"/>
    <rdfs:isDefinedBy rdf:resource="http://vocab.getty.edu/ontology"/>
    <rdfs:range rdf:resource="http://www.w3.org/2004/02/skos/core#Concept"/>
    <skos:prefLabel>tgn3005_possibly_identified_as</skos:prefLabel>
    <dc:identifier>3005</dc:identifier>
    <dc:title>possibly identified as - place</dc:title>
    <rdf:type rdf:resource="http://www.w3.org/2002/07/owl#ObjectProperty"/>
    <rdfs:isDefinedBy rdf:resource="http://vocab.getty.edu/tgn/"/>
  </rdf:Description>
  <rdf:Description rdf:about="http://vocab.getty.edu/ontology#ulan1302_associate_of">
    <rdfs:domain rdf:resource="http://www.w3.org/2004/02/skos/core#Concept"/>
    <skos:example>Frank Lloyd Wright was an associate of Giannini and Hilgart</skos:example>
    <dc:identifier>1302</dc:identifier>
    <rdf:type rdf:resource="http://www.w3.org/2002/07/owl#ObjectProperty"/>
    <skos:prefLabel>ulan1302_associate_of</skos:prefLabel>
    <rdfs:subPropertyOf rdf:resource="http://www.w3.org/2004/02/skos/core#related"/>
    <dc:title>associate of - person</dc:title>
    <rdfs:isDefinedBy rdf:resource="http://vocab.getty.edu/ulan/"/>
    <rdfs:range rdf:resource="http://www.w3.org/2004/02/skos/core#Concept"/>
    <rdfs:isDefinedBy rdf:resource="http://vocab.getty.edu/ontology"/>
    <rdf:type rdf:resource="http://www.w3.org/2002/07/owl#SymmetricProperty"/>
    <dct:description>person - associate of - person.&#13;
Example: Frank Lloyd Wright was an associate of Giannini and Hilgart</dct:description>
  </rdf:Description>
  <rdf:Description rdf:about="http://vocab.getty.edu/ontology#nationalityPreferred">
    <skos:prefLabel>nationalityPreferred</skos:prefLabel>
    <rdf:type rdf:resource="http://www.w3.org/2002/07/owl#ObjectProperty"/>
    <rdfs:label>nationalityPreferred</rdfs:label>
    <rdfs:comment>Preferred nationality/culture/race/ethnicity/religion/sexual orientation of an ULAN agent. Domain is schema:Person/Organization, range is AAT concept</rdfs:comment>
    <dct:description>Preferred nationality/culture/race/ethnicity/religion/sexual orientation of an ULAN agent. Domain is schema:Person/Organization, range is AAT concept</dct:description>
    <rdfs:isDefinedBy rdf:resource="http://vocab.getty.edu/ontology"/>
    <rdfs:subPropertyOf rdf:resource="http://schema.org/nationality"/>
    <rdfs:range rdf:resource="http://vocab.getty.edu/ontology#Subject"/>
  </rdf:Description>
  <rdf:Description rdf:about="http://vocab.getty.edu/ontology#aat2431_required_for">
    <skos:prefLabel>aat2431_required_for</skos:prefLabel>
    <dc:identifier>2431</dc:identifier>
    <rdf:type rdf:resource="http://www.w3.org/2002/07/owl#ObjectProperty"/>
    <dc:title>required for - activity/event/process</dc:title>
    <dct:description>things/equipment - [are] required for - activity/event/process.&#13;
Example: painting equipment is required for painting (image making); dowels are required for doweling</dct:description>
    <rdfs:isDefinedBy rdf:resource="http://vocab.getty.edu/aat/"/>
    <owl:inverseOf rdf:resource="http://vocab.getty.edu/ontology#aat2432_requires"/>
    <skos:example>dowels are required for doweling</skos:example>
    <skos:example>painting equipment is required for painting (image making)</skos:example>
    <rdfs:isDefinedBy rdf:resource="http://vocab.getty.edu/ontology"/>
    <rdfs:subPropertyOf rdf:resource="http://www.w3.org/2004/02/skos/core#related"/>
    <rdfs:domain rdf:resource="http://www.w3.org/2004/02/skos/core#Concept"/>
    <rdfs:range rdf:resource="http://www.w3.org/2004/02/skos/core#Concept"/>
  </rdf:Description>
  <rdf:Description rdf:about="http://vocab.getty.edu/ontology#ulan2574_director_of">
    <owl:inverseOf rdf:resource="http://vocab.getty.edu/ontology#ulan2575_directed_by"/>
    <rdfs:range rdf:resource="http://www.w3.org/2004/02/skos/core#Concept"/>
    <rdf:type rdf:resource="http://www.w3.org/2002/07/owl#ObjectProperty"/>
    <dc:identifier>2574</dc:identifier>
    <skos:example>Jean Jans I directed Gobelins Tapestry Manufactory</skos:example>
    <rdfs:isDefinedBy rdf:resource="http://vocab.getty.edu/ulan/"/>
    <dct:description>person - director of - institution.&#13;
Example: Jean Jans I directed Gobelins Tapestry Manufactory</dct:description>
    <dc:title>director of - institution</dc:title>
    <rdfs:isDefinedBy rdf:resource="http://vocab.getty.edu/ontology"/>
    <rdfs:domain rdf:resource="http://www.w3.org/2004/02/skos/core#Concept"/>
    <rdfs:subPropertyOf rdf:resource="http://www.w3.org/2004/02/skos/core#related"/>
    <skos:prefLabel>ulan2574_director_of</skos:prefLabel>
  </rdf:Description>
  <rdf:Description rdf:about="http://vocab.getty.edu/ontology#ulan1541_spouse_of">
    <rdfs:domain rdf:resource="http://www.w3.org/2004/02/skos/core#Concept"/>
    <skos:example>Alfred Stieglitz and Georgia O'Keeffe were married to each other</skos:example>
    <dc:title>spouse of - person</dc:title>
    <rdf:type rdf:resource="http://www.w3.org/2002/07/owl#ObjectProperty"/>
    <dct:description>person - spouse of - person.&#13;
Example: Alfred Stieglitz and Georgia O'Keeffe were married to each other</dct:description>
    <rdfs:subPropertyOf rdf:resource="http://www.w3.org/2004/02/skos/core#related"/>
    <rdfs:isDefinedBy rdf:resource="http://vocab.getty.edu/ulan/"/>
    <rdfs:range rdf:resource="http://www.w3.org/2004/02/skos/core#Concept"/>
    <dc:identifier>1541</dc:identifier>
    <rdfs:isDefinedBy rdf:resource="http://vocab.getty.edu/ontology"/>
    <skos:prefLabel>ulan1541_spouse_of</skos:prefLabel>
    <rdf:type rdf:resource="http://www.w3.org/2002/07/owl#SymmetricProperty"/>
  </rdf:Description>
  <rdf:Description rdf:about="http://vocab.getty.edu/ontology#ulan2674_professor_at">
    <rdf:type rdf:resource="http://www.w3.org/2002/07/owl#ObjectProperty"/>
    <owl:inverseOf rdf:resource="http://vocab.getty.edu/ontology#ulan2675_professor_was"/>
    <dc:title>professor at - institution</dc:title>
    <dct:description>person - professor at - institution.&#13;
Example: Paul Klee was a professor at Bauhaus</dct:description>
    <rdfs:range rdf:resource="http://www.w3.org/2004/02/skos/core#Concept"/>
    <dc:identifier>2674</dc:identifier>
    <rdfs:domain rdf:resource="http://www.w3.org/2004/02/skos/core#Concept"/>
    <rdfs:isDefinedBy rdf:resource="http://vocab.getty.edu/ontology"/>
    <skos:example>Paul Klee was a professor at Bauhaus</skos:example>
    <skos:prefLabel>ulan2674_professor_at</skos:prefLabel>
    <rdfs:isDefinedBy rdf:resource="http://vocab.getty.edu/ulan/"/>
    <rdfs:subPropertyOf rdf:resource="http://www.w3.org/2004/02/skos/core#related"/>
  </rdf:Description>
  <rdf:Description rdf:about="http://vocab.getty.edu/ontology#ulan1554_adoptive_parent_of">
    <rdf:type rdf:resource="http://www.w3.org/2002/07/owl#ObjectProperty"/>
    <skos:prefLabel>ulan1554_adoptive_parent_of</skos:prefLabel>
    <dc:title>adoptive parent of - person</dc:title>
    <rdfs:range rdf:resource="http://www.w3.org/2004/02/skos/core#Concept"/>
    <owl:inverseOf rdf:resource="http://vocab.getty.edu/ontology#ulan1555_adopted_child_of"/>
    <skos:example>Julius Caesar is the adoptive parent of Augustus, Emperor of Rome</skos:example>
    <rdfs:subPropertyOf rdf:resource="http://www.w3.org/2004/02/skos/core#related"/>
    <dc:identifier>1554</dc:identifier>
    <rdfs:isDefinedBy rdf:resource="http://vocab.getty.edu/ulan/"/>
    <dct:description>person - adoptive parent of - person.&#13;
Example: Julius Caesar is the adoptive parent of Augustus, Emperor of Rome</dct:description>
    <rdfs:isDefinedBy rdf:resource="http://vocab.getty.edu/ontology"/>
    <rdfs:domain rdf:resource="http://www.w3.org/2004/02/skos/core#Concept"/>
  </rdf:Description>
  <rdf:Description rdf:about="http://vocab.getty.edu/ontology#aat2824_has_parallels_with">
    <rdf:type rdf:resource="http://www.w3.org/2002/07/owl#SymmetricProperty"/>
    <dct:description>style/period/culture/[religion/ideology] - has parallels with - style/period/culture/[religion/ideology].&#13;
Example: Lagozza [culture] has parallels with Chasseen [culture];  Gnathian (pottery style) has parallels with West Slope (pottery style)</dct:description>
    <rdfs:isDefinedBy rdf:resource="http://vocab.getty.edu/ontology"/>
    <skos:example>Lagozza [culture] has parallels with Chasseen [culture]</skos:example>
    <skos:prefLabel>aat2824_has_parallels_with</skos:prefLabel>
    <dc:title>has parallels with - style/period/culture</dc:title>
    <rdfs:subPropertyOf rdf:resource="http://www.w3.org/2004/02/skos/core#related"/>
    <dc:identifier>2824</dc:identifier>
    <skos:example>Gnathian (pottery style) has parallels with West Slope (pottery style)</skos:example>
    <rdf:type rdf:resource="http://www.w3.org/2002/07/owl#ObjectProperty"/>
    <rdfs:isDefinedBy rdf:resource="http://vocab.getty.edu/aat/"/>
    <rdfs:range rdf:resource="http://www.w3.org/2004/02/skos/core#Concept"/>
    <rdfs:domain rdf:resource="http://www.w3.org/2004/02/skos/core#Concept"/>
  </rdf:Description>
  <rdf:Description rdf:about="http://vocab.getty.edu/ontology#aat2558_reflected_in">
    <skos:example>Ancient Greek [culture] is reflected in classics (discipline)</skos:example>
    <dc:title>reflected in - field/discipline</dc:title>
    <rdfs:isDefinedBy rdf:resource="http://vocab.getty.edu/ontology"/>
    <dc:identifier>2558</dc:identifier>
    <skos:example>Buddhism is reflected in bugatu [dance discipline]</skos:example>
    <rdfs:subPropertyOf rdf:resource="http://www.w3.org/2004/02/skos/core#related"/>
    <skos:prefLabel>aat2558_reflected_in</skos:prefLabel>
    <rdf:type rdf:resource="http://www.w3.org/2002/07/owl#ObjectProperty"/>
    <skos:example>Christianity is reflected in church history</skos:example>
    <dct:description>style/period/culture /[religion/ideology] - [is] reflected in field/discipline.&#13;
Example: Buddhism is reflected in bugatu [dance discipline]; Christianity is reflected in church history; Ancient Greek [culture] is reflected in classics (discipline)</dct:description>
    <rdfs:isDefinedBy rdf:resource="http://vocab.getty.edu/aat/"/>
    <rdfs:range rdf:resource="http://www.w3.org/2004/02/skos/core#Concept"/>
    <rdfs:domain rdf:resource="http://www.w3.org/2004/02/skos/core#Concept"/>
  </rdf:Description>
  <rdf:Description rdf:about="http://vocab.getty.edu/ontology#ulan1303_collaborated_with">
    <rdfs:domain rdf:resource="http://www.w3.org/2004/02/skos/core#Concept"/>
    <dc:identifier>1303</dc:identifier>
    <rdfs:isDefinedBy rdf:resource="http://vocab.getty.edu/ulan/"/>
    <dc:title>collaborated with - person</dc:title>
    <skos:prefLabel>ulan1303_collaborated_with</skos:prefLabel>
    <rdf:type rdf:resource="http://www.w3.org/2002/07/owl#ObjectProperty"/>
    <rdfs:subPropertyOf rdf:resource="http://www.w3.org/2004/02/skos/core#related"/>
    <skos:example>Pablo Picasso collaborated with Georges Braque</skos:example>
    <rdfs:range rdf:resource="http://www.w3.org/2004/02/skos/core#Concept"/>
    <dct:description>person - collaborated with - person.&#13;
Example: Pablo Picasso collaborated with Georges Braque</dct:description>
    <rdf:type rdf:resource="http://www.w3.org/2002/07/owl#SymmetricProperty"/>
    <rdfs:isDefinedBy rdf:resource="http://vocab.getty.edu/ontology"/>
  </rdf:Description>
  <rdf:Description rdf:about="http://vocab.getty.edu/ontology#aat2425_produces">
    <dc:identifier>2425</dc:identifier>
    <rdf:type rdf:resource="http://www.w3.org/2002/07/owl#ObjectProperty"/>
    <skos:example>wiredrawing produces wire</skos:example>
    <dc:title>produces - material</dc:title>
    <rdfs:subPropertyOf rdf:resource="http://www.w3.org/2004/02/skos/core#related"/>
    <rdfs:domain rdf:resource="http://www.w3.org/2004/02/skos/core#Concept"/>
    <rdfs:isDefinedBy rdf:resource="http://vocab.getty.edu/ontology"/>
    <rdfs:isDefinedBy rdf:resource="http://vocab.getty.edu/aat/"/>
    <skos:prefLabel>aat2425_produces</skos:prefLabel>
    <rdfs:range rdf:resource="http://www.w3.org/2004/02/skos/core#Concept"/>
    <skos:example>papermaking produces paper</skos:example>
    <dct:description>activity/event/process - produces - material.&#13;
Example: wiredrawing produces wire; papermaking produces paper</dct:description>
  </rdf:Description>
  <rdf:Description rdf:about="http://vocab.getty.edu/ontology#ulan2692_president_of">
    <rdfs:range rdf:resource="http://www.w3.org/2004/02/skos/core#Concept"/>
    <skos:example>David K. E. Bruce was president of National Gallery of Art</skos:example>
    <rdfs:isDefinedBy rdf:resource="http://vocab.getty.edu/ontology"/>
    <rdfs:domain rdf:resource="http://www.w3.org/2004/02/skos/core#Concept"/>
    <rdfs:subPropertyOf rdf:resource="http://www.w3.org/2004/02/skos/core#related"/>
    <dct:description>person - president of - institution.&#13;
Example: David K. E. Bruce was president of National Gallery of Art</dct:description>
    <rdfs:isDefinedBy rdf:resource="http://vocab.getty.edu/ulan/"/>
    <rdf:type rdf:resource="http://www.w3.org/2002/07/owl#ObjectProperty"/>
    <owl:inverseOf rdf:resource="http://vocab.getty.edu/ontology#ulan2693_president_was"/>
    <dc:title>president of - institution</dc:title>
    <skos:prefLabel>ulan2692_president_of</skos:prefLabel>
    <dc:identifier>2692</dc:identifier>
  </rdf:Description>
  <rdf:Description rdf:about="http://vocab.getty.edu/ontology#ulan1501_sibling_of">
    <rdfs:range rdf:resource="http://www.w3.org/2004/02/skos/core#Concept"/>
    <skos:prefLabel>ulan1501_sibling_of</skos:prefLabel>
    <skos:example>Philippe Rubens is the sibling of Peter Paul Rubens</skos:example>
    <rdf:type rdf:resource="http://www.w3.org/2002/07/owl#ObjectProperty"/>
    <dc:title>sibling of - person</dc:title>
    <rdfs:isDefinedBy rdf:resource="http://vocab.getty.edu/ulan/"/>
    <rdfs:subPropertyOf rdf:resource="http://www.w3.org/2004/02/skos/core#related"/>
    <rdfs:domain rdf:resource="http://www.w3.org/2004/02/skos/core#Concept"/>
    <rdf:type rdf:resource="http://www.w3.org/2002/07/owl#SymmetricProperty"/>
    <dc:identifier>1501</dc:identifier>
    <rdfs:isDefinedBy rdf:resource="http://vocab.getty.edu/ontology"/>
    <dct:description>person - sibling of - person.&#13;
Example: Philippe Rubens is the sibling of Peter Paul Rubens</dct:description>
  </rdf:Description>
  <rdf:Description rdf:about="http://vocab.getty.edu/ontology#ulan1413_administration_overlaps_with">
    <dc:identifier>1413</dc:identifier>
    <rdfs:range rdf:resource="http://www.w3.org/2004/02/skos/core#Concept"/>
    <skos:example>The administration of the Numismatic Collection overlaps with Bode Museum</skos:example>
    <dct:description>firm/group - administration overlaps with - firm/group.&#13;
Example: The administration of the Numismatic Collection overlaps with Bode Museum</dct:description>
    <rdfs:subPropertyOf rdf:resource="http://www.w3.org/2004/02/skos/core#related"/>
    <rdf:type rdf:resource="http://www.w3.org/2002/07/owl#ObjectProperty"/>
    <skos:prefLabel>ulan1413_administration_overlaps_with</skos:prefLabel>
    <rdfs:isDefinedBy rdf:resource="http://vocab.getty.edu/ulan/"/>
    <rdfs:domain rdf:resource="http://www.w3.org/2004/02/skos/core#Concept"/>
    <dc:title>administration overlaps with - firm/group</dc:title>
    <rdf:type rdf:resource="http://www.w3.org/2002/07/owl#SymmetricProperty"/>
    <rdfs:isDefinedBy rdf:resource="http://vocab.getty.edu/ontology"/>
  </rdf:Description>
  <rdf:Description rdf:about="http://vocab.getty.edu/ontology#ulan2577_patron_was">
    <rdfs:subPropertyOf rdf:resource="http://www.w3.org/2004/02/skos/core#related"/>
    <dc:title>patron was - person</dc:title>
    <rdf:type rdf:resource="http://www.w3.org/2002/07/owl#ObjectProperty"/>
    <rdfs:range rdf:resource="http://www.w3.org/2004/02/skos/core#Concept"/>
    <skos:prefLabel>ulan2577_patron_was</skos:prefLabel>
    <dct:description>person - patron was - person.&#13;
Example: James Caulfiel, Earl of Charlemont was the patron of William Chambers</dct:description>
    <rdfs:isDefinedBy rdf:resource="http://vocab.getty.edu/ontology"/>
    <dc:identifier>2577</dc:identifier>
    <rdfs:domain rdf:resource="http://www.w3.org/2004/02/skos/core#Concept"/>
    <skos:example>James Caulfiel, Earl of Charlemont was the patron of William Chambers</skos:example>
    <rdfs:isDefinedBy rdf:resource="http://vocab.getty.edu/ulan/"/>
  </rdf:Description>
  <rdf:Description rdf:about="http://vocab.getty.edu/ontology#aat2321_used_by">
    <rdfs:domain rdf:resource="http://www.w3.org/2004/02/skos/core#Concept"/>
    <rdfs:isDefinedBy rdf:resource="http://vocab.getty.edu/ontology"/>
    <skos:example>violoncellos are used by violoncellists</skos:example>
    <rdfs:isDefinedBy rdf:resource="http://vocab.getty.edu/aat/"/>
    <rdfs:range rdf:resource="http://www.w3.org/2004/02/skos/core#Concept"/>
    <skos:example>surveying instruments are used by surveyors</skos:example>
    <dc:identifier>2321</dc:identifier>
    <owl:inverseOf rdf:resource="http://vocab.getty.edu/ontology#aat2322_use"/>
    <dc:title>used by - role</dc:title>
    <rdf:type rdf:resource="http://www.w3.org/2002/07/owl#ObjectProperty"/>
    <dct:description>things/equipment - [are] used by - [actors having] role.&#13;
Example: violoncellos are used by violoncellists; surveying instruments are used by surveyors</dct:description>
    <rdfs:subPropertyOf rdf:resource="http://www.w3.org/2004/02/skos/core#related"/>
    <skos:prefLabel>aat2321_used_by</skos:prefLabel>
  </rdf:Description>
  <rdf:Description rdf:about="http://vocab.getty.edu/ontology#ulan2675_professor_was">
    <rdf:type rdf:resource="http://www.w3.org/2002/07/owl#ObjectProperty"/>
    <dct:description>institution - professor was - person.&#13;
Example: A professor at Bauhaus was Paul Klee</dct:description>
    <rdfs:range rdf:resource="http://www.w3.org/2004/02/skos/core#Concept"/>
    <rdfs:domain rdf:resource="http://www.w3.org/2004/02/skos/core#Concept"/>
    <rdfs:isDefinedBy rdf:resource="http://vocab.getty.edu/ontology"/>
    <dc:identifier>2675</dc:identifier>
    <dc:title>professor was - person</dc:title>
    <skos:example>A professor at Bauhaus was Paul Klee</skos:example>
    <rdfs:isDefinedBy rdf:resource="http://vocab.getty.edu/ulan/"/>
    <skos:prefLabel>ulan2675_professor_was</skos:prefLabel>
    <rdfs:subPropertyOf rdf:resource="http://www.w3.org/2004/02/skos/core#related"/>
  </rdf:Description>
  <rdf:Description rdf:about="http://vocab.getty.edu/ontology#aat2879_followed-developed_from">
    <skos:example>Egyptian, Coptic (language) followed/developed from Ancient Egyptian (language)</skos:example>
    <skos:example>Greek (modern language) followed/developed from Ancient Greek (language)</skos:example>
    <rdf:type rdf:resource="http://www.w3.org/2002/07/owl#ObjectProperty"/>
    <rdfs:range rdf:resource="http://www.w3.org/2004/02/skos/core#Concept"/>
    <dc:identifier>2879</dc:identifier>
    <rdfs:isDefinedBy rdf:resource="http://vocab.getty.edu/aat/"/>
    <skos:prefLabel>aat2879_followed-developed_from</skos:prefLabel>
    <dct:description>language - followed/developed from - language.&#13;
Example: Greek (modern language) followed/developed from Ancient Greek (language); Egyptian, Coptic (language) followed/developed from Ancient Egyptian (language)</dct:description>
    <rdfs:subPropertyOf rdf:resource="http://www.w3.org/2004/02/skos/core#related"/>
    <dc:title>followed/developed from - language</dc:title>
    <rdfs:isDefinedBy rdf:resource="http://vocab.getty.edu/ontology"/>
    <rdfs:domain rdf:resource="http://www.w3.org/2004/02/skos/core#Concept"/>
  </rdf:Description>
  <rdf:Description rdf:about="http://vocab.getty.edu/ontology#ulan1221_appointed_by">
    <rdfs:subPropertyOf rdf:resource="http://www.w3.org/2004/02/skos/core#related"/>
    <rdfs:isDefinedBy rdf:resource="http://vocab.getty.edu/ulan/"/>
    <skos:example>Pope Urban VIII appointed Virginio Cesarini</skos:example>
    <dc:identifier>1221</dc:identifier>
    <rdfs:range rdf:resource="http://www.w3.org/2004/02/skos/core#Concept"/>
    <rdfs:isDefinedBy rdf:resource="http://vocab.getty.edu/ontology"/>
    <owl:inverseOf rdf:resource="http://vocab.getty.edu/ontology#ulan1222_appointee_of"/>
    <rdfs:domain rdf:resource="http://www.w3.org/2004/02/skos/core#Concept"/>
    <dct:description>person - appointed by - person.&#13;
Example: Pope Urban VIII appointed Virginio Cesarini</dct:description>
    <dc:title>appointed by - person</dc:title>
    <skos:prefLabel>ulan1221_appointed_by</skos:prefLabel>
    <rdf:type rdf:resource="http://www.w3.org/2002/07/owl#ObjectProperty"/>
  </rdf:Description>
  <rdf:Description rdf:about="http://vocab.getty.edu/term/flag/LiteralTranslation">
    <skos:prefLabel>Literal Translation</skos:prefLabel>
    <skos:scopeNote>Literal translation of a name.  Defined for ULAN, but currently there are no examples of this</skos:scopeNote>
    <dct:description>Literal translation of a name.  Defined for ULAN, but currently there are no examples of this</dct:description>
    <skos:notation>T</skos:notation>
    <skos:inScheme rdf:resource="http://vocab.getty.edu/term/flag/"/>
    <rdf:type rdf:resource="http://www.w3.org/2004/02/skos/core#Concept"/>
  </rdf:Description>
  <rdf:Description rdf:about="http://vocab.getty.edu/ontology#ulan2650_publisher_was">
    <dc:title>publisher was - firm</dc:title>
    <rdf:type rdf:resource="http://www.w3.org/2002/07/owl#ObjectProperty"/>
    <dct:description>person - publisher was - firm.&#13;
Example: The publisher for Pierre Joseph Rossier was Negretti and Zambra</dct:description>
    <rdfs:isDefinedBy rdf:resource="http://vocab.getty.edu/ontology"/>
    <skos:example>The publisher for Pierre Joseph Rossier was Negretti and Zambra</skos:example>
    <owl:inverseOf rdf:resource="http://vocab.getty.edu/ontology#ulan2651_publisher_of"/>
    <rdfs:domain rdf:resource="http://www.w3.org/2004/02/skos/core#Concept"/>
    <rdfs:subPropertyOf rdf:resource="http://www.w3.org/2004/02/skos/core#related"/>
    <rdfs:isDefinedBy rdf:resource="http://vocab.getty.edu/ulan/"/>
    <skos:prefLabel>ulan2650_publisher_was</skos:prefLabel>
    <dc:identifier>2650</dc:identifier>
    <rdfs:range rdf:resource="http://www.w3.org/2004/02/skos/core#Concept"/>
  </rdf:Description>
  <rdf:Description rdf:about="http://vocab.getty.edu/ontology#aat2336_has_associates">
    <skos:example>Abstract (fine arts style) has associates abstract artists</skos:example>
    <dct:description>style/period/culture/[relgion] - has associates - [actors having] role.&#13;
Example: Abstract (fine arts style) has associates abstract artists; Roman Catholicism has associates popes</dct:description>
    <rdfs:isDefinedBy rdf:resource="http://vocab.getty.edu/ontology"/>
    <rdfs:subPropertyOf rdf:resource="http://www.w3.org/2004/02/skos/core#related"/>
    <rdf:type rdf:resource="http://www.w3.org/2002/07/owl#ObjectProperty"/>
    <skos:example>Roman Catholicism has associates popes</skos:example>
    <dc:title>has associates - role</dc:title>
    <skos:prefLabel>aat2336_has_associates</skos:prefLabel>
    <dc:identifier>2336</dc:identifier>
    <rdfs:isDefinedBy rdf:resource="http://vocab.getty.edu/aat/"/>
    <rdfs:range rdf:resource="http://www.w3.org/2004/02/skos/core#Concept"/>
    <rdfs:domain rdf:resource="http://www.w3.org/2004/02/skos/core#Concept"/>
  </rdf:Description>
  <rdf:Description rdf:about="http://vocab.getty.edu/ontology#termType">
    <rdfs:label>termType</rdfs:label>
    <rdfs:range rdf:resource="http://www.w3.org/2004/02/skos/core#Concept"/>
    <rdfs:isDefinedBy rdf:resource="http://vocab.getty.edu/ontology"/>
    <rdf:type rdf:resource="http://www.w3.org/2002/07/owl#ObjectProperty"/>
    <rdfs:domain rdf:resource="http://www.w3.org/2008/05/skos-xl#Label"/>
    <skos:prefLabel>termType</skos:prefLabel>
    <dct:description>Term Type</dct:description>
  </rdf:Description>
  <rdf:Description rdf:about="http://vocab.getty.edu/ontology#tgn3317_member_of">
    <rdfs:subPropertyOf rdf:resource="http://www.w3.org/2004/02/skos/core#related"/>
    <dct:description>nation - member of - union.&#13;
Example: Austria is a member of the European Union since 1915; Belgium is a member of the European Union since 1958</dct:description>
    <rdfs:domain rdf:resource="http://www.w3.org/2004/02/skos/core#Concept"/>
    <skos:example>Belgium is a member of the European Union since 1958</skos:example>
    <rdfs:isDefinedBy rdf:resource="http://vocab.getty.edu/ontology"/>
    <rdfs:range rdf:resource="http://www.w3.org/2004/02/skos/core#Concept"/>
    <dc:title>member of - union</dc:title>
    <skos:prefLabel>tgn3317_member_of</skos:prefLabel>
    <dc:identifier>3317</dc:identifier>
    <skos:example>Austria is a member of the European Union since 1915</skos:example>
    <rdf:type rdf:resource="http://www.w3.org/2002/07/owl#ObjectProperty"/>
    <rdfs:isDefinedBy rdf:resource="http://vocab.getty.edu/tgn/"/>
    <owl:inverseOf rdf:resource="http://vocab.getty.edu/ontology#tgn3318_member_is"/>
  </rdf:Description>
  <rdf:Description rdf:about="http://vocab.getty.edu/ontology#aat2809_coexisted_with">
    <rdfs:subPropertyOf rdf:resource="http://www.w3.org/2004/02/skos/core#related"/>
    <skos:prefLabel>aat2809_coexisted_with</skos:prefLabel>
    <dct:description>style/period/culture/[religion/ideology] - coexisted with -  style/period/culture/[religion/ideology].&#13;
Example: Sangoan coexisted with Fauresmith; Early Minoan coexisted with Prepalatial</dct:description>
    <rdfs:range rdf:resource="http://www.w3.org/2004/02/skos/core#Concept"/>
    <rdfs:isDefinedBy rdf:resource="http://vocab.getty.edu/ontology"/>
    <rdf:type rdf:resource="http://www.w3.org/2002/07/owl#SymmetricProperty"/>
    <rdfs:domain rdf:resource="http://www.w3.org/2004/02/skos/core#Concept"/>
    <skos:example>Early Minoan coexisted with Prepalatial</skos:example>
    <skos:example>Sangoan coexisted with Fauresmith</skos:example>
    <dc:title>coexisted with - style/period/culture</dc:title>
    <rdf:type rdf:resource="http://www.w3.org/2002/07/owl#ObjectProperty"/>
    <rdfs:isDefinedBy rdf:resource="http://vocab.getty.edu/aat/"/>
    <dc:identifier>2809</dc:identifier>
  </rdf:Description>
  <rdf:Description rdf:about="http://vocab.getty.edu/term/kind/FIPSCode">
    <skos:prefLabel>FIPS Code</skos:prefLabel>
    <skos:example>"MX21" for Puebla, Mexico</skos:example>
    <rdf:type rdf:resource="http://www.w3.org/2004/02/skos/core#Concept"/>
    <skos:notation>FIPS</skos:notation>
    <skos:scopeNote>FIPS region code. Used in TGN</skos:scopeNote>
    <dct:description>FIPS region code. Used in TGN.
Example: "MX21" for Puebla, Mexico</dct:description>
    <skos:inScheme rdf:resource="http://vocab.getty.edu/term/kind/"/>
  </rdf:Description>
  <rdf:Description rdf:about="http://vocab.getty.edu/ontology#ulan2795_representative_was">
    <rdfs:domain rdf:resource="http://www.w3.org/2004/02/skos/core#Concept"/>
    <rdf:type rdf:resource="http://www.w3.org/2002/07/owl#ObjectProperty"/>
    <rdfs:subPropertyOf rdf:resource="http://www.w3.org/2004/02/skos/core#related"/>
    <rdfs:isDefinedBy rdf:resource="http://vocab.getty.edu/ulan/"/>
    <dc:title>representative was - person</dc:title>
    <skos:prefLabel>ulan2795_representative_was</skos:prefLabel>
    <rdfs:range rdf:resource="http://www.w3.org/2004/02/skos/core#Concept"/>
    <rdfs:isDefinedBy rdf:resource="http://vocab.getty.edu/ontology"/>
    <dct:description>institution - representative was - person.&#13;
Example: The Noguch Museum - representative was Isamu Noguchi</dct:description>
    <skos:example>The Noguch Museum - representative was Isamu Noguchi</skos:example>
    <dc:identifier>2795</dc:identifier>
  </rdf:Description>
  <rdf:Description rdf:about="http://vocab.getty.edu/ontology#broaderExtended">
    <skos:prefLabel>broaderExtended</skos:prefLabel>
    <rdf:type rdf:resource="http://www.w3.org/2002/07/owl#ObjectProperty"/>
    <dct:description>Appropriate ancestors. Meaningful closure of gvp:broader for query expansion. Use this, not skos:broaderTransitive.
Example: Mt Athos has ancestor places (BTPE) World, Europe, Greece, Macedonia, Pangaíon Óros regional division;
and place types (BTIE) inhabited place; and orthodox religious center, Christian religious center, religious center</dct:description>
    <rdfs:label>broaderExtended</rdfs:label>
    <rdfs:comment>Appropriate ancestors. Meaningful closure of gvp:broader for query expansion. Use this, not skos:broaderTransitive</rdfs:comment>
    <rdfs:range rdf:resource="http://vocab.getty.edu/ontology#Subject"/>
    <rdfs:domain rdf:resource="http://vocab.getty.edu/ontology#Subject"/>
    <rdfs:isDefinedBy rdf:resource="http://vocab.getty.edu/ontology"/>
    <skos:example>Mt Athos has ancestor places (BTPE) World, Europe, Greece, Macedonia, Pangaíon Óros regional division;
and place types (BTIE) inhabited place; and orthodox religious center, Christian religious center, religious center</skos:example>
  </rdf:Description>
  <rdf:Description rdf:about="http://vocab.getty.edu/ontology#broaderPartitive">
    <rdfs:subPropertyOf rdf:resource="http://vocab.getty.edu/ontology#broaderPartitiveExtended"/>
    <rdfs:range rdf:resource="http://vocab.getty.edu/ontology#Subject"/>
    <rdfs:domain rdf:resource="http://vocab.getty.edu/ontology#Subject"/>
    <rdfs:comment>BTP (Part/Whole, "part of") relation. We also infer iso-thes:broaderPartitive, which goes only between Concepts</rdfs:comment>
    <rdf:type rdf:resource="http://www.w3.org/2002/07/owl#ObjectProperty"/>
    <skos:prefLabel>broaderPartitive</skos:prefLabel>
    <rdfs:subPropertyOf rdf:resource="http://vocab.getty.edu/ontology#broader"/>
    <rdfs:label>broaderPartitive</rdfs:label>
    <skos:example>Tuscany (TGN) BTP Italy (TGN)</skos:example>
    <rdfs:isDefinedBy rdf:resource="http://vocab.getty.edu/ontology"/>
    <dct:description>BTP (Part/Whole, "part of") relation. We also infer iso-thes:broaderPartitive, which goes only between Concepts.
Example: Tuscany (TGN) BTP Italy (TGN)</dct:description>
  </rdf:Description>
  <rdf:Description rdf:about="http://vocab.getty.edu/term/kind/">
    <skos:prefLabel>Term Kind concept scheme</skos:prefLabel>
    <dct:description>Term Kind concept scheme</dct:description>
    <rdfs:isDefinedBy rdf:resource="http://vocab.getty.edu/ontology"/>
    <rdf:type rdf:resource="http://www.w3.org/2004/02/skos/core#ConceptScheme"/>
    <rdfs:label>Term Kind concept scheme</rdfs:label>
  </rdf:Description>
  <rdf:Description rdf:about="http://vocab.getty.edu/ontology#ulan1544_significant_other_of">
    <rdf:type rdf:resource="http://www.w3.org/2002/07/owl#ObjectProperty"/>
    <dc:title>significant other of - person</dc:title>
    <rdfs:range rdf:resource="http://www.w3.org/2004/02/skos/core#Concept"/>
    <skos:prefLabel>ulan1544_significant_other_of</skos:prefLabel>
    <rdfs:domain rdf:resource="http://www.w3.org/2004/02/skos/core#Concept"/>
    <rdfs:isDefinedBy rdf:resource="http://vocab.getty.edu/ontology"/>
    <skos:example>Jeanne Hebuterne was the significant other of Amedeo Modigliani</skos:example>
    <rdf:type rdf:resource="http://www.w3.org/2002/07/owl#SymmetricProperty"/>
    <rdfs:isDefinedBy rdf:resource="http://vocab.getty.edu/ulan/"/>
    <dct:description>person - significant other of - person.&#13;
Example: Jeanne Hebuterne was the significant other of Amedeo Modigliani</dct:description>
    <dc:identifier>1544</dc:identifier>
    <rdfs:subPropertyOf rdf:resource="http://www.w3.org/2004/02/skos/core#related"/>
  </rdf:Description>
  <rdf:Description rdf:about="http://vocab.getty.edu/ontology#ulan1213_court_artist_to">
    <dct:description>person - court artist to - person.&#13;
Example: Court artist to Gonzaga Vincenzo I, Duke of Mantua was Peter Paul Rubens; court artist to Charles IV, King of Spain was Francisco de Goya</dct:description>
    <skos:example>court artist to Charles IV, King of Spain was Francisco de Goya</skos:example>
    <rdf:type rdf:resource="http://www.w3.org/2002/07/owl#ObjectProperty"/>
    <owl:inverseOf rdf:resource="http://vocab.getty.edu/ontology#ulan1214_court_artist_was"/>
    <dc:title>court artist to - person</dc:title>
    <skos:example>Court artist to Gonzaga Vincenzo I, Duke of Mantua was Peter Paul Rubens</skos:example>
    <skos:prefLabel>ulan1213_court_artist_to</skos:prefLabel>
    <rdfs:isDefinedBy rdf:resource="http://vocab.getty.edu/ontology"/>
    <dc:identifier>1213</dc:identifier>
    <rdfs:domain rdf:resource="http://www.w3.org/2004/02/skos/core#Concept"/>
    <rdfs:subPropertyOf rdf:resource="http://www.w3.org/2004/02/skos/core#related"/>
    <rdfs:isDefinedBy rdf:resource="http://vocab.getty.edu/ulan/"/>
    <rdfs:range rdf:resource="http://www.w3.org/2004/02/skos/core#Concept"/>
  </rdf:Description>
  <rdf:Description rdf:about="http://vocab.getty.edu/ontology#aat2203_associated_with">
    <rdf:type rdf:resource="http://www.w3.org/2002/07/owl#SymmetricProperty"/>
    <dct:description>activity/event/[process/function] - [is] associated with - activity/event/[process/function].&#13;
Example: Easter is associated with Lent; cavalry exercises are associated with dressage</dct:description>
    <rdfs:isDefinedBy rdf:resource="http://vocab.getty.edu/ontology"/>
    <rdfs:subPropertyOf rdf:resource="http://www.w3.org/2004/02/skos/core#related"/>
    <rdfs:domain rdf:resource="http://www.w3.org/2004/02/skos/core#Concept"/>
    <rdfs:range rdf:resource="http://www.w3.org/2004/02/skos/core#Concept"/>
    <skos:prefLabel>aat2203_associated_with</skos:prefLabel>
    <skos:example>cavalry exercises are associated with dressage</skos:example>
    <rdf:type rdf:resource="http://www.w3.org/2002/07/owl#ObjectProperty"/>
    <dc:title>associated with - activity/event</dc:title>
    <dc:identifier>2203</dc:identifier>
    <skos:example>Easter is associated with Lent</skos:example>
    <rdfs:isDefinedBy rdf:resource="http://vocab.getty.edu/aat/"/>
  </rdf:Description>
  <rdf:Description rdf:about="http://vocab.getty.edu/ontology#ulan1590_possibly_related_to">
    <skos:prefLabel>ulan1590_possibly_related_to</skos:prefLabel>
    <dc:identifier>1590</dc:identifier>
    <rdfs:isDefinedBy rdf:resource="http://vocab.getty.edu/ulan/"/>
    <skos:example>A familial relationship between Ramon Destorrents, the younger and Ramon Destorrents, the elder is possible</skos:example>
    <rdfs:domain rdf:resource="http://www.w3.org/2004/02/skos/core#Concept"/>
    <dc:title>possibly related to - person</dc:title>
    <rdfs:range rdf:resource="http://www.w3.org/2004/02/skos/core#Concept"/>
    <rdfs:isDefinedBy rdf:resource="http://vocab.getty.edu/ontology"/>
    <rdf:type rdf:resource="http://www.w3.org/2002/07/owl#SymmetricProperty"/>
    <dct:description>person - possibly related to (familial relationship) - person.&#13;
Example: A familial relationship between Ramon Destorrents, the younger and Ramon Destorrents, the elder is possible</dct:description>
    <rdf:type rdf:resource="http://www.w3.org/2002/07/owl#ObjectProperty"/>
    <rdfs:subPropertyOf rdf:resource="http://www.w3.org/2004/02/skos/core#related"/>
  </rdf:Description>
  <rdf:Description rdf:about="http://vocab.getty.edu/ontology#ulan2794_representative_of">
    <rdfs:isDefinedBy rdf:resource="http://vocab.getty.edu/ulan/"/>
    <dc:identifier>2794</dc:identifier>
    <rdfs:subPropertyOf rdf:resource="http://www.w3.org/2004/02/skos/core#related"/>
    <rdfs:domain rdf:resource="http://www.w3.org/2004/02/skos/core#Concept"/>
    <skos:example>The Noguch Museum - representative was Isamu Noguchi</skos:example>
    <dc:title>representative of - institution</dc:title>
    <rdfs:isDefinedBy rdf:resource="http://vocab.getty.edu/ontology"/>
    <rdfs:range rdf:resource="http://www.w3.org/2004/02/skos/core#Concept"/>
    <skos:prefLabel>ulan2794_representative_of</skos:prefLabel>
    <dct:description>person - representative of - institution.&#13;
Example: The Noguch Museum - representative was Isamu Noguchi</dct:description>
    <owl:inverseOf rdf:resource="http://vocab.getty.edu/ontology#ulan2795_representative_was"/>
    <rdf:type rdf:resource="http://www.w3.org/2002/07/owl#ObjectProperty"/>
  </rdf:Description>
  <rdf:Description rdf:about="http://vocab.getty.edu/ontology#ulan2581_administrator_of">
    <rdf:type rdf:resource="http://www.w3.org/2002/07/owl#ObjectProperty"/>
    <owl:inverseOf rdf:resource="http://vocab.getty.edu/ontology#ulan2582_administered_by"/>
    <rdfs:isDefinedBy rdf:resource="http://vocab.getty.edu/ulan/"/>
    <rdfs:subPropertyOf rdf:resource="http://www.w3.org/2004/02/skos/core#related"/>
    <dct:description>person - administrator of - institution.&#13;
Example: Georges Mathieu was the administrator of Societe nationale des chemins de fer Francais. Agence des gares</dct:description>
    <rdfs:domain rdf:resource="http://www.w3.org/2004/02/skos/core#Concept"/>
    <rdfs:isDefinedBy rdf:resource="http://vocab.getty.edu/ontology"/>
    <skos:prefLabel>ulan2581_administrator_of</skos:prefLabel>
    <dc:title>administrator of - institution</dc:title>
    <rdfs:range rdf:resource="http://www.w3.org/2004/02/skos/core#Concept"/>
    <dc:identifier>2581</dc:identifier>
    <skos:example>Georges Mathieu was the administrator of Societe nationale des chemins de fer Francais. Agence des gares</skos:example>
  </rdf:Description>
  <rdf:Description rdf:about="http://vocab.getty.edu/term/kind/SiteName">
    <skos:notation>S</skos:notation>
    <skos:example>"Flavia Solva", a deserted settlement and archaeological site (TGN)</skos:example>
    <skos:scopeNote>Used in TGN only</skos:scopeNote>
    <rdf:type rdf:resource="http://www.w3.org/2004/02/skos/core#Concept"/>
    <skos:inScheme rdf:resource="http://vocab.getty.edu/term/kind/"/>
    <skos:prefLabel>Site Name</skos:prefLabel>
    <dct:description>Used in TGN only.
Example: "Flavia Solva", a deserted settlement and archaeological site (TGN)</dct:description>
  </rdf:Description>
  <rdf:Description rdf:about="http://vocab.getty.edu/ontology#aat2295_located_in">
    <skos:prefLabel>aat2295_located_in</skos:prefLabel>
    <rdf:type rdf:resource="http://www.w3.org/2002/07/owl#ObjectProperty"/>
    <rdfs:isDefinedBy rdf:resource="http://vocab.getty.edu/aat/"/>
    <skos:example>mountains are located in mountain ranges</skos:example>
    <rdfs:range rdf:resource="http://www.w3.org/2004/02/skos/core#Concept"/>
    <rdfs:domain rdf:resource="http://www.w3.org/2004/02/skos/core#Concept"/>
    <dc:title>located in - locus/setting</dc:title>
    <rdfs:isDefinedBy rdf:resource="http://vocab.getty.edu/ontology"/>
    <skos:example>national capitals are located in nations</skos:example>
    <dc:identifier>2295</dc:identifier>
    <rdfs:subPropertyOf rdf:resource="http://www.w3.org/2004/02/skos/core#related"/>
    <dct:description>locus/setting - [is] located in - locus/setting.&#13;
Example: national capitals are located in nations; mountains are located in mountain ranges</dct:description>
  </rdf:Description>
  <rdf:Description rdf:about="http://vocab.getty.edu/ontology#aat2211_produce">
    <owl:inverseOf rdf:resource="http://vocab.getty.edu/ontology#aat2212_produced_by"/>
    <rdfs:domain rdf:resource="http://www.w3.org/2004/02/skos/core#Concept"/>
    <skos:prefLabel>aat2211_produce</skos:prefLabel>
    <skos:example>punches (marking tools) produce punchwork</skos:example>
    <dc:identifier>2211</dc:identifier>
    <dc:title>produce - things</dc:title>
    <skos:example>stereoscopic cameras produce stereoscopic photographs</skos:example>
    <rdfs:subPropertyOf rdf:resource="http://www.w3.org/2004/02/skos/core#related"/>
    <rdf:type rdf:resource="http://www.w3.org/2002/07/owl#ObjectProperty"/>
    <dct:description>things/[equipment] - produce - things.&#13;
Example: stereoscopic cameras produce stereoscopic photographs; punches (marking tools) produce punchwork</dct:description>
    <rdfs:isDefinedBy rdf:resource="http://vocab.getty.edu/aat/"/>
    <rdfs:range rdf:resource="http://www.w3.org/2004/02/skos/core#Concept"/>
    <rdfs:isDefinedBy rdf:resource="http://vocab.getty.edu/ontology"/>
  </rdf:Description>
  <rdf:Description rdf:about="http://vocab.getty.edu/ontology#aat2557_reflects">
    <skos:example>classics (discipline) reflects Ancient Greek [culture]</skos:example>
    <skos:example>church history reflects Christianity</skos:example>
    <rdfs:domain rdf:resource="http://www.w3.org/2004/02/skos/core#Concept"/>
    <skos:prefLabel>aat2557_reflects</skos:prefLabel>
    <owl:inverseOf rdf:resource="http://vocab.getty.edu/ontology#aat2558_reflected_in"/>
    <skos:example>bugatu [dance discipline] reflects Buddhism</skos:example>
    <rdfs:isDefinedBy rdf:resource="http://vocab.getty.edu/ontology"/>
    <dct:description>field/discipline - reflects - style/period/culture /[religion/ideology].&#13;
Example: bugatu [dance discipline] reflects Buddhism; church history reflects Christianity; classics (discipline) reflects Ancient Greek [culture]</dct:description>
    <dc:title>reflects - style/period/culture</dc:title>
    <rdfs:range rdf:resource="http://www.w3.org/2004/02/skos/core#Concept"/>
    <rdfs:isDefinedBy rdf:resource="http://vocab.getty.edu/aat/"/>
    <dc:identifier>2557</dc:identifier>
    <rdfs:subPropertyOf rdf:resource="http://www.w3.org/2004/02/skos/core#related"/>
    <rdf:type rdf:resource="http://www.w3.org/2002/07/owl#ObjectProperty"/>
  </rdf:Description>
  <rdf:Description rdf:about="http://vocab.getty.edu/ontology#aat2607_caused_by-requires">
    <skos:prefLabel>aat2607_caused_by-requires</skos:prefLabel>
    <rdfs:range rdf:resource="http://www.w3.org/2004/02/skos/core#Concept"/>
    <skos:example>creases (condition) is caused by/requires creasing (process)</skos:example>
    <rdf:type rdf:resource="http://www.w3.org/2002/07/owl#ObjectProperty"/>
    <dc:title>caused by/requires - activity/event</dc:title>
    <skos:example>watertightness is caused by/requires waterproofing</skos:example>
    <owl:inverseOf rdf:resource="http://vocab.getty.edu/ontology#aat2608_causes-required_for"/>
    <dc:identifier>2607</dc:identifier>
    <rdfs:isDefinedBy rdf:resource="http://vocab.getty.edu/aat/"/>
    <dct:description>attributes /associated concepts - [is] caused by/requires - an activity/event/[process/function].&#13;
Example: watertightness is caused by/requires waterproofing; creases (condition) is caused by/requires creasing (process)</dct:description>
    <rdfs:subPropertyOf rdf:resource="http://www.w3.org/2004/02/skos/core#related"/>
    <rdfs:isDefinedBy rdf:resource="http://vocab.getty.edu/ontology"/>
    <rdfs:domain rdf:resource="http://www.w3.org/2004/02/skos/core#Concept"/>
  </rdf:Description>
  <rdf:Description rdf:about="http://vocab.getty.edu/ontology#aat2805_contextualized_in">
    <rdfs:domain rdf:resource="http://www.w3.org/2004/02/skos/core#Concept"/>
    <skos:example>predellas are contextualized in altarpieces</skos:example>
    <dct:description>[smaller] things - [are] contextualized in - [larger] things.&#13;
Example: predellas are contextualized in altarpieces; chapters are contextualized in books</dct:description>
    <skos:prefLabel>aat2805_contextualized_in</skos:prefLabel>
    <rdf:type rdf:resource="http://www.w3.org/2002/07/owl#ObjectProperty"/>
    <rdfs:isDefinedBy rdf:resource="http://vocab.getty.edu/aat/"/>
    <owl:inverseOf rdf:resource="http://vocab.getty.edu/ontology#aat2806_provide_context"/>
    <rdfs:subPropertyOf rdf:resource="http://www.w3.org/2004/02/skos/core#related"/>
    <dc:identifier>2805</dc:identifier>
    <skos:example>chapters are contextualized in books</skos:example>
    <rdfs:range rdf:resource="http://www.w3.org/2004/02/skos/core#Concept"/>
    <rdfs:isDefinedBy rdf:resource="http://vocab.getty.edu/ontology"/>
    <dc:title>contextualized in - things</dc:title>
  </rdf:Description>
  <rdf:Description rdf:about="http://vocab.getty.edu/ontology#ulan2573_founded_by">
    <skos:prefLabel>ulan2573_founded_by</skos:prefLabel>
    <rdfs:isDefinedBy rdf:resource="http://vocab.getty.edu/ulan/"/>
    <dct:description>institution - founded by - person.&#13;
Example: Tiffany Glass &amp; Decorating Company was founded by Louis Comfort Tiffany</dct:description>
    <rdfs:domain rdf:resource="http://www.w3.org/2004/02/skos/core#Concept"/>
    <rdfs:isDefinedBy rdf:resource="http://vocab.getty.edu/ontology"/>
    <skos:example>Tiffany Glass &amp; Decorating Company was founded by Louis Comfort Tiffany</skos:example>
    <rdfs:range rdf:resource="http://www.w3.org/2004/02/skos/core#Concept"/>
    <dc:title>founded by - person</dc:title>
    <dc:identifier>2573</dc:identifier>
    <rdfs:subPropertyOf rdf:resource="http://www.w3.org/2004/02/skos/core#related"/>
    <rdf:type rdf:resource="http://www.w3.org/2002/07/owl#ObjectProperty"/>
  </rdf:Description>
  <rdf:Description rdf:about="http://vocab.getty.edu/ontology#aat2878_preceded-source_for">
    <dc:title>preceded/source for - language</dc:title>
    <rdf:type rdf:resource="http://www.w3.org/2002/07/owl#ObjectProperty"/>
    <skos:prefLabel>aat2878_preceded-source_for</skos:prefLabel>
    <dct:description>language - preceded/[is] source for - language.&#13;
Example: Ancient Greek (language) preceded/is source for Greek (modern language); Ancient Egyptian (language) preceded/is source for Egyptian, Coptic (language)</dct:description>
    <skos:example>Ancient Greek (language) preceded/is source for Greek (modern language)</skos:example>
    <skos:example>Ancient Egyptian (language) preceded/is source for Egyptian, Coptic (language)</skos:example>
    <rdfs:isDefinedBy rdf:resource="http://vocab.getty.edu/aat/"/>
    <rdfs:isDefinedBy rdf:resource="http://vocab.getty.edu/ontology"/>
    <rdfs:subPropertyOf rdf:resource="http://www.w3.org/2004/02/skos/core#related"/>
    <dc:identifier>2878</dc:identifier>
    <rdfs:domain rdf:resource="http://www.w3.org/2004/02/skos/core#Concept"/>
    <rdfs:range rdf:resource="http://www.w3.org/2004/02/skos/core#Concept"/>
    <owl:inverseOf rdf:resource="http://vocab.getty.edu/ontology#aat2879_followed-developed_from"/>
  </rdf:Description>
  <rdf:Description rdf:about="http://vocab.getty.edu/ontology#AdminPlaceConcept">
    <rdfs:subClassOf rdf:resource="http://www.w3.org/2004/02/skos/core#Concept"/>
    <skos:prefLabel>AdminPlaceConcept</skos:prefLabel>
    <skos:example>Burgundy region in France (TGN)</skos:example>
    <rdfs:label>AdminPlaceConcept</rdfs:label>
    <rdfs:isDefinedBy rdf:resource="http://vocab.getty.edu/ontology"/>
    <dct:description>Place defined by administrative boundaries and conditions, including inhabited places, nations, and empires. Used in TGN only.
Example: Burgundy region in France (TGN)</dct:description>
    <rdfs:comment>Place defined by administrative boundaries and conditions, including inhabited places, nations, and empires. Used in TGN only</rdfs:comment>
    <rdf:type rdf:resource="http://www.w3.org/2002/07/owl#Class"/>
    <rdfs:subClassOf rdf:resource="http://vocab.getty.edu/ontology#Subject"/>
  </rdf:Description>
  <rdf:Description rdf:about="http://vocab.getty.edu/ontology#ulan1223_crowned_by">
    <skos:example>Pope Leo III crowned Emperor Charlemagne</skos:example>
    <dc:title>crowned by - person</dc:title>
    <rdfs:isDefinedBy rdf:resource="http://vocab.getty.edu/ulan/"/>
    <owl:inverseOf rdf:resource="http://vocab.getty.edu/ontology#ulan1224_crowned"/>
    <rdfs:subPropertyOf rdf:resource="http://www.w3.org/2004/02/skos/core#related"/>
    <dc:identifier>1223</dc:identifier>
    <rdf:type rdf:resource="http://www.w3.org/2002/07/owl#ObjectProperty"/>
    <rdfs:isDefinedBy rdf:resource="http://vocab.getty.edu/ontology"/>
    <skos:prefLabel>ulan1223_crowned_by</skos:prefLabel>
    <dct:description>person - crowned by - person.&#13;
Example: Pope Leo III crowned Emperor Charlemagne</dct:description>
    <rdfs:domain rdf:resource="http://www.w3.org/2004/02/skos/core#Concept"/>
    <rdfs:range rdf:resource="http://www.w3.org/2004/02/skos/core#Concept"/>
  </rdf:Description>
  <rdf:Description rdf:about="http://vocab.getty.edu/ontology#ulan1532_uncle-aunt_of">
    <skos:example>Edouard Manet is the uncle/aunt of Julie Manet</skos:example>
    <rdf:type rdf:resource="http://www.w3.org/2002/07/owl#ObjectProperty"/>
    <rdfs:isDefinedBy rdf:resource="http://vocab.getty.edu/ulan/"/>
    <rdfs:subPropertyOf rdf:resource="http://www.w3.org/2004/02/skos/core#related"/>
    <dc:title>uncle/aunt of - person</dc:title>
    <rdfs:domain rdf:resource="http://www.w3.org/2004/02/skos/core#Concept"/>
    <rdfs:isDefinedBy rdf:resource="http://vocab.getty.edu/ontology"/>
    <dc:identifier>1532</dc:identifier>
    <rdfs:range rdf:resource="http://www.w3.org/2004/02/skos/core#Concept"/>
    <skos:prefLabel>ulan1532_uncle-aunt_of</skos:prefLabel>
    <dct:description>person - uncle/aunt of - person.&#13;
Example: Edouard Manet is the uncle/aunt of Julie Manet</dct:description>
  </rdf:Description>
  <rdf:Description rdf:about="http://vocab.getty.edu/ontology#ulan2676_teacher_at">
    <rdfs:domain rdf:resource="http://www.w3.org/2004/02/skos/core#Concept"/>
    <owl:inverseOf rdf:resource="http://vocab.getty.edu/ontology#ulan2677_teacher_was"/>
    <rdf:type rdf:resource="http://www.w3.org/2002/07/owl#ObjectProperty"/>
    <dct:description>person - teacher at - institution.&#13;
Example: Willem De Kooning was a teacher at Black Mountain College</dct:description>
    <dc:identifier>2676</dc:identifier>
    <rdfs:subPropertyOf rdf:resource="http://www.w3.org/2004/02/skos/core#related"/>
    <dc:title>teacher at - institution</dc:title>
    <rdfs:isDefinedBy rdf:resource="http://vocab.getty.edu/ulan/"/>
    <skos:prefLabel>ulan2676_teacher_at</skos:prefLabel>
    <rdfs:range rdf:resource="http://www.w3.org/2004/02/skos/core#Concept"/>
    <rdfs:isDefinedBy rdf:resource="http://vocab.getty.edu/ontology"/>
    <skos:example>Willem De Kooning was a teacher at Black Mountain College</skos:example>
  </rdf:Description>
  <rdf:Description rdf:about="http://vocab.getty.edu/term/type/UsedForTerm">
    <dct:description>A synonym.
Example: "handschriften" (Dutch) instead of "manuscripten"</dct:description>
    <skos:notation>UF</skos:notation>
    <skos:prefLabel>Used for Term</skos:prefLabel>
    <skos:scopeNote>A synonym</skos:scopeNote>
    <skos:example>"handschriften" (Dutch) instead of "manuscripten"</skos:example>
    <rdf:type rdf:resource="http://www.w3.org/2004/02/skos/core#Concept"/>
    <skos:inScheme rdf:resource="http://vocab.getty.edu/term/type/"/>
  </rdf:Description>
  <rdf:Description rdf:about="http://vocab.getty.edu/ontology#tgn3401_moved_from">
    <rdfs:subPropertyOf rdf:resource="http://www.w3.org/2004/02/skos/core#related"/>
    <skos:scopeNote>Note: places that were physically moved from one location to another, often due to the threat or occurrence of natural disaster.</skos:scopeNote>
    <skos:prefLabel>tgn3401_moved_from</skos:prefLabel>
    <dc:identifier>3401</dc:identifier>
    <rdfs:isDefinedBy rdf:resource="http://vocab.getty.edu/ontology"/>
    <rdf:type rdf:resource="http://www.w3.org/2002/07/owl#ObjectProperty"/>
    <owl:inverseOf rdf:resource="http://vocab.getty.edu/ontology#tgn3402_moved_to"/>
    <rdfs:range rdf:resource="http://www.w3.org/2004/02/skos/core#Concept"/>
    <dc:title>moved from - place</dc:title>
    <dct:description>place - moved from - place; Note: places that were physically moved from one location to another, often due to the threat or occurrence of natural disaster..&#13;
Example: Troupville, Georgia, USA was moved to Valdosta (Lowndes county, Georgia, USA)</dct:description>
    <skos:example>Troupville, Georgia, USA was moved to Valdosta (Lowndes county, Georgia, USA)</skos:example>
    <rdfs:domain rdf:resource="http://www.w3.org/2004/02/skos/core#Concept"/>
    <rdfs:isDefinedBy rdf:resource="http://vocab.getty.edu/tgn/"/>
  </rdf:Description>
  <rdf:Description rdf:about="http://vocab.getty.edu/ontology#ulan1214_court_artist_was">
    <rdfs:subPropertyOf rdf:resource="http://www.w3.org/2004/02/skos/core#related"/>
    <rdfs:isDefinedBy rdf:resource="http://vocab.getty.edu/ulan/"/>
    <skos:example>Peter Paul Rubens was court artist to Gonzaga Vincenzo I, Duke of Mantua</skos:example>
    <rdfs:isDefinedBy rdf:resource="http://vocab.getty.edu/ontology"/>
    <skos:example>Francisco de Goya was court artist to Charles IV, King of Spain</skos:example>
    <rdfs:domain rdf:resource="http://www.w3.org/2004/02/skos/core#Concept"/>
    <skos:prefLabel>ulan1214_court_artist_was</skos:prefLabel>
    <dc:title>court artist was - person</dc:title>
    <rdf:type rdf:resource="http://www.w3.org/2002/07/owl#ObjectProperty"/>
    <rdfs:range rdf:resource="http://www.w3.org/2004/02/skos/core#Concept"/>
    <dc:identifier>1214</dc:identifier>
    <dct:description>person - court artist was - person.&#13;
Example: Peter Paul Rubens was court artist to Gonzaga Vincenzo I, Duke of Mantua; Francisco de Goya was court artist to Charles IV, King of Spain</dct:description>
  </rdf:Description>
  <rdf:Description rdf:about="http://vocab.getty.edu/ontology#aat2882_reflect">
    <dct:description>things - reflect - language.&#13;
Example: Greek alphabet reflects Greek (language); Vedas reflect Sanskrit</dct:description>
    <skos:example>Vedas reflect Sanskrit</skos:example>
    <rdfs:isDefinedBy rdf:resource="http://vocab.getty.edu/aat/"/>
    <rdf:type rdf:resource="http://www.w3.org/2002/07/owl#ObjectProperty"/>
    <rdfs:subPropertyOf rdf:resource="http://www.w3.org/2004/02/skos/core#related"/>
    <skos:example>Greek alphabet reflects Greek (language)</skos:example>
    <dc:title>reflect - language</dc:title>
    <skos:prefLabel>aat2882_reflect</skos:prefLabel>
    <rdfs:domain rdf:resource="http://www.w3.org/2004/02/skos/core#Concept"/>
    <rdfs:range rdf:resource="http://www.w3.org/2004/02/skos/core#Concept"/>
    <dc:identifier>2882</dc:identifier>
    <rdfs:isDefinedBy rdf:resource="http://vocab.getty.edu/ontology"/>
  </rdf:Description>
  <rdf:Description rdf:about="http://vocab.getty.edu/ontology#Infer_isoBroaderPartitive">
    <rdf:type rdf:resource="http://www.ontotext.com/proton/protontop#PropRestr"/>
    <ptop:premise rdf:resource="http://vocab.getty.edu/ontology#broaderPartitiveExtended"/>
    <ptop:restriction rdf:resource="http://www.w3.org/2004/02/skos/core#broader"/>
    <ptop:conclusion rdf:resource="http://purl.org/iso25964/skos-thes#broaderPartitive"/>
  </rdf:Description>
  <rdf:Description rdf:about="http://vocab.getty.edu/term/kind/USPSCode">
    <skos:prefLabel>US Postal Service Code</skos:prefLabel>
    <skos:notation>USPS</skos:notation>
    <skos:example>"CA" for California</skos:example>
    <dct:description>Used in TGN only.
Example: "CA" for California</dct:description>
    <skos:scopeNote>Used in TGN only</skos:scopeNote>
    <rdf:type rdf:resource="http://www.w3.org/2004/02/skos/core#Concept"/>
    <skos:inScheme rdf:resource="http://vocab.getty.edu/term/kind/"/>
  </rdf:Description>
  <rdf:Description rdf:about="http://vocab.getty.edu/ontology#aat2432_requires">
    <skos:example>painting (image making) requires painting equipment</skos:example>
    <skos:prefLabel>aat2432_requires</skos:prefLabel>
    <rdfs:isDefinedBy rdf:resource="http://vocab.getty.edu/ontology"/>
    <rdfs:domain rdf:resource="http://www.w3.org/2004/02/skos/core#Concept"/>
    <dc:title>requires - things</dc:title>
    <dct:description>activity/event/process - requires - things/equipment.&#13;
Example: painting (image making) requires painting equipment; doweling requires dowels</dct:description>
    <rdfs:isDefinedBy rdf:resource="http://vocab.getty.edu/aat/"/>
    <dc:identifier>2432</dc:identifier>
    <rdfs:subPropertyOf rdf:resource="http://www.w3.org/2004/02/skos/core#related"/>
    <skos:example>doweling requires dowels</skos:example>
    <rdf:type rdf:resource="http://www.w3.org/2002/07/owl#ObjectProperty"/>
    <rdfs:range rdf:resource="http://www.w3.org/2004/02/skos/core#Concept"/>
  </rdf:Description>
  <rdf:Description rdf:about="http://vocab.getty.edu/ontology#prefLabelGVP">
    <rdfs:isDefinedBy rdf:resource="http://vocab.getty.edu/ontology"/>
    <dct:description>Term preferred by the Getty Vocabulary Program. The language is usually English. Applicable to AAT, ULAN, TGN. Used with skosxl:prefLabel</dct:description>
    <rdfs:range rdf:resource="http://www.w3.org/2008/05/skos-xl#Label"/>
    <rdfs:label>prefLabelGVP</rdfs:label>
    <rdf:type rdf:resource="http://www.w3.org/2002/07/owl#ObjectProperty"/>
    <skos:prefLabel>prefLabelGVP</skos:prefLabel>
    <rdfs:comment>Term preferred by the Getty Vocabulary Program. The language is usually English. Applicable to AAT, ULAN, TGN. Used with skosxl:prefLabel</rdfs:comment>
    <rdfs:domain rdf:resource="http://vocab.getty.edu/ontology#Subject"/>
  </rdf:Description>
  <rdf:Description rdf:about="http://vocab.getty.edu/term/kind/ProvisionalName">
    <skos:example>"Rockton" was provisional name considered before adoption of "Kent" (Ohio)</skos:example>
    <dct:description>Used in TGN only.
Example: "Rockton" was provisional name considered before adoption of "Kent" (Ohio)</dct:description>
    <skos:inScheme rdf:resource="http://vocab.getty.edu/term/kind/"/>
    <skos:notation>PN</skos:notation>
    <rdf:type rdf:resource="http://www.w3.org/2004/02/skos/core#Concept"/>
    <skos:scopeNote>Used in TGN only</skos:scopeNote>
    <skos:prefLabel>Provisional Name</skos:prefLabel>
  </rdf:Description>
  <rdf:Description rdf:about="http://vocab.getty.edu/ontology#Facet">
    <skos:example>Objects Facet (AAT), World (TGN), Artists (ULAN)</skos:example>
    <rdfs:label>Facet</rdfs:label>
    <rdfs:comment>One of the major divisions of a vocabulary</rdfs:comment>
    <skos:prefLabel>Facet</skos:prefLabel>
    <dct:description>One of the major divisions of a vocabulary.
Example: Objects Facet (AAT), World (TGN), Artists (ULAN)</dct:description>
    <rdfs:isDefinedBy rdf:resource="http://vocab.getty.edu/ontology"/>
    <rdfs:subClassOf rdf:resource="http://vocab.getty.edu/ontology#Subject"/>
    <rdfs:subClassOf rdf:resource="http://purl.org/iso25964/skos-thes#ThesaurusArray"/>
    <rdf:type rdf:resource="http://www.w3.org/2002/07/owl#Class"/>
  </rdf:Description>
  <rdf:Description rdf:about="http://vocab.getty.edu/ontology#tgn3202_capital_is">
    <rdfs:domain rdf:resource="http://www.w3.org/2004/02/skos/core#Concept"/>
    <skos:prefLabel>tgn3202_capital_is</skos:prefLabel>
    <rdfs:subPropertyOf rdf:resource="http://www.w3.org/2004/02/skos/core#related"/>
    <rdfs:isDefinedBy rdf:resource="http://vocab.getty.edu/ontology"/>
    <rdfs:isDefinedBy rdf:resource="http://vocab.getty.edu/tgn/"/>
    <rdf:type rdf:resource="http://www.w3.org/2002/07/owl#ObjectProperty"/>
    <dct:description>nation - capital is - city.&#13;
Example: London was the capital of Maxima Caesariensis from 296 to 800 CE</dct:description>
    <skos:example>London was the capital of Maxima Caesariensis from 296 to 800 CE</skos:example>
    <rdfs:range rdf:resource="http://www.w3.org/2004/02/skos/core#Concept"/>
    <dc:identifier>3202</dc:identifier>
    <dc:title>capital is - city</dc:title>
  </rdf:Description>
  <rdf:Description rdf:about="http://vocab.getty.edu/ontology#ulan1106_apprentice_was">
    <rdfs:isDefinedBy rdf:resource="http://vocab.getty.edu/ulan/"/>
    <rdfs:subPropertyOf rdf:resource="http://www.w3.org/2004/02/skos/core#related"/>
    <rdfs:domain rdf:resource="http://www.w3.org/2004/02/skos/core#Concept"/>
    <rdfs:isDefinedBy rdf:resource="http://vocab.getty.edu/ontology"/>
    <rdfs:range rdf:resource="http://www.w3.org/2004/02/skos/core#Concept"/>
    <skos:prefLabel>ulan1106_apprentice_was</skos:prefLabel>
    <dct:description>person - apprentice was - person.&#13;
Example: Nicolas Hawksmoor was the apprentice of Christopher Wren</dct:description>
    <skos:example>Nicolas Hawksmoor was the apprentice of Christopher Wren</skos:example>
    <rdf:type rdf:resource="http://www.w3.org/2002/07/owl#ObjectProperty"/>
    <dc:title>apprentice was - person</dc:title>
    <dc:identifier>1106</dc:identifier>
  </rdf:Description>
  <rdf:Description rdf:about="http://vocab.getty.edu/ontology#aat2398_focuses_on">
    <skos:example>musicology focuses on music</skos:example>
    <dct:description>field [of study]/discipline - focuses on - any.&#13;
Example: codicology focuses on manuscripts; musicology focuses on music; bontany focuses on Plantae (kingdom)</dct:description>
    <dc:identifier>2398</dc:identifier>
    <rdfs:isDefinedBy rdf:resource="http://vocab.getty.edu/ontology"/>
    <rdfs:subPropertyOf rdf:resource="http://www.w3.org/2004/02/skos/core#related"/>
    <skos:example>codicology focuses on manuscripts</skos:example>
    <skos:example>bontany focuses on Plantae (kingdom)</skos:example>
    <dc:title>focuses on - any</dc:title>
    <rdfs:isDefinedBy rdf:resource="http://vocab.getty.edu/aat/"/>
    <skos:prefLabel>aat2398_focuses_on</skos:prefLabel>
    <rdf:type rdf:resource="http://www.w3.org/2002/07/owl#ObjectProperty"/>
    <rdfs:range rdf:resource="http://www.w3.org/2004/02/skos/core#Concept"/>
    <rdfs:domain rdf:resource="http://www.w3.org/2004/02/skos/core#Concept"/>
  </rdf:Description>
  <rdf:Description rdf:about="http://vocab.getty.edu/ontology#ulan1314_partner_was">
    <skos:example>Louis H. Sullivan and Dankmar Adler were partners in Adler and Sullivan</skos:example>
    <rdfs:isDefinedBy rdf:resource="http://vocab.getty.edu/ulan/"/>
    <dc:identifier>1314</dc:identifier>
    <rdfs:subPropertyOf rdf:resource="http://www.w3.org/2004/02/skos/core#related"/>
    <dct:description>firm - partner was - person.&#13;
Example: Louis H. Sullivan and Dankmar Adler were partners in Adler and Sullivan</dct:description>
    <rdf:type rdf:resource="http://www.w3.org/2002/07/owl#ObjectProperty"/>
    <rdfs:domain rdf:resource="http://www.w3.org/2004/02/skos/core#Concept"/>
    <skos:prefLabel>ulan1314_partner_was</skos:prefLabel>
    <dc:title>partner was - person</dc:title>
    <rdfs:range rdf:resource="http://www.w3.org/2004/02/skos/core#Concept"/>
    <rdfs:isDefinedBy rdf:resource="http://vocab.getty.edu/ontology"/>
  </rdf:Description>
  <rdf:Description rdf:about="http://vocab.getty.edu/ontology#aat2801_conjuncted_with">
    <rdfs:range rdf:resource="http://www.w3.org/2004/02/skos/core#Concept"/>
    <skos:example>cups are conjuncted with saucers</skos:example>
    <dct:description>things - [are] conjuncted with - things.&#13;
Example: cups are conjuncted with saucers; dining tables are conjuncted with dining chairs</dct:description>
    <dc:title>conjuncted with - things</dc:title>
    <skos:example>dining tables are conjuncted with dining chairs</skos:example>
    <rdf:type rdf:resource="http://www.w3.org/2002/07/owl#ObjectProperty"/>
    <rdfs:isDefinedBy rdf:resource="http://vocab.getty.edu/aat/"/>
    <skos:prefLabel>aat2801_conjuncted_with</skos:prefLabel>
    <rdfs:subPropertyOf rdf:resource="http://www.w3.org/2004/02/skos/core#related"/>
    <rdfs:domain rdf:resource="http://www.w3.org/2004/02/skos/core#Concept"/>
    <rdf:type rdf:resource="http://www.w3.org/2002/07/owl#SymmetricProperty"/>
    <rdfs:isDefinedBy rdf:resource="http://vocab.getty.edu/ontology"/>
    <dc:identifier>2801</dc:identifier>
  </rdf:Description>
  <rdf:Description rdf:about="http://vocab.getty.edu/ontology#termFlag">
    <dct:description>Term Flag</dct:description>
    <skos:prefLabel>termFlag</skos:prefLabel>
    <rdfs:label>termFlag</rdfs:label>
    <rdfs:range rdf:resource="http://www.w3.org/2004/02/skos/core#Concept"/>
    <rdfs:domain rdf:resource="http://www.w3.org/2008/05/skos-xl#Label"/>
    <rdf:type rdf:resource="http://www.w3.org/2002/07/owl#ObjectProperty"/>
    <rdfs:isDefinedBy rdf:resource="http://vocab.getty.edu/ontology"/>
  </rdf:Description>
  <rdf:Description rdf:about="http://vocab.getty.edu/ontology#aat2209_used-located_in">
    <rdf:type rdf:resource="http://www.w3.org/2002/07/owl#ObjectProperty"/>
    <skos:example>glassware is used/located in glassworks (buildings)</skos:example>
    <skos:example>cave paintings are located in caves</skos:example>
    <rdfs:isDefinedBy rdf:resource="http://vocab.getty.edu/aat/"/>
    <rdfs:range rdf:resource="http://www.w3.org/2004/02/skos/core#Concept"/>
    <rdfs:domain rdf:resource="http://www.w3.org/2004/02/skos/core#Concept"/>
    <rdfs:isDefinedBy rdf:resource="http://vocab.getty.edu/ontology"/>
    <dc:identifier>2209</dc:identifier>
    <skos:prefLabel>aat2209_used-located_in</skos:prefLabel>
    <rdfs:subPropertyOf rdf:resource="http://www.w3.org/2004/02/skos/core#related"/>
    <dct:description>things -used/located in -  locus/setting.&#13;
Example: glassware is used/located in glassworks (buildings); cave paintings are located in caves</dct:description>
    <dc:title>used/located in - locus/setting</dc:title>
  </rdf:Description>
  <rdf:Description rdf:about="http://vocab.getty.edu/ontology#aat2802_exemplified_by">
    <rdfs:range rdf:resource="http://www.w3.org/2004/02/skos/core#Concept"/>
    <skos:prefLabel>aat2802_exemplified_by</skos:prefLabel>
    <dc:identifier>2802</dc:identifier>
    <rdf:type rdf:resource="http://www.w3.org/2002/07/owl#ObjectProperty"/>
    <skos:example>polytetrafluoroethyelene is exemplified by Teflon (TM)</skos:example>
    <dc:title>exemplified by - brand name</dc:title>
    <rdfs:isDefinedBy rdf:resource="http://vocab.getty.edu/aat/"/>
    <rdfs:subPropertyOf rdf:resource="http://www.w3.org/2004/02/skos/core#related"/>
    <rdfs:domain rdf:resource="http://www.w3.org/2004/02/skos/core#Concept"/>
    <rdfs:isDefinedBy rdf:resource="http://vocab.getty.edu/ontology"/>
    <dct:description>material - [is] exemplified by - brand name.&#13;
Example: petrolium jelly is exemplified by Vaseline (TM); polytetrafluoroethyelene is exemplified by Teflon (TM)</dct:description>
    <skos:example>petrolium jelly is exemplified by Vaseline (TM)</skos:example>
    <owl:inverseOf rdf:resource="http://vocab.getty.edu/ontology#aat2803_example_of"/>
  </rdf:Description>
  <rdf:Description rdf:about="http://vocab.getty.edu/ontology#ulan1008_meaning_-usage_overlaps_with">
    <skos:prefLabel>ulan1008_meaning_-usage_overlaps_with</skos:prefLabel>
    <dct:description>any - meaning /usage overlaps with - any.&#13;
Example: The meaning or usage of unknown Zimbabwean overlaps with unknown Rodesian</dct:description>
    <rdfs:isDefinedBy rdf:resource="http://vocab.getty.edu/ulan/"/>
    <rdfs:domain rdf:resource="http://www.w3.org/2004/02/skos/core#Concept"/>
    <rdf:type rdf:resource="http://www.w3.org/2002/07/owl#SymmetricProperty"/>
    <rdfs:range rdf:resource="http://www.w3.org/2004/02/skos/core#Concept"/>
    <rdfs:isDefinedBy rdf:resource="http://vocab.getty.edu/ontology"/>
    <skos:example>The meaning or usage of unknown Zimbabwean overlaps with unknown Rodesian</skos:example>
    <dc:identifier>1008</dc:identifier>
    <rdf:type rdf:resource="http://www.w3.org/2002/07/owl#ObjectProperty"/>
    <dc:title>meaning /usage overlaps with - any</dc:title>
    <rdfs:subPropertyOf rdf:resource="http://www.w3.org/2004/02/skos/core#related"/>
  </rdf:Description>
  <rdf:Description rdf:about="http://vocab.getty.edu/ontology#placeTypeNonPreferred">
    <rdfs:isDefinedBy rdf:resource="http://vocab.getty.edu/ontology"/>
    <rdfs:range rdf:resource="http://vocab.getty.edu/ontology#Subject"/>
    <rdfs:subPropertyOf rdf:resource="http://vocab.getty.edu/ontology#placeType"/>
    <skos:example>A non-preferred type of Machupicchu, Peru is "Inca center" (historical)</skos:example>
    <skos:prefLabel>placeTypeNonPreferred</skos:prefLabel>
    <rdf:type rdf:resource="http://www.w3.org/2002/07/owl#ObjectProperty"/>
    <rdfs:comment>A secondary type for a TGN Place. Domain is TGN concept, range is AAT concept</rdfs:comment>
    <dct:description>A secondary type for a TGN Place. Domain is TGN concept, range is AAT concept.
Example: A non-preferred type of Machupicchu, Peru is "Inca center" (historical)</dct:description>
    <rdfs:domain rdf:resource="http://vocab.getty.edu/ontology#Subject"/>
    <rdfs:label>placeTypeNonPreferred</rdfs:label>
  </rdf:Description>
  <rdf:Description rdf:about="http://vocab.getty.edu/ontology#aat2817_derived-made_from">
    <rdfs:domain rdf:resource="http://www.w3.org/2004/02/skos/core#Concept"/>
    <skos:example>wood board is derived/made from timber (lumber)</skos:example>
    <owl:inverseOf rdf:resource="http://vocab.getty.edu/ontology#aat2818_source_for"/>
    <skos:prefLabel>aat2817_derived-made_from</skos:prefLabel>
    <dct:description>material - [is] derived/made from - material.&#13;
Example: gypsum is derived/made from from anhydrite; wood board is derived/made from timber (lumber)</dct:description>
    <skos:example>gypsum is derived/made from from anhydrite</skos:example>
    <rdf:type rdf:resource="http://www.w3.org/2002/07/owl#ObjectProperty"/>
    <rdfs:isDefinedBy rdf:resource="http://vocab.getty.edu/aat/"/>
    <rdfs:subPropertyOf rdf:resource="http://www.w3.org/2004/02/skos/core#related"/>
    <dc:title>derived/made from - material</dc:title>
    <rdfs:range rdf:resource="http://www.w3.org/2004/02/skos/core#Concept"/>
    <rdfs:isDefinedBy rdf:resource="http://vocab.getty.edu/ontology"/>
    <dc:identifier>2817</dc:identifier>
  </rdf:Description>
  <rdf:Description rdf:about="http://vocab.getty.edu/ontology#ulan1547_romantic_partner_of">
    <rdfs:domain rdf:resource="http://www.w3.org/2004/02/skos/core#Concept"/>
    <skos:prefLabel>ulan1547_romantic_partner_of</skos:prefLabel>
    <rdfs:isDefinedBy rdf:resource="http://vocab.getty.edu/ontology"/>
    <skos:example>Vincent van Gogh and Clasina Hoornik were romantic partners</skos:example>
    <rdfs:range rdf:resource="http://www.w3.org/2004/02/skos/core#Concept"/>
    <skos:example>Pablo Picasso and Gaby Lespinasse were romantic partners</skos:example>
    <rdf:type rdf:resource="http://www.w3.org/2002/07/owl#ObjectProperty"/>
    <dct:description>person - romantic partner of - person.&#13;
Example: Pablo Picasso and Gaby Lespinasse were romantic partners; Vincent van Gogh and Clasina Hoornik were romantic partners</dct:description>
    <rdfs:isDefinedBy rdf:resource="http://vocab.getty.edu/ulan/"/>
    <dc:title>romantic partner of - person</dc:title>
    <rdfs:subPropertyOf rdf:resource="http://www.w3.org/2004/02/skos/core#related"/>
    <dc:identifier>1547</dc:identifier>
    <rdf:type rdf:resource="http://www.w3.org/2002/07/owl#SymmetricProperty"/>
  </rdf:Description>
  <rdf:Description rdf:about="http://vocab.getty.edu/ontology#broaderGeneric">
    <dct:description>BTG (Genus/Species, "is a") relation. We also infer iso-thes:broaderGeneric, which goes only between Concepts.
Example: calcite (AAT) BTG mineral (AAT)</dct:description>
    <rdf:type rdf:resource="http://www.w3.org/2002/07/owl#ObjectProperty"/>
    <rdfs:comment>BTG (Genus/Species, "is a") relation. We also infer iso-thes:broaderGeneric, which goes only between Concepts</rdfs:comment>
    <rdfs:subPropertyOf rdf:resource="http://vocab.getty.edu/ontology#broaderGenericExtended"/>
    <skos:example>calcite (AAT) BTG mineral (AAT)</skos:example>
    <rdfs:subPropertyOf rdf:resource="http://vocab.getty.edu/ontology#broader"/>
    <rdfs:label>broaderGeneric</rdfs:label>
    <rdfs:range rdf:resource="http://vocab.getty.edu/ontology#Subject"/>
    <skos:prefLabel>broaderGeneric</skos:prefLabel>
    <rdfs:isDefinedBy rdf:resource="http://vocab.getty.edu/ontology"/>
    <rdfs:domain rdf:resource="http://vocab.getty.edu/ontology#Subject"/>
  </rdf:Description>
  <rdf:Description rdf:about="http://vocab.getty.edu/aat/">
    <foaf:homepage rdf:resource="http://www.getty.edu/research/tools/vocabularies/aat/"/>
    <rdfs:comment>The Art and Architecture Thesaurus concept scheme</rdfs:comment>
    <skos:prefLabel>Art and Architecture Thesaurus</skos:prefLabel>
    <rdfs:label>Art and Architecture Thesaurus</rdfs:label>
    <vann:preferredNamespaceUri>http://vocab.getty.edu/aat/</vann:preferredNamespaceUri>
    <dct:creator rdf:resource="http://www.ontotext.com"/>
    <dct:creator rdf:resource="http://www.getty.edu/research/"/>
    <dct:created rdf:datatype="http://www.w3.org/2001/XMLSchema#date">2014-02-20</dct:created>
    <vann:preferredNamespacePrefix>aat</vann:preferredNamespacePrefix>
    <rdfs:seeAlso rdf:resource="http://www.getty.edu/research/tools/vocabularies/lod/"/>
    <rdfs:seeAlso rdf:resource="http://vocab.getty.edu/"/>
    <rdfs:seeAlso rdf:resource="http://vocab.getty.edu/.well-known/void"/>
    <rdf:type rdf:resource="http://www.w3.org/2004/02/skos/core#ConceptScheme"/>
  </rdf:Description>
  <rdf:Description rdf:about="http://vocab.getty.edu/ontology#ulan1204_donor_was">
    <skos:example>Donor to the National Gallery of Art was Andrew W. Mellon</skos:example>
    <rdfs:isDefinedBy rdf:resource="http://vocab.getty.edu/ontology"/>
    <dc:title>donor was - person/firm/family</dc:title>
    <dct:description>person/firm/family - donor was - person/firm/family.&#13;
Example: Donor to the National Gallery of Art was Andrew W. Mellon</dct:description>
    <rdfs:isDefinedBy rdf:resource="http://vocab.getty.edu/ulan/"/>
    <rdfs:subPropertyOf rdf:resource="http://www.w3.org/2004/02/skos/core#related"/>
    <rdfs:range rdf:resource="http://www.w3.org/2004/02/skos/core#Concept"/>
    <dc:identifier>1204</dc:identifier>
    <rdf:type rdf:resource="http://www.w3.org/2002/07/owl#ObjectProperty"/>
    <skos:prefLabel>ulan1204_donor_was</skos:prefLabel>
    <rdfs:domain rdf:resource="http://www.w3.org/2004/02/skos/core#Concept"/>
  </rdf:Description>
  <rdf:Description rdf:about="http://vocab.getty.edu/ontology#aat2848_involved_in">
    <dc:title>involved in - activity/event</dc:title>
    <skos:example>bulls (animals) are involved in bullfighting</skos:example>
    <skos:prefLabel>aat2848_involved_in</skos:prefLabel>
    <owl:inverseOf rdf:resource="http://vocab.getty.edu/ontology#aat2849_involves"/>
    <dc:identifier>2848</dc:identifier>
    <rdfs:subPropertyOf rdf:resource="http://www.w3.org/2004/02/skos/core#related"/>
    <rdf:type rdf:resource="http://www.w3.org/2002/07/owl#ObjectProperty"/>
    <dct:description>genus/species - is involved in - activity/event.&#13;
Example: bulls (animals) are involved in bullfighting; Equus caballus (species) is involved in polo(field sport)</dct:description>
    <skos:example>Equus caballus (species) is involved in polo(field sport)</skos:example>
    <rdfs:isDefinedBy rdf:resource="http://vocab.getty.edu/aat/"/>
    <rdfs:range rdf:resource="http://www.w3.org/2004/02/skos/core#Concept"/>
    <rdfs:domain rdf:resource="http://www.w3.org/2004/02/skos/core#Concept"/>
    <rdfs:isDefinedBy rdf:resource="http://vocab.getty.edu/ontology"/>
  </rdf:Description>
  <rdf:Description rdf:about="http://vocab.getty.edu/ontology#ulan1007_distinguished_from">
    <rdfs:domain rdf:resource="http://www.w3.org/2004/02/skos/core#Concept"/>
    <skos:prefLabel>ulan1007_distinguished_from</skos:prefLabel>
    <rdfs:isDefinedBy rdf:resource="http://vocab.getty.edu/ulan/"/>
    <dct:description>any - distinguished from - any.&#13;
Example: Laura Theresa Alma-Tadema is distinguished from Lawrence Alma-Tadema; The Noguchi Museum is distinguished form Isamu Noguchi Garden Museum Japan</dct:description>
    <dc:title>distinguished from - any</dc:title>
    <rdf:type rdf:resource="http://www.w3.org/2002/07/owl#ObjectProperty"/>
    <rdfs:subPropertyOf rdf:resource="http://www.w3.org/2004/02/skos/core#related"/>
    <skos:example>The Noguchi Museum is distinguished form Isamu Noguchi Garden Museum Japan</skos:example>
    <rdfs:range rdf:resource="http://www.w3.org/2004/02/skos/core#Concept"/>
    <skos:example>Laura Theresa Alma-Tadema is distinguished from Lawrence Alma-Tadema</skos:example>
    <rdf:type rdf:resource="http://www.w3.org/2002/07/owl#SymmetricProperty"/>
    <rdfs:isDefinedBy rdf:resource="http://vocab.getty.edu/ontology"/>
    <dc:identifier>1007</dc:identifier>
  </rdf:Description>
  <rdf:Description rdf:about="http://vocab.getty.edu/ontology#tgn3612_administrative_entity_for">
    <rdf:type rdf:resource="http://www.w3.org/2002/07/owl#ObjectProperty"/>
    <dc:title>administrative entity for - place</dc:title>
    <rdfs:range rdf:resource="http://www.w3.org/2004/02/skos/core#Concept"/>
    <skos:example>Ortonovo (Massa-Carra province, Tuscany, Italy) is the administrative entity for Luni (La Spezia province, Liguria, Italy)</skos:example>
    <skos:prefLabel>tgn3612_administrative_entity_for</skos:prefLabel>
    <dc:identifier>3612</dc:identifier>
    <rdfs:domain rdf:resource="http://www.w3.org/2004/02/skos/core#Concept"/>
    <dct:description>place - administrative entity for - place.&#13;
Example: Ortonovo (Massa-Carra province, Tuscany, Italy) is the administrative entity for Luni (La Spezia province, Liguria, Italy)</dct:description>
    <rdfs:subPropertyOf rdf:resource="http://www.w3.org/2004/02/skos/core#related"/>
    <rdfs:isDefinedBy rdf:resource="http://vocab.getty.edu/ontology"/>
    <rdfs:isDefinedBy rdf:resource="http://vocab.getty.edu/tgn/"/>
  </rdf:Description>
  <rdf:Description rdf:about="http://vocab.getty.edu/ontology#aat2205_causes-is_required">
    <dc:title>causes/is required - activity/event</dc:title>
    <rdfs:isDefinedBy rdf:resource="http://vocab.getty.edu/aat/"/>
    <dct:description>activity/event/[process/function] - causes/is required for - activity/event/[process/function].&#13;
Example: on-demand printing causes/is required for on-demand publishing;  preserving causes/is required for preservation</dct:description>
    <rdfs:domain rdf:resource="http://www.w3.org/2004/02/skos/core#Concept"/>
    <rdfs:isDefinedBy rdf:resource="http://vocab.getty.edu/ontology"/>
    <rdfs:subPropertyOf rdf:resource="http://www.w3.org/2004/02/skos/core#related"/>
    <skos:example>preserving causes/is required for preservation</skos:example>
    <owl:inverseOf rdf:resource="http://vocab.getty.edu/ontology#aat2206_caused_by-requires"/>
    <skos:prefLabel>aat2205_causes-is_required</skos:prefLabel>
    <rdfs:range rdf:resource="http://www.w3.org/2004/02/skos/core#Concept"/>
    <rdf:type rdf:resource="http://www.w3.org/2002/07/owl#ObjectProperty"/>
    <dc:identifier>2205</dc:identifier>
    <skos:example>on-demand printing causes/is required for on-demand publishing</skos:example>
  </rdf:Description>
  <rdf:Description rdf:about="http://vocab.getty.edu/ontology#ulan1542_consort_of">
    <rdfs:isDefinedBy rdf:resource="http://vocab.getty.edu/ulan/"/>
    <skos:prefLabel>ulan1542_consort_of</skos:prefLabel>
    <rdfs:domain rdf:resource="http://www.w3.org/2004/02/skos/core#Concept"/>
    <owl:inverseOf rdf:resource="http://vocab.getty.edu/ontology#ulan1543_consort_was"/>
    <dc:title>consort of - person</dc:title>
    <skos:example>Empress Livia was the consort of Augustus, Emperor of Rome</skos:example>
    <rdfs:isDefinedBy rdf:resource="http://vocab.getty.edu/ontology"/>
    <rdfs:range rdf:resource="http://www.w3.org/2004/02/skos/core#Concept"/>
    <dc:identifier>1542</dc:identifier>
    <dct:description>person - consort of - person.&#13;
Example: Empress Livia was the consort of Augustus, Emperor of Rome</dct:description>
    <rdfs:subPropertyOf rdf:resource="http://www.w3.org/2004/02/skos/core#related"/>
    <rdf:type rdf:resource="http://www.w3.org/2002/07/owl#ObjectProperty"/>
  </rdf:Description>
  <rdf:Description rdf:about="http://vocab.getty.edu/term/kind/ScientificOrTechnical">
    <rdf:type rdf:resource="http://www.w3.org/2004/02/skos/core#Concept"/>
    <skos:inScheme rdf:resource="http://vocab.getty.edu/term/kind/"/>
    <skos:scopeNote>Scientific taxon name (genus, species, etc). Used in AAT only. All such are emitted marked with English language, and most have the same string marked with Latin</skos:scopeNote>
    <skos:example>"Boswellia sacra"@la, also emitted as "Boswellia sacra"@en, is scientific name of "frankincense"</skos:example>
    <dct:description>Scientific taxon name (genus, species, etc). Used in AAT only. All such are emitted marked with English language, and most have the same string marked with Latin.
Example: "Boswellia sacra"@la, also emitted as "Boswellia sacra"@en, is scientific name of "frankincense"</dct:description>
    <skos:notation>S</skos:notation>
    <skos:prefLabel>Scientific or Technical term</skos:prefLabel>
  </rdf:Description>
  <rdf:Description rdf:about="http://vocab.getty.edu/ontology#tgn3510_historical_connection">
    <rdfs:range rdf:resource="http://www.w3.org/2004/02/skos/core#Concept"/>
    <rdf:type rdf:resource="http://www.w3.org/2002/07/owl#SymmetricProperty"/>
    <rdfs:isDefinedBy rdf:resource="http://vocab.getty.edu/ontology"/>
    <skos:prefLabel>tgn3510_historical_connection</skos:prefLabel>
    <dc:title>historical connection - any</dc:title>
    <rdfs:domain rdf:resource="http://www.w3.org/2004/02/skos/core#Concept"/>
    <rdfs:subPropertyOf rdf:resource="http://www.w3.org/2004/02/skos/core#related"/>
    <rdf:type rdf:resource="http://www.w3.org/2002/07/owl#ObjectProperty"/>
    <rdfs:isDefinedBy rdf:resource="http://vocab.getty.edu/tgn/"/>
    <dc:identifier>3510</dc:identifier>
    <skos:example>Guyenne, France (historical region) has a historical connection to Gascogne (France) (historical region)</skos:example>
    <dct:description>any - historical connection - any.&#13;
Example: Guyenne, France (historical region) has a historical connection to Gascogne (France) (historical region)</dct:description>
  </rdf:Description>
  <rdf:Description rdf:about="http://vocab.getty.edu/ontology#ulan1332_worker_was">
    <rdf:type rdf:resource="http://www.w3.org/2002/07/owl#ObjectProperty"/>
    <skos:prefLabel>ulan1332_worker_was</skos:prefLabel>
    <dct:description>person - worker was - any.&#13;
Example: Workers for the Carracci family included Scarsellino and Domenichino</dct:description>
    <rdfs:range rdf:resource="http://www.w3.org/2004/02/skos/core#Concept"/>
    <rdfs:isDefinedBy rdf:resource="http://vocab.getty.edu/ontology"/>
    <rdfs:domain rdf:resource="http://www.w3.org/2004/02/skos/core#Concept"/>
    <skos:example>Workers for the Carracci family included Scarsellino and Domenichino</skos:example>
    <rdfs:isDefinedBy rdf:resource="http://vocab.getty.edu/ulan/"/>
    <dc:title>worker was - any</dc:title>
    <rdfs:subPropertyOf rdf:resource="http://www.w3.org/2004/02/skos/core#related"/>
    <dc:identifier>1332</dc:identifier>
  </rdf:Description>
  <rdf:Description rdf:about="http://vocab.getty.edu/ontology#ulan1582_ancestor_of">
    <rdf:type rdf:resource="http://www.w3.org/2002/07/owl#ObjectProperty"/>
    <dc:title>ancestor of - person</dc:title>
    <skos:prefLabel>ulan1582_ancestor_of</skos:prefLabel>
    <dct:description>person - ancestor of - person.&#13;
Example: Paolo Veronese is the ancestor of Paolo Caliari</dct:description>
    <rdfs:isDefinedBy rdf:resource="http://vocab.getty.edu/ontology"/>
    <skos:example>Paolo Veronese is the ancestor of Paolo Caliari</skos:example>
    <rdfs:domain rdf:resource="http://www.w3.org/2004/02/skos/core#Concept"/>
    <rdfs:subPropertyOf rdf:resource="http://www.w3.org/2004/02/skos/core#related"/>
    <rdfs:isDefinedBy rdf:resource="http://vocab.getty.edu/ulan/"/>
    <rdfs:range rdf:resource="http://www.w3.org/2004/02/skos/core#Concept"/>
    <dc:identifier>1582</dc:identifier>
  </rdf:Description>
  <rdf:Description rdf:about="http://vocab.getty.edu/ontology#aat2212_produced_by">
    <rdf:type rdf:resource="http://www.w3.org/2002/07/owl#ObjectProperty"/>
    <skos:example>punchwork is produced by punches (marking tools)</skos:example>
    <dct:description>things - [are] produced by - things/[equipment].&#13;
Example: stereoscopic photographs are produced by stereoscopic cameras; punchwork is produced by punches (marking tools)</dct:description>
    <dc:identifier>2212</dc:identifier>
    <rdfs:range rdf:resource="http://www.w3.org/2004/02/skos/core#Concept"/>
    <rdfs:isDefinedBy rdf:resource="http://vocab.getty.edu/aat/"/>
    <rdfs:isDefinedBy rdf:resource="http://vocab.getty.edu/ontology"/>
    <skos:prefLabel>aat2212_produced_by</skos:prefLabel>
    <rdfs:domain rdf:resource="http://www.w3.org/2004/02/skos/core#Concept"/>
    <dc:title>produced by - things</dc:title>
    <skos:example>stereoscopic photographs are produced by stereoscopic cameras</skos:example>
    <rdfs:subPropertyOf rdf:resource="http://www.w3.org/2004/02/skos/core#related"/>
  </rdf:Description>
  <rdf:Description rdf:about="http://vocab.getty.edu/ontology#tgn3611_administrative_dependent_of">
    <rdf:type rdf:resource="http://www.w3.org/2002/07/owl#ObjectProperty"/>
    <skos:prefLabel>tgn3611_administrative_dependent_of</skos:prefLabel>
    <owl:inverseOf rdf:resource="http://vocab.getty.edu/ontology#tgn3612_administrative_entity_for"/>
    <rdfs:range rdf:resource="http://www.w3.org/2004/02/skos/core#Concept"/>
    <rdfs:domain rdf:resource="http://www.w3.org/2004/02/skos/core#Concept"/>
    <rdfs:isDefinedBy rdf:resource="http://vocab.getty.edu/ontology"/>
    <dc:identifier>3611</dc:identifier>
    <dct:description>place - administrative dependent of - place; New.&#13;
Example: Luni (La Spezia province, Liguria, Italy) is the admisistrative dependent of Ortonovo (Massa-Carrara province, Tuscany, Italy)</dct:description>
    <skos:scopeNote>New</skos:scopeNote>
    <rdfs:subPropertyOf rdf:resource="http://www.w3.org/2004/02/skos/core#related"/>
    <rdfs:isDefinedBy rdf:resource="http://vocab.getty.edu/tgn/"/>
    <dc:title>administrative dependent of - place</dc:title>
    <skos:example>Luni (La Spezia province, Liguria, Italy) is the admisistrative dependent of Ortonovo (Massa-Carrara province, Tuscany, Italy)</skos:example>
  </rdf:Description>
  <rdf:Description rdf:about="http://vocab.getty.edu/ontology#aat2876_characterized_by">
    <rdfs:subPropertyOf rdf:resource="http://www.w3.org/2004/02/skos/core#related"/>
    <dct:description>style/period/culture - [is] characterized by - language.&#13;
Example: Afar (culture) is characterized by Afar (language); Celtic (culture) is characterized by Celtic (language)</dct:description>
    <dc:title>characterized by - language</dc:title>
    <rdfs:isDefinedBy rdf:resource="http://vocab.getty.edu/ontology"/>
    <rdf:type rdf:resource="http://www.w3.org/2002/07/owl#ObjectProperty"/>
    <skos:example>Afar (culture) is characterized by Afar (language)</skos:example>
    <skos:prefLabel>aat2876_characterized_by</skos:prefLabel>
    <rdfs:range rdf:resource="http://www.w3.org/2004/02/skos/core#Concept"/>
    <rdfs:domain rdf:resource="http://www.w3.org/2004/02/skos/core#Concept"/>
    <rdfs:isDefinedBy rdf:resource="http://vocab.getty.edu/aat/"/>
    <dc:identifier>2876</dc:identifier>
    <skos:example>Celtic (culture) is characterized by Celtic (language)</skos:example>
  </rdf:Description>
  <rdf:Description rdf:about="http://vocab.getty.edu/ontology#aat2507_produce-process">
    <rdfs:isDefinedBy rdf:resource="http://vocab.getty.edu/ontology"/>
    <skos:example>cotton (fiber) is produced/processed by cotton gins</skos:example>
    <skos:example>groundwater is produced/processed by water wells</skos:example>
    <skos:prefLabel>aat2507_produce-process</skos:prefLabel>
    <dc:identifier>2507</dc:identifier>
    <rdfs:subPropertyOf rdf:resource="http://www.w3.org/2004/02/skos/core#related"/>
    <rdf:type rdf:resource="http://www.w3.org/2002/07/owl#ObjectProperty"/>
    <rdfs:isDefinedBy rdf:resource="http://vocab.getty.edu/aat/"/>
    <dct:description>things/[equipment] - produce/process - material.&#13;
Example: cotton (fiber) is produced/processed by cotton gins; groundwater is produced/processed by water wells</dct:description>
    <rdfs:range rdf:resource="http://www.w3.org/2004/02/skos/core#Concept"/>
    <owl:inverseOf rdf:resource="http://vocab.getty.edu/ontology#aat2508_produced-processed_by"/>
    <dc:title>produce/process - material</dc:title>
    <rdfs:domain rdf:resource="http://www.w3.org/2004/02/skos/core#Concept"/>
  </rdf:Description>
  <rdf:Description rdf:about="http://vocab.getty.edu/ontology#ulan2575_directed_by">
    <dc:identifier>2575</dc:identifier>
    <rdfs:isDefinedBy rdf:resource="http://vocab.getty.edu/ontology"/>
    <rdfs:subPropertyOf rdf:resource="http://www.w3.org/2004/02/skos/core#related"/>
    <rdfs:domain rdf:resource="http://www.w3.org/2004/02/skos/core#Concept"/>
    <dct:description>institution - directed by - person.&#13;
Example: Gobelins Tapestry Manufactory was directed by Jean Jans I</dct:description>
    <skos:example>Gobelins Tapestry Manufactory was directed by Jean Jans I</skos:example>
    <rdfs:range rdf:resource="http://www.w3.org/2004/02/skos/core#Concept"/>
    <rdf:type rdf:resource="http://www.w3.org/2002/07/owl#ObjectProperty"/>
    <skos:prefLabel>ulan2575_directed_by</skos:prefLabel>
    <rdfs:isDefinedBy rdf:resource="http://vocab.getty.edu/ulan/"/>
    <dc:title>directed by - person</dc:title>
  </rdf:Description>
  <rdf:Description rdf:about="http://vocab.getty.edu/ontology#ulan1203_donor_of">
    <rdfs:subPropertyOf rdf:resource="http://www.w3.org/2004/02/skos/core#related"/>
    <rdfs:isDefinedBy rdf:resource="http://vocab.getty.edu/ulan/"/>
    <dc:identifier>1203</dc:identifier>
    <rdfs:range rdf:resource="http://www.w3.org/2004/02/skos/core#Concept"/>
    <rdfs:isDefinedBy rdf:resource="http://vocab.getty.edu/ontology"/>
    <skos:example>Andrew W. Mellon was a donor of National Gallery of Art</skos:example>
    <dct:description>person/firm/family - donor of - person/firm/family.&#13;
Example: Andrew W. Mellon was a donor of National Gallery of Art</dct:description>
    <rdfs:domain rdf:resource="http://www.w3.org/2004/02/skos/core#Concept"/>
    <owl:inverseOf rdf:resource="http://vocab.getty.edu/ontology#ulan1204_donor_was"/>
    <skos:prefLabel>ulan1203_donor_of</skos:prefLabel>
    <dc:title>donor of - person/firm/family</dc:title>
    <rdf:type rdf:resource="http://www.w3.org/2002/07/owl#ObjectProperty"/>
  </rdf:Description>
  <rdf:Description rdf:about="http://vocab.getty.edu/ontology#ulan2583_chairman_of">
    <skos:prefLabel>ulan2583_chairman_of</skos:prefLabel>
    <rdfs:isDefinedBy rdf:resource="http://vocab.getty.edu/ulan/"/>
    <rdf:type rdf:resource="http://www.w3.org/2002/07/owl#ObjectProperty"/>
    <rdfs:range rdf:resource="http://www.w3.org/2004/02/skos/core#Concept"/>
    <dc:title>chairman of - institution</dc:title>
    <rdfs:domain rdf:resource="http://www.w3.org/2004/02/skos/core#Concept"/>
    <dc:identifier>2583</dc:identifier>
    <rdfs:subPropertyOf rdf:resource="http://www.w3.org/2004/02/skos/core#related"/>
    <rdfs:isDefinedBy rdf:resource="http://vocab.getty.edu/ontology"/>
    <dct:description>person - chairman of - institution</dct:description>
    <owl:inverseOf rdf:resource="http://vocab.getty.edu/ontology#ulan2584_chaired_by"/>
  </rdf:Description>
  <rdf:Description rdf:about="http://vocab.getty.edu/ontology#ulan1574_godparent_of">
    <rdfs:domain rdf:resource="http://www.w3.org/2004/02/skos/core#Concept"/>
    <owl:inverseOf rdf:resource="http://vocab.getty.edu/ontology#ulan1575_godchild_of"/>
    <rdfs:isDefinedBy rdf:resource="http://vocab.getty.edu/ulan/"/>
    <dct:description>person - godparent of - person.&#13;
Example: Jean-Baptiste Goy is godparent of Jean I Nocret</dct:description>
    <rdfs:subPropertyOf rdf:resource="http://www.w3.org/2004/02/skos/core#related"/>
    <rdf:type rdf:resource="http://www.w3.org/2002/07/owl#ObjectProperty"/>
    <skos:prefLabel>ulan1574_godparent_of</skos:prefLabel>
    <dc:identifier>1574</dc:identifier>
    <dc:title>godparent of - person</dc:title>
    <rdfs:range rdf:resource="http://www.w3.org/2004/02/skos/core#Concept"/>
    <rdfs:isDefinedBy rdf:resource="http://vocab.getty.edu/ontology"/>
    <skos:example>Jean-Baptiste Goy is godparent of Jean I Nocret</skos:example>
  </rdf:Description>
  <rdf:Description rdf:about="http://vocab.getty.edu/ontology#aat2292_work-live_in">
    <dc:title>work/live in - locus/setting</dc:title>
    <dc:identifier>2292</dc:identifier>
    <rdfs:domain rdf:resource="http://www.w3.org/2004/02/skos/core#Concept"/>
    <rdfs:isDefinedBy rdf:resource="http://vocab.getty.edu/aat/"/>
    <skos:example>rope-makers live/work in roperies</skos:example>
    <rdf:type rdf:resource="http://www.w3.org/2002/07/owl#ObjectProperty"/>
    <rdfs:subPropertyOf rdf:resource="http://www.w3.org/2004/02/skos/core#related"/>
    <rdfs:range rdf:resource="http://www.w3.org/2004/02/skos/core#Concept"/>
    <skos:example>nuns live/work in convents (nunneries)</skos:example>
    <skos:prefLabel>aat2292_work-live_in</skos:prefLabel>
    <skos:example>libraries (institutions) live/work in libraries (buildings)</skos:example>
    <rdfs:isDefinedBy rdf:resource="http://vocab.getty.edu/ontology"/>
    <dct:description>[actor or institution having] role - work/live/[exist] in - locus/setting.&#13;
Example: rope-makers live/work in roperies; nuns live/work in convents (nunneries); libraries (institutions) live/work in libraries (buildings)</dct:description>
  </rdf:Description>
  <rdf:Description rdf:about="http://vocab.getty.edu/term/kind/OfficialName">
    <skos:inScheme rdf:resource="http://vocab.getty.edu/term/kind/"/>
    <rdf:type rdf:resource="http://www.w3.org/2004/02/skos/core#Concept"/>
    <skos:example>"Noyen-sur-Seine" is official name of 7030197 "Noyen" (TGN)</skos:example>
    <dct:description>Used in TGN and ULAN.
Example: "Noyen-sur-Seine" is official name of 7030197 "Noyen" (TGN)</dct:description>
    <skos:notation>O</skos:notation>
    <skos:prefLabel>Official Name</skos:prefLabel>
    <skos:scopeNote>Used in TGN and ULAN</skos:scopeNote>
  </rdf:Description>
  <rdf:Description rdf:about="http://vocab.getty.edu/term/kind/ChemicalName">
    <skos:scopeNote>Term is the chemical name for the descriptor. Used in AAT only</skos:scopeNote>
    <skos:notation>CN</skos:notation>
    <skos:prefLabel>Chemical Name</skos:prefLabel>
    <rdf:type rdf:resource="http://www.w3.org/2004/02/skos/core#Concept"/>
    <skos:example>"sodium tetraborate decahydrate" is chemical name for "borax"</skos:example>
    <skos:inScheme rdf:resource="http://vocab.getty.edu/term/kind/"/>
    <dct:description>Term is the chemical name for the descriptor. Used in AAT only.
Example: "sodium tetraborate decahydrate" is chemical name for "borax"</dct:description>
  </rdf:Description>
  <rdf:Description rdf:about="http://vocab.getty.edu/ontology#aat2602_possess-exist_in">
    <dc:title>possess/exist in - attributes /associated concepts</dc:title>
    <dc:identifier>2602</dc:identifier>
    <rdfs:isDefinedBy rdf:resource="http://vocab.getty.edu/aat/"/>
    <rdf:type rdf:resource="http://www.w3.org/2002/07/owl#ObjectProperty"/>
    <skos:prefLabel>aat2602_possess-exist_in</skos:prefLabel>
    <rdfs:subPropertyOf rdf:resource="http://www.w3.org/2004/02/skos/core#related"/>
    <skos:example>nomads possess/exist in [state of] nomadism</skos:example>
    <skos:example>adults possess/exist in adulthood</skos:example>
    <dct:description>role [of actors] - possess/exist in - attributes /associated concepts.&#13;
Example: adults possess/exist in adulthood; nomads possess/exist in [state of] nomadism</dct:description>
    <rdfs:domain rdf:resource="http://www.w3.org/2004/02/skos/core#Concept"/>
    <rdfs:range rdf:resource="http://www.w3.org/2004/02/skos/core#Concept"/>
    <rdfs:isDefinedBy rdf:resource="http://vocab.getty.edu/ontology"/>
  </rdf:Description>
  <rdf:Description rdf:about="http://vocab.getty.edu/ontology#agentTypePreferred">
    <rdfs:range rdf:resource="http://vocab.getty.edu/ontology#Subject"/>
    <rdfs:domain rdf:resource="http://vocab.getty.edu/ontology#Subject"/>
    <rdfs:isDefinedBy rdf:resource="http://vocab.getty.edu/ontology"/>
    <dct:description>The primary type of a ULAN Person or Corporate body. Domain is ULAN concept, range is AAT concept.
Example: The preferred type of "Albrecht Duerer Workshop" (ULAN) is "workshop" (AAT)</dct:description>
    <rdfs:subPropertyOf rdf:resource="http://vocab.getty.edu/ontology#agentType"/>
    <rdfs:label>agentTypePreferred</rdfs:label>
    <skos:example>The preferred type of "Albrecht Duerer Workshop" (ULAN) is "workshop" (AAT)</skos:example>
    <rdf:type rdf:resource="http://www.w3.org/2002/07/owl#ObjectProperty"/>
    <skos:prefLabel>agentTypePreferred</skos:prefLabel>
    <rdfs:comment>The primary type of a ULAN Person or Corporate body. Domain is ULAN concept, range is AAT concept</rdfs:comment>
  </rdf:Description>
  <rdf:Description rdf:about="http://vocab.getty.edu/ontology#aat2837_source_for">
    <dct:description>genus/species [or its parts] - [is] source for - things.&#13;
Example: Phormium tenax (species) is the source for k?kaku; Struthio camelus(species) is the source for ostrich-egg cups</dct:description>
    <rdfs:domain rdf:resource="http://www.w3.org/2004/02/skos/core#Concept"/>
    <dc:title>source for - things</dc:title>
    <rdfs:subPropertyOf rdf:resource="http://www.w3.org/2004/02/skos/core#related"/>
    <rdfs:isDefinedBy rdf:resource="http://vocab.getty.edu/ontology"/>
    <dc:identifier>2837</dc:identifier>
    <rdfs:isDefinedBy rdf:resource="http://vocab.getty.edu/aat/"/>
    <skos:example>Phormium tenax (species) is the source for k?kaku</skos:example>
    <skos:example>Struthio camelus(species) is the source for ostrich-egg cups</skos:example>
    <rdf:type rdf:resource="http://www.w3.org/2002/07/owl#ObjectProperty"/>
    <rdfs:range rdf:resource="http://www.w3.org/2004/02/skos/core#Concept"/>
    <skos:prefLabel>aat2837_source_for</skos:prefLabel>
  </rdf:Description>
  <rdf:Description rdf:about="http://vocab.getty.edu/ontology#aat2841_derived-made_from">
    <dc:identifier>2841</dc:identifier>
    <rdf:type rdf:resource="http://www.w3.org/2002/07/owl#ObjectProperty"/>
    <dct:description>material - [is] derived/made from - genus/species.&#13;
Example: alpaca (wool) is derived from Vicugna pacos (species); maple (wood) is derived from Acer (genus)</dct:description>
    <rdfs:range rdf:resource="http://www.w3.org/2004/02/skos/core#Concept"/>
    <skos:example>alpaca (wool) is derived from Vicugna pacos (species)</skos:example>
    <dc:title>derived/made from - genus/species</dc:title>
    <owl:inverseOf rdf:resource="http://vocab.getty.edu/ontology#aat2842_source_for"/>
    <rdfs:domain rdf:resource="http://www.w3.org/2004/02/skos/core#Concept"/>
    <rdfs:subPropertyOf rdf:resource="http://www.w3.org/2004/02/skos/core#related"/>
    <rdfs:isDefinedBy rdf:resource="http://vocab.getty.edu/ontology"/>
    <skos:example>maple (wood) is derived from Acer (genus)</skos:example>
    <rdfs:isDefinedBy rdf:resource="http://vocab.getty.edu/aat/"/>
    <skos:prefLabel>aat2841_derived-made_from</skos:prefLabel>
  </rdf:Description>
  <rdf:Description rdf:about="http://vocab.getty.edu/ontology#aat2814_constituent_of">
    <rdfs:isDefinedBy rdf:resource="http://vocab.getty.edu/ontology"/>
    <dc:identifier>2814</dc:identifier>
    <skos:example>iron oxide is a constituent of desert varnish</skos:example>
    <skos:example>titanium white is a constituent of composite white</skos:example>
    <rdfs:subPropertyOf rdf:resource="http://www.w3.org/2004/02/skos/core#related"/>
    <owl:inverseOf rdf:resource="http://vocab.getty.edu/ontology#aat2815_composed_of"/>
    <rdf:type rdf:resource="http://www.w3.org/2002/07/owl#ObjectProperty"/>
    <rdfs:isDefinedBy rdf:resource="http://vocab.getty.edu/aat/"/>
    <skos:prefLabel>aat2814_constituent_of</skos:prefLabel>
    <dc:title>constituent of - material</dc:title>
    <rdfs:range rdf:resource="http://www.w3.org/2004/02/skos/core#Concept"/>
    <rdfs:domain rdf:resource="http://www.w3.org/2004/02/skos/core#Concept"/>
    <dct:description>material - [is] constituent of - material.&#13;
Example: titanium white is a constituent of composite white; iron oxide is a constituent of desert varnish</dct:description>
  </rdf:Description>
  <rdf:Description rdf:about="http://vocab.getty.edu/ontology#aat2807_derived_from_common_source">
    <skos:example>mustard(material) is derived from common source with mustard oil</skos:example>
    <dc:identifier>2807</dc:identifier>
    <rdfs:subPropertyOf rdf:resource="http://www.w3.org/2004/02/skos/core#related"/>
    <dct:description>material - [is] derived from common source [as] - material.&#13;
Example: malachite (mineral) is derived from common source with azurite (mineral); mustard(material) is derived from common source with mustard oil</dct:description>
    <rdfs:domain rdf:resource="http://www.w3.org/2004/02/skos/core#Concept"/>
    <rdf:type rdf:resource="http://www.w3.org/2002/07/owl#SymmetricProperty"/>
    <rdfs:isDefinedBy rdf:resource="http://vocab.getty.edu/ontology"/>
    <rdfs:range rdf:resource="http://www.w3.org/2004/02/skos/core#Concept"/>
    <skos:example>malachite (mineral) is derived from common source with azurite (mineral)</skos:example>
    <dc:title>derived from common source - material</dc:title>
    <rdf:type rdf:resource="http://www.w3.org/2002/07/owl#ObjectProperty"/>
    <rdfs:isDefinedBy rdf:resource="http://vocab.getty.edu/aat/"/>
    <skos:prefLabel>aat2807_derived_from_common_source</skos:prefLabel>
  </rdf:Description>
  <rdf:Description rdf:about="http://vocab.getty.edu/ontology#aat2316_use">
    <rdfs:subPropertyOf rdf:resource="http://www.w3.org/2004/02/skos/core#related"/>
    <dc:title>use - material</dc:title>
    <rdfs:range rdf:resource="http://www.w3.org/2004/02/skos/core#Concept"/>
    <skos:prefLabel>aat2316_use</skos:prefLabel>
    <skos:example>lapidaries use precious stone</skos:example>
    <rdfs:isDefinedBy rdf:resource="http://vocab.getty.edu/ontology"/>
    <rdfs:domain rdf:resource="http://www.w3.org/2004/02/skos/core#Concept"/>
    <skos:example>braziers (metalworkers) use brass (alloy)</skos:example>
    <dc:identifier>2316</dc:identifier>
    <dct:description>[actors having] role - use - material.&#13;
Example: lapidaries use precious stone; braziers (metalworkers) use brass (alloy)</dct:description>
    <rdf:type rdf:resource="http://www.w3.org/2002/07/owl#ObjectProperty"/>
    <rdfs:isDefinedBy rdf:resource="http://vocab.getty.edu/aat/"/>
  </rdf:Description>
  <rdf:Description rdf:about="http://vocab.getty.edu/ontology#broaderInstantial">
    <rdfs:range rdf:resource="http://vocab.getty.edu/ontology#Subject"/>
    <dct:description>BTI (Kind/Instance, "example of") relation. We also infer iso-thes:broaderInstantial, which goes only between Concepts.
Example: Rembrandt van Rijn BTI Persons/Artists (ULAN)</dct:description>
    <rdfs:domain rdf:resource="http://vocab.getty.edu/ontology#Subject"/>
    <rdfs:isDefinedBy rdf:resource="http://vocab.getty.edu/ontology"/>
    <skos:example>Rembrandt van Rijn BTI Persons/Artists (ULAN)</skos:example>
    <rdfs:subPropertyOf rdf:resource="http://vocab.getty.edu/ontology#broaderInstantialExtended"/>
    <rdfs:label>broaderInstantial</rdfs:label>
    <skos:prefLabel>broaderInstantial</skos:prefLabel>
    <rdf:type rdf:resource="http://www.w3.org/2002/07/owl#ObjectProperty"/>
    <rdfs:subPropertyOf rdf:resource="http://vocab.getty.edu/ontology#broader"/>
    <rdfs:comment>BTI (Kind/Instance, "example of") relation. We also infer iso-thes:broaderInstantial, which goes only between Concepts</rdfs:comment>
  </rdf:Description>
  <rdf:Description rdf:about="http://vocab.getty.edu/ontology#ulan1511_child_of">
    <skos:example>Rembrandt van Rijn is the child of Neeltgen Willemsdr van Zuydtbroeck</skos:example>
    <dc:title>child of - person</dc:title>
    <skos:prefLabel>ulan1511_child_of</skos:prefLabel>
    <owl:inverseOf rdf:resource="http://vocab.getty.edu/ontology#ulan1512_parent_of"/>
    <rdfs:range rdf:resource="http://www.w3.org/2004/02/skos/core#Concept"/>
    <dct:description>person - child of - person.&#13;
Example: Rembrandt van Rijn is the child of Neeltgen Willemsdr van Zuydtbroeck</dct:description>
    <rdfs:isDefinedBy rdf:resource="http://vocab.getty.edu/ontology"/>
    <rdfs:domain rdf:resource="http://www.w3.org/2004/02/skos/core#Concept"/>
    <rdfs:subPropertyOf rdf:resource="http://www.w3.org/2004/02/skos/core#related"/>
    <dc:identifier>1511</dc:identifier>
    <rdfs:isDefinedBy rdf:resource="http://vocab.getty.edu/ulan/"/>
    <rdf:type rdf:resource="http://www.w3.org/2002/07/owl#ObjectProperty"/>
  </rdf:Description>
  <rdf:Description rdf:about="http://vocab.getty.edu/ontology#ulan1515_great-grandparent_of">
    <rdf:type rdf:resource="http://www.w3.org/2002/07/owl#ObjectProperty"/>
    <dct:description>person - great-grandparent of - person.&#13;
Example: Albrecht Adam is the great-grandparent of Richard Benno Adam</dct:description>
    <rdfs:range rdf:resource="http://www.w3.org/2004/02/skos/core#Concept"/>
    <rdfs:domain rdf:resource="http://www.w3.org/2004/02/skos/core#Concept"/>
    <rdfs:isDefinedBy rdf:resource="http://vocab.getty.edu/ontology"/>
    <owl:inverseOf rdf:resource="http://vocab.getty.edu/ontology#ulan1516_great-grandchild_of"/>
    <rdfs:isDefinedBy rdf:resource="http://vocab.getty.edu/ulan/"/>
    <dc:identifier>1515</dc:identifier>
    <dc:title>great-grandparent of - person</dc:title>
    <skos:prefLabel>ulan1515_great-grandparent_of</skos:prefLabel>
    <rdfs:subPropertyOf rdf:resource="http://www.w3.org/2004/02/skos/core#related"/>
    <skos:example>Albrecht Adam is the great-grandparent of Richard Benno Adam</skos:example>
  </rdf:Description>
  <rdf:Description rdf:about="http://vocab.getty.edu/ontology#contributorAlternatePreferred">
    <rdfs:label>contributorAlternatePreferred</rdfs:label>
    <rdfs:subPropertyOf rdf:resource="http://purl.org/dc/terms/contributor"/>
    <rdf:type rdf:resource="http://www.w3.org/2002/07/owl#ObjectProperty"/>
    <skos:prefLabel>contributorAlternatePreferred</skos:prefLabel>
    <rdfs:range rdf:resource="http://xmlns.com/foaf/0.1/Agent"/>
    <rdfs:comment>Contributor for which the term is Alternate Preferred. Range is foaf:Agent</rdfs:comment>
    <dct:description>Contributor for which the term is Alternate Preferred. Range is foaf:Agent</dct:description>
    <rdfs:domain rdf:resource="http://www.w3.org/2008/05/skos-xl#Label"/>
    <rdfs:isDefinedBy rdf:resource="http://vocab.getty.edu/ontology"/>
  </rdf:Description>
  <rdf:Description rdf:about="http://vocab.getty.edu/tgn/">
    <rdfs:label>Thesaurus of Geographic Names</rdfs:label>
    <vann:preferredNamespacePrefix>tgn</vann:preferredNamespacePrefix>
    <rdf:type rdf:resource="http://www.w3.org/2004/02/skos/core#ConceptScheme"/>
    <dct:created rdf:datatype="http://www.w3.org/2001/XMLSchema#date">2014-06-15</dct:created>
    <rdfs:comment>The Thesaurus of Geographic Names concept scheme</rdfs:comment>
    <skos:prefLabel>Thesaurus of Geographic Names</skos:prefLabel>
    <rdfs:seeAlso rdf:resource="http://www.getty.edu/research/tools/vocabularies/lod/"/>
    <dct:creator rdf:resource="http://www.ontotext.com"/>
    <vann:preferredNamespaceUri>http://vocab.getty.edu/tgn/</vann:preferredNamespaceUri>
    <dct:creator rdf:resource="http://www.getty.edu/research/"/>
    <rdfs:seeAlso rdf:resource="http://vocab.getty.edu/.well-known/void"/>
    <rdfs:seeAlso rdf:resource="http://vocab.getty.edu/"/>
    <foaf:homepage rdf:resource="http://www.getty.edu/research/tools/vocabularies/tgn/"/>
  </rdf:Description>
  <rdf:Description rdf:about="http://vocab.getty.edu/ontology#ulan1562_step-parent_of">
    <rdfs:isDefinedBy rdf:resource="http://vocab.getty.edu/ulan/"/>
    <rdf:type rdf:resource="http://www.w3.org/2002/07/owl#ObjectProperty"/>
    <skos:example>Napoleon I, Emperor of the French is the step-parent of Hortense, Quene consort of Louis Bonaparte</skos:example>
    <rdfs:domain rdf:resource="http://www.w3.org/2004/02/skos/core#Concept"/>
    <rdfs:isDefinedBy rdf:resource="http://vocab.getty.edu/ontology"/>
    <dc:identifier>1562</dc:identifier>
    <rdfs:subPropertyOf rdf:resource="http://www.w3.org/2004/02/skos/core#related"/>
    <dct:description>person - step-parent of - person.&#13;
Example: Napoleon I, Emperor of the French is the step-parent of Hortense, Quene consort of Louis Bonaparte</dct:description>
    <skos:prefLabel>ulan1562_step-parent_of</skos:prefLabel>
    <dc:title>step-parent of - person</dc:title>
    <rdfs:range rdf:resource="http://www.w3.org/2004/02/skos/core#Concept"/>
  </rdf:Description>
  <rdf:Description rdf:about="http://vocab.getty.edu/ontology#aat2419_used_for">
    <rdfs:domain rdf:resource="http://www.w3.org/2004/02/skos/core#Concept"/>
    <skos:example>astronomical instruments are used for astronomy</skos:example>
    <rdf:type rdf:resource="http://www.w3.org/2002/07/owl#ObjectProperty"/>
    <rdfs:isDefinedBy rdf:resource="http://vocab.getty.edu/aat/"/>
    <skos:prefLabel>aat2419_used_for</skos:prefLabel>
    <rdfs:subPropertyOf rdf:resource="http://www.w3.org/2004/02/skos/core#related"/>
    <dc:title>used for - field/discipline</dc:title>
    <rdfs:range rdf:resource="http://www.w3.org/2004/02/skos/core#Concept"/>
    <dct:description>things/[equipment] - [are] used for - field [of study]/discipline.&#13;
Example: astronomical instruments are used for astronomy; divination objects are used for divination [discipline]</dct:description>
    <rdfs:isDefinedBy rdf:resource="http://vocab.getty.edu/ontology"/>
    <skos:example>divination objects are used for divination [discipline]</skos:example>
    <dc:identifier>2419</dc:identifier>
  </rdf:Description>
  <rdf:Description rdf:about="http://vocab.getty.edu/ontology#agentType">
    <rdfs:domain rdf:resource="http://vocab.getty.edu/ontology#Subject"/>
    <rdf:type rdf:resource="http://www.w3.org/2002/07/owl#ObjectProperty"/>
    <rdfs:comment>Type of a ULAN PersonConcept or GroupConcept. Domain is ULAN concept, range is AAT concept</rdfs:comment>
    <dct:description>Type of a ULAN PersonConcept or GroupConcept. Domain is ULAN concept, range is AAT concept</dct:description>
    <rdfs:isDefinedBy rdf:resource="http://vocab.getty.edu/ontology"/>
    <skos:prefLabel>agentType</skos:prefLabel>
    <rdfs:label>agentType</rdfs:label>
    <rdfs:range rdf:resource="http://vocab.getty.edu/ontology#Subject"/>
  </rdf:Description>
  <rdf:Description rdf:about="http://vocab.getty.edu/ontology#aat2821_based_on">
    <rdfs:range rdf:resource="http://www.w3.org/2004/02/skos/core#Concept"/>
    <dct:description>any - [is] based on - any.&#13;
Example: Neo-Gothic is based on Gothic (Medieval); curved [form attribute] is based on curves (geometric figures); pencils are based on plummets</dct:description>
    <rdfs:isDefinedBy rdf:resource="http://vocab.getty.edu/ontology"/>
    <rdfs:domain rdf:resource="http://www.w3.org/2004/02/skos/core#Concept"/>
    <dc:title>based on - any</dc:title>
    <rdfs:isDefinedBy rdf:resource="http://vocab.getty.edu/aat/"/>
    <dc:identifier>2821</dc:identifier>
    <rdfs:subPropertyOf rdf:resource="http://www.w3.org/2004/02/skos/core#related"/>
    <skos:example>pencils are based on plummets</skos:example>
    <skos:example>Neo-Gothic is based on Gothic (Medieval)</skos:example>
    <rdf:type rdf:resource="http://www.w3.org/2002/07/owl#ObjectProperty"/>
    <skos:example>curved [form attribute] is based on curves (geometric figures)</skos:example>
    <owl:inverseOf rdf:resource="http://vocab.getty.edu/ontology#aat2822_basis_of"/>
    <skos:prefLabel>aat2821_based_on</skos:prefLabel>
  </rdf:Description>
  <rdf:Description rdf:about="http://vocab.getty.edu/ontology#aat2315_used_by">
    <rdfs:range rdf:resource="http://www.w3.org/2004/02/skos/core#Concept"/>
    <rdfs:isDefinedBy rdf:resource="http://vocab.getty.edu/ontology"/>
    <skos:example>precious stone is used by lapidiaries</skos:example>
    <owl:inverseOf rdf:resource="http://vocab.getty.edu/ontology#aat2316_use"/>
    <rdfs:domain rdf:resource="http://www.w3.org/2004/02/skos/core#Concept"/>
    <rdfs:subPropertyOf rdf:resource="http://www.w3.org/2004/02/skos/core#related"/>
    <skos:example>brass (alloy) is used by braziers (metalworkers)</skos:example>
    <skos:prefLabel>aat2315_used_by</skos:prefLabel>
    <dc:title>used by - role</dc:title>
    <rdf:type rdf:resource="http://www.w3.org/2002/07/owl#ObjectProperty"/>
    <rdfs:isDefinedBy rdf:resource="http://vocab.getty.edu/aat/"/>
    <dc:identifier>2315</dc:identifier>
    <dct:description>material - [is] used by - [actor having] role.&#13;
Example: precious stone is used by lapidiaries; brass (alloy) is used by braziers (metalworkers)</dct:description>
  </rdf:Description>
  <rdf:Description rdf:about="http://vocab.getty.edu/ontology#ulan1313_partner_in">
    <rdfs:isDefinedBy rdf:resource="http://vocab.getty.edu/ontology"/>
    <rdfs:subPropertyOf rdf:resource="http://www.w3.org/2004/02/skos/core#related"/>
    <dc:identifier>1313</dc:identifier>
    <rdfs:domain rdf:resource="http://www.w3.org/2004/02/skos/core#Concept"/>
    <owl:inverseOf rdf:resource="http://vocab.getty.edu/ontology#ulan1314_partner_was"/>
    <skos:example>Parners of Adler and Sullivan included Louis H. Sullivan and Dankmar Adler</skos:example>
    <dc:title>partner in - firm</dc:title>
    <rdfs:range rdf:resource="http://www.w3.org/2004/02/skos/core#Concept"/>
    <skos:prefLabel>ulan1313_partner_in</skos:prefLabel>
    <dct:description>person - partner in - firm.&#13;
Example: Parners of Adler and Sullivan included Louis H. Sullivan and Dankmar Adler</dct:description>
    <rdf:type rdf:resource="http://www.w3.org/2002/07/owl#ObjectProperty"/>
    <rdfs:isDefinedBy rdf:resource="http://vocab.getty.edu/ulan/"/>
  </rdf:Description>
  <rdf:Description rdf:about="http://vocab.getty.edu/ontology#broaderNonPreferred">
    <skos:example>Non-preferred: "baking dishes" BTG "dishes (vessels)" (AAT)</skos:example>
    <dct:description>Auxiliary parents of a subject. Very often there are several non-preferred parents (poly-hierarchy). Can use to mark such parents with [N] in displays .
Example: Non-preferred: "baking dishes" BTG "dishes (vessels)" (AAT)</dct:description>
    <rdfs:range rdf:resource="http://vocab.getty.edu/ontology#Subject"/>
    <rdf:type rdf:resource="http://www.w3.org/2002/07/owl#ObjectProperty"/>
    <rdfs:subPropertyOf rdf:resource="http://vocab.getty.edu/ontology#broader"/>
    <skos:prefLabel>broaderNonPreferred</skos:prefLabel>
    <rdfs:label>broaderNonPreferred</rdfs:label>
    <rdfs:comment>Auxiliary parents of a subject. Very often there are several non-preferred parents (poly-hierarchy). Can use to mark such parents with [N] in displays </rdfs:comment>
    <rdfs:domain rdf:resource="http://vocab.getty.edu/ontology#Subject"/>
    <rdfs:isDefinedBy rdf:resource="http://vocab.getty.edu/ontology"/>
  </rdf:Description>
  <rdf:Description rdf:about="http://vocab.getty.edu/ontology#aat2335_associated_with">
    <dc:identifier>2335</dc:identifier>
    <rdfs:range rdf:resource="http://www.w3.org/2004/02/skos/core#Concept"/>
    <skos:prefLabel>aat2335_associated_with</skos:prefLabel>
    <rdf:type rdf:resource="http://www.w3.org/2002/07/owl#ObjectProperty"/>
    <rdfs:isDefinedBy rdf:resource="http://vocab.getty.edu/aat/"/>
    <rdfs:isDefinedBy rdf:resource="http://vocab.getty.edu/ontology"/>
    <rdfs:domain rdf:resource="http://www.w3.org/2004/02/skos/core#Concept"/>
    <rdfs:subPropertyOf rdf:resource="http://www.w3.org/2004/02/skos/core#related"/>
    <skos:example>popes are associated with Roman Catholicism</skos:example>
    <skos:example>abstract artists are associated with Abstract (fine arts style)</skos:example>
    <dct:description>[actors having] role - [are] associated with - style/period/culture/[religion/ideology].&#13;
Example: abstract artists are associated with Abstract (fine arts style); popes are associated with Roman Catholicism</dct:description>
    <dc:title>associated with - style/period/culture</dc:title>
    <owl:inverseOf rdf:resource="http://vocab.getty.edu/ontology#aat2336_has_associates"/>
  </rdf:Description>
  <rdf:Description rdf:about="http://vocab.getty.edu/ontology#aat2218_used-function_as">
    <skos:prefLabel>aat2218_used-function_as</skos:prefLabel>
    <rdfs:domain rdf:resource="http://www.w3.org/2004/02/skos/core#Concept"/>
    <rdfs:subPropertyOf rdf:resource="http://www.w3.org/2004/02/skos/core#related"/>
    <rdfs:isDefinedBy rdf:resource="http://vocab.getty.edu/ontology"/>
    <dc:identifier>2218</dc:identifier>
    <owl:inverseOf rdf:resource="http://vocab.getty.edu/ontology#aat2219_have_form"/>
    <rdfs:isDefinedBy rdf:resource="http://vocab.getty.edu/aat/"/>
    <rdf:type rdf:resource="http://www.w3.org/2002/07/owl#ObjectProperty"/>
    <rdfs:range rdf:resource="http://www.w3.org/2004/02/skos/core#Concept"/>
    <skos:example>arc lamps are used/function as lighthouse lamps</skos:example>
    <dct:description>things - [are] used/function as - things.&#13;
Example: arc lamps are used/function as lighthouse lamps;  toile peinte is used/function as cartoons (working drawings)</dct:description>
    <skos:example>toile peinte is used/function as cartoons (working drawings)</skos:example>
    <dc:title>used/function as - things</dc:title>
  </rdf:Description>
  <rdf:Description rdf:about="http://vocab.getty.edu/ontology#ulan2778_owner_of">
    <dc:title>owner of - person</dc:title>
    <dc:identifier>2778</dc:identifier>
    <rdfs:range rdf:resource="http://www.w3.org/2004/02/skos/core#Concept"/>
    <rdf:type rdf:resource="http://www.w3.org/2002/07/owl#ObjectProperty"/>
    <owl:inverseOf rdf:resource="http://vocab.getty.edu/ontology#ulan2779_owned_by"/>
    <rdfs:isDefinedBy rdf:resource="http://vocab.getty.edu/ulan/"/>
    <dct:description>firm - owner of - person.&#13;
Example: Walter Scott Lenox was the owner of Lenox China Co.</dct:description>
    <rdfs:subPropertyOf rdf:resource="http://www.w3.org/2004/02/skos/core#related"/>
    <rdfs:domain rdf:resource="http://www.w3.org/2004/02/skos/core#Concept"/>
    <rdfs:isDefinedBy rdf:resource="http://vocab.getty.edu/ontology"/>
    <skos:example>Walter Scott Lenox was the owner of Lenox China Co.</skos:example>
    <skos:prefLabel>ulan2778_owner_of</skos:prefLabel>
  </rdf:Description>
  <rdf:Description rdf:about="http://vocab.getty.edu/ontology#aat2501_made_of-require">
    <rdfs:range rdf:resource="http://www.w3.org/2004/02/skos/core#Concept"/>
    <skos:example>ivories (sculptures) are made of/require ivory</skos:example>
    <owl:inverseOf rdf:resource="http://vocab.getty.edu/ontology#aat2502_material_for"/>
    <rdf:type rdf:resource="http://www.w3.org/2002/07/owl#ObjectProperty"/>
    <rdfs:isDefinedBy rdf:resource="http://vocab.getty.edu/aat/"/>
    <dct:description>things - [are] made of/require - material.&#13;
Example: obsidian mirrors are made of/require obsidian; ivories (sculptures) are made of/require ivory</dct:description>
    <rdfs:subPropertyOf rdf:resource="http://www.w3.org/2004/02/skos/core#related"/>
    <skos:prefLabel>aat2501_made_of-require</skos:prefLabel>
    <skos:example>obsidian mirrors are made of/require obsidian</skos:example>
    <rdfs:domain rdf:resource="http://www.w3.org/2004/02/skos/core#Concept"/>
    <dc:identifier>2501</dc:identifier>
    <dc:title>made of/require - material</dc:title>
    <rdfs:isDefinedBy rdf:resource="http://vocab.getty.edu/ontology"/>
  </rdf:Description>
  <rdf:Description rdf:about="http://vocab.getty.edu/term/kind/ISOnumeric2">
    <skos:inScheme rdf:resource="http://vocab.getty.edu/term/kind/"/>
    <rdf:type rdf:resource="http://www.w3.org/2004/02/skos/core#Concept"/>
    <skos:scopeNote>May be used in TGN, but no code of this kind is present</skos:scopeNote>
    <skos:prefLabel>ISO numeric-2 code</skos:prefLabel>
    <dct:description>May be used in TGN, but no code of this kind is present</dct:description>
    <skos:notation>ISO2N</skos:notation>
  </rdf:Description>
  <rdf:Description rdf:about="http://vocab.getty.edu/ontology#ulan1309_advisor_of">
    <rdf:type rdf:resource="http://www.w3.org/2002/07/owl#ObjectProperty"/>
    <dc:identifier>1309</dc:identifier>
    <dc:title>advisor of - person</dc:title>
    <skos:prefLabel>ulan1309_advisor_of</skos:prefLabel>
    <owl:inverseOf rdf:resource="http://vocab.getty.edu/ontology#ulan1310_advised_by"/>
    <dct:description>person - advisor of - person.&#13;
Example: Thomas Cromwell, Earl of Essex was the advisor of Henry VIII, King of England</dct:description>
    <rdfs:isDefinedBy rdf:resource="http://vocab.getty.edu/ontology"/>
    <rdfs:domain rdf:resource="http://www.w3.org/2004/02/skos/core#Concept"/>
    <skos:example>Thomas Cromwell, Earl of Essex was the advisor of Henry VIII, King of England</skos:example>
    <rdfs:isDefinedBy rdf:resource="http://vocab.getty.edu/ulan/"/>
    <rdfs:subPropertyOf rdf:resource="http://www.w3.org/2004/02/skos/core#related"/>
    <rdfs:range rdf:resource="http://www.w3.org/2004/02/skos/core#Concept"/>
  </rdf:Description>
  <rdf:Description rdf:about="http://vocab.getty.edu/ontology#ulan1543_consort_was">
    <skos:prefLabel>ulan1543_consort_was</skos:prefLabel>
    <dc:identifier>1543</dc:identifier>
    <rdfs:isDefinedBy rdf:resource="http://vocab.getty.edu/ulan/"/>
    <rdfs:domain rdf:resource="http://www.w3.org/2004/02/skos/core#Concept"/>
    <rdfs:range rdf:resource="http://www.w3.org/2004/02/skos/core#Concept"/>
    <rdfs:isDefinedBy rdf:resource="http://vocab.getty.edu/ontology"/>
    <dct:description>person - consort was - person.&#13;
Example: Augustus, Emperor of Rome's consort was Empress Livia</dct:description>
    <dc:title>consort was - person</dc:title>
    <skos:example>Augustus, Emperor of Rome's consort was Empress Livia</skos:example>
    <rdf:type rdf:resource="http://www.w3.org/2002/07/owl#ObjectProperty"/>
    <rdfs:subPropertyOf rdf:resource="http://www.w3.org/2004/02/skos/core#related"/>
  </rdf:Description>
  <rdf:Description rdf:about="http://vocab.getty.edu/ontology#aat2551_reflect-produced_by">
    <dc:title>reflect/produced by - style/period/culture</dc:title>
    <rdfs:subPropertyOf rdf:resource="http://www.w3.org/2004/02/skos/core#related"/>
    <skos:example>Nasca lines reflect/are produced by Nasca [culture]</skos:example>
    <skos:prefLabel>aat2551_reflect-produced_by</skos:prefLabel>
    <rdfs:isDefinedBy rdf:resource="http://vocab.getty.edu/ontology"/>
    <rdf:type rdf:resource="http://www.w3.org/2002/07/owl#ObjectProperty"/>
    <owl:inverseOf rdf:resource="http://vocab.getty.edu/ontology#aat2552_reflected_in-produces"/>
    <rdfs:domain rdf:resource="http://www.w3.org/2004/02/skos/core#Concept"/>
    <dc:identifier>2551</dc:identifier>
    <skos:example>Judaica reflects/is produced by Judaism</skos:example>
    <dct:description>things - reflect/[are] produced by - style/period/culture/[religion/ideology].&#13;
Example: Nasca lines reflect/are produced by Nasca [culture]; Judaica reflects/is produced by Judaism</dct:description>
    <rdfs:range rdf:resource="http://www.w3.org/2004/02/skos/core#Concept"/>
    <rdfs:isDefinedBy rdf:resource="http://vocab.getty.edu/aat/"/>
  </rdf:Description>
  <rdf:Description rdf:about="http://vocab.getty.edu/ontology#ulan1422_founded">
    <rdfs:range rdf:resource="http://www.w3.org/2004/02/skos/core#Concept"/>
    <rdf:type rdf:resource="http://www.w3.org/2002/07/owl#ObjectProperty"/>
    <rdfs:isDefinedBy rdf:resource="http://vocab.getty.edu/ulan/"/>
    <skos:example>The United States Congress founded the National Gallery of Art</skos:example>
    <dc:title>founded - firm/group</dc:title>
    <dc:identifier>1422</dc:identifier>
    <rdfs:isDefinedBy rdf:resource="http://vocab.getty.edu/ontology"/>
    <rdfs:subPropertyOf rdf:resource="http://www.w3.org/2004/02/skos/core#related"/>
    <rdfs:domain rdf:resource="http://www.w3.org/2004/02/skos/core#Concept"/>
    <skos:prefLabel>ulan1422_founded</skos:prefLabel>
    <dct:description>firm/group - founded - firm/group.&#13;
Example: The United States Congress founded the National Gallery of Art</dct:description>
  </rdf:Description>
  <rdf:Description rdf:about="http://vocab.getty.edu/ontology#ulan1205_client_of">
    <dc:title>client of - person/firm/family</dc:title>
    <rdfs:domain rdf:resource="http://www.w3.org/2004/02/skos/core#Concept"/>
    <owl:inverseOf rdf:resource="http://vocab.getty.edu/ontology#ulan1206_client_was"/>
    <rdfs:isDefinedBy rdf:resource="http://vocab.getty.edu/ulan/"/>
    <skos:example>The Chicago Herald was the client of Burnham and Root</skos:example>
    <dct:description>person/firm/family - client of - person/firm/family.&#13;
Example: The Chicago Herald was the client of Burnham and Root</dct:description>
    <rdf:type rdf:resource="http://www.w3.org/2002/07/owl#ObjectProperty"/>
    <rdfs:subPropertyOf rdf:resource="http://www.w3.org/2004/02/skos/core#related"/>
    <skos:prefLabel>ulan1205_client_of</skos:prefLabel>
    <rdfs:range rdf:resource="http://www.w3.org/2004/02/skos/core#Concept"/>
    <dc:identifier>1205</dc:identifier>
    <rdfs:isDefinedBy rdf:resource="http://vocab.getty.edu/ontology"/>
  </rdf:Description>
  <rdf:Description rdf:about="http://vocab.getty.edu/ontology#aat2613_possess-exist_in">
    <skos:prefLabel>aat2613_possess-exist_in</skos:prefLabel>
    <rdfs:isDefinedBy rdf:resource="http://vocab.getty.edu/aat/"/>
    <skos:example>dielectric (material) possesses/exists in dielectric properties</skos:example>
    <dct:description>material - possesses/exists in - condition/state/[property].&#13;
Example: wood(plant material) possesses/exists in [condition of] dry rot; dielectric (material) possesses/exists in dielectric properties</dct:description>
    <rdfs:range rdf:resource="http://www.w3.org/2004/02/skos/core#Concept"/>
    <skos:example>wood(plant material) possesses/exists in [condition of] dry rot</skos:example>
    <rdfs:isDefinedBy rdf:resource="http://vocab.getty.edu/ontology"/>
    <rdfs:domain rdf:resource="http://www.w3.org/2004/02/skos/core#Concept"/>
    <dc:title>possess/exist in - attributes /associated concepts</dc:title>
    <rdfs:subPropertyOf rdf:resource="http://www.w3.org/2004/02/skos/core#related"/>
    <dc:identifier>2613</dc:identifier>
    <rdf:type rdf:resource="http://www.w3.org/2002/07/owl#ObjectProperty"/>
  </rdf:Description>
  <rdf:Description rdf:about="http://vocab.getty.edu/ontology#aat2562_locus-setting_for">
    <skos:example>agraharas are the locus/setting for Brahmanism</skos:example>
    <owl:inverseOf rdf:resource="http://vocab.getty.edu/ontology#aat2563_located_in"/>
    <dc:identifier>2562</dc:identifier>
    <rdfs:subPropertyOf rdf:resource="http://www.w3.org/2004/02/skos/core#related"/>
    <dct:description>locus/setting - [is] locus/setting for - style/period/culture/[religion/ideology].&#13;
Example: First Nations reserves are the locus/setting for First Nations (culture); agraharas are the locus/setting for Brahmanism</dct:description>
    <dc:title>locus/setting for - style/period/culture</dc:title>
    <rdf:type rdf:resource="http://www.w3.org/2002/07/owl#ObjectProperty"/>
    <skos:prefLabel>aat2562_locus-setting_for</skos:prefLabel>
    <skos:example>First Nations reserves are the locus/setting for First Nations (culture)</skos:example>
    <rdfs:isDefinedBy rdf:resource="http://vocab.getty.edu/aat/"/>
    <rdfs:range rdf:resource="http://www.w3.org/2004/02/skos/core#Concept"/>
    <rdfs:domain rdf:resource="http://www.w3.org/2004/02/skos/core#Concept"/>
    <rdfs:isDefinedBy rdf:resource="http://vocab.getty.edu/ontology"/>
  </rdf:Description>
  <rdf:Description rdf:about="http://vocab.getty.edu/term/POS/PastParticiple">
    <rdf:type rdf:resource="http://www.w3.org/2004/02/skos/core#Concept"/>
    <skos:prefLabel>Past Participle</skos:prefLabel>
    <dct:description>Rarely used but if at all, is most likely to apply in Attributes and Properties.
Example: hand-painted</dct:description>
    <skos:example>hand-painted</skos:example>
    <skos:scopeNote>Rarely used but if at all, is most likely to apply in Attributes and Properties</skos:scopeNote>
    <skos:notation>PP</skos:notation>
    <skos:inScheme rdf:resource="http://vocab.getty.edu/term/POS/"/>
  </rdf:Description>
  <rdf:Description rdf:about="http://vocab.getty.edu/ontology#aat2845_used-located_in">
    <dc:identifier>2845</dc:identifier>
    <owl:inverseOf rdf:resource="http://vocab.getty.edu/ontology#aat2846_locus-setting_for"/>
    <rdfs:subPropertyOf rdf:resource="http://www.w3.org/2004/02/skos/core#related"/>
    <dc:title>used/located in - locus/setting</dc:title>
    <rdfs:isDefinedBy rdf:resource="http://vocab.getty.edu/ontology"/>
    <skos:prefLabel>aat2845_used-located_in</skos:prefLabel>
    <rdfs:domain rdf:resource="http://www.w3.org/2004/02/skos/core#Concept"/>
    <dct:description>genus/species - [is] used/located in -  locus/setting.&#13;
Example: Elephantidae(family) are used/located in elephant houses; Vitaceae (family) is used/located in vineyards</dct:description>
    <skos:example>Vitaceae (family) is used/located in vineyards</skos:example>
    <skos:example>Elephantidae(family) are used/located in elephant houses</skos:example>
    <rdf:type rdf:resource="http://www.w3.org/2002/07/owl#ObjectProperty"/>
    <rdfs:range rdf:resource="http://www.w3.org/2004/02/skos/core#Concept"/>
    <rdfs:isDefinedBy rdf:resource="http://vocab.getty.edu/aat/"/>
  </rdf:Description>
  <rdf:Description rdf:about="http://vocab.getty.edu/ontology#sourcePreferred">
    <skos:example>"Isfahan" is preferred in Webster's New Geographical Dictionary (1988)</skos:example>
    <rdfs:comment>Source for which the term is Preferred. Range is bibo:Document or bibo:DocumentPart</rdfs:comment>
    <rdfs:isDefinedBy rdf:resource="http://vocab.getty.edu/ontology"/>
    <dct:description>Source for which the term is Preferred. Range is bibo:Document or bibo:DocumentPart.
Example: "Isfahan" is preferred in Webster's New Geographical Dictionary (1988)</dct:description>
    <rdfs:label>sourcePreferred</rdfs:label>
    <skos:prefLabel>sourcePreferred</skos:prefLabel>
    <rdfs:range rdf:resource="http://purl.org/ontology/bibo/Document"/>
    <rdf:type rdf:resource="http://www.w3.org/2002/07/owl#ObjectProperty"/>
    <rdfs:domain rdf:resource="http://www.w3.org/2008/05/skos-xl#Label"/>
    <rdfs:subPropertyOf rdf:resource="http://purl.org/dc/terms/source"/>
  </rdf:Description>
  <rdf:Description rdf:about="http://vocab.getty.edu/ontology#ulan1573_ward_of">
    <skos:prefLabel>ulan1573_ward_of</skos:prefLabel>
    <rdfs:subPropertyOf rdf:resource="http://www.w3.org/2004/02/skos/core#related"/>
    <rdfs:isDefinedBy rdf:resource="http://vocab.getty.edu/ulan/"/>
    <dct:description>person - ward of - person.&#13;
Example: Samuel Cooper was a ward of John Hoskins, the elder</dct:description>
    <dc:identifier>1573</dc:identifier>
    <skos:example>Samuel Cooper was a ward of John Hoskins, the elder</skos:example>
    <rdfs:isDefinedBy rdf:resource="http://vocab.getty.edu/ontology"/>
    <rdfs:domain rdf:resource="http://www.w3.org/2004/02/skos/core#Concept"/>
    <rdf:type rdf:resource="http://www.w3.org/2002/07/owl#ObjectProperty"/>
    <rdfs:range rdf:resource="http://www.w3.org/2004/02/skos/core#Concept"/>
    <dc:title>ward of - person</dc:title>
  </rdf:Description>
  <rdf:Description rdf:about="http://vocab.getty.edu/ontology#tgn3318_member_is">
    <rdfs:range rdf:resource="http://www.w3.org/2004/02/skos/core#Concept"/>
    <skos:example>Austria is a member of the European Union since 1915</skos:example>
    <rdf:type rdf:resource="http://www.w3.org/2002/07/owl#ObjectProperty"/>
    <skos:prefLabel>tgn3318_member_is</skos:prefLabel>
    <rdfs:isDefinedBy rdf:resource="http://vocab.getty.edu/tgn/"/>
    <dc:title>member is - nation</dc:title>
    <dct:description>union - member is - nation.&#13;
Example: Austria is a member of the European Union since 1915; Belgium is a member of the European Union since 1958</dct:description>
    <rdfs:subPropertyOf rdf:resource="http://www.w3.org/2004/02/skos/core#related"/>
    <dc:identifier>3318</dc:identifier>
    <rdfs:domain rdf:resource="http://www.w3.org/2004/02/skos/core#Concept"/>
    <skos:example>Belgium is a member of the European Union since 1958</skos:example>
    <rdfs:isDefinedBy rdf:resource="http://vocab.getty.edu/ontology"/>
  </rdf:Description>
  <rdf:Description rdf:about="http://vocab.getty.edu/ontology#aat2421_locus-setting_for">
    <skos:example>smelters (metalworking plants) are the locus/setting for smelting</skos:example>
    <rdfs:domain rdf:resource="http://www.w3.org/2004/02/skos/core#Concept"/>
    <rdfs:isDefinedBy rdf:resource="http://vocab.getty.edu/ontology"/>
    <owl:inverseOf rdf:resource="http://vocab.getty.edu/ontology#aat2422_takes_place_in"/>
    <dc:title>locus/setting for - activity/event</dc:title>
    <skos:example>pilgrimage centers are the locus/setting for pilgrimages</skos:example>
    <rdfs:range rdf:resource="http://www.w3.org/2004/02/skos/core#Concept"/>
    <skos:prefLabel>aat2421_locus-setting_for</skos:prefLabel>
    <rdfs:isDefinedBy rdf:resource="http://vocab.getty.edu/aat/"/>
    <dct:description>locus/setting - [is] locus/setting for - activity/event/[process/function].&#13;
Example: smelters (metalworking plants) are the locus/setting for smelting; pilgrimage centers are the locus/setting for pilgrimages</dct:description>
    <dc:identifier>2421</dc:identifier>
    <rdfs:subPropertyOf rdf:resource="http://www.w3.org/2004/02/skos/core#related"/>
    <rdf:type rdf:resource="http://www.w3.org/2002/07/owl#ObjectProperty"/>
  </rdf:Description>
  <rdf:Description rdf:about="http://vocab.getty.edu/ontology#ulan1411_successor_of">
    <rdfs:domain rdf:resource="http://www.w3.org/2004/02/skos/core#Concept"/>
    <rdfs:subPropertyOf rdf:resource="http://www.w3.org/2004/02/skos/core#related"/>
    <rdfs:isDefinedBy rdf:resource="http://vocab.getty.edu/ontology"/>
    <skos:prefLabel>ulan1411_successor_of</skos:prefLabel>
    <dc:title>successor of - firm/group</dc:title>
    <dc:identifier>1411</dc:identifier>
    <rdfs:isDefinedBy rdf:resource="http://vocab.getty.edu/ulan/"/>
    <rdf:type rdf:resource="http://www.w3.org/2002/07/owl#ObjectProperty"/>
    <dct:description>firm/group - successor of - firm/group.&#13;
Example: Richard Meier &amp; Partners Architects LLP is the successor of Richard Meier &amp; Associates</dct:description>
    <rdfs:range rdf:resource="http://www.w3.org/2004/02/skos/core#Concept"/>
    <owl:inverseOf rdf:resource="http://vocab.getty.edu/ontology#ulan1412_predecessor_of"/>
    <skos:example>Richard Meier &amp; Partners Architects LLP is the successor of Richard Meier &amp; Associates</skos:example>
  </rdf:Description>
  <rdf:Description rdf:about="http://vocab.getty.edu/term/kind/CommonName">
    <skos:inScheme rdf:resource="http://vocab.getty.edu/term/kind/"/>
    <skos:prefLabel>Common Name</skos:prefLabel>
    <skos:example>TODO</skos:example>
    <dct:description>Common Name of an ULAN agent.
Example: TODO</dct:description>
    <skos:notation>CN</skos:notation>
    <skos:scopeNote>Common Name of an ULAN agent</skos:scopeNote>
    <rdf:type rdf:resource="http://www.w3.org/2004/02/skos/core#Concept"/>
  </rdf:Description>
  <rdf:Description rdf:about="http://vocab.getty.edu/ontology#aat2397_focus_of">
    <dc:identifier>2397</dc:identifier>
    <rdfs:isDefinedBy rdf:resource="http://vocab.getty.edu/ontology"/>
    <owl:inverseOf rdf:resource="http://vocab.getty.edu/ontology#aat2398_focuses_on"/>
    <dct:description>any - [is] focus of - field [of study]/discipline.&#13;
Example: manuscripts are the focus of codicology; music is the focus of musicology; Plantae (kingdom) is the focus of botany</dct:description>
    <rdfs:isDefinedBy rdf:resource="http://vocab.getty.edu/aat/"/>
    <rdfs:domain rdf:resource="http://www.w3.org/2004/02/skos/core#Concept"/>
    <rdfs:range rdf:resource="http://www.w3.org/2004/02/skos/core#Concept"/>
    <skos:example>manuscripts are the focus of codicology</skos:example>
    <skos:example>Plantae (kingdom) is the focus of botany</skos:example>
    <rdf:type rdf:resource="http://www.w3.org/2002/07/owl#ObjectProperty"/>
    <skos:example>music is the focus of musicology</skos:example>
    <skos:prefLabel>aat2397_focus_of</skos:prefLabel>
    <rdfs:subPropertyOf rdf:resource="http://www.w3.org/2004/02/skos/core#related"/>
    <dc:title>focus of - field/discipline</dc:title>
  </rdf:Description>
  <rdf:Description rdf:about="http://vocab.getty.edu/ontology#aat2422_takes_place_in">
    <skos:example>pilgrimages take place in pilgrimage centers</skos:example>
    <rdfs:range rdf:resource="http://www.w3.org/2004/02/skos/core#Concept"/>
    <skos:example>smelting takes place in smelters (metalworking plants)</skos:example>
    <rdf:type rdf:resource="http://www.w3.org/2002/07/owl#ObjectProperty"/>
    <dct:description>activity/event/[process/function] - takes place in - locus/setting.&#13;
Example: smelting takes place in smelters (metalworking plants); pilgrimages take place in pilgrimage centers</dct:description>
    <skos:prefLabel>aat2422_takes_place_in</skos:prefLabel>
    <dc:identifier>2422</dc:identifier>
    <rdfs:isDefinedBy rdf:resource="http://vocab.getty.edu/aat/"/>
    <rdfs:domain rdf:resource="http://www.w3.org/2004/02/skos/core#Concept"/>
    <rdfs:subPropertyOf rdf:resource="http://www.w3.org/2004/02/skos/core#related"/>
    <rdfs:isDefinedBy rdf:resource="http://vocab.getty.edu/ontology"/>
    <dc:title>takes place in - locus/setting</dc:title>
  </rdf:Description>
  <rdf:Description rdf:about="http://vocab.getty.edu/ontology#aat2434_contextualized_in">
    <rdf:type rdf:resource="http://www.w3.org/2002/07/owl#ObjectProperty"/>
    <dc:identifier>2434</dc:identifier>
    <rdfs:isDefinedBy rdf:resource="http://vocab.getty.edu/aat/"/>
    <rdfs:range rdf:resource="http://www.w3.org/2004/02/skos/core#Concept"/>
    <rdfs:domain rdf:resource="http://www.w3.org/2004/02/skos/core#Concept"/>
    <rdfs:isDefinedBy rdf:resource="http://vocab.getty.edu/ontology"/>
    <skos:example>funeral books are contextualized in funerals</skos:example>
    <dct:description>things - [are] context for - activity/event/process.&#13;
Example: funeral books are contextualized in funerals; Christmas trees are contextualized in Christmas</dct:description>
    <owl:inverseOf rdf:resource="http://vocab.getty.edu/ontology#aat2435_context_for"/>
    <skos:example>Christmas trees are contextualized in Christmas</skos:example>
    <dc:title>contextualized in - activity/event/process</dc:title>
    <skos:prefLabel>aat2434_contextualized_in</skos:prefLabel>
    <rdfs:subPropertyOf rdf:resource="http://www.w3.org/2004/02/skos/core#related"/>
  </rdf:Description>
  <rdf:Description rdf:about="http://vocab.getty.edu/ontology#ulan1414_joint_venture_with">
    <dc:title>joint venture with - firm/group</dc:title>
    <rdfs:range rdf:resource="http://www.w3.org/2004/02/skos/core#Concept"/>
    <skos:example>Schwetye Luchini Architects is in a joint venture with ACME Architects</skos:example>
    <rdf:type rdf:resource="http://www.w3.org/2002/07/owl#ObjectProperty"/>
    <rdfs:isDefinedBy rdf:resource="http://vocab.getty.edu/ulan/"/>
    <dct:description>firm/group - joint venture with - firm/group.&#13;
Example: Schwetye Luchini Architects is in a joint venture with ACME Architects</dct:description>
    <dc:identifier>1414</dc:identifier>
    <rdfs:domain rdf:resource="http://www.w3.org/2004/02/skos/core#Concept"/>
    <rdfs:subPropertyOf rdf:resource="http://www.w3.org/2004/02/skos/core#related"/>
    <rdfs:isDefinedBy rdf:resource="http://vocab.getty.edu/ontology"/>
    <rdf:type rdf:resource="http://www.w3.org/2002/07/owl#SymmetricProperty"/>
    <skos:prefLabel>ulan1414_joint_venture_with</skos:prefLabel>
  </rdf:Description>
  <rdf:Description rdf:about="http://vocab.getty.edu/ontology#ulan1308_assisted_by">
    <skos:example>Pablo Picasso was assisted by Bernard Castelli</skos:example>
    <dc:title>assisted by - person</dc:title>
    <rdfs:range rdf:resource="http://www.w3.org/2004/02/skos/core#Concept"/>
    <dc:identifier>1308</dc:identifier>
    <rdfs:isDefinedBy rdf:resource="http://vocab.getty.edu/ontology"/>
    <rdfs:domain rdf:resource="http://www.w3.org/2004/02/skos/core#Concept"/>
    <dct:description>person - assisted by - person.&#13;
Example: Pablo Picasso was assisted by Bernard Castelli</dct:description>
    <rdfs:isDefinedBy rdf:resource="http://vocab.getty.edu/ulan/"/>
    <skos:prefLabel>ulan1308_assisted_by</skos:prefLabel>
    <rdf:type rdf:resource="http://www.w3.org/2002/07/owl#ObjectProperty"/>
    <rdfs:subPropertyOf rdf:resource="http://www.w3.org/2004/02/skos/core#related"/>
  </rdf:Description>
  <rdf:Description rdf:about="http://vocab.getty.edu/ontology#ulan1212_artist_was">
    <dct:description>person - artist was - person.&#13;
Example: Charles-Pierre Coustou was artist to Louis XIV, King of France</dct:description>
    <rdfs:isDefinedBy rdf:resource="http://vocab.getty.edu/ontology"/>
    <rdfs:subPropertyOf rdf:resource="http://www.w3.org/2004/02/skos/core#related"/>
    <dc:title>artist was - person</dc:title>
    <rdfs:domain rdf:resource="http://www.w3.org/2004/02/skos/core#Concept"/>
    <skos:prefLabel>ulan1212_artist_was</skos:prefLabel>
    <rdfs:range rdf:resource="http://www.w3.org/2004/02/skos/core#Concept"/>
    <skos:example>Charles-Pierre Coustou was artist to Louis XIV, King of France</skos:example>
    <dc:identifier>1212</dc:identifier>
    <rdf:type rdf:resource="http://www.w3.org/2002/07/owl#ObjectProperty"/>
    <rdfs:isDefinedBy rdf:resource="http://vocab.getty.edu/ulan/"/>
  </rdf:Description>
  <rdf:Description rdf:about="http://vocab.getty.edu/ontology#ulan1322_school_was">
    <rdfs:isDefinedBy rdf:resource="http://vocab.getty.edu/ulan/"/>
    <dc:identifier>1322</dc:identifier>
    <rdfs:subPropertyOf rdf:resource="http://www.w3.org/2004/02/skos/core#related"/>
    <dct:description>firm/group - school was - person.&#13;
Example: Pierre Saalburg attended Architectural Association. School of Architecture</dct:description>
    <rdfs:domain rdf:resource="http://www.w3.org/2004/02/skos/core#Concept"/>
    <rdfs:isDefinedBy rdf:resource="http://vocab.getty.edu/ontology"/>
    <rdfs:range rdf:resource="http://www.w3.org/2004/02/skos/core#Concept"/>
    <dc:title>school was - person</dc:title>
    <skos:prefLabel>ulan1322_school_was</skos:prefLabel>
    <rdf:type rdf:resource="http://www.w3.org/2002/07/owl#ObjectProperty"/>
    <skos:example>Pierre Saalburg attended Architectural Association. School of Architecture</skos:example>
  </rdf:Description>
  <rdf:Description rdf:about="http://vocab.getty.edu/ontology#termDisplay">
    <rdfs:isDefinedBy rdf:resource="http://vocab.getty.edu/ontology"/>
    <rdfs:label>termDisplay</rdfs:label>
    <rdf:type rdf:resource="http://www.w3.org/2002/07/owl#ObjectProperty"/>
    <dct:description>Term Display</dct:description>
    <rdfs:domain rdf:resource="http://www.w3.org/2008/05/skos-xl#Label"/>
    <skos:prefLabel>termDisplay</skos:prefLabel>
    <rdfs:range rdf:resource="http://www.w3.org/2004/02/skos/core#Concept"/>
  </rdf:Description>
  <rdf:Description rdf:about="http://vocab.getty.edu/ontology#tgn3000_related_to">
    <rdf:type rdf:resource="http://www.w3.org/2002/07/owl#ObjectProperty"/>
    <rdfs:isDefinedBy rdf:resource="http://vocab.getty.edu/tgn/"/>
    <dc:identifier>3000</dc:identifier>
    <skos:example>Austria-Hungary is related to Magyarorszag</skos:example>
    <rdfs:subPropertyOf rdf:resource="http://www.w3.org/2004/02/skos/core#related"/>
    <dc:title>related to - any</dc:title>
    <rdf:type rdf:resource="http://www.w3.org/2002/07/owl#SymmetricProperty"/>
    <rdfs:domain rdf:resource="http://www.w3.org/2004/02/skos/core#Concept"/>
    <rdfs:isDefinedBy rdf:resource="http://vocab.getty.edu/ontology"/>
    <skos:example>Fountains Abbey is related to Studley Royal</skos:example>
    <rdfs:range rdf:resource="http://www.w3.org/2004/02/skos/core#Concept"/>
    <skos:prefLabel>tgn3000_related_to</skos:prefLabel>
    <dct:description>any - related to - any.&#13;
Example: Fountains Abbey is related to Studley Royal; Austria-Hungary is related to Magyarorszag</dct:description>
  </rdf:Description>
  <rdf:Description rdf:about="http://vocab.getty.edu/ontology#GroupConcept">
    <rdfs:comment>Two or more people who generally worked together to collectively create art. Not necessarily legally incorporated. A family of artists may be considered a "corporate body". Corresponds to crm:E74_Group, not its subclass crm:E40_Legal_Body</rdfs:comment>
    <rdf:type rdf:resource="http://www.w3.org/2002/07/owl#Class"/>
    <rdfs:subClassOf rdf:resource="http://vocab.getty.edu/ontology#Subject"/>
    <dct:description>Two or more people who generally worked together to collectively create art. Not necessarily legally incorporated. A family of artists may be considered a "corporate body". Corresponds to crm:E74_Group, not its subclass crm:E40_Legal_Body.
Example: 500356337 Albrecht Duerer Workshop (ULAN)</dct:description>
    <skos:prefLabel>GroupConcept</skos:prefLabel>
    <rdfs:isDefinedBy rdf:resource="http://vocab.getty.edu/ontology"/>
    <skos:example>500356337 Albrecht Duerer Workshop (ULAN)</skos:example>
    <rdfs:subClassOf rdf:resource="http://www.w3.org/2004/02/skos/core#Concept"/>
    <rdfs:label>GroupConcept</rdfs:label>
  </rdf:Description>
  <rdf:Description rdf:about="http://vocab.getty.edu/term/kind/ISOalpha2">
    <skos:prefLabel>ISO alpha-2 code</skos:prefLabel>
    <rdf:type rdf:resource="http://www.w3.org/2004/02/skos/core#Concept"/>
    <skos:notation>ISO2L</skos:notation>
    <dct:description>ISO 3166-1 alpha-2 country code. Used in TGN.
Example: "AQ" for Antarctica</dct:description>
    <skos:scopeNote>ISO 3166-1 alpha-2 country code. Used in TGN</skos:scopeNote>
    <skos:example>"AQ" for Antarctica</skos:example>
    <skos:inScheme rdf:resource="http://vocab.getty.edu/term/kind/"/>
  </rdf:Description>
  <rdf:Description rdf:about="http://vocab.getty.edu/ontology#aat2849_involves">
    <rdfs:isDefinedBy rdf:resource="http://vocab.getty.edu/aat/"/>
    <rdfs:domain rdf:resource="http://www.w3.org/2004/02/skos/core#Concept"/>
    <rdfs:subPropertyOf rdf:resource="http://www.w3.org/2004/02/skos/core#related"/>
    <rdfs:isDefinedBy rdf:resource="http://vocab.getty.edu/ontology"/>
    <skos:example>polo (field sport) involves Equus caballus (species)</skos:example>
    <dc:title>involves - genus/species</dc:title>
    <dct:description>activity/event - involves - genus/species.&#13;
Example: bullfighting involves bulls (animals); polo (field sport) involves Equus caballus (species)</dct:description>
    <rdfs:range rdf:resource="http://www.w3.org/2004/02/skos/core#Concept"/>
    <skos:prefLabel>aat2849_involves</skos:prefLabel>
    <skos:example>bullfighting involves bulls (animals)</skos:example>
    <dc:identifier>2849</dc:identifier>
    <rdf:type rdf:resource="http://www.w3.org/2002/07/owl#ObjectProperty"/>
  </rdf:Description>
  <rdf:Description rdf:about="http://vocab.getty.edu/term/kind/Abbreviation">
    <skos:inScheme rdf:resource="http://vocab.getty.edu/term/kind/"/>
    <dct:description>Term is an abbreviation, initialism, or acronym.
Example: "FLIM" is abbrevaition for "fluorescence lifetime imaging microscopy"</dct:description>
    <skos:notation>A</skos:notation>
    <skos:prefLabel>Abbreviation</skos:prefLabel>
    <skos:scopeNote>Term is an abbreviation, initialism, or acronym</skos:scopeNote>
    <skos:example>"FLIM" is abbrevaition for "fluorescence lifetime imaging microscopy"</skos:example>
    <rdf:type rdf:resource="http://www.w3.org/2004/02/skos/core#Concept"/>
  </rdf:Description>
  <rdf:Description rdf:about="http://vocab.getty.edu/ontology#Subject">
    <rdfs:isDefinedBy rdf:resource="http://vocab.getty.edu/ontology"/>
    <dct:description>Node in a GVP vocabulary hierarchy. 
May be Facet, GuideTerm, Hierarchy, Concept, AdminPlaceConcept, PhysPlaceConcept, PhysAdminPlaceConcept, or ObsoleteSubject.
Implemented as skos:Concept or iso:ThesaurusArray and skos:Collection</dct:description>
    <rdfs:comment>Node in a GVP vocabulary hierarchy. 
May be Facet, GuideTerm, Hierarchy, Concept, AdminPlaceConcept, PhysPlaceConcept, PhysAdminPlaceConcept, or ObsoleteSubject.
Implemented as skos:Concept or iso:ThesaurusArray and skos:Collection</rdfs:comment>
    <rdf:type rdf:resource="http://www.w3.org/2002/07/owl#Class"/>
    <skos:prefLabel>Subject</skos:prefLabel>
    <rdfs:label>Subject</rdfs:label>
  </rdf:Description>
  <rdf:Description rdf:about="http://vocab.getty.edu/ontology#tgn3201_capital_of">
    <rdfs:isDefinedBy rdf:resource="http://vocab.getty.edu/ontology"/>
    <rdfs:domain rdf:resource="http://www.w3.org/2004/02/skos/core#Concept"/>
    <rdfs:isDefinedBy rdf:resource="http://vocab.getty.edu/tgn/"/>
    <skos:example>Thecapital of Maxima Caesariensis from 296 to 800 CE was London</skos:example>
    <skos:prefLabel>tgn3201_capital_of</skos:prefLabel>
    <rdfs:subPropertyOf rdf:resource="http://www.w3.org/2004/02/skos/core#related"/>
    <owl:inverseOf rdf:resource="http://vocab.getty.edu/ontology#tgn3202_capital_is"/>
    <rdf:type rdf:resource="http://www.w3.org/2002/07/owl#ObjectProperty"/>
    <dc:identifier>3201</dc:identifier>
    <dct:description>city - capital of - nation.&#13;
Example: Thecapital of Maxima Caesariensis from 296 to 800 CE was London</dct:description>
    <dc:title>capital of - nation</dc:title>
    <rdfs:range rdf:resource="http://www.w3.org/2004/02/skos/core#Concept"/>
  </rdf:Description>
  <rdf:Description rdf:about="http://vocab.getty.edu/ontology#aat2215_required_for">
    <dct:description>things - [are] required for -  things.&#13;
Example: eyelets are required for broderie anglaise; compact discs are required for compact disc players</dct:description>
    <skos:example>compact discs are required for compact disc players</skos:example>
    <skos:example>eyelets are required for broderie anglaise</skos:example>
    <rdfs:domain rdf:resource="http://www.w3.org/2004/02/skos/core#Concept"/>
    <rdfs:range rdf:resource="http://www.w3.org/2004/02/skos/core#Concept"/>
    <rdfs:isDefinedBy rdf:resource="http://vocab.getty.edu/ontology"/>
    <dc:identifier>2215</dc:identifier>
    <rdfs:subPropertyOf rdf:resource="http://www.w3.org/2004/02/skos/core#related"/>
    <rdfs:isDefinedBy rdf:resource="http://vocab.getty.edu/aat/"/>
    <skos:prefLabel>aat2215_required_for</skos:prefLabel>
    <rdf:type rdf:resource="http://www.w3.org/2002/07/owl#ObjectProperty"/>
    <owl:inverseOf rdf:resource="http://vocab.getty.edu/ontology#aat2216_require"/>
    <dc:title>required for - things</dc:title>
  </rdf:Description>
  <rdf:Description rdf:about="http://vocab.getty.edu/ontology#aat2604_possessed_by-existing_in">
    <rdfs:isDefinedBy rdf:resource="http://vocab.getty.edu/ontology"/>
    <rdfs:subPropertyOf rdf:resource="http://www.w3.org/2004/02/skos/core#related"/>
    <skos:prefLabel>aat2604_possessed_by-existing_in</skos:prefLabel>
    <rdfs:domain rdf:resource="http://www.w3.org/2004/02/skos/core#Concept"/>
    <rdfs:range rdf:resource="http://www.w3.org/2004/02/skos/core#Concept"/>
    <skos:example>boudoir (photograph size) is possessed by/existing in boudoir photographs</skos:example>
    <dc:identifier>2604</dc:identifier>
    <owl:inverseOf rdf:resource="http://vocab.getty.edu/ontology#aat2605_possess-exist_in"/>
    <dct:description>attributes /associated concepts - [is] possessed by/existing in - things.&#13;
Example: boudoir (photograph size) is possessed by/existing in boudoir photographs; ruined [condition] is possessed by/existing in ruins</dct:description>
    <rdf:type rdf:resource="http://www.w3.org/2002/07/owl#ObjectProperty"/>
    <skos:example>ruined [condition] is possessed by/existing in ruins</skos:example>
    <dc:title>possessed by/existing in - things</dc:title>
    <rdfs:isDefinedBy rdf:resource="http://vocab.getty.edu/aat/"/>
  </rdf:Description>
  <rdf:Description rdf:about="http://vocab.getty.edu/ontology#ulan1222_appointee_of">
    <rdfs:subPropertyOf rdf:resource="http://www.w3.org/2004/02/skos/core#related"/>
    <rdfs:isDefinedBy rdf:resource="http://vocab.getty.edu/ontology"/>
    <skos:prefLabel>ulan1222_appointee_of</skos:prefLabel>
    <rdfs:isDefinedBy rdf:resource="http://vocab.getty.edu/ulan/"/>
    <skos:example>Virginio Cesarini was appointee by Pope Urban VIII</skos:example>
    <dct:description>person - appointee of - person.&#13;
Example: Virginio Cesarini was appointee by Pope Urban VIII</dct:description>
    <rdf:type rdf:resource="http://www.w3.org/2002/07/owl#ObjectProperty"/>
    <dc:title>appointee of - person</dc:title>
    <rdfs:range rdf:resource="http://www.w3.org/2004/02/skos/core#Concept"/>
    <rdfs:domain rdf:resource="http://www.w3.org/2004/02/skos/core#Concept"/>
    <dc:identifier>1222</dc:identifier>
  </rdf:Description>
  <rdf:Description rdf:about="http://vocab.getty.edu/ontology#aat2505_locus-setting_for">
    <dc:title>locus/setting for - material</dc:title>
    <rdfs:isDefinedBy rdf:resource="http://vocab.getty.edu/ontology"/>
    <rdfs:subPropertyOf rdf:resource="http://www.w3.org/2004/02/skos/core#related"/>
    <skos:prefLabel>aat2505_locus-setting_for</skos:prefLabel>
    <rdfs:domain rdf:resource="http://www.w3.org/2004/02/skos/core#Concept"/>
    <rdfs:range rdf:resource="http://www.w3.org/2004/02/skos/core#Concept"/>
    <dct:description>locus/setting - [is] locus/setting for - material.&#13;
Example: volcanoes are locus/setting for  tephra; brickworks (factories) are locus/setting for brick (clay product)</dct:description>
    <skos:example>volcanoes are locus/setting for  tephra</skos:example>
    <rdf:type rdf:resource="http://www.w3.org/2002/07/owl#ObjectProperty"/>
    <skos:example>brickworks (factories) are locus/setting for brick (clay product)</skos:example>
    <dc:identifier>2505</dc:identifier>
    <rdfs:isDefinedBy rdf:resource="http://vocab.getty.edu/aat/"/>
  </rdf:Description>
  <rdf:Description rdf:about="http://vocab.getty.edu/ontology#ulan1107_influenced">
    <rdf:type rdf:resource="http://www.w3.org/2002/07/owl#ObjectProperty"/>
    <owl:inverseOf rdf:resource="http://vocab.getty.edu/ontology#ulan1108_influenced_by"/>
    <rdfs:isDefinedBy rdf:resource="http://vocab.getty.edu/ulan/"/>
    <dct:description>person - influenced - person.&#13;
Example: Rembrandt van Rijn influenced Salomon Koninck</dct:description>
    <rdfs:subPropertyOf rdf:resource="http://www.w3.org/2004/02/skos/core#related"/>
    <rdfs:isDefinedBy rdf:resource="http://vocab.getty.edu/ontology"/>
    <rdfs:domain rdf:resource="http://www.w3.org/2004/02/skos/core#Concept"/>
    <dc:identifier>1107</dc:identifier>
    <dc:title>influenced - person</dc:title>
    <rdfs:range rdf:resource="http://www.w3.org/2004/02/skos/core#Concept"/>
    <skos:example>Rembrandt van Rijn influenced Salomon Koninck</skos:example>
    <skos:prefLabel>ulan1107_influenced</skos:prefLabel>
  </rdf:Description>
  <rdf:Description rdf:about="http://vocab.getty.edu/ontology#aat2833_ancestor_of">
    <skos:example>Canis lupus is the ancestor of Canis familiaris</skos:example>
    <dc:title>ancestor of - genus/species</dc:title>
    <rdfs:isDefinedBy rdf:resource="http://vocab.getty.edu/ontology"/>
    <dc:identifier>2833</dc:identifier>
    <rdfs:subPropertyOf rdf:resource="http://www.w3.org/2004/02/skos/core#related"/>
    <rdfs:domain rdf:resource="http://www.w3.org/2004/02/skos/core#Concept"/>
    <rdf:type rdf:resource="http://www.w3.org/2002/07/owl#ObjectProperty"/>
    <rdfs:isDefinedBy rdf:resource="http://vocab.getty.edu/aat/"/>
    <rdfs:range rdf:resource="http://www.w3.org/2004/02/skos/core#Concept"/>
    <dct:description>genus/species - is ancestor of -  another genus/species.&#13;
Example: Canis lupus is the ancestor of Canis familiaris; Equus asinus is the ancestor of donkeys</dct:description>
    <skos:example>Equus asinus is the ancestor of donkeys</skos:example>
    <owl:inverseOf rdf:resource="http://vocab.getty.edu/ontology#aat2834_decendant_of"/>
    <skos:prefLabel>aat2833_ancestor_of</skos:prefLabel>
  </rdf:Description>
  <rdf:Description rdf:about="http://vocab.getty.edu/ontology#ulan2651_publisher_of">
    <rdf:type rdf:resource="http://www.w3.org/2002/07/owl#ObjectProperty"/>
    <dc:identifier>2651</dc:identifier>
    <dct:description>firm - publisher of - person.&#13;
Example: Negretti and Zambra was the publisher of Pierre Joseph Rossier</dct:description>
    <skos:example>Negretti and Zambra was the publisher of Pierre Joseph Rossier</skos:example>
    <rdfs:range rdf:resource="http://www.w3.org/2004/02/skos/core#Concept"/>
    <rdfs:domain rdf:resource="http://www.w3.org/2004/02/skos/core#Concept"/>
    <skos:prefLabel>ulan2651_publisher_of</skos:prefLabel>
    <rdfs:subPropertyOf rdf:resource="http://www.w3.org/2004/02/skos/core#related"/>
    <rdfs:isDefinedBy rdf:resource="http://vocab.getty.edu/ontology"/>
    <dc:title>publisher of - person</dc:title>
    <rdfs:isDefinedBy rdf:resource="http://vocab.getty.edu/ulan/"/>
  </rdf:Description>
  <rdf:Description rdf:about="http://vocab.getty.edu/ontology#aat2887_exemplified_by">
    <rdfs:subPropertyOf rdf:resource="http://www.w3.org/2004/02/skos/core#related"/>
    <skos:example>solvent - exemplified by - carbon disulfide</skos:example>
    <rdfs:domain rdf:resource="http://www.w3.org/2004/02/skos/core#Concept"/>
    <dc:identifier>2887</dc:identifier>
    <rdfs:isDefinedBy rdf:resource="http://vocab.getty.edu/ontology"/>
    <skos:prefLabel>aat2887_exemplified_by</skos:prefLabel>
    <dc:title>exemplified by - material</dc:title>
    <rdfs:range rdf:resource="http://www.w3.org/2004/02/skos/core#Concept"/>
    <dct:description>material - exemplified by - material.&#13;
Example: solvent - exemplified by - carbon disulfide</dct:description>
    <rdf:type rdf:resource="http://www.w3.org/2002/07/owl#ObjectProperty"/>
    <rdfs:isDefinedBy rdf:resource="http://vocab.getty.edu/aat/"/>
  </rdf:Description>
  <rdf:Description rdf:about="http://vocab.getty.edu/ontology#aat2325_created_by">
    <rdfs:isDefinedBy rdf:resource="http://vocab.getty.edu/aat/"/>
    <rdf:type rdf:resource="http://www.w3.org/2002/07/owl#ObjectProperty"/>
    <skos:prefLabel>aat2325_created_by</skos:prefLabel>
    <dc:identifier>2325</dc:identifier>
    <rdfs:range rdf:resource="http://www.w3.org/2004/02/skos/core#Concept"/>
    <dct:description>things - [are] created by - [actors having] role.&#13;
Example: drawings are created by draftsmen; poems are created by poets</dct:description>
    <rdfs:domain rdf:resource="http://www.w3.org/2004/02/skos/core#Concept"/>
    <skos:example>drawings are created by draftsmen</skos:example>
    <skos:example>poems are created by poets</skos:example>
    <rdfs:subPropertyOf rdf:resource="http://www.w3.org/2004/02/skos/core#related"/>
    <dc:title>created by - role</dc:title>
    <rdfs:isDefinedBy rdf:resource="http://vocab.getty.edu/ontology"/>
    <owl:inverseOf rdf:resource="http://vocab.getty.edu/ontology#aat2326_create"/>
  </rdf:Description>
  <rdf:Description rdf:about="http://vocab.getty.edu/ontology#ulan2582_administered_by">
    <dct:description>institution - administered by - person.&#13;
Example: Societe nationale des chemins de fer Francais. Agence des gares was administered by Georges Mathieu</dct:description>
    <rdfs:isDefinedBy rdf:resource="http://vocab.getty.edu/ulan/"/>
    <rdfs:isDefinedBy rdf:resource="http://vocab.getty.edu/ontology"/>
    <rdfs:subPropertyOf rdf:resource="http://www.w3.org/2004/02/skos/core#related"/>
    <rdf:type rdf:resource="http://www.w3.org/2002/07/owl#ObjectProperty"/>
    <dc:identifier>2582</dc:identifier>
    <rdfs:range rdf:resource="http://www.w3.org/2004/02/skos/core#Concept"/>
    <dc:title>administered by - person</dc:title>
    <skos:prefLabel>ulan2582_administered_by</skos:prefLabel>
    <skos:example>Societe nationale des chemins de fer Francais. Agence des gares was administered by Georges Mathieu</skos:example>
    <rdfs:domain rdf:resource="http://www.w3.org/2004/02/skos/core#Concept"/>
  </rdf:Description>
  <rdf:Description rdf:about="http://vocab.getty.edu/ontology#ulan2696_leader_of">
    <skos:prefLabel>ulan2696_leader_of</skos:prefLabel>
    <owl:inverseOf rdf:resource="http://vocab.getty.edu/ontology#ulan2697_leader_was"/>
    <rdfs:subPropertyOf rdf:resource="http://www.w3.org/2004/02/skos/core#related"/>
    <rdfs:isDefinedBy rdf:resource="http://vocab.getty.edu/ontology"/>
    <dct:description>person - leader of - institution.&#13;
Example: Rush Harrison Kress was the leader of Samuel H. Kress Foundation</dct:description>
    <rdfs:isDefinedBy rdf:resource="http://vocab.getty.edu/ulan/"/>
    <skos:example>Rush Harrison Kress was the leader of Samuel H. Kress Foundation</skos:example>
    <rdf:type rdf:resource="http://www.w3.org/2002/07/owl#ObjectProperty"/>
    <dc:identifier>2696</dc:identifier>
    <rdfs:range rdf:resource="http://www.w3.org/2004/02/skos/core#Concept"/>
    <rdfs:domain rdf:resource="http://www.w3.org/2004/02/skos/core#Concept"/>
    <dc:title>leader of - institution</dc:title>
  </rdf:Description>
  <rdf:Description rdf:about="http://vocab.getty.edu/ontology#ulan1111_master_of">
    <rdfs:range rdf:resource="http://www.w3.org/2004/02/skos/core#Concept"/>
    <rdf:type rdf:resource="http://www.w3.org/2002/07/owl#ObjectProperty"/>
    <skos:prefLabel>ulan1111_master_of</skos:prefLabel>
    <rdfs:isDefinedBy rdf:resource="http://vocab.getty.edu/ulan/"/>
    <dc:identifier>1111</dc:identifier>
    <owl:inverseOf rdf:resource="http://vocab.getty.edu/ontology#ulan1112_master_was"/>
    <skos:example>Peter Paul Rubens - master of Jan Thomas</skos:example>
    <rdfs:isDefinedBy rdf:resource="http://vocab.getty.edu/ontology"/>
    <rdfs:subPropertyOf rdf:resource="http://www.w3.org/2004/02/skos/core#related"/>
    <rdfs:domain rdf:resource="http://www.w3.org/2004/02/skos/core#Concept"/>
    <dct:description>person - master of - person.&#13;
Example: Peter Paul Rubens - master of Jan Thomas</dct:description>
    <dc:title>master of - person</dc:title>
  </rdf:Description>
  <rdf:Description rdf:about="http://vocab.getty.edu/term/kind/ISOalpha3">
    <skos:prefLabel>ISO alpha-3 code</skos:prefLabel>
    <skos:example>"ATA" for Antarctica</skos:example>
    <rdf:type rdf:resource="http://www.w3.org/2004/02/skos/core#Concept"/>
    <dct:description>ISO 3166-1 alpha-3 country code. Used in TGN.
Example: "ATA" for Antarctica</dct:description>
    <skos:notation>ISO3L</skos:notation>
    <skos:inScheme rdf:resource="http://vocab.getty.edu/term/kind/"/>
    <skos:scopeNote>ISO 3166-1 alpha-3 country code. Used in TGN</skos:scopeNote>
  </rdf:Description>
  <rdf:Description rdf:about="http://vocab.getty.edu/ontology#ulan1105_apprentice_of">
    <rdfs:isDefinedBy rdf:resource="http://vocab.getty.edu/ontology"/>
    <skos:example>Nicolas Hawksmoor was the apprentice of Christopher Wren</skos:example>
    <rdfs:domain rdf:resource="http://www.w3.org/2004/02/skos/core#Concept"/>
    <owl:inverseOf rdf:resource="http://vocab.getty.edu/ontology#ulan1106_apprentice_was"/>
    <rdfs:range rdf:resource="http://www.w3.org/2004/02/skos/core#Concept"/>
    <skos:prefLabel>ulan1105_apprentice_of</skos:prefLabel>
    <dct:description>person - apprentice of - person.&#13;
Example: Nicolas Hawksmoor was the apprentice of Christopher Wren</dct:description>
    <dc:title>apprentice of - person</dc:title>
    <rdf:type rdf:resource="http://www.w3.org/2002/07/owl#ObjectProperty"/>
    <dc:identifier>1105</dc:identifier>
    <rdfs:isDefinedBy rdf:resource="http://vocab.getty.edu/ulan/"/>
    <rdfs:subPropertyOf rdf:resource="http://www.w3.org/2004/02/skos/core#related"/>
  </rdf:Description>
  <rdf:Description rdf:about="http://vocab.getty.edu/ontology#aat2208_locus-setting_for">
    <owl:inverseOf rdf:resource="http://vocab.getty.edu/ontology#aat2209_used-located_in"/>
    <dct:description>locus/setting - [is] locus/setting for - things.&#13;
Example: glassworks (buildings) are the locus/setting for glassware; caves are the locus/setting for cave paintings</dct:description>
    <dc:title>locus/setting for - things</dc:title>
    <rdfs:subPropertyOf rdf:resource="http://www.w3.org/2004/02/skos/core#related"/>
    <dc:identifier>2208</dc:identifier>
    <rdf:type rdf:resource="http://www.w3.org/2002/07/owl#ObjectProperty"/>
    <skos:prefLabel>aat2208_locus-setting_for</skos:prefLabel>
    <skos:example>glassworks (buildings) are the locus/setting for glassware</skos:example>
    <rdfs:isDefinedBy rdf:resource="http://vocab.getty.edu/aat/"/>
    <rdfs:range rdf:resource="http://www.w3.org/2004/02/skos/core#Concept"/>
    <rdfs:isDefinedBy rdf:resource="http://vocab.getty.edu/ontology"/>
    <skos:example>caves are the locus/setting for cave paintings</skos:example>
    <rdfs:domain rdf:resource="http://www.w3.org/2004/02/skos/core#Concept"/>
  </rdf:Description>
  <rdf:Description rdf:about="http://vocab.getty.edu/ontology#ulan1412_predecessor_of">
    <rdfs:domain rdf:resource="http://www.w3.org/2004/02/skos/core#Concept"/>
    <rdfs:range rdf:resource="http://www.w3.org/2004/02/skos/core#Concept"/>
    <dct:description>firm/group - predecessor of - firm/group.&#13;
Example: Richard Meier &amp; Associates is the predecessor of Richard Meier &amp; Partners Architects LLP</dct:description>
    <rdfs:isDefinedBy rdf:resource="http://vocab.getty.edu/ontology"/>
    <dc:title>predecessor of - firm/group</dc:title>
    <dc:identifier>1412</dc:identifier>
    <skos:prefLabel>ulan1412_predecessor_of</skos:prefLabel>
    <rdfs:subPropertyOf rdf:resource="http://www.w3.org/2004/02/skos/core#related"/>
    <skos:example>Richard Meier &amp; Associates is the predecessor of Richard Meier &amp; Partners Architects LLP</skos:example>
    <rdfs:isDefinedBy rdf:resource="http://vocab.getty.edu/ulan/"/>
    <rdf:type rdf:resource="http://www.w3.org/2002/07/owl#ObjectProperty"/>
  </rdf:Description>
  <rdf:Description rdf:about="http://vocab.getty.edu/ontology#ulan1211_artist_to">
    <rdfs:range rdf:resource="http://www.w3.org/2004/02/skos/core#Concept"/>
    <dc:identifier>1211</dc:identifier>
    <skos:prefLabel>ulan1211_artist_to</skos:prefLabel>
    <dc:title>artist to - person</dc:title>
    <rdf:type rdf:resource="http://www.w3.org/2002/07/owl#ObjectProperty"/>
    <owl:inverseOf rdf:resource="http://vocab.getty.edu/ontology#ulan1212_artist_was"/>
    <rdfs:isDefinedBy rdf:resource="http://vocab.getty.edu/ulan/"/>
    <rdfs:isDefinedBy rdf:resource="http://vocab.getty.edu/ontology"/>
    <rdfs:subPropertyOf rdf:resource="http://www.w3.org/2004/02/skos/core#related"/>
    <rdfs:domain rdf:resource="http://www.w3.org/2004/02/skos/core#Concept"/>
    <dct:description>person - artist to - person.&#13;
Example: Artist to Louis XIV, King of France was Charles-Pierre Coustou</dct:description>
    <skos:example>Artist to Louis XIV, King of France was Charles-Pierre Coustou</skos:example>
  </rdf:Description>
  <rdf:Description rdf:about="http://vocab.getty.edu/ontology#tgn3104_is_location_of">
    <skos:prefLabel>tgn3104_is_location_of</skos:prefLabel>
    <dc:title>is location of - place</dc:title>
    <rdfs:subPropertyOf rdf:resource="http://www.w3.org/2004/02/skos/core#related"/>
    <skos:example>tgn:7031416 Silk Road is location of tgn:7018835 Palmyra</skos:example>
    <rdfs:domain rdf:resource="http://www.w3.org/2004/02/skos/core#Concept"/>
    <rdfs:isDefinedBy rdf:resource="http://vocab.getty.edu/ontology"/>
    <dc:identifier>3104</dc:identifier>
    <rdfs:range rdf:resource="http://www.w3.org/2004/02/skos/core#Concept"/>
    <rdf:type rdf:resource="http://www.w3.org/2002/07/owl#ObjectProperty"/>
    <dct:description>place - is location of - place.&#13;
Example: tgn:7031416 Silk Road is location of tgn:7018835 Palmyra</dct:description>
    <rdfs:isDefinedBy rdf:resource="http://vocab.getty.edu/tgn/"/>
  </rdf:Description>
  <rdf:Description rdf:about="http://vocab.getty.edu/ontology#ulan1305_worked_with">
    <rdf:type rdf:resource="http://www.w3.org/2002/07/owl#ObjectProperty"/>
    <dc:title>worked with - person</dc:title>
    <skos:prefLabel>ulan1305_worked_with</skos:prefLabel>
    <rdfs:isDefinedBy rdf:resource="http://vocab.getty.edu/ulan/"/>
    <rdfs:domain rdf:resource="http://www.w3.org/2004/02/skos/core#Concept"/>
    <skos:example>William Cleare worked with Christopher Wren</skos:example>
    <rdf:type rdf:resource="http://www.w3.org/2002/07/owl#SymmetricProperty"/>
    <rdfs:isDefinedBy rdf:resource="http://vocab.getty.edu/ontology"/>
    <rdfs:subPropertyOf rdf:resource="http://www.w3.org/2004/02/skos/core#related"/>
    <dct:description>person - worked with - person.&#13;
Example: William Cleare worked with Christopher Wren; Frank Lloyd Wright work with Aaron G. Green</dct:description>
    <dc:identifier>1305</dc:identifier>
    <skos:example>Frank Lloyd Wright work with Aaron G. Green</skos:example>
    <rdfs:range rdf:resource="http://www.w3.org/2004/02/skos/core#Concept"/>
  </rdf:Description>
  <rdf:Description rdf:about="http://vocab.getty.edu/ontology#broaderInstantialExtended">
    <rdf:type rdf:resource="http://www.w3.org/2002/07/owl#ObjectProperty"/>
    <dct:description>Ancestors (Instantial). Meaningful closure of gvp:broaderInstantial. Infers iso:broaderInstantial for pairs of directly related skos:Concepts.</dct:description>
    <rdfs:range rdf:resource="http://vocab.getty.edu/ontology#Subject"/>
    <rdfs:label>broaderInstantialExtended</rdfs:label>
    <skos:prefLabel>broaderInstantialExtended</skos:prefLabel>
    <rdfs:domain rdf:resource="http://vocab.getty.edu/ontology#Subject"/>
    <rdfs:isDefinedBy rdf:resource="http://vocab.getty.edu/ontology"/>
    <skos:example>Mt Athos (TGN) BTI orthodox religious center (AAT) BTG Christian religious center (AAT),
so Mt Athos (TGN) BTIE Christian religious center (AAT)</skos:example>
    <owl:propertyChainAxiom rdf:nodeID="Nb537c13fdf6e4e4ebc7554cfedb20057"/>
    <rdfs:subPropertyOf rdf:resource="http://vocab.getty.edu/ontology#broaderExtended"/>
  </rdf:Description>
  <rdf:Description rdf:about="http://vocab.getty.edu/ontology#ulan2829_student_was">
    <skos:prefLabel>ulan2829_student_was</skos:prefLabel>
    <rdf:type rdf:resource="http://www.w3.org/2002/07/owl#ObjectProperty"/>
    <dc:identifier>2829</dc:identifier>
    <rdfs:isDefinedBy rdf:resource="http://vocab.getty.edu/ulan/"/>
    <skos:example>Bauhaus student was Zdanek Rossman</skos:example>
    <dc:title>student was - person</dc:title>
    <rdfs:isDefinedBy rdf:resource="http://vocab.getty.edu/ontology"/>
    <rdfs:subPropertyOf rdf:resource="http://www.w3.org/2004/02/skos/core#related"/>
    <dct:description>institution - student was - person.&#13;
Example: Bauhaus student was Zdanek Rossman</dct:description>
    <rdfs:domain rdf:resource="http://www.w3.org/2004/02/skos/core#Concept"/>
    <rdfs:range rdf:resource="http://www.w3.org/2004/02/skos/core#Concept"/>
  </rdf:Description>
  <rdf:Description rdf:about="http://vocab.getty.edu/ontology#aat2612_possessed_by-existing_in">
    <dc:title>possessed by/existing in - material</dc:title>
    <rdf:type rdf:resource="http://www.w3.org/2002/07/owl#ObjectProperty"/>
    <skos:prefLabel>aat2612_possessed_by-existing_in</skos:prefLabel>
    <dc:identifier>2612</dc:identifier>
    <rdfs:subPropertyOf rdf:resource="http://www.w3.org/2004/02/skos/core#related"/>
    <owl:inverseOf rdf:resource="http://vocab.getty.edu/ontology#aat2613_possess-exist_in"/>
    <rdfs:domain rdf:resource="http://www.w3.org/2004/02/skos/core#Concept"/>
    <rdfs:isDefinedBy rdf:resource="http://vocab.getty.edu/ontology"/>
    <skos:example>dielectric properties are possessed by/existing in dielectric (material)</skos:example>
    <skos:example>dry rot is possessed by/existing in wood(plant material)</skos:example>
    <rdfs:isDefinedBy rdf:resource="http://vocab.getty.edu/aat/"/>
    <rdfs:range rdf:resource="http://www.w3.org/2004/02/skos/core#Concept"/>
    <dct:description>attributes /associated concepts - is possessed by/existing in - material.&#13;
Example: dry rot is possessed by/existing in wood(plant material); dielectric properties are possessed by/existing in dielectric (material)</dct:description>
  </rdf:Description>
  <rdf:Description rdf:about="http://vocab.getty.edu/term/kind/JargonOrSlang">
    <skos:inScheme rdf:resource="http://vocab.getty.edu/term/kind/"/>
    <skos:example>"fool's gold" is slang for "pyrite"</skos:example>
    <dct:description>Slang or jargon term. Used in AAT only.
Example: "fool's gold" is slang for "pyrite"</dct:description>
    <skos:scopeNote>Slang or jargon term. Used in AAT only</skos:scopeNote>
    <skos:prefLabel>Jargon or Slang</skos:prefLabel>
    <skos:notation>J</skos:notation>
    <rdf:type rdf:resource="http://www.w3.org/2004/02/skos/core#Concept"/>
  </rdf:Description>
  <rdf:Description rdf:about="http://vocab.getty.edu/ontology#ulan2779_owned_by">
    <skos:example>Walter Scott Lenox was owned by Lenox China Co.</skos:example>
    <dc:title>owned by - firm</dc:title>
    <rdfs:isDefinedBy rdf:resource="http://vocab.getty.edu/ontology"/>
    <rdfs:subPropertyOf rdf:resource="http://www.w3.org/2004/02/skos/core#related"/>
    <rdfs:domain rdf:resource="http://www.w3.org/2004/02/skos/core#Concept"/>
    <rdfs:range rdf:resource="http://www.w3.org/2004/02/skos/core#Concept"/>
    <skos:prefLabel>ulan2779_owned_by</skos:prefLabel>
    <dc:identifier>2779</dc:identifier>
    <rdfs:isDefinedBy rdf:resource="http://vocab.getty.edu/ulan/"/>
    <rdf:type rdf:resource="http://www.w3.org/2002/07/owl#ObjectProperty"/>
    <dct:description>person - owned by - firm.&#13;
Example: Walter Scott Lenox was owned by Lenox China Co.</dct:description>
  </rdf:Description>
  <rdf:Description rdf:about="http://vocab.getty.edu/ontology#ulan1318_member_was">
    <dc:identifier>1318</dc:identifier>
    <rdfs:range rdf:resource="http://www.w3.org/2004/02/skos/core#Concept"/>
    <skos:example>The National Gallery of Art was/is a member of the Foundation of Documentation of Architecture</skos:example>
    <rdfs:isDefinedBy rdf:resource="http://vocab.getty.edu/ontology"/>
    <dc:title>member was - firm/group</dc:title>
    <rdfs:domain rdf:resource="http://www.w3.org/2004/02/skos/core#Concept"/>
    <rdfs:isDefinedBy rdf:resource="http://vocab.getty.edu/ulan/"/>
    <skos:prefLabel>ulan1318_member_was</skos:prefLabel>
    <dct:description>person/firm/group - member was - firm/group.&#13;
Example: The National Gallery of Art was/is a member of the Foundation of Documentation of Architecture</dct:description>
    <rdf:type rdf:resource="http://www.w3.org/2002/07/owl#ObjectProperty"/>
    <rdfs:subPropertyOf rdf:resource="http://www.w3.org/2004/02/skos/core#related"/>
  </rdf:Description>
  <rdf:Description rdf:about="http://vocab.getty.edu/term/display/Display">
    <skos:notation>D</skos:notation>
    <skos:prefLabel>Use for Display</skos:prefLabel>
    <skos:notation>Y</skos:notation>
    <skos:inScheme rdf:resource="http://vocab.getty.edu/term/display/"/>
    <rdf:type rdf:resource="http://www.w3.org/2004/02/skos/core#Concept"/>
    <skos:scopeNote>Use in displays where natural order is appropriate</skos:scopeNote>
    <dct:description>Use in displays where natural order is appropriate</dct:description>
  </rdf:Description>
  <rdf:Description rdf:about="http://vocab.getty.edu/ontology#ulan1531_nephew-niece_of">
    <rdfs:subPropertyOf rdf:resource="http://www.w3.org/2004/02/skos/core#related"/>
    <owl:inverseOf rdf:resource="http://vocab.getty.edu/ontology#ulan1532_uncle-aunt_of"/>
    <rdf:type rdf:resource="http://www.w3.org/2002/07/owl#ObjectProperty"/>
    <skos:example>Jan Brueghel, the elder is the nephew/neice of  Pieter Coecke van Aeist, the younger</skos:example>
    <rdfs:range rdf:resource="http://www.w3.org/2004/02/skos/core#Concept"/>
    <skos:prefLabel>ulan1531_nephew-niece_of</skos:prefLabel>
    <rdfs:isDefinedBy rdf:resource="http://vocab.getty.edu/ontology"/>
    <dc:identifier>1531</dc:identifier>
    <dct:description>person - nephew/niece of - person.&#13;
Example: Jan Brueghel, the elder is the nephew/neice of  Pieter Coecke van Aeist, the younger</dct:description>
    <rdfs:domain rdf:resource="http://www.w3.org/2004/02/skos/core#Concept"/>
    <dc:title>nephew/niece of - person</dc:title>
    <rdfs:isDefinedBy rdf:resource="http://vocab.getty.edu/ulan/"/>
  </rdf:Description>
  <rdf:Description rdf:about="http://vocab.getty.edu/ontology#contributorPreferred">
    <rdfs:label>contributorPreferred</rdfs:label>
    <rdfs:isDefinedBy rdf:resource="http://vocab.getty.edu/ontology"/>
    <dct:description>Contributor for which the term is Preferred. Range is foaf:Agent.
Example: "organza" is preferred term for WHS</dct:description>
    <rdfs:comment>Contributor for which the term is Preferred. Range is foaf:Agent</rdfs:comment>
    <skos:example>"organza" is preferred term for WHS</skos:example>
    <rdfs:domain rdf:resource="http://www.w3.org/2008/05/skos-xl#Label"/>
    <rdfs:subPropertyOf rdf:resource="http://purl.org/dc/terms/contributor"/>
    <rdf:type rdf:resource="http://www.w3.org/2002/07/owl#ObjectProperty"/>
    <rdfs:range rdf:resource="http://xmlns.com/foaf/0.1/Agent"/>
    <skos:prefLabel>contributorPreferred</skos:prefLabel>
  </rdf:Description>
  <rdf:Description rdf:about="http://vocab.getty.edu/ontology#tgn3402_moved_to">
    <rdf:type rdf:resource="http://www.w3.org/2002/07/owl#ObjectProperty"/>
    <skos:example>Valdosta (Lowndes county, Georgia, USA) moved from Troupville (Georgia, USA)</skos:example>
    <dc:identifier>3402</dc:identifier>
    <rdfs:isDefinedBy rdf:resource="http://vocab.getty.edu/tgn/"/>
    <dct:description>place - moved to - place.&#13;
Example: Valdosta (Lowndes county, Georgia, USA) moved from Troupville (Georgia, USA)</dct:description>
    <skos:prefLabel>tgn3402_moved_to</skos:prefLabel>
    <rdfs:isDefinedBy rdf:resource="http://vocab.getty.edu/ontology"/>
    <rdfs:subPropertyOf rdf:resource="http://www.w3.org/2004/02/skos/core#related"/>
    <rdfs:domain rdf:resource="http://www.w3.org/2004/02/skos/core#Concept"/>
    <rdfs:range rdf:resource="http://www.w3.org/2004/02/skos/core#Concept"/>
    <dc:title>moved to - place</dc:title>
  </rdf:Description>
  <rdf:Description rdf:about="http://vocab.getty.edu/ontology#aat2853_involve">
    <skos:example>rose bowls involve Rosa (genus)</skos:example>
    <rdf:type rdf:resource="http://www.w3.org/2002/07/owl#ObjectProperty"/>
    <dc:title>involve - genus/species</dc:title>
    <rdfs:isDefinedBy rdf:resource="http://vocab.getty.edu/aat/"/>
    <dc:identifier>2853</dc:identifier>
    <rdfs:range rdf:resource="http://www.w3.org/2004/02/skos/core#Concept"/>
    <dct:description>things/[equipment] - involve - genus/species.&#13;
Example: rose bowls involve Rosa (genus); camel saddles involve Camelus (genus)</dct:description>
    <skos:example>camel saddles involve Camelus (genus)</skos:example>
    <rdfs:domain rdf:resource="http://www.w3.org/2004/02/skos/core#Concept"/>
    <rdfs:isDefinedBy rdf:resource="http://vocab.getty.edu/ontology"/>
    <rdfs:subPropertyOf rdf:resource="http://www.w3.org/2004/02/skos/core#related"/>
    <skos:prefLabel>aat2853_involve</skos:prefLabel>
  </rdf:Description>
  <rdf:Description rdf:about="http://vocab.getty.edu/ontology#aat2319_involves">
    <rdf:type rdf:resource="http://www.w3.org/2002/07/owl#ObjectProperty"/>
    <rdfs:isDefinedBy rdf:resource="http://vocab.getty.edu/aat/"/>
    <dc:title>involves - role</dc:title>
    <rdfs:range rdf:resource="http://www.w3.org/2004/02/skos/core#Concept"/>
    <dc:identifier>2319</dc:identifier>
    <rdfs:domain rdf:resource="http://www.w3.org/2004/02/skos/core#Concept"/>
    <skos:example>martyrdoms involve martyrs</skos:example>
    <rdfs:isDefinedBy rdf:resource="http://vocab.getty.edu/ontology"/>
    <skos:example>weddings involve bridegrooms</skos:example>
    <dct:description>activity/event - involves - [actors having] role.&#13;
Example: weddings involve bridegrooms; martyrdoms involve martyrs</dct:description>
    <skos:prefLabel>aat2319_involves</skos:prefLabel>
    <rdfs:subPropertyOf rdf:resource="http://www.w3.org/2004/02/skos/core#related"/>
  </rdf:Description>
  <rdf:Description rdf:about="http://vocab.getty.edu/ontology#ulan1006_formerly_identified_with">
    <rdfs:domain rdf:resource="http://www.w3.org/2004/02/skos/core#Concept"/>
    <rdf:type rdf:resource="http://www.w3.org/2002/07/owl#SymmetricProperty"/>
    <rdfs:subPropertyOf rdf:resource="http://www.w3.org/2004/02/skos/core#related"/>
    <rdfs:isDefinedBy rdf:resource="http://vocab.getty.edu/ontology"/>
    <dc:title>formerly identified with - any</dc:title>
    <skos:prefLabel>ulan1006_formerly_identified_with</skos:prefLabel>
    <skos:example>Tommaso is formerly identified with Tommaso di Stefano Lunetti</skos:example>
    <skos:example>GreenWorks is formerly identified with Mike Faha &amp; Associates</skos:example>
    <rdfs:isDefinedBy rdf:resource="http://vocab.getty.edu/ulan/"/>
    <dct:description>any - formerly identified with - any.&#13;
Example: Tommaso is formerly identified with Tommaso di Stefano Lunetti; GreenWorks is formerly identified with Mike Faha &amp; Associates</dct:description>
    <rdf:type rdf:resource="http://www.w3.org/2002/07/owl#ObjectProperty"/>
    <rdfs:range rdf:resource="http://www.w3.org/2004/02/skos/core#Concept"/>
    <dc:identifier>1006</dc:identifier>
  </rdf:Description>
  <rdf:Description rdf:about="http://vocab.getty.edu/historic/localUse">
    <skos:example>500051176 Abinetti (ULAN) is an unknown artist mentioned in documentation of lot 209 of an auction held 29 Jan 1824 in London</skos:example>
    <skos:inScheme rdf:resource="http://vocab.getty.edu/historic/"/>
    <skos:scopeNote>Used locally for Unidentified Named People mentioned in some document (ULAN only)</skos:scopeNote>
    <dct:description>Used locally for Unidentified Named People mentioned in some document (ULAN only).
Example: 500051176 Abinetti (ULAN) is an unknown artist mentioned in documentation of lot 209 of an auction held 29 Jan 1824 in London</dct:description>
    <skos:prefLabel>Local Use</skos:prefLabel>
    <skos:notation>LU</skos:notation>
    <rdf:type rdf:resource="http://www.w3.org/2004/02/skos/core#Concept"/>
  </rdf:Description>
  <rdf:Description rdf:about="http://vocab.getty.edu/ontology#aat2328_involved_with">
    <dc:identifier>2328</dc:identifier>
    <rdfs:isDefinedBy rdf:resource="http://vocab.getty.edu/aat/"/>
    <dc:title>involved with - things</dc:title>
    <skos:example>actors (performing artists) are involved with motion pictures (visual works)</skos:example>
    <skos:prefLabel>aat2328_involved_with</skos:prefLabel>
    <dct:description>[actors having] role - [are] involved in- things.&#13;
Example: sitters are involved with portraits; actors (performing artists) are involved with motion pictures (visual works)</dct:description>
    <rdfs:isDefinedBy rdf:resource="http://vocab.getty.edu/ontology"/>
    <skos:example>sitters are involved with portraits</skos:example>
    <rdfs:range rdf:resource="http://www.w3.org/2004/02/skos/core#Concept"/>
    <rdfs:domain rdf:resource="http://www.w3.org/2004/02/skos/core#Concept"/>
    <rdfs:subPropertyOf rdf:resource="http://www.w3.org/2004/02/skos/core#related"/>
    <owl:inverseOf rdf:resource="http://vocab.getty.edu/ontology#aat2329_involves"/>
    <rdf:type rdf:resource="http://www.w3.org/2002/07/owl#ObjectProperty"/>
  </rdf:Description>
  <rdf:Description rdf:about="http://vocab.getty.edu/ontology#ulan1421_founded_by">
    <rdf:type rdf:resource="http://www.w3.org/2002/07/owl#ObjectProperty"/>
    <dc:title>founded by - firm/group</dc:title>
    <dc:identifier>1421</dc:identifier>
    <skos:example>National Gallery of Art was founded by United States Congress</skos:example>
    <rdfs:range rdf:resource="http://www.w3.org/2004/02/skos/core#Concept"/>
    <owl:inverseOf rdf:resource="http://vocab.getty.edu/ontology#ulan1422_founded"/>
    <rdfs:domain rdf:resource="http://www.w3.org/2004/02/skos/core#Concept"/>
    <skos:prefLabel>ulan1421_founded_by</skos:prefLabel>
    <rdfs:isDefinedBy rdf:resource="http://vocab.getty.edu/ontology"/>
    <rdfs:subPropertyOf rdf:resource="http://www.w3.org/2004/02/skos/core#related"/>
    <rdfs:isDefinedBy rdf:resource="http://vocab.getty.edu/ulan/"/>
    <dct:description>firm/group - founded by - firm/group.&#13;
Example: National Gallery of Art was founded by United States Congress</dct:description>
  </rdf:Description>
  <rdf:Description rdf:about="http://vocab.getty.edu/ontology#aat2409_takes_place_in">
    <rdfs:subPropertyOf rdf:resource="http://www.w3.org/2004/02/skos/core#related"/>
    <dct:description>field of study/discipline - takes place in - locus/setting.&#13;
Example: education takes place in schools (buildings); medicine (discipline) takes place in hospitals (buildings)</dct:description>
    <rdfs:range rdf:resource="http://www.w3.org/2004/02/skos/core#Concept"/>
    <skos:example>medicine (discipline) takes place in hospitals (buildings)</skos:example>
    <rdfs:isDefinedBy rdf:resource="http://vocab.getty.edu/ontology"/>
    <skos:prefLabel>aat2409_takes_place_in</skos:prefLabel>
    <rdfs:domain rdf:resource="http://www.w3.org/2004/02/skos/core#Concept"/>
    <skos:example>education takes place in schools (buildings)</skos:example>
    <dc:identifier>2409</dc:identifier>
    <dc:title>takes place in - locus/setting</dc:title>
    <rdf:type rdf:resource="http://www.w3.org/2002/07/owl#ObjectProperty"/>
    <rdfs:isDefinedBy rdf:resource="http://vocab.getty.edu/aat/"/>
  </rdf:Description>
  <rdf:Description rdf:about="http://vocab.getty.edu/ontology#aat2286_practice-study">
    <rdfs:domain rdf:resource="http://www.w3.org/2004/02/skos/core#Concept"/>
    <dct:description>[actor having] role - practice/study - field [of study, genre]/discipline.&#13;
Example: Egyptologists practice/study Egyptology; architectural historians practice/study architectural history</dct:description>
    <skos:prefLabel>aat2286_practice-study</skos:prefLabel>
    <dc:identifier>2286</dc:identifier>
    <rdf:type rdf:resource="http://www.w3.org/2002/07/owl#ObjectProperty"/>
    <rdfs:isDefinedBy rdf:resource="http://vocab.getty.edu/aat/"/>
    <rdfs:subPropertyOf rdf:resource="http://www.w3.org/2004/02/skos/core#related"/>
    <skos:example>Egyptologists practice/study Egyptology</skos:example>
    <rdfs:range rdf:resource="http://www.w3.org/2004/02/skos/core#Concept"/>
    <rdfs:isDefinedBy rdf:resource="http://vocab.getty.edu/ontology"/>
    <dc:title>practice/study - field/discipline</dc:title>
    <skos:example>architectural historians practice/study architectural history</skos:example>
  </rdf:Description>
  <rdf:Description rdf:about="http://vocab.getty.edu/ontology#ulan2840_performer_with">
    <rdfs:range rdf:resource="http://www.w3.org/2004/02/skos/core#Concept"/>
    <dc:title>performer with - group</dc:title>
    <owl:inverseOf rdf:resource="http://vocab.getty.edu/ontology#ulan2841_performer_was"/>
    <rdf:type rdf:resource="http://www.w3.org/2002/07/owl#ObjectProperty"/>
    <dct:description>person - performer with - group</dct:description>
    <rdfs:isDefinedBy rdf:resource="http://vocab.getty.edu/ulan/"/>
    <skos:prefLabel>ulan2840_performer_with</skos:prefLabel>
    <rdfs:subPropertyOf rdf:resource="http://www.w3.org/2004/02/skos/core#related"/>
    <rdfs:domain rdf:resource="http://www.w3.org/2004/02/skos/core#Concept"/>
    <rdfs:isDefinedBy rdf:resource="http://vocab.getty.edu/ontology"/>
    <dc:identifier>2840</dc:identifier>
  </rdf:Description>
  <rdf:Description rdf:about="http://vocab.getty.edu/ontology#biographyPreferred">
    <rdfs:range rdf:resource="http://vocab.getty.edu/ontology#Biography"/>
    <rdfs:comment>Preferred biography of an ULAN agent. Domain is schema:Person/Organization, range is gvp:Biography. The biography fields are also directly available in the Person/Organization</rdfs:comment>
    <dct:description>Preferred biography of an ULAN agent. Domain is schema:Person/Organization, range is gvp:Biography. The biography fields are also directly available in the Person/Organization</dct:description>
    <rdfs:isDefinedBy rdf:resource="http://vocab.getty.edu/ontology"/>
    <skos:prefLabel>biographyPreferred</skos:prefLabel>
    <rdfs:subPropertyOf rdf:resource="http://vocab.getty.edu/ontology#biography"/>
    <rdfs:label>biographyPreferred</rdfs:label>
    <rdf:type rdf:resource="http://www.w3.org/2002/07/owl#ObjectProperty"/>
  </rdf:Description>
  <rdf:Description rdf:about="http://vocab.getty.edu/ontology#aat2836_derived-made_from">
    <dc:identifier>2836</dc:identifier>
    <rdfs:subPropertyOf rdf:resource="http://www.w3.org/2004/02/skos/core#related"/>
    <skos:example>ostrich-egg cups are derived/made from Struthio camelus (species)</skos:example>
    <rdfs:isDefinedBy rdf:resource="http://vocab.getty.edu/ontology"/>
    <owl:inverseOf rdf:resource="http://vocab.getty.edu/ontology#aat2837_source_for"/>
    <rdfs:domain rdf:resource="http://www.w3.org/2004/02/skos/core#Concept"/>
    <dct:description>things - [are] derived/made from - genus/species [or its parts].&#13;
Example: k?kaku are derived/made from Phormium tenax (species); ostrich-egg cups are derived/made from Struthio camelus (species)</dct:description>
    <dc:title>derived/made from - genus/species</dc:title>
    <rdf:type rdf:resource="http://www.w3.org/2002/07/owl#ObjectProperty"/>
    <skos:prefLabel>aat2836_derived-made_from</skos:prefLabel>
    <rdfs:range rdf:resource="http://www.w3.org/2004/02/skos/core#Concept"/>
    <rdfs:isDefinedBy rdf:resource="http://vocab.getty.edu/aat/"/>
    <skos:example>k?kaku are derived/made from Phormium tenax (species)</skos:example>
  </rdf:Description>
  <rdf:Description rdf:about="http://vocab.getty.edu/ontology#ulan1575_godchild_of">
    <rdfs:domain rdf:resource="http://www.w3.org/2004/02/skos/core#Concept"/>
    <rdfs:subPropertyOf rdf:resource="http://www.w3.org/2004/02/skos/core#related"/>
    <dc:identifier>1575</dc:identifier>
    <rdfs:isDefinedBy rdf:resource="http://vocab.getty.edu/ontology"/>
    <skos:example>Jean I Nocret is the godchild of Jean-Baptiste Goy</skos:example>
    <skos:prefLabel>ulan1575_godchild_of</skos:prefLabel>
    <rdfs:isDefinedBy rdf:resource="http://vocab.getty.edu/ulan/"/>
    <rdf:type rdf:resource="http://www.w3.org/2002/07/owl#ObjectProperty"/>
    <rdfs:range rdf:resource="http://www.w3.org/2004/02/skos/core#Concept"/>
    <dct:description>person - godchild of - person.&#13;
Example: Jean I Nocret is the godchild of Jean-Baptiste Goy</dct:description>
    <dc:title>godchild of - person</dc:title>
  </rdf:Description>
  <rdf:Description rdf:about="http://vocab.getty.edu/ontology#nationalityNonPreferred">
    <rdf:type rdf:resource="http://www.w3.org/2002/07/owl#ObjectProperty"/>
    <rdfs:isDefinedBy rdf:resource="http://vocab.getty.edu/ontology"/>
    <rdfs:comment>Non-preferred nationality/culture/race/ethnicity/religion/sexual orientation of an ULAN agent. Domain is schema:Person/Organization, range is AAT concept</rdfs:comment>
    <dct:description>Non-preferred nationality/culture/race/ethnicity/religion/sexual orientation of an ULAN agent. Domain is schema:Person/Organization, range is AAT concept</dct:description>
    <rdfs:subPropertyOf rdf:resource="http://schema.org/nationality"/>
    <skos:prefLabel>nationalityNonPreferred</skos:prefLabel>
    <rdfs:range rdf:resource="http://vocab.getty.edu/ontology#Subject"/>
    <rdfs:label>nationalityNonPreferred</rdfs:label>
  </rdf:Description>
  <rdf:Description rdf:about="http://vocab.getty.edu/ontology#ulan1552_parent_by_marriage_of">
    <rdfs:range rdf:resource="http://www.w3.org/2004/02/skos/core#Concept"/>
    <rdfs:isDefinedBy rdf:resource="http://vocab.getty.edu/ontology"/>
    <owl:inverseOf rdf:resource="http://vocab.getty.edu/ontology#ulan1553_child_by_marriage_of"/>
    <rdfs:domain rdf:resource="http://www.w3.org/2004/02/skos/core#Concept"/>
    <dct:description>person - parent by marriage (step parent) - person.&#13;
Example: Frans Hals is a parent by marriage of Pieter Gerritsz van Roestraten</dct:description>
    <rdfs:subPropertyOf rdf:resource="http://www.w3.org/2004/02/skos/core#related"/>
    <rdfs:isDefinedBy rdf:resource="http://vocab.getty.edu/ulan/"/>
    <rdf:type rdf:resource="http://www.w3.org/2002/07/owl#ObjectProperty"/>
    <dc:identifier>1552</dc:identifier>
    <skos:example>Frans Hals is a parent by marriage of Pieter Gerritsz van Roestraten</skos:example>
    <skos:prefLabel>ulan1552_parent_by_marriage_of</skos:prefLabel>
    <dc:title>parent by marriage of - person</dc:title>
  </rdf:Description>
  <rdf:Description rdf:about="http://vocab.getty.edu/ontology#Infer_skosBroader_PropChainType2">
    <ptop:conclusion rdf:resource="http://www.w3.org/2004/02/skos/core#broader"/>
    <ptop:type2 rdf:resource="http://www.w3.org/2004/02/skos/core#Concept"/>
    <rdf:type rdf:resource="http://www.ontotext.com/proton/protontop#PropChainType2"/>
    <ptop:premise2 rdf:resource="http://vocab.getty.edu/ontology#broader"/>
    <ptop:premise1 rdf:resource="http://vocab.getty.edu/ontology#broaderNonConcept"/>
  </rdf:Description>
  <rdf:Description rdf:about="http://vocab.getty.edu/ontology#ulan1316_principal_was">
    <rdfs:subPropertyOf rdf:resource="http://www.w3.org/2004/02/skos/core#related"/>
    <rdfs:isDefinedBy rdf:resource="http://vocab.getty.edu/ontology"/>
    <rdf:type rdf:resource="http://www.w3.org/2002/07/owl#ObjectProperty"/>
    <skos:example>Orazio Fontana was principal in Fontana Workshop</skos:example>
    <skos:prefLabel>ulan1316_principal_was</skos:prefLabel>
    <rdfs:range rdf:resource="http://www.w3.org/2004/02/skos/core#Concept"/>
    <dc:title>principal was - person</dc:title>
    <rdfs:isDefinedBy rdf:resource="http://vocab.getty.edu/ulan/"/>
    <rdfs:domain rdf:resource="http://www.w3.org/2004/02/skos/core#Concept"/>
    <dct:description>firm - principal was - person.&#13;
Example: Orazio Fontana was principal in Fontana Workshop</dct:description>
    <dc:identifier>1316</dc:identifier>
  </rdf:Description>
  <rdf:Description rdf:about="http://vocab.getty.edu/ontology#tgn3301_ally_of">
    <rdf:type rdf:resource="http://www.w3.org/2002/07/owl#ObjectProperty"/>
    <skos:example>Siena, Arezzo, Pisa, and Pistoia were Ghibeline allies during the 13th and 14th centuries.</skos:example>
    <rdfs:isDefinedBy rdf:resource="http://vocab.getty.edu/tgn/"/>
    <dc:identifier>3301</dc:identifier>
    <skos:prefLabel>tgn3301_ally_of</skos:prefLabel>
    <rdfs:subPropertyOf rdf:resource="http://www.w3.org/2004/02/skos/core#related"/>
    <dc:title>ally of - nation</dc:title>
    <rdf:type rdf:resource="http://www.w3.org/2002/07/owl#SymmetricProperty"/>
    <rdfs:domain rdf:resource="http://www.w3.org/2004/02/skos/core#Concept"/>
    <rdfs:isDefinedBy rdf:resource="http://vocab.getty.edu/ontology"/>
    <dct:description>nation - ally of - nation.&#13;
Example: Siena, Arezzo, Pisa, and Pistoia were Ghibeline allies during the 13th and 14th centuries.</dct:description>
    <rdfs:range rdf:resource="http://www.w3.org/2004/02/skos/core#Concept"/>
  </rdf:Description>
  <rdf:Description rdf:about="http://vocab.getty.edu/ontology#ulan2578_trustee_of">
    <rdfs:range rdf:resource="http://www.w3.org/2004/02/skos/core#Concept"/>
    <rdfs:isDefinedBy rdf:resource="http://vocab.getty.edu/ontology"/>
    <dc:identifier>2578</dc:identifier>
    <dc:title>trustee of - institution</dc:title>
    <rdfs:domain rdf:resource="http://www.w3.org/2004/02/skos/core#Concept"/>
    <rdfs:subPropertyOf rdf:resource="http://www.w3.org/2004/02/skos/core#related"/>
    <rdfs:isDefinedBy rdf:resource="http://vocab.getty.edu/ulan/"/>
    <rdf:type rdf:resource="http://www.w3.org/2002/07/owl#ObjectProperty"/>
    <skos:prefLabel>ulan2578_trustee_of</skos:prefLabel>
    <owl:inverseOf rdf:resource="http://vocab.getty.edu/ontology#ulan2579_trustee_was"/>
    <skos:example>George Douglas Haig was a trustee of the National Galleries of Scotland</skos:example>
    <dct:description>person - trustee of - institution.&#13;
Example: George Douglas Haig was a trustee of the National Galleries of Scotland</dct:description>
  </rdf:Description>
  <rdf:Description rdf:about="http://vocab.getty.edu/ontology#ulan1514_gandparent_of">
    <dc:title>gandparent of - person</dc:title>
    <rdfs:subPropertyOf rdf:resource="http://www.w3.org/2004/02/skos/core#related"/>
    <rdfs:isDefinedBy rdf:resource="http://vocab.getty.edu/ulan/"/>
    <dc:identifier>1514</dc:identifier>
    <skos:example>Frank Lloyd Wright is the grandparent of Eric Lloyd Wright</skos:example>
    <rdfs:isDefinedBy rdf:resource="http://vocab.getty.edu/ontology"/>
    <dct:description>person - gandparent of - person.&#13;
Example: Frank Lloyd Wright is the grandparent of Eric Lloyd Wright</dct:description>
    <rdfs:domain rdf:resource="http://www.w3.org/2004/02/skos/core#Concept"/>
    <skos:prefLabel>ulan1514_gandparent_of</skos:prefLabel>
    <rdf:type rdf:resource="http://www.w3.org/2002/07/owl#ObjectProperty"/>
    <rdfs:range rdf:resource="http://www.w3.org/2004/02/skos/core#Concept"/>
  </rdf:Description>
  <rdf:Description rdf:about="http://vocab.getty.edu/term/display/">
    <dct:description>Term Display concept scheme</dct:description>
    <rdf:type rdf:resource="http://www.w3.org/2004/02/skos/core#ConceptScheme"/>
    <skos:prefLabel>Term Display concept scheme</skos:prefLabel>
    <rdfs:isDefinedBy rdf:resource="http://vocab.getty.edu/ontology"/>
    <rdfs:label>Term Display concept scheme</rdfs:label>
  </rdf:Description>
  <rdf:Description rdf:about="http://vocab.getty.edu/ontology#parentStringAbbrev">
    <skos:prefLabel>parentStringAbbrev</skos:prefLabel>
    <rdfs:label>parentStringAbbrev</rdfs:label>
    <skos:example>For aat:300226882 baking dishes: bakeware, &lt;vessels for cooking food&gt;, ... Furnishings and Equipment (Hierarchy Name)</skos:example>
    <skos:note>Shortened display version of gvp:broaderPreferredExtended</skos:note>
    <dct:description>Preferred labels of *some* of the subject's preferred ancestors, listed bottom up. Useful to show the subject's context.
Shortened display version of gvp:broaderPreferredExtended.
Example for aat:300226882 baking dishes: bakeware, &lt;vessels for cooking food&gt;, ... Furnishings and Equipment (Hierarchy Name)</dct:description>
    <rdfs:comment>Preferred labels of *some* of the subject's preferred ancestors, listed bottom up. Useful to show the subject's context</rdfs:comment>
    <rdfs:range rdf:resource="http://www.w3.org/1999/02/22-rdf-syntax-ns#Literal"/>
    <rdf:type rdf:resource="http://www.w3.org/2002/07/owl#DatatypeProperty"/>
    <rdfs:domain rdf:resource="http://vocab.getty.edu/ontology#Subject"/>
    <rdfs:isDefinedBy rdf:resource="http://vocab.getty.edu/ontology"/>
  </rdf:Description>
  <rdf:Description rdf:about="http://vocab.getty.edu/ontology#agentTypeNonPreferred">
    <rdf:type rdf:resource="http://www.w3.org/2002/07/owl#ObjectProperty"/>
    <rdfs:subPropertyOf rdf:resource="http://vocab.getty.edu/ontology#agentType"/>
    <rdfs:comment>A secondary type of a ULAN Person or Corporate body. Domain is ULAN concept, range is AAT concept</rdfs:comment>
    <skos:example>Non-preferred types of "Albrecht Duerer Workshop" (ULAN) include "printmakers" and painters" (AAT)</skos:example>
    <rdfs:isDefinedBy rdf:resource="http://vocab.getty.edu/ontology"/>
    <rdfs:domain rdf:resource="http://vocab.getty.edu/ontology#Subject"/>
    <rdfs:label>agentTypeNonPreferred</rdfs:label>
    <dct:description>A secondary type of a ULAN Person or Corporate body. Domain is ULAN concept, range is AAT concept.
Example: Non-preferred types of "Albrecht Duerer Workshop" (ULAN) include "printmakers" and painters" (AAT)</dct:description>
    <rdfs:range rdf:resource="http://vocab.getty.edu/ontology#Subject"/>
    <skos:prefLabel>agentTypeNonPreferred</skos:prefLabel>
  </rdf:Description>
  <rdf:Description rdf:about="http://vocab.getty.edu/ontology#broaderGenericExtended">
    <rdfs:isDefinedBy rdf:resource="http://vocab.getty.edu/ontology"/>
    <owl:propertyChainAxiom rdf:nodeID="N6b1e97a28ead495895d1bc18dbd2d7fc"/>
    <rdfs:subPropertyOf rdf:resource="http://vocab.getty.edu/ontology#broaderExtended"/>
    <rdfs:range rdf:resource="http://vocab.getty.edu/ontology#Subject"/>
    <rdfs:domain rdf:resource="http://vocab.getty.edu/ontology#Subject"/>
    <rdf:type rdf:resource="http://www.w3.org/2002/07/owl#ObjectProperty"/>
    <skos:example>&lt;anvils and anvil accessories&gt; BTG &lt;forging and metal-shaping tools&gt; BTG &lt;forging and metal-shaping equipment&gt;,
so &lt;anvils and anvil accessories&gt; BTGE &lt;forging and metal-shaping equipment&gt;</skos:example>
    <rdfs:label>broaderGenericExtended</rdfs:label>
    <rdfs:comment>Ancestors (Generic). Meaningful closure of gvp:broaderGeneric. Infers iso:broaderGeneric for pairs of directly related skos:Concepts</rdfs:comment>
    <dct:description>Ancestors (Generic). Meaningful closure of gvp:broaderGeneric. Infers iso:broaderGeneric for pairs of directly related skos:Concepts.
Example: &lt;anvils and anvil accessories&gt; BTG &lt;forging and metal-shaping tools&gt; BTG &lt;forging and metal-shaping equipment&gt;,
so &lt;anvils and anvil accessories&gt; BTGE &lt;forging and metal-shaping equipment&gt;</dct:description>
    <skos:prefLabel>broaderGenericExtended</skos:prefLabel>
  </rdf:Description>
  <rdf:Description rdf:about="http://vocab.getty.edu/ontology#term">
    <rdfs:comment>Term (label), used as the basic (prefix) part of skosxsl:literalForm</rdfs:comment>
    <dct:description>Term (label), used as the basic (prefix) part of skosxsl:literalForm</dct:description>
    <skos:prefLabel>term</skos:prefLabel>
    <rdfs:label>term</rdfs:label>
    <rdf:type rdf:resource="http://www.w3.org/2002/07/owl#DatatypeProperty"/>
    <rdfs:range rdf:resource="http://www.w3.org/1999/02/22-rdf-syntax-ns#Literal"/>
    <rdfs:domain rdf:resource="http://www.w3.org/2008/05/skos-xl#Label"/>
    <rdfs:isDefinedBy rdf:resource="http://vocab.getty.edu/ontology"/>
  </rdf:Description>
  <rdf:Description rdf:about="http://vocab.getty.edu/ontology#PersonConcept">
    <rdfs:subClassOf rdf:resource="http://www.w3.org/2004/02/skos/core#Concept"/>
    <rdfs:comment>A single individual. Usually people engaged in the design or creation of art or architecture ("Artists"); but may also include donors, patrons, rulers, sitters, art historians, etc ("Non-Artists")</rdfs:comment>
    <skos:example>500115493 Duerer, Albrecht (ULAN)</skos:example>
    <rdfs:isDefinedBy rdf:resource="http://vocab.getty.edu/ontology"/>
    <dct:description>A single individual. Usually people engaged in the design or creation of art or architecture ("Artists"); but may also include donors, patrons, rulers, sitters, art historians, etc ("Non-Artists").
Example: 500115493 Duerer, Albrecht (ULAN)</dct:description>
    <rdfs:label>PersonConcept</rdfs:label>
    <skos:prefLabel>PersonConcept</skos:prefLabel>
    <rdf:type rdf:resource="http://www.w3.org/2002/07/owl#Class"/>
    <rdfs:subClassOf rdf:resource="http://vocab.getty.edu/ontology#Subject"/>
  </rdf:Description>
  <rdf:Description rdf:about="http://vocab.getty.edu/ontology#aat2333_have_affiliates">
    <skos:example>duchies have as affiliates dukes</skos:example>
    <skos:prefLabel>aat2333_have_affiliates</skos:prefLabel>
    <dc:identifier>2333</dc:identifier>
    <rdf:type rdf:resource="http://www.w3.org/2002/07/owl#ObjectProperty"/>
    <rdfs:range rdf:resource="http://www.w3.org/2004/02/skos/core#Concept"/>
    <rdfs:isDefinedBy rdf:resource="http://vocab.getty.edu/aat/"/>
    <skos:example>schools (organizations) have as affiliates students</skos:example>
    <rdfs:subPropertyOf rdf:resource="http://www.w3.org/2004/02/skos/core#related"/>
    <dc:title>have affiliates - role</dc:title>
    <dct:description>role [organizations] - have affiliates - [actors having] role.&#13;
Example: schools (organizations) have as affiliates students; duchies have as affiliates dukes</dct:description>
    <rdfs:isDefinedBy rdf:resource="http://vocab.getty.edu/ontology"/>
    <rdfs:domain rdf:resource="http://www.w3.org/2004/02/skos/core#Concept"/>
  </rdf:Description>
  <rdf:Description rdf:about="http://vocab.getty.edu/ontology#aat2332_affiliated_with">
    <skos:prefLabel>aat2332_affiliated_with</skos:prefLabel>
    <dct:description>[actors having] role - [are] affiliated with - role [organization].&#13;
Example: students are affiliated with schools (organizations); dukes are affiliated with duchies</dct:description>
    <rdfs:domain rdf:resource="http://www.w3.org/2004/02/skos/core#Concept"/>
    <owl:inverseOf rdf:resource="http://vocab.getty.edu/ontology#aat2333_have_affiliates"/>
    <rdfs:isDefinedBy rdf:resource="http://vocab.getty.edu/ontology"/>
    <skos:example>students are affiliated with schools (organizations)</skos:example>
    <dc:title>affiliated with - role</dc:title>
    <rdfs:range rdf:resource="http://www.w3.org/2004/02/skos/core#Concept"/>
    <skos:example>dukes are affiliated with duchies</skos:example>
    <rdfs:isDefinedBy rdf:resource="http://vocab.getty.edu/aat/"/>
    <rdfs:subPropertyOf rdf:resource="http://www.w3.org/2004/02/skos/core#related"/>
    <rdf:type rdf:resource="http://www.w3.org/2002/07/owl#ObjectProperty"/>
    <dc:identifier>2332</dc:identifier>
  </rdf:Description>
  <rdf:Description rdf:about="http://vocab.getty.edu/ontology#ulan1301_colleague_of">
    <rdf:type rdf:resource="http://www.w3.org/2002/07/owl#ObjectProperty"/>
    <rdfs:range rdf:resource="http://www.w3.org/2004/02/skos/core#Concept"/>
    <skos:example>Titian was a colleague of Maria Giovanni Verdizotti</skos:example>
    <rdfs:domain rdf:resource="http://www.w3.org/2004/02/skos/core#Concept"/>
    <skos:prefLabel>ulan1301_colleague_of</skos:prefLabel>
    <rdf:type rdf:resource="http://www.w3.org/2002/07/owl#SymmetricProperty"/>
    <dct:description>person - colleague of - person.&#13;
Example: Titian was a colleague of Maria Giovanni Verdizotti</dct:description>
    <rdfs:isDefinedBy rdf:resource="http://vocab.getty.edu/ontology"/>
    <dc:title>colleague of - person</dc:title>
    <rdfs:isDefinedBy rdf:resource="http://vocab.getty.edu/ulan/"/>
    <rdfs:subPropertyOf rdf:resource="http://www.w3.org/2004/02/skos/core#related"/>
    <dc:identifier>1301</dc:identifier>
  </rdf:Description>
  <rdf:Description rdf:about="http://vocab.getty.edu/ontology#aat2222_are_acted_upon">
    <skos:example>Acer saccharum(species) is acted upon by tappers</skos:example>
    <dc:identifier>2222</dc:identifier>
    <rdf:type rdf:resource="http://www.w3.org/2002/07/owl#ObjectProperty"/>
    <dct:description>genus/species - is acted upon [by] - [actors having] role.&#13;
Example: Equus caballus(species) is acted upon by jockeys; Acer saccharum(species) is acted upon by tappers</dct:description>
    <rdfs:range rdf:resource="http://www.w3.org/2004/02/skos/core#Concept"/>
    <rdfs:domain rdf:resource="http://www.w3.org/2004/02/skos/core#Concept"/>
    <skos:example>Equus caballus(species) is acted upon by jockeys</skos:example>
    <rdfs:subPropertyOf rdf:resource="http://www.w3.org/2004/02/skos/core#related"/>
    <rdfs:isDefinedBy rdf:resource="http://vocab.getty.edu/ontology"/>
    <skos:prefLabel>aat2222_are_acted_upon</skos:prefLabel>
    <dc:title>are acted upon - role</dc:title>
    <rdfs:isDefinedBy rdf:resource="http://vocab.getty.edu/aat/"/>
  </rdf:Description>
  <rdf:Description rdf:about="http://vocab.getty.edu/term/kind/FullName">
    <skos:inScheme rdf:resource="http://vocab.getty.edu/term/kind/"/>
    <skos:scopeNote>Full Name of an ULAN agent</skos:scopeNote>
    <skos:notation>FN</skos:notation>
    <skos:example>TODO</skos:example>
    <dct:description>Full Name of an ULAN agent.
Example: TODO</dct:description>
    <skos:prefLabel>Full Name</skos:prefLabel>
    <rdf:type rdf:resource="http://www.w3.org/2004/02/skos/core#Concept"/>
  </rdf:Description>
  <rdf:Description rdf:about="http://vocab.getty.edu/ontology#ulan1310_advised_by">
    <dc:title>advised by - person</dc:title>
    <rdfs:subPropertyOf rdf:resource="http://www.w3.org/2004/02/skos/core#related"/>
    <rdfs:isDefinedBy rdf:resource="http://vocab.getty.edu/ontology"/>
    <dc:identifier>1310</dc:identifier>
    <skos:example>Henry VIII, King of England was advised by Thomas Cromwell, Earl of Essex</skos:example>
    <rdfs:isDefinedBy rdf:resource="http://vocab.getty.edu/ulan/"/>
    <rdf:type rdf:resource="http://www.w3.org/2002/07/owl#ObjectProperty"/>
    <skos:prefLabel>ulan1310_advised_by</skos:prefLabel>
    <rdfs:range rdf:resource="http://www.w3.org/2004/02/skos/core#Concept"/>
    <rdfs:domain rdf:resource="http://www.w3.org/2004/02/skos/core#Concept"/>
    <dct:description>person - advised by - person.&#13;
Example: Henry VIII, King of England was advised by Thomas Cromwell, Earl of Essex</dct:description>
  </rdf:Description>
  <rdf:Description rdf:about="http://vocab.getty.edu/ontology#ulan1306_performs_with">
    <skos:example>Harry Kipper performs with Harry Kipper (as part of 'The Kipper Kids')</skos:example>
    <rdf:type rdf:resource="http://www.w3.org/2002/07/owl#SymmetricProperty"/>
    <rdfs:isDefinedBy rdf:resource="http://vocab.getty.edu/ontology"/>
    <rdfs:subPropertyOf rdf:resource="http://www.w3.org/2004/02/skos/core#related"/>
    <dc:identifier>1306</dc:identifier>
    <rdfs:domain rdf:resource="http://www.w3.org/2004/02/skos/core#Concept"/>
    <rdfs:range rdf:resource="http://www.w3.org/2004/02/skos/core#Concept"/>
    <dct:description>person - performs with - person.&#13;
Example: Harry Kipper performs with Harry Kipper (as part of 'The Kipper Kids')</dct:description>
    <rdf:type rdf:resource="http://www.w3.org/2002/07/owl#ObjectProperty"/>
    <dc:title>performs with - person</dc:title>
    <skos:prefLabel>ulan1306_performs_with</skos:prefLabel>
    <rdfs:isDefinedBy rdf:resource="http://vocab.getty.edu/ulan/"/>
  </rdf:Description>
  <rdf:Description rdf:about="http://vocab.getty.edu/ontology#aat2322_use">
    <rdfs:domain rdf:resource="http://www.w3.org/2004/02/skos/core#Concept"/>
    <dc:title>use - things</dc:title>
    <dc:identifier>2322</dc:identifier>
    <skos:example>violoncellists use violoncellos</skos:example>
    <skos:prefLabel>aat2322_use</skos:prefLabel>
    <skos:example>surveyors use surveying instruments</skos:example>
    <rdf:type rdf:resource="http://www.w3.org/2002/07/owl#ObjectProperty"/>
    <rdfs:subPropertyOf rdf:resource="http://www.w3.org/2004/02/skos/core#related"/>
    <rdfs:range rdf:resource="http://www.w3.org/2004/02/skos/core#Concept"/>
    <rdfs:isDefinedBy rdf:resource="http://vocab.getty.edu/aat/"/>
    <dct:description>[actors having] role - use - things/equipment.&#13;
Example: violoncellists use violoncellos; surveyors use surveying instruments</dct:description>
    <rdfs:isDefinedBy rdf:resource="http://vocab.getty.edu/ontology"/>
  </rdf:Description>
  <rdf:Description rdf:about="http://vocab.getty.edu/ontology#aat2806_provide_context">
    <rdfs:domain rdf:resource="http://www.w3.org/2004/02/skos/core#Concept"/>
    <rdfs:isDefinedBy rdf:resource="http://vocab.getty.edu/ontology"/>
    <dc:title>provide context - things</dc:title>
    <rdfs:isDefinedBy rdf:resource="http://vocab.getty.edu/aat/"/>
    <rdfs:range rdf:resource="http://www.w3.org/2004/02/skos/core#Concept"/>
    <dct:description>[larger] things - provide context [for] - [smaller] things.&#13;
Example: altarpieces provide context for predellas; books provide context for chapters</dct:description>
    <skos:example>books provide context for chapters</skos:example>
    <skos:prefLabel>aat2806_provide_context</skos:prefLabel>
    <rdf:type rdf:resource="http://www.w3.org/2002/07/owl#ObjectProperty"/>
    <dc:identifier>2806</dc:identifier>
    <skos:example>altarpieces provide context for predellas</skos:example>
    <rdfs:subPropertyOf rdf:resource="http://www.w3.org/2004/02/skos/core#related"/>
  </rdf:Description>
  <rdf:Description rdf:about="http://vocab.getty.edu/ontology#aat2411_involved_in">
    <rdfs:isDefinedBy rdf:resource="http://vocab.getty.edu/aat/"/>
    <skos:example>journalistic photography is involved in photojournalism (discipline)</skos:example>
    <rdf:type rdf:resource="http://www.w3.org/2002/07/owl#ObjectProperty"/>
    <rdfs:range rdf:resource="http://www.w3.org/2004/02/skos/core#Concept"/>
    <owl:inverseOf rdf:resource="http://vocab.getty.edu/ontology#aat2412_involves"/>
    <dct:description>activity/event/[process/function] - [is] involved in - field/discipline.&#13;
Example: journalistic photography is involved in photojournalism (discipline); gardening is involved in horticulture</dct:description>
    <rdfs:domain rdf:resource="http://www.w3.org/2004/02/skos/core#Concept"/>
    <skos:prefLabel>aat2411_involved_in</skos:prefLabel>
    <rdfs:subPropertyOf rdf:resource="http://www.w3.org/2004/02/skos/core#related"/>
    <rdfs:isDefinedBy rdf:resource="http://vocab.getty.edu/ontology"/>
    <dc:title>involved in - field/discipline</dc:title>
    <dc:identifier>2411</dc:identifier>
    <skos:example>gardening is involved in horticulture</skos:example>
  </rdf:Description>
  <rdf:Description rdf:about="http://vocab.getty.edu/ontology#ulan1521_cousin_of">
    <dc:title>cousin of - person</dc:title>
    <rdf:type rdf:resource="http://www.w3.org/2002/07/owl#ObjectProperty"/>
    <skos:example>Richard Meier and Frank Gehry are cousins</skos:example>
    <rdfs:isDefinedBy rdf:resource="http://vocab.getty.edu/ulan/"/>
    <rdfs:subPropertyOf rdf:resource="http://www.w3.org/2004/02/skos/core#related"/>
    <rdf:type rdf:resource="http://www.w3.org/2002/07/owl#SymmetricProperty"/>
    <rdfs:isDefinedBy rdf:resource="http://vocab.getty.edu/ontology"/>
    <skos:prefLabel>ulan1521_cousin_of</skos:prefLabel>
    <rdfs:domain rdf:resource="http://www.w3.org/2004/02/skos/core#Concept"/>
    <dc:identifier>1521</dc:identifier>
    <rdfs:range rdf:resource="http://www.w3.org/2004/02/skos/core#Concept"/>
    <dct:description>person - cousin of - person.&#13;
Example: Richard Meier and Frank Gehry are cousins</dct:description>
  </rdf:Description>
  <rdf:Description rdf:about="http://vocab.getty.edu/ontology#aat2834_decendant_of">
    <dc:title>decendant of - genus/species</dc:title>
    <rdf:type rdf:resource="http://www.w3.org/2002/07/owl#ObjectProperty"/>
    <skos:example>donkeys are the descendents of Equus asinus</skos:example>
    <rdfs:isDefinedBy rdf:resource="http://vocab.getty.edu/aat/"/>
    <rdfs:range rdf:resource="http://www.w3.org/2004/02/skos/core#Concept"/>
    <rdfs:subPropertyOf rdf:resource="http://www.w3.org/2004/02/skos/core#related"/>
    <rdfs:domain rdf:resource="http://www.w3.org/2004/02/skos/core#Concept"/>
    <skos:prefLabel>aat2834_decendant_of</skos:prefLabel>
    <dct:description>genus/species - is decendant of -  genus/species.&#13;
Example: Canis familiaris is the descendant of Canis lupus; donkeys are the descendents of Equus asinus</dct:description>
    <rdfs:isDefinedBy rdf:resource="http://vocab.getty.edu/ontology"/>
    <dc:identifier>2834</dc:identifier>
    <skos:example>Canis familiaris is the descendant of Canis lupus</skos:example>
  </rdf:Description>
  <rdf:Description rdf:about="http://vocab.getty.edu/ontology#aat2563_located_in">
    <rdf:type rdf:resource="http://www.w3.org/2002/07/owl#ObjectProperty"/>
    <skos:example>Brahmanism is located/reflected in agraharas</skos:example>
    <rdfs:subPropertyOf rdf:resource="http://www.w3.org/2004/02/skos/core#related"/>
    <dct:description>style/period/culture/[religion/ideology] - is located/[reflected] in - locus/setting.&#13;
Example: First Nations (culture) is located/reflected in First Nations reserves; Brahmanism is located/reflected in agraharas</dct:description>
    <dc:title>located in - locus/setting</dc:title>
    <rdfs:isDefinedBy rdf:resource="http://vocab.getty.edu/ontology"/>
    <rdfs:domain rdf:resource="http://www.w3.org/2004/02/skos/core#Concept"/>
    <rdfs:isDefinedBy rdf:resource="http://vocab.getty.edu/aat/"/>
    <rdfs:range rdf:resource="http://www.w3.org/2004/02/skos/core#Concept"/>
    <dc:identifier>2563</dc:identifier>
    <skos:example>First Nations (culture) is located/reflected in First Nations reserves</skos:example>
    <skos:prefLabel>aat2563_located_in</skos:prefLabel>
  </rdf:Description>
  <rdf:Description rdf:about="http://vocab.getty.edu/ontology#ulan1108_influenced_by">
    <rdfs:subPropertyOf rdf:resource="http://www.w3.org/2004/02/skos/core#related"/>
    <rdfs:isDefinedBy rdf:resource="http://vocab.getty.edu/ontology"/>
    <dct:description>person - influenced by - person.&#13;
Example: Salomon Koninck was influenced by Rembrandt van Rijn</dct:description>
    <skos:example>Salomon Koninck was influenced by Rembrandt van Rijn</skos:example>
    <rdf:type rdf:resource="http://www.w3.org/2002/07/owl#ObjectProperty"/>
    <dc:title>influenced by - person</dc:title>
    <skos:prefLabel>ulan1108_influenced_by</skos:prefLabel>
    <rdfs:range rdf:resource="http://www.w3.org/2004/02/skos/core#Concept"/>
    <rdfs:domain rdf:resource="http://www.w3.org/2004/02/skos/core#Concept"/>
    <dc:identifier>1108</dc:identifier>
    <rdfs:isDefinedBy rdf:resource="http://vocab.getty.edu/ulan/"/>
  </rdf:Description>
  <rdf:Description rdf:about="http://vocab.getty.edu/term/type/AlternateDescriptor">
    <dct:description>A lexical variant, eg singular.
Example: "manuscript" (English) instead of "manuscripts"</dct:description>
    <skos:inScheme rdf:resource="http://vocab.getty.edu/term/type/"/>
    <rdf:type rdf:resource="http://www.w3.org/2004/02/skos/core#Concept"/>
    <skos:scopeNote>A lexical variant, eg singular</skos:scopeNote>
    <skos:example>"manuscript" (English) instead of "manuscripts"</skos:example>
    <skos:prefLabel>Alternate Descriptor</skos:prefLabel>
    <skos:notation>AD</skos:notation>
  </rdf:Description>
  <rdf:Description rdf:about="http://vocab.getty.edu/ontology#displayOrder">
    <rdfs:comment>Display order of subject or term amongst its siblings.
If all are 1 then use alphabetical. Domain is gvp:Subject or skosxl:Label</rdfs:comment>
    <dct:description>Display order of subject or term amongst its siblings.
If all are 1 then use alphabetical. Domain is gvp:Subject or skosxl:Label</dct:description>
    <skos:prefLabel>displayOrder</skos:prefLabel>
    <rdfs:range rdf:resource="http://www.w3.org/2001/XMLSchema#positiveInteger"/>
    <rdfs:isDefinedBy rdf:resource="http://vocab.getty.edu/ontology"/>
    <rdfs:label>displayOrder</rdfs:label>
    <rdf:type rdf:resource="http://www.w3.org/2002/07/owl#DatatypeProperty"/>
  </rdf:Description>
  <rdf:Description rdf:about="http://vocab.getty.edu/term/POS/PluralNoun">
    <skos:example>"filigrane" is the Italian plural for "watermarks"</skos:example>
    <dct:description>A term that is plural (the same word may be singular in another language).
Example: "filigrane" is the Italian plural for "watermarks"</dct:description>
    <skos:prefLabel>Plural Noun</skos:prefLabel>
    <skos:notation>PN</skos:notation>
    <rdf:type rdf:resource="http://www.w3.org/2004/02/skos/core#Concept"/>
    <skos:inScheme rdf:resource="http://vocab.getty.edu/term/POS/"/>
    <skos:scopeNote>A term that is plural (the same word may be singular in another language)</skos:scopeNote>
  </rdf:Description>
  <rdf:Description rdf:about="http://vocab.getty.edu/ontology#aat2555_reflected_in">
    <skos:prefLabel>aat2555_reflected_in</skos:prefLabel>
    <dct:description>style/period/culture /[religion/ideology] - [is] reflected in activity/event.&#13;
Example: Dhokra (culture) is reflected in dhokra (casting technique); Red-figure [style] is reflected in red-figure vase painting</dct:description>
    <skos:example>Dhokra (culture) is reflected in dhokra (casting technique)</skos:example>
    <rdfs:isDefinedBy rdf:resource="http://vocab.getty.edu/ontology"/>
    <rdfs:domain rdf:resource="http://www.w3.org/2004/02/skos/core#Concept"/>
    <rdfs:isDefinedBy rdf:resource="http://vocab.getty.edu/aat/"/>
    <rdfs:subPropertyOf rdf:resource="http://www.w3.org/2004/02/skos/core#related"/>
    <dc:title>reflected in - activity/event</dc:title>
    <rdf:type rdf:resource="http://www.w3.org/2002/07/owl#ObjectProperty"/>
    <skos:example>Red-figure [style] is reflected in red-figure vase painting</skos:example>
    <dc:identifier>2555</dc:identifier>
    <rdfs:range rdf:resource="http://www.w3.org/2004/02/skos/core#Concept"/>
  </rdf:Description>
  <rdf:Description rdf:about="http://vocab.getty.edu/ontology#PhysAdminPlaceConcept">
    <rdfs:comment>Place that is both administrative and physical. Rarely used. Used in TGN only</rdfs:comment>
    <rdfs:label>PhysAdminPlaceConcept</rdfs:label>
    <rdfs:isDefinedBy rdf:resource="http://vocab.getty.edu/ontology"/>
    <skos:prefLabel>PhysAdminPlaceConcept</skos:prefLabel>
    <rdfs:subClassOf rdf:resource="http://vocab.getty.edu/ontology#Subject"/>
    <skos:example>6003090 Kiik-Koba (TGN)</skos:example>
    <rdfs:subClassOf rdf:resource="http://www.w3.org/2004/02/skos/core#Concept"/>
    <rdf:type rdf:resource="http://www.w3.org/2002/07/owl#Class"/>
    <dct:description>Place that is both administrative and physical. Rarely used. Used in TGN only.
Example: 6003090 Kiik-Koba (TGN)</dct:description>
  </rdf:Description>
  <rdf:Description rdf:about="http://vocab.getty.edu/ontology#eventPreferred">
    <rdf:type rdf:resource="http://www.w3.org/2002/07/owl#ObjectProperty"/>
    <rdfs:range rdf:resource="http://purl.org/vocab/bio/0.1/Event"/>
    <rdfs:subPropertyOf rdf:resource="http://purl.org/vocab/bio/0.1/event"/>
    <skos:prefLabel>eventPreferred</skos:prefLabel>
    <rdfs:label>eventPreferred</rdfs:label>
    <rdfs:isDefinedBy rdf:resource="http://vocab.getty.edu/ontology"/>
    <rdfs:comment>Preferred life event of an ULAN agent. Domain is schema:Person/Organization, range is bio:Event</rdfs:comment>
    <dct:description>Preferred life event of an ULAN agent. Domain is schema:Person/Organization, range is bio:Event</dct:description>
  </rdf:Description>
  <rdf:Description rdf:about="http://vocab.getty.edu/ontology#aat2891_exemplified_by">
    <skos:prefLabel>aat2891_exemplified_by</skos:prefLabel>
    <rdfs:isDefinedBy rdf:resource="http://vocab.getty.edu/ontology"/>
    <rdfs:domain rdf:resource="http://www.w3.org/2004/02/skos/core#Concept"/>
    <dct:description>things - [are] exemplied by - brand name.&#13;
Example: photothermographic transfer prints are exemplified by Pictrography (TM) prints</dct:description>
    <dc:title>exemplified by - brand name</dc:title>
    <rdfs:isDefinedBy rdf:resource="http://vocab.getty.edu/aat/"/>
    <rdfs:subPropertyOf rdf:resource="http://www.w3.org/2004/02/skos/core#related"/>
    <dc:identifier>2891</dc:identifier>
    <owl:inverseOf rdf:resource="http://vocab.getty.edu/ontology#aat2892_example_of"/>
    <rdf:type rdf:resource="http://www.w3.org/2002/07/owl#ObjectProperty"/>
    <skos:example>photothermographic transfer prints are exemplified by Pictrography (TM) prints</skos:example>
    <rdfs:range rdf:resource="http://www.w3.org/2004/02/skos/core#Concept"/>
  </rdf:Description>
  <rdf:Description rdf:about="http://vocab.getty.edu/ontology#aat2000_related_to">
    <skos:example>gulf red is related to light red (pigment)</skos:example>
    <rdfs:subPropertyOf rdf:resource="http://www.w3.org/2004/02/skos/core#related"/>
    <rdfs:range rdf:resource="http://www.w3.org/2004/02/skos/core#Concept"/>
    <rdfs:isDefinedBy rdf:resource="http://vocab.getty.edu/ontology"/>
    <skos:prefLabel>aat2000_related_to</skos:prefLabel>
    <dct:description>any - related to - any; generic relationship, not explained.&#13;
Example: gulf red is related to light red (pigment)</dct:description>
    <rdf:type rdf:resource="http://www.w3.org/2002/07/owl#SymmetricProperty"/>
    <rdfs:domain rdf:resource="http://www.w3.org/2004/02/skos/core#Concept"/>
    <dc:identifier>2000</dc:identifier>
    <dc:title>related to - any</dc:title>
    <skos:scopeNote>generic relationship, not explained</skos:scopeNote>
    <rdf:type rdf:resource="http://www.w3.org/2002/07/owl#ObjectProperty"/>
    <rdfs:isDefinedBy rdf:resource="http://vocab.getty.edu/aat/"/>
  </rdf:Description>
  <rdf:Description rdf:about="http://vocab.getty.edu/ontology#ulan1550_relative_by_marriage">
    <dct:description>person - relative by marriage (in-law) - person.&#13;
Example: Juana Galarza d Goicoechea and Francisco de Goya are related by marriage</dct:description>
    <rdfs:domain rdf:resource="http://www.w3.org/2004/02/skos/core#Concept"/>
    <rdf:type rdf:resource="http://www.w3.org/2002/07/owl#SymmetricProperty"/>
    <rdfs:subPropertyOf rdf:resource="http://www.w3.org/2004/02/skos/core#related"/>
    <rdfs:isDefinedBy rdf:resource="http://vocab.getty.edu/ontology"/>
    <skos:example>Juana Galarza d Goicoechea and Francisco de Goya are related by marriage</skos:example>
    <dc:identifier>1550</dc:identifier>
    <rdfs:isDefinedBy rdf:resource="http://vocab.getty.edu/ulan/"/>
    <skos:prefLabel>ulan1550_relative_by_marriage</skos:prefLabel>
    <rdf:type rdf:resource="http://www.w3.org/2002/07/owl#ObjectProperty"/>
    <rdfs:range rdf:resource="http://www.w3.org/2004/02/skos/core#Concept"/>
    <dc:title>relative by marriage - person</dc:title>
  </rdf:Description>
  <rdf:Description rdf:about="http://vocab.getty.edu/ontology#aat2846_locus-setting_for">
    <rdfs:isDefinedBy rdf:resource="http://vocab.getty.edu/aat/"/>
    <dc:identifier>2846</dc:identifier>
    <rdfs:subPropertyOf rdf:resource="http://www.w3.org/2004/02/skos/core#related"/>
    <dc:title>locus/setting for - genus/species</dc:title>
    <skos:example>vineyards are the locus/setting of Vitaceae (family)</skos:example>
    <rdfs:domain rdf:resource="http://www.w3.org/2004/02/skos/core#Concept"/>
    <rdfs:isDefinedBy rdf:resource="http://vocab.getty.edu/ontology"/>
    <skos:example>elephant houses are the locus/setting for Elephantidae(family)</skos:example>
    <rdfs:range rdf:resource="http://www.w3.org/2004/02/skos/core#Concept"/>
    <rdf:type rdf:resource="http://www.w3.org/2002/07/owl#ObjectProperty"/>
    <skos:prefLabel>aat2846_locus-setting_for</skos:prefLabel>
    <dct:description>locus/setting - [is] locus/setting for - genus/species.&#13;
Example: elephant houses are the locus/setting for Elephantidae(family); vineyards are the locus/setting of Vitaceae (family)</dct:description>
  </rdf:Description>
  <rdf:Description rdf:about="http://vocab.getty.edu/ontology#ulan1561_step-child_of">
    <dc:identifier>1561</dc:identifier>
    <rdf:type rdf:resource="http://www.w3.org/2002/07/owl#ObjectProperty"/>
    <dct:description>person - step-child of - person.&#13;
Example: Hortense, Quene consort of Louis Bonaparte is the step-child of Napoleon I, Emperor of the French</dct:description>
    <rdfs:range rdf:resource="http://www.w3.org/2004/02/skos/core#Concept"/>
    <dc:title>step-child of - person</dc:title>
    <rdfs:subPropertyOf rdf:resource="http://www.w3.org/2004/02/skos/core#related"/>
    <skos:prefLabel>ulan1561_step-child_of</skos:prefLabel>
    <rdfs:isDefinedBy rdf:resource="http://vocab.getty.edu/ulan/"/>
    <owl:inverseOf rdf:resource="http://vocab.getty.edu/ontology#ulan1562_step-parent_of"/>
    <skos:example>Hortense, Quene consort of Louis Bonaparte is the step-child of Napoleon I, Emperor of the French</skos:example>
    <rdfs:isDefinedBy rdf:resource="http://vocab.getty.edu/ontology"/>
    <rdfs:domain rdf:resource="http://www.w3.org/2004/02/skos/core#Concept"/>
  </rdf:Description>
  <rdf:Description rdf:about="http://vocab.getty.edu/ontology#aat2811_preceded">
    <rdfs:subPropertyOf rdf:resource="http://www.w3.org/2004/02/skos/core#related"/>
    <rdfs:domain rdf:resource="http://www.w3.org/2004/02/skos/core#Concept"/>
    <dc:title>preceded - style/period/culture</dc:title>
    <dc:identifier>2811</dc:identifier>
    <rdfs:isDefinedBy rdf:resource="http://vocab.getty.edu/ontology"/>
    <skos:example>Impressionist preceded Abstract Impressionist</skos:example>
    <rdfs:range rdf:resource="http://www.w3.org/2004/02/skos/core#Concept"/>
    <dct:description>style/period/culture/[religion/ideology] - preceded  - style/period/culture/[religion/ideology].&#13;
Example: Impressionist preceded Abstract Impressionist; Acheulian preceded Micoquian</dct:description>
    <owl:inverseOf rdf:resource="http://vocab.getty.edu/ontology#aat2812_followed"/>
    <skos:example>Acheulian preceded Micoquian</skos:example>
    <skos:prefLabel>aat2811_preceded</skos:prefLabel>
    <rdf:type rdf:resource="http://www.w3.org/2002/07/owl#ObjectProperty"/>
    <rdfs:isDefinedBy rdf:resource="http://vocab.getty.edu/aat/"/>
  </rdf:Description>
  <rdf:Description rdf:nodeID="N0e7c8cba70fe4e7cb81d6f70b73e2d46">
    <rdf:first rdf:resource="http://vocab.getty.edu/ontology#broaderPartitive"/>
    <rdf:rest rdf:resource="http://www.w3.org/1999/02/22-rdf-syntax-ns#nil"/>
  </rdf:Description>
  <rdf:Description rdf:about="http://vocab.getty.edu/ontology#aat2221_act_upon">
    <dc:title>act upon - genus/species</dc:title>
    <rdfs:isDefinedBy rdf:resource="http://vocab.getty.edu/ontology"/>
    <skos:example>tappers act upon Acer saccharum(species)</skos:example>
    <rdfs:domain rdf:resource="http://www.w3.org/2004/02/skos/core#Concept"/>
    <owl:inverseOf rdf:resource="http://vocab.getty.edu/ontology#aat2222_are_acted_upon"/>
    <skos:example>jockeys act upon Equus caballus(species)</skos:example>
    <rdfs:subPropertyOf rdf:resource="http://www.w3.org/2004/02/skos/core#related"/>
    <rdfs:range rdf:resource="http://www.w3.org/2004/02/skos/core#Concept"/>
    <dct:description>[actors having] role - act upon - genus/species.&#13;
Example: jockeys act upon Equus caballus(species); tappers act upon Acer saccharum(species)</dct:description>
    <skos:prefLabel>aat2221_act_upon</skos:prefLabel>
    <rdf:type rdf:resource="http://www.w3.org/2002/07/owl#ObjectProperty"/>
    <rdfs:isDefinedBy rdf:resource="http://vocab.getty.edu/aat/"/>
    <dc:identifier>2221</dc:identifier>
  </rdf:Description>
  <rdf:Description rdf:about="http://vocab.getty.edu/ontology#tgn3110_meaning-usage_overlaps_with">
    <dct:description>any - meaning/usage overlaps with - any.&#13;
Example: Judaea (Israel) (historical region) meaning/usage overlaps with Holy Land (Asia) (historical region)</dct:description>
    <rdfs:range rdf:resource="http://www.w3.org/2004/02/skos/core#Concept"/>
    <skos:prefLabel>tgn3110_meaning-usage_overlaps_with</skos:prefLabel>
    <skos:example>Judaea (Israel) (historical region) meaning/usage overlaps with Holy Land (Asia) (historical region)</skos:example>
    <dc:identifier>3110</dc:identifier>
    <rdfs:subPropertyOf rdf:resource="http://www.w3.org/2004/02/skos/core#related"/>
    <rdf:type rdf:resource="http://www.w3.org/2002/07/owl#ObjectProperty"/>
    <rdfs:domain rdf:resource="http://www.w3.org/2004/02/skos/core#Concept"/>
    <rdf:type rdf:resource="http://www.w3.org/2002/07/owl#SymmetricProperty"/>
    <rdfs:isDefinedBy rdf:resource="http://vocab.getty.edu/tgn/"/>
    <dc:title>meaning/usage overlaps with - any</dc:title>
    <rdfs:isDefinedBy rdf:resource="http://vocab.getty.edu/ontology"/>
  </rdf:Description>
  <rdf:Description rdf:about="http://vocab.getty.edu/ontology#aat2826_used_with">
    <skos:prefLabel>aat2826_used_with</skos:prefLabel>
    <rdf:type rdf:resource="http://www.w3.org/2002/07/owl#SymmetricProperty"/>
    <rdfs:isDefinedBy rdf:resource="http://vocab.getty.edu/ontology"/>
    <skos:example>arriccio is used with intonaco</skos:example>
    <rdfs:subPropertyOf rdf:resource="http://www.w3.org/2004/02/skos/core#related"/>
    <rdfs:domain rdf:resource="http://www.w3.org/2004/02/skos/core#Concept"/>
    <dct:description>material - [is] used with - material.&#13;
Example: watercolor paper is used with watercolor (paint); arriccio is used with intonaco</dct:description>
    <rdfs:range rdf:resource="http://www.w3.org/2004/02/skos/core#Concept"/>
    <dc:identifier>2826</dc:identifier>
    <dc:title>used with - material</dc:title>
    <skos:example>watercolor paper is used with watercolor (paint)</skos:example>
    <rdf:type rdf:resource="http://www.w3.org/2002/07/owl#ObjectProperty"/>
    <rdfs:isDefinedBy rdf:resource="http://vocab.getty.edu/aat/"/>
  </rdf:Description>
  <rdf:Description rdf:about="http://vocab.getty.edu/ontology#aat2895_example_of">
    <rdfs:domain rdf:resource="http://www.w3.org/2004/02/skos/core#Concept"/>
    <rdf:type rdf:resource="http://www.w3.org/2002/07/owl#ObjectProperty"/>
    <rdfs:subPropertyOf rdf:resource="http://www.w3.org/2004/02/skos/core#related"/>
    <dct:description>brand name - [is] example of - activity/event/[process/function].&#13;
Example: Papersave Process (TM) is example of deacidification [process/function]</dct:description>
    <skos:example>Papersave Process (TM) is example of deacidification [process/function]</skos:example>
    <dc:title>example of - activity/event</dc:title>
    <rdfs:range rdf:resource="http://www.w3.org/2004/02/skos/core#Concept"/>
    <rdfs:isDefinedBy rdf:resource="http://vocab.getty.edu/aat/"/>
    <skos:prefLabel>aat2895_example_of</skos:prefLabel>
    <dc:identifier>2895</dc:identifier>
    <rdfs:isDefinedBy rdf:resource="http://vocab.getty.edu/ontology"/>
  </rdf:Description>
  <rdf:Description rdf:about="http://vocab.getty.edu/term/POS/">
    <rdfs:isDefinedBy rdf:resource="http://vocab.getty.edu/ontology"/>
    <rdf:type rdf:resource="http://www.w3.org/2004/02/skos/core#ConceptScheme"/>
    <rdfs:label>Part of Speech concept scheme</rdfs:label>
    <dct:description>Part of Speech concept scheme</dct:description>
    <skos:prefLabel>Part of Speech concept scheme</skos:prefLabel>
  </rdf:Description>
  <rdf:Description rdf:about="http://vocab.getty.edu/ontology#aat2831_associated_with">
    <rdfs:isDefinedBy rdf:resource="http://vocab.getty.edu/ontology"/>
    <skos:prefLabel>aat2831_associated_with</skos:prefLabel>
    <dc:identifier>2831</dc:identifier>
    <rdf:type rdf:resource="http://www.w3.org/2002/07/owl#SymmetricProperty"/>
    <rdfs:domain rdf:resource="http://www.w3.org/2004/02/skos/core#Concept"/>
    <rdfs:subPropertyOf rdf:resource="http://www.w3.org/2004/02/skos/core#related"/>
    <skos:example>Amphiprioninae (subfamily) [clown fish] is associated with Actiniaria (order) [sea anemone]</skos:example>
    <dc:title>associated with - genus/species</dc:title>
    <rdfs:range rdf:resource="http://www.w3.org/2004/02/skos/core#Concept"/>
    <skos:example>Anthonomus grandis (species) [boll weevil] is associated with Gossypium (genus) [cotton]</skos:example>
    <dct:description>genus/species/[other living organism term] - [is] associated with - genus/species.&#13;
Example: Anthonomus grandis (species) [boll weevil] is associated with Gossypium (genus) [cotton]; Amphiprioninae (subfamily) [clown fish] is associated with Actiniaria (order) [sea anemone]</dct:description>
    <rdf:type rdf:resource="http://www.w3.org/2002/07/owl#ObjectProperty"/>
    <rdfs:isDefinedBy rdf:resource="http://vocab.getty.edu/aat/"/>
  </rdf:Description>
  <rdf:Description rdf:about="http://vocab.getty.edu/ontology#Hierarchy">
    <rdfs:isDefinedBy rdf:resource="http://vocab.getty.edu/ontology"/>
    <dct:description>Top of a hierarchy. Used in AAT only. Not used for indexing or cataloguing.
Example: Containers (Hierarchy Name) (AAT)</dct:description>
    <skos:example>Containers (Hierarchy Name) (AAT)</skos:example>
    <skos:prefLabel>Hierarchy</skos:prefLabel>
    <rdf:type rdf:resource="http://www.w3.org/2002/07/owl#Class"/>
    <rdfs:comment>Top of a hierarchy. Used in AAT only. Not used for indexing or cataloguing</rdfs:comment>
    <rdfs:label>Hierarchy</rdfs:label>
    <rdfs:subClassOf rdf:resource="http://purl.org/iso25964/skos-thes#ThesaurusArray"/>
    <rdfs:subClassOf rdf:resource="http://vocab.getty.edu/ontology#Subject"/>
  </rdf:Description>
  <rdf:Description rdf:about="http://vocab.getty.edu/ontology#broader">
    <rdf:type rdf:resource="http://www.w3.org/2002/07/owl#ObjectProperty"/>
    <dct:description>Parents of a subject. Each broader is also Preferred|NonPreferred and Partitive|Instantial|Generic</dct:description>
    <skos:prefLabel>broader</skos:prefLabel>
    <rdfs:range rdf:resource="http://vocab.getty.edu/ontology#Subject"/>
    <rdfs:label>broader</rdfs:label>
    <rdfs:isDefinedBy rdf:resource="http://vocab.getty.edu/ontology"/>
    <rdfs:domain rdf:resource="http://vocab.getty.edu/ontology#Subject"/>
    <rdfs:comment>Parents of a subject. Each broader is also Preferred|NonPreferred and Partitive|Instantial|Generic</rdfs:comment>
  </rdf:Description>
  <rdf:Description rdf:about="http://vocab.getty.edu/ontology#isNoted">
    <rdfs:comment>One amongst several homographic concepts may be especially noted so it's easier to find</rdfs:comment>
    <rdfs:domain rdf:resource="http://vocab.getty.edu/ontology#Subject"/>
    <skos:example>tgn:7008038 Paris, France is noted but tgn:2106600 Paris, Texas is not (except if you're Fassbinder)</skos:example>
    <rdfs:label>isNoted</rdfs:label>
    <rdfs:isDefinedBy rdf:resource="http://vocab.getty.edu/ontology"/>
    <dct:description>One amongst several homographic concepts may be especially noted so it's easier to find.
Example: tgn:7008038 Paris, France is noted but tgn:2106600 Paris, Texas is not (except if you're Fassbinder)</dct:description>
    <rdfs:range rdf:resource="http://www.w3.org/2001/XMLSchema#boolean"/>
    <rdf:type rdf:resource="http://www.w3.org/2002/07/owl#DatatypeProperty"/>
    <skos:prefLabel>isNoted</skos:prefLabel>
  </rdf:Description>
  <rdf:Description rdf:about="http://vocab.getty.edu/ontology#Infer_skosBroader_TypeRestr">
    <ptop:type2 rdf:resource="http://www.w3.org/2004/02/skos/core#Concept"/>
    <ptop:premise rdf:resource="http://vocab.getty.edu/ontology#broader"/>
    <rdf:type rdf:resource="http://www.ontotext.com/proton/protontop#TypeRestr"/>
    <ptop:type1 rdf:resource="http://www.w3.org/2004/02/skos/core#Concept"/>
    <ptop:conclusion rdf:resource="http://www.w3.org/2004/02/skos/core#broader"/>
  </rdf:Description>
  <rdf:Description rdf:about="http://vocab.getty.edu/ontology#ulan1113_fellow_student_of">
    <dc:identifier>1113</dc:identifier>
    <rdfs:isDefinedBy rdf:resource="http://vocab.getty.edu/ulan/"/>
    <rdf:type rdf:resource="http://www.w3.org/2002/07/owl#ObjectProperty"/>
    <skos:example>Alexander Calder was a fellow student of John Sloan</skos:example>
    <skos:prefLabel>ulan1113_fellow_student_of</skos:prefLabel>
    <rdfs:range rdf:resource="http://www.w3.org/2004/02/skos/core#Concept"/>
    <dc:title>fellow student of - person</dc:title>
    <rdfs:domain rdf:resource="http://www.w3.org/2004/02/skos/core#Concept"/>
    <rdf:type rdf:resource="http://www.w3.org/2002/07/owl#SymmetricProperty"/>
    <rdfs:subPropertyOf rdf:resource="http://www.w3.org/2004/02/skos/core#related"/>
    <rdfs:isDefinedBy rdf:resource="http://vocab.getty.edu/ontology"/>
    <skos:example>John Sloan was a fellow student of Thomas Hart Benton</skos:example>
    <dct:description>person - fellow student of - person.&#13;
Example: Alexander Calder was a fellow student of John Sloan; John Sloan was a fellow student of Thomas Hart Benton</dct:description>
  </rdf:Description>
  <rdf:Description rdf:about="http://vocab.getty.edu/ontology#sourceAlternatePreferred">
    <rdfs:label>sourceAlternatePreferred</rdfs:label>
    <skos:prefLabel>sourceAlternatePreferred</skos:prefLabel>
    <rdfs:subPropertyOf rdf:resource="http://purl.org/dc/terms/source"/>
    <rdfs:range rdf:resource="http://purl.org/ontology/bibo/Document"/>
    <rdf:type rdf:resource="http://www.w3.org/2002/07/owl#ObjectProperty"/>
    <rdfs:domain rdf:resource="http://www.w3.org/2008/05/skos-xl#Label"/>
    <rdfs:comment>Source for which the term is Alternate Preferred. Range is bibo:Document or bibo:DocumentPart</rdfs:comment>
    <dct:description>Source for which the term is Alternate Preferred. Range is bibo:Document or bibo:DocumentPart.
Example: "Kayseri" is alternate preferred in Webster's New Geographical Dictionary (1988)</dct:description>
    <skos:example>"Kayseri" is alternate preferred in Webster's New Geographical Dictionary (1988)</skos:example>
    <rdfs:isDefinedBy rdf:resource="http://vocab.getty.edu/ontology"/>
  </rdf:Description>
  <rdf:Description rdf:about="http://vocab.getty.edu/ontology#ulan2828_student_at">
    <owl:inverseOf rdf:resource="http://vocab.getty.edu/ontology#ulan2829_student_was"/>
    <rdf:type rdf:resource="http://www.w3.org/2002/07/owl#ObjectProperty"/>
    <skos:prefLabel>ulan2828_student_at</skos:prefLabel>
    <rdfs:range rdf:resource="http://www.w3.org/2004/02/skos/core#Concept"/>
    <rdfs:domain rdf:resource="http://www.w3.org/2004/02/skos/core#Concept"/>
    <dc:title>student at - institution</dc:title>
    <dc:identifier>2828</dc:identifier>
    <rdfs:subPropertyOf rdf:resource="http://www.w3.org/2004/02/skos/core#related"/>
    <rdfs:isDefinedBy rdf:resource="http://vocab.getty.edu/ontology"/>
    <skos:example>Zdanek Rossman was a student at Bauhaus</skos:example>
    <rdfs:isDefinedBy rdf:resource="http://vocab.getty.edu/ulan/"/>
    <dct:description>person - student at - institution.&#13;
Example: Zdanek Rossman was a student at Bauhaus</dct:description>
  </rdf:Description>
  <rdf:Description rdf:about="http://schema.org/dissolutionLocation">
    <dct:description>The place where the Organization was dissolved.
Schema has properties foundationLocation and dissolutionDate but no dissolutionLocation. 
In contrast, for a person all 4 properties are present: birth/death place/date.
We posted issue https://github.com/schemaorg/schemaorg/issues/302, which looks like it will have a positive outcome in the far future.
And we define the property here</dct:description>
    <skos:prefLabel>dissolutionLocation</skos:prefLabel>
    <rdfs:range rdf:resource="http://schema.org/Place"/>
    <rdfs:domain rdf:resource="http://schema.org/Organization"/>
    <rdfs:label>dissolutionLocation</rdfs:label>
    <rdfs:isDefinedBy rdf:resource="http://vocab.getty.edu/ontology"/>
    <rdfs:comment>The place where the Organization was dissolved</rdfs:comment>
    <rdfs:seeAlso rdf:resource="https://github.com/schemaorg/schemaorg/issues/302"/>
    <rdf:type rdf:resource="http://www.w3.org/2002/07/owl#ObjectProperty"/>
  </rdf:Description>
  <rdf:Description rdf:about="http://vocab.getty.edu/ontology#ulan2550_friend_of">
    <dc:title>friend of - person</dc:title>
    <skos:example>Alfred Stieglitz and Frank Simon Herrmann were friends</skos:example>
    <rdf:type rdf:resource="http://www.w3.org/2002/07/owl#ObjectProperty"/>
    <rdfs:isDefinedBy rdf:resource="http://vocab.getty.edu/ontology"/>
    <dct:description>person - friend of (personal relationship) - person.&#13;
Example: Alfred Stieglitz and Frank Simon Herrmann were friends</dct:description>
    <skos:prefLabel>ulan2550_friend_of</skos:prefLabel>
    <rdf:type rdf:resource="http://www.w3.org/2002/07/owl#SymmetricProperty"/>
    <rdfs:domain rdf:resource="http://www.w3.org/2004/02/skos/core#Concept"/>
    <rdfs:subPropertyOf rdf:resource="http://www.w3.org/2004/02/skos/core#related"/>
    <rdfs:isDefinedBy rdf:resource="http://vocab.getty.edu/ulan/"/>
    <dc:identifier>2550</dc:identifier>
    <rdfs:range rdf:resource="http://www.w3.org/2004/02/skos/core#Concept"/>
  </rdf:Description>
  <rdf:Description rdf:about="http://vocab.getty.edu/ontology#ulan1307_assistant_of">
    <skos:example>Bernard Castelli was assistant of Pablo Picasso</skos:example>
    <rdfs:isDefinedBy rdf:resource="http://vocab.getty.edu/ulan/"/>
    <dc:title>assistant of - person</dc:title>
    <owl:inverseOf rdf:resource="http://vocab.getty.edu/ontology#ulan1308_assisted_by"/>
    <rdfs:subPropertyOf rdf:resource="http://www.w3.org/2004/02/skos/core#related"/>
    <rdfs:domain rdf:resource="http://www.w3.org/2004/02/skos/core#Concept"/>
    <rdf:type rdf:resource="http://www.w3.org/2002/07/owl#ObjectProperty"/>
    <dc:identifier>1307</dc:identifier>
    <skos:prefLabel>ulan1307_assistant_of</skos:prefLabel>
    <dct:description>person - assistant of - person.&#13;
Example: Bernard Castelli was assistant of Pablo Picasso</dct:description>
    <rdfs:range rdf:resource="http://www.w3.org/2004/02/skos/core#Concept"/>
    <rdfs:isDefinedBy rdf:resource="http://vocab.getty.edu/ontology"/>
  </rdf:Description>
  <rdf:Description rdf:about="http://vocab.getty.edu/ontology#placeType">
    <skos:prefLabel>placeType</skos:prefLabel>
    <rdfs:comment>Type for a TGN place. Domain is TGN concept (AdminPlaceConcept or PhysPlaceConcept), range is AAT Concept</rdfs:comment>
    <skos:example>Machupicchu, Peru has preferred type "deserted settlement" (current) and non-preferred type "Inca center" (historic)</skos:example>
    <dct:description>Type for a TGN place. Domain is TGN concept (AdminPlaceConcept or PhysPlaceConcept), range is AAT Concept.
Example: Machupicchu, Peru has preferred type "deserted settlement" (current) and non-preferred type "Inca center" (historic)</dct:description>
    <rdfs:range rdf:resource="http://vocab.getty.edu/ontology#Subject"/>
    <rdf:type rdf:resource="http://www.w3.org/2002/07/owl#ObjectProperty"/>
    <rdfs:label>placeType</rdfs:label>
    <rdfs:domain rdf:resource="http://vocab.getty.edu/ontology#Subject"/>
    <rdfs:isDefinedBy rdf:resource="http://vocab.getty.edu/ontology"/>
  </rdf:Description>
  <rdf:Description rdf:about="http://vocab.getty.edu/ontology#ulan1202_patron_was">
    <dct:description>person/firm/family - patron was - person.&#13;
Example: The patron of Donatello was Cosimo I, Grand-Duke of Tuscany</dct:description>
    <rdfs:domain rdf:resource="http://www.w3.org/2004/02/skos/core#Concept"/>
    <skos:example>The patron of Donatello was Cosimo I, Grand-Duke of Tuscany</skos:example>
    <skos:prefLabel>ulan1202_patron_was</skos:prefLabel>
    <rdfs:isDefinedBy rdf:resource="http://vocab.getty.edu/ontology"/>
    <rdfs:subPropertyOf rdf:resource="http://www.w3.org/2004/02/skos/core#related"/>
    <dc:identifier>1202</dc:identifier>
    <rdfs:isDefinedBy rdf:resource="http://vocab.getty.edu/ulan/"/>
    <rdf:type rdf:resource="http://www.w3.org/2002/07/owl#ObjectProperty"/>
    <rdfs:range rdf:resource="http://www.w3.org/2004/02/skos/core#Concept"/>
    <dc:title>patron was - person</dc:title>
  </rdf:Description>
  <rdf:Description rdf:about="http://vocab.getty.edu/ontology#ulan1557_step-sibling_of">
    <skos:example>W. L. Wyllie and Lionel Percy Smythe are step-siblings</skos:example>
    <skos:prefLabel>ulan1557_step-sibling_of</skos:prefLabel>
    <dc:identifier>1557</dc:identifier>
    <rdfs:isDefinedBy rdf:resource="http://vocab.getty.edu/ulan/"/>
    <rdfs:domain rdf:resource="http://www.w3.org/2004/02/skos/core#Concept"/>
    <rdf:type rdf:resource="http://www.w3.org/2002/07/owl#SymmetricProperty"/>
    <rdfs:isDefinedBy rdf:resource="http://vocab.getty.edu/ontology"/>
    <rdfs:range rdf:resource="http://www.w3.org/2004/02/skos/core#Concept"/>
    <dct:description>person - step-sibling of - person.&#13;
Example: W. L. Wyllie and Lionel Percy Smythe are step-siblings</dct:description>
    <dc:title>step-sibling of - person</dc:title>
    <rdfs:subPropertyOf rdf:resource="http://www.w3.org/2004/02/skos/core#related"/>
    <rdf:type rdf:resource="http://www.w3.org/2002/07/owl#ObjectProperty"/>
  </rdf:Description>
  <rdf:Description rdf:about="http://vocab.getty.edu/ontology#aat2852_involved_with">
    <skos:prefLabel>aat2852_involved_with</skos:prefLabel>
    <rdfs:subPropertyOf rdf:resource="http://www.w3.org/2004/02/skos/core#related"/>
    <owl:inverseOf rdf:resource="http://vocab.getty.edu/ontology#aat2853_involve"/>
    <rdfs:domain rdf:resource="http://www.w3.org/2004/02/skos/core#Concept"/>
    <rdfs:isDefinedBy rdf:resource="http://vocab.getty.edu/ontology"/>
    <dct:description>genus/species - [is] involved with - things/[equipment].&#13;
Example: Rosa (genus) is involved with rose bowls; Camelus (genus) is involved with camel saddles</dct:description>
    <rdfs:range rdf:resource="http://www.w3.org/2004/02/skos/core#Concept"/>
    <dc:title>involved with - things</dc:title>
    <skos:example>Camelus (genus) is involved with camel saddles</skos:example>
    <dc:identifier>2852</dc:identifier>
    <rdf:type rdf:resource="http://www.w3.org/2002/07/owl#ObjectProperty"/>
    <rdfs:isDefinedBy rdf:resource="http://vocab.getty.edu/aat/"/>
    <skos:example>Rosa (genus) is involved with rose bowls</skos:example>
  </rdf:Description>
  <rdf:Description rdf:about="http://vocab.getty.edu/ontology#ulan1112_master_was">
    <rdfs:range rdf:resource="http://www.w3.org/2004/02/skos/core#Concept"/>
    <dct:description>person - master was - person.&#13;
Example: Peter Paul Rubens - master of Jan Thomas</dct:description>
    <rdf:type rdf:resource="http://www.w3.org/2002/07/owl#ObjectProperty"/>
    <rdfs:isDefinedBy rdf:resource="http://vocab.getty.edu/ulan/"/>
    <dc:identifier>1112</dc:identifier>
    <skos:example>Peter Paul Rubens - master of Jan Thomas</skos:example>
    <rdfs:domain rdf:resource="http://www.w3.org/2004/02/skos/core#Concept"/>
    <rdfs:subPropertyOf rdf:resource="http://www.w3.org/2004/02/skos/core#related"/>
    <rdfs:isDefinedBy rdf:resource="http://vocab.getty.edu/ontology"/>
    <skos:prefLabel>ulan1112_master_was</skos:prefLabel>
    <dc:title>master was - person</dc:title>
  </rdf:Description>
  <rdf:Description rdf:about="http://vocab.getty.edu/ontology#aat2829_used-required_for">
    <skos:example>wine is required/used for wine glasses</skos:example>
    <rdfs:domain rdf:resource="http://www.w3.org/2004/02/skos/core#Concept"/>
    <dc:identifier>2829</dc:identifier>
    <skos:prefLabel>aat2829_used-required_for</skos:prefLabel>
    <rdfs:range rdf:resource="http://www.w3.org/2004/02/skos/core#Concept"/>
    <rdfs:isDefinedBy rdf:resource="http://vocab.getty.edu/ontology"/>
    <dc:title>used/required for - things</dc:title>
    <dct:description>material - [is] required/used for - things.&#13;
Example: varnish is used/required for oil paintings; wine is required/used for wine glasses</dct:description>
    <rdfs:isDefinedBy rdf:resource="http://vocab.getty.edu/aat/"/>
    <skos:example>varnish is used/required for oil paintings</skos:example>
    <rdf:type rdf:resource="http://www.w3.org/2002/07/owl#ObjectProperty"/>
    <rdfs:subPropertyOf rdf:resource="http://www.w3.org/2004/02/skos/core#related"/>
  </rdf:Description>
  <rdf:Description rdf:about="http://vocab.getty.edu/term/POS/SingularNoun">
    <skos:scopeNote>A term that is singular (the same word may be plural in another language)</skos:scopeNote>
    <skos:notation>SN</skos:notation>
    <skos:inScheme rdf:resource="http://vocab.getty.edu/term/POS/"/>
    <skos:example>"filigrane" is the French singular for "watermark"</skos:example>
    <skos:prefLabel>Singular Noun</skos:prefLabel>
    <rdf:type rdf:resource="http://www.w3.org/2004/02/skos/core#Concept"/>
    <dct:description>A term that is singular (the same word may be plural in another language).
Example: "filigrane" is the French singular for "watermark"</dct:description>
  </rdf:Description>
  <rdf:Description rdf:about="http://vocab.getty.edu/ontology#aat2416_requires">
    <rdf:type rdf:resource="http://www.w3.org/2002/07/owl#ObjectProperty"/>
    <dc:identifier>2416</dc:identifier>
    <dc:title>requires - material</dc:title>
    <rdfs:subPropertyOf rdf:resource="http://www.w3.org/2004/02/skos/core#related"/>
    <skos:example>dying requires dye</skos:example>
    <skos:prefLabel>aat2416_requires</skos:prefLabel>
    <rdfs:isDefinedBy rdf:resource="http://vocab.getty.edu/ontology"/>
    <rdfs:domain rdf:resource="http://www.w3.org/2004/02/skos/core#Concept"/>
    <skos:example>pewtersmithing requires pewter</skos:example>
    <rdfs:isDefinedBy rdf:resource="http://vocab.getty.edu/aat/"/>
    <rdfs:range rdf:resource="http://www.w3.org/2004/02/skos/core#Concept"/>
    <dct:description>activity/event/[process/function] - requires - material.&#13;
Example: dying requires dye; pewtersmithing requires pewter</dct:description>
  </rdf:Description>
  <rdf:Description rdf:about="http://vocab.getty.edu/ontology#contributorNonPreferred">
    <rdfs:isDefinedBy rdf:resource="http://vocab.getty.edu/ontology"/>
    <rdfs:domain rdf:resource="http://www.w3.org/2008/05/skos-xl#Label"/>
    <rdfs:range rdf:resource="http://xmlns.com/foaf/0.1/Agent"/>
    <rdfs:comment>Contributor for which the term is Non-preferred. Range is foaf:Agent</rdfs:comment>
    <rdf:type rdf:resource="http://www.w3.org/2002/07/owl#ObjectProperty"/>
    <skos:example>"Lycra" is non-preferred term for WHS</skos:example>
    <rdfs:label>contributorNonPreferred</rdfs:label>
    <skos:prefLabel>contributorNonPreferred</skos:prefLabel>
    <rdfs:subPropertyOf rdf:resource="http://purl.org/dc/terms/contributor"/>
    <dct:description>Contributor for which the term is Non-preferred. Range is foaf:Agent.
Example: "Lycra" is non-preferred term for WHS</dct:description>
  </rdf:Description>
  <rdf:Description rdf:about="http://vocab.getty.edu/ontology#aat2892_example_of">
    <rdf:type rdf:resource="http://www.w3.org/2002/07/owl#ObjectProperty"/>
    <dc:identifier>2892</dc:identifier>
    <rdfs:subPropertyOf rdf:resource="http://www.w3.org/2004/02/skos/core#related"/>
    <skos:example>Pictrography (TM) prints are examples of photothermographic transfer prints</skos:example>
    <rdfs:isDefinedBy rdf:resource="http://vocab.getty.edu/ontology"/>
    <rdfs:domain rdf:resource="http://www.w3.org/2004/02/skos/core#Concept"/>
    <rdfs:isDefinedBy rdf:resource="http://vocab.getty.edu/aat/"/>
    <dc:title>example of - things</dc:title>
    <rdfs:range rdf:resource="http://www.w3.org/2004/02/skos/core#Concept"/>
    <dct:description>brand name - [is] example of - things.&#13;
Example: Pictrography (TM) prints are examples of photothermographic transfer prints</dct:description>
    <skos:prefLabel>aat2892_example_of</skos:prefLabel>
  </rdf:Description>
  <rdf:Description rdf:about="http://vocab.getty.edu/ontology#ulan1317_member_of">
    <dc:title>member of - person/firm/group</dc:title>
    <skos:example>A member of the Foundation of Documents of Architecture is the National Gallery of Art</skos:example>
    <rdf:type rdf:resource="http://www.w3.org/2002/07/owl#ObjectProperty"/>
    <dc:identifier>1317</dc:identifier>
    <rdfs:subPropertyOf rdf:resource="http://www.w3.org/2004/02/skos/core#related"/>
    <dct:description>firm/group - member of - person/firm/group.&#13;
Example: A member of the Foundation of Documents of Architecture is the National Gallery of Art</dct:description>
    <owl:inverseOf rdf:resource="http://vocab.getty.edu/ontology#ulan1318_member_was"/>
    <rdfs:isDefinedBy rdf:resource="http://vocab.getty.edu/ulan/"/>
    <rdfs:domain rdf:resource="http://www.w3.org/2004/02/skos/core#Concept"/>
    <rdfs:range rdf:resource="http://www.w3.org/2004/02/skos/core#Concept"/>
    <skos:prefLabel>ulan1317_member_of</skos:prefLabel>
    <rdfs:isDefinedBy rdf:resource="http://vocab.getty.edu/ontology"/>
  </rdf:Description>
  <rdf:Description rdf:about="http://vocab.getty.edu/ontology#ObsoleteSubject">
    <rdf:type rdf:resource="http://www.w3.org/2002/07/owl#Class"/>
    <rdfs:subClassOf rdf:resource="http://vocab.getty.edu/ontology#Subject"/>
    <rdfs:label>ObsoleteSubject</rdfs:label>
    <rdfs:isDefinedBy rdf:resource="http://vocab.getty.edu/ontology"/>
    <rdfs:comment>Obsolete subject: moved out of the publishable hierarchy, or merged to another (pointed by dct:isReplacedBy)</rdfs:comment>
    <dct:description>Obsolete subject: moved out of the publishable hierarchy, or merged to another (pointed by dct:isReplacedBy).
Example: 300375205 "shranks" (AAT) was merged to 300039264 "schranks" (AAT), so aat:300375205 dct:isReplacedBy aat:300039264</dct:description>
    <skos:example>300375205 "shranks" (AAT) was merged to 300039264 "schranks" (AAT), so aat:300375205 dct:isReplacedBy aat:300039264</skos:example>
    <skos:prefLabel>ObsoleteSubject</skos:prefLabel>
  </rdf:Description>
  <rdf:Description rdf:about="http://vocab.getty.edu/ontology#ulan2782_dedicated_to">
    <dc:title>dedicated to - person</dc:title>
    <dc:identifier>2782</dc:identifier>
    <rdfs:isDefinedBy rdf:resource="http://vocab.getty.edu/ontology"/>
    <rdfs:domain rdf:resource="http://www.w3.org/2004/02/skos/core#Concept"/>
    <rdfs:isDefinedBy rdf:resource="http://vocab.getty.edu/ulan/"/>
    <rdfs:subPropertyOf rdf:resource="http://www.w3.org/2004/02/skos/core#related"/>
    <dct:description>institution - dedicated to - person.&#13;
Example: The Rodin Museum in Philadelphia is didicated to Auguste Rodin</dct:description>
    <rdf:type rdf:resource="http://www.w3.org/2002/07/owl#ObjectProperty"/>
    <skos:example>The Rodin Museum in Philadelphia is didicated to Auguste Rodin</skos:example>
    <skos:prefLabel>ulan2782_dedicated_to</skos:prefLabel>
    <rdfs:range rdf:resource="http://www.w3.org/2004/02/skos/core#Concept"/>
  </rdf:Description>
  <rdf:Description rdf:about="http://vocab.getty.edu/ontology#tgn3101_near-adjacent_to">
    <dc:identifier>3101</dc:identifier>
    <dc:title>near/adjacent to - any</dc:title>
    <dct:description>any - near/adjacent to - any.&#13;
Example: Saint Paul (Minnesota, USA), is linked to its 'Twin City' Minneapolis (Hennepin county, Minnesota, USA)</dct:description>
    <rdf:type rdf:resource="http://www.w3.org/2002/07/owl#ObjectProperty"/>
    <rdfs:range rdf:resource="http://www.w3.org/2004/02/skos/core#Concept"/>
    <rdfs:subPropertyOf rdf:resource="http://www.w3.org/2004/02/skos/core#related"/>
    <skos:example>Saint Paul (Minnesota, USA), is linked to its 'Twin City' Minneapolis (Hennepin county, Minnesota, USA)</skos:example>
    <skos:prefLabel>tgn3101_near-adjacent_to</skos:prefLabel>
    <rdfs:isDefinedBy rdf:resource="http://vocab.getty.edu/tgn/"/>
    <rdfs:domain rdf:resource="http://www.w3.org/2004/02/skos/core#Concept"/>
    <rdf:type rdf:resource="http://www.w3.org/2002/07/owl#SymmetricProperty"/>
    <rdfs:isDefinedBy rdf:resource="http://vocab.getty.edu/ontology"/>
  </rdf:Description>
  <rdf:Description rdf:about="http://vocab.getty.edu/ontology#aat2554_reflects">
    <owl:inverseOf rdf:resource="http://vocab.getty.edu/ontology#aat2555_reflected_in"/>
    <skos:example>red-figure vase painting reflects Red-figure [style]</skos:example>
    <rdfs:isDefinedBy rdf:resource="http://vocab.getty.edu/aat/"/>
    <dct:description>activity/event - reflects - style/period/culture /[religion/ideology].&#13;
Example: dhokra (casting technique) reflects Dhokra (culture); red-figure vase painting reflects Red-figure [style]</dct:description>
    <skos:example>dhokra (casting technique) reflects Dhokra (culture)</skos:example>
    <skos:prefLabel>aat2554_reflects</skos:prefLabel>
    <dc:identifier>2554</dc:identifier>
    <dc:title>reflects - style/period/culture</dc:title>
    <rdfs:range rdf:resource="http://www.w3.org/2004/02/skos/core#Concept"/>
    <rdfs:isDefinedBy rdf:resource="http://vocab.getty.edu/ontology"/>
    <rdfs:domain rdf:resource="http://www.w3.org/2004/02/skos/core#Concept"/>
    <rdfs:subPropertyOf rdf:resource="http://www.w3.org/2004/02/skos/core#related"/>
    <rdf:type rdf:resource="http://www.w3.org/2002/07/owl#ObjectProperty"/>
  </rdf:Description>
  <rdf:Description rdf:about="http://vocab.getty.edu/ontology#ulan1516_great-grandchild_of">
    <rdf:type rdf:resource="http://www.w3.org/2002/07/owl#ObjectProperty"/>
    <dc:title>great-grandchild of - person</dc:title>
    <dct:description>person - great-grandchild of - person.&#13;
Example: Richard Benno Adam is the great-grandchild of Albrecht Adam</dct:description>
    <rdfs:range rdf:resource="http://www.w3.org/2004/02/skos/core#Concept"/>
    <dc:identifier>1516</dc:identifier>
    <rdfs:domain rdf:resource="http://www.w3.org/2004/02/skos/core#Concept"/>
    <skos:example>Richard Benno Adam is the great-grandchild of Albrecht Adam</skos:example>
    <rdfs:isDefinedBy rdf:resource="http://vocab.getty.edu/ontology"/>
    <skos:prefLabel>ulan1516_great-grandchild_of</skos:prefLabel>
    <rdfs:isDefinedBy rdf:resource="http://vocab.getty.edu/ulan/"/>
    <rdfs:subPropertyOf rdf:resource="http://www.w3.org/2004/02/skos/core#related"/>
  </rdf:Description>
  <rdf:Description rdf:about="http://vocab.getty.edu/ontology#tgn3412_predecessor_of">
    <skos:example>Persia is the predecessor of Iran (nation)</skos:example>
    <rdf:type rdf:resource="http://www.w3.org/2002/07/owl#ObjectProperty"/>
    <dc:identifier>3412</dc:identifier>
    <dct:description>nation - predecessor of - nation.&#13;
Example: Persia is the predecessor of Iran (nation)</dct:description>
    <rdfs:range rdf:resource="http://www.w3.org/2004/02/skos/core#Concept"/>
    <rdfs:domain rdf:resource="http://www.w3.org/2004/02/skos/core#Concept"/>
    <dc:title>predecessor of - nation</dc:title>
    <rdfs:subPropertyOf rdf:resource="http://www.w3.org/2004/02/skos/core#related"/>
    <rdfs:isDefinedBy rdf:resource="http://vocab.getty.edu/ontology"/>
    <skos:prefLabel>tgn3412_predecessor_of</skos:prefLabel>
    <rdfs:isDefinedBy rdf:resource="http://vocab.getty.edu/tgn/"/>
  </rdf:Description>
  <rdf:Description rdf:about="http://vocab.getty.edu/ontology#ulan1500_related_to">
    <dc:title>related to - person</dc:title>
    <dc:identifier>1500</dc:identifier>
    <rdfs:isDefinedBy rdf:resource="http://vocab.getty.edu/ulan/"/>
    <skos:example>Titian and Tizianello have a familial relationship with each other</skos:example>
    <rdf:type rdf:resource="http://www.w3.org/2002/07/owl#SymmetricProperty"/>
    <dct:description>person - related to (familial relationship) - person.&#13;
Example: Titian and Tizianello have a familial relationship with each other</dct:description>
    <rdfs:isDefinedBy rdf:resource="http://vocab.getty.edu/ontology"/>
    <rdfs:range rdf:resource="http://www.w3.org/2004/02/skos/core#Concept"/>
    <rdfs:domain rdf:resource="http://www.w3.org/2004/02/skos/core#Concept"/>
    <rdfs:subPropertyOf rdf:resource="http://www.w3.org/2004/02/skos/core#related"/>
    <skos:prefLabel>ulan1500_related_to</skos:prefLabel>
    <rdf:type rdf:resource="http://www.w3.org/2002/07/owl#ObjectProperty"/>
  </rdf:Description>
  <rdf:Description rdf:about="http://vocab.getty.edu/ontology#ulan1206_client_was">
    <rdf:type rdf:resource="http://www.w3.org/2002/07/owl#ObjectProperty"/>
    <dc:identifier>1206</dc:identifier>
    <skos:prefLabel>ulan1206_client_was</skos:prefLabel>
    <skos:example>Burnham and Root's client was the Chicago Herald</skos:example>
    <dc:title>client was - person/firm/family</dc:title>
    <rdfs:isDefinedBy rdf:resource="http://vocab.getty.edu/ontology"/>
    <dct:description>person/firm/family - client was - person/firm/family.&#13;
Example: Burnham and Root's client was the Chicago Herald</dct:description>
    <rdfs:domain rdf:resource="http://www.w3.org/2004/02/skos/core#Concept"/>
    <rdfs:subPropertyOf rdf:resource="http://www.w3.org/2004/02/skos/core#related"/>
    <rdfs:isDefinedBy rdf:resource="http://vocab.getty.edu/ulan/"/>
    <rdfs:range rdf:resource="http://www.w3.org/2004/02/skos/core#Concept"/>
  </rdf:Description>
  <rdf:Description rdf:about="http://vocab.getty.edu/ontology#ulan1005_possibly_identified_with">
    <rdfs:subPropertyOf rdf:resource="http://www.w3.org/2004/02/skos/core#related"/>
    <skos:example>Master of the Saint John Altarpiece is possibly identified with Hughe Jacobsz</skos:example>
    <skos:example>Bauart is possibly identified with Gruppe BAUart</skos:example>
    <skos:prefLabel>ulan1005_possibly_identified_with</skos:prefLabel>
    <rdfs:isDefinedBy rdf:resource="http://vocab.getty.edu/ulan/"/>
    <rdf:type rdf:resource="http://www.w3.org/2002/07/owl#SymmetricProperty"/>
    <rdfs:isDefinedBy rdf:resource="http://vocab.getty.edu/ontology"/>
    <rdfs:domain rdf:resource="http://www.w3.org/2004/02/skos/core#Concept"/>
    <rdfs:range rdf:resource="http://www.w3.org/2004/02/skos/core#Concept"/>
    <dc:title>possibly identified with - any</dc:title>
    <rdf:type rdf:resource="http://www.w3.org/2002/07/owl#ObjectProperty"/>
    <dct:description>any - possibly identified with - any.&#13;
Example: Master of the Saint John Altarpiece is possibly identified with Hughe Jacobsz; Bauart is possibly identified with Gruppe BAUart</dct:description>
    <dc:identifier>1005</dc:identifier>
  </rdf:Description>
  <rdf:Description rdf:about="http://vocab.getty.edu/ontology#Concept">
    <rdfs:subClassOf rdf:resource="http://www.w3.org/2004/02/skos/core#Concept"/>
    <rdfs:isDefinedBy rdf:resource="http://vocab.getty.edu/ontology"/>
    <skos:example>rhyta (AAT)</skos:example>
    <dct:description>Proper concept. Used in AAT only; TGN &amp; ULAN have their own, e.g. gvp:PhysPlaceConcept &amp; gvp:PersonConcept. Used for indexing and cataloguing.
Example: rhyta (AAT)</dct:description>
    <skos:prefLabel>Concept</skos:prefLabel>
    <rdf:type rdf:resource="http://www.w3.org/2002/07/owl#Class"/>
    <rdfs:comment>Proper concept. Used in AAT only; TGN &amp; ULAN have their own, e.g. gvp:PhysPlaceConcept &amp; gvp:PersonConcept. Used for indexing and cataloguing</rdfs:comment>
    <rdfs:label>Concept</rdfs:label>
    <rdfs:subClassOf rdf:resource="http://vocab.getty.edu/ontology#Subject"/>
  </rdf:Description>
  <rdf:Description rdf:about="http://vocab.getty.edu/ontology#aat2822_basis_of">
    <rdfs:subPropertyOf rdf:resource="http://www.w3.org/2004/02/skos/core#related"/>
    <rdfs:domain rdf:resource="http://www.w3.org/2004/02/skos/core#Concept"/>
    <dc:title>basis of - any</dc:title>
    <skos:example>curves (geometric figures) are the basis of curved [form attribute]</skos:example>
    <rdfs:isDefinedBy rdf:resource="http://vocab.getty.edu/ontology"/>
    <skos:example>plummets are the basis of pencils</skos:example>
    <rdfs:range rdf:resource="http://www.w3.org/2004/02/skos/core#Concept"/>
    <dct:description>any - [is] basis of - any.&#13;
Example: Gothic (Medieval) is the basis of Neo-Gothic; curves (geometric figures) are the basis of curved [form attribute]; plummets are the basis of pencils</dct:description>
    <skos:prefLabel>aat2822_basis_of</skos:prefLabel>
    <rdf:type rdf:resource="http://www.w3.org/2002/07/owl#ObjectProperty"/>
    <rdfs:isDefinedBy rdf:resource="http://vocab.getty.edu/aat/"/>
    <dc:identifier>2822</dc:identifier>
    <skos:example>Gothic (Medieval) is the basis of Neo-Gothic</skos:example>
  </rdf:Description>
  <rdf:Description rdf:about="http://vocab.getty.edu/ontology">
    <dct:creator rdf:resource="http://www.ontotext.com"/>
    <dc:format>meta/rdf-schema</dc:format>
    <owl:imports rdf:resource="http://www.w3.org/2004/02/skos/core"/>
    <owl:imports rdf:resource="http://purl.org/iso25964/skos-thes"/>
    <rdfs:seeAlso rdf:resource="http://vocab.getty.edu/.well-known/void"/>
    <vann:preferredNamespacePrefix>gvp</vann:preferredNamespacePrefix>
    <vann:preferredNamespaceUri>http://vocab.getty.edu/ontology#</vann:preferredNamespaceUri>
    <skos:changeNote rdf:resource="http://vocab.getty.edu/doc#Version_2.0"/>
    <rdfs:seeAlso rdf:resource="http://www.getty.edu/research/tools/vocabularies/lod/"/>
    <rdfs:seeAlso rdf:resource="http://lov.okfn.org/dataset/lov/details/vocabulary_gvp.html"/>
    <skos:changeNote>2.0 changes: replaced gvp:broaderTransitive with gvp:broaderExtended.
3.0 changes: replaced schema:startDate, endDate with gvp:estStart, estEnd; added ULAN). See details in referenced links.
3.1 &amp; 3.2: no changes.
3.3: added 6 associative relations: gvp:aat2886_used-function_as - gvp:aat2887_exemplified_by, gvp:tgn3103_located_on - gvp:tgn3104_is_location_of, and gvp:ulan2583_chairman_of - gvp:ulan2584_chaired_by</skos:changeNote>
    <skos:changeNote rdf:resource="http://vocab.getty.edu/doc#Version_3.0"/>
    <skos:changeNote rdf:resource="http://vocab.getty.edu/doc#Version_3.3"/>
    <rdf:type rdf:resource="http://purl.org/vocommons/voaf#Vocabulary"/>
    <rdfs:seeAlso rdf:resource="http://vocab.getty.edu/doc/queries"/>
    <dct:creator rdf:resource="http://www.getty.edu/research/"/>
    <rdfs:seeAlso rdf:resource="http://vocab.getty.edu/doc"/>
    <rdfs:label>Getty Vocabulary Program ontology</rdfs:label>
    <owl:versionInfo>3.3</owl:versionInfo>
    <owl:imports rdf:resource="http://www.w3.org/2008/05/skos-xl"/>
    <skos:prefLabel>Getty Vocabulary Program ontology</skos:prefLabel>
    <dct:issued rdf:datatype="http://www.w3.org/2001/XMLSchema#date">2014-02-20</dct:issued>
    <dct:modified rdf:datatype="http://www.w3.org/2001/XMLSchema#date">2016-04-25</dct:modified>
    <dct:created rdf:datatype="http://www.w3.org/2001/XMLSchema#date">2014-02-15</dct:created>
    <rdf:type rdf:resource="http://www.w3.org/2002/07/owl#Ontology"/>
    <rdfs:comment>The GVP Ontology defines classes, properties and values (skos:Concepts) used in GVP LOD.
As of version 3.0, it is complete regarding AAT, TGN and ULAN, and will be extended in time with more elements needed for other GVP vocabularies (CONA).
It uses the SKOS, SKOS-XL, ISO 25964; DC, DCT, BIBO, FOAF, BIO, Schema, PROV, WGS84 ontologies, but we import only the first 3</rdfs:comment>
  </rdf:Description>
  <rdf:Description rdf:about="http://vocab.getty.edu/ontology#ulan1102_student_of">
    <rdf:type rdf:resource="http://www.w3.org/2002/07/owl#ObjectProperty"/>
    <dc:identifier>1102</dc:identifier>
    <rdfs:range rdf:resource="http://www.w3.org/2004/02/skos/core#Concept"/>
    <skos:prefLabel>ulan1102_student_of</skos:prefLabel>
    <dc:title>student of - person</dc:title>
    <dct:description>person - student of - person.&#13;
Example: Pierre Subleyras was the student of Rivalz, Antoine</dct:description>
    <rdfs:domain rdf:resource="http://www.w3.org/2004/02/skos/core#Concept"/>
    <rdfs:isDefinedBy rdf:resource="http://vocab.getty.edu/ontology"/>
    <rdfs:isDefinedBy rdf:resource="http://vocab.getty.edu/ulan/"/>
    <rdfs:subPropertyOf rdf:resource="http://www.w3.org/2004/02/skos/core#related"/>
    <skos:example>Pierre Subleyras was the student of Rivalz, Antoine</skos:example>
  </rdf:Description>
  <rdf:Description rdf:about="http://vocab.getty.edu/ontology#ulan1218_employee_was">
    <rdf:type rdf:resource="http://www.w3.org/2002/07/owl#ObjectProperty"/>
    <skos:example>Jean Tijou was an employee of Christopher Wren</skos:example>
    <dc:identifier>1218</dc:identifier>
    <dct:description>person - employee was - person/firm.&#13;
Example: Jean Tijou was an employee of Christopher Wren</dct:description>
    <rdfs:subPropertyOf rdf:resource="http://www.w3.org/2004/02/skos/core#related"/>
    <rdfs:isDefinedBy rdf:resource="http://vocab.getty.edu/ulan/"/>
    <rdfs:isDefinedBy rdf:resource="http://vocab.getty.edu/ontology"/>
    <rdfs:domain rdf:resource="http://www.w3.org/2004/02/skos/core#Concept"/>
    <dc:title>employee was - person/firm</dc:title>
    <rdfs:range rdf:resource="http://www.w3.org/2004/02/skos/core#Concept"/>
    <skos:prefLabel>ulan1218_employee_was</skos:prefLabel>
  </rdf:Description>
  <rdf:Description rdf:about="http://vocab.getty.edu/ontology#estStart">
    <rdfs:label>estStart</rdfs:label>
    <dct:description>Estimated start date of term, relation, type assignment, event, biography</dct:description>
    <rdf:type rdf:resource="http://www.w3.org/2002/07/owl#DatatypeProperty"/>
    <rdfs:comment>Estimated start date of term, relation, type assignment, event, biography</rdfs:comment>
    <skos:prefLabel>estStart</skos:prefLabel>
    <rdfs:isDefinedBy rdf:resource="http://vocab.getty.edu/ontology"/>
  </rdf:Description>
  <rdf:Description rdf:nodeID="N5b11eeca07364f4c9e3107ce462b4750">
    <rdf:rest rdf:resource="http://www.w3.org/1999/02/22-rdf-syntax-ns#nil"/>
    <rdf:first rdf:resource="http://vocab.getty.edu/ontology#broaderGeneric"/>
  </rdf:Description>
  <rdf:Description rdf:about="http://vocab.getty.edu/ontology#tgn3103_located_on">
    <owl:inverseOf rdf:resource="http://vocab.getty.edu/ontology#tgn3104_is_location_of"/>
    <skos:prefLabel>tgn3103_located_on</skos:prefLabel>
    <rdfs:subPropertyOf rdf:resource="http://www.w3.org/2004/02/skos/core#related"/>
    <rdfs:isDefinedBy rdf:resource="http://vocab.getty.edu/ontology"/>
    <dc:title>located on - place</dc:title>
    <skos:example>tgn:7018835 Palmyra is located on tgn:7031416 Silk Road</skos:example>
    <rdfs:isDefinedBy rdf:resource="http://vocab.getty.edu/tgn/"/>
    <rdf:type rdf:resource="http://www.w3.org/2002/07/owl#ObjectProperty"/>
    <dct:description>place - located on - place.&#13;
Example: tgn:7018835 Palmyra is located on tgn:7031416 Silk Road</dct:description>
    <dc:identifier>3103</dc:identifier>
    <rdfs:range rdf:resource="http://www.w3.org/2004/02/skos/core#Concept"/>
    <rdfs:domain rdf:resource="http://www.w3.org/2004/02/skos/core#Concept"/>
  </rdf:Description>
  <rdf:Description rdf:about="http://vocab.getty.edu/ontology#broaderPreferredExtended">
    <rdfs:label>broaderPreferredExtended</rdfs:label>
    <rdfs:domain rdf:resource="http://vocab.getty.edu/ontology#Subject"/>
    <skos:prefLabel>broaderPreferredExtended</skos:prefLabel>
    <rdf:type rdf:resource="http://www.w3.org/2002/07/owl#ObjectProperty"/>
    <dct:description>Preferred Ancestors. Meaningful closure of gvp:broaderPreferred. Needed to display the hierarchy.
Example: Mt Athos has preferred ancestor places (BTPE) World, Europe, Greece, Macedonia, Pangaíon Óros regional division;
and prefererd place type (BTIE) inhabited place</dct:description>
    <rdfs:comment>Preferred Ancestors. Meaningful closure of gvp:broaderPreferred. Needed to display the hierarchy</rdfs:comment>
    <rdfs:range rdf:resource="http://vocab.getty.edu/ontology#Subject"/>
    <skos:example>Mt Athos has preferred ancestor places (BTPE) World, Europe, Greece, Macedonia, Pangaíon Óros regional division;
and prefererd place type (BTIE) inhabited place</skos:example>
    <rdfs:isDefinedBy rdf:resource="http://vocab.getty.edu/ontology"/>
  </rdf:Description>
  <rdf:Description rdf:about="http://vocab.getty.edu/ontology#aat2504_used-located_in">
    <dc:title>used/located in - locus/setting</dc:title>
    <rdf:type rdf:resource="http://www.w3.org/2002/07/owl#ObjectProperty"/>
    <rdfs:isDefinedBy rdf:resource="http://vocab.getty.edu/aat/"/>
    <rdfs:range rdf:resource="http://www.w3.org/2004/02/skos/core#Concept"/>
    <skos:prefLabel>aat2504_used-located_in</skos:prefLabel>
    <rdfs:domain rdf:resource="http://www.w3.org/2004/02/skos/core#Concept"/>
    <skos:example>brick (clay product) is used/located in brickworks (factories)</skos:example>
    <dct:description>material - [is] used/located in - locus/setting.&#13;
Example: tephra is used/located in [at] volcanoes; brick (clay product) is used/located in brickworks (factories)</dct:description>
    <skos:example>tephra is used/located in [at] volcanoes</skos:example>
    <owl:inverseOf rdf:resource="http://vocab.getty.edu/ontology#aat2505_locus-setting_for"/>
    <rdfs:isDefinedBy rdf:resource="http://vocab.getty.edu/ontology"/>
    <rdfs:subPropertyOf rdf:resource="http://www.w3.org/2004/02/skos/core#related"/>
    <dc:identifier>2504</dc:identifier>
  </rdf:Description>
  <rdf:Description rdf:about="http://vocab.getty.edu/ontology#ulan1003_associated_with">
    <dc:title>associated with - any</dc:title>
    <rdfs:domain rdf:resource="http://www.w3.org/2004/02/skos/core#Concept"/>
    <rdfs:isDefinedBy rdf:resource="http://vocab.getty.edu/ontology"/>
    <rdfs:range rdf:resource="http://www.w3.org/2004/02/skos/core#Concept"/>
    <dc:identifier>1003</dc:identifier>
    <skos:prefLabel>ulan1003_associated_with</skos:prefLabel>
    <skos:example>United Nations is associated with World Bank</skos:example>
    <rdf:type rdf:resource="http://www.w3.org/2002/07/owl#ObjectProperty"/>
    <skos:example>Richard Meier is associated with Renny B.Saltzman</skos:example>
    <rdfs:isDefinedBy rdf:resource="http://vocab.getty.edu/ulan/"/>
    <rdfs:subPropertyOf rdf:resource="http://www.w3.org/2004/02/skos/core#related"/>
    <dct:description>any - associated with - any.&#13;
Example: Richard Meier is associated with Renny B.Saltzman; United Nations is associated with World Bank</dct:description>
    <rdf:type rdf:resource="http://www.w3.org/2002/07/owl#SymmetricProperty"/>
  </rdf:Description>
  <rdf:Description rdf:about="http://vocab.getty.edu/ontology#aat2281_have_counterpart">
    <rdfs:domain rdf:resource="http://www.w3.org/2004/02/skos/core#Concept"/>
    <skos:prefLabel>aat2281_have_counterpart</skos:prefLabel>
    <skos:example>duchesses have counterpart dukes</skos:example>
    <rdf:type rdf:resource="http://www.w3.org/2002/07/owl#ObjectProperty"/>
    <rdfs:isDefinedBy rdf:resource="http://vocab.getty.edu/aat/"/>
    <dc:title>have counterpart - role</dc:title>
    <dc:identifier>2281</dc:identifier>
    <dct:description>role -[is] counterpart to - role.&#13;
Example: duchesses have counterpart dukes; godesses have counterpart gods</dct:description>
    <rdfs:subPropertyOf rdf:resource="http://www.w3.org/2004/02/skos/core#related"/>
    <skos:example>godesses have counterpart gods</skos:example>
    <rdfs:range rdf:resource="http://www.w3.org/2004/02/skos/core#Concept"/>
    <rdfs:isDefinedBy rdf:resource="http://vocab.getty.edu/ontology"/>
    <rdf:type rdf:resource="http://www.w3.org/2002/07/owl#SymmetricProperty"/>
  </rdf:Description>
  <rdf:Description rdf:about="http://vocab.getty.edu/ontology#tgn3411_successor_of">
    <owl:inverseOf rdf:resource="http://vocab.getty.edu/ontology#tgn3412_predecessor_of"/>
    <rdfs:isDefinedBy rdf:resource="http://vocab.getty.edu/tgn/"/>
    <skos:example>Iran (nation) is the successor of Persia</skos:example>
    <rdfs:domain rdf:resource="http://www.w3.org/2004/02/skos/core#Concept"/>
    <dc:identifier>3411</dc:identifier>
    <rdfs:range rdf:resource="http://www.w3.org/2004/02/skos/core#Concept"/>
    <rdfs:isDefinedBy rdf:resource="http://vocab.getty.edu/ontology"/>
    <skos:prefLabel>tgn3411_successor_of</skos:prefLabel>
    <dct:description>nation - successor of - nation.&#13;
Example: Iran (nation) is the successor of Persia</dct:description>
    <dc:title>successor of - nation</dc:title>
    <rdf:type rdf:resource="http://www.w3.org/2002/07/owl#ObjectProperty"/>
    <rdfs:subPropertyOf rdf:resource="http://www.w3.org/2004/02/skos/core#related"/>
  </rdf:Description>
  <rdf:Description rdf:about="http://vocab.getty.edu/term/kind/Neologism">
    <skos:inScheme rdf:resource="http://vocab.getty.edu/term/kind/"/>
    <rdf:type rdf:resource="http://www.w3.org/2004/02/skos/core#Concept"/>
    <skos:example>"folksonomy", "podcasting"</skos:example>
    <skos:notation>N</skos:notation>
    <skos:prefLabel>Neologism</skos:prefLabel>
    <skos:scopeNote>Term that is new to the language, generally having been coined due to new technology. Used in AAT only.</skos:scopeNote>
    <dct:description>Term that is new to the language, generally having been coined due to new technology. Used in AAT only..
Example: "folksonomy", "podcasting"</dct:description>
  </rdf:Description>
  <rdf:Description rdf:about="http://vocab.getty.edu/ontology#aat2318_involved_in">
    <skos:prefLabel>aat2318_involved_in</skos:prefLabel>
    <rdf:type rdf:resource="http://www.w3.org/2002/07/owl#ObjectProperty"/>
    <rdfs:domain rdf:resource="http://www.w3.org/2004/02/skos/core#Concept"/>
    <rdfs:isDefinedBy rdf:resource="http://vocab.getty.edu/aat/"/>
    <rdfs:isDefinedBy rdf:resource="http://vocab.getty.edu/ontology"/>
    <rdfs:range rdf:resource="http://www.w3.org/2004/02/skos/core#Concept"/>
    <skos:example>bridegrooms are involved in weddings</skos:example>
    <owl:inverseOf rdf:resource="http://vocab.getty.edu/ontology#aat2319_involves"/>
    <dct:description>[actors having] role -[are] involved - activity/event.&#13;
Example: bridegrooms are involved in weddings; martyrs are involved in martyrdoms</dct:description>
    <dc:identifier>2318</dc:identifier>
    <rdfs:subPropertyOf rdf:resource="http://www.w3.org/2004/02/skos/core#related"/>
    <skos:example>martyrs are involved in martyrdoms</skos:example>
    <dc:title>involved in - activity/event</dc:title>
  </rdf:Description>
  <rdf:Description rdf:about="http://vocab.getty.edu/ontology#aat2100_distinguished_from">
    <dc:title>distinguished from - any</dc:title>
    <rdfs:subPropertyOf rdf:resource="http://www.w3.org/2004/02/skos/core#related"/>
    <skos:prefLabel>aat2100_distinguished_from</skos:prefLabel>
    <rdfs:domain rdf:resource="http://www.w3.org/2004/02/skos/core#Concept"/>
    <rdf:type rdf:resource="http://www.w3.org/2002/07/owl#SymmetricProperty"/>
    <rdfs:isDefinedBy rdf:resource="http://vocab.getty.edu/ontology"/>
    <dct:description>any - distinguished from - any.&#13;
Example: historic farms are distinguished from abandoned farms; naive art is distinguished from outsider art</dct:description>
    <rdfs:range rdf:resource="http://www.w3.org/2004/02/skos/core#Concept"/>
    <skos:example>historic farms are distinguished from abandoned farms</skos:example>
    <skos:example>naive art is distinguished from outsider art</skos:example>
    <rdf:type rdf:resource="http://www.w3.org/2002/07/owl#ObjectProperty"/>
    <rdfs:isDefinedBy rdf:resource="http://vocab.getty.edu/aat/"/>
    <dc:identifier>2100</dc:identifier>
  </rdf:Description>
  <rdf:Description rdf:about="http://vocab.getty.edu/ontology#qualifier">
    <rdfs:comment>Clarifies and disambiguates terms with the same spelling but different meaning.
Appended in parentheses to gvp:term, forming skosxsl:literalForm.
Every qualifier is in the same language as the term</rdfs:comment>
    <rdfs:domain rdf:resource="http://www.w3.org/2008/05/skos-xl#Label"/>
    <dct:description>Clarifies and disambiguates terms with the same spelling but different meaning.
Appended in parentheses to gvp:term, forming skosxsl:literalForm.
Every qualifier is in the same language as the term.
Example: "Rhea (vessels)"=rhyta (a kind of drinking vessel) vs "Rhea (species)"=Boehmeria nivea (Chinese grass)</dct:description>
    <rdfs:isDefinedBy rdf:resource="http://vocab.getty.edu/ontology"/>
    <rdfs:range rdf:resource="http://www.w3.org/1999/02/22-rdf-syntax-ns#Literal"/>
    <skos:prefLabel>qualifier</skos:prefLabel>
    <rdf:type rdf:resource="http://www.w3.org/2002/07/owl#DatatypeProperty"/>
    <skos:example>Rhea (vessels)=rhyta (a kind of drinking vessel) vs rhea (species)=Boehmeria nivea (Chinese grass)</skos:example>
    <rdfs:label>qualifier</rdfs:label>
  </rdf:Description>
  <rdf:Description rdf:about="http://vocab.getty.edu/ontology#aat2812_followed">
    <rdfs:isDefinedBy rdf:resource="http://vocab.getty.edu/aat/"/>
    <rdfs:isDefinedBy rdf:resource="http://vocab.getty.edu/ontology"/>
    <rdfs:domain rdf:resource="http://www.w3.org/2004/02/skos/core#Concept"/>
    <dct:description>style/period/culture/[religion/ideology] - followed  - style/period/culture/[religion/ideology].&#13;
Example: Abstract Impressionism followed Impressionist; Micoquian followed Acheulian</dct:description>
    <rdfs:subPropertyOf rdf:resource="http://www.w3.org/2004/02/skos/core#related"/>
    <rdfs:range rdf:resource="http://www.w3.org/2004/02/skos/core#Concept"/>
    <skos:prefLabel>aat2812_followed</skos:prefLabel>
    <skos:example>Abstract Impressionism followed Impressionist</skos:example>
    <rdf:type rdf:resource="http://www.w3.org/2002/07/owl#ObjectProperty"/>
    <skos:example>Micoquian followed Acheulian</skos:example>
    <dc:identifier>2812</dc:identifier>
    <dc:title>followed - style/period/culture</dc:title>
  </rdf:Description>
  <rdf:Description rdf:about="http://vocab.getty.edu/ontology#aat2884_involved_with">
    <skos:example>climate is involved with climate change</skos:example>
    <skos:example>insect damage is involved with infestation</skos:example>
    <rdfs:subPropertyOf rdf:resource="http://www.w3.org/2004/02/skos/core#related"/>
    <rdfs:isDefinedBy rdf:resource="http://vocab.getty.edu/ontology"/>
    <dc:identifier>2884</dc:identifier>
    <rdfs:domain rdf:resource="http://www.w3.org/2004/02/skos/core#Concept"/>
    <rdfs:range rdf:resource="http://www.w3.org/2004/02/skos/core#Concept"/>
    <skos:example>Celtic crosses (design motif) are involved with Celtic culture</skos:example>
    <owl:inverseOf rdf:resource="http://vocab.getty.edu/ontology#aat2885_involves"/>
    <rdf:type rdf:resource="http://www.w3.org/2002/07/owl#ObjectProperty"/>
    <skos:prefLabel>aat2884_involved_with</skos:prefLabel>
    <dc:title>involved with - any</dc:title>
    <dct:description>attributes /associated concepts - [are] involved with - any.&#13;
Example: climate is involved with climate change; insect damage is involved with infestation; Celtic crosses (design motif) are involved with Celtic culture</dct:description>
    <rdfs:isDefinedBy rdf:resource="http://vocab.getty.edu/aat/"/>
  </rdf:Description>
  <rdf:Description rdf:about="http://vocab.getty.edu/ontology#ulan1000_related_to">
    <dct:description>any - related to - any.&#13;
Example: Frank Lloyd Wright is related to Francis Conroy Sullivan; Herman Miller, Inc. is related to Irving Harper; National Endowment for the Humanities is related to Connecticut Humanities Council</dct:description>
    <rdfs:range rdf:resource="http://www.w3.org/2004/02/skos/core#Concept"/>
    <dc:identifier>1000</dc:identifier>
    <rdfs:subPropertyOf rdf:resource="http://www.w3.org/2004/02/skos/core#related"/>
    <rdf:type rdf:resource="http://www.w3.org/2002/07/owl#ObjectProperty"/>
    <skos:prefLabel>ulan1000_related_to</skos:prefLabel>
    <rdf:type rdf:resource="http://www.w3.org/2002/07/owl#SymmetricProperty"/>
    <skos:example>Herman Miller, Inc. is related to Irving Harper</skos:example>
    <rdfs:isDefinedBy rdf:resource="http://vocab.getty.edu/ulan/"/>
    <dc:title>related to - any</dc:title>
    <rdfs:domain rdf:resource="http://www.w3.org/2004/02/skos/core#Concept"/>
    <skos:example>Frank Lloyd Wright is related to Francis Conroy Sullivan</skos:example>
    <rdfs:isDefinedBy rdf:resource="http://vocab.getty.edu/ontology"/>
    <skos:example>National Endowment for the Humanities is related to Connecticut Humanities Council</skos:example>
  </rdf:Description>
  <rdf:Description rdf:nodeID="N1ebab3ef3fac45408d3bd583c808ce8a">
    <rdf:first rdf:resource="http://www.w3.org/2008/05/skos-xl#prefLabel"/>
    <rdf:rest rdf:nodeID="N9dc1cffb8d29482c9c782a05a2048ce7"/>
  </rdf:Description>
  <rdf:Description rdf:about="http://vocab.getty.edu/ontology#aat2605_possess-exist_in">
    <rdfs:domain rdf:resource="http://www.w3.org/2004/02/skos/core#Concept"/>
    <dc:identifier>2605</dc:identifier>
    <skos:example>ruins possess/exist in ruined [contition]</skos:example>
    <skos:example>boudoir photographs possess/exist in boudoir (photograph size)</skos:example>
    <rdf:type rdf:resource="http://www.w3.org/2002/07/owl#ObjectProperty"/>
    <rdfs:subPropertyOf rdf:resource="http://www.w3.org/2004/02/skos/core#related"/>
    <dct:description>things - possess/exist in - attributes /associated concepts.&#13;
Example: boudoir photographs possess/exist in boudoir (photograph size); ruins possess/exist in ruined [contition]</dct:description>
    <dc:title>possess/exist in - attributes /associated concepts</dc:title>
    <rdfs:range rdf:resource="http://www.w3.org/2004/02/skos/core#Concept"/>
    <rdfs:isDefinedBy rdf:resource="http://vocab.getty.edu/aat/"/>
    <skos:prefLabel>aat2605_possess-exist_in</skos:prefLabel>
    <rdfs:isDefinedBy rdf:resource="http://vocab.getty.edu/ontology"/>
  </rdf:Description>
  <rdf:Description rdf:about="http://vocab.getty.edu/ontology#eventNonPreferred">
    <rdfs:comment>Non-preferred life event of an ULAN agent. Domain is schema:Person/Organization, range is bio:Event</rdfs:comment>
    <dct:description>Non-preferred life event of an ULAN agent. Domain is schema:Person/Organization, range is bio:Event</dct:description>
    <skos:prefLabel>eventNonPreferred</skos:prefLabel>
    <rdfs:label>eventNonPreferred</rdfs:label>
    <rdfs:range rdf:resource="http://purl.org/vocab/bio/0.1/Event"/>
    <rdfs:isDefinedBy rdf:resource="http://vocab.getty.edu/ontology"/>
    <rdfs:subPropertyOf rdf:resource="http://purl.org/vocab/bio/0.1/event"/>
    <rdf:type rdf:resource="http://www.w3.org/2002/07/owl#ObjectProperty"/>
  </rdf:Description>
  <rdf:Description rdf:about="http://vocab.getty.edu/ontology#aat2428_produces">
    <dct:description>activity/event/process - produces - things.&#13;
Example: vase painting (image making) produces vase paintings (visual works); forging (copying) produces forgeries</dct:description>
    <rdfs:domain rdf:resource="http://www.w3.org/2004/02/skos/core#Concept"/>
    <skos:example>forging (copying) produces forgeries</skos:example>
    <skos:example>vase painting (image making) produces vase paintings (visual works)</skos:example>
    <rdfs:isDefinedBy rdf:resource="http://vocab.getty.edu/ontology"/>
    <dc:identifier>2428</dc:identifier>
    <rdfs:range rdf:resource="http://www.w3.org/2004/02/skos/core#Concept"/>
    <dc:title>produces - things</dc:title>
    <rdfs:isDefinedBy rdf:resource="http://vocab.getty.edu/aat/"/>
    <skos:prefLabel>aat2428_produces</skos:prefLabel>
    <rdfs:subPropertyOf rdf:resource="http://www.w3.org/2004/02/skos/core#related"/>
    <rdf:type rdf:resource="http://www.w3.org/2002/07/owl#ObjectProperty"/>
  </rdf:Description>
  <rdf:Description rdf:nodeID="N6fafbb3f5a524fde95f35d19565c2579">
    <rdf:rest rdf:nodeID="N2a7944f25ea0429e8be3f707b7513b55"/>
    <rdf:first rdf:resource="http://vocab.getty.edu/ontology#broaderGeneric"/>
  </rdf:Description>
  <rdf:Description rdf:nodeID="N731c9cb66cef4e658afa515d3206747b">
    <rdf:first rdf:resource="http://vocab.getty.edu/ontology#broaderPartitiveExtended"/>
    <rdf:rest rdf:nodeID="N0e7c8cba70fe4e7cb81d6f70b73e2d46"/>
  </rdf:Description>
  <rdf:Description rdf:about="http://vocab.getty.edu/ontology#aat2552_reflected_in-produces">
    <dct:description>style/period/culture/[religion/ideology] - [is] reflected in/produces - things.&#13;
Example: Nasca [culture] produces/is reflected in Nasca lines; Judaism produces/is reflected in Judaica</dct:description>
    <rdfs:subPropertyOf rdf:resource="http://www.w3.org/2004/02/skos/core#related"/>
    <rdfs:isDefinedBy rdf:resource="http://vocab.getty.edu/ontology"/>
    <skos:example>Nasca [culture] produces/is reflected in Nasca lines</skos:example>
    <rdfs:isDefinedBy rdf:resource="http://vocab.getty.edu/aat/"/>
    <rdfs:domain rdf:resource="http://www.w3.org/2004/02/skos/core#Concept"/>
    <dc:title>reflected in/produces - things</dc:title>
    <rdf:type rdf:resource="http://www.w3.org/2002/07/owl#ObjectProperty"/>
    <dc:identifier>2552</dc:identifier>
    <rdfs:range rdf:resource="http://www.w3.org/2004/02/skos/core#Concept"/>
    <skos:prefLabel>aat2552_reflected_in-produces</skos:prefLabel>
    <skos:example>Judaism produces/is reflected in Judaica</skos:example>
  </rdf:Description>
  <rdf:Description rdf:nodeID="N902632d785fc4cb0b1919bc211810e50">
    <rdf:rest rdf:resource="http://www.w3.org/1999/02/22-rdf-syntax-ns#nil"/>
    <rdf:first rdf:resource="http://www.w3.org/2008/05/skos-xl#literalForm"/>
  </rdf:Description>
  <rdf:Description rdf:about="http://vocab.getty.edu/ontology#aat2415_required_for">
    <skos:example>dye is required for dying</skos:example>
    <rdfs:domain rdf:resource="http://www.w3.org/2004/02/skos/core#Concept"/>
    <owl:inverseOf rdf:resource="http://vocab.getty.edu/ontology#aat2416_requires"/>
    <rdfs:range rdf:resource="http://www.w3.org/2004/02/skos/core#Concept"/>
    <rdfs:isDefinedBy rdf:resource="http://vocab.getty.edu/ontology"/>
    <dct:description>material - [is] required for - activity/event/[process/function].&#13;
Example: dye is required for dying; pewter is required for pewtersmithing</dct:description>
    <skos:prefLabel>aat2415_required_for</skos:prefLabel>
    <rdfs:isDefinedBy rdf:resource="http://vocab.getty.edu/aat/"/>
    <dc:identifier>2415</dc:identifier>
    <skos:example>pewter is required for pewtersmithing</skos:example>
    <dc:title>required for - activity/event</dc:title>
    <rdf:type rdf:resource="http://www.w3.org/2002/07/owl#ObjectProperty"/>
    <rdfs:subPropertyOf rdf:resource="http://www.w3.org/2004/02/skos/core#related"/>
  </rdf:Description>
  <rdf:Description rdf:about="http://vocab.getty.edu/ontology#ulan2579_trustee_was">
    <rdfs:isDefinedBy rdf:resource="http://vocab.getty.edu/ulan/"/>
    <skos:prefLabel>ulan2579_trustee_was</skos:prefLabel>
    <rdfs:subPropertyOf rdf:resource="http://www.w3.org/2004/02/skos/core#related"/>
    <rdf:type rdf:resource="http://www.w3.org/2002/07/owl#ObjectProperty"/>
    <dc:identifier>2579</dc:identifier>
    <dct:description>institution - trustee was - person.&#13;
Example: National Galleries of Scotland trustee was George Douglas Haig</dct:description>
    <dc:title>trustee was - person</dc:title>
    <rdfs:domain rdf:resource="http://www.w3.org/2004/02/skos/core#Concept"/>
    <rdfs:range rdf:resource="http://www.w3.org/2004/02/skos/core#Concept"/>
    <rdfs:isDefinedBy rdf:resource="http://vocab.getty.edu/ontology"/>
    <skos:example>National Galleries of Scotland trustee was George Douglas Haig</skos:example>
  </rdf:Description>
  <rdf:Description rdf:about="http://vocab.getty.edu/ontology#aat2294_locus-setting_for">
    <dc:identifier>2294</dc:identifier>
    <rdf:type rdf:resource="http://www.w3.org/2002/07/owl#ObjectProperty"/>
    <skos:example>nations are the locus/setting for national capitals</skos:example>
    <rdfs:range rdf:resource="http://www.w3.org/2004/02/skos/core#Concept"/>
    <rdfs:isDefinedBy rdf:resource="http://vocab.getty.edu/aat/"/>
    <dc:title>locus/setting for - locus/setting</dc:title>
    <rdfs:subPropertyOf rdf:resource="http://www.w3.org/2004/02/skos/core#related"/>
    <rdfs:domain rdf:resource="http://www.w3.org/2004/02/skos/core#Concept"/>
    <dct:description>locus/setting - [is] locus setting for - locus/setting.&#13;
Example: nations are the locus/setting for national capitals; mountain ranges are the locus/setting for mountains</dct:description>
    <skos:example>mountain ranges are the locus/setting for mountains</skos:example>
    <rdfs:isDefinedBy rdf:resource="http://vocab.getty.edu/ontology"/>
    <skos:prefLabel>aat2294_locus-setting_for</skos:prefLabel>
    <owl:inverseOf rdf:resource="http://vocab.getty.edu/ontology#aat2295_located_in"/>
  </rdf:Description>
  <rdf:Description rdf:about="http://vocab.getty.edu/ontology#ulan1512_parent_of">
    <rdfs:isDefinedBy rdf:resource="http://vocab.getty.edu/ulan/"/>
    <rdfs:subPropertyOf rdf:resource="http://www.w3.org/2004/02/skos/core#related"/>
    <rdfs:domain rdf:resource="http://www.w3.org/2004/02/skos/core#Concept"/>
    <dc:title>parent of - person</dc:title>
    <rdfs:isDefinedBy rdf:resource="http://vocab.getty.edu/ontology"/>
    <dc:identifier>1512</dc:identifier>
    <skos:example>Rembrandt van Rijn is the parent of Rumbertus van Rijn</skos:example>
    <rdfs:range rdf:resource="http://www.w3.org/2004/02/skos/core#Concept"/>
    <skos:prefLabel>ulan1512_parent_of</skos:prefLabel>
    <rdf:type rdf:resource="http://www.w3.org/2002/07/owl#ObjectProperty"/>
    <dct:description>person - parent of - person.&#13;
Example: Rembrandt van Rijn is the parent of Rumbertus van Rijn</dct:description>
  </rdf:Description>
  <rdf:Description rdf:about="http://vocab.getty.edu/historic/historic">
    <skos:prefLabel>Historic</skos:prefLabel>
    <skos:scopeNote>Valid/used in the past but not currently</skos:scopeNote>
    <skos:example>"Lutetia" is a historic name for "Paris" (TGN). "weyneschot" is a 16th-century spelling for "wainscoting" (AAT)</skos:example>
    <rdf:type rdf:resource="http://www.w3.org/2004/02/skos/core#Concept"/>
    <dct:description>Valid/used in the past but not currently.
Example: "Lutetia" is a historic name for "Paris" (TGN). "weyneschot" is a 16th-century spelling for "wainscoting" (AAT)</dct:description>
    <skos:notation>H</skos:notation>
    <skos:inScheme rdf:resource="http://vocab.getty.edu/historic/"/>
  </rdf:Description>
  <rdf:Description rdf:about="http://vocab.getty.edu/historic/currentAndHistoric">
    <rdf:type rdf:resource="http://www.w3.org/2004/02/skos/core#Concept"/>
    <skos:notation>B</skos:notation>
    <skos:example>Saint Petersburg (TGN)</skos:example>
    <skos:inScheme rdf:resource="http://vocab.getty.edu/historic/"/>
    <skos:scopeNote>Valid/used both in the past and currently</skos:scopeNote>
    <dct:description>Valid/used both in the past and currently.
Example: Saint Petersburg (TGN)</dct:description>
    <skos:prefLabel>Both Current and Historic</skos:prefLabel>
  </rdf:Description>
  <rdf:Description rdf:about="http://vocab.getty.edu/ontology#aat2206_caused_by-requires">
    <rdfs:isDefinedBy rdf:resource="http://vocab.getty.edu/ontology"/>
    <dc:identifier>2206</dc:identifier>
    <skos:example>on-demand publishing is caused by/requires on-demand printing</skos:example>
    <dct:description>activity/event/[process/function] - [is] caused by/dependent upon - activity/event/[process/function].&#13;
Example: on-demand publishing is caused by/requires on-demand printing; preservation is caused by/requires preserving</dct:description>
    <rdfs:subPropertyOf rdf:resource="http://www.w3.org/2004/02/skos/core#related"/>
    <rdf:type rdf:resource="http://www.w3.org/2002/07/owl#ObjectProperty"/>
    <rdfs:isDefinedBy rdf:resource="http://vocab.getty.edu/aat/"/>
    <skos:prefLabel>aat2206_caused_by-requires</skos:prefLabel>
    <dc:title>caused by/requires - activity/event</dc:title>
    <rdfs:range rdf:resource="http://www.w3.org/2004/02/skos/core#Concept"/>
    <skos:example>preservation is caused by/requires preserving</skos:example>
    <rdfs:domain rdf:resource="http://www.w3.org/2004/02/skos/core#Concept"/>
  </rdf:Description>
  <rdf:Description rdf:about="http://vocab.getty.edu/ontology#ulan2572_founder_of">
    <rdfs:domain rdf:resource="http://www.w3.org/2004/02/skos/core#Concept"/>
    <owl:inverseOf rdf:resource="http://vocab.getty.edu/ontology#ulan2573_founded_by"/>
    <dc:identifier>2572</dc:identifier>
    <rdf:type rdf:resource="http://www.w3.org/2002/07/owl#ObjectProperty"/>
    <skos:prefLabel>ulan2572_founder_of</skos:prefLabel>
    <dct:description>person - founder of - institution.&#13;
Example: Louis Comfort Tiffany was the founder of Tiffany Glass &amp; Decorating Company</dct:description>
    <rdfs:subPropertyOf rdf:resource="http://www.w3.org/2004/02/skos/core#related"/>
    <rdfs:isDefinedBy rdf:resource="http://vocab.getty.edu/ulan/"/>
    <skos:example>Louis Comfort Tiffany was the founder of Tiffany Glass &amp; Decorating Company</skos:example>
    <rdfs:range rdf:resource="http://www.w3.org/2004/02/skos/core#Concept"/>
    <rdfs:isDefinedBy rdf:resource="http://vocab.getty.edu/ontology"/>
    <dc:title>founder of - institution</dc:title>
  </rdf:Description>
  <rdf:Description rdf:about="http://vocab.getty.edu/ulan/">
    <rdf:type rdf:resource="http://www.w3.org/2004/02/skos/core#ConceptScheme"/>
    <foaf:homepage rdf:resource="http://www.getty.edu/research/tools/vocabularies/ulan/"/>
    <rdfs:comment>The Union List of Artist Names concept scheme</rdfs:comment>
    <rdfs:seeAlso rdf:resource="http://vocab.getty.edu/"/>
    <rdfs:seeAlso rdf:resource="http://www.getty.edu/research/tools/vocabularies/lod/"/>
    <dct:created rdf:datatype="http://www.w3.org/2001/XMLSchema#date">2015-03-25</dct:created>
    <vann:preferredNamespaceUri>http://vocab.getty.edu/ulan/</vann:preferredNamespaceUri>
    <vann:preferredNamespacePrefix>ulan</vann:preferredNamespacePrefix>
    <dct:creator rdf:resource="http://www.getty.edu/research/"/>
    <dct:creator rdf:resource="http://www.ontotext.com"/>
    <skos:prefLabel>Union List of Artist Names</skos:prefLabel>
    <rdfs:label>Union List of Artist Names</rdfs:label>
    <rdfs:seeAlso rdf:resource="http://vocab.getty.edu/.well-known/void"/>
  </rdf:Description>
  <rdf:Description rdf:about="http://vocab.getty.edu/ontology#termKind">
    <rdf:type rdf:resource="http://www.w3.org/2002/07/owl#ObjectProperty"/>
    <rdfs:isDefinedBy rdf:resource="http://vocab.getty.edu/ontology"/>
    <dct:description>Term Kind</dct:description>
    <skos:prefLabel>termKind</skos:prefLabel>
    <rdfs:label>termKind</rdfs:label>
    <rdfs:range rdf:resource="http://www.w3.org/2004/02/skos/core#Concept"/>
    <rdfs:domain rdf:resource="http://www.w3.org/2008/05/skos-xl#Label"/>
  </rdf:Description>
  <rdf:Description rdf:about="http://vocab.getty.edu/ontology#tgn3006_formerly_identified_as">
    <rdfs:isDefinedBy rdf:resource="http://vocab.getty.edu/tgn/"/>
    <dc:title>formerly identified as - place</dc:title>
    <skos:scopeNote>New</skos:scopeNote>
    <dc:identifier>3006</dc:identifier>
    <skos:prefLabel>tgn3006_formerly_identified_as</skos:prefLabel>
    <rdf:type rdf:resource="http://www.w3.org/2002/07/owl#SymmetricProperty"/>
    <rdfs:range rdf:resource="http://www.w3.org/2004/02/skos/core#Concept"/>
    <rdfs:isDefinedBy rdf:resource="http://vocab.getty.edu/ontology"/>
    <skos:example>The deserted settlement of Machupicchu was formerly identified as Tampu Tocco</skos:example>
    <rdfs:domain rdf:resource="http://www.w3.org/2004/02/skos/core#Concept"/>
    <rdfs:subPropertyOf rdf:resource="http://www.w3.org/2004/02/skos/core#related"/>
    <dct:description>place - formerly identified as - place; New.&#13;
Example: The deserted settlement of Machupicchu was formerly identified as Tampu Tocco</dct:description>
    <rdf:type rdf:resource="http://www.w3.org/2002/07/owl#ObjectProperty"/>
  </rdf:Description>
  <rdf:Description rdf:about="http://vocab.getty.edu/ontology#ulan1331_worked_with">
    <skos:prefLabel>ulan1331_worked_with</skos:prefLabel>
    <skos:example>Scarsellino and Domenichino worked with the Carracci family</skos:example>
    <rdfs:isDefinedBy rdf:resource="http://vocab.getty.edu/ulan/"/>
    <rdfs:domain rdf:resource="http://www.w3.org/2004/02/skos/core#Concept"/>
    <rdfs:isDefinedBy rdf:resource="http://vocab.getty.edu/ontology"/>
    <dc:identifier>1331</dc:identifier>
    <dct:description>any - worked with - person.&#13;
Example: Scarsellino and Domenichino worked with the Carracci family</dct:description>
    <dc:title>worked with - person</dc:title>
    <rdfs:range rdf:resource="http://www.w3.org/2004/02/skos/core#Concept"/>
    <owl:inverseOf rdf:resource="http://vocab.getty.edu/ontology#ulan1332_worker_was"/>
    <rdfs:subPropertyOf rdf:resource="http://www.w3.org/2004/02/skos/core#related"/>
    <rdf:type rdf:resource="http://www.w3.org/2002/07/owl#ObjectProperty"/>
  </rdf:Description>
  <rdf:Description rdf:about="http://vocab.getty.edu/term/POS/Noun">
    <skos:notation>N</skos:notation>
    <skos:scopeNote>Term is a noun but we are uncertain if it is plural or singular</skos:scopeNote>
    <skos:prefLabel>Noun</skos:prefLabel>
    <dct:description>Term is a noun but we are uncertain if it is plural or singular.
Example: Panthera leo</dct:description>
    <skos:inScheme rdf:resource="http://vocab.getty.edu/term/POS/"/>
    <skos:example>Panthera leo</skos:example>
    <rdf:type rdf:resource="http://www.w3.org/2004/02/skos/core#Concept"/>
  </rdf:Description>
  <rdf:Description rdf:about="http://vocab.getty.edu/ontology#prefLabelLoC">
    <rdfs:isDefinedBy rdf:resource="http://vocab.getty.edu/ontology"/>
    <rdfs:comment>Term preferred by Library of Congress, thus used for cataloging according to AACR2. Applicable to AAT and ULAN. Used with skosxl:prefLabel</rdfs:comment>
    <dct:description>Term preferred by Library of Congress, thus used for cataloging according to AACR2. Applicable to AAT and ULAN. Used with skosxl:prefLabel</dct:description>
    <skos:prefLabel>prefLabelLoC</skos:prefLabel>
    <rdfs:domain rdf:resource="http://vocab.getty.edu/ontology#Subject"/>
    <rdf:type rdf:resource="http://www.w3.org/2002/07/owl#ObjectProperty"/>
    <rdfs:label>prefLabelLoC</rdfs:label>
    <rdfs:range rdf:resource="http://www.w3.org/2008/05/skos-xl#Label"/>
  </rdf:Description>
  <rdf:Description rdf:about="http://vocab.getty.edu/term/kind/CommonTerm">
    <skos:notation>C</skos:notation>
    <skos:prefLabel>Common term</skos:prefLabel>
    <skos:scopeNote>Preferred common language term. Used for subjects that also include a Scientific term. Used in AAT only</skos:scopeNote>
    <rdf:type rdf:resource="http://www.w3.org/2004/02/skos/core#Concept"/>
    <skos:inScheme rdf:resource="http://vocab.getty.edu/term/kind/"/>
    <skos:example>"frankincense" (species) is common term for "Boswellia sacra" (species)</skos:example>
    <dct:description>Preferred common language term. Used for subjects that also include a Scientific term. Used in AAT only.
Example: "frankincense" (species) is common term for "Boswellia sacra" (species)</dct:description>
  </rdf:Description>
  <rdf:Description rdf:about="http://vocab.getty.edu/ontology#historicFlag">
    <skos:prefLabel>historicFlag</skos:prefLabel>
    <rdf:type rdf:resource="http://www.w3.org/2002/07/owl#ObjectProperty"/>
    <rdfs:label>historicFlag</rdfs:label>
    <rdfs:isDefinedBy rdf:resource="http://vocab.getty.edu/ontology"/>
    <rdfs:range rdf:resource="http://www.w3.org/2004/02/skos/core#Concept"/>
    <dct:description>Historic Flag</dct:description>
  </rdf:Description>
  <rdf:Description rdf:about="http://vocab.getty.edu/ontology#Infer_isoBroaderInstantial">
    <ptop:conclusion rdf:resource="http://purl.org/iso25964/skos-thes#broaderInstantial"/>
    <ptop:premise rdf:resource="http://vocab.getty.edu/ontology#broaderInstantialExtended"/>
    <ptop:restriction rdf:resource="http://www.w3.org/2004/02/skos/core#broader"/>
    <rdf:type rdf:resource="http://www.ontotext.com/proton/protontop#PropRestr"/>
  </rdf:Description>
  <rdf:Description rdf:about="http://vocab.getty.edu/ontology#termPOS">
    <skos:prefLabel>termPOS</skos:prefLabel>
    <rdfs:domain rdf:resource="http://www.w3.org/2008/05/skos-xl#Label"/>
    <dct:description>Part of Speech</dct:description>
    <rdfs:isDefinedBy rdf:resource="http://vocab.getty.edu/ontology"/>
    <rdfs:label>termPOS</rdfs:label>
    <rdfs:range rdf:resource="http://www.w3.org/2004/02/skos/core#Concept"/>
    <rdf:type rdf:resource="http://www.w3.org/2002/07/owl#ObjectProperty"/>
  </rdf:Description>
  <rdf:Description rdf:about="http://vocab.getty.edu/ontology#aat2329_involves">
    <dc:title>involves - role</dc:title>
    <rdf:type rdf:resource="http://www.w3.org/2002/07/owl#ObjectProperty"/>
    <rdfs:isDefinedBy rdf:resource="http://vocab.getty.edu/aat/"/>
    <skos:prefLabel>aat2329_involves</skos:prefLabel>
    <skos:example>portraits involve sitters</skos:example>
    <skos:example>motion pictures (visual works) involve actors (performing artists)</skos:example>
    <dct:description>things - involve - [actors having] role.&#13;
Example: portraits involve sitters; motion pictures (visual works) involve actors (performing artists)</dct:description>
    <rdfs:isDefinedBy rdf:resource="http://vocab.getty.edu/ontology"/>
    <rdfs:domain rdf:resource="http://www.w3.org/2004/02/skos/core#Concept"/>
    <rdfs:subPropertyOf rdf:resource="http://www.w3.org/2004/02/skos/core#related"/>
    <rdfs:range rdf:resource="http://www.w3.org/2004/02/skos/core#Concept"/>
    <dc:identifier>2329</dc:identifier>
  </rdf:Description>
  <rdf:Description rdf:about="http://vocab.getty.edu/ontology#aat2311_performed_by">
    <skos:example>curating is performed by curators</skos:example>
    <rdf:type rdf:resource="http://www.w3.org/2002/07/owl#ObjectProperty"/>
    <dc:title>performed by - role</dc:title>
    <rdfs:range rdf:resource="http://www.w3.org/2004/02/skos/core#Concept"/>
    <dct:description>activity/event/[process/function] - [is] performed by - [actors having] a role.&#13;
Example: clockmaking is performed by clockmakers; curating is performed by curators</dct:description>
    <dc:identifier>2311</dc:identifier>
    <skos:prefLabel>aat2311_performed_by</skos:prefLabel>
    <skos:example>clockmaking is performed by clockmakers</skos:example>
    <rdfs:domain rdf:resource="http://www.w3.org/2004/02/skos/core#Concept"/>
    <owl:inverseOf rdf:resource="http://vocab.getty.edu/ontology#aat2312_perform"/>
    <rdfs:isDefinedBy rdf:resource="http://vocab.getty.edu/ontology"/>
    <rdfs:subPropertyOf rdf:resource="http://www.w3.org/2004/02/skos/core#related"/>
    <rdfs:isDefinedBy rdf:resource="http://vocab.getty.edu/aat/"/>
  </rdf:Description>
  <rdf:Description rdf:about="http://vocab.getty.edu/term/kind/ISOnumeric3">
    <rdf:type rdf:resource="http://www.w3.org/2004/02/skos/core#Concept"/>
    <skos:example>"ISO414" for Kuwait</skos:example>
    <skos:notation>ISO3N</skos:notation>
    <dct:description>ISO 3166-1 numeric country code as "ISOnnn" (though ISO specifies only "nnn"). Used in TGN only.
Example: "ISO414" for Kuwait</dct:description>
    <skos:prefLabel>ISO numeric-3 code</skos:prefLabel>
    <skos:scopeNote>ISO 3166-1 numeric country code as "ISOnnn" (though ISO specifies only "nnn"). Used in TGN only</skos:scopeNote>
    <skos:inScheme rdf:resource="http://vocab.getty.edu/term/kind/"/>
  </rdf:Description>
  <rdf:Description rdf:about="http://vocab.getty.edu/ontology#aat2900_miscellaneous_relationship">
    <rdf:type rdf:resource="http://www.w3.org/2002/07/owl#ObjectProperty"/>
    <dct:description>any - [has] miscellaneous relationship [to] - any.&#13;
Example: Conditions and Effects has miscellaneous relationship with Processes and Techniques</dct:description>
    <rdfs:subPropertyOf rdf:resource="http://www.w3.org/2004/02/skos/core#related"/>
    <dc:title>miscellaneous relationship - any</dc:title>
    <skos:prefLabel>aat2900_miscellaneous_relationship</skos:prefLabel>
    <dc:identifier>2900</dc:identifier>
    <rdf:type rdf:resource="http://www.w3.org/2002/07/owl#SymmetricProperty"/>
    <rdfs:isDefinedBy rdf:resource="http://vocab.getty.edu/ontology"/>
    <rdfs:domain rdf:resource="http://www.w3.org/2004/02/skos/core#Concept"/>
    <skos:example>Conditions and Effects has miscellaneous relationship with Processes and Techniques</skos:example>
    <rdfs:isDefinedBy rdf:resource="http://vocab.getty.edu/aat/"/>
    <rdfs:range rdf:resource="http://www.w3.org/2004/02/skos/core#Concept"/>
  </rdf:Description>
  <rdf:Description rdf:about="http://vocab.getty.edu/ontology#ulan1101_teacher_of">
    <dc:identifier>1101</dc:identifier>
    <skos:prefLabel>ulan1101_teacher_of</skos:prefLabel>
    <rdf:type rdf:resource="http://www.w3.org/2002/07/owl#ObjectProperty"/>
    <dc:title>teacher of - person</dc:title>
    <dct:description>person - teacher of - person.&#13;
Example: Rivalz, Antoine was the teacher of Pierre Subleyras</dct:description>
    <rdfs:range rdf:resource="http://www.w3.org/2004/02/skos/core#Concept"/>
    <rdfs:domain rdf:resource="http://www.w3.org/2004/02/skos/core#Concept"/>
    <rdfs:subPropertyOf rdf:resource="http://www.w3.org/2004/02/skos/core#related"/>
    <rdfs:isDefinedBy rdf:resource="http://vocab.getty.edu/ontology"/>
    <owl:inverseOf rdf:resource="http://vocab.getty.edu/ontology#ulan1102_student_of"/>
    <skos:example>Rivalz, Antoine was the teacher of Pierre Subleyras</skos:example>
    <rdfs:isDefinedBy rdf:resource="http://vocab.getty.edu/ulan/"/>
  </rdf:Description>
  <rdf:Description rdf:about="http://vocab.getty.edu/ontology#aat2418_uses">
    <rdfs:isDefinedBy rdf:resource="http://vocab.getty.edu/aat/"/>
    <skos:example>astronomy uses astronomical instruments</skos:example>
    <owl:inverseOf rdf:resource="http://vocab.getty.edu/ontology#aat2419_used_for"/>
    <rdf:type rdf:resource="http://www.w3.org/2002/07/owl#ObjectProperty"/>
    <skos:example>divination [discipline] uses divination objects</skos:example>
    <rdfs:range rdf:resource="http://www.w3.org/2004/02/skos/core#Concept"/>
    <skos:prefLabel>aat2418_uses</skos:prefLabel>
    <rdfs:domain rdf:resource="http://www.w3.org/2004/02/skos/core#Concept"/>
    <dc:identifier>2418</dc:identifier>
    <rdfs:subPropertyOf rdf:resource="http://www.w3.org/2004/02/skos/core#related"/>
    <dc:title>uses - things</dc:title>
    <rdfs:isDefinedBy rdf:resource="http://vocab.getty.edu/ontology"/>
    <dct:description>field [of study]/discipline - uses - things/[equipment].&#13;
Example: astronomy uses astronomical instruments; divination [discipline] uses divination objects</dct:description>
  </rdf:Description>
  <rdf:Description rdf:about="http://vocab.getty.edu/ontology#aat2312_perform">
    <dct:description>[actors having] a role - perform - activity/event/process.&#13;
Example: clockmakers perform clockmaking; curators perform curating</dct:description>
    <rdfs:range rdf:resource="http://www.w3.org/2004/02/skos/core#Concept"/>
    <rdfs:isDefinedBy rdf:resource="http://vocab.getty.edu/ontology"/>
    <rdfs:domain rdf:resource="http://www.w3.org/2004/02/skos/core#Concept"/>
    <skos:example>clockmakers perform clockmaking</skos:example>
    <skos:example>curators perform curating</skos:example>
    <rdfs:subPropertyOf rdf:resource="http://www.w3.org/2004/02/skos/core#related"/>
    <rdf:type rdf:resource="http://www.w3.org/2002/07/owl#ObjectProperty"/>
    <dc:identifier>2312</dc:identifier>
    <dc:title>perform - activity/event</dc:title>
    <rdfs:isDefinedBy rdf:resource="http://vocab.getty.edu/aat/"/>
    <skos:prefLabel>aat2312_perform</skos:prefLabel>
  </rdf:Description>
  <rdf:Description rdf:about="http://vocab.getty.edu/aat/300189557">
    <skos:exactMatch rdf:resource="http://www.wikidata.org/entity/Q6581072"/>
    <skos:exactMatch rdf:resource="http://rdaregistry.info/termList/gender/1001"/>
  </rdf:Description>
  <rdf:Description rdf:about="http://vocab.getty.edu/ontology#aat2815_composed_of">
    <skos:example>composite white is composed of titanium white</skos:example>
    <rdf:type rdf:resource="http://www.w3.org/2002/07/owl#ObjectProperty"/>
    <rdfs:range rdf:resource="http://www.w3.org/2004/02/skos/core#Concept"/>
    <skos:prefLabel>aat2815_composed_of</skos:prefLabel>
    <dc:identifier>2815</dc:identifier>
    <rdfs:domain rdf:resource="http://www.w3.org/2004/02/skos/core#Concept"/>
    <rdfs:subPropertyOf rdf:resource="http://www.w3.org/2004/02/skos/core#related"/>
    <rdfs:isDefinedBy rdf:resource="http://vocab.getty.edu/ontology"/>
    <dc:title>composed of - material</dc:title>
    <dct:description>material - [is] composed of - material.&#13;
Example: composite white is composed of titanium white; desert varnish is composed of iron oxide</dct:description>
    <rdfs:isDefinedBy rdf:resource="http://vocab.getty.edu/aat/"/>
    <skos:example>desert varnish is composed of iron oxide</skos:example>
  </rdf:Description>
  <rdf:Description rdf:about="http://vocab.getty.edu/term/kind/Pseudonym">
    <skos:inScheme rdf:resource="http://vocab.getty.edu/term/kind/"/>
    <skos:scopeNote>Used in TGN and ULAN</skos:scopeNote>
    <rdf:type rdf:resource="http://www.w3.org/2004/02/skos/core#Concept"/>
    <skos:example>"Frisco" is nickname for San Francisco (TGN)</skos:example>
    <dct:description>Used in TGN and ULAN.
Example: "Frisco" is nickname for San Francisco (TGN)</dct:description>
    <skos:notation>P</skos:notation>
    <skos:prefLabel>Pseudonym</skos:prefLabel>
  </rdf:Description>
  <rdf:Description rdf:about="http://vocab.getty.edu/ontology#ulan1321_school_of">
    <rdfs:range rdf:resource="http://www.w3.org/2004/02/skos/core#Concept"/>
    <rdf:type rdf:resource="http://www.w3.org/2002/07/owl#ObjectProperty"/>
    <owl:inverseOf rdf:resource="http://vocab.getty.edu/ontology#ulan1322_school_was"/>
    <dct:description>person - school of - firm/group.&#13;
Example: The school of Pierre Saalburg was the Architectural Association. School of Architecture</dct:description>
    <dc:identifier>1321</dc:identifier>
    <rdfs:isDefinedBy rdf:resource="http://vocab.getty.edu/ulan/"/>
    <dc:title>school of - firm/group</dc:title>
    <skos:prefLabel>ulan1321_school_of</skos:prefLabel>
    <rdfs:domain rdf:resource="http://www.w3.org/2004/02/skos/core#Concept"/>
    <rdfs:isDefinedBy rdf:resource="http://vocab.getty.edu/ontology"/>
    <rdfs:subPropertyOf rdf:resource="http://www.w3.org/2004/02/skos/core#related"/>
    <skos:example>The school of Pierre Saalburg was the Architectural Association. School of Architecture</skos:example>
  </rdf:Description>
  <rdf:Description rdf:about="http://vocab.getty.edu/ontology#aat2881_reflected_in">
    <dc:identifier>2881</dc:identifier>
    <rdfs:isDefinedBy rdf:resource="http://vocab.getty.edu/ontology"/>
    <rdfs:subPropertyOf rdf:resource="http://www.w3.org/2004/02/skos/core#related"/>
    <rdfs:domain rdf:resource="http://www.w3.org/2004/02/skos/core#Concept"/>
    <dct:description>language - [is] reflected in - things.&#13;
Example: Greek (language) is reflected in Greek alphabet; Sanskrit is reflected in Vedas</dct:description>
    <rdfs:range rdf:resource="http://www.w3.org/2004/02/skos/core#Concept"/>
    <skos:example>Greek (language) is reflected in Greek alphabet</skos:example>
    <dc:title>reflected in - things</dc:title>
    <rdf:type rdf:resource="http://www.w3.org/2002/07/owl#ObjectProperty"/>
    <skos:prefLabel>aat2881_reflected_in</skos:prefLabel>
    <owl:inverseOf rdf:resource="http://vocab.getty.edu/ontology#aat2882_reflect"/>
    <skos:example>Sanskrit is reflected in Vedas</skos:example>
    <rdfs:isDefinedBy rdf:resource="http://vocab.getty.edu/aat/"/>
  </rdf:Description>
  <rdf:Description rdf:about="http://vocab.getty.edu/ontology#parentString">
    <skos:prefLabel>parentString</skos:prefLabel>
    <rdfs:range rdf:resource="http://www.w3.org/1999/02/22-rdf-syntax-ns#Literal"/>
    <dct:description>Preferred labels of *all* of the subject's preferred ancestors, listed bottom up. Useful to show the subject's full context.
Display version of gvp:broaderPreferredExtended.
For aat:300226882 baking dishes: bakeware, &lt;vessels for cooking food&gt;, &lt;containers for cooking food&gt;, &lt;culinary containers&gt;, &lt;containers by function or context&gt;, containers (receptacles), Containers (Hierarchy Name), Furnishings and Equipment (Hierarchy Name), Objects Facet</dct:description>
    <rdfs:isDefinedBy rdf:resource="http://vocab.getty.edu/ontology"/>
    <skos:example>For aat:300226882 baking dishes: bakeware, &lt;vessels for cooking food&gt;, &lt;containers for cooking food&gt;, &lt;culinary containers&gt;, &lt;containers by function or context&gt;, containers (receptacles), Containers (Hierarchy Name), Furnishings and Equipment (Hierarchy Name), Objects Facet</skos:example>
    <rdfs:label>parentString</rdfs:label>
    <rdfs:domain rdf:resource="http://vocab.getty.edu/ontology#Subject"/>
    <rdfs:comment>Preferred labels of *all* of the subject's preferred ancestors, listed bottom up. Useful to show the subject's full context</rdfs:comment>
    <rdf:type rdf:resource="http://www.w3.org/2002/07/owl#DatatypeProperty"/>
    <skos:note>Display version of gvp:broaderPreferredExtended</skos:note>
  </rdf:Description>
  <rdf:Description rdf:about="http://vocab.getty.edu/term/POS/VerbalNounGerund">
    <skos:example>polishing</skos:example>
    <skos:scopeNote>Term is a verbal noun or gerund</skos:scopeNote>
    <skos:prefLabel>Verbal Noun/Gerund</skos:prefLabel>
    <dct:description>Term is a verbal noun or gerund.
Example: polishing</dct:description>
    <skos:inScheme rdf:resource="http://vocab.getty.edu/term/POS/"/>
    <skos:notation>VN</skos:notation>
    <rdf:type rdf:resource="http://www.w3.org/2004/02/skos/core#Concept"/>
  </rdf:Description>
  <rdf:Description rdf:about="http://www.ontotext.com">
    <rdf:type rdf:resource="http://xmlns.com/foaf/0.1/Organization"/>
    <skos:prefLabel>Ontotext Corp</skos:prefLabel>
    <rdfs:label>Ontotext Corp</rdfs:label>
    <foaf:name>Ontotext Corp</foaf:name>
  </rdf:Description>
  <rdf:Description rdf:about="http://vocab.getty.edu/ontology#ulan2693_president_was">
    <dc:title>president was - person</dc:title>
    <rdfs:subPropertyOf rdf:resource="http://www.w3.org/2004/02/skos/core#related"/>
    <rdfs:isDefinedBy rdf:resource="http://vocab.getty.edu/ontology"/>
    <skos:example>A president of National Gallery of Art was David K. E. Bruce</skos:example>
    <rdfs:isDefinedBy rdf:resource="http://vocab.getty.edu/ulan/"/>
    <rdf:type rdf:resource="http://www.w3.org/2002/07/owl#ObjectProperty"/>
    <dc:identifier>2693</dc:identifier>
    <skos:prefLabel>ulan2693_president_was</skos:prefLabel>
    <rdfs:range rdf:resource="http://www.w3.org/2004/02/skos/core#Concept"/>
    <dct:description>institution - president was - person.&#13;
Example: A president of National Gallery of Art was David K. E. Bruce</dct:description>
    <rdfs:domain rdf:resource="http://www.w3.org/2004/02/skos/core#Concept"/>
  </rdf:Description>
  <rdf:Description rdf:about="http://vocab.getty.edu/ontology#biographyNonPreferred">
    <skos:prefLabel>biographyNonPreferred</skos:prefLabel>
    <rdfs:range rdf:resource="http://vocab.getty.edu/ontology#Biography"/>
    <rdfs:isDefinedBy rdf:resource="http://vocab.getty.edu/ontology"/>
    <rdfs:subPropertyOf rdf:resource="http://vocab.getty.edu/ontology#biography"/>
    <rdfs:comment>Non-preferred biography of an ULAN agent. Domain is schema:Person/Organization, range is gvp:Biography</rdfs:comment>
    <dct:description>Non-preferred biography of an ULAN agent. Domain is schema:Person/Organization, range is gvp:Biography</dct:description>
    <rdf:type rdf:resource="http://www.w3.org/2002/07/owl#ObjectProperty"/>
    <rdfs:label>biographyNonPreferred</rdfs:label>
  </rdf:Description>
  <rdf:Description rdf:about="http://vocab.getty.edu/ontology#broaderPartitiveExtended">
    <rdfs:domain rdf:resource="http://vocab.getty.edu/ontology#Subject"/>
    <rdfs:isDefinedBy rdf:resource="http://vocab.getty.edu/ontology"/>
    <rdfs:range rdf:resource="http://vocab.getty.edu/ontology#Subject"/>
    <dct:description>Ancestors (Partitive). Meaningful closure of gvp:broaderPartitive. Infers iso:broaderPartitive for pairs of directly related skos:Concepts.
Example: anvil components BTP &lt;anvils and anvil accessories&gt; BTG &lt;forging and metal-shaping tools&gt;,
so anvil components BTPE &lt;forging and metal-shaping tools&gt;</dct:description>
    <rdfs:label>broaderPartitiveExtended</rdfs:label>
    <owl:propertyChainAxiom rdf:nodeID="Na4f426f3b86940199dc92fb434c8fc18"/>
    <skos:prefLabel>broaderPartitiveExtended</skos:prefLabel>
    <owl:propertyChainAxiom rdf:nodeID="N731c9cb66cef4e658afa515d3206747b"/>
    <rdf:type rdf:resource="http://www.w3.org/2002/07/owl#ObjectProperty"/>
    <skos:example>anvil components BTP &lt;anvils and anvil accessories&gt; BTG &lt;forging and metal-shaping tools&gt;,
so anvil components BTPE &lt;forging and metal-shaping tools&gt;</skos:example>
    <rdfs:subPropertyOf rdf:resource="http://vocab.getty.edu/ontology#broaderExtended"/>
    <owl:propertyChainAxiom rdf:nodeID="N6fafbb3f5a524fde95f35d19565c2579"/>
    <rdfs:comment>Ancestors (Partitive). Meaningful closure of gvp:broaderPartitive. Infers iso:broaderPartitive for pairs of directly related skos:Concepts</rdfs:comment>
  </rdf:Description>
  <rdf:Description rdf:about="http://vocab.getty.edu/term/flag/Vernacular">
    <skos:prefLabel>Vernacular</skos:prefLabel>
    <rdf:type rdf:resource="http://www.w3.org/2004/02/skos/core#Concept"/>
    <skos:scopeNote>Term is the vernacular for a certain place</skos:scopeNote>
    <skos:notation>V</skos:notation>
    <skos:inScheme rdf:resource="http://vocab.getty.edu/term/flag/"/>
    <dct:description>Term is the vernacular for a certain place.
Example: "kachoga" is the Vernacular for 300266169 "bird-and-flower paintings" (AAT). "Firenze" is the vernacular in Italian (TGN)</dct:description>
    <skos:example>"kachoga" is the Vernacular for 300266169 "bird-and-flower paintings" (AAT). "Firenze" is the vernacular in Italian (TGN)</skos:example>
  </rdf:Description>
  <rdf:Description rdf:about="http://vocab.getty.edu/ontology#aat2110_meaning-usage_overlaps_with">
    <rdfs:subPropertyOf rdf:resource="http://www.w3.org/2004/02/skos/core#related"/>
    <dc:title>meaning/usage overlaps with - any</dc:title>
    <rdf:type rdf:resource="http://www.w3.org/2002/07/owl#ObjectProperty"/>
    <dct:description>any - meaning/usage overlaps with - any.&#13;
Example: chimney hoods has meaning/usage that overlaps with chimney caps; scribes has meaning/usage that overlaps with copyists</dct:description>
    <dc:identifier>2110</dc:identifier>
    <skos:prefLabel>aat2110_meaning-usage_overlaps_with</skos:prefLabel>
    <rdfs:range rdf:resource="http://www.w3.org/2004/02/skos/core#Concept"/>
    <rdfs:domain rdf:resource="http://www.w3.org/2004/02/skos/core#Concept"/>
    <skos:example>chimney hoods has meaning/usage that overlaps with chimney caps</skos:example>
    <skos:example>scribes has meaning/usage that overlaps with copyists</skos:example>
    <rdf:type rdf:resource="http://www.w3.org/2002/07/owl#SymmetricProperty"/>
    <rdfs:isDefinedBy rdf:resource="http://vocab.getty.edu/ontology"/>
    <rdfs:isDefinedBy rdf:resource="http://vocab.getty.edu/aat/"/>
  </rdf:Description>
  <rdf:Description rdf:about="http://vocab.getty.edu/ontology#aat2001_formerly_referred_to">
    <skos:example>gigues formerly referred to fiddles</skos:example>
    <skos:prefLabel>aat2001_formerly_referred_to</skos:prefLabel>
    <rdf:type rdf:resource="http://www.w3.org/2002/07/owl#SymmetricProperty"/>
    <rdfs:isDefinedBy rdf:resource="http://vocab.getty.edu/ontology"/>
    <rdfs:subPropertyOf rdf:resource="http://www.w3.org/2004/02/skos/core#related"/>
    <dct:description>any - formerly referred - any.&#13;
Example: gigues formerly referred to fiddles</dct:description>
    <rdfs:domain rdf:resource="http://www.w3.org/2004/02/skos/core#Concept"/>
    <rdfs:range rdf:resource="http://www.w3.org/2004/02/skos/core#Concept"/>
    <rdf:type rdf:resource="http://www.w3.org/2002/07/owl#ObjectProperty"/>
    <dc:title>formerly referred to - any</dc:title>
    <dc:identifier>2001</dc:identifier>
    <rdfs:isDefinedBy rdf:resource="http://vocab.getty.edu/aat/"/>
  </rdf:Description>
  <rdf:Description rdf:about="http://vocab.getty.edu/ontology#ulan2697_leader_was">
    <rdfs:subPropertyOf rdf:resource="http://www.w3.org/2004/02/skos/core#related"/>
    <rdfs:isDefinedBy rdf:resource="http://vocab.getty.edu/ulan/"/>
    <skos:example>The leader of Samuel H. Kress Foundation was Rush Harrison Kress</skos:example>
    <skos:prefLabel>ulan2697_leader_was</skos:prefLabel>
    <rdfs:range rdf:resource="http://www.w3.org/2004/02/skos/core#Concept"/>
    <rdfs:isDefinedBy rdf:resource="http://vocab.getty.edu/ontology"/>
    <rdfs:domain rdf:resource="http://www.w3.org/2004/02/skos/core#Concept"/>
    <dct:description>institution - leader was - person.&#13;
Example: The leader of Samuel H. Kress Foundation was Rush Harrison Kress</dct:description>
    <dc:identifier>2697</dc:identifier>
    <dc:title>leader was - person</dc:title>
    <rdf:type rdf:resource="http://www.w3.org/2002/07/owl#ObjectProperty"/>
  </rdf:Description>
  <rdf:Description rdf:about="http://vocab.getty.edu/ontology#aat2435_context_for">
    <rdfs:subPropertyOf rdf:resource="http://www.w3.org/2004/02/skos/core#related"/>
    <rdfs:isDefinedBy rdf:resource="http://vocab.getty.edu/ontology"/>
    <dct:description>activity/event/process - [is] contextualized in - thing.&#13;
Example: funerals are the context for funeral books; Christmas is the context for Christmas trees</dct:description>
    <rdfs:range rdf:resource="http://www.w3.org/2004/02/skos/core#Concept"/>
    <rdfs:isDefinedBy rdf:resource="http://vocab.getty.edu/aat/"/>
    <rdf:type rdf:resource="http://www.w3.org/2002/07/owl#ObjectProperty"/>
    <skos:example>Christmas is the context for Christmas trees</skos:example>
    <skos:example>funerals are the context for funeral books</skos:example>
    <dc:title>context for - things</dc:title>
    <dc:identifier>2435</dc:identifier>
    <skos:prefLabel>aat2435_context_for</skos:prefLabel>
    <rdfs:domain rdf:resource="http://www.w3.org/2004/02/skos/core#Concept"/>
  </rdf:Description>
  <rdf:Description rdf:about="http://vocab.getty.edu/ontology#aat2842_source_for">
    <skos:example>Vicugna pacos (species) is the source for alpaca (wool)</skos:example>
    <rdfs:domain rdf:resource="http://www.w3.org/2004/02/skos/core#Concept"/>
    <skos:prefLabel>aat2842_source_for</skos:prefLabel>
    <rdfs:range rdf:resource="http://www.w3.org/2004/02/skos/core#Concept"/>
    <rdfs:isDefinedBy rdf:resource="http://vocab.getty.edu/ontology"/>
    <dc:title>source for - material</dc:title>
    <dct:description>genus/species - [is] source for - material.&#13;
Example: Vicugna pacos (species) is the source for alpaca (wool); Acer (genus) is the source for maple (wood)</dct:description>
    <rdfs:isDefinedBy rdf:resource="http://vocab.getty.edu/aat/"/>
    <skos:example>Acer (genus) is the source for maple (wood)</skos:example>
    <rdf:type rdf:resource="http://www.w3.org/2002/07/owl#ObjectProperty"/>
    <dc:identifier>2842</dc:identifier>
    <rdfs:subPropertyOf rdf:resource="http://www.w3.org/2004/02/skos/core#related"/>
  </rdf:Description>
  <rdf:Description rdf:about="http://vocab.getty.edu/ontology#ulan1311_partner_of">
    <dct:description>person - partner of - person.&#13;
Example: Frank Gehry and James Glymph are partners</dct:description>
    <skos:prefLabel>ulan1311_partner_of</skos:prefLabel>
    <dc:title>partner of - person</dc:title>
    <rdf:type rdf:resource="http://www.w3.org/2002/07/owl#SymmetricProperty"/>
    <rdf:type rdf:resource="http://www.w3.org/2002/07/owl#ObjectProperty"/>
    <rdfs:domain rdf:resource="http://www.w3.org/2004/02/skos/core#Concept"/>
    <rdfs:isDefinedBy rdf:resource="http://vocab.getty.edu/ontology"/>
    <rdfs:isDefinedBy rdf:resource="http://vocab.getty.edu/ulan/"/>
    <rdfs:subPropertyOf rdf:resource="http://www.w3.org/2004/02/skos/core#related"/>
    <dc:identifier>1311</dc:identifier>
    <skos:example>Frank Gehry and James Glymph are partners</skos:example>
    <rdfs:range rdf:resource="http://www.w3.org/2004/02/skos/core#Concept"/>
  </rdf:Description>
  <rdf:Description rdf:about="http://vocab.getty.edu/ontology#aat2502_material_for">
    <rdf:type rdf:resource="http://www.w3.org/2002/07/owl#ObjectProperty"/>
    <dc:identifier>2502</dc:identifier>
    <skos:prefLabel>aat2502_material_for</skos:prefLabel>
    <rdfs:subPropertyOf rdf:resource="http://www.w3.org/2004/02/skos/core#related"/>
    <skos:example>ivory is material for ivories (sculptures)</skos:example>
    <dc:title>material for - things</dc:title>
    <dct:description>material - [is] material for - things.&#13;
Example: obsidian is material for obsidian mirrors; ivory is material for ivories (sculptures)</dct:description>
    <rdfs:isDefinedBy rdf:resource="http://vocab.getty.edu/ontology"/>
    <rdfs:domain rdf:resource="http://www.w3.org/2004/02/skos/core#Concept"/>
    <skos:example>obsidian is material for obsidian mirrors</skos:example>
    <rdfs:isDefinedBy rdf:resource="http://vocab.getty.edu/aat/"/>
    <rdfs:range rdf:resource="http://www.w3.org/2004/02/skos/core#Concept"/>
  </rdf:Description>
  <rdf:Description rdf:about="http://vocab.getty.edu/term/flag/LoanTerm">
    <skos:notation>L</skos:notation>
    <skos:inScheme rdf:resource="http://vocab.getty.edu/term/flag/"/>
    <skos:prefLabel>Loan Term</skos:prefLabel>
    <rdf:type rdf:resource="http://www.w3.org/2004/02/skos/core#Concept"/>
    <skos:example>papier mache</skos:example>
    <skos:scopeNote>Term borrowed from another language that has become naturalized in American English</skos:scopeNote>
    <dct:description>Term borrowed from another language that has become naturalized in American English.
Example: papier mache</dct:description>
  </rdf:Description>
  <rdf:Description rdf:about="http://vocab.getty.edu/ontology#tgn3102_coextensive_with">
    <dc:title>coextensive with - place</dc:title>
    <rdf:type rdf:resource="http://www.w3.org/2002/07/owl#ObjectProperty"/>
    <skos:prefLabel>tgn3102_coextensive_with</skos:prefLabel>
    <dc:identifier>3102</dc:identifier>
    <skos:example>Kings county (New York, USA) is coextensive with Brooklyn (New York, USA)</skos:example>
    <rdfs:isDefinedBy rdf:resource="http://vocab.getty.edu/ontology"/>
    <dct:description>place - coextensive with - place.&#13;
Example: Kings county (New York, USA) is coextensive with Brooklyn (New York, USA)</dct:description>
    <rdfs:isDefinedBy rdf:resource="http://vocab.getty.edu/tgn/"/>
    <rdf:type rdf:resource="http://www.w3.org/2002/07/owl#SymmetricProperty"/>
    <rdfs:domain rdf:resource="http://www.w3.org/2004/02/skos/core#Concept"/>
    <rdfs:subPropertyOf rdf:resource="http://www.w3.org/2004/02/skos/core#related"/>
    <rdfs:range rdf:resource="http://www.w3.org/2004/02/skos/core#Concept"/>
  </rdf:Description>
  <rdf:Description rdf:about="http://vocab.getty.edu/ontology#aat2803_example_of">
    <dc:title>example of - material</dc:title>
    <rdfs:subPropertyOf rdf:resource="http://www.w3.org/2004/02/skos/core#related"/>
    <dc:identifier>2803</dc:identifier>
    <skos:prefLabel>aat2803_example_of</skos:prefLabel>
    <rdfs:domain rdf:resource="http://www.w3.org/2004/02/skos/core#Concept"/>
    <rdfs:isDefinedBy rdf:resource="http://vocab.getty.edu/ontology"/>
    <rdfs:range rdf:resource="http://www.w3.org/2004/02/skos/core#Concept"/>
    <skos:example>Vaseline (TM) is an example of petrolium jelly</skos:example>
    <skos:example>Teflon (TM) is an example of polytetrafluoroethyelene</skos:example>
    <rdf:type rdf:resource="http://www.w3.org/2002/07/owl#ObjectProperty"/>
    <rdfs:isDefinedBy rdf:resource="http://vocab.getty.edu/aat/"/>
    <dct:description>brand name - [is] example of - material.&#13;
Example: Vaseline (TM) is an example of petrolium jelly; Teflon (TM) is an example of polytetrafluoroethyelene</dct:description>
  </rdf:Description>
  <rdf:Description rdf:about="http://www.getty.edu/research/">
    <rdfs:label>Getty Research Institute</rdfs:label>
    <foaf:name>Getty Research Institute</foaf:name>
    <rdf:type rdf:resource="http://xmlns.com/foaf/0.1/Organization"/>
    <skos:prefLabel>Getty Research Institute</skos:prefLabel>
  </rdf:Description>
  <rdf:Description rdf:about="http://vocab.getty.edu/ontology#ulan1513_grandchild_of">
    <skos:example>Eric Lloyd Wright is the grandchild of Frank Lloyd Wright</skos:example>
    <rdfs:isDefinedBy rdf:resource="http://vocab.getty.edu/ulan/"/>
    <rdfs:subPropertyOf rdf:resource="http://www.w3.org/2004/02/skos/core#related"/>
    <rdfs:domain rdf:resource="http://www.w3.org/2004/02/skos/core#Concept"/>
    <rdfs:isDefinedBy rdf:resource="http://vocab.getty.edu/ontology"/>
    <skos:prefLabel>ulan1513_grandchild_of</skos:prefLabel>
    <dc:title>grandchild of - person</dc:title>
    <rdfs:range rdf:resource="http://www.w3.org/2004/02/skos/core#Concept"/>
    <dc:identifier>1513</dc:identifier>
    <dct:description>person - grandchild of - person.&#13;
Example: Eric Lloyd Wright is the grandchild of Frank Lloyd Wright</dct:description>
    <rdf:type rdf:resource="http://www.w3.org/2002/07/owl#ObjectProperty"/>
    <owl:inverseOf rdf:resource="http://vocab.getty.edu/ontology#ulan1514_gandparent_of"/>
  </rdf:Description>
  <rdf:Description rdf:about="http://vocab.getty.edu/ontology#biography">
    <rdfs:isDefinedBy rdf:resource="http://vocab.getty.edu/ontology"/>
    <dct:description>Biography of an ULAN agent. Domain is schema:Person/Organization, range is gvp:Biography. The preferred biography fields are also directly available in the Person/Organization</dct:description>
    <skos:prefLabel>biography</skos:prefLabel>
    <rdfs:range rdf:resource="http://vocab.getty.edu/ontology#Biography"/>
    <rdf:type rdf:resource="http://www.w3.org/2002/07/owl#ObjectProperty"/>
    <rdfs:subPropertyOf rdf:resource="http://vocab.getty.edu/ontology#biography"/>
    <rdfs:comment>Biography of an ULAN agent. Domain is schema:Person/Organization, range is gvp:Biography. The preferred biography fields are also directly available in the Person/Organization</rdfs:comment>
    <rdfs:label>biography</rdfs:label>
  </rdf:Description>
  <rdf:Description rdf:about="http://vocab.getty.edu/term/POS/BothSingularAndPlural">
    <skos:notation>B</skos:notation>
    <rdf:type rdf:resource="http://www.w3.org/2004/02/skos/core#Concept"/>
    <skos:prefLabel>Both Singular and Plural</skos:prefLabel>
    <skos:scopeNote>A term that is used for both the singular and plural in the same language</skos:scopeNote>
    <skos:example>"chassis" is both singular and plural in French</skos:example>
    <dct:description>A term that is used for both the singular and plural in the same language.
Example: "chassis" is both singular and plural in French</dct:description>
    <skos:inScheme rdf:resource="http://vocab.getty.edu/term/POS/"/>
  </rdf:Description>
  <rdf:Description rdf:about="http://vocab.getty.edu/ontology#aat2885_involves">
    <rdfs:subPropertyOf rdf:resource="http://www.w3.org/2004/02/skos/core#related"/>
    <rdfs:isDefinedBy rdf:resource="http://vocab.getty.edu/ontology"/>
    <rdf:type rdf:resource="http://www.w3.org/2002/07/owl#ObjectProperty"/>
    <skos:example>Celtic culture involves Celtic crosses (design motif)</skos:example>
    <skos:prefLabel>aat2885_involves</skos:prefLabel>
    <skos:example>climate change involves climate</skos:example>
    <rdfs:range rdf:resource="http://www.w3.org/2004/02/skos/core#Concept"/>
    <skos:example>infestation involves insect damage</skos:example>
    <rdfs:domain rdf:resource="http://www.w3.org/2004/02/skos/core#Concept"/>
    <dc:title>involves - attributes /associated concepts</dc:title>
    <dc:identifier>2885</dc:identifier>
    <dct:description>any - involves - attributes /associated concepts.&#13;
Example: climate change involves climate;  infestation involves insect damage; Celtic culture involves Celtic crosses (design motif)</dct:description>
    <rdfs:isDefinedBy rdf:resource="http://vocab.getty.edu/aat/"/>
  </rdf:Description>
  <rdf:Description rdf:about="http://vocab.getty.edu/ontology#aat2875_characteristic_of">
    <skos:prefLabel>aat2875_characteristic_of</skos:prefLabel>
    <rdfs:domain rdf:resource="http://www.w3.org/2004/02/skos/core#Concept"/>
    <rdfs:subPropertyOf rdf:resource="http://www.w3.org/2004/02/skos/core#related"/>
    <rdfs:isDefinedBy rdf:resource="http://vocab.getty.edu/ontology"/>
    <skos:example>Celtic (language) was characteristic of Celtic (culture)</skos:example>
    <dc:title>characteristic of - style/period/culture</dc:title>
    <dc:identifier>2875</dc:identifier>
    <dct:description>language - [is] characteristic of - style/period/culture.&#13;
Example: Afar (language) is characteristic of Afar (culture); Celtic (language) was characteristic of Celtic (culture)</dct:description>
    <rdfs:isDefinedBy rdf:resource="http://vocab.getty.edu/aat/"/>
    <rdf:type rdf:resource="http://www.w3.org/2002/07/owl#ObjectProperty"/>
    <rdfs:range rdf:resource="http://www.w3.org/2004/02/skos/core#Concept"/>
    <skos:example>Afar (language) is characteristic of Afar (culture)</skos:example>
    <owl:inverseOf rdf:resource="http://vocab.getty.edu/ontology#aat2876_characterized_by"/>
  </rdf:Description>
  <rdf:Description rdf:about="http://vocab.getty.edu/ontology#aat2601_possessed_by-existing_in">
    <skos:example>adulthood is possessed by/existing in adults</skos:example>
    <rdfs:subPropertyOf rdf:resource="http://www.w3.org/2004/02/skos/core#related"/>
    <rdfs:isDefinedBy rdf:resource="http://vocab.getty.edu/ontology"/>
    <skos:prefLabel>aat2601_possessed_by-existing_in</skos:prefLabel>
    <owl:inverseOf rdf:resource="http://vocab.getty.edu/ontology#aat2602_possess-exist_in"/>
    <dc:identifier>2601</dc:identifier>
    <rdfs:isDefinedBy rdf:resource="http://vocab.getty.edu/aat/"/>
    <rdfs:domain rdf:resource="http://www.w3.org/2004/02/skos/core#Concept"/>
    <rdf:type rdf:resource="http://www.w3.org/2002/07/owl#ObjectProperty"/>
    <dct:description>attributes /associated concepts - [is] possessed by/existing in - role [of actors].&#13;
Example: adulthood is possessed by/existing in adults; nomadism is possessed by/existing in nomads</dct:description>
    <dc:title>possessed by/existing in - role</dc:title>
    <rdfs:range rdf:resource="http://www.w3.org/2004/02/skos/core#Concept"/>
    <skos:example>nomadism is possessed by/existing in nomads</skos:example>
  </rdf:Description>
  <rdf:Description rdf:about="http://vocab.getty.edu/ontology#sourceNonPreferred">
    <rdfs:range rdf:resource="http://purl.org/ontology/bibo/Document"/>
    <rdfs:comment>Source for which the term is Non-preferred. Range is bibo:Document or bibo:DocumentPart</rdfs:comment>
    <rdf:type rdf:resource="http://www.w3.org/2002/07/owl#ObjectProperty"/>
    <rdfs:subPropertyOf rdf:resource="http://purl.org/dc/terms/source"/>
    <rdfs:domain rdf:resource="http://www.w3.org/2008/05/skos-xl#Label"/>
    <skos:example>"Panderma" is non-preferred in Webster's New Geographical Dictionary (1988)</skos:example>
    <skos:prefLabel>sourceNonPreferred</skos:prefLabel>
    <rdfs:label>sourceNonPreferred</rdfs:label>
    <dct:description>Source for which the term is Non-preferred. Range is bibo:Document or bibo:DocumentPart.
Example: "Panderma" is non-preferred in Webster's New Geographical Dictionary (1988)</dct:description>
    <rdfs:isDefinedBy rdf:resource="http://vocab.getty.edu/ontology"/>
  </rdf:Description>
  <rdf:Description rdf:about="http://vocab.getty.edu/ontology#aat2285_practiced-studied_by">
    <rdfs:isDefinedBy rdf:resource="http://vocab.getty.edu/ontology"/>
    <rdfs:domain rdf:resource="http://www.w3.org/2004/02/skos/core#Concept"/>
    <rdfs:isDefinedBy rdf:resource="http://vocab.getty.edu/aat/"/>
    <rdfs:range rdf:resource="http://www.w3.org/2004/02/skos/core#Concept"/>
    <skos:prefLabel>aat2285_practiced-studied_by</skos:prefLabel>
    <dc:identifier>2285</dc:identifier>
    <skos:example>architectural history is practiced/studied by architectural historians</skos:example>
    <owl:inverseOf rdf:resource="http://vocab.getty.edu/ontology#aat2286_practice-study"/>
    <rdf:type rdf:resource="http://www.w3.org/2002/07/owl#ObjectProperty"/>
    <skos:example>Egyptology is practiced/studied by Egyptologists</skos:example>
    <rdfs:subPropertyOf rdf:resource="http://www.w3.org/2004/02/skos/core#related"/>
    <dct:description>field [of study, genre]/discipline - [is] practiced/studied by - a role.&#13;
Example: Egyptology is practiced/studied by Egyptologists; architectural history is practiced/studied by architectural historians</dct:description>
    <dc:title>practiced/studied by - role</dc:title>
  </rdf:Description>
  <rdf:Description rdf:about="http://vocab.getty.edu/ontology#aat2326_create">
    <skos:example>poets create poems</skos:example>
    <rdfs:isDefinedBy rdf:resource="http://vocab.getty.edu/aat/"/>
    <skos:prefLabel>aat2326_create</skos:prefLabel>
    <skos:example>draftsmen create drawings</skos:example>
    <rdf:type rdf:resource="http://www.w3.org/2002/07/owl#ObjectProperty"/>
    <rdfs:subPropertyOf rdf:resource="http://www.w3.org/2004/02/skos/core#related"/>
    <dct:description>[actors having] role - create - things.&#13;
Example: draftsmen create drawings; poets create poems</dct:description>
    <dc:title>create - things</dc:title>
    <dc:identifier>2326</dc:identifier>
    <rdfs:domain rdf:resource="http://www.w3.org/2004/02/skos/core#Concept"/>
    <rdfs:range rdf:resource="http://www.w3.org/2004/02/skos/core#Concept"/>
    <rdfs:isDefinedBy rdf:resource="http://vocab.getty.edu/ontology"/>
  </rdf:Description>
  <rdf:Description rdf:about="http://vocab.getty.edu/term/POS/Adjectival">
    <skos:inScheme rdf:resource="http://vocab.getty.edu/term/POS/"/>
    <skos:prefLabel>Adjectival</skos:prefLabel>
    <skos:notation>A</skos:notation>
    <dct:description>This term may be combined with others in post-coordinated compound terms.
Example: "Renaissance" (as in "Renaissance cathedral"), "painter's" (as in "painter's smock")</dct:description>
    <skos:scopeNote>This term may be combined with others in post-coordinated compound terms</skos:scopeNote>
    <rdf:type rdf:resource="http://www.w3.org/2004/02/skos/core#Concept"/>
    <skos:example>"Renaissance" (as in "Renaissance cathedral"), "painter's" (as in "painter's smock")</skos:example>
  </rdf:Description>
  <rdf:Description rdf:about="http://vocab.getty.edu/ontology#estEnd">
    <rdfs:label>estEnd</rdfs:label>
    <rdfs:comment>Estimated end date of term, relation, type assignment, event, biography</rdfs:comment>
    <dct:description>Estimated end date of term, relation, type assignment, event, biography</dct:description>
    <skos:prefLabel>estEnd</skos:prefLabel>
    <rdfs:isDefinedBy rdf:resource="http://vocab.getty.edu/ontology"/>
    <rdf:type rdf:resource="http://www.w3.org/2002/07/owl#DatatypeProperty"/>
  </rdf:Description>
  <rdf:Description rdf:about="http://vocab.getty.edu/ontology#ulan2677_teacher_was">
    <rdfs:isDefinedBy rdf:resource="http://vocab.getty.edu/ulan/"/>
    <dc:identifier>2677</dc:identifier>
    <rdfs:domain rdf:resource="http://www.w3.org/2004/02/skos/core#Concept"/>
    <rdfs:range rdf:resource="http://www.w3.org/2004/02/skos/core#Concept"/>
    <rdfs:isDefinedBy rdf:resource="http://vocab.getty.edu/ontology"/>
    <dct:description>institution - teacher was - person.&#13;
Example: A teacher at Black Mountain College was Willem De Kooning</dct:description>
    <dc:title>teacher was - person</dc:title>
    <skos:example>A teacher at Black Mountain College was Willem De Kooning</skos:example>
    <skos:prefLabel>ulan2677_teacher_was</skos:prefLabel>
    <rdf:type rdf:resource="http://www.w3.org/2002/07/owl#ObjectProperty"/>
    <rdfs:subPropertyOf rdf:resource="http://www.w3.org/2004/02/skos/core#related"/>
  </rdf:Description>
  <rdf:Description rdf:about="http://vocab.getty.edu/ontology#UnknownPersonConcept">
    <rdfs:comment>Unknown person representing a nationality/culture (the Unknown People by Culture facet)</rdfs:comment>
    <rdfs:subClassOf rdf:resource="http://www.w3.org/2004/02/skos/core#Concept"/>
    <skos:example>500355202 Unknown Bulgarian (modern) (ULAN)</skos:example>
    <dct:description>Unknown person representing a nationality/culture (the Unknown People by Culture facet).
Example: 500355202 Unknown Bulgarian (modern) (ULAN)</dct:description>
    <rdfs:isDefinedBy rdf:resource="http://vocab.getty.edu/ontology"/>
    <skos:prefLabel>UnknownPersonConcept</skos:prefLabel>
    <rdfs:label>UnknownPersonConcept</rdfs:label>
    <rdf:type rdf:resource="http://www.w3.org/2002/07/owl#Class"/>
    <rdfs:subClassOf rdf:resource="http://vocab.getty.edu/ontology#Subject"/>
  </rdf:Description>
  <rdf:Description rdf:about="http://vocab.getty.edu/ontology#ulan1556_half-sibling_of">
    <dct:description>person - half-sibling of - person.&#13;
Example: Juan Bautista Monegro and Luis de Carbajal are half siblings</dct:description>
    <rdf:type rdf:resource="http://www.w3.org/2002/07/owl#ObjectProperty"/>
    <rdfs:range rdf:resource="http://www.w3.org/2004/02/skos/core#Concept"/>
    <dc:title>half-sibling of - person</dc:title>
    <skos:prefLabel>ulan1556_half-sibling_of</skos:prefLabel>
    <skos:example>Juan Bautista Monegro and Luis de Carbajal are half siblings</skos:example>
    <rdfs:subPropertyOf rdf:resource="http://www.w3.org/2004/02/skos/core#related"/>
    <rdfs:isDefinedBy rdf:resource="http://vocab.getty.edu/ulan/"/>
    <dc:identifier>1556</dc:identifier>
    <rdf:type rdf:resource="http://www.w3.org/2002/07/owl#SymmetricProperty"/>
    <rdfs:isDefinedBy rdf:resource="http://vocab.getty.edu/ontology"/>
    <rdfs:domain rdf:resource="http://www.w3.org/2004/02/skos/core#Concept"/>
  </rdf:Description>
  <rdf:Description rdf:about="http://vocab.getty.edu/term/type/">
    <dct:description>Term Type concept scheme</dct:description>
    <rdfs:label>Term Type concept scheme</rdfs:label>
    <rdfs:isDefinedBy rdf:resource="http://vocab.getty.edu/ontology"/>
    <rdf:type rdf:resource="http://www.w3.org/2004/02/skos/core#ConceptScheme"/>
    <skos:prefLabel>Term Type concept scheme</skos:prefLabel>
  </rdf:Description>
  <rdf:Description rdf:about="http://vocab.getty.edu/ontology#Infer_broaderNonConcept_PropChainType2">
    <rdf:type rdf:resource="http://www.ontotext.com/proton/protontop#PropChainType2"/>
    <ptop:premise2 rdf:resource="http://vocab.getty.edu/ontology#broader"/>
    <ptop:conclusion rdf:resource="http://vocab.getty.edu/ontology#broaderNonConcept"/>
    <ptop:premise1 rdf:resource="http://vocab.getty.edu/ontology#broaderNonConcept"/>
    <ptop:type2 rdf:resource="http://vocab.getty.edu/ontology#GuideTerm"/>
  </rdf:Description>
  <rdf:Description rdf:about="http://vocab.getty.edu/ontology#tgn3001_distinguished_from">
    <rdfs:domain rdf:resource="http://www.w3.org/2004/02/skos/core#Concept"/>
    <dc:identifier>3001</dc:identifier>
    <dc:title>distinguished from - any</dc:title>
    <skos:prefLabel>tgn3001_distinguished_from</skos:prefLabel>
    <rdf:type rdf:resource="http://www.w3.org/2002/07/owl#ObjectProperty"/>
    <rdfs:isDefinedBy rdf:resource="http://vocab.getty.edu/tgn/"/>
    <rdfs:subPropertyOf rdf:resource="http://www.w3.org/2004/02/skos/core#related"/>
    <skos:example>The Ancient Mesopotamian Kingdom 'Assyria' is distinguished from the Roman Province of the same name</skos:example>
    <rdfs:range rdf:resource="http://www.w3.org/2004/02/skos/core#Concept"/>
    <rdfs:isDefinedBy rdf:resource="http://vocab.getty.edu/ontology"/>
    <dct:description>any - distinguished from - any.&#13;
Example: The Ancient Mesopotamian Kingdom 'Assyria' is distinguished from the Roman Province of the same name</dct:description>
    <rdf:type rdf:resource="http://www.w3.org/2002/07/owl#SymmetricProperty"/>
  </rdf:Description>
  <rdf:Description rdf:nodeID="N2a7944f25ea0429e8be3f707b7513b55">
    <rdf:rest rdf:resource="http://www.w3.org/1999/02/22-rdf-syntax-ns#nil"/>
    <rdf:first rdf:resource="http://vocab.getty.edu/ontology#broaderPartitiveExtended"/>
  </rdf:Description>
  <rdf:Description rdf:about="http://vocab.getty.edu/ontology#aat2508_produced-processed_by">
    <rdfs:range rdf:resource="http://www.w3.org/2004/02/skos/core#Concept"/>
    <dc:identifier>2508</dc:identifier>
    <rdfs:isDefinedBy rdf:resource="http://vocab.getty.edu/aat/"/>
    <dct:description>material - [is] produced/processed by - things/[equipment].&#13;
Example: cotton gins produce/process cotton (fiber); waterwells produce/process groundwater</dct:description>
    <skos:example>waterwells produce/process groundwater</skos:example>
    <dc:title>produced/processed by - things</dc:title>
    <skos:prefLabel>aat2508_produced-processed_by</skos:prefLabel>
    <rdf:type rdf:resource="http://www.w3.org/2002/07/owl#ObjectProperty"/>
    <rdfs:subPropertyOf rdf:resource="http://www.w3.org/2004/02/skos/core#related"/>
    <rdfs:domain rdf:resource="http://www.w3.org/2004/02/skos/core#Concept"/>
    <skos:example>cotton gins produce/process cotton (fiber)</skos:example>
    <rdfs:isDefinedBy rdf:resource="http://vocab.getty.edu/ontology"/>
  </rdf:Description>
  <rdf:Description rdf:about="http://vocab.getty.edu/term/kind/Code">
    <skos:notation>79000</skos:notation>
    <skos:scopeNote>Code, similar to Abbreviation</skos:scopeNote>
    <skos:example>"sq yds", "m2"</skos:example>
    <skos:prefLabel>Code</skos:prefLabel>
    <rdf:type rdf:resource="http://www.w3.org/2004/02/skos/core#Concept"/>
    <dct:description>Code, similar to Abbreviation.
Example: "sq yds", "m2"</dct:description>
    <skos:inScheme rdf:resource="http://vocab.getty.edu/term/kind/"/>
  </rdf:Description>
  <rdf:Description rdf:about="http://vocab.getty.edu/ontology#ulan2576_patron_of">
    <rdf:type rdf:resource="http://www.w3.org/2002/07/owl#ObjectProperty"/>
    <owl:inverseOf rdf:resource="http://vocab.getty.edu/ontology#ulan2577_patron_was"/>
    <rdfs:isDefinedBy rdf:resource="http://vocab.getty.edu/ulan/"/>
    <rdfs:subPropertyOf rdf:resource="http://www.w3.org/2004/02/skos/core#related"/>
    <rdfs:isDefinedBy rdf:resource="http://vocab.getty.edu/ontology"/>
    <rdfs:domain rdf:resource="http://www.w3.org/2004/02/skos/core#Concept"/>
    <skos:example>The patron of William Chambers was James Caulfiel, Earl of Charlemont</skos:example>
    <dct:description>person - patron of - person.&#13;
Example: The patron of William Chambers was James Caulfiel, Earl of Charlemont</dct:description>
    <rdfs:range rdf:resource="http://www.w3.org/2004/02/skos/core#Concept"/>
    <skos:prefLabel>ulan2576_patron_of</skos:prefLabel>
    <dc:title>patron of - person</dc:title>
    <dc:identifier>2576</dc:identifier>
  </rdf:Description>
  <rdf:Description rdf:about="http://vocab.getty.edu/ontology#broaderNonConcept">
    <rdfs:isDefinedBy rdf:resource="http://vocab.getty.edu/ontology"/>
    <rdfs:domain rdf:resource="http://www.w3.org/2004/02/skos/core#Concept"/>
    <rdfs:comment>Chain of gvp:broader from Concept to GuideTerms, without intervening Concept</rdfs:comment>
    <dct:description>Chain of gvp:broader from Concept to GuideTerms, without intervening Concept</dct:description>
    <rdfs:label>broaderNonConcept</rdfs:label>
    <rdf:type rdf:resource="http://www.w3.org/2002/07/owl#ObjectProperty"/>
    <rdfs:range rdf:resource="http://vocab.getty.edu/ontology#GuideTerm"/>
    <skos:prefLabel>broaderNonConcept</skos:prefLabel>
  </rdf:Description>
  <rdf:Description rdf:about="http://vocab.getty.edu/ontology#aat2408_locus-setting_for">
    <skos:example>schools (buildings) are the locus/setting for education</skos:example>
    <rdf:type rdf:resource="http://www.w3.org/2002/07/owl#ObjectProperty"/>
    <rdfs:domain rdf:resource="http://www.w3.org/2004/02/skos/core#Concept"/>
    <rdfs:isDefinedBy rdf:resource="http://vocab.getty.edu/aat/"/>
    <dc:title>locus/setting for - field/discipline</dc:title>
    <skos:prefLabel>aat2408_locus-setting_for</skos:prefLabel>
    <owl:inverseOf rdf:resource="http://vocab.getty.edu/ontology#aat2409_takes_place_in"/>
    <dc:identifier>2408</dc:identifier>
    <rdfs:subPropertyOf rdf:resource="http://www.w3.org/2004/02/skos/core#related"/>
    <rdfs:isDefinedBy rdf:resource="http://vocab.getty.edu/ontology"/>
    <skos:example>hospitals (buildings) are the locus/setting for medicine (discipline)</skos:example>
    <rdfs:range rdf:resource="http://www.w3.org/2004/02/skos/core#Concept"/>
    <dct:description>locus/setting - [is] locus/setting for - field of study/discipline.&#13;
Example: schools (buildings) are the locus/setting for education; hospitals (buildings) are the locus/setting for medicine (discipline)</dct:description>
  </rdf:Description>
  <rdf:Description rdf:about="http://www.w3.org/2004/02/skos/core#prefLabel">
    <owl:propertyChainAxiom rdf:nodeID="N1ebab3ef3fac45408d3bd583c808ce8a"/>
  </rdf:Description>
  <rdf:Description rdf:nodeID="N6b1e97a28ead495895d1bc18dbd2d7fc">
    <rdf:rest rdf:nodeID="Ncc02757da87c49bab0218490b9be41c3"/>
    <rdf:first rdf:resource="http://vocab.getty.edu/ontology#broaderGenericExtended"/>
  </rdf:Description>
  <rdf:Description rdf:about="http://vocab.getty.edu/historic/current">
    <rdf:type rdf:resource="http://www.w3.org/2004/02/skos/core#Concept"/>
    <skos:inScheme rdf:resource="http://vocab.getty.edu/historic/"/>
    <skos:scopeNote>Valid/used currently</skos:scopeNote>
    <dct:description>Valid/used currently</dct:description>
    <skos:prefLabel>Current</skos:prefLabel>
    <skos:notation>C</skos:notation>
  </rdf:Description>
  <rdf:Description rdf:about="http://vocab.getty.edu/ontology#aat2219_have_form">
    <rdfs:subPropertyOf rdf:resource="http://www.w3.org/2004/02/skos/core#related"/>
    <dc:title>have form - things</dc:title>
    <rdfs:isDefinedBy rdf:resource="http://vocab.getty.edu/ontology"/>
    <skos:example>cartoons (working drawings) have the form of toile peinte</skos:example>
    <rdfs:domain rdf:resource="http://www.w3.org/2004/02/skos/core#Concept"/>
    <dct:description>things - have form [of] - things.&#13;
Example: lighthouse lamps have the form of arc lamps; cartoons (working drawings) have the form of toile peinte</dct:description>
    <skos:example>lighthouse lamps have the form of arc lamps</skos:example>
    <skos:prefLabel>aat2219_have_form</skos:prefLabel>
    <rdf:type rdf:resource="http://www.w3.org/2002/07/owl#ObjectProperty"/>
    <rdfs:range rdf:resource="http://www.w3.org/2004/02/skos/core#Concept"/>
    <rdfs:isDefinedBy rdf:resource="http://vocab.getty.edu/aat/"/>
    <dc:identifier>2219</dc:identifier>
  </rdf:Description>
  <rdf:Description rdf:about="http://vocab.getty.edu/ontology#aat2894_exemplified_by">
    <dct:description>activity/event/[process/function] - [is] exemplified by - brand name.&#13;
Example: deacidification [process/function] is exemplified by Papersave Process (TM)</dct:description>
    <rdfs:range rdf:resource="http://www.w3.org/2004/02/skos/core#Concept"/>
    <owl:inverseOf rdf:resource="http://vocab.getty.edu/ontology#aat2895_example_of"/>
    <skos:prefLabel>aat2894_exemplified_by</skos:prefLabel>
    <dc:title>exemplified by - brand name</dc:title>
    <rdfs:isDefinedBy rdf:resource="http://vocab.getty.edu/aat/"/>
    <rdfs:subPropertyOf rdf:resource="http://www.w3.org/2004/02/skos/core#related"/>
    <rdf:type rdf:resource="http://www.w3.org/2002/07/owl#ObjectProperty"/>
    <dc:identifier>2894</dc:identifier>
    <rdfs:domain rdf:resource="http://www.w3.org/2004/02/skos/core#Concept"/>
    <rdfs:isDefinedBy rdf:resource="http://vocab.getty.edu/ontology"/>
    <skos:example>deacidification [process/function] is exemplified by Papersave Process (TM)</skos:example>
  </rdf:Description>
  <rdf:Description rdf:about="http://vocab.getty.edu/ontology#ulan1571_guardian_of">
    <dct:description>person - guardian of - person.&#13;
Example: John Hoskins, the elder was the guardian of Samuel Cooper</dct:description>
    <rdf:type rdf:resource="http://www.w3.org/2002/07/owl#ObjectProperty"/>
    <rdfs:isDefinedBy rdf:resource="http://vocab.getty.edu/ulan/"/>
    <dc:identifier>1571</dc:identifier>
    <skos:prefLabel>ulan1571_guardian_of</skos:prefLabel>
    <skos:example>John Hoskins, the elder was the guardian of Samuel Cooper</skos:example>
    <owl:inverseOf rdf:resource="http://vocab.getty.edu/ontology#ulan1573_ward_of"/>
    <dc:title>guardian of - person</dc:title>
    <rdfs:isDefinedBy rdf:resource="http://vocab.getty.edu/ontology"/>
    <rdfs:subPropertyOf rdf:resource="http://www.w3.org/2004/02/skos/core#related"/>
    <rdfs:domain rdf:resource="http://www.w3.org/2004/02/skos/core#Concept"/>
    <rdfs:range rdf:resource="http://www.w3.org/2004/02/skos/core#Concept"/>
  </rdf:Description>
  <rdf:Description rdf:about="http://vocab.getty.edu/ontology#aat2427_produced_by">
    <rdf:type rdf:resource="http://www.w3.org/2002/07/owl#ObjectProperty"/>
    <dc:title>produced by - activity/event/process</dc:title>
    <dct:description>things - [are] produced by - activity/event/process.&#13;
Example: vase paintings (visual works) are produced by vase painting (image making); forgeries are produced by forging (copying)</dct:description>
    <rdfs:isDefinedBy rdf:resource="http://vocab.getty.edu/aat/"/>
    <rdfs:range rdf:resource="http://www.w3.org/2004/02/skos/core#Concept"/>
    <skos:example>vase paintings (visual works) are produced by vase painting (image making)</skos:example>
    <skos:example>forgeries are produced by forging (copying)</skos:example>
    <rdfs:subPropertyOf rdf:resource="http://www.w3.org/2004/02/skos/core#related"/>
    <skos:prefLabel>aat2427_produced_by</skos:prefLabel>
    <owl:inverseOf rdf:resource="http://vocab.getty.edu/ontology#aat2428_produces"/>
    <dc:identifier>2427</dc:identifier>
    <rdfs:isDefinedBy rdf:resource="http://vocab.getty.edu/ontology"/>
    <rdfs:domain rdf:resource="http://www.w3.org/2004/02/skos/core#Concept"/>
  </rdf:Description>
  <rdf:Description rdf:about="http://vocab.getty.edu/ontology#broaderPreferred">
    <skos:prefLabel>broaderPreferred</skos:prefLabel>
    <rdfs:isDefinedBy rdf:resource="http://vocab.getty.edu/ontology"/>
    <rdfs:label>broaderPreferred</rdfs:label>
    <rdfs:subPropertyOf rdf:resource="http://vocab.getty.edu/ontology#broaderPreferredExtended"/>
    <rdfs:range rdf:resource="http://vocab.getty.edu/ontology#Subject"/>
    <rdf:type rdf:resource="http://www.w3.org/2002/07/owl#ObjectProperty"/>
    <rdfs:subPropertyOf rdf:resource="http://vocab.getty.edu/ontology#broader"/>
    <skos:example>Preferred: "baking dishes" (AAT) BTG "bakeware" (AAT); Sofia (TGN) BTP Bulgaria (TGN)</skos:example>
    <rdfs:comment>Main parent of a subject. Needed to display the hierarchy</rdfs:comment>
    <rdfs:domain rdf:resource="http://vocab.getty.edu/ontology#Subject"/>
    <dct:description>Main parent of a subject. Needed to display the hierarchy.
Example: Preferred: "baking dishes" (AAT) BTG "bakeware" (AAT); Sofia (TGN) BTP Bulgaria (TGN)</dct:description>
  </rdf:Description>
  <rdf:Description rdf:about="http://vocab.getty.edu/ontology#PhysPlaceConcept">
    <skos:prefLabel>PhysPlaceConcept</skos:prefLabel>
    <dct:description>Physical feature, defined by its physical characteristics on planet Earth, including mountains, rivers, and oceans. Used in TGN only.
Example: Amazon River (TGN)</dct:description>
    <rdf:type rdf:resource="http://www.w3.org/2002/07/owl#Class"/>
    <rdfs:label>PhysPlaceConcept</rdfs:label>
    <rdfs:subClassOf rdf:resource="http://www.w3.org/2004/02/skos/core#Concept"/>
    <rdfs:isDefinedBy rdf:resource="http://vocab.getty.edu/ontology"/>
    <rdfs:subClassOf rdf:resource="http://vocab.getty.edu/ontology#Subject"/>
    <skos:example>Amazon River (TGN)</skos:example>
    <rdfs:comment>Physical feature, defined by its physical characteristics on planet Earth, including mountains, rivers, and oceans. Used in TGN only</rdfs:comment>
  </rdf:Description>
  <rdf:Description rdf:about="http://vocab.getty.edu/term/type/Descriptor">
    <skos:example>"manuscripts" (English)</skos:example>
    <skos:inScheme rdf:resource="http://vocab.getty.edu/term/type/"/>
    <skos:prefLabel>Descriptor</skos:prefLabel>
    <skos:scopeNote>Main term. Getty usually uses the plural</skos:scopeNote>
    <dct:description>Main term. Getty usually uses the plural.
Example: "manuscripts" (English)</dct:description>
    <rdf:type rdf:resource="http://www.w3.org/2004/02/skos/core#Concept"/>
    <skos:notation>D</skos:notation>
  </rdf:Description>
  <rdf:Description rdf:nodeID="N91bc116ad3504c77910c359eef18039d">
    <rdf:rest rdf:nodeID="N80f8ad91f64343b6860ccbc070ed4740"/>
    <rdf:first rdf:resource="http://www.w3.org/2008/05/skos-xl#altLabel"/>
  </rdf:Description>
  <rdf:Description rdf:about="http://vocab.getty.edu/ontology#ulan1224_crowned">
    <rdfs:range rdf:resource="http://www.w3.org/2004/02/skos/core#Concept"/>
    <dc:title>crowned - person</dc:title>
    <rdfs:isDefinedBy rdf:resource="http://vocab.getty.edu/ontology"/>
    <dct:description>person - crowned - person.&#13;
Example: Emperor Charlemagne was crowned by Pope Leo III</dct:description>
    <rdfs:domain rdf:resource="http://www.w3.org/2004/02/skos/core#Concept"/>
    <rdfs:isDefinedBy rdf:resource="http://vocab.getty.edu/ulan/"/>
    <dc:identifier>1224</dc:identifier>
    <skos:prefLabel>ulan1224_crowned</skos:prefLabel>
    <skos:example>Emperor Charlemagne was crowned by Pope Leo III</skos:example>
    <rdf:type rdf:resource="http://www.w3.org/2002/07/owl#ObjectProperty"/>
    <rdfs:subPropertyOf rdf:resource="http://www.w3.org/2004/02/skos/core#related"/>
  </rdf:Description>
  <rdf:Description rdf:about="http://vocab.getty.edu/ontology#ulan2841_performer_was">
    <rdfs:isDefinedBy rdf:resource="http://vocab.getty.edu/ontology"/>
    <skos:prefLabel>ulan2841_performer_was</skos:prefLabel>
    <rdfs:isDefinedBy rdf:resource="http://vocab.getty.edu/ulan/"/>
    <dc:identifier>2841</dc:identifier>
    <rdfs:subPropertyOf rdf:resource="http://www.w3.org/2004/02/skos/core#related"/>
    <rdf:type rdf:resource="http://www.w3.org/2002/07/owl#ObjectProperty"/>
    <dc:title>performer was - person</dc:title>
    <rdfs:range rdf:resource="http://www.w3.org/2004/02/skos/core#Concept"/>
    <dct:description>group - performer was - person</dct:description>
    <rdfs:domain rdf:resource="http://www.w3.org/2004/02/skos/core#Concept"/>
  </rdf:Description>
  <rdf:Description rdf:about="http://vocab.getty.edu/ontology#ulan1201_patron_of">
    <rdf:type rdf:resource="http://www.w3.org/2002/07/owl#ObjectProperty"/>
    <dc:title>patron of - person/firm/family</dc:title>
    <rdfs:range rdf:resource="http://www.w3.org/2004/02/skos/core#Concept"/>
    <dc:identifier>1201</dc:identifier>
    <rdfs:domain rdf:resource="http://www.w3.org/2004/02/skos/core#Concept"/>
    <rdfs:isDefinedBy rdf:resource="http://vocab.getty.edu/ontology"/>
    <dct:description>person - patron of - person/firm/family.&#13;
Example: Cosimo I, Grand-Duke of Tuscany was the patron of Donatello</dct:description>
    <skos:example>Cosimo I, Grand-Duke of Tuscany was the patron of Donatello</skos:example>
    <rdfs:isDefinedBy rdf:resource="http://vocab.getty.edu/ulan/"/>
    <skos:prefLabel>ulan1201_patron_of</skos:prefLabel>
    <owl:inverseOf rdf:resource="http://vocab.getty.edu/ontology#ulan1202_patron_was"/>
    <rdfs:subPropertyOf rdf:resource="http://www.w3.org/2004/02/skos/core#related"/>
  </rdf:Description>
  <rdf:Description rdf:about="http://vocab.getty.edu/historic/">
    <rdfs:label>Historic Flag concept scheme</rdfs:label>
    <rdf:type rdf:resource="http://www.w3.org/2004/02/skos/core#ConceptScheme"/>
    <rdfs:isDefinedBy rdf:resource="http://vocab.getty.edu/ontology"/>
    <dct:description>Historic Flag concept scheme</dct:description>
    <skos:prefLabel>Historic Flag concept scheme</skos:prefLabel>
  </rdf:Description>
  <rdf:Description rdf:nodeID="N80f8ad91f64343b6860ccbc070ed4740">
    <rdf:rest rdf:resource="http://www.w3.org/1999/02/22-rdf-syntax-ns#nil"/>
    <rdf:first rdf:resource="http://www.w3.org/2008/05/skos-xl#literalForm"/>
  </rdf:Description>
  <rdf:Description rdf:about="http://vocab.getty.edu/ontology#ScopeNote">
    <rdfs:isDefinedBy rdf:resource="http://vocab.getty.edu/ontology"/>
    <rdfs:comment>Defines a GVP subject or provides usage information. Has fields:
- dc:identifier: numeric ID, also used in the URL.
- rdf:value: the note itself (as per SKOS Primer: 4.2 Advanced Documentation Features) with language tag
- dct:language: matches the language tag
- gvp:displayOrder, order of this note amongst others
- gvp:historicFlag, gvp:estStart, gvp:estEnd, rdfs:comment: Historic Information about applicability
- dct:source or subproperties thereof 
- dct:contributor or subproperties thereof</rdfs:comment>
    <rdf:type rdf:resource="http://www.w3.org/2002/07/owl#Class"/>
    <dct:description>Defines a GVP subject or provides usage information. Has fields:
- dc:identifier: numeric ID, also used in the URL.
- rdf:value: the note itself (as per SKOS Primer: 4.2 Advanced Documentation Features) with language tag
- dct:language: matches the language tag
- gvp:displayOrder, order of this note amongst others
- gvp:historicFlag, vp:estStart, gvp:estEnd, rdfs:comment: Historic Information about applicability
- dct:source or subproperties thereof 
- dct:contributor or subproperties thereof</dct:description>
  </rdf:Description>
  <rdf:Description rdf:about="http://vocab.getty.edu/ontology#aat2886_used-function_as">
    <rdfs:range rdf:resource="http://www.w3.org/2004/02/skos/core#Concept"/>
    <dc:title>used/function as - material</dc:title>
    <rdf:type rdf:resource="http://www.w3.org/2002/07/owl#ObjectProperty"/>
    <rdfs:isDefinedBy rdf:resource="http://vocab.getty.edu/aat/"/>
    <dc:identifier>2886</dc:identifier>
    <skos:example>carbon disulfide - is used/functions as - solvent</skos:example>
    <rdfs:subPropertyOf rdf:resource="http://www.w3.org/2004/02/skos/core#related"/>
    <rdfs:domain rdf:resource="http://www.w3.org/2004/02/skos/core#Concept"/>
    <skos:prefLabel>aat2886_used-function_as</skos:prefLabel>
    <dct:description>material - used/function as - material.&#13;
Example: carbon disulfide - is used/functions as - solvent</dct:description>
    <rdfs:isDefinedBy rdf:resource="http://vocab.getty.edu/ontology"/>
    <owl:inverseOf rdf:resource="http://vocab.getty.edu/ontology#aat2887_exemplified_by"/>
  </rdf:Description>
  <rdf:Description rdf:about="http://www.w3.org/2004/02/skos/core#altLabel">
    <owl:propertyChainAxiom rdf:nodeID="N91bc116ad3504c77910c359eef18039d"/>
  </rdf:Description>
  <rdf:Description rdf:about="http://vocab.getty.edu/ontology#Infer_broaderPreferredExtended">
    <ptop:premise1 rdf:resource="http://vocab.getty.edu/ontology#broaderPreferredExtended"/>
    <ptop:conclusion rdf:resource="http://vocab.getty.edu/ontology#broaderPreferredExtended"/>
    <ptop:restriction rdf:resource="http://vocab.getty.edu/ontology#broaderExtended"/>
    <ptop:premise2 rdf:resource="http://vocab.getty.edu/ontology#broaderPreferred"/>
    <rdf:type rdf:resource="http://www.ontotext.com/proton/protontop#PropChainRestr"/>
  </rdf:Description>
  <rdf:Description rdf:about="http://vocab.getty.edu/ontology#Infer_broaderNonConcept_TypeRestr">
    <ptop:type2 rdf:resource="http://vocab.getty.edu/ontology#GuideTerm"/>
    <ptop:conclusion rdf:resource="http://vocab.getty.edu/ontology#broaderNonConcept"/>
    <rdf:type rdf:resource="http://www.ontotext.com/proton/protontop#TypeRestr"/>
    <ptop:premise rdf:resource="http://vocab.getty.edu/ontology#broader"/>
    <ptop:type1 rdf:resource="http://www.w3.org/2004/02/skos/core#Concept"/>
  </rdf:Description>
  <rdf:Description rdf:about="http://vocab.getty.edu/term/flag/">
    <dct:description>Term Flag concept scheme</dct:description>
    <skos:prefLabel>Term Flag concept scheme</skos:prefLabel>
    <rdfs:label>Term Flag concept scheme</rdfs:label>
    <rdf:type rdf:resource="http://www.w3.org/2004/02/skos/core#ConceptScheme"/>
    <rdfs:isDefinedBy rdf:resource="http://vocab.getty.edu/ontology"/>
  </rdf:Description>
  <rdf:Description rdf:about="http://vocab.getty.edu/ontology#ulan2584_chaired_by">
    <rdfs:range rdf:resource="http://www.w3.org/2004/02/skos/core#Concept"/>
    <dc:title>chaired by - person</dc:title>
    <dct:description>institution - chaired by - person</dct:description>
    <rdf:type rdf:resource="http://www.w3.org/2002/07/owl#ObjectProperty"/>
    <dc:identifier>2584</dc:identifier>
    <rdfs:isDefinedBy rdf:resource="http://vocab.getty.edu/ulan/"/>
    <rdfs:subPropertyOf rdf:resource="http://www.w3.org/2004/02/skos/core#related"/>
    <rdfs:domain rdf:resource="http://www.w3.org/2004/02/skos/core#Concept"/>
    <skos:prefLabel>ulan2584_chaired_by</skos:prefLabel>
    <rdfs:isDefinedBy rdf:resource="http://vocab.getty.edu/ontology"/>
  </rdf:Description>
  <rdf:Description rdf:about="http://vocab.getty.edu/ontology#ulan1551_sibling_by_marriage_of">
    <rdfs:domain rdf:resource="http://www.w3.org/2004/02/skos/core#Concept"/>
    <skos:prefLabel>ulan1551_sibling_by_marriage_of</skos:prefLabel>
    <rdf:type rdf:resource="http://www.w3.org/2002/07/owl#ObjectProperty"/>
    <skos:example>Peter Paul Rubens and Susanne Fourment are siblings by marriage</skos:example>
    <dc:title>sibling by marriage of - person</dc:title>
    <rdfs:subPropertyOf rdf:resource="http://www.w3.org/2004/02/skos/core#related"/>
    <rdfs:isDefinedBy rdf:resource="http://vocab.getty.edu/ulan/"/>
    <dct:description>person - sibling by marriage (step sibling) - person.&#13;
Example: Peter Paul Rubens and Susanne Fourment are siblings by marriage</dct:description>
    <rdfs:range rdf:resource="http://www.w3.org/2004/02/skos/core#Concept"/>
    <rdfs:isDefinedBy rdf:resource="http://vocab.getty.edu/ontology"/>
    <dc:identifier>1551</dc:identifier>
    <rdf:type rdf:resource="http://www.w3.org/2002/07/owl#SymmetricProperty"/>
  </rdf:Description>
  <rdf:Description rdf:about="http://vocab.getty.edu/term/kind/BirthName">
    <skos:example>TODO</skos:example>
    <dct:description>Birth Name of an ULAN agent.
Example: TODO</dct:description>
    <skos:notation>BN</skos:notation>
    <rdf:type rdf:resource="http://www.w3.org/2004/02/skos/core#Concept"/>
    <skos:prefLabel>Birth Name</skos:prefLabel>
    <skos:inScheme rdf:resource="http://vocab.getty.edu/term/kind/"/>
    <skos:scopeNote>Birth Name of an ULAN agent</skos:scopeNote>
  </rdf:Description>
  <rdf:Description rdf:nodeID="Nb3697f9ab12f4a61b93a7b0f6ef18ba8">
    <rdf:rest rdf:resource="http://www.w3.org/1999/02/22-rdf-syntax-ns#nil"/>
    <rdf:first rdf:resource="http://vocab.getty.edu/ontology#broaderGeneric"/>
  </rdf:Description>
  <rdf:Description rdf:nodeID="Na4f426f3b86940199dc92fb434c8fc18">
    <rdf:rest rdf:nodeID="N5b11eeca07364f4c9e3107ce462b4750"/>
    <rdf:first rdf:resource="http://vocab.getty.edu/ontology#broaderPartitiveExtended"/>
  </rdf:Description>
  <rdf:Description rdf:about="http://vocab.getty.edu/aat/300189559">
    <skos:exactMatch rdf:resource="http://rdaregistry.info/termList/gender/1002"/>
    <skos:exactMatch rdf:resource="http://www.wikidata.org/entity/Q6581097"/>
  </rdf:Description>
  <rdf:Description rdf:nodeID="N9dc1cffb8d29482c9c782a05a2048ce7">
    <rdf:rest rdf:resource="http://www.w3.org/1999/02/22-rdf-syntax-ns#nil"/>
    <rdf:first rdf:resource="http://www.w3.org/2008/05/skos-xl#literalForm"/>
  </rdf:Description>
  <rdf:Description rdf:about="http://vocab.getty.edu/ontology#Biography">
    <rdfs:isDefinedBy rdf:resource="http://vocab.getty.edu/ontology"/>
    <rdf:type rdf:resource="http://www.w3.org/2002/07/owl#Class"/>
    <rdfs:comment>Biography of a ULAN agent (schema:Person|Organization). Depending on the agent, has these fields:
- schema:description: one-line-biography
- gvp:estStart
- schema:birthPlace | foundationLocation, pointing to TGN
- gvp:estEnd
- schema:deathPlace | dissolutionLocation, pointing to TGN
- schema:gender, pointing to AAT (male, female, other)
- dct:contributor
The fields of the preferred biogrpahy are also available in the agent.</rdfs:comment>
  </rdf:Description>
  <rdf:Description rdf:about="http://www.w3.org/2004/02/skos/core#hiddenLabel">
    <owl:propertyChainAxiom rdf:nodeID="N8c1a90bd131243c0ae4503ccea2e2fb7"/>
  </rdf:Description>
  <rdf:Description rdf:nodeID="Nb537c13fdf6e4e4ebc7554cfedb20057">
    <rdf:first rdf:resource="http://vocab.getty.edu/ontology#broaderInstantialExtended"/>
    <rdf:rest rdf:nodeID="Nb3697f9ab12f4a61b93a7b0f6ef18ba8"/>
  </rdf:Description>
  <rdf:Description rdf:nodeID="Ncc02757da87c49bab0218490b9be41c3">
    <rdf:first rdf:resource="http://vocab.getty.edu/ontology#broaderGeneric"/>
    <rdf:rest rdf:resource="http://www.w3.org/1999/02/22-rdf-syntax-ns#nil"/>
  </rdf:Description>
  <rdf:Description rdf:about="http://purl.org/dc/terms/isReplacedBy">
    <owl:inverseOf rdf:resource="http://purl.org/dc/terms/replaces"/>
  </rdf:Description>
</rdf:RDF>
