<?xml version="1.0" encoding="UTF-8"?>
<rdf:RDF
   xmlns:dc="http://purl.org/dc/elements/1.1/"
   xmlns:dct="http://purl.org/dc/terms/"
   xmlns:foaf="http://xmlns.com/foaf/0.1/"
   xmlns:owl="http://www.w3.org/2002/07/owl#"
   xmlns:ptop="http://www.ontotext.com/proton/protontop#"
   xmlns:rdf="http://www.w3.org/1999/02/22-rdf-syntax-ns#"
   xmlns:rdfs="http://www.w3.org/2000/01/rdf-schema#"
   xmlns:skos="http://www.w3.org/2004/02/skos/core#"
   xmlns:vann="http://purl.org/vocab/vann/"
>
  <rdf:Description rdf:about="http://vocab.getty.edu/ontology#broaderInstantialExtended">
    <rdfs:domain rdf:resource="http://vocab.getty.edu/ontology#Subject"/>
    <rdfs:range rdf:resource="http://vocab.getty.edu/ontology#Subject"/>
    <skos:example>Mt Athos (TGN) BTI orthodox religious center (AAT) BTG Christian religious center (AAT),
so Mt Athos (TGN) BTIE Christian religious center (AAT)</skos:example>
    <skos:prefLabel>broaderInstantialExtended</skos:prefLabel>
    <skos:scopeNote>Ancestors (Instantial). Meaningful closure of gvp:broaderInstantial. Infers iso:broaderInstantial for pairs of directly related skos:Concepts.</skos:scopeNote>
    <owl:propertyChainAxiom rdf:nodeID="N44c4d2cbe9fe489fbe561b09d3239654"/>
    <rdfs:isDefinedBy rdf:resource="http://vocab.getty.edu/ontology"/>
    <rdfs:subPropertyOf rdf:resource="http://vocab.getty.edu/ontology#broaderExtended"/>
    <rdf:type rdf:resource="http://www.w3.org/2002/07/owl#ObjectProperty"/>
    <rdfs:label>broaderInstantialExtended</rdfs:label>
    <dct:description>Ancestors (Instantial). Meaningful closure of gvp:broaderInstantial. Infers iso:broaderInstantial for pairs of directly related skos:Concepts.</dct:description>
  </rdf:Description>
  <rdf:Description rdf:about="http://vocab.getty.edu/ontology#aat2000_related_to">
    <skos:prefLabel>aat2000_related_to</skos:prefLabel>
    <rdf:type rdf:resource="http://www.w3.org/2002/07/owl#SymmetricProperty"/>
    <dc:identifier>2000</dc:identifier>
    <rdfs:domain rdf:resource="http://www.w3.org/2004/02/skos/core#Concept"/>
    <skos:example>gulf red is related to light red (pigment)</skos:example>
    <rdfs:isDefinedBy rdf:resource="http://vocab.getty.edu/aat/"/>
    <dct:description>any - related to - any; generic relationship, not explained.&#13;
Example: gulf red is related to light red (pigment)</dct:description>
    <dc:title>related to - any</dc:title>
    <rdf:type rdf:resource="http://www.w3.org/2002/07/owl#ObjectProperty"/>
    <rdfs:isDefinedBy rdf:resource="http://vocab.getty.edu/ontology"/>
    <skos:scopeNote>generic relationship, not explained</skos:scopeNote>
    <rdfs:range rdf:resource="http://www.w3.org/2004/02/skos/core#Concept"/>
    <rdfs:subPropertyOf rdf:resource="http://www.w3.org/2004/02/skos/core#related"/>
  </rdf:Description>
  <rdf:Description rdf:about="http://vocab.getty.edu/historic/">
    <rdfs:label>Historic Flag concept scheme</rdfs:label>
    <dct:description>Historic Flag concept scheme</dct:description>
    <rdfs:isDefinedBy rdf:resource="http://vocab.getty.edu/ontology"/>
    <rdf:type rdf:resource="http://www.w3.org/2004/02/skos/core#ConceptScheme"/>
    <skos:scopeNote>Historic Flag concept scheme</skos:scopeNote>
    <skos:prefLabel>Historic Flag concept scheme</skos:prefLabel>
  </rdf:Description>
  <rdf:Description rdf:about="http://vocab.getty.edu/ontology#aat2206_caused_by-requires">
    <rdfs:subPropertyOf rdf:resource="http://www.w3.org/2004/02/skos/core#related"/>
    <skos:scopeNote>activity/event/[process/function] - [is] caused by/dependent upon - activity/event/[process/function].&#13;
Example: on-demand publishing is caused by/requires on-demand printing; preservation is caused by/requires preserving</skos:scopeNote>
    <dc:identifier>2206</dc:identifier>
    <skos:prefLabel>aat2206_caused_by-requires</skos:prefLabel>
    <rdfs:range rdf:resource="http://www.w3.org/2004/02/skos/core#Concept"/>
    <rdfs:isDefinedBy rdf:resource="http://vocab.getty.edu/aat/"/>
    <rdfs:domain rdf:resource="http://www.w3.org/2004/02/skos/core#Concept"/>
    <dct:description>activity/event/[process/function] - [is] caused by/dependent upon - activity/event/[process/function].&#13;
Example: on-demand publishing is caused by/requires on-demand printing; preservation is caused by/requires preserving</dct:description>
    <skos:example>preservation is caused by/requires preserving</skos:example>
    <skos:example>on-demand publishing is caused by/requires on-demand printing</skos:example>
    <dc:title>caused by/requires - activity/event</dc:title>
    <rdf:type rdf:resource="http://www.w3.org/2002/07/owl#ObjectProperty"/>
    <rdfs:isDefinedBy rdf:resource="http://vocab.getty.edu/ontology"/>
  </rdf:Description>
  <rdf:Description rdf:about="http://vocab.getty.edu/ontology#ulan1311_partner_of">
    <dct:description>person - partner of - person.&#13;
Example: Frank Gehry and James Glymph are partners</dct:description>
    <rdf:type rdf:resource="http://www.w3.org/2002/07/owl#SymmetricProperty"/>
    <rdfs:domain rdf:resource="http://www.w3.org/2004/02/skos/core#Concept"/>
    <rdfs:range rdf:resource="http://www.w3.org/2004/02/skos/core#Concept"/>
    <dc:identifier>1311</dc:identifier>
    <rdfs:isDefinedBy rdf:resource="http://vocab.getty.edu/ulan/"/>
    <skos:prefLabel>ulan1311_partner_of</skos:prefLabel>
    <dc:title>partner of - person</dc:title>
    <skos:example>Frank Gehry and James Glymph are partners</skos:example>
    <skos:scopeNote>person - partner of - person.&#13;
Example: Frank Gehry and James Glymph are partners</skos:scopeNote>
    <rdfs:subPropertyOf rdf:resource="http://www.w3.org/2004/02/skos/core#related"/>
    <rdfs:isDefinedBy rdf:resource="http://vocab.getty.edu/ontology"/>
    <rdf:type rdf:resource="http://www.w3.org/2002/07/owl#ObjectProperty"/>
  </rdf:Description>
  <rdf:Description rdf:about="http://vocab.getty.edu/ontology#aat2562_locus-setting_for">
    <rdfs:isDefinedBy rdf:resource="http://vocab.getty.edu/aat/"/>
    <dc:identifier>2562</dc:identifier>
    <rdfs:isDefinedBy rdf:resource="http://vocab.getty.edu/ontology"/>
    <skos:scopeNote>locus/setting - [is] locus/setting for - style/period/culture/[religion/ideology].&#13;
Example: First Nations reserves are the locus/setting for First Nations (culture); agraharas are the locus/setting for Brahmanism</skos:scopeNote>
    <rdf:type rdf:resource="http://www.w3.org/2002/07/owl#ObjectProperty"/>
    <rdfs:domain rdf:resource="http://www.w3.org/2004/02/skos/core#Concept"/>
    <rdfs:range rdf:resource="http://www.w3.org/2004/02/skos/core#Concept"/>
    <rdfs:subPropertyOf rdf:resource="http://www.w3.org/2004/02/skos/core#related"/>
    <skos:prefLabel>aat2562_locus-setting_for</skos:prefLabel>
    <dct:description>locus/setting - [is] locus/setting for - style/period/culture/[religion/ideology].&#13;
Example: First Nations reserves are the locus/setting for First Nations (culture); agraharas are the locus/setting for Brahmanism</dct:description>
    <dc:title>locus/setting for - style/period/culture</dc:title>
    <skos:example>agraharas are the locus/setting for Brahmanism</skos:example>
    <owl:inverseOf rdf:resource="http://vocab.getty.edu/ontology#aat2563_located_in"/>
    <skos:example>First Nations reserves are the locus/setting for First Nations (culture)</skos:example>
  </rdf:Description>
  <rdf:Description rdf:about="http://vocab.getty.edu/ontology#ulan1302_associate_of">
    <dc:title>associate of - person</dc:title>
    <rdf:type rdf:resource="http://www.w3.org/2002/07/owl#ObjectProperty"/>
    <skos:prefLabel>ulan1302_associate_of</skos:prefLabel>
    <dct:description>person - associate of - person.&#13;
Example: Frank Lloyd Wright was an associate of Giannini and Hilgart</dct:description>
    <rdfs:domain rdf:resource="http://www.w3.org/2004/02/skos/core#Concept"/>
    <rdfs:isDefinedBy rdf:resource="http://vocab.getty.edu/ulan/"/>
    <dc:identifier>1302</dc:identifier>
    <skos:scopeNote>person - associate of - person.&#13;
Example: Frank Lloyd Wright was an associate of Giannini and Hilgart</skos:scopeNote>
    <skos:example>Frank Lloyd Wright was an associate of Giannini and Hilgart</skos:example>
    <rdfs:isDefinedBy rdf:resource="http://vocab.getty.edu/ontology"/>
    <rdf:type rdf:resource="http://www.w3.org/2002/07/owl#SymmetricProperty"/>
    <rdfs:subPropertyOf rdf:resource="http://www.w3.org/2004/02/skos/core#related"/>
    <rdfs:range rdf:resource="http://www.w3.org/2004/02/skos/core#Concept"/>
  </rdf:Description>
  <rdf:Description rdf:about="http://vocab.getty.edu/ontology#estEnd">
    <skos:scopeNote>Estimated end date of term, relation, type assignment, event, biography</skos:scopeNote>
    <rdfs:comment>Estimated end date of term, relation, type assignment, event, biography</rdfs:comment>
    <rdf:type rdf:resource="http://www.w3.org/2002/07/owl#DatatypeProperty"/>
    <dct:description>Estimated end date of term, relation, type assignment, event, biography</dct:description>
    <rdfs:isDefinedBy rdf:resource="http://vocab.getty.edu/ontology"/>
    <rdfs:label>estEnd</rdfs:label>
    <skos:prefLabel>estEnd</skos:prefLabel>
    <skos:definition>Estimated end date of term, relation, type assignment, event, biography</skos:definition>
  </rdf:Description>
  <rdf:Description rdf:about="http://vocab.getty.edu/ontology#aat2891_exemplified_by">
    <dc:identifier>2891</dc:identifier>
    <rdfs:subPropertyOf rdf:resource="http://www.w3.org/2004/02/skos/core#related"/>
    <rdfs:domain rdf:resource="http://www.w3.org/2004/02/skos/core#Concept"/>
    <dc:title>exemplified by - brand name</dc:title>
    <dct:description>things - [are] exemplied by - brand name.&#13;
Example: photothermographic transfer prints are exemplified by Pictrography (TM) prints</dct:description>
    <skos:scopeNote>things - [are] exemplied by - brand name.&#13;
Example: photothermographic transfer prints are exemplified by Pictrography (TM) prints</skos:scopeNote>
    <rdfs:isDefinedBy rdf:resource="http://vocab.getty.edu/aat/"/>
    <rdf:type rdf:resource="http://www.w3.org/2002/07/owl#ObjectProperty"/>
    <rdfs:isDefinedBy rdf:resource="http://vocab.getty.edu/ontology"/>
    <owl:inverseOf rdf:resource="http://vocab.getty.edu/ontology#aat2892_example_of"/>
    <skos:prefLabel>aat2891_exemplified_by</skos:prefLabel>
    <skos:example>photothermographic transfer prints are exemplified by Pictrography (TM) prints</skos:example>
    <rdfs:range rdf:resource="http://www.w3.org/2004/02/skos/core#Concept"/>
  </rdf:Description>
  <rdf:Description rdf:about="http://vocab.getty.edu/ontology#aat2852_involved_with">
    <rdfs:domain rdf:resource="http://www.w3.org/2004/02/skos/core#Concept"/>
    <rdfs:range rdf:resource="http://www.w3.org/2004/02/skos/core#Concept"/>
    <rdfs:subPropertyOf rdf:resource="http://www.w3.org/2004/02/skos/core#related"/>
    <rdfs:isDefinedBy rdf:resource="http://vocab.getty.edu/ontology"/>
    <owl:inverseOf rdf:resource="http://vocab.getty.edu/ontology#aat2853_involve"/>
    <rdf:type rdf:resource="http://www.w3.org/2002/07/owl#ObjectProperty"/>
    <dc:identifier>2852</dc:identifier>
    <skos:example>Rosa (genus) is involved with rose bowls</skos:example>
    <skos:prefLabel>aat2852_involved_with</skos:prefLabel>
    <rdfs:isDefinedBy rdf:resource="http://vocab.getty.edu/aat/"/>
    <dct:description>genus/species - [is] involved with - things/[equipment].&#13;
Example: Rosa (genus) is involved with rose bowls; Camelus (genus) is involved with camel saddles</dct:description>
    <skos:example>Camelus (genus) is involved with camel saddles</skos:example>
    <skos:scopeNote>genus/species - [is] involved with - things/[equipment].&#13;
Example: Rosa (genus) is involved with rose bowls; Camelus (genus) is involved with camel saddles</skos:scopeNote>
    <dc:title>involved with - things</dc:title>
  </rdf:Description>
  <rdf:Description rdf:about="http://vocab.getty.edu/ontology#broaderExtended">
    <rdfs:label>broaderExtended</rdfs:label>
    <rdfs:domain rdf:resource="http://vocab.getty.edu/ontology#Subject"/>
    <rdfs:range rdf:resource="http://vocab.getty.edu/ontology#Subject"/>
    <rdfs:comment>Appropriate ancestors. Meaningful closure of gvp:broader for query expansion. Use this, not skos:broaderTransitive</rdfs:comment>
    <skos:example>Mt Athos has ancestor places (BTPE) World, Europe, Greece, Macedonia, Pangaíon Óros regional division;
and place types (BTIE) inhabited place; and orthodox religious center, Christian religious center, religious center</skos:example>
    <dct:description>Appropriate ancestors. Meaningful closure of gvp:broader for query expansion. Use this, not skos:broaderTransitive.
Example: Mt Athos has ancestor places (BTPE) World, Europe, Greece, Macedonia, Pangaíon Óros regional division;
and place types (BTIE) inhabited place; and orthodox religious center, Christian religious center, religious center</dct:description>
    <skos:definition>Appropriate ancestors. Meaningful closure of gvp:broader for query expansion. Use this, not skos:broaderTransitive</skos:definition>
    <skos:prefLabel>broaderExtended</skos:prefLabel>
    <rdf:type rdf:resource="http://www.w3.org/2002/07/owl#ObjectProperty"/>
    <rdfs:isDefinedBy rdf:resource="http://vocab.getty.edu/ontology"/>
    <skos:scopeNote>Appropriate ancestors. Meaningful closure of gvp:broader for query expansion. Use this, not skos:broaderTransitive.
Example: Mt Athos has ancestor places (BTPE) World, Europe, Greece, Macedonia, Pangaíon Óros regional division;
and place types (BTIE) inhabited place; and orthodox religious center, Christian religious center, religious center</skos:scopeNote>
  </rdf:Description>
  <rdf:Description rdf:about="http://vocab.getty.edu/ontology#tgn3102_coextensive_with">
    <rdfs:isDefinedBy rdf:resource="http://vocab.getty.edu/tgn/"/>
    <rdf:type rdf:resource="http://www.w3.org/2002/07/owl#SymmetricProperty"/>
    <skos:prefLabel>tgn3102_coextensive_with</skos:prefLabel>
    <dct:description>place - coextensive with - place.&#13;
Example: Kings county (New York, USA) is coextensive with Brooklyn (New York, USA)</dct:description>
    <rdfs:domain rdf:resource="http://www.w3.org/2004/02/skos/core#Concept"/>
    <rdfs:range rdf:resource="http://www.w3.org/2004/02/skos/core#Concept"/>
    <skos:example>Kings county (New York, USA) is coextensive with Brooklyn (New York, USA)</skos:example>
    <dc:identifier>3102</dc:identifier>
    <rdfs:subPropertyOf rdf:resource="http://www.w3.org/2004/02/skos/core#related"/>
    <rdfs:isDefinedBy rdf:resource="http://vocab.getty.edu/ontology"/>
    <skos:scopeNote>place - coextensive with - place.&#13;
Example: Kings county (New York, USA) is coextensive with Brooklyn (New York, USA)</skos:scopeNote>
    <dc:title>coextensive with - place</dc:title>
    <rdf:type rdf:resource="http://www.w3.org/2002/07/owl#ObjectProperty"/>
  </rdf:Description>
  <rdf:Description rdf:about="http://vocab.getty.edu/ontology#ulan1553_child_by_marriage_of">
    <rdf:type rdf:resource="http://www.w3.org/2002/07/owl#ObjectProperty"/>
    <dc:title>child by marriage of - person</dc:title>
    <rdfs:range rdf:resource="http://www.w3.org/2004/02/skos/core#Concept"/>
    <rdfs:isDefinedBy rdf:resource="http://vocab.getty.edu/ulan/"/>
    <rdfs:subPropertyOf rdf:resource="http://www.w3.org/2004/02/skos/core#related"/>
    <skos:scopeNote>person - child by marriage (step child) - person.&#13;
Example: Pieter Gerritsz van Roestraten is the child by marriage of Frans Hals</skos:scopeNote>
    <skos:example>Pieter Gerritsz van Roestraten is the child by marriage of Frans Hals</skos:example>
    <dct:description>person - child by marriage (step child) - person.&#13;
Example: Pieter Gerritsz van Roestraten is the child by marriage of Frans Hals</dct:description>
    <dc:identifier>1553</dc:identifier>
    <rdfs:domain rdf:resource="http://www.w3.org/2004/02/skos/core#Concept"/>
    <rdfs:isDefinedBy rdf:resource="http://vocab.getty.edu/ontology"/>
    <skos:prefLabel>ulan1553_child_by_marriage_of</skos:prefLabel>
  </rdf:Description>
  <rdf:Description rdf:about="http://vocab.getty.edu/ontology#tgn3201_capital_of">
    <rdfs:range rdf:resource="http://www.w3.org/2004/02/skos/core#Concept"/>
    <rdfs:domain rdf:resource="http://www.w3.org/2004/02/skos/core#Concept"/>
    <rdfs:subPropertyOf rdf:resource="http://www.w3.org/2004/02/skos/core#related"/>
    <rdfs:isDefinedBy rdf:resource="http://vocab.getty.edu/ontology"/>
    <skos:example>Thecapital of Maxima Caesariensis from 296 to 800 CE was London</skos:example>
    <dc:identifier>3201</dc:identifier>
    <rdf:type rdf:resource="http://www.w3.org/2002/07/owl#ObjectProperty"/>
    <owl:inverseOf rdf:resource="http://vocab.getty.edu/ontology#tgn3202_capital_is"/>
    <dct:description>city - capital of - nation.&#13;
Example: Thecapital of Maxima Caesariensis from 296 to 800 CE was London</dct:description>
    <rdfs:isDefinedBy rdf:resource="http://vocab.getty.edu/tgn/"/>
    <dc:title>capital of - nation</dc:title>
    <skos:scopeNote>city - capital of - nation.&#13;
Example: Thecapital of Maxima Caesariensis from 296 to 800 CE was London</skos:scopeNote>
    <skos:prefLabel>tgn3201_capital_of</skos:prefLabel>
  </rdf:Description>
  <rdf:Description rdf:about="http://vocab.getty.edu/ontology#ulan1322_school_was">
    <rdf:type rdf:resource="http://www.w3.org/2002/07/owl#ObjectProperty"/>
    <rdfs:isDefinedBy rdf:resource="http://vocab.getty.edu/ontology"/>
    <dc:identifier>1322</dc:identifier>
    <rdfs:domain rdf:resource="http://www.w3.org/2004/02/skos/core#Concept"/>
    <rdfs:range rdf:resource="http://www.w3.org/2004/02/skos/core#Concept"/>
    <skos:scopeNote>firm/group - school was - person.&#13;
Example: Pierre Saalburg attended Architectural Association. School of Architecture</skos:scopeNote>
    <skos:prefLabel>ulan1322_school_was</skos:prefLabel>
    <dct:description>firm/group - school was - person.&#13;
Example: Pierre Saalburg attended Architectural Association. School of Architecture</dct:description>
    <rdfs:isDefinedBy rdf:resource="http://vocab.getty.edu/ulan/"/>
    <rdfs:subPropertyOf rdf:resource="http://www.w3.org/2004/02/skos/core#related"/>
    <skos:example>Pierre Saalburg attended Architectural Association. School of Architecture</skos:example>
    <dc:title>school was - person</dc:title>
  </rdf:Description>
  <rdf:Description rdf:about="http://vocab.getty.edu/ontology#ulan1500_related_to">
    <rdfs:subPropertyOf rdf:resource="http://www.w3.org/2004/02/skos/core#related"/>
    <rdfs:range rdf:resource="http://www.w3.org/2004/02/skos/core#Concept"/>
    <rdfs:domain rdf:resource="http://www.w3.org/2004/02/skos/core#Concept"/>
    <dct:description>person - related to (familial relationship) - person.&#13;
Example: Titian and Tizianello have a familial relationship with each other</dct:description>
    <rdf:type rdf:resource="http://www.w3.org/2002/07/owl#ObjectProperty"/>
    <rdfs:isDefinedBy rdf:resource="http://vocab.getty.edu/ontology"/>
    <skos:prefLabel>ulan1500_related_to</skos:prefLabel>
    <skos:scopeNote>person - related to (familial relationship) - person.&#13;
Example: Titian and Tizianello have a familial relationship with each other</skos:scopeNote>
    <skos:example>Titian and Tizianello have a familial relationship with each other</skos:example>
    <dc:title>related to - person</dc:title>
    <rdf:type rdf:resource="http://www.w3.org/2002/07/owl#SymmetricProperty"/>
    <dc:identifier>1500</dc:identifier>
    <rdfs:isDefinedBy rdf:resource="http://vocab.getty.edu/ulan/"/>
  </rdf:Description>
  <rdf:Description rdf:about="http://vocab.getty.edu/ontology#sourceAlternatePreferred">
    <rdfs:range rdf:resource="http://purl.org/ontology/bibo/Document"/>
    <rdfs:subPropertyOf rdf:resource="http://purl.org/dc/terms/source"/>
    <skos:definition>Source for which the term is Alternate Preferred. Range is bibo:Document or bibo:DocumentPart</skos:definition>
    <rdfs:domain rdf:resource="http://www.w3.org/2008/05/skos-xl#Label"/>
    <rdfs:comment>Source for which the term is Alternate Preferred. Range is bibo:Document or bibo:DocumentPart</rdfs:comment>
    <dct:description>Source for which the term is Alternate Preferred. Range is bibo:Document or bibo:DocumentPart.
Example: "Kayseri" is alternate preferred in Webster's New Geographical Dictionary (1988)</dct:description>
    <skos:prefLabel>sourceAlternatePreferred</skos:prefLabel>
    <skos:scopeNote>Source for which the term is Alternate Preferred. Range is bibo:Document or bibo:DocumentPart.
Example: "Kayseri" is alternate preferred in Webster's New Geographical Dictionary (1988)</skos:scopeNote>
    <rdf:type rdf:resource="http://www.w3.org/2002/07/owl#ObjectProperty"/>
    <skos:example>"Kayseri" is alternate preferred in Webster's New Geographical Dictionary (1988)</skos:example>
    <rdfs:isDefinedBy rdf:resource="http://vocab.getty.edu/ontology"/>
    <rdfs:label>sourceAlternatePreferred</rdfs:label>
  </rdf:Description>
  <rdf:Description rdf:about="http://vocab.getty.edu/ontology#ObsoleteSubject">
    <skos:prefLabel>ObsoleteSubject</skos:prefLabel>
    <rdfs:label>ObsoleteSubject</rdfs:label>
    <skos:scopeNote>Obsolete subject: moved out of the publishable hierarchy, or merged to another (pointed by dct:isReplacedBy).
Example: 300375205 "shranks" (AAT) was merged to 300039264 "schranks" (AAT), so aat:300375205 dct:isReplacedBy aat:300039264</skos:scopeNote>
    <rdfs:comment>Obsolete subject: moved out of the publishable hierarchy, or merged to another (pointed by dct:isReplacedBy)</rdfs:comment>
    <skos:example>300375205 "shranks" (AAT) was merged to 300039264 "schranks" (AAT), so aat:300375205 dct:isReplacedBy aat:300039264</skos:example>
    <dct:description>Obsolete subject: moved out of the publishable hierarchy, or merged to another (pointed by dct:isReplacedBy).
Example: 300375205 "shranks" (AAT) was merged to 300039264 "schranks" (AAT), so aat:300375205 dct:isReplacedBy aat:300039264</dct:description>
    <skos:broader rdf:resource="http://vocab.getty.edu/ontology#Subject"/>
    <skos:definition>Obsolete subject: moved out of the publishable hierarchy, or merged to another (pointed by dct:isReplacedBy)</skos:definition>
    <rdfs:isDefinedBy rdf:resource="http://vocab.getty.edu/ontology"/>
    <rdf:type rdf:resource="http://www.w3.org/2002/07/owl#Class"/>
    <rdfs:subClassOf rdf:resource="http://vocab.getty.edu/ontology#Subject"/>
  </rdf:Description>
  <rdf:Description rdf:about="http://vocab.getty.edu/ontology#aat2411_involved_in">
    <skos:prefLabel>aat2411_involved_in</skos:prefLabel>
    <dc:identifier>2411</dc:identifier>
    <dct:description>activity/event/[process/function] - [is] involved in - field/discipline.&#13;
Example: journalistic photography is involved in photojournalism (discipline); gardening is involved in horticulture</dct:description>
    <rdfs:isDefinedBy rdf:resource="http://vocab.getty.edu/aat/"/>
    <skos:example>gardening is involved in horticulture</skos:example>
    <skos:scopeNote>activity/event/[process/function] - [is] involved in - field/discipline.&#13;
Example: journalistic photography is involved in photojournalism (discipline); gardening is involved in horticulture</skos:scopeNote>
    <rdfs:range rdf:resource="http://www.w3.org/2004/02/skos/core#Concept"/>
    <rdfs:domain rdf:resource="http://www.w3.org/2004/02/skos/core#Concept"/>
    <rdfs:isDefinedBy rdf:resource="http://vocab.getty.edu/ontology"/>
    <rdfs:subPropertyOf rdf:resource="http://www.w3.org/2004/02/skos/core#related"/>
    <rdf:type rdf:resource="http://www.w3.org/2002/07/owl#ObjectProperty"/>
    <skos:example>journalistic photography is involved in photojournalism (discipline)</skos:example>
    <owl:inverseOf rdf:resource="http://vocab.getty.edu/ontology#aat2412_involves"/>
    <dc:title>involved in - field/discipline</dc:title>
  </rdf:Description>
  <rdf:Description rdf:about="http://vocab.getty.edu/ontology#ulan1222_appointee_of">
    <rdfs:isDefinedBy rdf:resource="http://vocab.getty.edu/ontology"/>
    <rdfs:range rdf:resource="http://www.w3.org/2004/02/skos/core#Concept"/>
    <rdfs:domain rdf:resource="http://www.w3.org/2004/02/skos/core#Concept"/>
    <dc:title>appointee of - person</dc:title>
    <dc:identifier>1222</dc:identifier>
    <skos:prefLabel>ulan1222_appointee_of</skos:prefLabel>
    <skos:scopeNote>person - appointee of - person.&#13;
Example: Virginio Cesarini was appointee by Pope Urban VIII</skos:scopeNote>
    <rdfs:subPropertyOf rdf:resource="http://www.w3.org/2004/02/skos/core#related"/>
    <skos:example>Virginio Cesarini was appointee by Pope Urban VIII</skos:example>
    <dct:description>person - appointee of - person.&#13;
Example: Virginio Cesarini was appointee by Pope Urban VIII</dct:description>
    <rdfs:isDefinedBy rdf:resource="http://vocab.getty.edu/ulan/"/>
    <rdf:type rdf:resource="http://www.w3.org/2002/07/owl#ObjectProperty"/>
  </rdf:Description>
  <rdf:Description rdf:about="http://vocab.getty.edu/ontology#aat2221_act_upon">
    <dct:description>[actors having] role - act upon - genus/species.&#13;
Example: jockeys act upon Equus caballus(species); tappers act upon Acer saccharum(species)</dct:description>
    <rdfs:domain rdf:resource="http://www.w3.org/2004/02/skos/core#Concept"/>
    <rdfs:range rdf:resource="http://www.w3.org/2004/02/skos/core#Concept"/>
    <rdfs:isDefinedBy rdf:resource="http://vocab.getty.edu/ontology"/>
    <dc:title>act upon - genus/species</dc:title>
    <skos:example>tappers act upon Acer saccharum(species)</skos:example>
    <rdfs:isDefinedBy rdf:resource="http://vocab.getty.edu/aat/"/>
    <skos:scopeNote>[actors having] role - act upon - genus/species.&#13;
Example: jockeys act upon Equus caballus(species); tappers act upon Acer saccharum(species)</skos:scopeNote>
    <dc:identifier>2221</dc:identifier>
    <skos:example>jockeys act upon Equus caballus(species)</skos:example>
    <owl:inverseOf rdf:resource="http://vocab.getty.edu/ontology#aat2222_are_acted_upon"/>
    <skos:prefLabel>aat2221_act_upon</skos:prefLabel>
    <rdfs:subPropertyOf rdf:resource="http://www.w3.org/2004/02/skos/core#related"/>
    <rdf:type rdf:resource="http://www.w3.org/2002/07/owl#ObjectProperty"/>
  </rdf:Description>
  <rdf:Description rdf:about="http://vocab.getty.edu/ontology#tgn3000_related_to">
    <dc:title>related to - any</dc:title>
    <dct:description>any - related to - any.&#13;
Example: Fountains Abbey is related to Studley Royal; Austria-Hungary is related to Magyarorszag</dct:description>
    <rdf:type rdf:resource="http://www.w3.org/2002/07/owl#ObjectProperty"/>
    <rdfs:domain rdf:resource="http://www.w3.org/2004/02/skos/core#Concept"/>
    <rdfs:isDefinedBy rdf:resource="http://vocab.getty.edu/ontology"/>
    <skos:example>Austria-Hungary is related to Magyarorszag</skos:example>
    <skos:prefLabel>tgn3000_related_to</skos:prefLabel>
    <dc:identifier>3000</dc:identifier>
    <rdfs:isDefinedBy rdf:resource="http://vocab.getty.edu/tgn/"/>
    <rdf:type rdf:resource="http://www.w3.org/2002/07/owl#SymmetricProperty"/>
    <skos:example>Fountains Abbey is related to Studley Royal</skos:example>
    <skos:scopeNote>any - related to - any.&#13;
Example: Fountains Abbey is related to Studley Royal; Austria-Hungary is related to Magyarorszag</skos:scopeNote>
    <rdfs:range rdf:resource="http://www.w3.org/2004/02/skos/core#Concept"/>
    <rdfs:subPropertyOf rdf:resource="http://www.w3.org/2004/02/skos/core#related"/>
  </rdf:Description>
  <rdf:Description rdf:about="http://vocab.getty.edu/ontology#ulan1005_possibly_identified_with">
    <rdfs:subPropertyOf rdf:resource="http://www.w3.org/2004/02/skos/core#related"/>
    <rdfs:range rdf:resource="http://www.w3.org/2004/02/skos/core#Concept"/>
    <skos:prefLabel>ulan1005_possibly_identified_with</skos:prefLabel>
    <rdf:type rdf:resource="http://www.w3.org/2002/07/owl#SymmetricProperty"/>
    <dc:title>possibly identified with - any</dc:title>
    <rdfs:domain rdf:resource="http://www.w3.org/2004/02/skos/core#Concept"/>
    <dct:description>any - possibly identified with - any.&#13;
Example: Master of the Saint John Altarpiece is possibly identified with Hughe Jacobsz; Bauart is possibly identified with Gruppe BAUart</dct:description>
    <rdf:type rdf:resource="http://www.w3.org/2002/07/owl#ObjectProperty"/>
    <rdfs:isDefinedBy rdf:resource="http://vocab.getty.edu/ontology"/>
    <skos:scopeNote>any - possibly identified with - any.&#13;
Example: Master of the Saint John Altarpiece is possibly identified with Hughe Jacobsz; Bauart is possibly identified with Gruppe BAUart</skos:scopeNote>
    <dc:identifier>1005</dc:identifier>
    <skos:example>Master of the Saint John Altarpiece is possibly identified with Hughe Jacobsz</skos:example>
    <rdfs:isDefinedBy rdf:resource="http://vocab.getty.edu/ulan/"/>
    <skos:example>Bauart is possibly identified with Gruppe BAUart</skos:example>
  </rdf:Description>
  <rdf:Description rdf:about="http://vocab.getty.edu/ontology#ulan1554_adoptive_parent_of">
    <rdf:type rdf:resource="http://www.w3.org/2002/07/owl#ObjectProperty"/>
    <owl:inverseOf rdf:resource="http://vocab.getty.edu/ontology#ulan1555_adopted_child_of"/>
    <rdfs:isDefinedBy rdf:resource="http://vocab.getty.edu/ontology"/>
    <skos:prefLabel>ulan1554_adoptive_parent_of</skos:prefLabel>
    <rdfs:isDefinedBy rdf:resource="http://vocab.getty.edu/ulan/"/>
    <skos:scopeNote>person - adoptive parent of - person.&#13;
Example: Julius Caesar is the adoptive parent of Augustus, Emperor of Rome</skos:scopeNote>
    <dc:identifier>1554</dc:identifier>
    <rdfs:domain rdf:resource="http://www.w3.org/2004/02/skos/core#Concept"/>
    <rdfs:range rdf:resource="http://www.w3.org/2004/02/skos/core#Concept"/>
    <dct:description>person - adoptive parent of - person.&#13;
Example: Julius Caesar is the adoptive parent of Augustus, Emperor of Rome</dct:description>
    <dc:title>adoptive parent of - person</dc:title>
    <rdfs:subPropertyOf rdf:resource="http://www.w3.org/2004/02/skos/core#related"/>
    <skos:example>Julius Caesar is the adoptive parent of Augustus, Emperor of Rome</skos:example>
  </rdf:Description>
  <rdf:Description rdf:about="http://vocab.getty.edu/ontology#aat2398_focuses_on">
    <skos:example>musicology focuses on music</skos:example>
    <rdfs:isDefinedBy rdf:resource="http://vocab.getty.edu/aat/"/>
    <rdf:type rdf:resource="http://www.w3.org/2002/07/owl#ObjectProperty"/>
    <rdfs:isDefinedBy rdf:resource="http://vocab.getty.edu/ontology"/>
    <skos:example>bontany focuses on Plantae (kingdom)</skos:example>
    <skos:scopeNote>field [of study]/discipline - focuses on - any.&#13;
Example: codicology focuses on manuscripts; musicology focuses on music; bontany focuses on Plantae (kingdom)</skos:scopeNote>
    <skos:example>codicology focuses on manuscripts</skos:example>
    <rdfs:range rdf:resource="http://www.w3.org/2004/02/skos/core#Concept"/>
    <rdfs:domain rdf:resource="http://www.w3.org/2004/02/skos/core#Concept"/>
    <dc:identifier>2398</dc:identifier>
    <rdfs:subPropertyOf rdf:resource="http://www.w3.org/2004/02/skos/core#related"/>
    <dct:description>field [of study]/discipline - focuses on - any.&#13;
Example: codicology focuses on manuscripts; musicology focuses on music; bontany focuses on Plantae (kingdom)</dct:description>
    <skos:prefLabel>aat2398_focuses_on</skos:prefLabel>
    <dc:title>focuses on - any</dc:title>
  </rdf:Description>
  <rdf:Description rdf:about="http://vocab.getty.edu/ontology#aat2332_affiliated_with">
    <skos:scopeNote>[actors having] role - [are] affiliated with - role [organization].&#13;
Example: students are affiliated with schools (organizations); dukes are affiliated with duchies</skos:scopeNote>
    <skos:prefLabel>aat2332_affiliated_with</skos:prefLabel>
    <rdfs:domain rdf:resource="http://www.w3.org/2004/02/skos/core#Concept"/>
    <rdfs:range rdf:resource="http://www.w3.org/2004/02/skos/core#Concept"/>
    <skos:example>dukes are affiliated with duchies</skos:example>
    <rdfs:subPropertyOf rdf:resource="http://www.w3.org/2004/02/skos/core#related"/>
    <dc:title>affiliated with - role</dc:title>
    <dc:identifier>2332</dc:identifier>
    <owl:inverseOf rdf:resource="http://vocab.getty.edu/ontology#aat2333_have_affiliates"/>
    <rdf:type rdf:resource="http://www.w3.org/2002/07/owl#ObjectProperty"/>
    <skos:example>students are affiliated with schools (organizations)</skos:example>
    <rdfs:isDefinedBy rdf:resource="http://vocab.getty.edu/ontology"/>
    <rdfs:isDefinedBy rdf:resource="http://vocab.getty.edu/aat/"/>
    <dct:description>[actors having] role - [are] affiliated with - role [organization].&#13;
Example: students are affiliated with schools (organizations); dukes are affiliated with duchies</dct:description>
  </rdf:Description>
  <rdf:Description rdf:about="http://vocab.getty.edu/ontology#aat2427_produced_by">
    <skos:example>forgeries are produced by forging (copying)</skos:example>
    <rdfs:subPropertyOf rdf:resource="http://www.w3.org/2004/02/skos/core#related"/>
    <skos:example>vase paintings (visual works) are produced by vase painting (image making)</skos:example>
    <rdfs:range rdf:resource="http://www.w3.org/2004/02/skos/core#Concept"/>
    <owl:inverseOf rdf:resource="http://vocab.getty.edu/ontology#aat2428_produces"/>
    <skos:prefLabel>aat2427_produced_by</skos:prefLabel>
    <dct:description>things - [are] produced by - activity/event/process.&#13;
Example: vase paintings (visual works) are produced by vase painting (image making); forgeries are produced by forging (copying)</dct:description>
    <dc:title>produced by - activity/event/process</dc:title>
    <rdfs:isDefinedBy rdf:resource="http://vocab.getty.edu/aat/"/>
    <rdf:type rdf:resource="http://www.w3.org/2002/07/owl#ObjectProperty"/>
    <rdfs:isDefinedBy rdf:resource="http://vocab.getty.edu/ontology"/>
    <skos:scopeNote>things - [are] produced by - activity/event/process.&#13;
Example: vase paintings (visual works) are produced by vase painting (image making); forgeries are produced by forging (copying)</skos:scopeNote>
    <rdfs:domain rdf:resource="http://www.w3.org/2004/02/skos/core#Concept"/>
    <dc:identifier>2427</dc:identifier>
  </rdf:Description>
  <rdf:Description rdf:about="http://vocab.getty.edu/ontology#aat2212_produced_by">
    <skos:example>stereoscopic photographs are produced by stereoscopic cameras</skos:example>
    <dct:description>things - [are] produced by - things/[equipment].&#13;
Example: stereoscopic photographs are produced by stereoscopic cameras; punchwork is produced by punches (marking tools)</dct:description>
    <rdf:type rdf:resource="http://www.w3.org/2002/07/owl#ObjectProperty"/>
    <rdfs:isDefinedBy rdf:resource="http://vocab.getty.edu/aat/"/>
    <rdfs:range rdf:resource="http://www.w3.org/2004/02/skos/core#Concept"/>
    <rdfs:domain rdf:resource="http://www.w3.org/2004/02/skos/core#Concept"/>
    <dc:title>produced by - things</dc:title>
    <skos:scopeNote>things - [are] produced by - things/[equipment].&#13;
Example: stereoscopic photographs are produced by stereoscopic cameras; punchwork is produced by punches (marking tools)</skos:scopeNote>
    <skos:example>punchwork is produced by punches (marking tools)</skos:example>
    <skos:prefLabel>aat2212_produced_by</skos:prefLabel>
    <dc:identifier>2212</dc:identifier>
    <rdfs:subPropertyOf rdf:resource="http://www.w3.org/2004/02/skos/core#related"/>
    <rdfs:isDefinedBy rdf:resource="http://vocab.getty.edu/ontology"/>
  </rdf:Description>
  <rdf:Description rdf:about="http://vocab.getty.edu/ontology#aat2613_possess-exist_in">
    <rdfs:subPropertyOf rdf:resource="http://www.w3.org/2004/02/skos/core#related"/>
    <dc:identifier>2613</dc:identifier>
    <skos:example>wood(plant material) possesses/exists in [condition of] dry rot</skos:example>
    <skos:example>dielectric (material) possesses/exists in dielectric properties</skos:example>
    <dct:description>material - possesses/exists in - condition/state/[property].&#13;
Example: wood(plant material) possesses/exists in [condition of] dry rot; dielectric (material) possesses/exists in dielectric properties</dct:description>
    <rdfs:isDefinedBy rdf:resource="http://vocab.getty.edu/aat/"/>
    <skos:prefLabel>aat2613_possess-exist_in</skos:prefLabel>
    <rdfs:isDefinedBy rdf:resource="http://vocab.getty.edu/ontology"/>
    <dc:title>possess/exist in - attributes /associated concepts</dc:title>
    <rdf:type rdf:resource="http://www.w3.org/2002/07/owl#ObjectProperty"/>
    <rdfs:domain rdf:resource="http://www.w3.org/2004/02/skos/core#Concept"/>
    <skos:scopeNote>material - possesses/exists in - condition/state/[property].&#13;
Example: wood(plant material) possesses/exists in [condition of] dry rot; dielectric (material) possesses/exists in dielectric properties</skos:scopeNote>
    <rdfs:range rdf:resource="http://www.w3.org/2004/02/skos/core#Concept"/>
  </rdf:Description>
  <rdf:Description rdf:about="http://vocab.getty.edu/ontology#aat2318_involved_in">
    <skos:example>martyrs are involved in martyrdoms</skos:example>
    <rdfs:subPropertyOf rdf:resource="http://www.w3.org/2004/02/skos/core#related"/>
    <skos:example>bridegrooms are involved in weddings</skos:example>
    <owl:inverseOf rdf:resource="http://vocab.getty.edu/ontology#aat2319_involves"/>
    <skos:prefLabel>aat2318_involved_in</skos:prefLabel>
    <dc:title>involved in - activity/event</dc:title>
    <skos:scopeNote>[actors having] role -[are] involved - activity/event.&#13;
Example: bridegrooms are involved in weddings; martyrs are involved in martyrdoms</skos:scopeNote>
    <rdfs:isDefinedBy rdf:resource="http://vocab.getty.edu/aat/"/>
    <rdf:type rdf:resource="http://www.w3.org/2002/07/owl#ObjectProperty"/>
    <dct:description>[actors having] role -[are] involved - activity/event.&#13;
Example: bridegrooms are involved in weddings; martyrs are involved in martyrdoms</dct:description>
    <rdfs:isDefinedBy rdf:resource="http://vocab.getty.edu/ontology"/>
    <rdfs:range rdf:resource="http://www.w3.org/2004/02/skos/core#Concept"/>
    <dc:identifier>2318</dc:identifier>
    <rdfs:domain rdf:resource="http://www.w3.org/2004/02/skos/core#Concept"/>
  </rdf:Description>
  <rdf:Description rdf:about="http://vocab.getty.edu/ontology#tgn3411_successor_of">
    <rdf:type rdf:resource="http://www.w3.org/2002/07/owl#ObjectProperty"/>
    <dct:description>nation - successor of - nation.&#13;
Example: Iran (nation) is the successor of Persia</dct:description>
    <skos:prefLabel>tgn3411_successor_of</skos:prefLabel>
    <rdfs:subPropertyOf rdf:resource="http://www.w3.org/2004/02/skos/core#related"/>
    <rdfs:isDefinedBy rdf:resource="http://vocab.getty.edu/tgn/"/>
    <skos:scopeNote>nation - successor of - nation.&#13;
Example: Iran (nation) is the successor of Persia</skos:scopeNote>
    <dc:identifier>3411</dc:identifier>
    <skos:example>Iran (nation) is the successor of Persia</skos:example>
    <rdfs:domain rdf:resource="http://www.w3.org/2004/02/skos/core#Concept"/>
    <owl:inverseOf rdf:resource="http://vocab.getty.edu/ontology#tgn3412_predecessor_of"/>
    <rdfs:range rdf:resource="http://www.w3.org/2004/02/skos/core#Concept"/>
    <dc:title>successor of - nation</dc:title>
    <rdfs:isDefinedBy rdf:resource="http://vocab.getty.edu/ontology"/>
  </rdf:Description>
  <rdf:Description rdf:about="http://vocab.getty.edu/ontology#ulan1512_parent_of">
    <rdf:type rdf:resource="http://www.w3.org/2002/07/owl#ObjectProperty"/>
    <skos:prefLabel>ulan1512_parent_of</skos:prefLabel>
    <dc:identifier>1512</dc:identifier>
    <dc:title>parent of - person</dc:title>
    <rdfs:domain rdf:resource="http://www.w3.org/2004/02/skos/core#Concept"/>
    <rdfs:range rdf:resource="http://www.w3.org/2004/02/skos/core#Concept"/>
    <skos:scopeNote>person - parent of - person.&#13;
Example: Rembrandt van Rijn is the parent of Rumbertus van Rijn</skos:scopeNote>
    <skos:example>Rembrandt van Rijn is the parent of Rumbertus van Rijn</skos:example>
    <rdfs:isDefinedBy rdf:resource="http://vocab.getty.edu/ulan/"/>
    <dct:description>person - parent of - person.&#13;
Example: Rembrandt van Rijn is the parent of Rumbertus van Rijn</dct:description>
    <rdfs:subPropertyOf rdf:resource="http://www.w3.org/2004/02/skos/core#related"/>
    <rdfs:isDefinedBy rdf:resource="http://vocab.getty.edu/ontology"/>
  </rdf:Description>
  <rdf:Description rdf:about="http://vocab.getty.edu/ontology#ulan2576_patron_of">
    <rdfs:subPropertyOf rdf:resource="http://www.w3.org/2004/02/skos/core#related"/>
    <skos:scopeNote>person - patron of - person.&#13;
Example: The patron of William Chambers was James Caulfiel, Earl of Charlemont</skos:scopeNote>
    <skos:example>The patron of William Chambers was James Caulfiel, Earl of Charlemont</skos:example>
    <rdfs:range rdf:resource="http://www.w3.org/2004/02/skos/core#Concept"/>
    <skos:prefLabel>ulan2576_patron_of</skos:prefLabel>
    <dc:title>patron of - person</dc:title>
    <owl:inverseOf rdf:resource="http://vocab.getty.edu/ontology#ulan2577_patron_was"/>
    <dct:description>person - patron of - person.&#13;
Example: The patron of William Chambers was James Caulfiel, Earl of Charlemont</dct:description>
    <rdfs:isDefinedBy rdf:resource="http://vocab.getty.edu/ontology"/>
    <dc:identifier>2576</dc:identifier>
    <rdf:type rdf:resource="http://www.w3.org/2002/07/owl#ObjectProperty"/>
    <rdfs:isDefinedBy rdf:resource="http://vocab.getty.edu/ulan/"/>
    <rdfs:domain rdf:resource="http://www.w3.org/2004/02/skos/core#Concept"/>
  </rdf:Description>
  <rdf:Description rdf:about="http://vocab.getty.edu/ontology#termDisplay">
    <rdf:type rdf:resource="http://www.w3.org/2002/07/owl#ObjectProperty"/>
    <skos:prefLabel>termDisplay</skos:prefLabel>
    <dct:description>Term Display</dct:description>
    <rdfs:label>termDisplay</rdfs:label>
    <rdfs:domain rdf:resource="http://www.w3.org/2008/05/skos-xl#Label"/>
    <skos:scopeNote>Term Display</skos:scopeNote>
    <rdfs:range rdf:resource="http://www.w3.org/2004/02/skos/core#Concept"/>
    <rdfs:isDefinedBy rdf:resource="http://vocab.getty.edu/ontology"/>
  </rdf:Description>
  <rdf:Description rdf:about="http://vocab.getty.edu/ontology#aat2558_reflected_in">
    <dc:title>reflected in - field/discipline</dc:title>
    <dct:description>style/period/culture /[religion/ideology] - [is] reflected in field/discipline.&#13;
Example: Buddhism is reflected in bugatu [dance discipline]; Christianity is reflected in church history; Ancient Greek [culture] is reflected in classics (discipline)</dct:description>
    <skos:prefLabel>aat2558_reflected_in</skos:prefLabel>
    <rdfs:subPropertyOf rdf:resource="http://www.w3.org/2004/02/skos/core#related"/>
    <rdfs:domain rdf:resource="http://www.w3.org/2004/02/skos/core#Concept"/>
    <rdfs:range rdf:resource="http://www.w3.org/2004/02/skos/core#Concept"/>
    <rdfs:isDefinedBy rdf:resource="http://vocab.getty.edu/ontology"/>
    <dc:identifier>2558</dc:identifier>
    <skos:scopeNote>style/period/culture /[religion/ideology] - [is] reflected in field/discipline.&#13;
Example: Buddhism is reflected in bugatu [dance discipline]; Christianity is reflected in church history; Ancient Greek [culture] is reflected in classics (discipline)</skos:scopeNote>
    <rdf:type rdf:resource="http://www.w3.org/2002/07/owl#ObjectProperty"/>
    <skos:example>Ancient Greek [culture] is reflected in classics (discipline)</skos:example>
    <skos:example>Christianity is reflected in church history</skos:example>
    <skos:example>Buddhism is reflected in bugatu [dance discipline]</skos:example>
    <rdfs:isDefinedBy rdf:resource="http://vocab.getty.edu/aat/"/>
  </rdf:Description>
  <rdf:Description rdf:about="http://vocab.getty.edu/ontology#ulan1105_apprentice_of">
    <dc:identifier>1105</dc:identifier>
    <rdfs:subPropertyOf rdf:resource="http://www.w3.org/2004/02/skos/core#related"/>
    <rdfs:isDefinedBy rdf:resource="http://vocab.getty.edu/ulan/"/>
    <skos:example>Nicolas Hawksmoor was the apprentice of Christopher Wren</skos:example>
    <rdf:type rdf:resource="http://www.w3.org/2002/07/owl#ObjectProperty"/>
    <rdfs:isDefinedBy rdf:resource="http://vocab.getty.edu/ontology"/>
    <skos:scopeNote>person - apprentice of - person.&#13;
Example: Nicolas Hawksmoor was the apprentice of Christopher Wren</skos:scopeNote>
    <rdfs:domain rdf:resource="http://www.w3.org/2004/02/skos/core#Concept"/>
    <rdfs:range rdf:resource="http://www.w3.org/2004/02/skos/core#Concept"/>
    <dc:title>apprentice of - person</dc:title>
    <owl:inverseOf rdf:resource="http://vocab.getty.edu/ontology#ulan1106_apprentice_was"/>
    <dct:description>person - apprentice of - person.&#13;
Example: Nicolas Hawksmoor was the apprentice of Christopher Wren</dct:description>
    <skos:prefLabel>ulan1105_apprentice_of</skos:prefLabel>
  </rdf:Description>
  <rdf:Description rdf:about="http://vocab.getty.edu/ontology#aat2434_contextualized_in">
    <rdfs:isDefinedBy rdf:resource="http://vocab.getty.edu/ontology"/>
    <rdfs:subPropertyOf rdf:resource="http://www.w3.org/2004/02/skos/core#related"/>
    <owl:inverseOf rdf:resource="http://vocab.getty.edu/ontology#aat2435_context_for"/>
    <skos:scopeNote>things - [are] context for - activity/event/process.&#13;
Example: funeral books are contextualized in funerals; Christmas trees are contextualized in Christmas</skos:scopeNote>
    <rdfs:isDefinedBy rdf:resource="http://vocab.getty.edu/aat/"/>
    <rdf:type rdf:resource="http://www.w3.org/2002/07/owl#ObjectProperty"/>
    <rdfs:domain rdf:resource="http://www.w3.org/2004/02/skos/core#Concept"/>
    <skos:example>funeral books are contextualized in funerals</skos:example>
    <dct:description>things - [are] context for - activity/event/process.&#13;
Example: funeral books are contextualized in funerals; Christmas trees are contextualized in Christmas</dct:description>
    <rdfs:range rdf:resource="http://www.w3.org/2004/02/skos/core#Concept"/>
    <dc:title>contextualized in - activity/event/process</dc:title>
    <dc:identifier>2434</dc:identifier>
    <skos:prefLabel>aat2434_contextualized_in</skos:prefLabel>
    <skos:example>Christmas trees are contextualized in Christmas</skos:example>
  </rdf:Description>
  <rdf:Description rdf:about="http://vocab.getty.edu/ontology#aat2887_exemplified_by">
    <skos:scopeNote>material - exemplified by - material.&#13;
Example: solvent - exemplified by - carbon disulfide</skos:scopeNote>
    <dc:identifier>2887</dc:identifier>
    <dc:title>exemplified by - material</dc:title>
    <rdfs:range rdf:resource="http://www.w3.org/2004/02/skos/core#Concept"/>
    <skos:example>solvent - exemplified by - carbon disulfide</skos:example>
    <rdfs:domain rdf:resource="http://www.w3.org/2004/02/skos/core#Concept"/>
    <rdfs:isDefinedBy rdf:resource="http://vocab.getty.edu/aat/"/>
    <dct:description>material - exemplified by - material.&#13;
Example: solvent - exemplified by - carbon disulfide</dct:description>
    <skos:prefLabel>aat2887_exemplified_by</skos:prefLabel>
    <rdfs:isDefinedBy rdf:resource="http://vocab.getty.edu/ontology"/>
    <rdfs:subPropertyOf rdf:resource="http://www.w3.org/2004/02/skos/core#related"/>
    <rdf:type rdf:resource="http://www.w3.org/2002/07/owl#ObjectProperty"/>
  </rdf:Description>
  <rdf:Description rdf:about="http://vocab.getty.edu/ontology#tgn3402_moved_to">
    <rdfs:subPropertyOf rdf:resource="http://www.w3.org/2004/02/skos/core#related"/>
    <rdfs:range rdf:resource="http://www.w3.org/2004/02/skos/core#Concept"/>
    <rdfs:domain rdf:resource="http://www.w3.org/2004/02/skos/core#Concept"/>
    <skos:scopeNote>place - moved to - place.&#13;
Example: Valdosta (Lowndes county, Georgia, USA) moved from Troupville (Georgia, USA)</skos:scopeNote>
    <rdf:type rdf:resource="http://www.w3.org/2002/07/owl#ObjectProperty"/>
    <rdfs:isDefinedBy rdf:resource="http://vocab.getty.edu/ontology"/>
    <rdfs:isDefinedBy rdf:resource="http://vocab.getty.edu/tgn/"/>
    <dct:description>place - moved to - place.&#13;
Example: Valdosta (Lowndes county, Georgia, USA) moved from Troupville (Georgia, USA)</dct:description>
    <dc:title>moved to - place</dc:title>
    <skos:prefLabel>tgn3402_moved_to</skos:prefLabel>
    <dc:identifier>3402</dc:identifier>
    <skos:example>Valdosta (Lowndes county, Georgia, USA) moved from Troupville (Georgia, USA)</skos:example>
  </rdf:Description>
  <rdf:Description rdf:about="http://vocab.getty.edu/ontology#aat2879_followed-developed_from">
    <skos:example>Greek (modern language) followed/developed from Ancient Greek (language)</skos:example>
    <skos:scopeNote>language - followed/developed from - language.&#13;
Example: Greek (modern language) followed/developed from Ancient Greek (language); Egyptian, Coptic (language) followed/developed from Ancient Egyptian (language)</skos:scopeNote>
    <skos:example>Egyptian, Coptic (language) followed/developed from Ancient Egyptian (language)</skos:example>
    <rdfs:domain rdf:resource="http://www.w3.org/2004/02/skos/core#Concept"/>
    <rdfs:range rdf:resource="http://www.w3.org/2004/02/skos/core#Concept"/>
    <rdfs:subPropertyOf rdf:resource="http://www.w3.org/2004/02/skos/core#related"/>
    <rdf:type rdf:resource="http://www.w3.org/2002/07/owl#ObjectProperty"/>
    <skos:prefLabel>aat2879_followed-developed_from</skos:prefLabel>
    <rdfs:isDefinedBy rdf:resource="http://vocab.getty.edu/ontology"/>
    <dct:description>language - followed/developed from - language.&#13;
Example: Greek (modern language) followed/developed from Ancient Greek (language); Egyptian, Coptic (language) followed/developed from Ancient Egyptian (language)</dct:description>
    <rdfs:isDefinedBy rdf:resource="http://vocab.getty.edu/aat/"/>
    <dc:title>followed/developed from - language</dc:title>
    <dc:identifier>2879</dc:identifier>
  </rdf:Description>
  <rdf:Description rdf:about="http://vocab.getty.edu/ontology#ulan1521_cousin_of">
    <skos:scopeNote>person - cousin of - person.&#13;
Example: Richard Meier and Frank Gehry are cousins</skos:scopeNote>
    <rdfs:subPropertyOf rdf:resource="http://www.w3.org/2004/02/skos/core#related"/>
    <rdfs:isDefinedBy rdf:resource="http://vocab.getty.edu/ontology"/>
    <rdf:type rdf:resource="http://www.w3.org/2002/07/owl#ObjectProperty"/>
    <dc:title>cousin of - person</dc:title>
    <rdf:type rdf:resource="http://www.w3.org/2002/07/owl#SymmetricProperty"/>
    <skos:prefLabel>ulan1521_cousin_of</skos:prefLabel>
    <skos:example>Richard Meier and Frank Gehry are cousins</skos:example>
    <dct:description>person - cousin of - person.&#13;
Example: Richard Meier and Frank Gehry are cousins</dct:description>
    <rdfs:range rdf:resource="http://www.w3.org/2004/02/skos/core#Concept"/>
    <rdfs:domain rdf:resource="http://www.w3.org/2004/02/skos/core#Concept"/>
    <rdfs:isDefinedBy rdf:resource="http://vocab.getty.edu/ulan/"/>
    <dc:identifier>1521</dc:identifier>
  </rdf:Description>
  <rdf:Description rdf:about="http://vocab.getty.edu/ontology#broaderPreferred">
    <rdfs:subPropertyOf rdf:resource="http://vocab.getty.edu/ontology#broader"/>
    <rdfs:range rdf:resource="http://vocab.getty.edu/ontology#Subject"/>
    <rdfs:label>broaderPreferred</rdfs:label>
    <skos:example>Preferred: "baking dishes" (AAT) BTG "bakeware" (AAT); Sofia (TGN) BTP Bulgaria (TGN)</skos:example>
    <rdf:type rdf:resource="http://www.w3.org/2002/07/owl#ObjectProperty"/>
    <rdfs:isDefinedBy rdf:resource="http://vocab.getty.edu/ontology"/>
    <skos:scopeNote>Main parent of a subject. Needed to display the hierarchy.
Example: Preferred: "baking dishes" (AAT) BTG "bakeware" (AAT); Sofia (TGN) BTP Bulgaria (TGN)</skos:scopeNote>
    <rdfs:subPropertyOf rdf:resource="http://vocab.getty.edu/ontology#broaderPreferredExtended"/>
    <dct:description>Main parent of a subject. Needed to display the hierarchy.
Example: Preferred: "baking dishes" (AAT) BTG "bakeware" (AAT); Sofia (TGN) BTP Bulgaria (TGN)</dct:description>
    <rdfs:domain rdf:resource="http://vocab.getty.edu/ontology#Subject"/>
    <skos:definition>Main parent of a subject. Needed to display the hierarchy</skos:definition>
    <skos:prefLabel>broaderPreferred</skos:prefLabel>
    <rdfs:comment>Main parent of a subject. Needed to display the hierarchy</rdfs:comment>
  </rdf:Description>
  <rdf:Description rdf:about="http://vocab.getty.edu/ontology#ulan1551_sibling_by_marriage_of">
    <skos:prefLabel>ulan1551_sibling_by_marriage_of</skos:prefLabel>
    <dc:title>sibling by marriage of - person</dc:title>
    <rdfs:subPropertyOf rdf:resource="http://www.w3.org/2004/02/skos/core#related"/>
    <skos:scopeNote>person - sibling by marriage (step sibling) - person.&#13;
Example: Peter Paul Rubens and Susanne Fourment are siblings by marriage</skos:scopeNote>
    <rdfs:isDefinedBy rdf:resource="http://vocab.getty.edu/ulan/"/>
    <rdf:type rdf:resource="http://www.w3.org/2002/07/owl#ObjectProperty"/>
    <skos:example>Peter Paul Rubens and Susanne Fourment are siblings by marriage</skos:example>
    <rdf:type rdf:resource="http://www.w3.org/2002/07/owl#SymmetricProperty"/>
    <dct:description>person - sibling by marriage (step sibling) - person.&#13;
Example: Peter Paul Rubens and Susanne Fourment are siblings by marriage</dct:description>
    <rdfs:isDefinedBy rdf:resource="http://vocab.getty.edu/ontology"/>
    <rdfs:domain rdf:resource="http://www.w3.org/2004/02/skos/core#Concept"/>
    <rdfs:range rdf:resource="http://www.w3.org/2004/02/skos/core#Concept"/>
    <dc:identifier>1551</dc:identifier>
  </rdf:Description>
  <rdf:Description rdf:about="http://vocab.getty.edu/ontology#ulan2829_student_was">
    <dc:identifier>2829</dc:identifier>
    <rdfs:range rdf:resource="http://www.w3.org/2004/02/skos/core#Concept"/>
    <rdfs:domain rdf:resource="http://www.w3.org/2004/02/skos/core#Concept"/>
    <rdfs:isDefinedBy rdf:resource="http://vocab.getty.edu/ontology"/>
    <rdfs:subPropertyOf rdf:resource="http://www.w3.org/2004/02/skos/core#related"/>
    <rdf:type rdf:resource="http://www.w3.org/2002/07/owl#ObjectProperty"/>
    <rdfs:isDefinedBy rdf:resource="http://vocab.getty.edu/ulan/"/>
    <skos:scopeNote>institution - student was - person.&#13;
Example: Bauhaus student was Zdanek Rossman</skos:scopeNote>
    <dc:title>student was - person</dc:title>
    <skos:example>Bauhaus student was Zdanek Rossman</skos:example>
    <dct:description>institution - student was - person.&#13;
Example: Bauhaus student was Zdanek Rossman</dct:description>
    <skos:prefLabel>ulan2829_student_was</skos:prefLabel>
  </rdf:Description>
  <rdf:Description rdf:about="http://vocab.getty.edu/term/kind/ProvisionalName">
    <dct:description>Used in TGN only.
Example: "Rockton" was provisional name considered before adoption of "Kent" (Ohio)</dct:description>
    <rdf:type rdf:resource="http://www.w3.org/2004/02/skos/core#Concept"/>
    <skos:notation>PN</skos:notation>
    <skos:example>"Rockton" was provisional name considered before adoption of "Kent" (Ohio)</skos:example>
    <skos:prefLabel>Provisional Name</skos:prefLabel>
    <skos:inScheme rdf:resource="http://vocab.getty.edu/term/kind/"/>
    <skos:scopeNote>Used in TGN only</skos:scopeNote>
  </rdf:Description>
  <rdf:Description rdf:about="http://vocab.getty.edu/ontology#aat2286_practice-study">
    <rdf:type rdf:resource="http://www.w3.org/2002/07/owl#ObjectProperty"/>
    <dc:title>practice/study - field/discipline</dc:title>
    <rdfs:subPropertyOf rdf:resource="http://www.w3.org/2004/02/skos/core#related"/>
    <skos:example>Egyptologists practice/study Egyptology</skos:example>
    <dct:description>[actor having] role - practice/study - field [of study, genre]/discipline.&#13;
Example: Egyptologists practice/study Egyptology; architectural historians practice/study architectural history</dct:description>
    <rdfs:isDefinedBy rdf:resource="http://vocab.getty.edu/aat/"/>
    <skos:prefLabel>aat2286_practice-study</skos:prefLabel>
    <dc:identifier>2286</dc:identifier>
    <rdfs:domain rdf:resource="http://www.w3.org/2004/02/skos/core#Concept"/>
    <skos:example>architectural historians practice/study architectural history</skos:example>
    <rdfs:range rdf:resource="http://www.w3.org/2004/02/skos/core#Concept"/>
    <rdfs:isDefinedBy rdf:resource="http://vocab.getty.edu/ontology"/>
    <skos:scopeNote>[actor having] role - practice/study - field [of study, genre]/discipline.&#13;
Example: Egyptologists practice/study Egyptology; architectural historians practice/study architectural history</skos:scopeNote>
  </rdf:Description>
  <rdf:Description rdf:about="http://vocab.getty.edu/ontology#aat2501_made_of-require">
    <rdfs:domain rdf:resource="http://www.w3.org/2004/02/skos/core#Concept"/>
    <skos:prefLabel>aat2501_made_of-require</skos:prefLabel>
    <skos:example>ivories (sculptures) are made of/require ivory</skos:example>
    <rdfs:isDefinedBy rdf:resource="http://vocab.getty.edu/ontology"/>
    <dc:title>made of/require - material</dc:title>
    <dct:description>things - [are] made of/require - material.&#13;
Example: obsidian mirrors are made of/require obsidian; ivories (sculptures) are made of/require ivory</dct:description>
    <rdf:type rdf:resource="http://www.w3.org/2002/07/owl#ObjectProperty"/>
    <rdfs:subPropertyOf rdf:resource="http://www.w3.org/2004/02/skos/core#related"/>
    <owl:inverseOf rdf:resource="http://vocab.getty.edu/ontology#aat2502_material_for"/>
    <skos:scopeNote>things - [are] made of/require - material.&#13;
Example: obsidian mirrors are made of/require obsidian; ivories (sculptures) are made of/require ivory</skos:scopeNote>
    <rdfs:range rdf:resource="http://www.w3.org/2004/02/skos/core#Concept"/>
    <skos:example>obsidian mirrors are made of/require obsidian</skos:example>
    <rdfs:isDefinedBy rdf:resource="http://vocab.getty.edu/aat/"/>
    <dc:identifier>2501</dc:identifier>
  </rdf:Description>
  <rdf:Description rdf:about="http://vocab.getty.edu/ontology#ulan1111_master_of">
    <rdfs:subPropertyOf rdf:resource="http://www.w3.org/2004/02/skos/core#related"/>
    <skos:example>Peter Paul Rubens - master of Jan Thomas</skos:example>
    <dct:description>person - master of - person.&#13;
Example: Peter Paul Rubens - master of Jan Thomas</dct:description>
    <skos:prefLabel>ulan1111_master_of</skos:prefLabel>
    <owl:inverseOf rdf:resource="http://vocab.getty.edu/ontology#ulan1112_master_was"/>
    <rdfs:isDefinedBy rdf:resource="http://vocab.getty.edu/ontology"/>
    <dc:identifier>1111</dc:identifier>
    <skos:scopeNote>person - master of - person.&#13;
Example: Peter Paul Rubens - master of Jan Thomas</skos:scopeNote>
    <rdfs:domain rdf:resource="http://www.w3.org/2004/02/skos/core#Concept"/>
    <rdf:type rdf:resource="http://www.w3.org/2002/07/owl#ObjectProperty"/>
    <dc:title>master of - person</dc:title>
    <rdfs:isDefinedBy rdf:resource="http://vocab.getty.edu/ulan/"/>
    <rdfs:range rdf:resource="http://www.w3.org/2004/02/skos/core#Concept"/>
  </rdf:Description>
  <rdf:Description rdf:about="http://vocab.getty.edu/ontology#ulan1411_successor_of">
    <dc:identifier>1411</dc:identifier>
    <skos:prefLabel>ulan1411_successor_of</skos:prefLabel>
    <dc:title>successor of - firm/group</dc:title>
    <rdfs:isDefinedBy rdf:resource="http://vocab.getty.edu/ulan/"/>
    <dct:description>firm/group - successor of - firm/group.&#13;
Example: Richard Meier &amp; Partners Architects LLP is the successor of Richard Meier &amp; Associates</dct:description>
    <owl:inverseOf rdf:resource="http://vocab.getty.edu/ontology#ulan1412_predecessor_of"/>
    <rdfs:range rdf:resource="http://www.w3.org/2004/02/skos/core#Concept"/>
    <rdf:type rdf:resource="http://www.w3.org/2002/07/owl#ObjectProperty"/>
    <rdfs:isDefinedBy rdf:resource="http://vocab.getty.edu/ontology"/>
    <skos:scopeNote>firm/group - successor of - firm/group.&#13;
Example: Richard Meier &amp; Partners Architects LLP is the successor of Richard Meier &amp; Associates</skos:scopeNote>
    <rdfs:domain rdf:resource="http://www.w3.org/2004/02/skos/core#Concept"/>
    <rdfs:subPropertyOf rdf:resource="http://www.w3.org/2004/02/skos/core#related"/>
    <skos:example>Richard Meier &amp; Partners Architects LLP is the successor of Richard Meier &amp; Associates</skos:example>
  </rdf:Description>
  <rdf:Description rdf:about="http://vocab.getty.edu/ontology#ulan1306_performs_with">
    <dc:identifier>1306</dc:identifier>
    <dct:description>person - performs with - person.&#13;
Example: Harry Kipper performs with Harry Kipper (as part of 'The Kipper Kids')</dct:description>
    <dc:title>performs with - person</dc:title>
    <rdf:type rdf:resource="http://www.w3.org/2002/07/owl#ObjectProperty"/>
    <skos:scopeNote>person - performs with - person.&#13;
Example: Harry Kipper performs with Harry Kipper (as part of 'The Kipper Kids')</skos:scopeNote>
    <rdfs:isDefinedBy rdf:resource="http://vocab.getty.edu/ulan/"/>
    <rdfs:isDefinedBy rdf:resource="http://vocab.getty.edu/ontology"/>
    <skos:prefLabel>ulan1306_performs_with</skos:prefLabel>
    <rdf:type rdf:resource="http://www.w3.org/2002/07/owl#SymmetricProperty"/>
    <skos:example>Harry Kipper performs with Harry Kipper (as part of 'The Kipper Kids')</skos:example>
    <rdfs:range rdf:resource="http://www.w3.org/2004/02/skos/core#Concept"/>
    <rdfs:subPropertyOf rdf:resource="http://www.w3.org/2004/02/skos/core#related"/>
    <rdfs:domain rdf:resource="http://www.w3.org/2004/02/skos/core#Concept"/>
  </rdf:Description>
  <rdf:Description rdf:about="http://vocab.getty.edu/ontology#aat2211_produce">
    <rdf:type rdf:resource="http://www.w3.org/2002/07/owl#ObjectProperty"/>
    <rdfs:isDefinedBy rdf:resource="http://vocab.getty.edu/ontology"/>
    <rdfs:range rdf:resource="http://www.w3.org/2004/02/skos/core#Concept"/>
    <rdfs:subPropertyOf rdf:resource="http://www.w3.org/2004/02/skos/core#related"/>
    <rdfs:domain rdf:resource="http://www.w3.org/2004/02/skos/core#Concept"/>
    <skos:example>stereoscopic cameras produce stereoscopic photographs</skos:example>
    <skos:prefLabel>aat2211_produce</skos:prefLabel>
    <dc:identifier>2211</dc:identifier>
    <dct:description>things/[equipment] - produce - things.&#13;
Example: stereoscopic cameras produce stereoscopic photographs; punches (marking tools) produce punchwork</dct:description>
    <owl:inverseOf rdf:resource="http://vocab.getty.edu/ontology#aat2212_produced_by"/>
    <skos:example>punches (marking tools) produce punchwork</skos:example>
    <dc:title>produce - things</dc:title>
    <skos:scopeNote>things/[equipment] - produce - things.&#13;
Example: stereoscopic cameras produce stereoscopic photographs; punches (marking tools) produce punchwork</skos:scopeNote>
    <rdfs:isDefinedBy rdf:resource="http://vocab.getty.edu/aat/"/>
  </rdf:Description>
  <rdf:Description rdf:about="http://vocab.getty.edu/ontology#ulan1107_influenced">
    <dc:title>influenced - person</dc:title>
    <owl:inverseOf rdf:resource="http://vocab.getty.edu/ontology#ulan1108_influenced_by"/>
    <skos:scopeNote>person - influenced - person.&#13;
Example: Rembrandt van Rijn influenced Salomon Koninck</skos:scopeNote>
    <rdfs:range rdf:resource="http://www.w3.org/2004/02/skos/core#Concept"/>
    <rdfs:domain rdf:resource="http://www.w3.org/2004/02/skos/core#Concept"/>
    <rdfs:subPropertyOf rdf:resource="http://www.w3.org/2004/02/skos/core#related"/>
    <skos:prefLabel>ulan1107_influenced</skos:prefLabel>
    <rdfs:isDefinedBy rdf:resource="http://vocab.getty.edu/ulan/"/>
    <dc:identifier>1107</dc:identifier>
    <rdf:type rdf:resource="http://www.w3.org/2002/07/owl#ObjectProperty"/>
    <rdfs:isDefinedBy rdf:resource="http://vocab.getty.edu/ontology"/>
    <skos:example>Rembrandt van Rijn influenced Salomon Koninck</skos:example>
    <dct:description>person - influenced - person.&#13;
Example: Rembrandt van Rijn influenced Salomon Koninck</dct:description>
  </rdf:Description>
  <rdf:Description rdf:about="http://vocab.getty.edu/ontology#historicFlag">
    <dct:description>Historic Flag</dct:description>
    <rdf:type rdf:resource="http://www.w3.org/2002/07/owl#ObjectProperty"/>
    <rdfs:isDefinedBy rdf:resource="http://vocab.getty.edu/ontology"/>
    <rdfs:label>historicFlag</rdfs:label>
    <skos:prefLabel>historicFlag</skos:prefLabel>
    <rdfs:range rdf:resource="http://www.w3.org/2004/02/skos/core#Concept"/>
    <skos:scopeNote>Historic Flag</skos:scopeNote>
  </rdf:Description>
  <rdf:Description rdf:about="http://vocab.getty.edu/ontology#ulan1548_domestic_partner_of">
    <rdf:type rdf:resource="http://www.w3.org/2002/07/owl#ObjectProperty"/>
    <rdfs:isDefinedBy rdf:resource="http://vocab.getty.edu/ontology"/>
    <skos:scopeNote>person - domestic partner of - person</skos:scopeNote>
    <rdfs:range rdf:resource="http://www.w3.org/2004/02/skos/core#Concept"/>
    <rdfs:subPropertyOf rdf:resource="http://www.w3.org/2004/02/skos/core#related"/>
    <rdfs:domain rdf:resource="http://www.w3.org/2004/02/skos/core#Concept"/>
    <dc:title>domestic partner of - person</dc:title>
    <rdfs:isDefinedBy rdf:resource="http://vocab.getty.edu/ulan/"/>
    <dc:identifier>1548</dc:identifier>
    <dct:description>person - domestic partner of - person</dct:description>
    <rdf:type rdf:resource="http://www.w3.org/2002/07/owl#SymmetricProperty"/>
    <skos:prefLabel>ulan1548_domestic_partner_of</skos:prefLabel>
  </rdf:Description>
  <rdf:Description rdf:about="http://vocab.getty.edu/ontology#aat2335_associated_with">
    <dc:identifier>2335</dc:identifier>
    <dct:description>[actors having] role - [are] associated with - style/period/culture/[religion/ideology].&#13;
Example: abstract artists are associated with Abstract (fine arts style); popes are associated with Roman Catholicism</dct:description>
    <rdfs:domain rdf:resource="http://www.w3.org/2004/02/skos/core#Concept"/>
    <rdfs:isDefinedBy rdf:resource="http://vocab.getty.edu/aat/"/>
    <rdfs:range rdf:resource="http://www.w3.org/2004/02/skos/core#Concept"/>
    <skos:example>popes are associated with Roman Catholicism</skos:example>
    <owl:inverseOf rdf:resource="http://vocab.getty.edu/ontology#aat2336_has_associates"/>
    <skos:example>abstract artists are associated with Abstract (fine arts style)</skos:example>
    <rdfs:isDefinedBy rdf:resource="http://vocab.getty.edu/ontology"/>
    <dc:title>associated with - style/period/culture</dc:title>
    <rdf:type rdf:resource="http://www.w3.org/2002/07/owl#ObjectProperty"/>
    <skos:prefLabel>aat2335_associated_with</skos:prefLabel>
    <skos:scopeNote>[actors having] role - [are] associated with - style/period/culture/[religion/ideology].&#13;
Example: abstract artists are associated with Abstract (fine arts style); popes are associated with Roman Catholicism</skos:scopeNote>
    <rdfs:subPropertyOf rdf:resource="http://www.w3.org/2004/02/skos/core#related"/>
  </rdf:Description>
  <rdf:Description rdf:about="http://vocab.getty.edu/ontology#ulan1532_uncle-aunt_of">
    <rdfs:subPropertyOf rdf:resource="http://www.w3.org/2004/02/skos/core#related"/>
    <dc:identifier>1532</dc:identifier>
    <dct:description>person - uncle/aunt of - person.&#13;
Example: Edouard Manet is the uncle/aunt of Julie Manet</dct:description>
    <rdfs:isDefinedBy rdf:resource="http://vocab.getty.edu/ontology"/>
    <skos:example>Edouard Manet is the uncle/aunt of Julie Manet</skos:example>
    <skos:scopeNote>person - uncle/aunt of - person.&#13;
Example: Edouard Manet is the uncle/aunt of Julie Manet</skos:scopeNote>
    <rdf:type rdf:resource="http://www.w3.org/2002/07/owl#ObjectProperty"/>
    <rdfs:range rdf:resource="http://www.w3.org/2004/02/skos/core#Concept"/>
    <dc:title>uncle/aunt of - person</dc:title>
    <skos:prefLabel>ulan1532_uncle-aunt_of</skos:prefLabel>
    <rdfs:isDefinedBy rdf:resource="http://vocab.getty.edu/ulan/"/>
    <rdfs:domain rdf:resource="http://www.w3.org/2004/02/skos/core#Concept"/>
  </rdf:Description>
  <rdf:Description rdf:about="http://vocab.getty.edu/ontology#Concept">
    <skos:prefLabel>Concept</skos:prefLabel>
    <rdf:type rdf:resource="http://www.w3.org/2002/07/owl#Class"/>
    <rdfs:isDefinedBy rdf:resource="http://vocab.getty.edu/ontology"/>
    <rdfs:subClassOf rdf:resource="http://vocab.getty.edu/ontology#Subject"/>
    <skos:broader rdf:resource="http://vocab.getty.edu/ontology#Subject"/>
    <dct:description>Proper concept. Used in AAT only; TGN &amp; ULAN have their own, e.g. gvp:PhysPlaceConcept &amp; gvp:PersonConcept. Used for indexing and cataloguing.
Example: rhyta (AAT)</dct:description>
    <skos:example>rhyta (AAT)</skos:example>
    <rdfs:comment>Proper concept. Used in AAT only; TGN &amp; ULAN have their own, e.g. gvp:PhysPlaceConcept &amp; gvp:PersonConcept. Used for indexing and cataloguing</rdfs:comment>
    <rdfs:subClassOf rdf:resource="http://www.w3.org/2004/02/skos/core#Concept"/>
    <skos:definition>Proper concept. Used in AAT only; TGN &amp; ULAN have their own, e.g. gvp:PhysPlaceConcept &amp; gvp:PersonConcept. Used for indexing and cataloguing</skos:definition>
    <skos:scopeNote>Proper concept. Used in AAT only; TGN &amp; ULAN have their own, e.g. gvp:PhysPlaceConcept &amp; gvp:PersonConcept. Used for indexing and cataloguing.
Example: rhyta (AAT)</skos:scopeNote>
    <rdfs:label>Concept</rdfs:label>
  </rdf:Description>
  <rdf:Description rdf:about="http://vocab.getty.edu/ontology#ulan1574_godparent_of">
    <skos:prefLabel>ulan1574_godparent_of</skos:prefLabel>
    <rdfs:range rdf:resource="http://www.w3.org/2004/02/skos/core#Concept"/>
    <rdfs:domain rdf:resource="http://www.w3.org/2004/02/skos/core#Concept"/>
    <owl:inverseOf rdf:resource="http://vocab.getty.edu/ontology#ulan1575_godchild_of"/>
    <dct:description>person - godparent of - person.&#13;
Example: Jean-Baptiste Goy is godparent of Jean I Nocret</dct:description>
    <dc:identifier>1574</dc:identifier>
    <dc:title>godparent of - person</dc:title>
    <rdf:type rdf:resource="http://www.w3.org/2002/07/owl#ObjectProperty"/>
    <skos:example>Jean-Baptiste Goy is godparent of Jean I Nocret</skos:example>
    <rdfs:isDefinedBy rdf:resource="http://vocab.getty.edu/ontology"/>
    <rdfs:subPropertyOf rdf:resource="http://www.w3.org/2004/02/skos/core#related"/>
    <skos:scopeNote>person - godparent of - person.&#13;
Example: Jean-Baptiste Goy is godparent of Jean I Nocret</skos:scopeNote>
    <rdfs:isDefinedBy rdf:resource="http://vocab.getty.edu/ulan/"/>
  </rdf:Description>
  <rdf:Description rdf:about="http://vocab.getty.edu/ontology#aat2422_takes_place_in">
    <rdf:type rdf:resource="http://www.w3.org/2002/07/owl#ObjectProperty"/>
    <rdfs:isDefinedBy rdf:resource="http://vocab.getty.edu/ontology"/>
    <dct:description>activity/event/[process/function] - takes place in - locus/setting.&#13;
Example: smelting takes place in smelters (metalworking plants); pilgrimages take place in pilgrimage centers</dct:description>
    <rdfs:isDefinedBy rdf:resource="http://vocab.getty.edu/aat/"/>
    <skos:example>pilgrimages take place in pilgrimage centers</skos:example>
    <dc:identifier>2422</dc:identifier>
    <dc:title>takes place in - locus/setting</dc:title>
    <rdfs:domain rdf:resource="http://www.w3.org/2004/02/skos/core#Concept"/>
    <rdfs:range rdf:resource="http://www.w3.org/2004/02/skos/core#Concept"/>
    <skos:prefLabel>aat2422_takes_place_in</skos:prefLabel>
    <skos:example>smelting takes place in smelters (metalworking plants)</skos:example>
    <rdfs:subPropertyOf rdf:resource="http://www.w3.org/2004/02/skos/core#related"/>
    <skos:scopeNote>activity/event/[process/function] - takes place in - locus/setting.&#13;
Example: smelting takes place in smelters (metalworking plants); pilgrimages take place in pilgrimage centers</skos:scopeNote>
  </rdf:Description>
  <rdf:Description rdf:about="http://vocab.getty.edu/ontology#tgn3110_meaning-usage_overlaps_with">
    <rdfs:domain rdf:resource="http://www.w3.org/2004/02/skos/core#Concept"/>
    <rdfs:range rdf:resource="http://www.w3.org/2004/02/skos/core#Concept"/>
    <rdfs:isDefinedBy rdf:resource="http://vocab.getty.edu/tgn/"/>
    <rdfs:isDefinedBy rdf:resource="http://vocab.getty.edu/ontology"/>
    <skos:prefLabel>tgn3110_meaning-usage_overlaps_with</skos:prefLabel>
    <rdfs:subPropertyOf rdf:resource="http://www.w3.org/2004/02/skos/core#related"/>
    <rdf:type rdf:resource="http://www.w3.org/2002/07/owl#ObjectProperty"/>
    <skos:scopeNote>any - meaning/usage overlaps with - any.&#13;
Example: Judaea (Israel) (historical region) meaning/usage overlaps with Holy Land (Asia) (historical region)</skos:scopeNote>
    <dct:description>any - meaning/usage overlaps with - any.&#13;
Example: Judaea (Israel) (historical region) meaning/usage overlaps with Holy Land (Asia) (historical region)</dct:description>
    <dc:identifier>3110</dc:identifier>
    <skos:example>Judaea (Israel) (historical region) meaning/usage overlaps with Holy Land (Asia) (historical region)</skos:example>
    <rdf:type rdf:resource="http://www.w3.org/2002/07/owl#SymmetricProperty"/>
    <dc:title>meaning/usage overlaps with - any</dc:title>
  </rdf:Description>
  <rdf:Description rdf:about="http://vocab.getty.edu/ontology#aat2563_located_in">
    <dc:identifier>2563</dc:identifier>
    <skos:scopeNote>style/period/culture/[religion/ideology] - is located/[reflected] in - locus/setting.&#13;
Example: First Nations (culture) is located/reflected in First Nations reserves; Brahmanism is located/reflected in agraharas</skos:scopeNote>
    <rdf:type rdf:resource="http://www.w3.org/2002/07/owl#ObjectProperty"/>
    <rdfs:isDefinedBy rdf:resource="http://vocab.getty.edu/ontology"/>
    <dc:title>located in - locus/setting</dc:title>
    <rdfs:range rdf:resource="http://www.w3.org/2004/02/skos/core#Concept"/>
    <rdfs:subPropertyOf rdf:resource="http://www.w3.org/2004/02/skos/core#related"/>
    <rdfs:domain rdf:resource="http://www.w3.org/2004/02/skos/core#Concept"/>
    <skos:example>Brahmanism is located/reflected in agraharas</skos:example>
    <skos:prefLabel>aat2563_located_in</skos:prefLabel>
    <skos:example>First Nations (culture) is located/reflected in First Nations reserves</skos:example>
    <dct:description>style/period/culture/[religion/ideology] - is located/[reflected] in - locus/setting.&#13;
Example: First Nations (culture) is located/reflected in First Nations reserves; Brahmanism is located/reflected in agraharas</dct:description>
    <rdfs:isDefinedBy rdf:resource="http://vocab.getty.edu/aat/"/>
  </rdf:Description>
  <rdf:Description rdf:about="http://vocab.getty.edu/ontology#aat2608_causes-required_for">
    <dct:description>activity/event/[process/function] - causes/[is] required for - [a] state/condition/attributes.&#13;
Example: waterproofing causes/is required for watertighness; creasing (process) causes/is required for creases (condition)</dct:description>
    <dc:identifier>2608</dc:identifier>
    <rdfs:isDefinedBy rdf:resource="http://vocab.getty.edu/aat/"/>
    <rdfs:range rdf:resource="http://www.w3.org/2004/02/skos/core#Concept"/>
    <skos:prefLabel>aat2608_causes-required_for</skos:prefLabel>
    <rdfs:domain rdf:resource="http://www.w3.org/2004/02/skos/core#Concept"/>
    <skos:example>waterproofing causes/is required for watertighness</skos:example>
    <rdf:type rdf:resource="http://www.w3.org/2002/07/owl#ObjectProperty"/>
    <dc:title>causes/required for - attributes /associated concepts</dc:title>
    <rdfs:isDefinedBy rdf:resource="http://vocab.getty.edu/ontology"/>
    <skos:scopeNote>activity/event/[process/function] - causes/[is] required for - [a] state/condition/attributes.&#13;
Example: waterproofing causes/is required for watertighness; creasing (process) causes/is required for creases (condition)</skos:scopeNote>
    <rdfs:subPropertyOf rdf:resource="http://www.w3.org/2004/02/skos/core#related"/>
    <skos:example>creasing (process) causes/is required for creases (condition)</skos:example>
  </rdf:Description>
  <rdf:Description rdf:about="http://vocab.getty.edu/ontology#aat2805_contextualized_in">
    <rdfs:range rdf:resource="http://www.w3.org/2004/02/skos/core#Concept"/>
    <rdfs:domain rdf:resource="http://www.w3.org/2004/02/skos/core#Concept"/>
    <rdfs:subPropertyOf rdf:resource="http://www.w3.org/2004/02/skos/core#related"/>
    <skos:example>predellas are contextualized in altarpieces</skos:example>
    <rdfs:isDefinedBy rdf:resource="http://vocab.getty.edu/ontology"/>
    <dc:identifier>2805</dc:identifier>
    <rdf:type rdf:resource="http://www.w3.org/2002/07/owl#ObjectProperty"/>
    <dct:description>[smaller] things - [are] contextualized in - [larger] things.&#13;
Example: predellas are contextualized in altarpieces; chapters are contextualized in books</dct:description>
    <skos:prefLabel>aat2805_contextualized_in</skos:prefLabel>
    <owl:inverseOf rdf:resource="http://vocab.getty.edu/ontology#aat2806_provide_context"/>
    <rdfs:isDefinedBy rdf:resource="http://vocab.getty.edu/aat/"/>
    <skos:example>chapters are contextualized in books</skos:example>
    <dc:title>contextualized in - things</dc:title>
    <skos:scopeNote>[smaller] things - [are] contextualized in - [larger] things.&#13;
Example: predellas are contextualized in altarpieces; chapters are contextualized in books</skos:scopeNote>
  </rdf:Description>
  <rdf:Description rdf:about="http://vocab.getty.edu/ontology#ulan1000_related_to">
    <rdfs:isDefinedBy rdf:resource="http://vocab.getty.edu/ulan/"/>
    <skos:prefLabel>ulan1000_related_to</skos:prefLabel>
    <dc:identifier>1000</dc:identifier>
    <dc:title>related to - any</dc:title>
    <rdf:type rdf:resource="http://www.w3.org/2002/07/owl#ObjectProperty"/>
    <rdfs:isDefinedBy rdf:resource="http://vocab.getty.edu/ontology"/>
    <rdfs:domain rdf:resource="http://www.w3.org/2004/02/skos/core#Concept"/>
    <skos:example>National Endowment for the Humanities is related to Connecticut Humanities Council</skos:example>
    <skos:scopeNote>any - related to - any.&#13;
Example: Frank Lloyd Wright is related to Francis Conroy Sullivan; Herman Miller, Inc. is related to Irving Harper; National Endowment for the Humanities is related to Connecticut Humanities Council</skos:scopeNote>
    <skos:example>Herman Miller, Inc. is related to Irving Harper</skos:example>
    <skos:example>Frank Lloyd Wright is related to Francis Conroy Sullivan</skos:example>
    <rdf:type rdf:resource="http://www.w3.org/2002/07/owl#SymmetricProperty"/>
    <dct:description>any - related to - any.&#13;
Example: Frank Lloyd Wright is related to Francis Conroy Sullivan; Herman Miller, Inc. is related to Irving Harper; National Endowment for the Humanities is related to Connecticut Humanities Council</dct:description>
    <rdfs:range rdf:resource="http://www.w3.org/2004/02/skos/core#Concept"/>
    <rdfs:subPropertyOf rdf:resource="http://www.w3.org/2004/02/skos/core#related"/>
  </rdf:Description>
  <rdf:Description rdf:about="http://vocab.getty.edu/ontology#ulan1201_patron_of">
    <rdfs:isDefinedBy rdf:resource="http://vocab.getty.edu/ulan/"/>
    <skos:example>Cosimo I, Grand-Duke of Tuscany was the patron of Donatello</skos:example>
    <rdfs:range rdf:resource="http://www.w3.org/2004/02/skos/core#Concept"/>
    <rdf:type rdf:resource="http://www.w3.org/2002/07/owl#ObjectProperty"/>
    <owl:inverseOf rdf:resource="http://vocab.getty.edu/ontology#ulan1202_patron_was"/>
    <rdfs:isDefinedBy rdf:resource="http://vocab.getty.edu/ontology"/>
    <dc:title>patron of - person/firm/family</dc:title>
    <skos:prefLabel>ulan1201_patron_of</skos:prefLabel>
    <dc:identifier>1201</dc:identifier>
    <skos:scopeNote>person - patron of - person/firm/family.&#13;
Example: Cosimo I, Grand-Duke of Tuscany was the patron of Donatello</skos:scopeNote>
    <rdfs:domain rdf:resource="http://www.w3.org/2004/02/skos/core#Concept"/>
    <dct:description>person - patron of - person/firm/family.&#13;
Example: Cosimo I, Grand-Duke of Tuscany was the patron of Donatello</dct:description>
    <rdfs:subPropertyOf rdf:resource="http://www.w3.org/2004/02/skos/core#related"/>
  </rdf:Description>
  <rdf:Description rdf:about="http://vocab.getty.edu/ontology#aat2837_source_for">
    <rdfs:subPropertyOf rdf:resource="http://www.w3.org/2004/02/skos/core#related"/>
    <skos:example>Phormium tenax (species) is the source for k?kaku</skos:example>
    <dc:title>source for - things</dc:title>
    <skos:example>Struthio camelus(species) is the source for ostrich-egg cups</skos:example>
    <skos:prefLabel>aat2837_source_for</skos:prefLabel>
    <skos:scopeNote>genus/species [or its parts] - [is] source for - things.&#13;
Example: Phormium tenax (species) is the source for k?kaku; Struthio camelus(species) is the source for ostrich-egg cups</skos:scopeNote>
    <rdfs:isDefinedBy rdf:resource="http://vocab.getty.edu/aat/"/>
    <rdfs:isDefinedBy rdf:resource="http://vocab.getty.edu/ontology"/>
    <rdfs:domain rdf:resource="http://www.w3.org/2004/02/skos/core#Concept"/>
    <rdf:type rdf:resource="http://www.w3.org/2002/07/owl#ObjectProperty"/>
    <rdfs:range rdf:resource="http://www.w3.org/2004/02/skos/core#Concept"/>
    <dct:description>genus/species [or its parts] - [is] source for - things.&#13;
Example: Phormium tenax (species) is the source for k?kaku; Struthio camelus(species) is the source for ostrich-egg cups</dct:description>
    <dc:identifier>2837</dc:identifier>
  </rdf:Description>
  <rdf:Description rdf:about="http://vocab.getty.edu/ontology#broaderPartitive">
    <rdfs:subPropertyOf rdf:resource="http://vocab.getty.edu/ontology#broaderPartitiveExtended"/>
    <rdfs:subPropertyOf rdf:resource="http://vocab.getty.edu/ontology#broader"/>
    <skos:prefLabel>broaderPartitive</skos:prefLabel>
    <rdf:type rdf:resource="http://www.w3.org/2002/07/owl#ObjectProperty"/>
    <rdfs:domain rdf:resource="http://vocab.getty.edu/ontology#Subject"/>
    <rdfs:isDefinedBy rdf:resource="http://vocab.getty.edu/ontology"/>
    <dct:description>BTP (Part/Whole, "part of") relation. We also infer iso-thes:broaderPartitive, which goes only between Concepts.
Example: Tuscany (TGN) BTP Italy (TGN)</dct:description>
    <rdfs:range rdf:resource="http://vocab.getty.edu/ontology#Subject"/>
    <skos:scopeNote>BTP (Part/Whole, "part of") relation. We also infer iso-thes:broaderPartitive, which goes only between Concepts.
Example: Tuscany (TGN) BTP Italy (TGN)</skos:scopeNote>
    <skos:example>Tuscany (TGN) BTP Italy (TGN)</skos:example>
    <rdfs:label>broaderPartitive</rdfs:label>
    <skos:definition>BTP (Part/Whole, "part of") relation. We also infer iso-thes:broaderPartitive, which goes only between Concepts</skos:definition>
    <rdfs:comment>BTP (Part/Whole, "part of") relation. We also infer iso-thes:broaderPartitive, which goes only between Concepts</rdfs:comment>
  </rdf:Description>
  <rdf:Description rdf:about="http://vocab.getty.edu/ontology#aat2876_characterized_by">
    <skos:example>Celtic (culture) is characterized by Celtic (language)</skos:example>
    <dc:identifier>2876</dc:identifier>
    <skos:scopeNote>style/period/culture - [is] characterized by - language.&#13;
Example: Afar (culture) is characterized by Afar (language); Celtic (culture) is characterized by Celtic (language)</skos:scopeNote>
    <dct:description>style/period/culture - [is] characterized by - language.&#13;
Example: Afar (culture) is characterized by Afar (language); Celtic (culture) is characterized by Celtic (language)</dct:description>
    <rdfs:domain rdf:resource="http://www.w3.org/2004/02/skos/core#Concept"/>
    <dc:title>characterized by - language</dc:title>
    <rdfs:range rdf:resource="http://www.w3.org/2004/02/skos/core#Concept"/>
    <rdfs:subPropertyOf rdf:resource="http://www.w3.org/2004/02/skos/core#related"/>
    <skos:prefLabel>aat2876_characterized_by</skos:prefLabel>
    <rdf:type rdf:resource="http://www.w3.org/2002/07/owl#ObjectProperty"/>
    <rdfs:isDefinedBy rdf:resource="http://vocab.getty.edu/ontology"/>
    <skos:example>Afar (culture) is characterized by Afar (language)</skos:example>
    <rdfs:isDefinedBy rdf:resource="http://vocab.getty.edu/aat/"/>
  </rdf:Description>
  <rdf:Description rdf:about="http://vocab.getty.edu/ontology#ulan1214_court_artist_was">
    <dc:identifier>1214</dc:identifier>
    <dct:description>person - court artist was - person.&#13;
Example: Peter Paul Rubens was court artist to Gonzaga Vincenzo I, Duke of Mantua; Francisco de Goya was court artist to Charles IV, King of Spain</dct:description>
    <rdfs:range rdf:resource="http://www.w3.org/2004/02/skos/core#Concept"/>
    <rdfs:domain rdf:resource="http://www.w3.org/2004/02/skos/core#Concept"/>
    <dc:title>court artist was - person</dc:title>
    <rdfs:isDefinedBy rdf:resource="http://vocab.getty.edu/ulan/"/>
    <skos:example>Francisco de Goya was court artist to Charles IV, King of Spain</skos:example>
    <skos:example>Peter Paul Rubens was court artist to Gonzaga Vincenzo I, Duke of Mantua</skos:example>
    <skos:scopeNote>person - court artist was - person.&#13;
Example: Peter Paul Rubens was court artist to Gonzaga Vincenzo I, Duke of Mantua; Francisco de Goya was court artist to Charles IV, King of Spain</skos:scopeNote>
    <rdfs:subPropertyOf rdf:resource="http://www.w3.org/2004/02/skos/core#related"/>
    <rdfs:isDefinedBy rdf:resource="http://vocab.getty.edu/ontology"/>
    <rdf:type rdf:resource="http://www.w3.org/2002/07/owl#ObjectProperty"/>
    <skos:prefLabel>ulan1214_court_artist_was</skos:prefLabel>
  </rdf:Description>
  <rdf:Description rdf:about="http://vocab.getty.edu/ontology#aat2821_based_on">
    <dct:description>any - [is] based on - any.&#13;
Example: Neo-Gothic is based on Gothic (Medieval); curved [form attribute] is based on curves (geometric figures); pencils are based on plummets</dct:description>
    <rdf:type rdf:resource="http://www.w3.org/2002/07/owl#ObjectProperty"/>
    <rdfs:isDefinedBy rdf:resource="http://vocab.getty.edu/ontology"/>
    <dc:title>based on - any</dc:title>
    <rdfs:domain rdf:resource="http://www.w3.org/2004/02/skos/core#Concept"/>
    <rdfs:subPropertyOf rdf:resource="http://www.w3.org/2004/02/skos/core#related"/>
    <skos:prefLabel>aat2821_based_on</skos:prefLabel>
    <rdfs:range rdf:resource="http://www.w3.org/2004/02/skos/core#Concept"/>
    <skos:scopeNote>any - [is] based on - any.&#13;
Example: Neo-Gothic is based on Gothic (Medieval); curved [form attribute] is based on curves (geometric figures); pencils are based on plummets</skos:scopeNote>
    <skos:example>pencils are based on plummets</skos:example>
    <dc:identifier>2821</dc:identifier>
    <skos:example>curved [form attribute] is based on curves (geometric figures)</skos:example>
    <owl:inverseOf rdf:resource="http://vocab.getty.edu/ontology#aat2822_basis_of"/>
    <skos:example>Neo-Gothic is based on Gothic (Medieval)</skos:example>
    <rdfs:isDefinedBy rdf:resource="http://vocab.getty.edu/aat/"/>
  </rdf:Description>
  <rdf:Description rdf:about="http://vocab.getty.edu/ontology#ulan2697_leader_was">
    <dc:title>leader was - person</dc:title>
    <rdf:type rdf:resource="http://www.w3.org/2002/07/owl#ObjectProperty"/>
    <skos:prefLabel>ulan2697_leader_was</skos:prefLabel>
    <skos:scopeNote>institution - leader was - person.&#13;
Example: The leader of Samuel H. Kress Foundation was Rush Harrison Kress</skos:scopeNote>
    <rdfs:range rdf:resource="http://www.w3.org/2004/02/skos/core#Concept"/>
    <dc:identifier>2697</dc:identifier>
    <rdfs:domain rdf:resource="http://www.w3.org/2004/02/skos/core#Concept"/>
    <dct:description>institution - leader was - person.&#13;
Example: The leader of Samuel H. Kress Foundation was Rush Harrison Kress</dct:description>
    <rdfs:isDefinedBy rdf:resource="http://vocab.getty.edu/ulan/"/>
    <skos:example>The leader of Samuel H. Kress Foundation was Rush Harrison Kress</skos:example>
    <rdfs:subPropertyOf rdf:resource="http://www.w3.org/2004/02/skos/core#related"/>
    <rdfs:isDefinedBy rdf:resource="http://vocab.getty.edu/ontology"/>
  </rdf:Description>
  <rdf:Description rdf:about="http://vocab.getty.edu/ontology#ulan1552_parent_by_marriage_of">
    <rdfs:isDefinedBy rdf:resource="http://vocab.getty.edu/ulan/"/>
    <dct:description>person - parent by marriage (step parent) - person.&#13;
Example: Frans Hals is a parent by marriage of Pieter Gerritsz van Roestraten</dct:description>
    <owl:inverseOf rdf:resource="http://vocab.getty.edu/ontology#ulan1553_child_by_marriage_of"/>
    <skos:prefLabel>ulan1552_parent_by_marriage_of</skos:prefLabel>
    <skos:scopeNote>person - parent by marriage (step parent) - person.&#13;
Example: Frans Hals is a parent by marriage of Pieter Gerritsz van Roestraten</skos:scopeNote>
    <dc:identifier>1552</dc:identifier>
    <rdfs:subPropertyOf rdf:resource="http://www.w3.org/2004/02/skos/core#related"/>
    <dc:title>parent by marriage of - person</dc:title>
    <rdfs:domain rdf:resource="http://www.w3.org/2004/02/skos/core#Concept"/>
    <rdfs:range rdf:resource="http://www.w3.org/2004/02/skos/core#Concept"/>
    <skos:example>Frans Hals is a parent by marriage of Pieter Gerritsz van Roestraten</skos:example>
    <rdf:type rdf:resource="http://www.w3.org/2002/07/owl#ObjectProperty"/>
    <rdfs:isDefinedBy rdf:resource="http://vocab.getty.edu/ontology"/>
  </rdf:Description>
  <rdf:Description rdf:about="http://vocab.getty.edu/ontology#tgn3412_predecessor_of">
    <rdf:type rdf:resource="http://www.w3.org/2002/07/owl#ObjectProperty"/>
    <rdfs:isDefinedBy rdf:resource="http://vocab.getty.edu/ontology"/>
    <dc:identifier>3412</dc:identifier>
    <dc:title>predecessor of - nation</dc:title>
    <rdfs:domain rdf:resource="http://www.w3.org/2004/02/skos/core#Concept"/>
    <rdfs:range rdf:resource="http://www.w3.org/2004/02/skos/core#Concept"/>
    <skos:example>Persia is the predecessor of Iran (nation)</skos:example>
    <skos:scopeNote>nation - predecessor of - nation.&#13;
Example: Persia is the predecessor of Iran (nation)</skos:scopeNote>
    <rdfs:isDefinedBy rdf:resource="http://vocab.getty.edu/tgn/"/>
    <dct:description>nation - predecessor of - nation.&#13;
Example: Persia is the predecessor of Iran (nation)</dct:description>
    <skos:prefLabel>tgn3412_predecessor_of</skos:prefLabel>
    <rdfs:subPropertyOf rdf:resource="http://www.w3.org/2004/02/skos/core#related"/>
  </rdf:Description>
  <rdf:Description rdf:about="http://vocab.getty.edu/ontology#aat2325_created_by">
    <rdfs:isDefinedBy rdf:resource="http://vocab.getty.edu/aat/"/>
    <skos:scopeNote>things - [are] created by - [actors having] role.&#13;
Example: drawings are created by draftsmen; poems are created by poets</skos:scopeNote>
    <skos:prefLabel>aat2325_created_by</skos:prefLabel>
    <skos:example>drawings are created by draftsmen</skos:example>
    <skos:example>poems are created by poets</skos:example>
    <rdfs:domain rdf:resource="http://www.w3.org/2004/02/skos/core#Concept"/>
    <dct:description>things - [are] created by - [actors having] role.&#13;
Example: drawings are created by draftsmen; poems are created by poets</dct:description>
    <rdfs:range rdf:resource="http://www.w3.org/2004/02/skos/core#Concept"/>
    <rdfs:subPropertyOf rdf:resource="http://www.w3.org/2004/02/skos/core#related"/>
    <rdfs:isDefinedBy rdf:resource="http://vocab.getty.edu/ontology"/>
    <dc:identifier>2325</dc:identifier>
    <dc:title>created by - role</dc:title>
    <rdf:type rdf:resource="http://www.w3.org/2002/07/owl#ObjectProperty"/>
    <owl:inverseOf rdf:resource="http://vocab.getty.edu/ontology#aat2326_create"/>
  </rdf:Description>
  <rdf:Description rdf:about="http://vocab.getty.edu/ontology#ulan1112_master_was">
    <rdfs:isDefinedBy rdf:resource="http://vocab.getty.edu/ulan/"/>
    <rdfs:range rdf:resource="http://www.w3.org/2004/02/skos/core#Concept"/>
    <dc:title>master was - person</dc:title>
    <rdf:type rdf:resource="http://www.w3.org/2002/07/owl#ObjectProperty"/>
    <dct:description>person - master was - person.&#13;
Example: Peter Paul Rubens - master of Jan Thomas</dct:description>
    <skos:prefLabel>ulan1112_master_was</skos:prefLabel>
    <rdfs:isDefinedBy rdf:resource="http://vocab.getty.edu/ontology"/>
    <skos:scopeNote>person - master was - person.&#13;
Example: Peter Paul Rubens - master of Jan Thomas</skos:scopeNote>
    <dc:identifier>1112</dc:identifier>
    <skos:example>Peter Paul Rubens - master of Jan Thomas</skos:example>
    <rdfs:domain rdf:resource="http://www.w3.org/2004/02/skos/core#Concept"/>
    <rdfs:subPropertyOf rdf:resource="http://www.w3.org/2004/02/skos/core#related"/>
  </rdf:Description>
  <rdf:Description rdf:about="http://vocab.getty.edu/ontology#broaderGeneric">
    <skos:scopeNote>BTG (Genus/Species, "is a") relation. We also infer iso-thes:broaderGeneric, which goes only between Concepts.
Example: calcite (AAT) BTG mineral (AAT)</skos:scopeNote>
    <rdfs:subPropertyOf rdf:resource="http://vocab.getty.edu/ontology#broaderGenericExtended"/>
    <rdfs:domain rdf:resource="http://vocab.getty.edu/ontology#Subject"/>
    <skos:prefLabel>broaderGeneric</skos:prefLabel>
    <skos:definition>BTG (Genus/Species, "is a") relation. We also infer iso-thes:broaderGeneric, which goes only between Concepts</skos:definition>
    <rdfs:comment>BTG (Genus/Species, "is a") relation. We also infer iso-thes:broaderGeneric, which goes only between Concepts</rdfs:comment>
    <dct:description>BTG (Genus/Species, "is a") relation. We also infer iso-thes:broaderGeneric, which goes only between Concepts.
Example: calcite (AAT) BTG mineral (AAT)</dct:description>
    <rdf:type rdf:resource="http://www.w3.org/2002/07/owl#ObjectProperty"/>
    <rdfs:isDefinedBy rdf:resource="http://vocab.getty.edu/ontology"/>
    <rdfs:subPropertyOf rdf:resource="http://vocab.getty.edu/ontology#broader"/>
    <skos:example>calcite (AAT) BTG mineral (AAT)</skos:example>
    <rdfs:range rdf:resource="http://vocab.getty.edu/ontology#Subject"/>
    <rdfs:label>broaderGeneric</rdfs:label>
  </rdf:Description>
  <rdf:Description rdf:about="http://vocab.getty.edu/ontology#ulan2584_chaired_by">
    <rdfs:domain rdf:resource="http://www.w3.org/2004/02/skos/core#Concept"/>
    <rdf:type rdf:resource="http://www.w3.org/2002/07/owl#ObjectProperty"/>
    <skos:prefLabel>ulan2584_chaired_by</skos:prefLabel>
    <rdfs:isDefinedBy rdf:resource="http://vocab.getty.edu/ulan/"/>
    <rdfs:subPropertyOf rdf:resource="http://www.w3.org/2004/02/skos/core#related"/>
    <skos:scopeNote>institution - chaired by - person</skos:scopeNote>
    <dc:title>chaired by - person</dc:title>
    <dct:description>institution - chaired by - person</dct:description>
    <rdfs:range rdf:resource="http://www.w3.org/2004/02/skos/core#Concept"/>
    <rdfs:isDefinedBy rdf:resource="http://vocab.getty.edu/ontology"/>
    <dc:identifier>2584</dc:identifier>
  </rdf:Description>
  <rdf:Description rdf:about="http://vocab.getty.edu/ontology#termFlag">
    <rdfs:isDefinedBy rdf:resource="http://vocab.getty.edu/ontology"/>
    <rdf:type rdf:resource="http://www.w3.org/2002/07/owl#ObjectProperty"/>
    <rdfs:domain rdf:resource="http://www.w3.org/2008/05/skos-xl#Label"/>
    <skos:prefLabel>termFlag</skos:prefLabel>
    <rdfs:range rdf:resource="http://www.w3.org/2004/02/skos/core#Concept"/>
    <dct:description>Term Flag</dct:description>
    <rdfs:label>termFlag</rdfs:label>
    <skos:scopeNote>Term Flag</skos:scopeNote>
  </rdf:Description>
  <rdf:Description rdf:about="http://vocab.getty.edu/ontology#aat2432_requires">
    <rdfs:range rdf:resource="http://www.w3.org/2004/02/skos/core#Concept"/>
    <rdfs:domain rdf:resource="http://www.w3.org/2004/02/skos/core#Concept"/>
    <dc:identifier>2432</dc:identifier>
    <rdfs:subPropertyOf rdf:resource="http://www.w3.org/2004/02/skos/core#related"/>
    <rdfs:isDefinedBy rdf:resource="http://vocab.getty.edu/ontology"/>
    <skos:example>doweling requires dowels</skos:example>
    <skos:scopeNote>activity/event/process - requires - things/equipment.&#13;
Example: painting (image making) requires painting equipment; doweling requires dowels</skos:scopeNote>
    <skos:example>painting (image making) requires painting equipment</skos:example>
    <rdf:type rdf:resource="http://www.w3.org/2002/07/owl#ObjectProperty"/>
    <skos:prefLabel>aat2432_requires</skos:prefLabel>
    <rdfs:isDefinedBy rdf:resource="http://vocab.getty.edu/aat/"/>
    <dc:title>requires - things</dc:title>
    <dct:description>activity/event/process - requires - things/equipment.&#13;
Example: painting (image making) requires painting equipment; doweling requires dowels</dct:description>
  </rdf:Description>
  <rdf:Description rdf:about="http://vocab.getty.edu/ontology#aat2612_possessed_by-existing_in">
    <dct:description>attributes /associated concepts - is possessed by/existing in - material.&#13;
Example: dry rot is possessed by/existing in wood(plant material); dielectric properties are possessed by/existing in dielectric (material)</dct:description>
    <rdfs:subPropertyOf rdf:resource="http://www.w3.org/2004/02/skos/core#related"/>
    <owl:inverseOf rdf:resource="http://vocab.getty.edu/ontology#aat2613_possess-exist_in"/>
    <skos:example>dielectric properties are possessed by/existing in dielectric (material)</skos:example>
    <skos:prefLabel>aat2612_possessed_by-existing_in</skos:prefLabel>
    <dc:identifier>2612</dc:identifier>
    <rdfs:domain rdf:resource="http://www.w3.org/2004/02/skos/core#Concept"/>
    <rdfs:range rdf:resource="http://www.w3.org/2004/02/skos/core#Concept"/>
    <dc:title>possessed by/existing in - material</dc:title>
    <rdfs:isDefinedBy rdf:resource="http://vocab.getty.edu/aat/"/>
    <skos:scopeNote>attributes /associated concepts - is possessed by/existing in - material.&#13;
Example: dry rot is possessed by/existing in wood(plant material); dielectric properties are possessed by/existing in dielectric (material)</skos:scopeNote>
    <rdf:type rdf:resource="http://www.w3.org/2002/07/owl#ObjectProperty"/>
    <skos:example>dry rot is possessed by/existing in wood(plant material)</skos:example>
    <rdfs:isDefinedBy rdf:resource="http://vocab.getty.edu/ontology"/>
  </rdf:Description>
  <rdf:Description rdf:about="http://vocab.getty.edu/ontology#ulan1006_formerly_identified_with">
    <skos:example>Tommaso is formerly identified with Tommaso di Stefano Lunetti</skos:example>
    <dc:identifier>1006</dc:identifier>
    <rdf:type rdf:resource="http://www.w3.org/2002/07/owl#SymmetricProperty"/>
    <skos:scopeNote>any - formerly identified with - any.&#13;
Example: Tommaso is formerly identified with Tommaso di Stefano Lunetti; GreenWorks is formerly identified with Mike Faha &amp; Associates</skos:scopeNote>
    <rdfs:isDefinedBy rdf:resource="http://vocab.getty.edu/ulan/"/>
    <dct:description>any - formerly identified with - any.&#13;
Example: Tommaso is formerly identified with Tommaso di Stefano Lunetti; GreenWorks is formerly identified with Mike Faha &amp; Associates</dct:description>
    <rdfs:domain rdf:resource="http://www.w3.org/2004/02/skos/core#Concept"/>
    <rdfs:range rdf:resource="http://www.w3.org/2004/02/skos/core#Concept"/>
    <rdfs:subPropertyOf rdf:resource="http://www.w3.org/2004/02/skos/core#related"/>
    <rdfs:isDefinedBy rdf:resource="http://vocab.getty.edu/ontology"/>
    <rdf:type rdf:resource="http://www.w3.org/2002/07/owl#ObjectProperty"/>
    <skos:prefLabel>ulan1006_formerly_identified_with</skos:prefLabel>
    <skos:example>GreenWorks is formerly identified with Mike Faha &amp; Associates</skos:example>
    <dc:title>formerly identified with - any</dc:title>
  </rdf:Description>
  <rdf:Description rdf:about="http://vocab.getty.edu/ontology#ulan1212_artist_was">
    <rdfs:isDefinedBy rdf:resource="http://vocab.getty.edu/ulan/"/>
    <dc:title>artist was - person</dc:title>
    <rdfs:range rdf:resource="http://www.w3.org/2004/02/skos/core#Concept"/>
    <rdfs:domain rdf:resource="http://www.w3.org/2004/02/skos/core#Concept"/>
    <rdfs:subPropertyOf rdf:resource="http://www.w3.org/2004/02/skos/core#related"/>
    <skos:example>Charles-Pierre Coustou was artist to Louis XIV, King of France</skos:example>
    <skos:scopeNote>person - artist was - person.&#13;
Example: Charles-Pierre Coustou was artist to Louis XIV, King of France</skos:scopeNote>
    <rdfs:isDefinedBy rdf:resource="http://vocab.getty.edu/ontology"/>
    <skos:prefLabel>ulan1212_artist_was</skos:prefLabel>
    <dc:identifier>1212</dc:identifier>
    <dct:description>person - artist was - person.&#13;
Example: Charles-Pierre Coustou was artist to Louis XIV, King of France</dct:description>
    <rdf:type rdf:resource="http://www.w3.org/2002/07/owl#ObjectProperty"/>
  </rdf:Description>
  <rdf:Description rdf:about="http://vocab.getty.edu/ontology#ulan1414_joint_venture_with">
    <rdf:type rdf:resource="http://www.w3.org/2002/07/owl#ObjectProperty"/>
    <rdfs:isDefinedBy rdf:resource="http://vocab.getty.edu/ontology"/>
    <skos:example>Schwetye Luchini Architects is in a joint venture with ACME Architects</skos:example>
    <dc:identifier>1414</dc:identifier>
    <skos:prefLabel>ulan1414_joint_venture_with</skos:prefLabel>
    <dct:description>firm/group - joint venture with - firm/group.&#13;
Example: Schwetye Luchini Architects is in a joint venture with ACME Architects</dct:description>
    <rdfs:isDefinedBy rdf:resource="http://vocab.getty.edu/ulan/"/>
    <rdfs:domain rdf:resource="http://www.w3.org/2004/02/skos/core#Concept"/>
    <rdfs:range rdf:resource="http://www.w3.org/2004/02/skos/core#Concept"/>
    <rdfs:subPropertyOf rdf:resource="http://www.w3.org/2004/02/skos/core#related"/>
    <skos:scopeNote>firm/group - joint venture with - firm/group.&#13;
Example: Schwetye Luchini Architects is in a joint venture with ACME Architects</skos:scopeNote>
    <rdf:type rdf:resource="http://www.w3.org/2002/07/owl#SymmetricProperty"/>
    <dc:title>joint venture with - firm/group</dc:title>
  </rdf:Description>
  <rdf:Description rdf:about="http://vocab.getty.edu/ontology#biographyNonPreferred">
    <rdfs:isDefinedBy rdf:resource="http://vocab.getty.edu/ontology"/>
    <rdf:type rdf:resource="http://www.w3.org/2002/07/owl#ObjectProperty"/>
    <rdfs:subPropertyOf rdf:resource="http://vocab.getty.edu/ontology#biography"/>
    <rdfs:range rdf:resource="http://vocab.getty.edu/ontology#Biography"/>
    <dct:description>Non-preferred biography of an ULAN agent. Domain is schema:Person/Organization, range is gvp:Biography</dct:description>
    <rdfs:comment>Non-preferred biography of an ULAN agent. Domain is schema:Person/Organization, range is gvp:Biography</rdfs:comment>
    <skos:prefLabel>biographyNonPreferred</skos:prefLabel>
    <rdfs:label>biographyNonPreferred</rdfs:label>
    <skos:scopeNote>Non-preferred biography of an ULAN agent. Domain is schema:Person/Organization, range is gvp:Biography</skos:scopeNote>
    <skos:definition>Non-preferred biography of an ULAN agent. Domain is schema:Person/Organization, range is gvp:Biography</skos:definition>
  </rdf:Description>
  <rdf:Description rdf:about="http://vocab.getty.edu/ontology#aat2884_involved_with">
    <skos:scopeNote>attributes /associated concepts - [are] involved with - any.&#13;
Example: climate is involved with climate change; insect damage is involved with infestation; Celtic crosses (design motif) are involved with Celtic culture</skos:scopeNote>
    <rdfs:subPropertyOf rdf:resource="http://www.w3.org/2004/02/skos/core#related"/>
    <rdfs:range rdf:resource="http://www.w3.org/2004/02/skos/core#Concept"/>
    <rdfs:domain rdf:resource="http://www.w3.org/2004/02/skos/core#Concept"/>
    <skos:example>Celtic crosses (design motif) are involved with Celtic culture</skos:example>
    <rdf:type rdf:resource="http://www.w3.org/2002/07/owl#ObjectProperty"/>
    <rdfs:isDefinedBy rdf:resource="http://vocab.getty.edu/ontology"/>
    <rdfs:isDefinedBy rdf:resource="http://vocab.getty.edu/aat/"/>
    <skos:example>insect damage is involved with infestation</skos:example>
    <dc:identifier>2884</dc:identifier>
    <dc:title>involved with - any</dc:title>
    <skos:prefLabel>aat2884_involved_with</skos:prefLabel>
    <dct:description>attributes /associated concepts - [are] involved with - any.&#13;
Example: climate is involved with climate change; insect damage is involved with infestation; Celtic crosses (design motif) are involved with Celtic culture</dct:description>
    <owl:inverseOf rdf:resource="http://vocab.getty.edu/ontology#aat2885_involves"/>
    <skos:example>climate is involved with climate change</skos:example>
  </rdf:Description>
  <rdf:Description rdf:about="http://vocab.getty.edu/ontology#aat2853_involve">
    <dc:title>involve - genus/species</dc:title>
    <rdf:type rdf:resource="http://www.w3.org/2002/07/owl#ObjectProperty"/>
    <rdfs:range rdf:resource="http://www.w3.org/2004/02/skos/core#Concept"/>
    <skos:scopeNote>things/[equipment] - involve - genus/species.&#13;
Example: rose bowls involve Rosa (genus); camel saddles involve Camelus (genus)</skos:scopeNote>
    <skos:example>camel saddles involve Camelus (genus)</skos:example>
    <rdfs:isDefinedBy rdf:resource="http://vocab.getty.edu/aat/"/>
    <skos:prefLabel>aat2853_involve</skos:prefLabel>
    <rdfs:domain rdf:resource="http://www.w3.org/2004/02/skos/core#Concept"/>
    <dc:identifier>2853</dc:identifier>
    <skos:example>rose bowls involve Rosa (genus)</skos:example>
    <dct:description>things/[equipment] - involve - genus/species.&#13;
Example: rose bowls involve Rosa (genus); camel saddles involve Camelus (genus)</dct:description>
    <rdfs:subPropertyOf rdf:resource="http://www.w3.org/2004/02/skos/core#related"/>
    <rdfs:isDefinedBy rdf:resource="http://vocab.getty.edu/ontology"/>
  </rdf:Description>
  <rdf:Description rdf:about="http://vocab.getty.edu/ontology#isNoted">
    <rdf:type rdf:resource="http://www.w3.org/2002/07/owl#DatatypeProperty"/>
    <rdfs:range rdf:resource="http://www.w3.org/2001/XMLSchema#boolean"/>
    <skos:scopeNote>One amongst several homographic concepts may be especially noted so it's easier to find.
Example: tgn:7008038 Paris, France is noted but tgn:2106600 Paris, Texas is not (except if you're Fassbinder)</skos:scopeNote>
    <rdfs:isDefinedBy rdf:resource="http://vocab.getty.edu/ontology"/>
    <rdfs:label>isNoted</rdfs:label>
    <rdfs:comment>One amongst several homographic concepts may be especially noted so it's easier to find</rdfs:comment>
    <skos:example>tgn:7008038 Paris, France is noted but tgn:2106600 Paris, Texas is not (except if you're Fassbinder)</skos:example>
    <skos:definition>One amongst several homographic concepts may be especially noted so it's easier to find</skos:definition>
    <rdfs:domain rdf:resource="http://vocab.getty.edu/ontology#Subject"/>
    <skos:prefLabel>isNoted</skos:prefLabel>
    <dct:description>One amongst several homographic concepts may be especially noted so it's easier to find.
Example: tgn:7008038 Paris, France is noted but tgn:2106600 Paris, Texas is not (except if you're Fassbinder)</dct:description>
  </rdf:Description>
  <rdf:Description rdf:about="http://vocab.getty.edu/ontology#ulan2581_administrator_of">
    <dc:identifier>2581</dc:identifier>
    <rdfs:isDefinedBy rdf:resource="http://vocab.getty.edu/ulan/"/>
    <rdf:type rdf:resource="http://www.w3.org/2002/07/owl#ObjectProperty"/>
    <rdfs:isDefinedBy rdf:resource="http://vocab.getty.edu/ontology"/>
    <skos:prefLabel>ulan2581_administrator_of</skos:prefLabel>
    <dc:title>administrator of - institution</dc:title>
    <skos:scopeNote>person - administrator of - institution.&#13;
Example: Georges Mathieu was the administrator of Societe nationale des chemins de fer Francais. Agence des gares</skos:scopeNote>
    <owl:inverseOf rdf:resource="http://vocab.getty.edu/ontology#ulan2582_administered_by"/>
    <skos:example>Georges Mathieu was the administrator of Societe nationale des chemins de fer Francais. Agence des gares</skos:example>
    <dct:description>person - administrator of - institution.&#13;
Example: Georges Mathieu was the administrator of Societe nationale des chemins de fer Francais. Agence des gares</dct:description>
    <rdfs:range rdf:resource="http://www.w3.org/2004/02/skos/core#Concept"/>
    <rdfs:domain rdf:resource="http://www.w3.org/2004/02/skos/core#Concept"/>
    <rdfs:subPropertyOf rdf:resource="http://www.w3.org/2004/02/skos/core#related"/>
  </rdf:Description>
  <rdf:Description rdf:about="http://vocab.getty.edu/ontology#placeTypePreferred">
    <skos:scopeNote>The primary type of a TGN Place. Domain is TGN concept, range is AAT concept.
Example: The preferred place type of Machupicchu, Peru is "deserted settlement" (current)</skos:scopeNote>
    <skos:example>The preferred place type of Machupicchu, Peru is "deserted settlement" (current)</skos:example>
    <rdfs:domain rdf:resource="http://vocab.getty.edu/ontology#Subject"/>
    <rdfs:range rdf:resource="http://vocab.getty.edu/ontology#Subject"/>
    <dct:description>The primary type of a TGN Place. Domain is TGN concept, range is AAT concept.
Example: The preferred place type of Machupicchu, Peru is "deserted settlement" (current)</dct:description>
    <rdfs:comment>The primary type of a TGN Place. Domain is TGN concept, range is AAT concept</rdfs:comment>
    <rdfs:label>placeTypePreferred</rdfs:label>
    <rdfs:isDefinedBy rdf:resource="http://vocab.getty.edu/ontology"/>
    <skos:prefLabel>placeTypePreferred</skos:prefLabel>
    <skos:definition>The primary type of a TGN Place. Domain is TGN concept, range is AAT concept</skos:definition>
    <rdfs:subPropertyOf rdf:resource="http://vocab.getty.edu/ontology#placeType"/>
    <rdf:type rdf:resource="http://www.w3.org/2002/07/owl#ObjectProperty"/>
  </rdf:Description>
  <rdf:Description rdf:about="http://vocab.getty.edu/ontology#ulan1514_gandparent_of">
    <skos:prefLabel>ulan1514_gandparent_of</skos:prefLabel>
    <dc:title>gandparent of - person</dc:title>
    <dct:description>person - gandparent of - person.&#13;
Example: Frank Lloyd Wright is the grandparent of Eric Lloyd Wright</dct:description>
    <rdfs:range rdf:resource="http://www.w3.org/2004/02/skos/core#Concept"/>
    <rdfs:domain rdf:resource="http://www.w3.org/2004/02/skos/core#Concept"/>
    <skos:example>Frank Lloyd Wright is the grandparent of Eric Lloyd Wright</skos:example>
    <rdfs:subPropertyOf rdf:resource="http://www.w3.org/2004/02/skos/core#related"/>
    <rdfs:isDefinedBy rdf:resource="http://vocab.getty.edu/ulan/"/>
    <dc:identifier>1514</dc:identifier>
    <rdf:type rdf:resource="http://www.w3.org/2002/07/owl#ObjectProperty"/>
    <rdfs:isDefinedBy rdf:resource="http://vocab.getty.edu/ontology"/>
    <skos:scopeNote>person - gandparent of - person.&#13;
Example: Frank Lloyd Wright is the grandparent of Eric Lloyd Wright</skos:scopeNote>
  </rdf:Description>
  <rdf:Description rdf:about="http://vocab.getty.edu/ontology#ulan2650_publisher_was">
    <dc:title>publisher was - firm</dc:title>
    <rdfs:subPropertyOf rdf:resource="http://www.w3.org/2004/02/skos/core#related"/>
    <rdfs:isDefinedBy rdf:resource="http://vocab.getty.edu/ulan/"/>
    <dct:description>person - publisher was - firm.&#13;
Example: The publisher for Pierre Joseph Rossier was Negretti and Zambra</dct:description>
    <rdf:type rdf:resource="http://www.w3.org/2002/07/owl#ObjectProperty"/>
    <skos:example>The publisher for Pierre Joseph Rossier was Negretti and Zambra</skos:example>
    <rdfs:isDefinedBy rdf:resource="http://vocab.getty.edu/ontology"/>
    <owl:inverseOf rdf:resource="http://vocab.getty.edu/ontology#ulan2651_publisher_of"/>
    <skos:scopeNote>person - publisher was - firm.&#13;
Example: The publisher for Pierre Joseph Rossier was Negretti and Zambra</skos:scopeNote>
    <rdfs:range rdf:resource="http://www.w3.org/2004/02/skos/core#Concept"/>
    <rdfs:domain rdf:resource="http://www.w3.org/2004/02/skos/core#Concept"/>
    <dc:identifier>2650</dc:identifier>
    <skos:prefLabel>ulan2650_publisher_was</skos:prefLabel>
  </rdf:Description>
  <rdf:Description rdf:about="http://vocab.getty.edu/ontology#ulan2841_performer_was">
    <rdfs:isDefinedBy rdf:resource="http://vocab.getty.edu/ulan/"/>
    <skos:scopeNote>group - performer was - person</skos:scopeNote>
    <skos:prefLabel>ulan2841_performer_was</skos:prefLabel>
    <dct:description>group - performer was - person</dct:description>
    <rdfs:subPropertyOf rdf:resource="http://www.w3.org/2004/02/skos/core#related"/>
    <rdfs:range rdf:resource="http://www.w3.org/2004/02/skos/core#Concept"/>
    <rdfs:domain rdf:resource="http://www.w3.org/2004/02/skos/core#Concept"/>
    <rdfs:isDefinedBy rdf:resource="http://vocab.getty.edu/ontology"/>
    <rdf:type rdf:resource="http://www.w3.org/2002/07/owl#ObjectProperty"/>
    <dc:identifier>2841</dc:identifier>
    <dc:title>performer was - person</dc:title>
  </rdf:Description>
  <rdf:Description rdf:about="http://vocab.getty.edu/ontology#aat2431_required_for">
    <skos:prefLabel>aat2431_required_for</skos:prefLabel>
    <rdfs:isDefinedBy rdf:resource="http://vocab.getty.edu/ontology"/>
    <skos:scopeNote>things/equipment - [are] required for - activity/event/process.&#13;
Example: painting equipment is required for painting (image making); dowels are required for doweling</skos:scopeNote>
    <rdfs:range rdf:resource="http://www.w3.org/2004/02/skos/core#Concept"/>
    <dc:title>required for - activity/event/process</dc:title>
    <dct:description>things/equipment - [are] required for - activity/event/process.&#13;
Example: painting equipment is required for painting (image making); dowels are required for doweling</dct:description>
    <rdfs:subPropertyOf rdf:resource="http://www.w3.org/2004/02/skos/core#related"/>
    <rdfs:domain rdf:resource="http://www.w3.org/2004/02/skos/core#Concept"/>
    <skos:example>painting equipment is required for painting (image making)</skos:example>
    <dc:identifier>2431</dc:identifier>
    <rdf:type rdf:resource="http://www.w3.org/2002/07/owl#ObjectProperty"/>
    <owl:inverseOf rdf:resource="http://vocab.getty.edu/ontology#aat2432_requires"/>
    <rdfs:isDefinedBy rdf:resource="http://vocab.getty.edu/aat/"/>
    <skos:example>dowels are required for doweling</skos:example>
  </rdf:Description>
  <rdf:Description rdf:about="http://vocab.getty.edu/ontology#ulan1206_client_was">
    <dc:title>client was - person/firm/family</dc:title>
    <rdf:type rdf:resource="http://www.w3.org/2002/07/owl#ObjectProperty"/>
    <skos:prefLabel>ulan1206_client_was</skos:prefLabel>
    <rdfs:domain rdf:resource="http://www.w3.org/2004/02/skos/core#Concept"/>
    <rdfs:range rdf:resource="http://www.w3.org/2004/02/skos/core#Concept"/>
    <skos:scopeNote>person/firm/family - client was - person/firm/family.&#13;
Example: Burnham and Root's client was the Chicago Herald</skos:scopeNote>
    <rdfs:isDefinedBy rdf:resource="http://vocab.getty.edu/ulan/"/>
    <dc:identifier>1206</dc:identifier>
    <skos:example>Burnham and Root's client was the Chicago Herald</skos:example>
    <rdfs:subPropertyOf rdf:resource="http://www.w3.org/2004/02/skos/core#related"/>
    <rdfs:isDefinedBy rdf:resource="http://vocab.getty.edu/ontology"/>
    <dct:description>person/firm/family - client was - person/firm/family.&#13;
Example: Burnham and Root's client was the Chicago Herald</dct:description>
  </rdf:Description>
  <rdf:Description rdf:about="http://vocab.getty.edu/ontology#ulan1571_guardian_of">
    <dc:identifier>1571</dc:identifier>
    <skos:prefLabel>ulan1571_guardian_of</skos:prefLabel>
    <dct:description>person - guardian of - person.&#13;
Example: John Hoskins, the elder was the guardian of Samuel Cooper</dct:description>
    <rdfs:subPropertyOf rdf:resource="http://www.w3.org/2004/02/skos/core#related"/>
    <rdfs:isDefinedBy rdf:resource="http://vocab.getty.edu/ulan/"/>
    <skos:example>John Hoskins, the elder was the guardian of Samuel Cooper</skos:example>
    <rdfs:range rdf:resource="http://www.w3.org/2004/02/skos/core#Concept"/>
    <rdfs:domain rdf:resource="http://www.w3.org/2004/02/skos/core#Concept"/>
    <owl:inverseOf rdf:resource="http://vocab.getty.edu/ontology#ulan1573_ward_of"/>
    <skos:scopeNote>person - guardian of - person.&#13;
Example: John Hoskins, the elder was the guardian of Samuel Cooper</skos:scopeNote>
    <dc:title>guardian of - person</dc:title>
    <rdf:type rdf:resource="http://www.w3.org/2002/07/owl#ObjectProperty"/>
    <rdfs:isDefinedBy rdf:resource="http://vocab.getty.edu/ontology"/>
  </rdf:Description>
  <rdf:Description rdf:about="http://vocab.getty.edu/ontology#aat2412_involves">
    <dc:title>involves - activity/event</dc:title>
    <rdfs:isDefinedBy rdf:resource="http://vocab.getty.edu/aat/"/>
    <dc:identifier>2412</dc:identifier>
    <skos:scopeNote>field/discipline - involves - activity/event/[process/function].&#13;
Example: photojournalism (discipline) involves journalistic photography; horticulture involves gardening</skos:scopeNote>
    <rdf:type rdf:resource="http://www.w3.org/2002/07/owl#ObjectProperty"/>
    <rdfs:range rdf:resource="http://www.w3.org/2004/02/skos/core#Concept"/>
    <rdfs:isDefinedBy rdf:resource="http://vocab.getty.edu/ontology"/>
    <skos:example>photojournalism (discipline) involves journalistic photography</skos:example>
    <dct:description>field/discipline - involves - activity/event/[process/function].&#13;
Example: photojournalism (discipline) involves journalistic photography; horticulture involves gardening</dct:description>
    <skos:prefLabel>aat2412_involves</skos:prefLabel>
    <rdfs:subPropertyOf rdf:resource="http://www.w3.org/2004/02/skos/core#related"/>
    <skos:example>horticulture involves gardening</skos:example>
    <rdfs:domain rdf:resource="http://www.w3.org/2004/02/skos/core#Concept"/>
  </rdf:Description>
  <rdf:Description rdf:about="http://vocab.getty.edu/ontology#aat2811_preceded">
    <skos:prefLabel>aat2811_preceded</skos:prefLabel>
    <rdf:type rdf:resource="http://www.w3.org/2002/07/owl#ObjectProperty"/>
    <skos:scopeNote>style/period/culture/[religion/ideology] - preceded  - style/period/culture/[religion/ideology].&#13;
Example: Impressionist preceded Abstract Impressionist; Acheulian preceded Micoquian</skos:scopeNote>
    <rdfs:isDefinedBy rdf:resource="http://vocab.getty.edu/aat/"/>
    <dc:identifier>2811</dc:identifier>
    <dc:title>preceded - style/period/culture</dc:title>
    <skos:example>Impressionist preceded Abstract Impressionist</skos:example>
    <rdfs:domain rdf:resource="http://www.w3.org/2004/02/skos/core#Concept"/>
    <owl:inverseOf rdf:resource="http://vocab.getty.edu/ontology#aat2812_followed"/>
    <dct:description>style/period/culture/[religion/ideology] - preceded  - style/period/culture/[religion/ideology].&#13;
Example: Impressionist preceded Abstract Impressionist; Acheulian preceded Micoquian</dct:description>
    <rdfs:isDefinedBy rdf:resource="http://vocab.getty.edu/ontology"/>
    <rdfs:subPropertyOf rdf:resource="http://www.w3.org/2004/02/skos/core#related"/>
    <rdfs:range rdf:resource="http://www.w3.org/2004/02/skos/core#Concept"/>
    <skos:example>Acheulian preceded Micoquian</skos:example>
  </rdf:Description>
  <rdf:Description rdf:about="http://vocab.getty.edu/ontology#ulan2550_friend_of">
    <rdf:type rdf:resource="http://www.w3.org/2002/07/owl#ObjectProperty"/>
    <rdfs:isDefinedBy rdf:resource="http://vocab.getty.edu/ontology"/>
    <rdfs:range rdf:resource="http://www.w3.org/2004/02/skos/core#Concept"/>
    <dc:title>friend of - person</dc:title>
    <rdfs:domain rdf:resource="http://www.w3.org/2004/02/skos/core#Concept"/>
    <skos:prefLabel>ulan2550_friend_of</skos:prefLabel>
    <skos:example>Alfred Stieglitz and Frank Simon Herrmann were friends</skos:example>
    <skos:scopeNote>person - friend of (personal relationship) - person.&#13;
Example: Alfred Stieglitz and Frank Simon Herrmann were friends</skos:scopeNote>
    <dc:identifier>2550</dc:identifier>
    <rdfs:isDefinedBy rdf:resource="http://vocab.getty.edu/ulan/"/>
    <dct:description>person - friend of (personal relationship) - person.&#13;
Example: Alfred Stieglitz and Frank Simon Herrmann were friends</dct:description>
    <rdfs:subPropertyOf rdf:resource="http://www.w3.org/2004/02/skos/core#related"/>
    <rdf:type rdf:resource="http://www.w3.org/2002/07/owl#SymmetricProperty"/>
  </rdf:Description>
  <rdf:Description rdf:about="http://vocab.getty.edu/ontology#aat2110_meaning-usage_overlaps_with">
    <skos:example>scribes has meaning/usage that overlaps with copyists</skos:example>
    <rdfs:subPropertyOf rdf:resource="http://www.w3.org/2004/02/skos/core#related"/>
    <dc:title>meaning/usage overlaps with - any</dc:title>
    <rdf:type rdf:resource="http://www.w3.org/2002/07/owl#ObjectProperty"/>
    <rdf:type rdf:resource="http://www.w3.org/2002/07/owl#SymmetricProperty"/>
    <rdfs:isDefinedBy rdf:resource="http://vocab.getty.edu/ontology"/>
    <dc:identifier>2110</dc:identifier>
    <skos:example>chimney hoods has meaning/usage that overlaps with chimney caps</skos:example>
    <rdfs:isDefinedBy rdf:resource="http://vocab.getty.edu/aat/"/>
    <rdfs:range rdf:resource="http://www.w3.org/2004/02/skos/core#Concept"/>
    <rdfs:domain rdf:resource="http://www.w3.org/2004/02/skos/core#Concept"/>
    <skos:scopeNote>any - meaning/usage overlaps with - any.&#13;
Example: chimney hoods has meaning/usage that overlaps with chimney caps; scribes has meaning/usage that overlaps with copyists</skos:scopeNote>
    <dct:description>any - meaning/usage overlaps with - any.&#13;
Example: chimney hoods has meaning/usage that overlaps with chimney caps; scribes has meaning/usage that overlaps with copyists</dct:description>
    <skos:prefLabel>aat2110_meaning-usage_overlaps_with</skos:prefLabel>
  </rdf:Description>
  <rdf:Description rdf:about="http://vocab.getty.edu/ontology#aat2842_source_for">
    <dc:title>source for - material</dc:title>
    <rdf:type rdf:resource="http://www.w3.org/2002/07/owl#ObjectProperty"/>
    <rdfs:domain rdf:resource="http://www.w3.org/2004/02/skos/core#Concept"/>
    <skos:example>Acer (genus) is the source for maple (wood)</skos:example>
    <rdfs:subPropertyOf rdf:resource="http://www.w3.org/2004/02/skos/core#related"/>
    <dc:identifier>2842</dc:identifier>
    <skos:example>Vicugna pacos (species) is the source for alpaca (wool)</skos:example>
    <skos:prefLabel>aat2842_source_for</skos:prefLabel>
    <skos:scopeNote>genus/species - [is] source for - material.&#13;
Example: Vicugna pacos (species) is the source for alpaca (wool); Acer (genus) is the source for maple (wood)</skos:scopeNote>
    <rdfs:range rdf:resource="http://www.w3.org/2004/02/skos/core#Concept"/>
    <rdfs:isDefinedBy rdf:resource="http://vocab.getty.edu/aat/"/>
    <rdfs:isDefinedBy rdf:resource="http://vocab.getty.edu/ontology"/>
    <dct:description>genus/species - [is] source for - material.&#13;
Example: Vicugna pacos (species) is the source for alpaca (wool); Acer (genus) is the source for maple (wood)</dct:description>
  </rdf:Description>
  <rdf:Description rdf:about="http://vocab.getty.edu/ontology#aat2807_derived_from_common_source">
    <dct:description>material - [is] derived from common source [as] - material.&#13;
Example: malachite (mineral) is derived from common source with azurite (mineral); mustard(material) is derived from common source with mustard oil</dct:description>
    <rdf:type rdf:resource="http://www.w3.org/2002/07/owl#SymmetricProperty"/>
    <skos:example>mustard(material) is derived from common source with mustard oil</skos:example>
    <dc:title>derived from common source - material</dc:title>
    <dc:identifier>2807</dc:identifier>
    <skos:example>malachite (mineral) is derived from common source with azurite (mineral)</skos:example>
    <rdfs:domain rdf:resource="http://www.w3.org/2004/02/skos/core#Concept"/>
    <rdfs:range rdf:resource="http://www.w3.org/2004/02/skos/core#Concept"/>
    <rdfs:subPropertyOf rdf:resource="http://www.w3.org/2004/02/skos/core#related"/>
    <rdf:type rdf:resource="http://www.w3.org/2002/07/owl#ObjectProperty"/>
    <rdfs:isDefinedBy rdf:resource="http://vocab.getty.edu/ontology"/>
    <skos:scopeNote>material - [is] derived from common source [as] - material.&#13;
Example: malachite (mineral) is derived from common source with azurite (mineral); mustard(material) is derived from common source with mustard oil</skos:scopeNote>
    <rdfs:isDefinedBy rdf:resource="http://vocab.getty.edu/aat/"/>
    <skos:prefLabel>aat2807_derived_from_common_source</skos:prefLabel>
  </rdf:Description>
  <rdf:Description rdf:about="http://vocab.getty.edu/ontology#GroupConcept">
    <skos:scopeNote>Two or more people who generally worked together to collectively create art. Not necessarily legally incorporated. A family of artists may be considered a "corporate body". Corresponds to crm:E74_Group, not its subclass crm:E40_Legal_Body.
Example: 500356337 Albrecht Duerer Workshop (ULAN)</skos:scopeNote>
    <rdf:type rdf:resource="http://www.w3.org/2002/07/owl#Class"/>
    <rdfs:subClassOf rdf:resource="http://vocab.getty.edu/ontology#Subject"/>
    <skos:prefLabel>GroupConcept</skos:prefLabel>
    <skos:example>500356337 Albrecht Duerer Workshop (ULAN)</skos:example>
    <skos:definition>Two or more people who generally worked together to collectively create art. Not necessarily legally incorporated. A family of artists may be considered a "corporate body". Corresponds to crm:E74_Group, not its subclass crm:E40_Legal_Body</skos:definition>
    <rdfs:label>GroupConcept</rdfs:label>
    <skos:broader rdf:resource="http://vocab.getty.edu/ontology#Subject"/>
    <rdfs:isDefinedBy rdf:resource="http://vocab.getty.edu/ontology"/>
    <dct:description>Two or more people who generally worked together to collectively create art. Not necessarily legally incorporated. A family of artists may be considered a "corporate body". Corresponds to crm:E74_Group, not its subclass crm:E40_Legal_Body.
Example: 500356337 Albrecht Duerer Workshop (ULAN)</dct:description>
    <rdfs:comment>Two or more people who generally worked together to collectively create art. Not necessarily legally incorporated. A family of artists may be considered a "corporate body". Corresponds to crm:E74_Group, not its subclass crm:E40_Legal_Body</rdfs:comment>
    <rdfs:subClassOf rdf:resource="http://www.w3.org/2004/02/skos/core#Concept"/>
  </rdf:Description>
  <rdf:Description rdf:about="http://vocab.getty.edu/ontology#prefLabelLoC">
    <rdf:type rdf:resource="http://www.w3.org/2002/07/owl#ObjectProperty"/>
    <rdfs:isDefinedBy rdf:resource="http://vocab.getty.edu/ontology"/>
    <dct:description>Term preferred by Library of Congress, thus used for cataloging according to AACR2. Applicable to AAT and ULAN. Used with skosxl:prefLabel</dct:description>
    <skos:definition>Term preferred by Library of Congress, thus used for cataloging according to AACR2. Applicable to AAT and ULAN. Used with skosxl:prefLabel</skos:definition>
    <rdfs:range rdf:resource="http://www.w3.org/2008/05/skos-xl#Label"/>
    <rdfs:domain rdf:resource="http://vocab.getty.edu/ontology#Subject"/>
    <skos:scopeNote>Term preferred by Library of Congress, thus used for cataloging according to AACR2. Applicable to AAT and ULAN. Used with skosxl:prefLabel</skos:scopeNote>
    <rdfs:label>prefLabelLoC</rdfs:label>
    <rdfs:comment>Term preferred by Library of Congress, thus used for cataloging according to AACR2. Applicable to AAT and ULAN. Used with skosxl:prefLabel</rdfs:comment>
    <skos:prefLabel>prefLabelLoC</skos:prefLabel>
  </rdf:Description>
  <rdf:Description rdf:about="http://vocab.getty.edu/ontology#ulan1204_donor_was">
    <dc:identifier>1204</dc:identifier>
    <rdfs:isDefinedBy rdf:resource="http://vocab.getty.edu/ontology"/>
    <skos:scopeNote>person/firm/family - donor was - person/firm/family.&#13;
Example: Donor to the National Gallery of Art was Andrew W. Mellon</skos:scopeNote>
    <rdf:type rdf:resource="http://www.w3.org/2002/07/owl#ObjectProperty"/>
    <rdfs:isDefinedBy rdf:resource="http://vocab.getty.edu/ulan/"/>
    <rdfs:domain rdf:resource="http://www.w3.org/2004/02/skos/core#Concept"/>
    <rdfs:subPropertyOf rdf:resource="http://www.w3.org/2004/02/skos/core#related"/>
    <skos:prefLabel>ulan1204_donor_was</skos:prefLabel>
    <rdfs:range rdf:resource="http://www.w3.org/2004/02/skos/core#Concept"/>
    <dct:description>person/firm/family - donor was - person/firm/family.&#13;
Example: Donor to the National Gallery of Art was Andrew W. Mellon</dct:description>
    <dc:title>donor was - person/firm/family</dc:title>
    <skos:example>Donor to the National Gallery of Art was Andrew W. Mellon</skos:example>
  </rdf:Description>
  <rdf:Description rdf:about="http://vocab.getty.edu/ontology#aat2319_involves">
    <skos:scopeNote>activity/event - involves - [actors having] role.&#13;
Example: weddings involve bridegrooms; martyrdoms involve martyrs</skos:scopeNote>
    <rdfs:subPropertyOf rdf:resource="http://www.w3.org/2004/02/skos/core#related"/>
    <rdfs:domain rdf:resource="http://www.w3.org/2004/02/skos/core#Concept"/>
    <rdfs:range rdf:resource="http://www.w3.org/2004/02/skos/core#Concept"/>
    <skos:prefLabel>aat2319_involves</skos:prefLabel>
    <rdf:type rdf:resource="http://www.w3.org/2002/07/owl#ObjectProperty"/>
    <rdfs:isDefinedBy rdf:resource="http://vocab.getty.edu/ontology"/>
    <skos:example>weddings involve bridegrooms</skos:example>
    <dc:title>involves - role</dc:title>
    <rdfs:isDefinedBy rdf:resource="http://vocab.getty.edu/aat/"/>
    <skos:example>martyrdoms involve martyrs</skos:example>
    <dct:description>activity/event - involves - [actors having] role.&#13;
Example: weddings involve bridegrooms; martyrdoms involve martyrs</dct:description>
    <dc:identifier>2319</dc:identifier>
  </rdf:Description>
  <rdf:Description rdf:about="http://vocab.getty.edu/ontology#ulan1561_step-child_of">
    <rdfs:isDefinedBy rdf:resource="http://vocab.getty.edu/ulan/"/>
    <rdf:type rdf:resource="http://www.w3.org/2002/07/owl#ObjectProperty"/>
    <owl:inverseOf rdf:resource="http://vocab.getty.edu/ontology#ulan1562_step-parent_of"/>
    <rdfs:isDefinedBy rdf:resource="http://vocab.getty.edu/ontology"/>
    <skos:scopeNote>person - step-child of - person.&#13;
Example: Hortense, Quene consort of Louis Bonaparte is the step-child of Napoleon I, Emperor of the French</skos:scopeNote>
    <skos:example>Hortense, Quene consort of Louis Bonaparte is the step-child of Napoleon I, Emperor of the French</skos:example>
    <skos:prefLabel>ulan1561_step-child_of</skos:prefLabel>
    <dct:description>person - step-child of - person.&#13;
Example: Hortense, Quene consort of Louis Bonaparte is the step-child of Napoleon I, Emperor of the French</dct:description>
    <dc:title>step-child of - person</dc:title>
    <dc:identifier>1561</dc:identifier>
    <rdfs:range rdf:resource="http://www.w3.org/2004/02/skos/core#Concept"/>
    <rdfs:domain rdf:resource="http://www.w3.org/2004/02/skos/core#Concept"/>
    <rdfs:subPropertyOf rdf:resource="http://www.w3.org/2004/02/skos/core#related"/>
  </rdf:Description>
  <rdf:Description rdf:about="http://vocab.getty.edu/ontology#contributorPreferred">
    <rdfs:comment>Contributor for which the term is Preferred. Range is foaf:Agent</rdfs:comment>
    <rdfs:subPropertyOf rdf:resource="http://purl.org/dc/terms/contributor"/>
    <skos:example>"organza" is preferred term for WHS</skos:example>
    <dct:description>Contributor for which the term is Preferred. Range is foaf:Agent.
Example: "organza" is preferred term for WHS</dct:description>
    <rdfs:label>contributorPreferred</rdfs:label>
    <rdf:type rdf:resource="http://www.w3.org/2002/07/owl#ObjectProperty"/>
    <rdfs:isDefinedBy rdf:resource="http://vocab.getty.edu/ontology"/>
    <skos:scopeNote>Contributor for which the term is Preferred. Range is foaf:Agent.
Example: "organza" is preferred term for WHS</skos:scopeNote>
    <skos:prefLabel>contributorPreferred</skos:prefLabel>
    <rdfs:domain rdf:resource="http://www.w3.org/2008/05/skos-xl#Label"/>
    <skos:definition>Contributor for which the term is Preferred. Range is foaf:Agent</skos:definition>
    <rdfs:range rdf:resource="http://xmlns.com/foaf/0.1/Agent"/>
  </rdf:Description>
  <rdf:Description rdf:about="http://vocab.getty.edu/ontology#ulan1303_collaborated_with">
    <skos:scopeNote>person - collaborated with - person.&#13;
Example: Pablo Picasso collaborated with Georges Braque</skos:scopeNote>
    <rdf:type rdf:resource="http://www.w3.org/2002/07/owl#ObjectProperty"/>
    <skos:example>Pablo Picasso collaborated with Georges Braque</skos:example>
    <rdfs:isDefinedBy rdf:resource="http://vocab.getty.edu/ontology"/>
    <rdfs:isDefinedBy rdf:resource="http://vocab.getty.edu/ulan/"/>
    <rdfs:domain rdf:resource="http://www.w3.org/2004/02/skos/core#Concept"/>
    <dct:description>person - collaborated with - person.&#13;
Example: Pablo Picasso collaborated with Georges Braque</dct:description>
    <skos:prefLabel>ulan1303_collaborated_with</skos:prefLabel>
    <rdfs:range rdf:resource="http://www.w3.org/2004/02/skos/core#Concept"/>
    <dc:title>collaborated with - person</dc:title>
    <rdfs:subPropertyOf rdf:resource="http://www.w3.org/2004/02/skos/core#related"/>
    <rdf:type rdf:resource="http://www.w3.org/2002/07/owl#SymmetricProperty"/>
    <dc:identifier>1303</dc:identifier>
  </rdf:Description>
  <rdf:Description rdf:about="http://vocab.getty.edu/ontology#aat2416_requires">
    <skos:example>dying requires dye</skos:example>
    <rdf:type rdf:resource="http://www.w3.org/2002/07/owl#ObjectProperty"/>
    <dc:title>requires - material</dc:title>
    <rdfs:isDefinedBy rdf:resource="http://vocab.getty.edu/ontology"/>
    <rdfs:isDefinedBy rdf:resource="http://vocab.getty.edu/aat/"/>
    <dct:description>activity/event/[process/function] - requires - material.&#13;
Example: dying requires dye; pewtersmithing requires pewter</dct:description>
    <rdfs:range rdf:resource="http://www.w3.org/2004/02/skos/core#Concept"/>
    <rdfs:domain rdf:resource="http://www.w3.org/2004/02/skos/core#Concept"/>
    <dc:identifier>2416</dc:identifier>
    <rdfs:subPropertyOf rdf:resource="http://www.w3.org/2004/02/skos/core#related"/>
    <skos:scopeNote>activity/event/[process/function] - requires - material.&#13;
Example: dying requires dye; pewtersmithing requires pewter</skos:scopeNote>
    <skos:prefLabel>aat2416_requires</skos:prefLabel>
    <skos:example>pewtersmithing requires pewter</skos:example>
  </rdf:Description>
  <rdf:Description rdf:about="http://vocab.getty.edu/ontology#aat2292_work-live_in">
    <skos:example>nuns live/work in convents (nunneries)</skos:example>
    <skos:scopeNote>[actor or institution having] role - work/live/[exist] in - locus/setting.&#13;
Example: rope-makers live/work in roperies; nuns live/work in convents (nunneries); libraries (institutions) live/work in libraries (buildings)</skos:scopeNote>
    <skos:example>libraries (institutions) live/work in libraries (buildings)</skos:example>
    <rdfs:isDefinedBy rdf:resource="http://vocab.getty.edu/aat/"/>
    <skos:prefLabel>aat2292_work-live_in</skos:prefLabel>
    <dct:description>[actor or institution having] role - work/live/[exist] in - locus/setting.&#13;
Example: rope-makers live/work in roperies; nuns live/work in convents (nunneries); libraries (institutions) live/work in libraries (buildings)</dct:description>
    <rdfs:domain rdf:resource="http://www.w3.org/2004/02/skos/core#Concept"/>
    <rdf:type rdf:resource="http://www.w3.org/2002/07/owl#ObjectProperty"/>
    <dc:title>work/live in - locus/setting</dc:title>
    <rdfs:isDefinedBy rdf:resource="http://vocab.getty.edu/ontology"/>
    <skos:example>rope-makers live/work in roperies</skos:example>
    <dc:identifier>2292</dc:identifier>
    <rdfs:range rdf:resource="http://www.w3.org/2004/02/skos/core#Concept"/>
    <rdfs:subPropertyOf rdf:resource="http://www.w3.org/2004/02/skos/core#related"/>
  </rdf:Description>
  <rdf:Description rdf:about="http://vocab.getty.edu/ontology#placeType">
    <rdf:type rdf:resource="http://www.w3.org/2002/07/owl#ObjectProperty"/>
    <skos:prefLabel>placeType</skos:prefLabel>
    <dct:description>Type for a TGN place. Domain is TGN concept (AdminPlaceConcept or PhysPlaceConcept), range is AAT Concept.
Example: Machupicchu, Peru has preferred type "deserted settlement" (current) and non-preferred type "Inca center" (historic)</dct:description>
    <skos:scopeNote>Type for a TGN place. Domain is TGN concept (AdminPlaceConcept or PhysPlaceConcept), range is AAT Concept.
Example: Machupicchu, Peru has preferred type "deserted settlement" (current) and non-preferred type "Inca center" (historic)</skos:scopeNote>
    <rdfs:domain rdf:resource="http://vocab.getty.edu/ontology#Subject"/>
    <rdfs:range rdf:resource="http://vocab.getty.edu/ontology#Subject"/>
    <skos:definition>Type for a TGN place. Domain is TGN concept (AdminPlaceConcept or PhysPlaceConcept), range is AAT Concept</skos:definition>
    <rdfs:comment>Type for a TGN place. Domain is TGN concept (AdminPlaceConcept or PhysPlaceConcept), range is AAT Concept</rdfs:comment>
    <rdfs:label>placeType</rdfs:label>
    <rdfs:isDefinedBy rdf:resource="http://vocab.getty.edu/ontology"/>
    <skos:example>Machupicchu, Peru has preferred type "deserted settlement" (current) and non-preferred type "Inca center" (historic)</skos:example>
  </rdf:Description>
  <rdf:Description rdf:about="http://vocab.getty.edu/ontology#ulan1331_worked_with">
    <owl:inverseOf rdf:resource="http://vocab.getty.edu/ontology#ulan1332_worker_was"/>
    <rdfs:isDefinedBy rdf:resource="http://vocab.getty.edu/ontology"/>
    <skos:example>Scarsellino and Domenichino worked with the Carracci family</skos:example>
    <rdfs:range rdf:resource="http://www.w3.org/2004/02/skos/core#Concept"/>
    <rdfs:domain rdf:resource="http://www.w3.org/2004/02/skos/core#Concept"/>
    <skos:scopeNote>any - worked with - person.&#13;
Example: Scarsellino and Domenichino worked with the Carracci family</skos:scopeNote>
    <dc:title>worked with - person</dc:title>
    <dc:identifier>1331</dc:identifier>
    <skos:prefLabel>ulan1331_worked_with</skos:prefLabel>
    <dct:description>any - worked with - person.&#13;
Example: Scarsellino and Domenichino worked with the Carracci family</dct:description>
    <rdfs:subPropertyOf rdf:resource="http://www.w3.org/2004/02/skos/core#related"/>
    <rdfs:isDefinedBy rdf:resource="http://vocab.getty.edu/ulan/"/>
    <rdf:type rdf:resource="http://www.w3.org/2002/07/owl#ObjectProperty"/>
  </rdf:Description>
  <rdf:Description rdf:about="http://vocab.getty.edu/ontology#ulan2575_directed_by">
    <rdfs:isDefinedBy rdf:resource="http://vocab.getty.edu/ulan/"/>
    <dc:title>directed by - person</dc:title>
    <rdf:type rdf:resource="http://www.w3.org/2002/07/owl#ObjectProperty"/>
    <rdfs:isDefinedBy rdf:resource="http://vocab.getty.edu/ontology"/>
    <skos:example>Gobelins Tapestry Manufactory was directed by Jean Jans I</skos:example>
    <rdfs:domain rdf:resource="http://www.w3.org/2004/02/skos/core#Concept"/>
    <skos:scopeNote>institution - directed by - person.&#13;
Example: Gobelins Tapestry Manufactory was directed by Jean Jans I</skos:scopeNote>
    <dct:description>institution - directed by - person.&#13;
Example: Gobelins Tapestry Manufactory was directed by Jean Jans I</dct:description>
    <dc:identifier>2575</dc:identifier>
    <rdfs:range rdf:resource="http://www.w3.org/2004/02/skos/core#Concept"/>
    <skos:prefLabel>ulan2575_directed_by</skos:prefLabel>
    <rdfs:subPropertyOf rdf:resource="http://www.w3.org/2004/02/skos/core#related"/>
  </rdf:Description>
  <rdf:Description rdf:about="http://vocab.getty.edu/ontology#aat2421_locus-setting_for">
    <owl:inverseOf rdf:resource="http://vocab.getty.edu/ontology#aat2422_takes_place_in"/>
    <dct:description>locus/setting - [is] locus/setting for - activity/event/[process/function].&#13;
Example: smelters (metalworking plants) are the locus/setting for smelting; pilgrimage centers are the locus/setting for pilgrimages</dct:description>
    <rdfs:range rdf:resource="http://www.w3.org/2004/02/skos/core#Concept"/>
    <rdfs:subPropertyOf rdf:resource="http://www.w3.org/2004/02/skos/core#related"/>
    <rdfs:domain rdf:resource="http://www.w3.org/2004/02/skos/core#Concept"/>
    <skos:prefLabel>aat2421_locus-setting_for</skos:prefLabel>
    <rdf:type rdf:resource="http://www.w3.org/2002/07/owl#ObjectProperty"/>
    <skos:scopeNote>locus/setting - [is] locus/setting for - activity/event/[process/function].&#13;
Example: smelters (metalworking plants) are the locus/setting for smelting; pilgrimage centers are the locus/setting for pilgrimages</skos:scopeNote>
    <rdfs:isDefinedBy rdf:resource="http://vocab.getty.edu/ontology"/>
    <rdfs:isDefinedBy rdf:resource="http://vocab.getty.edu/aat/"/>
    <dc:identifier>2421</dc:identifier>
    <skos:example>pilgrimage centers are the locus/setting for pilgrimages</skos:example>
    <dc:title>locus/setting for - activity/event</dc:title>
    <skos:example>smelters (metalworking plants) are the locus/setting for smelting</skos:example>
  </rdf:Description>
  <rdf:Description rdf:about="http://vocab.getty.edu/ontology#broaderNonPreferred">
    <dct:description>Auxiliary parents of a subject. Very often there are several non-preferred parents (poly-hierarchy). Can use to mark such parents with [N] in displays .
Example: Non-preferred: "baking dishes" BTG "dishes (vessels)" (AAT)</dct:description>
    <rdf:type rdf:resource="http://www.w3.org/2002/07/owl#ObjectProperty"/>
    <skos:example>Non-preferred: "baking dishes" BTG "dishes (vessels)" (AAT)</skos:example>
    <skos:definition>Auxiliary parents of a subject. Very often there are several non-preferred parents (poly-hierarchy). Can use to mark such parents with [N] in displays </skos:definition>
    <skos:prefLabel>broaderNonPreferred</skos:prefLabel>
    <rdfs:label>broaderNonPreferred</rdfs:label>
    <skos:scopeNote>Auxiliary parents of a subject. Very often there are several non-preferred parents (poly-hierarchy). Can use to mark such parents with [N] in displays .
Example: Non-preferred: "baking dishes" BTG "dishes (vessels)" (AAT)</skos:scopeNote>
    <rdfs:isDefinedBy rdf:resource="http://vocab.getty.edu/ontology"/>
    <rdfs:subPropertyOf rdf:resource="http://vocab.getty.edu/ontology#broader"/>
    <rdfs:range rdf:resource="http://vocab.getty.edu/ontology#Subject"/>
    <rdfs:domain rdf:resource="http://vocab.getty.edu/ontology#Subject"/>
    <rdfs:comment>Auxiliary parents of a subject. Very often there are several non-preferred parents (poly-hierarchy). Can use to mark such parents with [N] in displays </rdfs:comment>
  </rdf:Description>
  <rdf:Description rdf:about="http://vocab.getty.edu/ontology#ulan1008_meaning_-usage_overlaps_with">
    <skos:example>The meaning or usage of unknown Zimbabwean overlaps with unknown Rodesian</skos:example>
    <rdfs:domain rdf:resource="http://www.w3.org/2004/02/skos/core#Concept"/>
    <rdfs:range rdf:resource="http://www.w3.org/2004/02/skos/core#Concept"/>
    <rdfs:isDefinedBy rdf:resource="http://vocab.getty.edu/ulan/"/>
    <dct:description>any - meaning /usage overlaps with - any.&#13;
Example: The meaning or usage of unknown Zimbabwean overlaps with unknown Rodesian</dct:description>
    <rdfs:subPropertyOf rdf:resource="http://www.w3.org/2004/02/skos/core#related"/>
    <dc:title>meaning /usage overlaps with - any</dc:title>
    <rdf:type rdf:resource="http://www.w3.org/2002/07/owl#SymmetricProperty"/>
    <skos:scopeNote>any - meaning /usage overlaps with - any.&#13;
Example: The meaning or usage of unknown Zimbabwean overlaps with unknown Rodesian</skos:scopeNote>
    <rdf:type rdf:resource="http://www.w3.org/2002/07/owl#ObjectProperty"/>
    <rdfs:isDefinedBy rdf:resource="http://vocab.getty.edu/ontology"/>
    <dc:identifier>1008</dc:identifier>
    <skos:prefLabel>ulan1008_meaning_-usage_overlaps_with</skos:prefLabel>
  </rdf:Description>
  <rdf:Description rdf:about="http://vocab.getty.edu/ontology#aat2878_preceded-source_for">
    <dct:description>language - preceded/[is] source for - language.&#13;
Example: Ancient Greek (language) preceded/is source for Greek (modern language); Ancient Egyptian (language) preceded/is source for Egyptian, Coptic (language)</dct:description>
    <dc:title>preceded/source for - language</dc:title>
    <rdfs:range rdf:resource="http://www.w3.org/2004/02/skos/core#Concept"/>
    <rdfs:domain rdf:resource="http://www.w3.org/2004/02/skos/core#Concept"/>
    <rdfs:isDefinedBy rdf:resource="http://vocab.getty.edu/aat/"/>
    <rdf:type rdf:resource="http://www.w3.org/2002/07/owl#ObjectProperty"/>
    <skos:prefLabel>aat2878_preceded-source_for</skos:prefLabel>
    <rdfs:isDefinedBy rdf:resource="http://vocab.getty.edu/ontology"/>
    <owl:inverseOf rdf:resource="http://vocab.getty.edu/ontology#aat2879_followed-developed_from"/>
    <skos:scopeNote>language - preceded/[is] source for - language.&#13;
Example: Ancient Greek (language) preceded/is source for Greek (modern language); Ancient Egyptian (language) preceded/is source for Egyptian, Coptic (language)</skos:scopeNote>
    <dc:identifier>2878</dc:identifier>
    <rdfs:subPropertyOf rdf:resource="http://www.w3.org/2004/02/skos/core#related"/>
    <skos:example>Ancient Egyptian (language) preceded/is source for Egyptian, Coptic (language)</skos:example>
    <skos:example>Ancient Greek (language) preceded/is source for Greek (modern language)</skos:example>
  </rdf:Description>
  <rdf:Description rdf:about="http://vocab.getty.edu/ontology#ulan1550_relative_by_marriage">
    <rdfs:domain rdf:resource="http://www.w3.org/2004/02/skos/core#Concept"/>
    <skos:prefLabel>ulan1550_relative_by_marriage</skos:prefLabel>
    <rdfs:range rdf:resource="http://www.w3.org/2004/02/skos/core#Concept"/>
    <rdfs:subPropertyOf rdf:resource="http://www.w3.org/2004/02/skos/core#related"/>
    <rdfs:isDefinedBy rdf:resource="http://vocab.getty.edu/ontology"/>
    <dct:description>person - relative by marriage (in-law) - person.&#13;
Example: Juana Galarza d Goicoechea and Francisco de Goya are related by marriage</dct:description>
    <rdf:type rdf:resource="http://www.w3.org/2002/07/owl#ObjectProperty"/>
    <dc:identifier>1550</dc:identifier>
    <rdf:type rdf:resource="http://www.w3.org/2002/07/owl#SymmetricProperty"/>
    <dc:title>relative by marriage - person</dc:title>
    <skos:example>Juana Galarza d Goicoechea and Francisco de Goya are related by marriage</skos:example>
    <skos:scopeNote>person - relative by marriage (in-law) - person.&#13;
Example: Juana Galarza d Goicoechea and Francisco de Goya are related by marriage</skos:scopeNote>
    <rdfs:isDefinedBy rdf:resource="http://vocab.getty.edu/ulan/"/>
  </rdf:Description>
  <rdf:Description rdf:about="http://vocab.getty.edu/ontology#ulan2692_president_of">
    <owl:inverseOf rdf:resource="http://vocab.getty.edu/ontology#ulan2693_president_was"/>
    <rdfs:subPropertyOf rdf:resource="http://www.w3.org/2004/02/skos/core#related"/>
    <dc:title>president of - institution</dc:title>
    <dct:description>person - president of - institution.&#13;
Example: David K. E. Bruce was president of National Gallery of Art</dct:description>
    <rdfs:isDefinedBy rdf:resource="http://vocab.getty.edu/ulan/"/>
    <rdfs:range rdf:resource="http://www.w3.org/2004/02/skos/core#Concept"/>
    <rdfs:domain rdf:resource="http://www.w3.org/2004/02/skos/core#Concept"/>
    <dc:identifier>2692</dc:identifier>
    <skos:scopeNote>person - president of - institution.&#13;
Example: David K. E. Bruce was president of National Gallery of Art</skos:scopeNote>
    <skos:prefLabel>ulan2692_president_of</skos:prefLabel>
    <skos:example>David K. E. Bruce was president of National Gallery of Art</skos:example>
    <rdf:type rdf:resource="http://www.w3.org/2002/07/owl#ObjectProperty"/>
    <rdfs:isDefinedBy rdf:resource="http://vocab.getty.edu/ontology"/>
  </rdf:Description>
  <rdf:Description rdf:about="http://vocab.getty.edu/ontology#aat2602_possess-exist_in">
    <skos:prefLabel>aat2602_possess-exist_in</skos:prefLabel>
    <rdfs:domain rdf:resource="http://www.w3.org/2004/02/skos/core#Concept"/>
    <rdfs:range rdf:resource="http://www.w3.org/2004/02/skos/core#Concept"/>
    <dct:description>role [of actors] - possess/exist in - attributes /associated concepts.&#13;
Example: adults possess/exist in adulthood; nomads possess/exist in [state of] nomadism</dct:description>
    <skos:example>adults possess/exist in adulthood</skos:example>
    <rdfs:subPropertyOf rdf:resource="http://www.w3.org/2004/02/skos/core#related"/>
    <dc:title>possess/exist in - attributes /associated concepts</dc:title>
    <skos:scopeNote>role [of actors] - possess/exist in - attributes /associated concepts.&#13;
Example: adults possess/exist in adulthood; nomads possess/exist in [state of] nomadism</skos:scopeNote>
    <rdf:type rdf:resource="http://www.w3.org/2002/07/owl#ObjectProperty"/>
    <rdfs:isDefinedBy rdf:resource="http://vocab.getty.edu/ontology"/>
    <rdfs:isDefinedBy rdf:resource="http://vocab.getty.edu/aat/"/>
    <skos:example>nomads possess/exist in [state of] nomadism</skos:example>
    <dc:identifier>2602</dc:identifier>
  </rdf:Description>
  <rdf:Description rdf:about="http://vocab.getty.edu/ontology#aat2209_used-located_in">
    <skos:prefLabel>aat2209_used-located_in</skos:prefLabel>
    <skos:scopeNote>things -used/located in -  locus/setting.&#13;
Example: glassware is used/located in glassworks (buildings); cave paintings are located in caves</skos:scopeNote>
    <skos:example>glassware is used/located in glassworks (buildings)</skos:example>
    <skos:example>cave paintings are located in caves</skos:example>
    <rdfs:subPropertyOf rdf:resource="http://www.w3.org/2004/02/skos/core#related"/>
    <rdfs:range rdf:resource="http://www.w3.org/2004/02/skos/core#Concept"/>
    <rdfs:domain rdf:resource="http://www.w3.org/2004/02/skos/core#Concept"/>
    <rdfs:isDefinedBy rdf:resource="http://vocab.getty.edu/ontology"/>
    <rdf:type rdf:resource="http://www.w3.org/2002/07/owl#ObjectProperty"/>
    <dct:description>things -used/located in -  locus/setting.&#13;
Example: glassware is used/located in glassworks (buildings); cave paintings are located in caves</dct:description>
    <rdfs:isDefinedBy rdf:resource="http://vocab.getty.edu/aat/"/>
    <dc:title>used/located in - locus/setting</dc:title>
    <dc:identifier>2209</dc:identifier>
  </rdf:Description>
  <rdf:Description rdf:about="http://vocab.getty.edu/ontology#aat2315_used_by">
    <dc:identifier>2315</dc:identifier>
    <skos:prefLabel>aat2315_used_by</skos:prefLabel>
    <skos:example>brass (alloy) is used by braziers (metalworkers)</skos:example>
    <rdf:type rdf:resource="http://www.w3.org/2002/07/owl#ObjectProperty"/>
    <rdfs:isDefinedBy rdf:resource="http://vocab.getty.edu/ontology"/>
    <rdfs:isDefinedBy rdf:resource="http://vocab.getty.edu/aat/"/>
    <skos:scopeNote>material - [is] used by - [actor having] role.&#13;
Example: precious stone is used by lapidiaries; brass (alloy) is used by braziers (metalworkers)</skos:scopeNote>
    <skos:example>precious stone is used by lapidiaries</skos:example>
    <dc:title>used by - role</dc:title>
    <dct:description>material - [is] used by - [actor having] role.&#13;
Example: precious stone is used by lapidiaries; brass (alloy) is used by braziers (metalworkers)</dct:description>
    <rdfs:domain rdf:resource="http://www.w3.org/2004/02/skos/core#Concept"/>
    <owl:inverseOf rdf:resource="http://vocab.getty.edu/ontology#aat2316_use"/>
    <rdfs:range rdf:resource="http://www.w3.org/2004/02/skos/core#Concept"/>
    <rdfs:subPropertyOf rdf:resource="http://www.w3.org/2004/02/skos/core#related"/>
  </rdf:Description>
  <rdf:Description rdf:about="http://vocab.getty.edu/ontology#ulan1542_consort_of">
    <rdfs:subPropertyOf rdf:resource="http://www.w3.org/2004/02/skos/core#related"/>
    <dc:identifier>1542</dc:identifier>
    <skos:prefLabel>ulan1542_consort_of</skos:prefLabel>
    <owl:inverseOf rdf:resource="http://vocab.getty.edu/ontology#ulan1543_consort_was"/>
    <skos:scopeNote>person - consort of - person.&#13;
Example: Empress Livia was the consort of Augustus, Emperor of Rome</skos:scopeNote>
    <dct:description>person - consort of - person.&#13;
Example: Empress Livia was the consort of Augustus, Emperor of Rome</dct:description>
    <rdfs:isDefinedBy rdf:resource="http://vocab.getty.edu/ontology"/>
    <rdfs:domain rdf:resource="http://www.w3.org/2004/02/skos/core#Concept"/>
    <dc:title>consort of - person</dc:title>
    <rdf:type rdf:resource="http://www.w3.org/2002/07/owl#ObjectProperty"/>
    <skos:example>Empress Livia was the consort of Augustus, Emperor of Rome</skos:example>
    <rdfs:isDefinedBy rdf:resource="http://vocab.getty.edu/ulan/"/>
    <rdfs:range rdf:resource="http://www.w3.org/2004/02/skos/core#Concept"/>
  </rdf:Description>
  <rdf:Description rdf:about="http://vocab.getty.edu/ontology#ulan1203_donor_of">
    <rdfs:isDefinedBy rdf:resource="http://vocab.getty.edu/ontology"/>
    <skos:scopeNote>person/firm/family - donor of - person/firm/family.&#13;
Example: Andrew W. Mellon was a donor of National Gallery of Art</skos:scopeNote>
    <rdfs:range rdf:resource="http://www.w3.org/2004/02/skos/core#Concept"/>
    <rdfs:domain rdf:resource="http://www.w3.org/2004/02/skos/core#Concept"/>
    <dc:identifier>1203</dc:identifier>
    <skos:prefLabel>ulan1203_donor_of</skos:prefLabel>
    <dct:description>person/firm/family - donor of - person/firm/family.&#13;
Example: Andrew W. Mellon was a donor of National Gallery of Art</dct:description>
    <dc:title>donor of - person/firm/family</dc:title>
    <rdfs:subPropertyOf rdf:resource="http://www.w3.org/2004/02/skos/core#related"/>
    <rdfs:isDefinedBy rdf:resource="http://vocab.getty.edu/ulan/"/>
    <skos:example>Andrew W. Mellon was a donor of National Gallery of Art</skos:example>
    <rdf:type rdf:resource="http://www.w3.org/2002/07/owl#ObjectProperty"/>
    <owl:inverseOf rdf:resource="http://vocab.getty.edu/ontology#ulan1204_donor_was"/>
  </rdf:Description>
  <rdf:Description rdf:about="http://vocab.getty.edu/ontology#biography">
    <rdfs:label>biography</rdfs:label>
    <skos:definition>Biography of an ULAN agent. Domain is schema:Person/Organization, range is gvp:Biography. The preferred biography fields are also directly available in the Person/Organization</skos:definition>
    <rdfs:comment>Biography of an ULAN agent. Domain is schema:Person/Organization, range is gvp:Biography. The preferred biography fields are also directly available in the Person/Organization</rdfs:comment>
    <rdfs:subPropertyOf rdf:resource="http://vocab.getty.edu/ontology#biography"/>
    <skos:scopeNote>Biography of an ULAN agent. Domain is schema:Person/Organization, range is gvp:Biography. The preferred biography fields are also directly available in the Person/Organization</skos:scopeNote>
    <rdfs:range rdf:resource="http://vocab.getty.edu/ontology#Biography"/>
    <skos:prefLabel>biography</skos:prefLabel>
    <rdf:type rdf:resource="http://www.w3.org/2002/07/owl#ObjectProperty"/>
    <dct:description>Biography of an ULAN agent. Domain is schema:Person/Organization, range is gvp:Biography. The preferred biography fields are also directly available in the Person/Organization</dct:description>
    <rdfs:isDefinedBy rdf:resource="http://vocab.getty.edu/ontology"/>
  </rdf:Description>
  <rdf:Description rdf:about="http://vocab.getty.edu/ontology#ulan1581_descendant_of">
    <dc:identifier>1581</dc:identifier>
    <rdfs:isDefinedBy rdf:resource="http://vocab.getty.edu/ontology"/>
    <dct:description>person - descendant of - person.&#13;
Example: Paolo Caliari is the descendant of Paolo Veronese</dct:description>
    <skos:prefLabel>ulan1581_descendant_of</skos:prefLabel>
    <rdfs:subPropertyOf rdf:resource="http://www.w3.org/2004/02/skos/core#related"/>
    <rdf:type rdf:resource="http://www.w3.org/2002/07/owl#ObjectProperty"/>
    <dc:title>descendant of - person</dc:title>
    <owl:inverseOf rdf:resource="http://vocab.getty.edu/ontology#ulan1582_ancestor_of"/>
    <rdfs:range rdf:resource="http://www.w3.org/2004/02/skos/core#Concept"/>
    <rdfs:domain rdf:resource="http://www.w3.org/2004/02/skos/core#Concept"/>
    <skos:scopeNote>person - descendant of - person.&#13;
Example: Paolo Caliari is the descendant of Paolo Veronese</skos:scopeNote>
    <rdfs:isDefinedBy rdf:resource="http://vocab.getty.edu/ulan/"/>
    <skos:example>Paolo Caliari is the descendant of Paolo Veronese</skos:example>
  </rdf:Description>
  <rdf:Description rdf:about="http://vocab.getty.edu/ontology#aat2605_possess-exist_in">
    <rdfs:domain rdf:resource="http://www.w3.org/2004/02/skos/core#Concept"/>
    <rdfs:range rdf:resource="http://www.w3.org/2004/02/skos/core#Concept"/>
    <rdfs:subPropertyOf rdf:resource="http://www.w3.org/2004/02/skos/core#related"/>
    <rdfs:isDefinedBy rdf:resource="http://vocab.getty.edu/ontology"/>
    <dc:identifier>2605</dc:identifier>
    <skos:prefLabel>aat2605_possess-exist_in</skos:prefLabel>
    <dc:title>possess/exist in - attributes /associated concepts</dc:title>
    <rdf:type rdf:resource="http://www.w3.org/2002/07/owl#ObjectProperty"/>
    <skos:scopeNote>things - possess/exist in - attributes /associated concepts.&#13;
Example: boudoir photographs possess/exist in boudoir (photograph size); ruins possess/exist in ruined [contition]</skos:scopeNote>
    <skos:example>ruins possess/exist in ruined [contition]</skos:example>
    <rdfs:isDefinedBy rdf:resource="http://vocab.getty.edu/aat/"/>
    <skos:example>boudoir photographs possess/exist in boudoir (photograph size)</skos:example>
    <dct:description>things - possess/exist in - attributes /associated concepts.&#13;
Example: boudoir photographs possess/exist in boudoir (photograph size); ruins possess/exist in ruined [contition]</dct:description>
  </rdf:Description>
  <rdf:Description rdf:about="http://vocab.getty.edu/ontology#ulan2828_student_at">
    <skos:scopeNote>person - student at - institution.&#13;
Example: Zdanek Rossman was a student at Bauhaus</skos:scopeNote>
    <rdfs:subPropertyOf rdf:resource="http://www.w3.org/2004/02/skos/core#related"/>
    <rdfs:isDefinedBy rdf:resource="http://vocab.getty.edu/ontology"/>
    <rdf:type rdf:resource="http://www.w3.org/2002/07/owl#ObjectProperty"/>
    <dc:title>student at - institution</dc:title>
    <skos:example>Zdanek Rossman was a student at Bauhaus</skos:example>
    <owl:inverseOf rdf:resource="http://vocab.getty.edu/ontology#ulan2829_student_was"/>
    <dct:description>person - student at - institution.&#13;
Example: Zdanek Rossman was a student at Bauhaus</dct:description>
    <rdfs:domain rdf:resource="http://www.w3.org/2004/02/skos/core#Concept"/>
    <rdfs:range rdf:resource="http://www.w3.org/2004/02/skos/core#Concept"/>
    <dc:identifier>2828</dc:identifier>
    <skos:prefLabel>ulan2828_student_at</skos:prefLabel>
    <rdfs:isDefinedBy rdf:resource="http://vocab.getty.edu/ulan/"/>
  </rdf:Description>
  <rdf:Description rdf:about="http://vocab.getty.edu/ontology#tgn3006_formerly_identified_as">
    <rdfs:domain rdf:resource="http://www.w3.org/2004/02/skos/core#Concept"/>
    <rdfs:range rdf:resource="http://www.w3.org/2004/02/skos/core#Concept"/>
    <dc:title>formerly identified as - place</dc:title>
    <dct:description>place - formerly identified as - place; New.&#13;
Example: The deserted settlement of Machupicchu was formerly identified as Tampu Tocco</dct:description>
    <rdf:type rdf:resource="http://www.w3.org/2002/07/owl#ObjectProperty"/>
    <rdfs:isDefinedBy rdf:resource="http://vocab.getty.edu/ontology"/>
    <rdf:type rdf:resource="http://www.w3.org/2002/07/owl#SymmetricProperty"/>
    <rdfs:subPropertyOf rdf:resource="http://www.w3.org/2004/02/skos/core#related"/>
    <rdfs:isDefinedBy rdf:resource="http://vocab.getty.edu/tgn/"/>
    <skos:scopeNote>New</skos:scopeNote>
    <skos:example>The deserted settlement of Machupicchu was formerly identified as Tampu Tocco</skos:example>
    <dc:identifier>3006</dc:identifier>
    <skos:prefLabel>tgn3006_formerly_identified_as</skos:prefLabel>
  </rdf:Description>
  <rdf:Description rdf:about="http://vocab.getty.edu/ontology#ulan1313_partner_in">
    <rdfs:range rdf:resource="http://www.w3.org/2004/02/skos/core#Concept"/>
    <rdfs:domain rdf:resource="http://www.w3.org/2004/02/skos/core#Concept"/>
    <rdfs:subPropertyOf rdf:resource="http://www.w3.org/2004/02/skos/core#related"/>
    <rdfs:isDefinedBy rdf:resource="http://vocab.getty.edu/ontology"/>
    <dct:description>person - partner in - firm.&#13;
Example: Parners of Adler and Sullivan included Louis H. Sullivan and Dankmar Adler</dct:description>
    <rdf:type rdf:resource="http://www.w3.org/2002/07/owl#ObjectProperty"/>
    <skos:scopeNote>person - partner in - firm.&#13;
Example: Parners of Adler and Sullivan included Louis H. Sullivan and Dankmar Adler</skos:scopeNote>
    <dc:identifier>1313</dc:identifier>
    <dc:title>partner in - firm</dc:title>
    <owl:inverseOf rdf:resource="http://vocab.getty.edu/ontology#ulan1314_partner_was"/>
    <skos:example>Parners of Adler and Sullivan included Louis H. Sullivan and Dankmar Adler</skos:example>
    <skos:prefLabel>ulan1313_partner_in</skos:prefLabel>
    <rdfs:isDefinedBy rdf:resource="http://vocab.getty.edu/ulan/"/>
  </rdf:Description>
  <rdf:Description rdf:about="http://vocab.getty.edu/ontology#GuideTerm">
    <rdfs:label>GuideTerm</rdfs:label>
    <rdfs:comment>Guide Term: place holder to create a level in the hierarchy. Used in AAT and ULAN. Not used for indexing or cataloguing.</rdfs:comment>
    <skos:scopeNote>Guide Term: place holder to create a level in the hierarchy. Used in AAT and ULAN. Not used for indexing or cataloguing..
Example: &lt;vessels for serving and consuming food&gt; (AAT), ulan:500353455 &lt;named animals&gt; under facet Non-Artists (ULAN)</skos:scopeNote>
    <rdf:type rdf:resource="http://www.w3.org/2002/07/owl#Class"/>
    <rdfs:isDefinedBy rdf:resource="http://vocab.getty.edu/ontology"/>
    <rdfs:subClassOf rdf:resource="http://vocab.getty.edu/ontology#Subject"/>
    <skos:definition>Guide Term: place holder to create a level in the hierarchy. Used in AAT and ULAN. Not used for indexing or cataloguing.</skos:definition>
    <rdfs:subClassOf rdf:resource="http://purl.org/iso25964/skos-thes#ThesaurusArray"/>
    <skos:example>&lt;vessels for serving and consuming food&gt; (AAT), ulan:500353455 &lt;named animals&gt; under facet Non-Artists (ULAN)</skos:example>
    <dct:description>Guide Term: place holder to create a level in the hierarchy. Used in AAT and ULAN. Not used for indexing or cataloguing..
Example: &lt;vessels for serving and consuming food&gt; (AAT), ulan:500353455 &lt;named animals&gt; under facet Non-Artists (ULAN)</dct:description>
    <skos:prefLabel>GuideTerm</skos:prefLabel>
    <skos:broader rdf:resource="http://purl.org/iso25964/skos-thes#ThesaurusArray"/>
  </rdf:Description>
  <rdf:Description rdf:about="http://vocab.getty.edu/ontology#aat2203_associated_with">
    <rdf:type rdf:resource="http://www.w3.org/2002/07/owl#SymmetricProperty"/>
    <dct:description>activity/event/[process/function] - [is] associated with - activity/event/[process/function].&#13;
Example: Easter is associated with Lent; cavalry exercises are associated with dressage</dct:description>
    <rdfs:subPropertyOf rdf:resource="http://www.w3.org/2004/02/skos/core#related"/>
    <skos:prefLabel>aat2203_associated_with</skos:prefLabel>
    <skos:scopeNote>activity/event/[process/function] - [is] associated with - activity/event/[process/function].&#13;
Example: Easter is associated with Lent; cavalry exercises are associated with dressage</skos:scopeNote>
    <rdfs:range rdf:resource="http://www.w3.org/2004/02/skos/core#Concept"/>
    <dc:identifier>2203</dc:identifier>
    <rdfs:domain rdf:resource="http://www.w3.org/2004/02/skos/core#Concept"/>
    <rdfs:isDefinedBy rdf:resource="http://vocab.getty.edu/aat/"/>
    <dc:title>associated with - activity/event</dc:title>
    <skos:example>cavalry exercises are associated with dressage</skos:example>
    <rdf:type rdf:resource="http://www.w3.org/2002/07/owl#ObjectProperty"/>
    <skos:example>Easter is associated with Lent</skos:example>
    <rdfs:isDefinedBy rdf:resource="http://vocab.getty.edu/ontology"/>
  </rdf:Description>
  <rdf:Description rdf:about="http://vocab.getty.edu/ontology#term">
    <rdfs:label>term</rdfs:label>
    <rdfs:comment>Term (label), used as the basic (prefix) part of skosxsl:literalForm</rdfs:comment>
    <skos:definition>Term (label), used as the basic (prefix) part of skosxsl:literalForm</skos:definition>
    <rdf:type rdf:resource="http://www.w3.org/2002/07/owl#DatatypeProperty"/>
    <rdfs:range rdf:resource="http://www.w3.org/1999/02/22-rdf-syntax-ns#Literal"/>
    <dct:description>Term (label), used as the basic (prefix) part of skosxsl:literalForm</dct:description>
    <rdfs:isDefinedBy rdf:resource="http://vocab.getty.edu/ontology"/>
    <skos:prefLabel>term</skos:prefLabel>
    <rdfs:domain rdf:resource="http://www.w3.org/2008/05/skos-xl#Label"/>
    <skos:scopeNote>Term (label), used as the basic (prefix) part of skosxsl:literalForm</skos:scopeNote>
  </rdf:Description>
  <rdf:Description rdf:about="http://vocab.getty.edu/ontology#Infer_isoBroaderPartitive">
    <rdf:type rdf:resource="http://www.ontotext.com/proton/protontop#PropRestr"/>
    <ptop:restriction rdf:resource="http://www.w3.org/2004/02/skos/core#broader"/>
    <ptop:conclusion rdf:resource="http://purl.org/iso25964/skos-thes#broaderPartitive"/>
    <ptop:premise rdf:resource="http://vocab.getty.edu/ontology#broaderPartitiveExtended"/>
  </rdf:Description>
  <rdf:Description rdf:about="http://vocab.getty.edu/ontology#aat2818_source_for">
    <skos:example>anhydrite is the source for gypsum</skos:example>
    <rdfs:isDefinedBy rdf:resource="http://vocab.getty.edu/aat/"/>
    <dct:description>material - [is] source for - material.&#13;
Example: anhydrite is the source for gypsum; timber (lumber) is the source for wood board</dct:description>
    <dc:title>source for - material</dc:title>
    <rdfs:isDefinedBy rdf:resource="http://vocab.getty.edu/ontology"/>
    <rdfs:domain rdf:resource="http://www.w3.org/2004/02/skos/core#Concept"/>
    <rdfs:range rdf:resource="http://www.w3.org/2004/02/skos/core#Concept"/>
    <skos:scopeNote>material - [is] source for - material.&#13;
Example: anhydrite is the source for gypsum; timber (lumber) is the source for wood board</skos:scopeNote>
    <rdfs:subPropertyOf rdf:resource="http://www.w3.org/2004/02/skos/core#related"/>
    <rdf:type rdf:resource="http://www.w3.org/2002/07/owl#ObjectProperty"/>
    <skos:example>timber (lumber) is the source for wood board</skos:example>
    <skos:prefLabel>aat2818_source_for</skos:prefLabel>
    <dc:identifier>2818</dc:identifier>
  </rdf:Description>
  <rdf:Description rdf:about="http://vocab.getty.edu/ontology#ulan1421_founded_by">
    <dc:identifier>1421</dc:identifier>
    <rdf:type rdf:resource="http://www.w3.org/2002/07/owl#ObjectProperty"/>
    <skos:scopeNote>firm/group - founded by - firm/group.&#13;
Example: National Gallery of Art was founded by United States Congress</skos:scopeNote>
    <skos:example>National Gallery of Art was founded by United States Congress</skos:example>
    <skos:prefLabel>ulan1421_founded_by</skos:prefLabel>
    <rdfs:domain rdf:resource="http://www.w3.org/2004/02/skos/core#Concept"/>
    <rdfs:range rdf:resource="http://www.w3.org/2004/02/skos/core#Concept"/>
    <owl:inverseOf rdf:resource="http://vocab.getty.edu/ontology#ulan1422_founded"/>
    <dc:title>founded by - firm/group</dc:title>
    <rdfs:isDefinedBy rdf:resource="http://vocab.getty.edu/ulan/"/>
    <dct:description>firm/group - founded by - firm/group.&#13;
Example: National Gallery of Art was founded by United States Congress</dct:description>
    <rdfs:subPropertyOf rdf:resource="http://www.w3.org/2004/02/skos/core#related"/>
    <rdfs:isDefinedBy rdf:resource="http://vocab.getty.edu/ontology"/>
  </rdf:Description>
  <rdf:Description rdf:about="http://vocab.getty.edu/term/kind/CommonName">
    <dct:description>Common Name of an ULAN agent.
Example: TODO</dct:description>
    <skos:inScheme rdf:resource="http://vocab.getty.edu/term/kind/"/>
    <skos:example>TODO</skos:example>
    <rdf:type rdf:resource="http://www.w3.org/2004/02/skos/core#Concept"/>
    <skos:scopeNote>Common Name of an ULAN agent</skos:scopeNote>
    <skos:prefLabel>Common Name</skos:prefLabel>
    <skos:notation>CN</skos:notation>
  </rdf:Description>
  <rdf:Description rdf:about="http://vocab.getty.edu/ontology#aat2311_performed_by">
    <dc:title>performed by - role</dc:title>
    <dct:description>activity/event/[process/function] - [is] performed by - [actors having] a role.&#13;
Example: clockmaking is performed by clockmakers; curating is performed by curators</dct:description>
    <skos:example>curating is performed by curators</skos:example>
    <owl:inverseOf rdf:resource="http://vocab.getty.edu/ontology#aat2312_perform"/>
    <rdfs:isDefinedBy rdf:resource="http://vocab.getty.edu/ontology"/>
    <skos:prefLabel>aat2311_performed_by</skos:prefLabel>
    <rdfs:subPropertyOf rdf:resource="http://www.w3.org/2004/02/skos/core#related"/>
    <rdfs:domain rdf:resource="http://www.w3.org/2004/02/skos/core#Concept"/>
    <rdf:type rdf:resource="http://www.w3.org/2002/07/owl#ObjectProperty"/>
    <rdfs:isDefinedBy rdf:resource="http://vocab.getty.edu/aat/"/>
    <skos:scopeNote>activity/event/[process/function] - [is] performed by - [actors having] a role.&#13;
Example: clockmaking is performed by clockmakers; curating is performed by curators</skos:scopeNote>
    <dc:identifier>2311</dc:identifier>
    <rdfs:range rdf:resource="http://www.w3.org/2004/02/skos/core#Concept"/>
    <skos:example>clockmaking is performed by clockmakers</skos:example>
  </rdf:Description>
  <rdf:Description rdf:about="http://vocab.getty.edu/ontology#ulan2675_professor_was">
    <rdfs:isDefinedBy rdf:resource="http://vocab.getty.edu/ulan/"/>
    <dc:identifier>2675</dc:identifier>
    <skos:scopeNote>institution - professor was - person.&#13;
Example: A professor at Bauhaus was Paul Klee</skos:scopeNote>
    <dct:description>institution - professor was - person.&#13;
Example: A professor at Bauhaus was Paul Klee</dct:description>
    <rdfs:subPropertyOf rdf:resource="http://www.w3.org/2004/02/skos/core#related"/>
    <rdfs:isDefinedBy rdf:resource="http://vocab.getty.edu/ontology"/>
    <rdf:type rdf:resource="http://www.w3.org/2002/07/owl#ObjectProperty"/>
    <dc:title>professor was - person</dc:title>
    <rdfs:domain rdf:resource="http://www.w3.org/2004/02/skos/core#Concept"/>
    <rdfs:range rdf:resource="http://www.w3.org/2004/02/skos/core#Concept"/>
    <skos:example>A professor at Bauhaus was Paul Klee</skos:example>
    <skos:prefLabel>ulan2675_professor_was</skos:prefLabel>
  </rdf:Description>
  <rdf:Description rdf:about="http://vocab.getty.edu/ontology#aat2316_use">
    <dc:identifier>2316</dc:identifier>
    <rdfs:range rdf:resource="http://www.w3.org/2004/02/skos/core#Concept"/>
    <dct:description>[actors having] role - use - material.&#13;
Example: lapidaries use precious stone; braziers (metalworkers) use brass (alloy)</dct:description>
    <dc:title>use - material</dc:title>
    <rdfs:isDefinedBy rdf:resource="http://vocab.getty.edu/aat/"/>
    <skos:example>braziers (metalworkers) use brass (alloy)</skos:example>
    <skos:prefLabel>aat2316_use</skos:prefLabel>
    <rdf:type rdf:resource="http://www.w3.org/2002/07/owl#ObjectProperty"/>
    <skos:scopeNote>[actors having] role - use - material.&#13;
Example: lapidaries use precious stone; braziers (metalworkers) use brass (alloy)</skos:scopeNote>
    <rdfs:isDefinedBy rdf:resource="http://vocab.getty.edu/ontology"/>
    <rdfs:domain rdf:resource="http://www.w3.org/2004/02/skos/core#Concept"/>
    <rdfs:subPropertyOf rdf:resource="http://www.w3.org/2004/02/skos/core#related"/>
    <skos:example>lapidaries use precious stone</skos:example>
  </rdf:Description>
  <rdf:Description rdf:about="http://vocab.getty.edu/ontology">
    <owl:imports rdf:resource="http://www.w3.org/2008/05/skos-xl"/>
    <skos:prefLabel>Getty Vocabulary Program ontology</skos:prefLabel>
    <skos:changeNote rdf:resource="http://vocab.getty.edu/doc#Version_3.3"/>
    <vann:preferredNamespaceUri>http://vocab.getty.edu/ontology#</vann:preferredNamespaceUri>
    <dct:creator rdf:resource="http://www.ontotext.com"/>
    <rdf:type rdf:resource="http://www.w3.org/2002/07/owl#Ontology"/>
    <skos:definition>The GVP Ontology defines classes, properties and values (skos:Concepts) used in GVP LOD.
As of version 3.0, it is complete regarding AAT, TGN and ULAN, and will be extended in time with more elements needed for other GVP vocabularies (CONA).
It uses the SKOS, SKOS-XL, ISO 25964; DC, DCT, BIBO, FOAF, BIO, Schema, PROV, WGS84 ontologies, but we import only the first 3</skos:definition>
    <rdfs:seeAlso rdf:resource="http://vocab.getty.edu/.well-known/void"/>
    <rdfs:seeAlso rdf:resource="http://www.getty.edu/research/tools/vocabularies/lod/"/>
    <rdf:type rdf:resource="http://purl.org/vocommons/voaf#Vocabulary"/>
    <vann:preferredNamespacePrefix>gvp</vann:preferredNamespacePrefix>
    <skos:changeNote rdf:resource="http://vocab.getty.edu/doc#Version_3.0"/>
    <owl:imports rdf:resource="http://www.w3.org/2004/02/skos/core"/>
    <dct:issued rdf:datatype="http://www.w3.org/2001/XMLSchema#date">2014-02-20</dct:issued>
    <owl:imports rdf:resource="http://purl.org/iso25964/skos-thes"/>
    <rdfs:seeAlso rdf:resource="http://vocab.getty.edu/doc"/>
    <rdfs:comment>The GVP Ontology defines classes, properties and values (skos:Concepts) used in GVP LOD.
As of version 3.0, it is complete regarding AAT, TGN and ULAN, and will be extended in time with more elements needed for other GVP vocabularies (CONA).
It uses the SKOS, SKOS-XL, ISO 25964; DC, DCT, BIBO, FOAF, BIO, Schema, PROV, WGS84 ontologies, but we import only the first 3</rdfs:comment>
    <dct:created rdf:datatype="http://www.w3.org/2001/XMLSchema#date">2014-02-15</dct:created>
    <skos:changeNote rdf:resource="http://vocab.getty.edu/doc#Version_2.0"/>
    <dc:format>meta/rdf-schema</dc:format>
    <rdfs:label>Getty Vocabulary Program ontology</rdfs:label>
    <owl:versionInfo>3.3</owl:versionInfo>
    <rdfs:seeAlso rdf:resource="http://lov.okfn.org/dataset/lov/details/vocabulary_gvp.html"/>
    <skos:changeNote>2.0 changes: replaced gvp:broaderTransitive with gvp:broaderExtended.
3.0 changes: replaced schema:startDate, endDate with gvp:estStart, estEnd; added ULAN). See details in referenced links.
3.1 &amp; 3.2: no changes.
3.3: added 6 associative relations: gvp:aat2886_used-function_as - gvp:aat2887_exemplified_by, gvp:tgn3103_located_on - gvp:tgn3104_is_location_of, and gvp:ulan2583_chairman_of - gvp:ulan2584_chaired_by</skos:changeNote>
    <dct:modified rdf:datatype="http://www.w3.org/2001/XMLSchema#date">2016-04-25</dct:modified>
    <dct:creator rdf:resource="http://www.getty.edu/research/"/>
    <rdfs:seeAlso rdf:resource="http://vocab.getty.edu/doc/queries"/>
  </rdf:Description>
  <rdf:Description rdf:about="http://vocab.getty.edu/ontology#ulan1305_worked_with">
    <rdfs:range rdf:resource="http://www.w3.org/2004/02/skos/core#Concept"/>
    <rdfs:domain rdf:resource="http://www.w3.org/2004/02/skos/core#Concept"/>
    <skos:example>William Cleare worked with Christopher Wren</skos:example>
    <rdfs:subPropertyOf rdf:resource="http://www.w3.org/2004/02/skos/core#related"/>
    <rdfs:isDefinedBy rdf:resource="http://vocab.getty.edu/ontology"/>
    <skos:scopeNote>person - worked with - person.&#13;
Example: William Cleare worked with Christopher Wren; Frank Lloyd Wright work with Aaron G. Green</skos:scopeNote>
    <rdf:type rdf:resource="http://www.w3.org/2002/07/owl#ObjectProperty"/>
    <dc:title>worked with - person</dc:title>
    <skos:prefLabel>ulan1305_worked_with</skos:prefLabel>
    <rdf:type rdf:resource="http://www.w3.org/2002/07/owl#SymmetricProperty"/>
    <dct:description>person - worked with - person.&#13;
Example: William Cleare worked with Christopher Wren; Frank Lloyd Wright work with Aaron G. Green</dct:description>
    <dc:identifier>1305</dc:identifier>
    <skos:example>Frank Lloyd Wright work with Aaron G. Green</skos:example>
    <rdfs:isDefinedBy rdf:resource="http://vocab.getty.edu/ulan/"/>
  </rdf:Description>
  <rdf:Description rdf:about="http://vocab.getty.edu/ontology#ulan1555_adopted_child_of">
    <skos:example>Augusts, Emperor of Rome is the adopted child of Julius Caesar</skos:example>
    <skos:prefLabel>ulan1555_adopted_child_of</skos:prefLabel>
    <dct:description>person - adopted child of - person.&#13;
Example: Augusts, Emperor of Rome is the adopted child of Julius Caesar</dct:description>
    <rdfs:isDefinedBy rdf:resource="http://vocab.getty.edu/ulan/"/>
    <rdfs:subPropertyOf rdf:resource="http://www.w3.org/2004/02/skos/core#related"/>
    <rdfs:domain rdf:resource="http://www.w3.org/2004/02/skos/core#Concept"/>
    <rdfs:range rdf:resource="http://www.w3.org/2004/02/skos/core#Concept"/>
    <skos:scopeNote>person - adopted child of - person.&#13;
Example: Augusts, Emperor of Rome is the adopted child of Julius Caesar</skos:scopeNote>
    <dc:identifier>1555</dc:identifier>
    <rdf:type rdf:resource="http://www.w3.org/2002/07/owl#ObjectProperty"/>
    <rdfs:isDefinedBy rdf:resource="http://vocab.getty.edu/ontology"/>
    <dc:title>adopted child of - person</dc:title>
  </rdf:Description>
  <rdf:Description rdf:about="http://vocab.getty.edu/ontology#ulan2573_founded_by">
    <dct:description>institution - founded by - person.&#13;
Example: Tiffany Glass &amp; Decorating Company was founded by Louis Comfort Tiffany</dct:description>
    <skos:example>Tiffany Glass &amp; Decorating Company was founded by Louis Comfort Tiffany</skos:example>
    <rdfs:range rdf:resource="http://www.w3.org/2004/02/skos/core#Concept"/>
    <rdfs:domain rdf:resource="http://www.w3.org/2004/02/skos/core#Concept"/>
    <rdfs:subPropertyOf rdf:resource="http://www.w3.org/2004/02/skos/core#related"/>
    <dc:identifier>2573</dc:identifier>
    <rdfs:isDefinedBy rdf:resource="http://vocab.getty.edu/ulan/"/>
    <skos:scopeNote>institution - founded by - person.&#13;
Example: Tiffany Glass &amp; Decorating Company was founded by Louis Comfort Tiffany</skos:scopeNote>
    <skos:prefLabel>ulan2573_founded_by</skos:prefLabel>
    <rdf:type rdf:resource="http://www.w3.org/2002/07/owl#ObjectProperty"/>
    <rdfs:isDefinedBy rdf:resource="http://vocab.getty.edu/ontology"/>
    <dc:title>founded by - person</dc:title>
  </rdf:Description>
  <rdf:Description rdf:about="http://vocab.getty.edu/ontology#aat2285_practiced-studied_by">
    <skos:prefLabel>aat2285_practiced-studied_by</skos:prefLabel>
    <skos:example>architectural history is practiced/studied by architectural historians</skos:example>
    <dc:title>practiced/studied by - role</dc:title>
    <rdfs:range rdf:resource="http://www.w3.org/2004/02/skos/core#Concept"/>
    <rdfs:isDefinedBy rdf:resource="http://vocab.getty.edu/aat/"/>
    <rdfs:domain rdf:resource="http://www.w3.org/2004/02/skos/core#Concept"/>
    <rdfs:isDefinedBy rdf:resource="http://vocab.getty.edu/ontology"/>
    <skos:example>Egyptology is practiced/studied by Egyptologists</skos:example>
    <skos:scopeNote>field [of study, genre]/discipline - [is] practiced/studied by - a role.&#13;
Example: Egyptology is practiced/studied by Egyptologists; architectural history is practiced/studied by architectural historians</skos:scopeNote>
    <rdf:type rdf:resource="http://www.w3.org/2002/07/owl#ObjectProperty"/>
    <dc:identifier>2285</dc:identifier>
    <rdfs:subPropertyOf rdf:resource="http://www.w3.org/2004/02/skos/core#related"/>
    <owl:inverseOf rdf:resource="http://vocab.getty.edu/ontology#aat2286_practice-study"/>
    <dct:description>field [of study, genre]/discipline - [is] practiced/studied by - a role.&#13;
Example: Egyptology is practiced/studied by Egyptologists; architectural history is practiced/studied by architectural historians</dct:description>
  </rdf:Description>
  <rdf:Description rdf:about="http://vocab.getty.edu/ontology#eventNonPreferred">
    <rdfs:comment>Non-preferred life event of an ULAN agent. Domain is schema:Person/Organization, range is bio:Event</rdfs:comment>
    <rdfs:range rdf:resource="http://purl.org/vocab/bio/0.1/Event"/>
    <skos:prefLabel>eventNonPreferred</skos:prefLabel>
    <skos:scopeNote>Non-preferred life event of an ULAN agent. Domain is schema:Person/Organization, range is bio:Event</skos:scopeNote>
    <rdfs:label>eventNonPreferred</rdfs:label>
    <rdfs:subPropertyOf rdf:resource="http://purl.org/vocab/bio/0.1/event"/>
    <rdfs:isDefinedBy rdf:resource="http://vocab.getty.edu/ontology"/>
    <dct:description>Non-preferred life event of an ULAN agent. Domain is schema:Person/Organization, range is bio:Event</dct:description>
    <rdf:type rdf:resource="http://www.w3.org/2002/07/owl#ObjectProperty"/>
    <skos:definition>Non-preferred life event of an ULAN agent. Domain is schema:Person/Organization, range is bio:Event</skos:definition>
  </rdf:Description>
  <rdf:Description rdf:about="http://vocab.getty.edu/ontology#aat2829_used-required_for">
    <dct:description>material - [is] required/used for - things.&#13;
Example: varnish is used/required for oil paintings; wine is required/used for wine glasses</dct:description>
    <skos:example>varnish is used/required for oil paintings</skos:example>
    <dc:identifier>2829</dc:identifier>
    <rdfs:range rdf:resource="http://www.w3.org/2004/02/skos/core#Concept"/>
    <rdfs:domain rdf:resource="http://www.w3.org/2004/02/skos/core#Concept"/>
    <skos:example>wine is required/used for wine glasses</skos:example>
    <rdfs:subPropertyOf rdf:resource="http://www.w3.org/2004/02/skos/core#related"/>
    <dc:title>used/required for - things</dc:title>
    <skos:prefLabel>aat2829_used-required_for</skos:prefLabel>
    <rdf:type rdf:resource="http://www.w3.org/2002/07/owl#ObjectProperty"/>
    <rdfs:isDefinedBy rdf:resource="http://vocab.getty.edu/ontology"/>
    <rdfs:isDefinedBy rdf:resource="http://vocab.getty.edu/aat/"/>
    <skos:scopeNote>material - [is] required/used for - things.&#13;
Example: varnish is used/required for oil paintings; wine is required/used for wine glasses</skos:scopeNote>
  </rdf:Description>
  <rdf:Description rdf:about="http://vocab.getty.edu/ontology#ulan1501_sibling_of">
    <skos:prefLabel>ulan1501_sibling_of</skos:prefLabel>
    <rdf:type rdf:resource="http://www.w3.org/2002/07/owl#SymmetricProperty"/>
    <rdfs:domain rdf:resource="http://www.w3.org/2004/02/skos/core#Concept"/>
    <rdfs:range rdf:resource="http://www.w3.org/2004/02/skos/core#Concept"/>
    <dct:description>person - sibling of - person.&#13;
Example: Philippe Rubens is the sibling of Peter Paul Rubens</dct:description>
    <rdfs:subPropertyOf rdf:resource="http://www.w3.org/2004/02/skos/core#related"/>
    <rdfs:isDefinedBy rdf:resource="http://vocab.getty.edu/ulan/"/>
    <skos:scopeNote>person - sibling of - person.&#13;
Example: Philippe Rubens is the sibling of Peter Paul Rubens</skos:scopeNote>
    <rdfs:isDefinedBy rdf:resource="http://vocab.getty.edu/ontology"/>
    <rdf:type rdf:resource="http://www.w3.org/2002/07/owl#ObjectProperty"/>
    <dc:identifier>1501</dc:identifier>
    <dc:title>sibling of - person</dc:title>
    <skos:example>Philippe Rubens is the sibling of Peter Paul Rubens</skos:example>
  </rdf:Description>
  <rdf:Description rdf:about="http://vocab.getty.edu/ontology#aat2502_material_for">
    <skos:prefLabel>aat2502_material_for</skos:prefLabel>
    <skos:example>ivory is material for ivories (sculptures)</skos:example>
    <dc:title>material for - things</dc:title>
    <dc:identifier>2502</dc:identifier>
    <rdfs:range rdf:resource="http://www.w3.org/2004/02/skos/core#Concept"/>
    <skos:example>obsidian is material for obsidian mirrors</skos:example>
    <rdfs:domain rdf:resource="http://www.w3.org/2004/02/skos/core#Concept"/>
    <rdfs:subPropertyOf rdf:resource="http://www.w3.org/2004/02/skos/core#related"/>
    <rdfs:isDefinedBy rdf:resource="http://vocab.getty.edu/ontology"/>
    <dct:description>material - [is] material for - things.&#13;
Example: obsidian is material for obsidian mirrors; ivory is material for ivories (sculptures)</dct:description>
    <skos:scopeNote>material - [is] material for - things.&#13;
Example: obsidian is material for obsidian mirrors; ivory is material for ivories (sculptures)</skos:scopeNote>
    <rdf:type rdf:resource="http://www.w3.org/2002/07/owl#ObjectProperty"/>
    <rdfs:isDefinedBy rdf:resource="http://vocab.getty.edu/aat/"/>
  </rdf:Description>
  <rdf:Description rdf:about="http://vocab.getty.edu/ontology#aat2425_produces">
    <rdf:type rdf:resource="http://www.w3.org/2002/07/owl#ObjectProperty"/>
    <rdfs:isDefinedBy rdf:resource="http://vocab.getty.edu/aat/"/>
    <rdfs:domain rdf:resource="http://www.w3.org/2004/02/skos/core#Concept"/>
    <dct:description>activity/event/process - produces - material.&#13;
Example: wiredrawing produces wire; papermaking produces paper</dct:description>
    <skos:example>wiredrawing produces wire</skos:example>
    <rdfs:range rdf:resource="http://www.w3.org/2004/02/skos/core#Concept"/>
    <dc:identifier>2425</dc:identifier>
    <dc:title>produces - material</dc:title>
    <skos:example>papermaking produces paper</skos:example>
    <skos:scopeNote>activity/event/process - produces - material.&#13;
Example: wiredrawing produces wire; papermaking produces paper</skos:scopeNote>
    <skos:prefLabel>aat2425_produces</skos:prefLabel>
    <rdfs:subPropertyOf rdf:resource="http://www.w3.org/2004/02/skos/core#related"/>
    <rdfs:isDefinedBy rdf:resource="http://vocab.getty.edu/ontology"/>
  </rdf:Description>
  <rdf:Description rdf:about="http://vocab.getty.edu/ontology#aat2607_caused_by-requires">
    <skos:example>creases (condition) is caused by/requires creasing (process)</skos:example>
    <owl:inverseOf rdf:resource="http://vocab.getty.edu/ontology#aat2608_causes-required_for"/>
    <rdfs:range rdf:resource="http://www.w3.org/2004/02/skos/core#Concept"/>
    <rdfs:domain rdf:resource="http://www.w3.org/2004/02/skos/core#Concept"/>
    <dc:identifier>2607</dc:identifier>
    <skos:prefLabel>aat2607_caused_by-requires</skos:prefLabel>
    <rdfs:isDefinedBy rdf:resource="http://vocab.getty.edu/aat/"/>
    <rdf:type rdf:resource="http://www.w3.org/2002/07/owl#ObjectProperty"/>
    <rdfs:isDefinedBy rdf:resource="http://vocab.getty.edu/ontology"/>
    <skos:example>watertightness is caused by/requires waterproofing</skos:example>
    <dc:title>caused by/requires - activity/event</dc:title>
    <skos:scopeNote>attributes /associated concepts - [is] caused by/requires - an activity/event/[process/function].&#13;
Example: watertightness is caused by/requires waterproofing; creases (condition) is caused by/requires creasing (process)</skos:scopeNote>
    <rdfs:subPropertyOf rdf:resource="http://www.w3.org/2004/02/skos/core#related"/>
    <dct:description>attributes /associated concepts - [is] caused by/requires - an activity/event/[process/function].&#13;
Example: watertightness is caused by/requires waterproofing; creases (condition) is caused by/requires creasing (process)</dct:description>
  </rdf:Description>
  <rdf:Description rdf:about="http://vocab.getty.edu/ontology#aat2833_ancestor_of">
    <skos:example>Equus asinus is the ancestor of donkeys</skos:example>
    <rdfs:isDefinedBy rdf:resource="http://vocab.getty.edu/ontology"/>
    <dc:title>ancestor of - genus/species</dc:title>
    <dc:identifier>2833</dc:identifier>
    <skos:prefLabel>aat2833_ancestor_of</skos:prefLabel>
    <rdfs:subPropertyOf rdf:resource="http://www.w3.org/2004/02/skos/core#related"/>
    <rdf:type rdf:resource="http://www.w3.org/2002/07/owl#ObjectProperty"/>
    <rdfs:domain rdf:resource="http://www.w3.org/2004/02/skos/core#Concept"/>
    <skos:scopeNote>genus/species - is ancestor of -  another genus/species.&#13;
Example: Canis lupus is the ancestor of Canis familiaris; Equus asinus is the ancestor of donkeys</skos:scopeNote>
    <skos:example>Canis lupus is the ancestor of Canis familiaris</skos:example>
    <rdfs:range rdf:resource="http://www.w3.org/2004/02/skos/core#Concept"/>
    <dct:description>genus/species - is ancestor of -  another genus/species.&#13;
Example: Canis lupus is the ancestor of Canis familiaris; Equus asinus is the ancestor of donkeys</dct:description>
    <owl:inverseOf rdf:resource="http://vocab.getty.edu/ontology#aat2834_decendant_of"/>
    <rdfs:isDefinedBy rdf:resource="http://vocab.getty.edu/aat/"/>
  </rdf:Description>
  <rdf:Description rdf:about="http://vocab.getty.edu/ontology#aat2849_involves">
    <dc:identifier>2849</dc:identifier>
    <skos:prefLabel>aat2849_involves</skos:prefLabel>
    <dct:description>activity/event - involves - genus/species.&#13;
Example: bullfighting involves bulls (animals); polo (field sport) involves Equus caballus (species)</dct:description>
    <rdfs:domain rdf:resource="http://www.w3.org/2004/02/skos/core#Concept"/>
    <rdfs:range rdf:resource="http://www.w3.org/2004/02/skos/core#Concept"/>
    <skos:scopeNote>activity/event - involves - genus/species.&#13;
Example: bullfighting involves bulls (animals); polo (field sport) involves Equus caballus (species)</skos:scopeNote>
    <rdfs:subPropertyOf rdf:resource="http://www.w3.org/2004/02/skos/core#related"/>
    <skos:example>polo (field sport) involves Equus caballus (species)</skos:example>
    <rdfs:isDefinedBy rdf:resource="http://vocab.getty.edu/ontology"/>
    <dc:title>involves - genus/species</dc:title>
    <rdf:type rdf:resource="http://www.w3.org/2002/07/owl#ObjectProperty"/>
    <skos:example>bullfighting involves bulls (animals)</skos:example>
    <rdfs:isDefinedBy rdf:resource="http://vocab.getty.edu/aat/"/>
  </rdf:Description>
  <rdf:Description rdf:about="http://vocab.getty.edu/ontology#aat2333_have_affiliates">
    <dc:title>have affiliates - role</dc:title>
    <skos:prefLabel>aat2333_have_affiliates</skos:prefLabel>
    <rdfs:domain rdf:resource="http://www.w3.org/2004/02/skos/core#Concept"/>
    <rdfs:range rdf:resource="http://www.w3.org/2004/02/skos/core#Concept"/>
    <rdfs:isDefinedBy rdf:resource="http://vocab.getty.edu/aat/"/>
    <dc:identifier>2333</dc:identifier>
    <skos:example>schools (organizations) have as affiliates students</skos:example>
    <rdf:type rdf:resource="http://www.w3.org/2002/07/owl#ObjectProperty"/>
    <rdfs:isDefinedBy rdf:resource="http://vocab.getty.edu/ontology"/>
    <skos:scopeNote>role [organizations] - have affiliates - [actors having] role.&#13;
Example: schools (organizations) have as affiliates students; duchies have as affiliates dukes</skos:scopeNote>
    <rdfs:subPropertyOf rdf:resource="http://www.w3.org/2004/02/skos/core#related"/>
    <skos:example>duchies have as affiliates dukes</skos:example>
    <dct:description>role [organizations] - have affiliates - [actors having] role.&#13;
Example: schools (organizations) have as affiliates students; duchies have as affiliates dukes</dct:description>
  </rdf:Description>
  <rdf:Description rdf:about="http://vocab.getty.edu/ontology#broaderPartitiveExtended">
    <rdfs:comment>Ancestors (Partitive). Meaningful closure of gvp:broaderPartitive. Infers iso:broaderPartitive for pairs of directly related skos:Concepts</rdfs:comment>
    <owl:propertyChainAxiom rdf:nodeID="N9c386dc021084c29bfcaa74d6d7c1db7"/>
    <skos:example>anvil components BTP &lt;anvils and anvil accessories&gt; BTG &lt;forging and metal-shaping tools&gt;,
so anvil components BTPE &lt;forging and metal-shaping tools&gt;</skos:example>
    <skos:definition>Ancestors (Partitive). Meaningful closure of gvp:broaderPartitive. Infers iso:broaderPartitive for pairs of directly related skos:Concepts</skos:definition>
    <rdfs:domain rdf:resource="http://vocab.getty.edu/ontology#Subject"/>
    <rdfs:range rdf:resource="http://vocab.getty.edu/ontology#Subject"/>
    <skos:scopeNote>Ancestors (Partitive). Meaningful closure of gvp:broaderPartitive. Infers iso:broaderPartitive for pairs of directly related skos:Concepts.
Example: anvil components BTP &lt;anvils and anvil accessories&gt; BTG &lt;forging and metal-shaping tools&gt;,
so anvil components BTPE &lt;forging and metal-shaping tools&gt;</skos:scopeNote>
    <rdfs:label>broaderPartitiveExtended</rdfs:label>
    <owl:propertyChainAxiom rdf:nodeID="N52cd7acc51f54260bfe30b76ba441dc7"/>
    <rdfs:subPropertyOf rdf:resource="http://vocab.getty.edu/ontology#broaderExtended"/>
    <skos:prefLabel>broaderPartitiveExtended</skos:prefLabel>
    <owl:propertyChainAxiom rdf:nodeID="N8eab80e9df0a4f29aa7d04c3bd66fd47"/>
    <rdf:type rdf:resource="http://www.w3.org/2002/07/owl#ObjectProperty"/>
    <rdfs:isDefinedBy rdf:resource="http://vocab.getty.edu/ontology"/>
    <dct:description>Ancestors (Partitive). Meaningful closure of gvp:broaderPartitive. Infers iso:broaderPartitive for pairs of directly related skos:Concepts.
Example: anvil components BTP &lt;anvils and anvil accessories&gt; BTG &lt;forging and metal-shaping tools&gt;,
so anvil components BTPE &lt;forging and metal-shaping tools&gt;</dct:description>
  </rdf:Description>
  <rdf:Description rdf:about="http://vocab.getty.edu/ontology#tgn3318_member_is">
    <skos:scopeNote>union - member is - nation.&#13;
Example: Austria is a member of the European Union since 1915; Belgium is a member of the European Union since 1958</skos:scopeNote>
    <rdfs:domain rdf:resource="http://www.w3.org/2004/02/skos/core#Concept"/>
    <skos:example>Belgium is a member of the European Union since 1958</skos:example>
    <rdfs:range rdf:resource="http://www.w3.org/2004/02/skos/core#Concept"/>
    <skos:example>Austria is a member of the European Union since 1915</skos:example>
    <dct:description>union - member is - nation.&#13;
Example: Austria is a member of the European Union since 1915; Belgium is a member of the European Union since 1958</dct:description>
    <rdf:type rdf:resource="http://www.w3.org/2002/07/owl#ObjectProperty"/>
    <skos:prefLabel>tgn3318_member_is</skos:prefLabel>
    <rdfs:isDefinedBy rdf:resource="http://vocab.getty.edu/ontology"/>
    <rdfs:subPropertyOf rdf:resource="http://www.w3.org/2004/02/skos/core#related"/>
    <rdfs:isDefinedBy rdf:resource="http://vocab.getty.edu/tgn/"/>
    <dc:title>member is - nation</dc:title>
    <dc:identifier>3318</dc:identifier>
  </rdf:Description>
  <rdf:Description rdf:about="http://vocab.getty.edu/ontology#ulan1106_apprentice_was">
    <skos:prefLabel>ulan1106_apprentice_was</skos:prefLabel>
    <rdf:type rdf:resource="http://www.w3.org/2002/07/owl#ObjectProperty"/>
    <rdfs:isDefinedBy rdf:resource="http://vocab.getty.edu/ontology"/>
    <dc:title>apprentice was - person</dc:title>
    <skos:example>Nicolas Hawksmoor was the apprentice of Christopher Wren</skos:example>
    <rdfs:range rdf:resource="http://www.w3.org/2004/02/skos/core#Concept"/>
    <rdfs:domain rdf:resource="http://www.w3.org/2004/02/skos/core#Concept"/>
    <rdfs:isDefinedBy rdf:resource="http://vocab.getty.edu/ulan/"/>
    <dct:description>person - apprentice was - person.&#13;
Example: Nicolas Hawksmoor was the apprentice of Christopher Wren</dct:description>
    <rdfs:subPropertyOf rdf:resource="http://www.w3.org/2004/02/skos/core#related"/>
    <dc:identifier>1106</dc:identifier>
    <skos:scopeNote>person - apprentice was - person.&#13;
Example: Nicolas Hawksmoor was the apprentice of Christopher Wren</skos:scopeNote>
  </rdf:Description>
  <rdf:Description rdf:about="http://vocab.getty.edu/ontology#ulan1113_fellow_student_of">
    <rdf:type rdf:resource="http://www.w3.org/2002/07/owl#SymmetricProperty"/>
    <rdfs:isDefinedBy rdf:resource="http://vocab.getty.edu/ulan/"/>
    <skos:example>John Sloan was a fellow student of Thomas Hart Benton</skos:example>
    <skos:scopeNote>person - fellow student of - person.&#13;
Example: Alexander Calder was a fellow student of John Sloan; John Sloan was a fellow student of Thomas Hart Benton</skos:scopeNote>
    <rdfs:subPropertyOf rdf:resource="http://www.w3.org/2004/02/skos/core#related"/>
    <skos:prefLabel>ulan1113_fellow_student_of</skos:prefLabel>
    <dct:description>person - fellow student of - person.&#13;
Example: Alexander Calder was a fellow student of John Sloan; John Sloan was a fellow student of Thomas Hart Benton</dct:description>
    <dc:identifier>1113</dc:identifier>
    <rdfs:domain rdf:resource="http://www.w3.org/2004/02/skos/core#Concept"/>
    <rdfs:range rdf:resource="http://www.w3.org/2004/02/skos/core#Concept"/>
    <dc:title>fellow student of - person</dc:title>
    <skos:example>Alexander Calder was a fellow student of John Sloan</skos:example>
    <rdf:type rdf:resource="http://www.w3.org/2002/07/owl#ObjectProperty"/>
    <rdfs:isDefinedBy rdf:resource="http://vocab.getty.edu/ontology"/>
  </rdf:Description>
  <rdf:Description rdf:about="http://vocab.getty.edu/ontology#ulan1422_founded">
    <skos:example>The United States Congress founded the National Gallery of Art</skos:example>
    <rdfs:domain rdf:resource="http://www.w3.org/2004/02/skos/core#Concept"/>
    <skos:prefLabel>ulan1422_founded</skos:prefLabel>
    <rdfs:range rdf:resource="http://www.w3.org/2004/02/skos/core#Concept"/>
    <dct:description>firm/group - founded - firm/group.&#13;
Example: The United States Congress founded the National Gallery of Art</dct:description>
    <rdf:type rdf:resource="http://www.w3.org/2002/07/owl#ObjectProperty"/>
    <rdfs:isDefinedBy rdf:resource="http://vocab.getty.edu/ontology"/>
    <dc:title>founded - firm/group</dc:title>
    <rdfs:isDefinedBy rdf:resource="http://vocab.getty.edu/ulan/"/>
    <skos:scopeNote>firm/group - founded - firm/group.&#13;
Example: The United States Congress founded the National Gallery of Art</skos:scopeNote>
    <rdfs:subPropertyOf rdf:resource="http://www.w3.org/2004/02/skos/core#related"/>
    <dc:identifier>1422</dc:identifier>
  </rdf:Description>
  <rdf:Description rdf:about="http://vocab.getty.edu/ontology#aat2322_use">
    <dc:title>use - things</dc:title>
    <dc:identifier>2322</dc:identifier>
    <rdfs:subPropertyOf rdf:resource="http://www.w3.org/2004/02/skos/core#related"/>
    <rdfs:isDefinedBy rdf:resource="http://vocab.getty.edu/ontology"/>
    <skos:scopeNote>[actors having] role - use - things/equipment.&#13;
Example: violoncellists use violoncellos; surveyors use surveying instruments</skos:scopeNote>
    <skos:example>violoncellists use violoncellos</skos:example>
    <rdf:type rdf:resource="http://www.w3.org/2002/07/owl#ObjectProperty"/>
    <rdfs:isDefinedBy rdf:resource="http://vocab.getty.edu/aat/"/>
    <skos:prefLabel>aat2322_use</skos:prefLabel>
    <rdfs:range rdf:resource="http://www.w3.org/2004/02/skos/core#Concept"/>
    <rdfs:domain rdf:resource="http://www.w3.org/2004/02/skos/core#Concept"/>
    <dct:description>[actors having] role - use - things/equipment.&#13;
Example: violoncellists use violoncellos; surveyors use surveying instruments</dct:description>
    <skos:example>surveyors use surveying instruments</skos:example>
  </rdf:Description>
  <rdf:Description rdf:about="http://vocab.getty.edu/ontology#ulan1317_member_of">
    <skos:example>A member of the Foundation of Documents of Architecture is the National Gallery of Art</skos:example>
    <rdfs:subPropertyOf rdf:resource="http://www.w3.org/2004/02/skos/core#related"/>
    <skos:prefLabel>ulan1317_member_of</skos:prefLabel>
    <dc:title>member of - person/firm/group</dc:title>
    <dct:description>firm/group - member of - person/firm/group.&#13;
Example: A member of the Foundation of Documents of Architecture is the National Gallery of Art</dct:description>
    <rdfs:isDefinedBy rdf:resource="http://vocab.getty.edu/ontology"/>
    <dc:identifier>1317</dc:identifier>
    <rdfs:domain rdf:resource="http://www.w3.org/2004/02/skos/core#Concept"/>
    <owl:inverseOf rdf:resource="http://vocab.getty.edu/ontology#ulan1318_member_was"/>
    <rdf:type rdf:resource="http://www.w3.org/2002/07/owl#ObjectProperty"/>
    <skos:scopeNote>firm/group - member of - person/firm/group.&#13;
Example: A member of the Foundation of Documents of Architecture is the National Gallery of Art</skos:scopeNote>
    <rdfs:isDefinedBy rdf:resource="http://vocab.getty.edu/ulan/"/>
    <rdfs:range rdf:resource="http://www.w3.org/2004/02/skos/core#Concept"/>
  </rdf:Description>
  <rdf:Description rdf:about="http://vocab.getty.edu/ontology#ulan1573_ward_of">
    <skos:prefLabel>ulan1573_ward_of</skos:prefLabel>
    <rdfs:subPropertyOf rdf:resource="http://www.w3.org/2004/02/skos/core#related"/>
    <skos:example>Samuel Cooper was a ward of John Hoskins, the elder</skos:example>
    <dct:description>person - ward of - person.&#13;
Example: Samuel Cooper was a ward of John Hoskins, the elder</dct:description>
    <rdfs:isDefinedBy rdf:resource="http://vocab.getty.edu/ulan/"/>
    <rdfs:range rdf:resource="http://www.w3.org/2004/02/skos/core#Concept"/>
    <rdfs:domain rdf:resource="http://www.w3.org/2004/02/skos/core#Concept"/>
    <dc:title>ward of - person</dc:title>
    <dc:identifier>1573</dc:identifier>
    <skos:scopeNote>person - ward of - person.&#13;
Example: Samuel Cooper was a ward of John Hoskins, the elder</skos:scopeNote>
    <rdf:type rdf:resource="http://www.w3.org/2002/07/owl#ObjectProperty"/>
    <rdfs:isDefinedBy rdf:resource="http://vocab.getty.edu/ontology"/>
  </rdf:Description>
  <rdf:Description rdf:about="http://vocab.getty.edu/ontology#placeTypeNonPreferred">
    <rdfs:comment>A secondary type for a TGN Place. Domain is TGN concept, range is AAT concept</rdfs:comment>
    <rdfs:domain rdf:resource="http://vocab.getty.edu/ontology#Subject"/>
    <rdfs:range rdf:resource="http://vocab.getty.edu/ontology#Subject"/>
    <rdfs:label>placeTypeNonPreferred</rdfs:label>
    <skos:scopeNote>A secondary type for a TGN Place. Domain is TGN concept, range is AAT concept.
Example: A non-preferred type of Machupicchu, Peru is "Inca center" (historical)</skos:scopeNote>
    <rdfs:isDefinedBy rdf:resource="http://vocab.getty.edu/ontology"/>
    <skos:example>A non-preferred type of Machupicchu, Peru is "Inca center" (historical)</skos:example>
    <rdf:type rdf:resource="http://www.w3.org/2002/07/owl#ObjectProperty"/>
    <rdfs:subPropertyOf rdf:resource="http://vocab.getty.edu/ontology#placeType"/>
    <skos:prefLabel>placeTypeNonPreferred</skos:prefLabel>
    <dct:description>A secondary type for a TGN Place. Domain is TGN concept, range is AAT concept.
Example: A non-preferred type of Machupicchu, Peru is "Inca center" (historical)</dct:description>
    <skos:definition>A secondary type for a TGN Place. Domain is TGN concept, range is AAT concept</skos:definition>
  </rdf:Description>
  <rdf:Description rdf:about="http://vocab.getty.edu/ontology#parentStringAbbrev">
    <rdfs:isDefinedBy rdf:resource="http://vocab.getty.edu/ontology"/>
    <rdf:type rdf:resource="http://www.w3.org/2002/07/owl#DatatypeProperty"/>
    <skos:scopeNote>Preferred labels of *some* of the subject's preferred ancestors, listed bottom up. Useful to show the subject's context.
Shortened display version of gvp:broaderPreferredExtended.
Example for aat:300226882 baking dishes: bakeware, &lt;vessels for cooking food&gt;, ... Furnishings and Equipment (Hierarchy Name)</skos:scopeNote>
    <skos:definition>Preferred labels of *some* of the subject's preferred ancestors, listed bottom up. Useful to show the subject's context</skos:definition>
    <skos:prefLabel>parentStringAbbrev</skos:prefLabel>
    <rdfs:comment>Preferred labels of *some* of the subject's preferred ancestors, listed bottom up. Useful to show the subject's context</rdfs:comment>
    <rdfs:label>parentStringAbbrev</rdfs:label>
    <dct:description>Preferred labels of *some* of the subject's preferred ancestors, listed bottom up. Useful to show the subject's context.
Shortened display version of gvp:broaderPreferredExtended.
Example for aat:300226882 baking dishes: bakeware, &lt;vessels for cooking food&gt;, ... Furnishings and Equipment (Hierarchy Name)</dct:description>
    <rdfs:domain rdf:resource="http://vocab.getty.edu/ontology#Subject"/>
    <skos:note>Shortened display version of gvp:broaderPreferredExtended</skos:note>
    <rdfs:range rdf:resource="http://www.w3.org/1999/02/22-rdf-syntax-ns#Literal"/>
    <skos:example>For aat:300226882 baking dishes: bakeware, &lt;vessels for cooking food&gt;, ... Furnishings and Equipment (Hierarchy Name)</skos:example>
  </rdf:Description>
  <rdf:Description rdf:about="http://vocab.getty.edu/ontology#aat2885_involves">
    <rdf:type rdf:resource="http://www.w3.org/2002/07/owl#ObjectProperty"/>
    <skos:example>Celtic culture involves Celtic crosses (design motif)</skos:example>
    <dc:title>involves - attributes /associated concepts</dc:title>
    <rdfs:subPropertyOf rdf:resource="http://www.w3.org/2004/02/skos/core#related"/>
    <rdfs:domain rdf:resource="http://www.w3.org/2004/02/skos/core#Concept"/>
    <dct:description>any - involves - attributes /associated concepts.&#13;
Example: climate change involves climate;  infestation involves insect damage; Celtic culture involves Celtic crosses (design motif)</dct:description>
    <skos:example>climate change involves climate</skos:example>
    <skos:prefLabel>aat2885_involves</skos:prefLabel>
    <dc:identifier>2885</dc:identifier>
    <skos:scopeNote>any - involves - attributes /associated concepts.&#13;
Example: climate change involves climate;  infestation involves insect damage; Celtic culture involves Celtic crosses (design motif)</skos:scopeNote>
    <rdfs:range rdf:resource="http://www.w3.org/2004/02/skos/core#Concept"/>
    <rdfs:isDefinedBy rdf:resource="http://vocab.getty.edu/aat/"/>
    <skos:example>infestation involves insect damage</skos:example>
    <rdfs:isDefinedBy rdf:resource="http://vocab.getty.edu/ontology"/>
  </rdf:Description>
  <rdf:Description rdf:about="http://vocab.getty.edu/ontology#ulan2574_director_of">
    <owl:inverseOf rdf:resource="http://vocab.getty.edu/ontology#ulan2575_directed_by"/>
    <skos:scopeNote>person - director of - institution.&#13;
Example: Jean Jans I directed Gobelins Tapestry Manufactory</skos:scopeNote>
    <rdfs:domain rdf:resource="http://www.w3.org/2004/02/skos/core#Concept"/>
    <rdfs:range rdf:resource="http://www.w3.org/2004/02/skos/core#Concept"/>
    <rdfs:isDefinedBy rdf:resource="http://vocab.getty.edu/ontology"/>
    <dc:title>director of - institution</dc:title>
    <rdf:type rdf:resource="http://www.w3.org/2002/07/owl#ObjectProperty"/>
    <dc:identifier>2574</dc:identifier>
    <skos:prefLabel>ulan2574_director_of</skos:prefLabel>
    <rdfs:isDefinedBy rdf:resource="http://vocab.getty.edu/ulan/"/>
    <rdfs:subPropertyOf rdf:resource="http://www.w3.org/2004/02/skos/core#related"/>
    <dct:description>person - director of - institution.&#13;
Example: Jean Jans I directed Gobelins Tapestry Manufactory</dct:description>
    <skos:example>Jean Jans I directed Gobelins Tapestry Manufactory</skos:example>
  </rdf:Description>
  <rdf:Description rdf:about="http://vocab.getty.edu/ontology#aat2100_distinguished_from">
    <skos:scopeNote>any - distinguished from - any.&#13;
Example: historic farms are distinguished from abandoned farms; naive art is distinguished from outsider art</skos:scopeNote>
    <dc:title>distinguished from - any</dc:title>
    <rdfs:domain rdf:resource="http://www.w3.org/2004/02/skos/core#Concept"/>
    <rdfs:isDefinedBy rdf:resource="http://vocab.getty.edu/aat/"/>
    <rdfs:range rdf:resource="http://www.w3.org/2004/02/skos/core#Concept"/>
    <rdfs:isDefinedBy rdf:resource="http://vocab.getty.edu/ontology"/>
    <rdf:type rdf:resource="http://www.w3.org/2002/07/owl#SymmetricProperty"/>
    <skos:example>historic farms are distinguished from abandoned farms</skos:example>
    <dc:identifier>2100</dc:identifier>
    <dct:description>any - distinguished from - any.&#13;
Example: historic farms are distinguished from abandoned farms; naive art is distinguished from outsider art</dct:description>
    <rdf:type rdf:resource="http://www.w3.org/2002/07/owl#ObjectProperty"/>
    <skos:prefLabel>aat2100_distinguished_from</skos:prefLabel>
    <rdfs:subPropertyOf rdf:resource="http://www.w3.org/2004/02/skos/core#related"/>
    <skos:example>naive art is distinguished from outsider art</skos:example>
  </rdf:Description>
  <rdf:Description rdf:about="http://vocab.getty.edu/ontology#aat2001_formerly_referred_to">
    <skos:example>gigues formerly referred to fiddles</skos:example>
    <rdf:type rdf:resource="http://www.w3.org/2002/07/owl#SymmetricProperty"/>
    <skos:scopeNote>any - formerly referred - any.&#13;
Example: gigues formerly referred to fiddles</skos:scopeNote>
    <skos:prefLabel>aat2001_formerly_referred_to</skos:prefLabel>
    <rdfs:subPropertyOf rdf:resource="http://www.w3.org/2004/02/skos/core#related"/>
    <dc:identifier>2001</dc:identifier>
    <dc:title>formerly referred to - any</dc:title>
    <rdfs:domain rdf:resource="http://www.w3.org/2004/02/skos/core#Concept"/>
    <rdfs:range rdf:resource="http://www.w3.org/2004/02/skos/core#Concept"/>
    <dct:description>any - formerly referred - any.&#13;
Example: gigues formerly referred to fiddles</dct:description>
    <rdfs:isDefinedBy rdf:resource="http://vocab.getty.edu/aat/"/>
    <rdf:type rdf:resource="http://www.w3.org/2002/07/owl#ObjectProperty"/>
    <rdfs:isDefinedBy rdf:resource="http://vocab.getty.edu/ontology"/>
  </rdf:Description>
  <rdf:Description rdf:about="http://vocab.getty.edu/term/kind/ScientificOrTechnical">
    <rdf:type rdf:resource="http://www.w3.org/2004/02/skos/core#Concept"/>
    <skos:notation>S</skos:notation>
    <skos:scopeNote>Scientific taxon name (genus, species, etc). Used in AAT only. All such are emitted marked with English language, and most have the same string marked with Latin</skos:scopeNote>
    <skos:example>"Boswellia sacra"@la, also emitted as "Boswellia sacra"@en, is scientific name of "frankincense"</skos:example>
    <skos:inScheme rdf:resource="http://vocab.getty.edu/term/kind/"/>
    <skos:prefLabel>Scientific or Technical term</skos:prefLabel>
    <dct:description>Scientific taxon name (genus, species, etc). Used in AAT only. All such are emitted marked with English language, and most have the same string marked with Latin.
Example: "Boswellia sacra"@la, also emitted as "Boswellia sacra"@en, is scientific name of "frankincense"</dct:description>
  </rdf:Description>
  <rdf:Description rdf:about="http://vocab.getty.edu/ontology#ulan1556_half-sibling_of">
    <dc:title>half-sibling of - person</dc:title>
    <rdfs:isDefinedBy rdf:resource="http://vocab.getty.edu/ulan/"/>
    <dct:description>person - half-sibling of - person.&#13;
Example: Juan Bautista Monegro and Luis de Carbajal are half siblings</dct:description>
    <rdf:type rdf:resource="http://www.w3.org/2002/07/owl#SymmetricProperty"/>
    <rdfs:isDefinedBy rdf:resource="http://vocab.getty.edu/ontology"/>
    <rdfs:domain rdf:resource="http://www.w3.org/2004/02/skos/core#Concept"/>
    <rdfs:subPropertyOf rdf:resource="http://www.w3.org/2004/02/skos/core#related"/>
    <rdf:type rdf:resource="http://www.w3.org/2002/07/owl#ObjectProperty"/>
    <skos:example>Juan Bautista Monegro and Luis de Carbajal are half siblings</skos:example>
    <rdfs:range rdf:resource="http://www.w3.org/2004/02/skos/core#Concept"/>
    <skos:prefLabel>ulan1556_half-sibling_of</skos:prefLabel>
    <dc:identifier>1556</dc:identifier>
    <skos:scopeNote>person - half-sibling of - person.&#13;
Example: Juan Bautista Monegro and Luis de Carbajal are half siblings</skos:scopeNote>
  </rdf:Description>
  <rdf:Description rdf:about="http://vocab.getty.edu/ontology#ulan1516_great-grandchild_of">
    <skos:example>Richard Benno Adam is the great-grandchild of Albrecht Adam</skos:example>
    <dc:title>great-grandchild of - person</dc:title>
    <rdfs:isDefinedBy rdf:resource="http://vocab.getty.edu/ulan/"/>
    <dc:identifier>1516</dc:identifier>
    <rdfs:subPropertyOf rdf:resource="http://www.w3.org/2004/02/skos/core#related"/>
    <rdf:type rdf:resource="http://www.w3.org/2002/07/owl#ObjectProperty"/>
    <skos:prefLabel>ulan1516_great-grandchild_of</skos:prefLabel>
    <rdfs:isDefinedBy rdf:resource="http://vocab.getty.edu/ontology"/>
    <skos:scopeNote>person - great-grandchild of - person.&#13;
Example: Richard Benno Adam is the great-grandchild of Albrecht Adam</skos:scopeNote>
    <rdfs:domain rdf:resource="http://www.w3.org/2004/02/skos/core#Concept"/>
    <rdfs:range rdf:resource="http://www.w3.org/2004/02/skos/core#Concept"/>
    <dct:description>person - great-grandchild of - person.&#13;
Example: Richard Benno Adam is the great-grandchild of Albrecht Adam</dct:description>
  </rdf:Description>
  <rdf:Description rdf:about="http://vocab.getty.edu/ontology#ulan2782_dedicated_to">
    <skos:example>The Rodin Museum in Philadelphia is didicated to Auguste Rodin</skos:example>
    <dc:title>dedicated to - person</dc:title>
    <rdfs:isDefinedBy rdf:resource="http://vocab.getty.edu/ulan/"/>
    <dc:identifier>2782</dc:identifier>
    <skos:scopeNote>institution - dedicated to - person.&#13;
Example: The Rodin Museum in Philadelphia is didicated to Auguste Rodin</skos:scopeNote>
    <dct:description>institution - dedicated to - person.&#13;
Example: The Rodin Museum in Philadelphia is didicated to Auguste Rodin</dct:description>
    <rdf:type rdf:resource="http://www.w3.org/2002/07/owl#ObjectProperty"/>
    <skos:prefLabel>ulan2782_dedicated_to</skos:prefLabel>
    <rdfs:isDefinedBy rdf:resource="http://vocab.getty.edu/ontology"/>
    <rdfs:domain rdf:resource="http://www.w3.org/2004/02/skos/core#Concept"/>
    <rdfs:subPropertyOf rdf:resource="http://www.w3.org/2004/02/skos/core#related"/>
    <rdfs:range rdf:resource="http://www.w3.org/2004/02/skos/core#Concept"/>
  </rdf:Description>
  <rdf:Description rdf:about="http://vocab.getty.edu/ontology#ulan1413_administration_overlaps_with">
    <rdf:type rdf:resource="http://www.w3.org/2002/07/owl#SymmetricProperty"/>
    <rdfs:isDefinedBy rdf:resource="http://vocab.getty.edu/ulan/"/>
    <dct:description>firm/group - administration overlaps with - firm/group.&#13;
Example: The administration of the Numismatic Collection overlaps with Bode Museum</dct:description>
    <dc:identifier>1413</dc:identifier>
    <skos:example>The administration of the Numismatic Collection overlaps with Bode Museum</skos:example>
    <rdfs:subPropertyOf rdf:resource="http://www.w3.org/2004/02/skos/core#related"/>
    <dc:title>administration overlaps with - firm/group</dc:title>
    <skos:prefLabel>ulan1413_administration_overlaps_with</skos:prefLabel>
    <rdfs:domain rdf:resource="http://www.w3.org/2004/02/skos/core#Concept"/>
    <rdfs:range rdf:resource="http://www.w3.org/2004/02/skos/core#Concept"/>
    <skos:scopeNote>firm/group - administration overlaps with - firm/group.&#13;
Example: The administration of the Numismatic Collection overlaps with Bode Museum</skos:scopeNote>
    <rdf:type rdf:resource="http://www.w3.org/2002/07/owl#ObjectProperty"/>
    <rdfs:isDefinedBy rdf:resource="http://vocab.getty.edu/ontology"/>
  </rdf:Description>
  <rdf:Description rdf:about="http://vocab.getty.edu/historic/historic">
    <skos:notation>H</skos:notation>
    <skos:inScheme rdf:resource="http://vocab.getty.edu/historic/"/>
    <skos:prefLabel>Historic</skos:prefLabel>
    <skos:example>"Lutetia" is a historic name for "Paris" (TGN). "weyneschot" is a 16th-century spelling for "wainscoting" (AAT)</skos:example>
    <rdf:type rdf:resource="http://www.w3.org/2004/02/skos/core#Concept"/>
    <dct:description>Valid/used in the past but not currently.
Example: "Lutetia" is a historic name for "Paris" (TGN). "weyneschot" is a 16th-century spelling for "wainscoting" (AAT)</dct:description>
    <skos:scopeNote>Valid/used in the past but not currently</skos:scopeNote>
  </rdf:Description>
  <rdf:Description rdf:about="http://vocab.getty.edu/ontology#ulan1314_partner_was">
    <rdfs:subPropertyOf rdf:resource="http://www.w3.org/2004/02/skos/core#related"/>
    <rdfs:isDefinedBy rdf:resource="http://vocab.getty.edu/ulan/"/>
    <dct:description>firm - partner was - person.&#13;
Example: Louis H. Sullivan and Dankmar Adler were partners in Adler and Sullivan</dct:description>
    <skos:prefLabel>ulan1314_partner_was</skos:prefLabel>
    <skos:example>Louis H. Sullivan and Dankmar Adler were partners in Adler and Sullivan</skos:example>
    <rdfs:range rdf:resource="http://www.w3.org/2004/02/skos/core#Concept"/>
    <rdfs:domain rdf:resource="http://www.w3.org/2004/02/skos/core#Concept"/>
    <dc:title>partner was - person</dc:title>
    <dc:identifier>1314</dc:identifier>
    <rdf:type rdf:resource="http://www.w3.org/2002/07/owl#ObjectProperty"/>
    <skos:scopeNote>firm - partner was - person.&#13;
Example: Louis H. Sullivan and Dankmar Adler were partners in Adler and Sullivan</skos:scopeNote>
    <rdfs:isDefinedBy rdf:resource="http://vocab.getty.edu/ontology"/>
  </rdf:Description>
  <rdf:Description rdf:about="http://vocab.getty.edu/ontology#aat2841_derived-made_from">
    <skos:example>alpaca (wool) is derived from Vicugna pacos (species)</skos:example>
    <rdfs:domain rdf:resource="http://www.w3.org/2004/02/skos/core#Concept"/>
    <rdfs:range rdf:resource="http://www.w3.org/2004/02/skos/core#Concept"/>
    <rdfs:isDefinedBy rdf:resource="http://vocab.getty.edu/ontology"/>
    <rdfs:subPropertyOf rdf:resource="http://www.w3.org/2004/02/skos/core#related"/>
    <rdf:type rdf:resource="http://www.w3.org/2002/07/owl#ObjectProperty"/>
    <dct:description>material - [is] derived/made from - genus/species.&#13;
Example: alpaca (wool) is derived from Vicugna pacos (species); maple (wood) is derived from Acer (genus)</dct:description>
    <owl:inverseOf rdf:resource="http://vocab.getty.edu/ontology#aat2842_source_for"/>
    <dc:identifier>2841</dc:identifier>
    <skos:prefLabel>aat2841_derived-made_from</skos:prefLabel>
    <skos:example>maple (wood) is derived from Acer (genus)</skos:example>
    <dc:title>derived/made from - genus/species</dc:title>
    <skos:scopeNote>material - [is] derived/made from - genus/species.&#13;
Example: alpaca (wool) is derived from Vicugna pacos (species); maple (wood) is derived from Acer (genus)</skos:scopeNote>
    <rdfs:isDefinedBy rdf:resource="http://vocab.getty.edu/aat/"/>
  </rdf:Description>
  <rdf:Description rdf:about="http://vocab.getty.edu/ontology#qualifier">
    <skos:prefLabel>qualifier</skos:prefLabel>
    <rdfs:isDefinedBy rdf:resource="http://vocab.getty.edu/ontology"/>
    <rdfs:range rdf:resource="http://www.w3.org/1999/02/22-rdf-syntax-ns#Literal"/>
    <rdfs:label>qualifier</rdfs:label>
    <skos:scopeNote>Clarifies and disambiguates terms with the same spelling but different meaning.
Appended in parentheses to gvp:term, forming skosxsl:literalForm.
Every qualifier is in the same language as the term.
Example: "Rhea (vessels)"=rhyta (a kind of drinking vessel) vs "Rhea (species)"=Boehmeria nivea (Chinese grass)</skos:scopeNote>
    <skos:definition>Clarifies and disambiguates terms with the same spelling but different meaning.
Appended in parentheses to gvp:term, forming skosxsl:literalForm.
Every qualifier is in the same language as the term</skos:definition>
    <rdfs:domain rdf:resource="http://www.w3.org/2008/05/skos-xl#Label"/>
    <skos:example>Rhea (vessels)=rhyta (a kind of drinking vessel) vs rhea (species)=Boehmeria nivea (Chinese grass)</skos:example>
    <dct:description>Clarifies and disambiguates terms with the same spelling but different meaning.
Appended in parentheses to gvp:term, forming skosxsl:literalForm.
Every qualifier is in the same language as the term.
Example: "Rhea (vessels)"=rhyta (a kind of drinking vessel) vs "Rhea (species)"=Boehmeria nivea (Chinese grass)</dct:description>
    <rdf:type rdf:resource="http://www.w3.org/2002/07/owl#DatatypeProperty"/>
    <rdfs:comment>Clarifies and disambiguates terms with the same spelling but different meaning.
Appended in parentheses to gvp:term, forming skosxsl:literalForm.
Every qualifier is in the same language as the term</rdfs:comment>
  </rdf:Description>
  <rdf:Description rdf:about="http://vocab.getty.edu/ontology#aat2218_used-function_as">
    <skos:example>arc lamps are used/function as lighthouse lamps</skos:example>
    <rdfs:isDefinedBy rdf:resource="http://vocab.getty.edu/ontology"/>
    <dc:title>used/function as - things</dc:title>
    <skos:example>toile peinte is used/function as cartoons (working drawings)</skos:example>
    <dc:identifier>2218</dc:identifier>
    <rdfs:domain rdf:resource="http://www.w3.org/2004/02/skos/core#Concept"/>
    <rdfs:subPropertyOf rdf:resource="http://www.w3.org/2004/02/skos/core#related"/>
    <rdf:type rdf:resource="http://www.w3.org/2002/07/owl#ObjectProperty"/>
    <rdfs:range rdf:resource="http://www.w3.org/2004/02/skos/core#Concept"/>
    <skos:scopeNote>things - [are] used/function as - things.&#13;
Example: arc lamps are used/function as lighthouse lamps;  toile peinte is used/function as cartoons (working drawings)</skos:scopeNote>
    <dct:description>things - [are] used/function as - things.&#13;
Example: arc lamps are used/function as lighthouse lamps;  toile peinte is used/function as cartoons (working drawings)</dct:description>
    <skos:prefLabel>aat2218_used-function_as</skos:prefLabel>
    <rdfs:isDefinedBy rdf:resource="http://vocab.getty.edu/aat/"/>
    <owl:inverseOf rdf:resource="http://vocab.getty.edu/ontology#aat2219_have_form"/>
  </rdf:Description>
  <rdf:Description rdf:about="http://vocab.getty.edu/tgn/">
    <dct:creator rdf:resource="http://www.getty.edu/research/"/>
    <skos:prefLabel>Thesaurus of Geographic Names</skos:prefLabel>
    <rdfs:seeAlso rdf:resource="http://vocab.getty.edu/"/>
    <rdfs:label>Thesaurus of Geographic Names</rdfs:label>
    <foaf:homepage rdf:resource="http://www.getty.edu/research/tools/vocabularies/tgn/"/>
    <rdf:type rdf:resource="http://www.w3.org/2004/02/skos/core#ConceptScheme"/>
    <vann:preferredNamespaceUri>http://vocab.getty.edu/tgn/</vann:preferredNamespaceUri>
    <rdfs:seeAlso rdf:resource="http://vocab.getty.edu/.well-known/void"/>
    <skos:definition>The Thesaurus of Geographic Names concept scheme</skos:definition>
    <vann:preferredNamespacePrefix>tgn</vann:preferredNamespacePrefix>
    <dct:creator rdf:resource="http://www.ontotext.com"/>
    <dct:created rdf:datatype="http://www.w3.org/2001/XMLSchema#date">2014-06-15</dct:created>
    <rdfs:comment>The Thesaurus of Geographic Names concept scheme</rdfs:comment>
    <rdfs:seeAlso rdf:resource="http://www.getty.edu/research/tools/vocabularies/lod/"/>
  </rdf:Description>
  <rdf:Description rdf:about="http://vocab.getty.edu/ontology#ulan2794_representative_of">
    <rdf:type rdf:resource="http://www.w3.org/2002/07/owl#ObjectProperty"/>
    <dc:identifier>2794</dc:identifier>
    <rdfs:isDefinedBy rdf:resource="http://vocab.getty.edu/ontology"/>
    <skos:scopeNote>person - representative of - institution.&#13;
Example: The Noguch Museum - representative was Isamu Noguchi</skos:scopeNote>
    <rdfs:domain rdf:resource="http://www.w3.org/2004/02/skos/core#Concept"/>
    <rdfs:range rdf:resource="http://www.w3.org/2004/02/skos/core#Concept"/>
    <dct:description>person - representative of - institution.&#13;
Example: The Noguch Museum - representative was Isamu Noguchi</dct:description>
    <dc:title>representative of - institution</dc:title>
    <owl:inverseOf rdf:resource="http://vocab.getty.edu/ontology#ulan2795_representative_was"/>
    <rdfs:isDefinedBy rdf:resource="http://vocab.getty.edu/ulan/"/>
    <rdfs:subPropertyOf rdf:resource="http://www.w3.org/2004/02/skos/core#related"/>
    <skos:example>The Noguch Museum - representative was Isamu Noguchi</skos:example>
    <skos:prefLabel>ulan2794_representative_of</skos:prefLabel>
  </rdf:Description>
  <rdf:Description rdf:about="http://vocab.getty.edu/ontology#aat2831_associated_with">
    <rdfs:isDefinedBy rdf:resource="http://vocab.getty.edu/aat/"/>
    <rdf:type rdf:resource="http://www.w3.org/2002/07/owl#ObjectProperty"/>
    <skos:scopeNote>genus/species/[other living organism term] - [is] associated with - genus/species.&#13;
Example: Anthonomus grandis (species) [boll weevil] is associated with Gossypium (genus) [cotton]; Amphiprioninae (subfamily) [clown fish] is associated with Actiniaria (order) [sea anemone]</skos:scopeNote>
    <rdfs:isDefinedBy rdf:resource="http://vocab.getty.edu/ontology"/>
    <dct:description>genus/species/[other living organism term] - [is] associated with - genus/species.&#13;
Example: Anthonomus grandis (species) [boll weevil] is associated with Gossypium (genus) [cotton]; Amphiprioninae (subfamily) [clown fish] is associated with Actiniaria (order) [sea anemone]</dct:description>
    <dc:identifier>2831</dc:identifier>
    <rdfs:domain rdf:resource="http://www.w3.org/2004/02/skos/core#Concept"/>
    <dc:title>associated with - genus/species</dc:title>
    <skos:example>Anthonomus grandis (species) [boll weevil] is associated with Gossypium (genus) [cotton]</skos:example>
    <rdfs:range rdf:resource="http://www.w3.org/2004/02/skos/core#Concept"/>
    <rdfs:subPropertyOf rdf:resource="http://www.w3.org/2004/02/skos/core#related"/>
    <skos:prefLabel>aat2831_associated_with</skos:prefLabel>
    <rdf:type rdf:resource="http://www.w3.org/2002/07/owl#SymmetricProperty"/>
    <skos:example>Amphiprioninae (subfamily) [clown fish] is associated with Actiniaria (order) [sea anemone]</skos:example>
  </rdf:Description>
  <rdf:Description rdf:about="http://vocab.getty.edu/ontology#ulan1547_romantic_partner_of">
    <dc:title>romantic partner of - person</dc:title>
    <rdfs:subPropertyOf rdf:resource="http://www.w3.org/2004/02/skos/core#related"/>
    <rdfs:isDefinedBy rdf:resource="http://vocab.getty.edu/ulan/"/>
    <skos:example>Pablo Picasso and Gaby Lespinasse were romantic partners</skos:example>
    <skos:example>Vincent van Gogh and Clasina Hoornik were romantic partners</skos:example>
    <skos:scopeNote>person - romantic partner of - person.&#13;
Example: Pablo Picasso and Gaby Lespinasse were romantic partners; Vincent van Gogh and Clasina Hoornik were romantic partners</skos:scopeNote>
    <dc:identifier>1547</dc:identifier>
    <rdf:type rdf:resource="http://www.w3.org/2002/07/owl#SymmetricProperty"/>
    <rdf:type rdf:resource="http://www.w3.org/2002/07/owl#ObjectProperty"/>
    <rdfs:isDefinedBy rdf:resource="http://vocab.getty.edu/ontology"/>
    <rdfs:domain rdf:resource="http://www.w3.org/2004/02/skos/core#Concept"/>
    <rdfs:range rdf:resource="http://www.w3.org/2004/02/skos/core#Concept"/>
    <dct:description>person - romantic partner of - person.&#13;
Example: Pablo Picasso and Gaby Lespinasse were romantic partners; Vincent van Gogh and Clasina Hoornik were romantic partners</dct:description>
    <skos:prefLabel>ulan1547_romantic_partner_of</skos:prefLabel>
  </rdf:Description>
  <rdf:Description rdf:about="http://vocab.getty.edu/ontology#ulan1582_ancestor_of">
    <rdfs:domain rdf:resource="http://www.w3.org/2004/02/skos/core#Concept"/>
    <dct:description>person - ancestor of - person.&#13;
Example: Paolo Veronese is the ancestor of Paolo Caliari</dct:description>
    <dc:title>ancestor of - person</dc:title>
    <rdfs:subPropertyOf rdf:resource="http://www.w3.org/2004/02/skos/core#related"/>
    <rdfs:range rdf:resource="http://www.w3.org/2004/02/skos/core#Concept"/>
    <rdfs:isDefinedBy rdf:resource="http://vocab.getty.edu/ontology"/>
    <rdf:type rdf:resource="http://www.w3.org/2002/07/owl#ObjectProperty"/>
    <skos:example>Paolo Veronese is the ancestor of Paolo Caliari</skos:example>
    <skos:scopeNote>person - ancestor of - person.&#13;
Example: Paolo Veronese is the ancestor of Paolo Caliari</skos:scopeNote>
    <dc:identifier>1582</dc:identifier>
    <skos:prefLabel>ulan1582_ancestor_of</skos:prefLabel>
    <rdfs:isDefinedBy rdf:resource="http://vocab.getty.edu/ulan/"/>
  </rdf:Description>
  <rdf:Description rdf:about="http://vocab.getty.edu/term/kind/USPSCode">
    <skos:inScheme rdf:resource="http://vocab.getty.edu/term/kind/"/>
    <skos:notation>USPS</skos:notation>
    <dct:description>Used in TGN only.
Example: "CA" for California</dct:description>
    <skos:example>"CA" for California</skos:example>
    <skos:prefLabel>US Postal Service Code</skos:prefLabel>
    <skos:scopeNote>Used in TGN only</skos:scopeNote>
    <rdf:type rdf:resource="http://www.w3.org/2004/02/skos/core#Concept"/>
  </rdf:Description>
  <rdf:Description rdf:about="http://vocab.getty.edu/ontology#PhysPlaceConcept">
    <skos:example>Amazon River (TGN)</skos:example>
    <dct:description>Physical feature, defined by its physical characteristics on planet Earth, including mountains, rivers, and oceans. Used in TGN only.
Example: Amazon River (TGN)</dct:description>
    <skos:definition>Physical feature, defined by its physical characteristics on planet Earth, including mountains, rivers, and oceans. Used in TGN only</skos:definition>
    <rdfs:comment>Physical feature, defined by its physical characteristics on planet Earth, including mountains, rivers, and oceans. Used in TGN only</rdfs:comment>
    <rdfs:label>PhysPlaceConcept</rdfs:label>
    <rdfs:isDefinedBy rdf:resource="http://vocab.getty.edu/ontology"/>
    <rdfs:subClassOf rdf:resource="http://vocab.getty.edu/ontology#Subject"/>
    <skos:prefLabel>PhysPlaceConcept</skos:prefLabel>
    <skos:broader rdf:resource="http://vocab.getty.edu/ontology#Subject"/>
    <rdf:type rdf:resource="http://www.w3.org/2002/07/owl#Class"/>
    <skos:scopeNote>Physical feature, defined by its physical characteristics on planet Earth, including mountains, rivers, and oceans. Used in TGN only.
Example: Amazon River (TGN)</skos:scopeNote>
    <rdfs:subClassOf rdf:resource="http://www.w3.org/2004/02/skos/core#Concept"/>
  </rdf:Description>
  <rdf:Description rdf:about="http://vocab.getty.edu/ontology#aat2892_example_of">
    <rdfs:range rdf:resource="http://www.w3.org/2004/02/skos/core#Concept"/>
    <skos:example>Pictrography (TM) prints are examples of photothermographic transfer prints</skos:example>
    <rdfs:domain rdf:resource="http://www.w3.org/2004/02/skos/core#Concept"/>
    <dc:identifier>2892</dc:identifier>
    <rdfs:isDefinedBy rdf:resource="http://vocab.getty.edu/ontology"/>
    <rdfs:subPropertyOf rdf:resource="http://www.w3.org/2004/02/skos/core#related"/>
    <rdf:type rdf:resource="http://www.w3.org/2002/07/owl#ObjectProperty"/>
    <dct:description>brand name - [is] example of - things.&#13;
Example: Pictrography (TM) prints are examples of photothermographic transfer prints</dct:description>
    <rdfs:isDefinedBy rdf:resource="http://vocab.getty.edu/aat/"/>
    <skos:prefLabel>aat2892_example_of</skos:prefLabel>
    <dc:title>example of - things</dc:title>
    <skos:scopeNote>brand name - [is] example of - things.&#13;
Example: Pictrography (TM) prints are examples of photothermographic transfer prints</skos:scopeNote>
  </rdf:Description>
  <rdf:Description rdf:about="http://vocab.getty.edu/ontology#tgn3611_administrative_dependent_of">
    <rdf:type rdf:resource="http://www.w3.org/2002/07/owl#ObjectProperty"/>
    <rdfs:isDefinedBy rdf:resource="http://vocab.getty.edu/ontology"/>
    <rdfs:range rdf:resource="http://www.w3.org/2004/02/skos/core#Concept"/>
    <rdfs:domain rdf:resource="http://www.w3.org/2004/02/skos/core#Concept"/>
    <dc:title>administrative dependent of - place</dc:title>
    <skos:prefLabel>tgn3611_administrative_dependent_of</skos:prefLabel>
    <dc:identifier>3611</dc:identifier>
    <owl:inverseOf rdf:resource="http://vocab.getty.edu/ontology#tgn3612_administrative_entity_for"/>
    <rdfs:isDefinedBy rdf:resource="http://vocab.getty.edu/tgn/"/>
    <skos:scopeNote>New</skos:scopeNote>
    <dct:description>place - administrative dependent of - place; New.&#13;
Example: Luni (La Spezia province, Liguria, Italy) is the admisistrative dependent of Ortonovo (Massa-Carrara province, Tuscany, Italy)</dct:description>
    <rdfs:subPropertyOf rdf:resource="http://www.w3.org/2004/02/skos/core#related"/>
    <skos:example>Luni (La Spezia province, Liguria, Italy) is the admisistrative dependent of Ortonovo (Massa-Carrara province, Tuscany, Italy)</skos:example>
  </rdf:Description>
  <rdf:Description rdf:about="http://vocab.getty.edu/ontology#aat2815_composed_of">
    <rdf:type rdf:resource="http://www.w3.org/2002/07/owl#ObjectProperty"/>
    <rdfs:isDefinedBy rdf:resource="http://vocab.getty.edu/ontology"/>
    <rdfs:isDefinedBy rdf:resource="http://vocab.getty.edu/aat/"/>
    <skos:scopeNote>material - [is] composed of - material.&#13;
Example: composite white is composed of titanium white; desert varnish is composed of iron oxide</skos:scopeNote>
    <rdfs:domain rdf:resource="http://www.w3.org/2004/02/skos/core#Concept"/>
    <dc:title>composed of - material</dc:title>
    <rdfs:range rdf:resource="http://www.w3.org/2004/02/skos/core#Concept"/>
    <dc:identifier>2815</dc:identifier>
    <dct:description>material - [is] composed of - material.&#13;
Example: composite white is composed of titanium white; desert varnish is composed of iron oxide</dct:description>
    <skos:example>composite white is composed of titanium white</skos:example>
    <skos:example>desert varnish is composed of iron oxide</skos:example>
    <rdfs:subPropertyOf rdf:resource="http://www.w3.org/2004/02/skos/core#related"/>
    <skos:prefLabel>aat2815_composed_of</skos:prefLabel>
  </rdf:Description>
  <rdf:Description rdf:about="http://vocab.getty.edu/ontology#ulan1412_predecessor_of">
    <rdfs:subPropertyOf rdf:resource="http://www.w3.org/2004/02/skos/core#related"/>
    <dct:description>firm/group - predecessor of - firm/group.&#13;
Example: Richard Meier &amp; Associates is the predecessor of Richard Meier &amp; Partners Architects LLP</dct:description>
    <skos:example>Richard Meier &amp; Associates is the predecessor of Richard Meier &amp; Partners Architects LLP</skos:example>
    <dc:identifier>1412</dc:identifier>
    <rdfs:domain rdf:resource="http://www.w3.org/2004/02/skos/core#Concept"/>
    <rdf:type rdf:resource="http://www.w3.org/2002/07/owl#ObjectProperty"/>
    <rdfs:isDefinedBy rdf:resource="http://vocab.getty.edu/ontology"/>
    <dc:title>predecessor of - firm/group</dc:title>
    <skos:scopeNote>firm/group - predecessor of - firm/group.&#13;
Example: Richard Meier &amp; Associates is the predecessor of Richard Meier &amp; Partners Architects LLP</skos:scopeNote>
    <skos:prefLabel>ulan1412_predecessor_of</skos:prefLabel>
    <rdfs:isDefinedBy rdf:resource="http://vocab.getty.edu/ulan/"/>
    <rdfs:range rdf:resource="http://www.w3.org/2004/02/skos/core#Concept"/>
  </rdf:Description>
  <rdf:Description rdf:about="http://vocab.getty.edu/term/POS/PluralNoun">
    <skos:scopeNote>A term that is plural (the same word may be singular in another language)</skos:scopeNote>
    <skos:prefLabel>Plural Noun</skos:prefLabel>
    <skos:inScheme rdf:resource="http://vocab.getty.edu/term/POS/"/>
    <skos:example>"filigrane" is the Italian plural for "watermarks"</skos:example>
    <dct:description>A term that is plural (the same word may be singular in another language).
Example: "filigrane" is the Italian plural for "watermarks"</dct:description>
    <rdf:type rdf:resource="http://www.w3.org/2004/02/skos/core#Concept"/>
    <skos:notation>PN</skos:notation>
  </rdf:Description>
  <rdf:Description rdf:about="http://vocab.getty.edu/ontology#aat2415_required_for">
    <skos:example>pewter is required for pewtersmithing</skos:example>
    <owl:inverseOf rdf:resource="http://vocab.getty.edu/ontology#aat2416_requires"/>
    <rdfs:domain rdf:resource="http://www.w3.org/2004/02/skos/core#Concept"/>
    <dc:identifier>2415</dc:identifier>
    <rdfs:range rdf:resource="http://www.w3.org/2004/02/skos/core#Concept"/>
    <rdfs:isDefinedBy rdf:resource="http://vocab.getty.edu/aat/"/>
    <rdf:type rdf:resource="http://www.w3.org/2002/07/owl#ObjectProperty"/>
    <skos:prefLabel>aat2415_required_for</skos:prefLabel>
    <rdfs:isDefinedBy rdf:resource="http://vocab.getty.edu/ontology"/>
    <skos:example>dye is required for dying</skos:example>
    <skos:scopeNote>material - [is] required for - activity/event/[process/function].&#13;
Example: dye is required for dying; pewter is required for pewtersmithing</skos:scopeNote>
    <rdfs:subPropertyOf rdf:resource="http://www.w3.org/2004/02/skos/core#related"/>
    <dc:title>required for - activity/event</dc:title>
    <dct:description>material - [is] required for - activity/event/[process/function].&#13;
Example: dye is required for dying; pewter is required for pewtersmithing</dct:description>
  </rdf:Description>
  <rdf:Description rdf:about="http://vocab.getty.edu/ontology#ulan1221_appointed_by">
    <rdfs:domain rdf:resource="http://www.w3.org/2004/02/skos/core#Concept"/>
    <rdfs:isDefinedBy rdf:resource="http://vocab.getty.edu/ulan/"/>
    <dc:identifier>1221</dc:identifier>
    <rdfs:subPropertyOf rdf:resource="http://www.w3.org/2004/02/skos/core#related"/>
    <rdfs:isDefinedBy rdf:resource="http://vocab.getty.edu/ontology"/>
    <dct:description>person - appointed by - person.&#13;
Example: Pope Urban VIII appointed Virginio Cesarini</dct:description>
    <skos:example>Pope Urban VIII appointed Virginio Cesarini</skos:example>
    <owl:inverseOf rdf:resource="http://vocab.getty.edu/ontology#ulan1222_appointee_of"/>
    <rdf:type rdf:resource="http://www.w3.org/2002/07/owl#ObjectProperty"/>
    <dc:title>appointed by - person</dc:title>
    <rdfs:range rdf:resource="http://www.w3.org/2004/02/skos/core#Concept"/>
    <skos:prefLabel>ulan1221_appointed_by</skos:prefLabel>
    <skos:scopeNote>person - appointed by - person.&#13;
Example: Pope Urban VIII appointed Virginio Cesarini</skos:scopeNote>
  </rdf:Description>
  <rdf:Description rdf:about="http://vocab.getty.edu/ontology#aat2397_focus_of">
    <dct:description>any - [is] focus of - field [of study]/discipline.&#13;
Example: manuscripts are the focus of codicology; music is the focus of musicology; Plantae (kingdom) is the focus of botany</dct:description>
    <rdfs:isDefinedBy rdf:resource="http://vocab.getty.edu/ontology"/>
    <rdfs:range rdf:resource="http://www.w3.org/2004/02/skos/core#Concept"/>
    <rdfs:domain rdf:resource="http://www.w3.org/2004/02/skos/core#Concept"/>
    <rdfs:subPropertyOf rdf:resource="http://www.w3.org/2004/02/skos/core#related"/>
    <rdf:type rdf:resource="http://www.w3.org/2002/07/owl#ObjectProperty"/>
    <skos:example>music is the focus of musicology</skos:example>
    <skos:scopeNote>any - [is] focus of - field [of study]/discipline.&#13;
Example: manuscripts are the focus of codicology; music is the focus of musicology; Plantae (kingdom) is the focus of botany</skos:scopeNote>
    <skos:example>manuscripts are the focus of codicology</skos:example>
    <dc:identifier>2397</dc:identifier>
    <rdfs:isDefinedBy rdf:resource="http://vocab.getty.edu/aat/"/>
    <owl:inverseOf rdf:resource="http://vocab.getty.edu/ontology#aat2398_focuses_on"/>
    <dc:title>focus of - field/discipline</dc:title>
    <skos:prefLabel>aat2397_focus_of</skos:prefLabel>
    <skos:example>Plantae (kingdom) is the focus of botany</skos:example>
  </rdf:Description>
  <rdf:Description rdf:about="http://vocab.getty.edu/ontology#ulan1202_patron_was">
    <skos:scopeNote>person/firm/family - patron was - person.&#13;
Example: The patron of Donatello was Cosimo I, Grand-Duke of Tuscany</skos:scopeNote>
    <dc:title>patron was - person</dc:title>
    <skos:example>The patron of Donatello was Cosimo I, Grand-Duke of Tuscany</skos:example>
    <rdfs:isDefinedBy rdf:resource="http://vocab.getty.edu/ulan/"/>
    <rdfs:subPropertyOf rdf:resource="http://www.w3.org/2004/02/skos/core#related"/>
    <rdfs:domain rdf:resource="http://www.w3.org/2004/02/skos/core#Concept"/>
    <rdfs:range rdf:resource="http://www.w3.org/2004/02/skos/core#Concept"/>
    <dc:identifier>1202</dc:identifier>
    <skos:prefLabel>ulan1202_patron_was</skos:prefLabel>
    <rdf:type rdf:resource="http://www.w3.org/2002/07/owl#ObjectProperty"/>
    <dct:description>person/firm/family - patron was - person.&#13;
Example: The patron of Donatello was Cosimo I, Grand-Duke of Tuscany</dct:description>
    <rdfs:isDefinedBy rdf:resource="http://vocab.getty.edu/ontology"/>
  </rdf:Description>
  <rdf:Description rdf:about="http://vocab.getty.edu/ontology#aat2418_uses">
    <owl:inverseOf rdf:resource="http://vocab.getty.edu/ontology#aat2419_used_for"/>
    <skos:example>astronomy uses astronomical instruments</skos:example>
    <rdfs:range rdf:resource="http://www.w3.org/2004/02/skos/core#Concept"/>
    <dc:identifier>2418</dc:identifier>
    <skos:scopeNote>field [of study]/discipline - uses - things/[equipment].&#13;
Example: astronomy uses astronomical instruments; divination [discipline] uses divination objects</skos:scopeNote>
    <skos:prefLabel>aat2418_uses</skos:prefLabel>
    <rdfs:isDefinedBy rdf:resource="http://vocab.getty.edu/aat/"/>
    <dc:title>uses - things</dc:title>
    <dct:description>field [of study]/discipline - uses - things/[equipment].&#13;
Example: astronomy uses astronomical instruments; divination [discipline] uses divination objects</dct:description>
    <rdf:type rdf:resource="http://www.w3.org/2002/07/owl#ObjectProperty"/>
    <rdfs:isDefinedBy rdf:resource="http://vocab.getty.edu/ontology"/>
    <rdfs:domain rdf:resource="http://www.w3.org/2004/02/skos/core#Concept"/>
    <rdfs:subPropertyOf rdf:resource="http://www.w3.org/2004/02/skos/core#related"/>
    <skos:example>divination [discipline] uses divination objects</skos:example>
  </rdf:Description>
  <rdf:Description rdf:about="http://vocab.getty.edu/ontology#aat2312_perform">
    <rdfs:isDefinedBy rdf:resource="http://vocab.getty.edu/aat/"/>
    <skos:example>clockmakers perform clockmaking</skos:example>
    <rdfs:isDefinedBy rdf:resource="http://vocab.getty.edu/ontology"/>
    <dc:identifier>2312</dc:identifier>
    <skos:scopeNote>[actors having] a role - perform - activity/event/process.&#13;
Example: clockmakers perform clockmaking; curators perform curating</skos:scopeNote>
    <rdf:type rdf:resource="http://www.w3.org/2002/07/owl#ObjectProperty"/>
    <rdfs:domain rdf:resource="http://www.w3.org/2004/02/skos/core#Concept"/>
    <rdfs:subPropertyOf rdf:resource="http://www.w3.org/2004/02/skos/core#related"/>
    <rdfs:range rdf:resource="http://www.w3.org/2004/02/skos/core#Concept"/>
    <dc:title>perform - activity/event</dc:title>
    <skos:prefLabel>aat2312_perform</skos:prefLabel>
    <skos:example>curators perform curating</skos:example>
    <dct:description>[actors having] a role - perform - activity/event/process.&#13;
Example: clockmakers perform clockmaking; curators perform curating</dct:description>
  </rdf:Description>
  <rdf:Description rdf:about="http://vocab.getty.edu/ontology#aat2507_produce-process">
    <skos:prefLabel>aat2507_produce-process</skos:prefLabel>
    <rdf:type rdf:resource="http://www.w3.org/2002/07/owl#ObjectProperty"/>
    <owl:inverseOf rdf:resource="http://vocab.getty.edu/ontology#aat2508_produced-processed_by"/>
    <dc:identifier>2507</dc:identifier>
    <rdfs:subPropertyOf rdf:resource="http://www.w3.org/2004/02/skos/core#related"/>
    <skos:scopeNote>things/[equipment] - produce/process - material.&#13;
Example: cotton (fiber) is produced/processed by cotton gins; groundwater is produced/processed by water wells</skos:scopeNote>
    <skos:example>groundwater is produced/processed by water wells</skos:example>
    <dc:title>produce/process - material</dc:title>
    <rdfs:range rdf:resource="http://www.w3.org/2004/02/skos/core#Concept"/>
    <rdfs:isDefinedBy rdf:resource="http://vocab.getty.edu/aat/"/>
    <rdfs:domain rdf:resource="http://www.w3.org/2004/02/skos/core#Concept"/>
    <rdfs:isDefinedBy rdf:resource="http://vocab.getty.edu/ontology"/>
    <skos:example>cotton (fiber) is produced/processed by cotton gins</skos:example>
    <dct:description>things/[equipment] - produce/process - material.&#13;
Example: cotton (fiber) is produced/processed by cotton gins; groundwater is produced/processed by water wells</dct:description>
  </rdf:Description>
  <rdf:Description rdf:about="http://vocab.getty.edu/ontology#aat2216_require">
    <rdfs:subPropertyOf rdf:resource="http://www.w3.org/2004/02/skos/core#related"/>
    <dc:title>require - things</dc:title>
    <skos:example>broderie anglaise requires eyelets</skos:example>
    <skos:example>compact disc players require compact discs</skos:example>
    <skos:scopeNote>things - require - things [in order to exist or work].&#13;
Example: broderie anglaise requires eyelets; compact disc players require compact discs</skos:scopeNote>
    <rdfs:domain rdf:resource="http://www.w3.org/2004/02/skos/core#Concept"/>
    <rdfs:isDefinedBy rdf:resource="http://vocab.getty.edu/aat/"/>
    <rdfs:range rdf:resource="http://www.w3.org/2004/02/skos/core#Concept"/>
    <dc:identifier>2216</dc:identifier>
    <dct:description>things - require - things [in order to exist or work].&#13;
Example: broderie anglaise requires eyelets; compact disc players require compact discs</dct:description>
    <skos:prefLabel>aat2216_require</skos:prefLabel>
    <rdf:type rdf:resource="http://www.w3.org/2002/07/owl#ObjectProperty"/>
    <rdfs:isDefinedBy rdf:resource="http://vocab.getty.edu/ontology"/>
  </rdf:Description>
  <rdf:Description rdf:about="http://vocab.getty.edu/ontology#ulan1575_godchild_of">
    <dc:title>godchild of - person</dc:title>
    <dc:identifier>1575</dc:identifier>
    <rdfs:isDefinedBy rdf:resource="http://vocab.getty.edu/ulan/"/>
    <skos:prefLabel>ulan1575_godchild_of</skos:prefLabel>
    <rdfs:subPropertyOf rdf:resource="http://www.w3.org/2004/02/skos/core#related"/>
    <skos:scopeNote>person - godchild of - person.&#13;
Example: Jean I Nocret is the godchild of Jean-Baptiste Goy</skos:scopeNote>
    <skos:example>Jean I Nocret is the godchild of Jean-Baptiste Goy</skos:example>
    <rdfs:domain rdf:resource="http://www.w3.org/2004/02/skos/core#Concept"/>
    <rdfs:range rdf:resource="http://www.w3.org/2004/02/skos/core#Concept"/>
    <rdf:type rdf:resource="http://www.w3.org/2002/07/owl#ObjectProperty"/>
    <rdfs:isDefinedBy rdf:resource="http://vocab.getty.edu/ontology"/>
    <dct:description>person - godchild of - person.&#13;
Example: Jean I Nocret is the godchild of Jean-Baptiste Goy</dct:description>
  </rdf:Description>
  <rdf:Description rdf:about="http://vocab.getty.edu/ontology#ulan1562_step-parent_of">
    <skos:example>Napoleon I, Emperor of the French is the step-parent of Hortense, Quene consort of Louis Bonaparte</skos:example>
    <skos:scopeNote>person - step-parent of - person.&#13;
Example: Napoleon I, Emperor of the French is the step-parent of Hortense, Quene consort of Louis Bonaparte</skos:scopeNote>
    <dc:title>step-parent of - person</dc:title>
    <rdfs:isDefinedBy rdf:resource="http://vocab.getty.edu/ulan/"/>
    <rdfs:subPropertyOf rdf:resource="http://www.w3.org/2004/02/skos/core#related"/>
    <rdfs:range rdf:resource="http://www.w3.org/2004/02/skos/core#Concept"/>
    <rdfs:domain rdf:resource="http://www.w3.org/2004/02/skos/core#Concept"/>
    <rdf:type rdf:resource="http://www.w3.org/2002/07/owl#ObjectProperty"/>
    <skos:prefLabel>ulan1562_step-parent_of</skos:prefLabel>
    <rdfs:isDefinedBy rdf:resource="http://vocab.getty.edu/ontology"/>
    <dc:identifier>1562</dc:identifier>
    <dct:description>person - step-parent of - person.&#13;
Example: Napoleon I, Emperor of the French is the step-parent of Hortense, Quene consort of Louis Bonaparte</dct:description>
  </rdf:Description>
  <rdf:Description rdf:about="http://vocab.getty.edu/ontology#aat2508_produced-processed_by">
    <skos:example>cotton gins produce/process cotton (fiber)</skos:example>
    <dc:identifier>2508</dc:identifier>
    <rdfs:subPropertyOf rdf:resource="http://www.w3.org/2004/02/skos/core#related"/>
    <skos:example>waterwells produce/process groundwater</skos:example>
    <dct:description>material - [is] produced/processed by - things/[equipment].&#13;
Example: cotton gins produce/process cotton (fiber); waterwells produce/process groundwater</dct:description>
    <dc:title>produced/processed by - things</dc:title>
    <skos:scopeNote>material - [is] produced/processed by - things/[equipment].&#13;
Example: cotton gins produce/process cotton (fiber); waterwells produce/process groundwater</skos:scopeNote>
    <rdfs:domain rdf:resource="http://www.w3.org/2004/02/skos/core#Concept"/>
    <rdfs:range rdf:resource="http://www.w3.org/2004/02/skos/core#Concept"/>
    <skos:prefLabel>aat2508_produced-processed_by</skos:prefLabel>
    <rdfs:isDefinedBy rdf:resource="http://vocab.getty.edu/aat/"/>
    <rdf:type rdf:resource="http://www.w3.org/2002/07/owl#ObjectProperty"/>
    <rdfs:isDefinedBy rdf:resource="http://vocab.getty.edu/ontology"/>
  </rdf:Description>
  <rdf:Description rdf:about="http://vocab.getty.edu/ontology#aat2215_required_for">
    <rdfs:subPropertyOf rdf:resource="http://www.w3.org/2004/02/skos/core#related"/>
    <skos:prefLabel>aat2215_required_for</skos:prefLabel>
    <owl:inverseOf rdf:resource="http://vocab.getty.edu/ontology#aat2216_require"/>
    <rdfs:domain rdf:resource="http://www.w3.org/2004/02/skos/core#Concept"/>
    <skos:example>compact discs are required for compact disc players</skos:example>
    <skos:scopeNote>things - [are] required for -  things.&#13;
Example: eyelets are required for broderie anglaise; compact discs are required for compact disc players</skos:scopeNote>
    <rdfs:isDefinedBy rdf:resource="http://vocab.getty.edu/aat/"/>
    <dct:description>things - [are] required for -  things.&#13;
Example: eyelets are required for broderie anglaise; compact discs are required for compact disc players</dct:description>
    <rdfs:isDefinedBy rdf:resource="http://vocab.getty.edu/ontology"/>
    <dc:title>required for - things</dc:title>
    <rdf:type rdf:resource="http://www.w3.org/2002/07/owl#ObjectProperty"/>
    <skos:example>eyelets are required for broderie anglaise</skos:example>
    <dc:identifier>2215</dc:identifier>
    <rdfs:range rdf:resource="http://www.w3.org/2004/02/skos/core#Concept"/>
  </rdf:Description>
  <rdf:Description rdf:about="http://vocab.getty.edu/ontology#aat2329_involves">
    <dct:description>things - involve - [actors having] role.&#13;
Example: portraits involve sitters; motion pictures (visual works) involve actors (performing artists)</dct:description>
    <rdfs:isDefinedBy rdf:resource="http://vocab.getty.edu/aat/"/>
    <dc:title>involves - role</dc:title>
    <skos:scopeNote>things - involve - [actors having] role.&#13;
Example: portraits involve sitters; motion pictures (visual works) involve actors (performing artists)</skos:scopeNote>
    <skos:example>motion pictures (visual works) involve actors (performing artists)</skos:example>
    <rdfs:range rdf:resource="http://www.w3.org/2004/02/skos/core#Concept"/>
    <rdfs:domain rdf:resource="http://www.w3.org/2004/02/skos/core#Concept"/>
    <rdfs:isDefinedBy rdf:resource="http://vocab.getty.edu/ontology"/>
    <skos:example>portraits involve sitters</skos:example>
    <dc:identifier>2329</dc:identifier>
    <rdfs:subPropertyOf rdf:resource="http://www.w3.org/2004/02/skos/core#related"/>
    <rdf:type rdf:resource="http://www.w3.org/2002/07/owl#ObjectProperty"/>
    <skos:prefLabel>aat2329_involves</skos:prefLabel>
  </rdf:Description>
  <rdf:Description rdf:about="http://vocab.getty.edu/ontology#aat2836_derived-made_from">
    <dct:description>things - [are] derived/made from - genus/species [or its parts].&#13;
Example: k?kaku are derived/made from Phormium tenax (species); ostrich-egg cups are derived/made from Struthio camelus (species)</dct:description>
    <skos:scopeNote>things - [are] derived/made from - genus/species [or its parts].&#13;
Example: k?kaku are derived/made from Phormium tenax (species); ostrich-egg cups are derived/made from Struthio camelus (species)</skos:scopeNote>
    <dc:identifier>2836</dc:identifier>
    <rdfs:subPropertyOf rdf:resource="http://www.w3.org/2004/02/skos/core#related"/>
    <rdfs:range rdf:resource="http://www.w3.org/2004/02/skos/core#Concept"/>
    <rdfs:domain rdf:resource="http://www.w3.org/2004/02/skos/core#Concept"/>
    <dc:title>derived/made from - genus/species</dc:title>
    <owl:inverseOf rdf:resource="http://vocab.getty.edu/ontology#aat2837_source_for"/>
    <skos:example>k?kaku are derived/made from Phormium tenax (species)</skos:example>
    <skos:example>ostrich-egg cups are derived/made from Struthio camelus (species)</skos:example>
    <rdf:type rdf:resource="http://www.w3.org/2002/07/owl#ObjectProperty"/>
    <skos:prefLabel>aat2836_derived-made_from</skos:prefLabel>
    <rdfs:isDefinedBy rdf:resource="http://vocab.getty.edu/ontology"/>
    <rdfs:isDefinedBy rdf:resource="http://vocab.getty.edu/aat/"/>
  </rdf:Description>
  <rdf:Description rdf:about="http://vocab.getty.edu/ontology#tgn3401_moved_from">
    <skos:example>Troupville, Georgia, USA was moved to Valdosta (Lowndes county, Georgia, USA)</skos:example>
    <owl:inverseOf rdf:resource="http://vocab.getty.edu/ontology#tgn3402_moved_to"/>
    <rdf:type rdf:resource="http://www.w3.org/2002/07/owl#ObjectProperty"/>
    <skos:scopeNote>Note: places that were physically moved from one location to another, often due to the threat or occurrence of natural disaster.</skos:scopeNote>
    <rdfs:isDefinedBy rdf:resource="http://vocab.getty.edu/ontology"/>
    <rdfs:range rdf:resource="http://www.w3.org/2004/02/skos/core#Concept"/>
    <dct:description>place - moved from - place; Note: places that were physically moved from one location to another, often due to the threat or occurrence of natural disaster..&#13;
Example: Troupville, Georgia, USA was moved to Valdosta (Lowndes county, Georgia, USA)</dct:description>
    <rdfs:domain rdf:resource="http://www.w3.org/2004/02/skos/core#Concept"/>
    <rdfs:subPropertyOf rdf:resource="http://www.w3.org/2004/02/skos/core#related"/>
    <skos:prefLabel>tgn3401_moved_from</skos:prefLabel>
    <dc:title>moved from - place</dc:title>
    <rdfs:isDefinedBy rdf:resource="http://vocab.getty.edu/tgn/"/>
    <dc:identifier>3401</dc:identifier>
  </rdf:Description>
  <rdf:Description rdf:about="http://vocab.getty.edu/ontology#ulan2795_representative_was">
    <rdf:type rdf:resource="http://www.w3.org/2002/07/owl#ObjectProperty"/>
    <dc:identifier>2795</dc:identifier>
    <rdfs:range rdf:resource="http://www.w3.org/2004/02/skos/core#Concept"/>
    <rdfs:isDefinedBy rdf:resource="http://vocab.getty.edu/ulan/"/>
    <skos:example>The Noguch Museum - representative was Isamu Noguchi</skos:example>
    <dc:title>representative was - person</dc:title>
    <rdfs:subPropertyOf rdf:resource="http://www.w3.org/2004/02/skos/core#related"/>
    <dct:description>institution - representative was - person.&#13;
Example: The Noguch Museum - representative was Isamu Noguchi</dct:description>
    <skos:scopeNote>institution - representative was - person.&#13;
Example: The Noguch Museum - representative was Isamu Noguchi</skos:scopeNote>
    <rdfs:domain rdf:resource="http://www.w3.org/2004/02/skos/core#Concept"/>
    <rdfs:isDefinedBy rdf:resource="http://vocab.getty.edu/ontology"/>
    <skos:prefLabel>ulan2795_representative_was</skos:prefLabel>
  </rdf:Description>
  <rdf:Description rdf:about="http://vocab.getty.edu/ontology#ulan1309_advisor_of">
    <dc:identifier>1309</dc:identifier>
    <rdf:type rdf:resource="http://www.w3.org/2002/07/owl#ObjectProperty"/>
    <rdfs:domain rdf:resource="http://www.w3.org/2004/02/skos/core#Concept"/>
    <dct:description>person - advisor of - person.&#13;
Example: Thomas Cromwell, Earl of Essex was the advisor of Henry VIII, King of England</dct:description>
    <dc:title>advisor of - person</dc:title>
    <skos:scopeNote>person - advisor of - person.&#13;
Example: Thomas Cromwell, Earl of Essex was the advisor of Henry VIII, King of England</skos:scopeNote>
    <rdfs:range rdf:resource="http://www.w3.org/2004/02/skos/core#Concept"/>
    <rdfs:isDefinedBy rdf:resource="http://vocab.getty.edu/ulan/"/>
    <owl:inverseOf rdf:resource="http://vocab.getty.edu/ontology#ulan1310_advised_by"/>
    <skos:example>Thomas Cromwell, Earl of Essex was the advisor of Henry VIII, King of England</skos:example>
    <skos:prefLabel>ulan1309_advisor_of</skos:prefLabel>
    <rdfs:subPropertyOf rdf:resource="http://www.w3.org/2004/02/skos/core#related"/>
    <rdfs:isDefinedBy rdf:resource="http://vocab.getty.edu/ontology"/>
  </rdf:Description>
  <rdf:Description rdf:about="http://vocab.getty.edu/ontology#aat2826_used_with">
    <skos:prefLabel>aat2826_used_with</skos:prefLabel>
    <rdf:type rdf:resource="http://www.w3.org/2002/07/owl#ObjectProperty"/>
    <rdfs:isDefinedBy rdf:resource="http://vocab.getty.edu/ontology"/>
    <skos:example>arriccio is used with intonaco</skos:example>
    <dc:title>used with - material</dc:title>
    <rdfs:isDefinedBy rdf:resource="http://vocab.getty.edu/aat/"/>
    <skos:scopeNote>material - [is] used with - material.&#13;
Example: watercolor paper is used with watercolor (paint); arriccio is used with intonaco</skos:scopeNote>
    <rdfs:range rdf:resource="http://www.w3.org/2004/02/skos/core#Concept"/>
    <dct:description>material - [is] used with - material.&#13;
Example: watercolor paper is used with watercolor (paint); arriccio is used with intonaco</dct:description>
    <rdfs:domain rdf:resource="http://www.w3.org/2004/02/skos/core#Concept"/>
    <skos:example>watercolor paper is used with watercolor (paint)</skos:example>
    <dc:identifier>2826</dc:identifier>
    <rdfs:subPropertyOf rdf:resource="http://www.w3.org/2004/02/skos/core#related"/>
    <rdf:type rdf:resource="http://www.w3.org/2002/07/owl#SymmetricProperty"/>
  </rdf:Description>
  <rdf:Description rdf:about="http://vocab.getty.edu/ontology#tgn3005_possibly_identified_as">
    <skos:prefLabel>tgn3005_possibly_identified_as</skos:prefLabel>
    <rdfs:isDefinedBy rdf:resource="http://vocab.getty.edu/ontology"/>
    <rdfs:range rdf:resource="http://www.w3.org/2004/02/skos/core#Concept"/>
    <rdfs:domain rdf:resource="http://www.w3.org/2004/02/skos/core#Concept"/>
    <skos:scopeNote>place - possibly identified as - place.&#13;
Example: The lost settlement of Sharuhen is possibly identified as Tel el-Far'ah (As Suwayda', Syria) (deserted settlement)</skos:scopeNote>
    <skos:example>The lost settlement of Sharuhen is possibly identified as Tel el-Far'ah (As Suwayda', Syria) (deserted settlement)</skos:example>
    <dc:title>possibly identified as - place</dc:title>
    <dc:identifier>3005</dc:identifier>
    <rdfs:isDefinedBy rdf:resource="http://vocab.getty.edu/tgn/"/>
    <rdfs:subPropertyOf rdf:resource="http://www.w3.org/2004/02/skos/core#related"/>
    <dct:description>place - possibly identified as - place.&#13;
Example: The lost settlement of Sharuhen is possibly identified as Tel el-Far'ah (As Suwayda', Syria) (deserted settlement)</dct:description>
    <rdf:type rdf:resource="http://www.w3.org/2002/07/owl#ObjectProperty"/>
    <rdf:type rdf:resource="http://www.w3.org/2002/07/owl#SymmetricProperty"/>
  </rdf:Description>
  <rdf:Description rdf:about="http://vocab.getty.edu/ontology#ulan1224_crowned">
    <rdfs:subPropertyOf rdf:resource="http://www.w3.org/2004/02/skos/core#related"/>
    <rdfs:domain rdf:resource="http://www.w3.org/2004/02/skos/core#Concept"/>
    <rdfs:range rdf:resource="http://www.w3.org/2004/02/skos/core#Concept"/>
    <rdf:type rdf:resource="http://www.w3.org/2002/07/owl#ObjectProperty"/>
    <rdfs:isDefinedBy rdf:resource="http://vocab.getty.edu/ontology"/>
    <dc:title>crowned - person</dc:title>
    <skos:prefLabel>ulan1224_crowned</skos:prefLabel>
    <dct:description>person - crowned - person.&#13;
Example: Emperor Charlemagne was crowned by Pope Leo III</dct:description>
    <skos:example>Emperor Charlemagne was crowned by Pope Leo III</skos:example>
    <skos:scopeNote>person - crowned - person.&#13;
Example: Emperor Charlemagne was crowned by Pope Leo III</skos:scopeNote>
    <dc:identifier>1224</dc:identifier>
    <rdfs:isDefinedBy rdf:resource="http://vocab.getty.edu/ulan/"/>
  </rdf:Description>
  <rdf:Description rdf:about="http://vocab.getty.edu/ontology#aat2428_produces">
    <skos:example>forging (copying) produces forgeries</skos:example>
    <rdfs:isDefinedBy rdf:resource="http://vocab.getty.edu/aat/"/>
    <skos:scopeNote>activity/event/process - produces - things.&#13;
Example: vase painting (image making) produces vase paintings (visual works); forging (copying) produces forgeries</skos:scopeNote>
    <rdfs:domain rdf:resource="http://www.w3.org/2004/02/skos/core#Concept"/>
    <rdfs:range rdf:resource="http://www.w3.org/2004/02/skos/core#Concept"/>
    <skos:prefLabel>aat2428_produces</skos:prefLabel>
    <skos:example>vase painting (image making) produces vase paintings (visual works)</skos:example>
    <dc:identifier>2428</dc:identifier>
    <rdfs:subPropertyOf rdf:resource="http://www.w3.org/2004/02/skos/core#related"/>
    <rdfs:isDefinedBy rdf:resource="http://vocab.getty.edu/ontology"/>
    <dct:description>activity/event/process - produces - things.&#13;
Example: vase painting (image making) produces vase paintings (visual works); forging (copying) produces forgeries</dct:description>
    <dc:title>produces - things</dc:title>
    <rdf:type rdf:resource="http://www.w3.org/2002/07/owl#ObjectProperty"/>
  </rdf:Description>
  <rdf:Description rdf:about="http://vocab.getty.edu/ontology#ulan1541_spouse_of">
    <rdf:type rdf:resource="http://www.w3.org/2002/07/owl#SymmetricProperty"/>
    <rdfs:isDefinedBy rdf:resource="http://vocab.getty.edu/ulan/"/>
    <dc:title>spouse of - person</dc:title>
    <skos:scopeNote>person - spouse of - person.&#13;
Example: Alfred Stieglitz and Georgia O'Keeffe were married to each other</skos:scopeNote>
    <rdfs:range rdf:resource="http://www.w3.org/2004/02/skos/core#Concept"/>
    <rdfs:domain rdf:resource="http://www.w3.org/2004/02/skos/core#Concept"/>
    <skos:prefLabel>ulan1541_spouse_of</skos:prefLabel>
    <rdfs:subPropertyOf rdf:resource="http://www.w3.org/2004/02/skos/core#related"/>
    <rdfs:isDefinedBy rdf:resource="http://vocab.getty.edu/ontology"/>
    <dc:identifier>1541</dc:identifier>
    <skos:example>Alfred Stieglitz and Georgia O'Keeffe were married to each other</skos:example>
    <rdf:type rdf:resource="http://www.w3.org/2002/07/owl#ObjectProperty"/>
    <dct:description>person - spouse of - person.&#13;
Example: Alfred Stieglitz and Georgia O'Keeffe were married to each other</dct:description>
  </rdf:Description>
  <rdf:Description rdf:about="http://vocab.getty.edu/ontology#ulan1101_teacher_of">
    <rdfs:isDefinedBy rdf:resource="http://vocab.getty.edu/ontology"/>
    <owl:inverseOf rdf:resource="http://vocab.getty.edu/ontology#ulan1102_student_of"/>
    <dc:identifier>1101</dc:identifier>
    <rdf:type rdf:resource="http://www.w3.org/2002/07/owl#ObjectProperty"/>
    <dct:description>person - teacher of - person.&#13;
Example: Rivalz, Antoine was the teacher of Pierre Subleyras</dct:description>
    <skos:example>Rivalz, Antoine was the teacher of Pierre Subleyras</skos:example>
    <rdfs:isDefinedBy rdf:resource="http://vocab.getty.edu/ulan/"/>
    <rdfs:range rdf:resource="http://www.w3.org/2004/02/skos/core#Concept"/>
    <rdfs:subPropertyOf rdf:resource="http://www.w3.org/2004/02/skos/core#related"/>
    <rdfs:domain rdf:resource="http://www.w3.org/2004/02/skos/core#Concept"/>
    <skos:scopeNote>person - teacher of - person.&#13;
Example: Rivalz, Antoine was the teacher of Pierre Subleyras</skos:scopeNote>
    <skos:prefLabel>ulan1101_teacher_of</skos:prefLabel>
    <dc:title>teacher of - person</dc:title>
  </rdf:Description>
  <rdf:Description rdf:about="http://vocab.getty.edu/ontology#sourcePreferred">
    <rdfs:subPropertyOf rdf:resource="http://purl.org/dc/terms/source"/>
    <skos:definition>Source for which the term is Preferred. Range is bibo:Document or bibo:DocumentPart</skos:definition>
    <skos:scopeNote>Source for which the term is Preferred. Range is bibo:Document or bibo:DocumentPart.
Example: "Isfahan" is preferred in Webster's New Geographical Dictionary (1988)</skos:scopeNote>
    <skos:prefLabel>sourcePreferred</skos:prefLabel>
    <rdfs:range rdf:resource="http://purl.org/ontology/bibo/Document"/>
    <rdfs:label>sourcePreferred</rdfs:label>
    <skos:example>"Isfahan" is preferred in Webster's New Geographical Dictionary (1988)</skos:example>
    <rdf:type rdf:resource="http://www.w3.org/2002/07/owl#ObjectProperty"/>
    <rdfs:isDefinedBy rdf:resource="http://vocab.getty.edu/ontology"/>
    <rdfs:comment>Source for which the term is Preferred. Range is bibo:Document or bibo:DocumentPart</rdfs:comment>
    <dct:description>Source for which the term is Preferred. Range is bibo:Document or bibo:DocumentPart.
Example: "Isfahan" is preferred in Webster's New Geographical Dictionary (1988)</dct:description>
    <rdfs:domain rdf:resource="http://www.w3.org/2008/05/skos-xl#Label"/>
  </rdf:Description>
  <rdf:Description rdf:about="http://vocab.getty.edu/ontology#ulan1315_principal_in">
    <skos:example>Principal in Fontana Workshop was Orazio Fontana</skos:example>
    <dc:title>principal in - firm</dc:title>
    <owl:inverseOf rdf:resource="http://vocab.getty.edu/ontology#ulan1316_principal_was"/>
    <dct:description>person - principal in - firm.&#13;
Example: Principal in Fontana Workshop was Orazio Fontana</dct:description>
    <rdfs:isDefinedBy rdf:resource="http://vocab.getty.edu/ulan/"/>
    <rdfs:range rdf:resource="http://www.w3.org/2004/02/skos/core#Concept"/>
    <rdfs:domain rdf:resource="http://www.w3.org/2004/02/skos/core#Concept"/>
    <rdfs:subPropertyOf rdf:resource="http://www.w3.org/2004/02/skos/core#related"/>
    <rdfs:isDefinedBy rdf:resource="http://vocab.getty.edu/ontology"/>
    <dc:identifier>1315</dc:identifier>
    <skos:scopeNote>person - principal in - firm.&#13;
Example: Principal in Fontana Workshop was Orazio Fontana</skos:scopeNote>
    <rdf:type rdf:resource="http://www.w3.org/2002/07/owl#ObjectProperty"/>
    <skos:prefLabel>ulan1315_principal_in</skos:prefLabel>
  </rdf:Description>
  <rdf:Description rdf:about="http://vocab.getty.edu/ontology#broader">
    <rdfs:isDefinedBy rdf:resource="http://vocab.getty.edu/ontology"/>
    <rdfs:comment>Parents of a subject. Each broader is also Preferred|NonPreferred and Partitive|Instantial|Generic</rdfs:comment>
    <rdf:type rdf:resource="http://www.w3.org/2002/07/owl#ObjectProperty"/>
    <skos:prefLabel>broader</skos:prefLabel>
    <skos:definition>Parents of a subject. Each broader is also Preferred|NonPreferred and Partitive|Instantial|Generic</skos:definition>
    <rdfs:label>broader</rdfs:label>
    <skos:scopeNote>Parents of a subject. Each broader is also Preferred|NonPreferred and Partitive|Instantial|Generic</skos:scopeNote>
    <rdfs:domain rdf:resource="http://vocab.getty.edu/ontology#Subject"/>
    <rdfs:range rdf:resource="http://vocab.getty.edu/ontology#Subject"/>
    <dct:description>Parents of a subject. Each broader is also Preferred|NonPreferred and Partitive|Instantial|Generic</dct:description>
  </rdf:Description>
  <rdf:Description rdf:about="http://vocab.getty.edu/aat/">
    <vann:preferredNamespacePrefix>aat</vann:preferredNamespacePrefix>
    <dct:creator rdf:resource="http://www.ontotext.com"/>
    <skos:prefLabel>Art and Architecture Thesaurus</skos:prefLabel>
    <rdfs:seeAlso rdf:resource="http://vocab.getty.edu/"/>
    <rdfs:label>Art and Architecture Thesaurus</rdfs:label>
    <vann:preferredNamespaceUri>http://vocab.getty.edu/aat/</vann:preferredNamespaceUri>
    <skos:definition>The Art and Architecture Thesaurus concept scheme</skos:definition>
    <rdf:type rdf:resource="http://www.w3.org/2004/02/skos/core#ConceptScheme"/>
    <rdfs:comment>The Art and Architecture Thesaurus concept scheme</rdfs:comment>
    <rdfs:seeAlso rdf:resource="http://vocab.getty.edu/.well-known/void"/>
    <rdfs:seeAlso rdf:resource="http://www.getty.edu/research/tools/vocabularies/lod/"/>
    <dct:creator rdf:resource="http://www.getty.edu/research/"/>
    <foaf:homepage rdf:resource="http://www.getty.edu/research/tools/vocabularies/aat/"/>
    <dct:created rdf:datatype="http://www.w3.org/2001/XMLSchema#date">2014-02-20</dct:created>
  </rdf:Description>
  <rdf:Description rdf:about="http://vocab.getty.edu/ontology#aat2551_reflect-produced_by">
    <skos:scopeNote>things - reflect/[are] produced by - style/period/culture/[religion/ideology].&#13;
Example: Nasca lines reflect/are produced by Nasca [culture]; Judaica reflects/is produced by Judaism</skos:scopeNote>
    <dc:identifier>2551</dc:identifier>
    <dc:title>reflect/produced by - style/period/culture</dc:title>
    <skos:prefLabel>aat2551_reflect-produced_by</skos:prefLabel>
    <rdfs:range rdf:resource="http://www.w3.org/2004/02/skos/core#Concept"/>
    <skos:example>Nasca lines reflect/are produced by Nasca [culture]</skos:example>
    <skos:example>Judaica reflects/is produced by Judaism</skos:example>
    <rdfs:domain rdf:resource="http://www.w3.org/2004/02/skos/core#Concept"/>
    <rdfs:subPropertyOf rdf:resource="http://www.w3.org/2004/02/skos/core#related"/>
    <rdf:type rdf:resource="http://www.w3.org/2002/07/owl#ObjectProperty"/>
    <rdfs:isDefinedBy rdf:resource="http://vocab.getty.edu/ontology"/>
    <rdfs:isDefinedBy rdf:resource="http://vocab.getty.edu/aat/"/>
    <dct:description>things - reflect/[are] produced by - style/period/culture/[religion/ideology].&#13;
Example: Nasca lines reflect/are produced by Nasca [culture]; Judaica reflects/is produced by Judaism</dct:description>
    <owl:inverseOf rdf:resource="http://vocab.getty.edu/ontology#aat2552_reflected_in-produces"/>
  </rdf:Description>
  <rdf:Description rdf:about="http://vocab.getty.edu/ontology#aat2824_has_parallels_with">
    <rdfs:isDefinedBy rdf:resource="http://vocab.getty.edu/aat/"/>
    <rdfs:isDefinedBy rdf:resource="http://vocab.getty.edu/ontology"/>
    <skos:example>Lagozza [culture] has parallels with Chasseen [culture]</skos:example>
    <skos:example>Gnathian (pottery style) has parallels with West Slope (pottery style)</skos:example>
    <rdf:type rdf:resource="http://www.w3.org/2002/07/owl#ObjectProperty"/>
    <dc:identifier>2824</dc:identifier>
    <dc:title>has parallels with - style/period/culture</dc:title>
    <rdfs:range rdf:resource="http://www.w3.org/2004/02/skos/core#Concept"/>
    <rdfs:subPropertyOf rdf:resource="http://www.w3.org/2004/02/skos/core#related"/>
    <rdfs:domain rdf:resource="http://www.w3.org/2004/02/skos/core#Concept"/>
    <dct:description>style/period/culture/[religion/ideology] - has parallels with - style/period/culture/[religion/ideology].&#13;
Example: Lagozza [culture] has parallels with Chasseen [culture];  Gnathian (pottery style) has parallels with West Slope (pottery style)</dct:description>
    <rdf:type rdf:resource="http://www.w3.org/2002/07/owl#SymmetricProperty"/>
    <skos:scopeNote>style/period/culture/[religion/ideology] - has parallels with - style/period/culture/[religion/ideology].&#13;
Example: Lagozza [culture] has parallels with Chasseen [culture];  Gnathian (pottery style) has parallels with West Slope (pottery style)</skos:scopeNote>
    <skos:prefLabel>aat2824_has_parallels_with</skos:prefLabel>
  </rdf:Description>
  <rdf:Description rdf:about="http://vocab.getty.edu/ontology#parentString">
    <skos:prefLabel>parentString</skos:prefLabel>
    <rdfs:isDefinedBy rdf:resource="http://vocab.getty.edu/ontology"/>
    <skos:scopeNote>Preferred labels of *all* of the subject's preferred ancestors, listed bottom up. Useful to show the subject's full context.
Display version of gvp:broaderPreferredExtended.
For aat:300226882 baking dishes: bakeware, &lt;vessels for cooking food&gt;, &lt;containers for cooking food&gt;, &lt;culinary containers&gt;, &lt;containers by function or context&gt;, containers (receptacles), Containers (Hierarchy Name), Furnishings and Equipment (Hierarchy Name), Objects Facet</skos:scopeNote>
    <rdfs:label>parentString</rdfs:label>
    <rdfs:domain rdf:resource="http://vocab.getty.edu/ontology#Subject"/>
    <skos:example>For aat:300226882 baking dishes: bakeware, &lt;vessels for cooking food&gt;, &lt;containers for cooking food&gt;, &lt;culinary containers&gt;, &lt;containers by function or context&gt;, containers (receptacles), Containers (Hierarchy Name), Furnishings and Equipment (Hierarchy Name), Objects Facet</skos:example>
    <rdfs:range rdf:resource="http://www.w3.org/1999/02/22-rdf-syntax-ns#Literal"/>
    <rdfs:comment>Preferred labels of *all* of the subject's preferred ancestors, listed bottom up. Useful to show the subject's full context</rdfs:comment>
    <dct:description>Preferred labels of *all* of the subject's preferred ancestors, listed bottom up. Useful to show the subject's full context.
Display version of gvp:broaderPreferredExtended.
For aat:300226882 baking dishes: bakeware, &lt;vessels for cooking food&gt;, &lt;containers for cooking food&gt;, &lt;culinary containers&gt;, &lt;containers by function or context&gt;, containers (receptacles), Containers (Hierarchy Name), Furnishings and Equipment (Hierarchy Name), Objects Facet</dct:description>
    <skos:definition>Preferred labels of *all* of the subject's preferred ancestors, listed bottom up. Useful to show the subject's full context</skos:definition>
    <skos:note>Display version of gvp:broaderPreferredExtended</skos:note>
    <rdf:type rdf:resource="http://www.w3.org/2002/07/owl#DatatypeProperty"/>
  </rdf:Description>
  <rdf:Description rdf:about="http://vocab.getty.edu/ontology#ulan1308_assisted_by">
    <rdf:type rdf:resource="http://www.w3.org/2002/07/owl#ObjectProperty"/>
    <skos:scopeNote>person - assisted by - person.&#13;
Example: Pablo Picasso was assisted by Bernard Castelli</skos:scopeNote>
    <skos:example>Pablo Picasso was assisted by Bernard Castelli</skos:example>
    <rdfs:isDefinedBy rdf:resource="http://vocab.getty.edu/ulan/"/>
    <rdfs:subPropertyOf rdf:resource="http://www.w3.org/2004/02/skos/core#related"/>
    <skos:prefLabel>ulan1308_assisted_by</skos:prefLabel>
    <dct:description>person - assisted by - person.&#13;
Example: Pablo Picasso was assisted by Bernard Castelli</dct:description>
    <dc:title>assisted by - person</dc:title>
    <rdfs:domain rdf:resource="http://www.w3.org/2004/02/skos/core#Concept"/>
    <dc:identifier>1308</dc:identifier>
    <rdfs:range rdf:resource="http://www.w3.org/2004/02/skos/core#Concept"/>
    <rdfs:isDefinedBy rdf:resource="http://vocab.getty.edu/ontology"/>
  </rdf:Description>
  <rdf:Description rdf:about="http://vocab.getty.edu/ontology#agentTypePreferred">
    <skos:scopeNote>The primary type of a ULAN Person or Corporate body. Domain is ULAN concept, range is AAT concept.
Example: The preferred type of "Albrecht Duerer Workshop" (ULAN) is "workshop" (AAT)</skos:scopeNote>
    <rdfs:domain rdf:resource="http://vocab.getty.edu/ontology#Subject"/>
    <rdfs:range rdf:resource="http://vocab.getty.edu/ontology#Subject"/>
    <skos:example>The preferred type of "Albrecht Duerer Workshop" (ULAN) is "workshop" (AAT)</skos:example>
    <rdfs:subPropertyOf rdf:resource="http://vocab.getty.edu/ontology#agentType"/>
    <dct:description>The primary type of a ULAN Person or Corporate body. Domain is ULAN concept, range is AAT concept.
Example: The preferred type of "Albrecht Duerer Workshop" (ULAN) is "workshop" (AAT)</dct:description>
    <skos:prefLabel>agentTypePreferred</skos:prefLabel>
    <rdfs:comment>The primary type of a ULAN Person or Corporate body. Domain is ULAN concept, range is AAT concept</rdfs:comment>
    <rdf:type rdf:resource="http://www.w3.org/2002/07/owl#ObjectProperty"/>
    <skos:definition>The primary type of a ULAN Person or Corporate body. Domain is ULAN concept, range is AAT concept</skos:definition>
    <rdfs:label>agentTypePreferred</rdfs:label>
    <rdfs:isDefinedBy rdf:resource="http://vocab.getty.edu/ontology"/>
  </rdf:Description>
  <rdf:Description rdf:about="http://vocab.getty.edu/ontology#aat2886_used-function_as">
    <rdf:type rdf:resource="http://www.w3.org/2002/07/owl#ObjectProperty"/>
    <rdfs:isDefinedBy rdf:resource="http://vocab.getty.edu/ontology"/>
    <dc:identifier>2886</dc:identifier>
    <rdfs:domain rdf:resource="http://www.w3.org/2004/02/skos/core#Concept"/>
    <rdfs:subPropertyOf rdf:resource="http://www.w3.org/2004/02/skos/core#related"/>
    <dc:title>used/function as - material</dc:title>
    <rdfs:range rdf:resource="http://www.w3.org/2004/02/skos/core#Concept"/>
    <dct:description>material - used/function as - material.&#13;
Example: carbon disulfide - is used/functions as - solvent</dct:description>
    <owl:inverseOf rdf:resource="http://vocab.getty.edu/ontology#aat2887_exemplified_by"/>
    <skos:scopeNote>material - used/function as - material.&#13;
Example: carbon disulfide - is used/functions as - solvent</skos:scopeNote>
    <rdfs:isDefinedBy rdf:resource="http://vocab.getty.edu/aat/"/>
    <skos:example>carbon disulfide - is used/functions as - solvent</skos:example>
    <skos:prefLabel>aat2886_used-function_as</skos:prefLabel>
  </rdf:Description>
  <rdf:Description rdf:about="http://vocab.getty.edu/ontology#aat2408_locus-setting_for">
    <dc:title>locus/setting for - field/discipline</dc:title>
    <rdf:type rdf:resource="http://www.w3.org/2002/07/owl#ObjectProperty"/>
    <skos:prefLabel>aat2408_locus-setting_for</skos:prefLabel>
    <dct:description>locus/setting - [is] locus/setting for - field of study/discipline.&#13;
Example: schools (buildings) are the locus/setting for education; hospitals (buildings) are the locus/setting for medicine (discipline)</dct:description>
    <rdfs:isDefinedBy rdf:resource="http://vocab.getty.edu/aat/"/>
    <rdfs:domain rdf:resource="http://www.w3.org/2004/02/skos/core#Concept"/>
    <skos:example>hospitals (buildings) are the locus/setting for medicine (discipline)</skos:example>
    <rdfs:range rdf:resource="http://www.w3.org/2004/02/skos/core#Concept"/>
    <skos:example>schools (buildings) are the locus/setting for education</skos:example>
    <owl:inverseOf rdf:resource="http://vocab.getty.edu/ontology#aat2409_takes_place_in"/>
    <dc:identifier>2408</dc:identifier>
    <skos:scopeNote>locus/setting - [is] locus/setting for - field of study/discipline.&#13;
Example: schools (buildings) are the locus/setting for education; hospitals (buildings) are the locus/setting for medicine (discipline)</skos:scopeNote>
    <rdfs:subPropertyOf rdf:resource="http://www.w3.org/2004/02/skos/core#related"/>
    <rdfs:isDefinedBy rdf:resource="http://vocab.getty.edu/ontology"/>
  </rdf:Description>
  <rdf:Description rdf:about="http://vocab.getty.edu/ontology#broaderInstantial">
    <rdfs:subPropertyOf rdf:resource="http://vocab.getty.edu/ontology#broaderInstantialExtended"/>
    <dct:description>BTI (Kind/Instance, "example of") relation. We also infer iso-thes:broaderInstantial, which goes only between Concepts.
Example: Rembrandt van Rijn BTI Persons/Artists (ULAN)</dct:description>
    <rdfs:domain rdf:resource="http://vocab.getty.edu/ontology#Subject"/>
    <rdfs:subPropertyOf rdf:resource="http://vocab.getty.edu/ontology#broader"/>
    <skos:scopeNote>BTI (Kind/Instance, "example of") relation. We also infer iso-thes:broaderInstantial, which goes only between Concepts.
Example: Rembrandt van Rijn BTI Persons/Artists (ULAN)</skos:scopeNote>
    <skos:example>Rembrandt van Rijn BTI Persons/Artists (ULAN)</skos:example>
    <rdf:type rdf:resource="http://www.w3.org/2002/07/owl#ObjectProperty"/>
    <rdfs:isDefinedBy rdf:resource="http://vocab.getty.edu/ontology"/>
    <rdfs:comment>BTI (Kind/Instance, "example of") relation. We also infer iso-thes:broaderInstantial, which goes only between Concepts</rdfs:comment>
    <rdfs:label>broaderInstantial</rdfs:label>
    <skos:definition>BTI (Kind/Instance, "example of") relation. We also infer iso-thes:broaderInstantial, which goes only between Concepts</skos:definition>
    <skos:prefLabel>broaderInstantial</skos:prefLabel>
    <rdfs:range rdf:resource="http://vocab.getty.edu/ontology#Subject"/>
  </rdf:Description>
  <rdf:Description rdf:about="http://vocab.getty.edu/ontology#tgn3103_located_on">
    <rdfs:isDefinedBy rdf:resource="http://vocab.getty.edu/ontology"/>
    <owl:inverseOf rdf:resource="http://vocab.getty.edu/ontology#tgn3104_is_location_of"/>
    <skos:prefLabel>tgn3103_located_on</skos:prefLabel>
    <rdfs:domain rdf:resource="http://www.w3.org/2004/02/skos/core#Concept"/>
    <rdfs:range rdf:resource="http://www.w3.org/2004/02/skos/core#Concept"/>
    <dc:identifier>3103</dc:identifier>
    <dc:title>located on - place</dc:title>
    <skos:example>tgn:7018835 Palmyra is located on tgn:7031416 Silk Road</skos:example>
    <skos:scopeNote>place - located on - place.&#13;
Example: tgn:7018835 Palmyra is located on tgn:7031416 Silk Road</skos:scopeNote>
    <rdfs:isDefinedBy rdf:resource="http://vocab.getty.edu/tgn/"/>
    <rdfs:subPropertyOf rdf:resource="http://www.w3.org/2004/02/skos/core#related"/>
    <dct:description>place - located on - place.&#13;
Example: tgn:7018835 Palmyra is located on tgn:7031416 Silk Road</dct:description>
    <rdf:type rdf:resource="http://www.w3.org/2002/07/owl#ObjectProperty"/>
  </rdf:Description>
  <rdf:Description rdf:about="http://vocab.getty.edu/ontology#aat2845_used-located_in">
    <skos:prefLabel>aat2845_used-located_in</skos:prefLabel>
    <owl:inverseOf rdf:resource="http://vocab.getty.edu/ontology#aat2846_locus-setting_for"/>
    <skos:example>Elephantidae(family) are used/located in elephant houses</skos:example>
    <rdf:type rdf:resource="http://www.w3.org/2002/07/owl#ObjectProperty"/>
    <dc:identifier>2845</dc:identifier>
    <rdfs:isDefinedBy rdf:resource="http://vocab.getty.edu/ontology"/>
    <skos:scopeNote>genus/species - [is] used/located in -  locus/setting.&#13;
Example: Elephantidae(family) are used/located in elephant houses; Vitaceae (family) is used/located in vineyards</skos:scopeNote>
    <rdfs:isDefinedBy rdf:resource="http://vocab.getty.edu/aat/"/>
    <rdfs:subPropertyOf rdf:resource="http://www.w3.org/2004/02/skos/core#related"/>
    <dc:title>used/located in - locus/setting</dc:title>
    <skos:example>Vitaceae (family) is used/located in vineyards</skos:example>
    <rdfs:range rdf:resource="http://www.w3.org/2004/02/skos/core#Concept"/>
    <rdfs:domain rdf:resource="http://www.w3.org/2004/02/skos/core#Concept"/>
    <dct:description>genus/species - [is] used/located in -  locus/setting.&#13;
Example: Elephantidae(family) are used/located in elephant houses; Vitaceae (family) is used/located in vineyards</dct:description>
  </rdf:Description>
  <rdf:Description rdf:about="http://vocab.getty.edu/historic/current">
    <skos:notation>C</skos:notation>
    <skos:prefLabel>Current</skos:prefLabel>
    <rdf:type rdf:resource="http://www.w3.org/2004/02/skos/core#Concept"/>
    <skos:scopeNote>Valid/used currently</skos:scopeNote>
    <skos:inScheme rdf:resource="http://vocab.getty.edu/historic/"/>
    <dct:description>Valid/used currently</dct:description>
  </rdf:Description>
  <rdf:Description rdf:about="http://vocab.getty.edu/ontology#aat2881_reflected_in">
    <skos:example>Greek (language) is reflected in Greek alphabet</skos:example>
    <dc:identifier>2881</dc:identifier>
    <dc:title>reflected in - things</dc:title>
    <rdfs:domain rdf:resource="http://www.w3.org/2004/02/skos/core#Concept"/>
    <rdfs:range rdf:resource="http://www.w3.org/2004/02/skos/core#Concept"/>
    <skos:scopeNote>language - [is] reflected in - things.&#13;
Example: Greek (language) is reflected in Greek alphabet; Sanskrit is reflected in Vedas</skos:scopeNote>
    <rdfs:subPropertyOf rdf:resource="http://www.w3.org/2004/02/skos/core#related"/>
    <rdfs:isDefinedBy rdf:resource="http://vocab.getty.edu/ontology"/>
    <dct:description>language - [is] reflected in - things.&#13;
Example: Greek (language) is reflected in Greek alphabet; Sanskrit is reflected in Vedas</dct:description>
    <skos:prefLabel>aat2881_reflected_in</skos:prefLabel>
    <rdf:type rdf:resource="http://www.w3.org/2002/07/owl#ObjectProperty"/>
    <skos:example>Sanskrit is reflected in Vedas</skos:example>
    <rdfs:isDefinedBy rdf:resource="http://vocab.getty.edu/aat/"/>
    <owl:inverseOf rdf:resource="http://vocab.getty.edu/ontology#aat2882_reflect"/>
  </rdf:Description>
  <rdf:Description rdf:about="http://vocab.getty.edu/ontology#ulan1531_nephew-niece_of">
    <skos:prefLabel>ulan1531_nephew-niece_of</skos:prefLabel>
    <owl:inverseOf rdf:resource="http://vocab.getty.edu/ontology#ulan1532_uncle-aunt_of"/>
    <rdfs:subPropertyOf rdf:resource="http://www.w3.org/2004/02/skos/core#related"/>
    <skos:example>Jan Brueghel, the elder is the nephew/neice of  Pieter Coecke van Aeist, the younger</skos:example>
    <dct:description>person - nephew/niece of - person.&#13;
Example: Jan Brueghel, the elder is the nephew/neice of  Pieter Coecke van Aeist, the younger</dct:description>
    <rdfs:isDefinedBy rdf:resource="http://vocab.getty.edu/ulan/"/>
    <rdfs:range rdf:resource="http://www.w3.org/2004/02/skos/core#Concept"/>
    <rdfs:domain rdf:resource="http://www.w3.org/2004/02/skos/core#Concept"/>
    <dc:title>nephew/niece of - person</dc:title>
    <skos:scopeNote>person - nephew/niece of - person.&#13;
Example: Jan Brueghel, the elder is the nephew/neice of  Pieter Coecke van Aeist, the younger</skos:scopeNote>
    <dc:identifier>1531</dc:identifier>
    <rdf:type rdf:resource="http://www.w3.org/2002/07/owl#ObjectProperty"/>
    <rdfs:isDefinedBy rdf:resource="http://vocab.getty.edu/ontology"/>
  </rdf:Description>
  <rdf:Description rdf:about="http://vocab.getty.edu/ontology#aat2814_constituent_of">
    <rdfs:domain rdf:resource="http://www.w3.org/2004/02/skos/core#Concept"/>
    <rdfs:range rdf:resource="http://www.w3.org/2004/02/skos/core#Concept"/>
    <owl:inverseOf rdf:resource="http://vocab.getty.edu/ontology#aat2815_composed_of"/>
    <rdfs:subPropertyOf rdf:resource="http://www.w3.org/2004/02/skos/core#related"/>
    <rdfs:isDefinedBy rdf:resource="http://vocab.getty.edu/ontology"/>
    <skos:example>iron oxide is a constituent of desert varnish</skos:example>
    <dct:description>material - [is] constituent of - material.&#13;
Example: titanium white is a constituent of composite white; iron oxide is a constituent of desert varnish</dct:description>
    <rdf:type rdf:resource="http://www.w3.org/2002/07/owl#ObjectProperty"/>
    <rdfs:isDefinedBy rdf:resource="http://vocab.getty.edu/aat/"/>
    <dc:title>constituent of - material</dc:title>
    <skos:scopeNote>material - [is] constituent of - material.&#13;
Example: titanium white is a constituent of composite white; iron oxide is a constituent of desert varnish</skos:scopeNote>
    <skos:prefLabel>aat2814_constituent_of</skos:prefLabel>
    <skos:example>titanium white is a constituent of composite white</skos:example>
    <dc:identifier>2814</dc:identifier>
  </rdf:Description>
  <rdf:Description rdf:about="http://vocab.getty.edu/ontology#aat2219_have_form">
    <skos:example>cartoons (working drawings) have the form of toile peinte</skos:example>
    <rdfs:isDefinedBy rdf:resource="http://vocab.getty.edu/ontology"/>
    <skos:example>lighthouse lamps have the form of arc lamps</skos:example>
    <rdfs:subPropertyOf rdf:resource="http://www.w3.org/2004/02/skos/core#related"/>
    <rdfs:range rdf:resource="http://www.w3.org/2004/02/skos/core#Concept"/>
    <rdfs:domain rdf:resource="http://www.w3.org/2004/02/skos/core#Concept"/>
    <skos:prefLabel>aat2219_have_form</skos:prefLabel>
    <skos:scopeNote>things - have form [of] - things.&#13;
Example: lighthouse lamps have the form of arc lamps; cartoons (working drawings) have the form of toile peinte</skos:scopeNote>
    <dct:description>things - have form [of] - things.&#13;
Example: lighthouse lamps have the form of arc lamps; cartoons (working drawings) have the form of toile peinte</dct:description>
    <rdf:type rdf:resource="http://www.w3.org/2002/07/owl#ObjectProperty"/>
    <dc:title>have form - things</dc:title>
    <dc:identifier>2219</dc:identifier>
    <rdfs:isDefinedBy rdf:resource="http://vocab.getty.edu/aat/"/>
  </rdf:Description>
  <rdf:Description rdf:about="http://vocab.getty.edu/ontology#ulan1003_associated_with">
    <rdf:type rdf:resource="http://www.w3.org/2002/07/owl#ObjectProperty"/>
    <dc:title>associated with - any</dc:title>
    <skos:scopeNote>any - associated with - any.&#13;
Example: Richard Meier is associated with Renny B.Saltzman; United Nations is associated with World Bank</skos:scopeNote>
    <skos:example>Richard Meier is associated with Renny B.Saltzman</skos:example>
    <dc:identifier>1003</dc:identifier>
    <rdfs:isDefinedBy rdf:resource="http://vocab.getty.edu/ontology"/>
    <rdfs:isDefinedBy rdf:resource="http://vocab.getty.edu/ulan/"/>
    <dct:description>any - associated with - any.&#13;
Example: Richard Meier is associated with Renny B.Saltzman; United Nations is associated with World Bank</dct:description>
    <rdf:type rdf:resource="http://www.w3.org/2002/07/owl#SymmetricProperty"/>
    <rdfs:domain rdf:resource="http://www.w3.org/2004/02/skos/core#Concept"/>
    <skos:example>United Nations is associated with World Bank</skos:example>
    <rdfs:subPropertyOf rdf:resource="http://www.w3.org/2004/02/skos/core#related"/>
    <rdfs:range rdf:resource="http://www.w3.org/2004/02/skos/core#Concept"/>
    <skos:prefLabel>ulan1003_associated_with</skos:prefLabel>
  </rdf:Description>
  <rdf:Description rdf:about="http://vocab.getty.edu/ontology#tgn3510_historical_connection">
    <rdfs:isDefinedBy rdf:resource="http://vocab.getty.edu/tgn/"/>
    <rdf:type rdf:resource="http://www.w3.org/2002/07/owl#SymmetricProperty"/>
    <skos:example>Guyenne, France (historical region) has a historical connection to Gascogne (France) (historical region)</skos:example>
    <skos:prefLabel>tgn3510_historical_connection</skos:prefLabel>
    <skos:scopeNote>any - historical connection - any.&#13;
Example: Guyenne, France (historical region) has a historical connection to Gascogne (France) (historical region)</skos:scopeNote>
    <rdfs:domain rdf:resource="http://www.w3.org/2004/02/skos/core#Concept"/>
    <rdfs:range rdf:resource="http://www.w3.org/2004/02/skos/core#Concept"/>
    <dc:identifier>3510</dc:identifier>
    <rdfs:subPropertyOf rdf:resource="http://www.w3.org/2004/02/skos/core#related"/>
    <rdfs:isDefinedBy rdf:resource="http://vocab.getty.edu/ontology"/>
    <dc:title>historical connection - any</dc:title>
    <dct:description>any - historical connection - any.&#13;
Example: Guyenne, France (historical region) has a historical connection to Gascogne (France) (historical region)</dct:description>
    <rdf:type rdf:resource="http://www.w3.org/2002/07/owl#ObjectProperty"/>
  </rdf:Description>
  <rdf:Description rdf:about="http://vocab.getty.edu/ontology#aat2281_have_counterpart">
    <skos:example>duchesses have counterpart dukes</skos:example>
    <rdfs:domain rdf:resource="http://www.w3.org/2004/02/skos/core#Concept"/>
    <rdfs:isDefinedBy rdf:resource="http://vocab.getty.edu/aat/"/>
    <rdfs:range rdf:resource="http://www.w3.org/2004/02/skos/core#Concept"/>
    <dct:description>role -[is] counterpart to - role.&#13;
Example: duchesses have counterpart dukes; godesses have counterpart gods</dct:description>
    <rdfs:isDefinedBy rdf:resource="http://vocab.getty.edu/ontology"/>
    <rdf:type rdf:resource="http://www.w3.org/2002/07/owl#SymmetricProperty"/>
    <skos:example>godesses have counterpart gods</skos:example>
    <dc:identifier>2281</dc:identifier>
    <rdf:type rdf:resource="http://www.w3.org/2002/07/owl#ObjectProperty"/>
    <skos:scopeNote>role -[is] counterpart to - role.&#13;
Example: duchesses have counterpart dukes; godesses have counterpart gods</skos:scopeNote>
    <rdfs:subPropertyOf rdf:resource="http://www.w3.org/2004/02/skos/core#related"/>
    <dc:title>have counterpart - role</dc:title>
    <skos:prefLabel>aat2281_have_counterpart</skos:prefLabel>
  </rdf:Description>
  <rdf:Description rdf:about="http://vocab.getty.edu/term/flag/">
    <skos:scopeNote>Term Flag concept scheme</skos:scopeNote>
    <skos:prefLabel>Term Flag concept scheme</skos:prefLabel>
    <dct:description>Term Flag concept scheme</dct:description>
    <rdfs:isDefinedBy rdf:resource="http://vocab.getty.edu/ontology"/>
    <rdf:type rdf:resource="http://www.w3.org/2004/02/skos/core#ConceptScheme"/>
    <rdfs:label>Term Flag concept scheme</rdfs:label>
  </rdf:Description>
  <rdf:Description rdf:about="http://vocab.getty.edu/ontology#ulan1205_client_of">
    <rdfs:subPropertyOf rdf:resource="http://www.w3.org/2004/02/skos/core#related"/>
    <dct:description>person/firm/family - client of - person/firm/family.&#13;
Example: The Chicago Herald was the client of Burnham and Root</dct:description>
    <skos:prefLabel>ulan1205_client_of</skos:prefLabel>
    <owl:inverseOf rdf:resource="http://vocab.getty.edu/ontology#ulan1206_client_was"/>
    <skos:example>The Chicago Herald was the client of Burnham and Root</skos:example>
    <rdfs:isDefinedBy rdf:resource="http://vocab.getty.edu/ontology"/>
    <dc:identifier>1205</dc:identifier>
    <skos:scopeNote>person/firm/family - client of - person/firm/family.&#13;
Example: The Chicago Herald was the client of Burnham and Root</skos:scopeNote>
    <dc:title>client of - person/firm/family</dc:title>
    <rdf:type rdf:resource="http://www.w3.org/2002/07/owl#ObjectProperty"/>
    <rdfs:range rdf:resource="http://www.w3.org/2004/02/skos/core#Concept"/>
    <rdfs:isDefinedBy rdf:resource="http://vocab.getty.edu/ulan/"/>
    <rdfs:domain rdf:resource="http://www.w3.org/2004/02/skos/core#Concept"/>
  </rdf:Description>
  <rdf:Description rdf:about="http://vocab.getty.edu/ontology#aat2291_locus-setting_for">
    <skos:prefLabel>aat2291_locus-setting_for</skos:prefLabel>
    <skos:scopeNote>locus/setting - [is] locus setting for - [actor or institution having] role.&#13;
Example: roperies are the locus/setting of rope-makers; convents (built complexes) are the locus/setting of nuns; libraries (buildings) are the locus/setting of libraries (institutions)</skos:scopeNote>
    <skos:example>libraries (buildings) are the locus/setting of libraries (institutions)</skos:example>
    <dc:identifier>2291</dc:identifier>
    <skos:example>roperies are the locus/setting of rope-makers</skos:example>
    <rdfs:subPropertyOf rdf:resource="http://www.w3.org/2004/02/skos/core#related"/>
    <rdfs:range rdf:resource="http://www.w3.org/2004/02/skos/core#Concept"/>
    <rdfs:isDefinedBy rdf:resource="http://vocab.getty.edu/ontology"/>
    <rdfs:domain rdf:resource="http://www.w3.org/2004/02/skos/core#Concept"/>
    <owl:inverseOf rdf:resource="http://vocab.getty.edu/ontology#aat2292_work-live_in"/>
    <dct:description>locus/setting - [is] locus setting for - [actor or institution having] role.&#13;
Example: roperies are the locus/setting of rope-makers; convents (built complexes) are the locus/setting of nuns; libraries (buildings) are the locus/setting of libraries (institutions)</dct:description>
    <rdf:type rdf:resource="http://www.w3.org/2002/07/owl#ObjectProperty"/>
    <rdfs:isDefinedBy rdf:resource="http://vocab.getty.edu/aat/"/>
    <skos:example>convents (built complexes) are the locus/setting of nuns</skos:example>
    <dc:title>locus/setting for - role</dc:title>
  </rdf:Description>
  <rdf:Description rdf:about="http://vocab.getty.edu/term/kind/OfficialName">
    <skos:notation>O</skos:notation>
    <skos:scopeNote>Used in TGN and ULAN</skos:scopeNote>
    <skos:inScheme rdf:resource="http://vocab.getty.edu/term/kind/"/>
    <dct:description>Used in TGN and ULAN.
Example: "Noyen-sur-Seine" is official name of 7030197 "Noyen" (TGN)</dct:description>
    <rdf:type rdf:resource="http://www.w3.org/2004/02/skos/core#Concept"/>
    <skos:example>"Noyen-sur-Seine" is official name of 7030197 "Noyen" (TGN)</skos:example>
    <skos:prefLabel>Official Name</skos:prefLabel>
  </rdf:Description>
  <rdf:Description rdf:about="http://vocab.getty.edu/ontology#aat2894_exemplified_by">
    <skos:prefLabel>aat2894_exemplified_by</skos:prefLabel>
    <rdf:type rdf:resource="http://www.w3.org/2002/07/owl#ObjectProperty"/>
    <skos:scopeNote>activity/event/[process/function] - [is] exemplified by - brand name.&#13;
Example: deacidification [process/function] is exemplified by Papersave Process (TM)</skos:scopeNote>
    <dc:identifier>2894</dc:identifier>
    <rdfs:isDefinedBy rdf:resource="http://vocab.getty.edu/aat/"/>
    <owl:inverseOf rdf:resource="http://vocab.getty.edu/ontology#aat2895_example_of"/>
    <rdfs:subPropertyOf rdf:resource="http://www.w3.org/2004/02/skos/core#related"/>
    <dc:title>exemplified by - brand name</dc:title>
    <skos:example>deacidification [process/function] is exemplified by Papersave Process (TM)</skos:example>
    <dct:description>activity/event/[process/function] - [is] exemplified by - brand name.&#13;
Example: deacidification [process/function] is exemplified by Papersave Process (TM)</dct:description>
    <rdfs:range rdf:resource="http://www.w3.org/2004/02/skos/core#Concept"/>
    <rdfs:isDefinedBy rdf:resource="http://vocab.getty.edu/ontology"/>
    <rdfs:domain rdf:resource="http://www.w3.org/2004/02/skos/core#Concept"/>
  </rdf:Description>
  <rdf:Description rdf:about="http://vocab.getty.edu/ulan/">
    <vann:preferredNamespacePrefix>ulan</vann:preferredNamespacePrefix>
    <foaf:homepage rdf:resource="http://www.getty.edu/research/tools/vocabularies/ulan/"/>
    <rdfs:label>Union List of Artist Names</rdfs:label>
    <dct:creator rdf:resource="http://www.ontotext.com"/>
    <rdfs:seeAlso rdf:resource="http://vocab.getty.edu/"/>
    <dct:created rdf:datatype="http://www.w3.org/2001/XMLSchema#date">2015-03-25</dct:created>
    <vann:preferredNamespaceUri>http://vocab.getty.edu/ulan/</vann:preferredNamespaceUri>
    <rdf:type rdf:resource="http://www.w3.org/2004/02/skos/core#ConceptScheme"/>
    <skos:prefLabel>Union List of Artist Names</skos:prefLabel>
    <rdfs:seeAlso rdf:resource="http://vocab.getty.edu/.well-known/void"/>
    <skos:definition>The Union List of Artist Names concept scheme</skos:definition>
    <dct:creator rdf:resource="http://www.getty.edu/research/"/>
    <rdfs:seeAlso rdf:resource="http://www.getty.edu/research/tools/vocabularies/lod/"/>
    <rdfs:comment>The Union List of Artist Names concept scheme</rdfs:comment>
  </rdf:Description>
  <rdf:Description rdf:about="http://vocab.getty.edu/ontology#ulan1515_great-grandparent_of">
    <rdfs:subPropertyOf rdf:resource="http://www.w3.org/2004/02/skos/core#related"/>
    <skos:scopeNote>person - great-grandparent of - person.&#13;
Example: Albrecht Adam is the great-grandparent of Richard Benno Adam</skos:scopeNote>
    <skos:example>Albrecht Adam is the great-grandparent of Richard Benno Adam</skos:example>
    <dc:title>great-grandparent of - person</dc:title>
    <owl:inverseOf rdf:resource="http://vocab.getty.edu/ontology#ulan1516_great-grandchild_of"/>
    <rdfs:domain rdf:resource="http://www.w3.org/2004/02/skos/core#Concept"/>
    <rdf:type rdf:resource="http://www.w3.org/2002/07/owl#ObjectProperty"/>
    <dc:identifier>1515</dc:identifier>
    <skos:prefLabel>ulan1515_great-grandparent_of</skos:prefLabel>
    <dct:description>person - great-grandparent of - person.&#13;
Example: Albrecht Adam is the great-grandparent of Richard Benno Adam</dct:description>
    <rdfs:isDefinedBy rdf:resource="http://vocab.getty.edu/ontology"/>
    <rdfs:isDefinedBy rdf:resource="http://vocab.getty.edu/ulan/"/>
    <rdfs:range rdf:resource="http://www.w3.org/2004/02/skos/core#Concept"/>
  </rdf:Description>
  <rdf:Description rdf:about="http://schema.org/dissolutionLocation">
    <dct:description>The place where the Organization was dissolved.
Schema has properties foundationLocation and dissolutionDate but no dissolutionLocation. 
In contrast, for a person all 4 properties are present: birth/death place/date.
We posted issue https://github.com/schemaorg/schemaorg/issues/302, which looks like it will have a positive outcome in the far future.
And we define the property here</dct:description>
    <rdfs:seeAlso rdf:resource="https://github.com/schemaorg/schemaorg/issues/302"/>
    <skos:scopeNote>The place where the Organization was dissolved.
Schema has properties foundationLocation and dissolutionDate but no dissolutionLocation. 
In contrast, for a person all 4 properties are present: birth/death place/date.
We posted issue https://github.com/schemaorg/schemaorg/issues/302, which looks like it will have a positive outcome in the far future.
And we define the property here</skos:scopeNote>
    <skos:definition>The place where the Organization was dissolved</skos:definition>
    <rdf:type rdf:resource="http://www.w3.org/2002/07/owl#ObjectProperty"/>
    <rdfs:range rdf:resource="http://schema.org/Place"/>
    <rdfs:isDefinedBy rdf:resource="http://vocab.getty.edu/ontology"/>
    <rdfs:comment>The place where the Organization was dissolved</rdfs:comment>
    <rdfs:domain rdf:resource="http://schema.org/Organization"/>
    <skos:prefLabel>dissolutionLocation</skos:prefLabel>
    <rdfs:label>dissolutionLocation</rdfs:label>
  </rdf:Description>
  <rdf:Description rdf:about="http://vocab.getty.edu/term/kind/Abbreviation">
    <skos:notation>A</skos:notation>
    <skos:example>"FLIM" is abbrevaition for "fluorescence lifetime imaging microscopy"</skos:example>
    <skos:prefLabel>Abbreviation</skos:prefLabel>
    <skos:scopeNote>Term is an abbreviation, initialism, or acronym</skos:scopeNote>
    <rdf:type rdf:resource="http://www.w3.org/2004/02/skos/core#Concept"/>
    <dct:description>Term is an abbreviation, initialism, or acronym.
Example: "FLIM" is abbrevaition for "fluorescence lifetime imaging microscopy"</dct:description>
    <skos:inScheme rdf:resource="http://vocab.getty.edu/term/kind/"/>
  </rdf:Description>
  <rdf:Description rdf:about="http://vocab.getty.edu/ontology#aat2803_example_of">
    <dc:identifier>2803</dc:identifier>
    <skos:prefLabel>aat2803_example_of</skos:prefLabel>
    <rdfs:subPropertyOf rdf:resource="http://www.w3.org/2004/02/skos/core#related"/>
    <rdfs:domain rdf:resource="http://www.w3.org/2004/02/skos/core#Concept"/>
    <skos:example>Vaseline (TM) is an example of petrolium jelly</skos:example>
    <dct:description>brand name - [is] example of - material.&#13;
Example: Vaseline (TM) is an example of petrolium jelly; Teflon (TM) is an example of polytetrafluoroethyelene</dct:description>
    <rdfs:range rdf:resource="http://www.w3.org/2004/02/skos/core#Concept"/>
    <dc:title>example of - material</dc:title>
    <rdf:type rdf:resource="http://www.w3.org/2002/07/owl#ObjectProperty"/>
    <rdfs:isDefinedBy rdf:resource="http://vocab.getty.edu/ontology"/>
    <skos:scopeNote>brand name - [is] example of - material.&#13;
Example: Vaseline (TM) is an example of petrolium jelly; Teflon (TM) is an example of polytetrafluoroethyelene</skos:scopeNote>
    <rdfs:isDefinedBy rdf:resource="http://vocab.getty.edu/aat/"/>
    <skos:example>Teflon (TM) is an example of polytetrafluoroethyelene</skos:example>
  </rdf:Description>
  <rdf:Description rdf:about="http://vocab.getty.edu/ontology#aat2809_coexisted_with">
    <rdf:type rdf:resource="http://www.w3.org/2002/07/owl#SymmetricProperty"/>
    <dc:title>coexisted with - style/period/culture</dc:title>
    <skos:example>Early Minoan coexisted with Prepalatial</skos:example>
    <rdfs:domain rdf:resource="http://www.w3.org/2004/02/skos/core#Concept"/>
    <rdfs:range rdf:resource="http://www.w3.org/2004/02/skos/core#Concept"/>
    <rdfs:subPropertyOf rdf:resource="http://www.w3.org/2004/02/skos/core#related"/>
    <dct:description>style/period/culture/[religion/ideology] - coexisted with -  style/period/culture/[religion/ideology].&#13;
Example: Sangoan coexisted with Fauresmith; Early Minoan coexisted with Prepalatial</dct:description>
    <skos:example>Sangoan coexisted with Fauresmith</skos:example>
    <skos:prefLabel>aat2809_coexisted_with</skos:prefLabel>
    <rdf:type rdf:resource="http://www.w3.org/2002/07/owl#ObjectProperty"/>
    <skos:scopeNote>style/period/culture/[religion/ideology] - coexisted with -  style/period/culture/[religion/ideology].&#13;
Example: Sangoan coexisted with Fauresmith; Early Minoan coexisted with Prepalatial</skos:scopeNote>
    <rdfs:isDefinedBy rdf:resource="http://vocab.getty.edu/ontology"/>
    <rdfs:isDefinedBy rdf:resource="http://vocab.getty.edu/aat/"/>
    <dc:identifier>2809</dc:identifier>
  </rdf:Description>
  <rdf:Description rdf:about="http://vocab.getty.edu/ontology#ulan1108_influenced_by">
    <skos:example>Salomon Koninck was influenced by Rembrandt van Rijn</skos:example>
    <rdfs:subPropertyOf rdf:resource="http://www.w3.org/2004/02/skos/core#related"/>
    <rdfs:isDefinedBy rdf:resource="http://vocab.getty.edu/ulan/"/>
    <dc:title>influenced by - person</dc:title>
    <dct:description>person - influenced by - person.&#13;
Example: Salomon Koninck was influenced by Rembrandt van Rijn</dct:description>
    <dc:identifier>1108</dc:identifier>
    <rdfs:domain rdf:resource="http://www.w3.org/2004/02/skos/core#Concept"/>
    <rdfs:range rdf:resource="http://www.w3.org/2004/02/skos/core#Concept"/>
    <skos:scopeNote>person - influenced by - person.&#13;
Example: Salomon Koninck was influenced by Rembrandt van Rijn</skos:scopeNote>
    <rdf:type rdf:resource="http://www.w3.org/2002/07/owl#ObjectProperty"/>
    <skos:prefLabel>ulan1108_influenced_by</skos:prefLabel>
    <rdfs:isDefinedBy rdf:resource="http://vocab.getty.edu/ontology"/>
  </rdf:Description>
  <rdf:Description rdf:about="http://vocab.getty.edu/ontology#aat2828_use-require">
    <skos:example>oil paintings use/require varnish</skos:example>
    <dct:description>things - use/require - material.&#13;
Example: oil paintings use/require varnish; wine glasses use/require wine</dct:description>
    <skos:prefLabel>aat2828_use-require</skos:prefLabel>
    <owl:inverseOf rdf:resource="http://vocab.getty.edu/ontology#aat2829_used-required_for"/>
    <rdfs:subPropertyOf rdf:resource="http://www.w3.org/2004/02/skos/core#related"/>
    <skos:example>wine glasses use/require wine</skos:example>
    <skos:scopeNote>things - use/require - material.&#13;
Example: oil paintings use/require varnish; wine glasses use/require wine</skos:scopeNote>
    <dc:identifier>2828</dc:identifier>
    <rdfs:domain rdf:resource="http://www.w3.org/2004/02/skos/core#Concept"/>
    <rdfs:range rdf:resource="http://www.w3.org/2004/02/skos/core#Concept"/>
    <dc:title>use/require - material</dc:title>
    <rdfs:isDefinedBy rdf:resource="http://vocab.getty.edu/aat/"/>
    <rdf:type rdf:resource="http://www.w3.org/2002/07/owl#ObjectProperty"/>
    <rdfs:isDefinedBy rdf:resource="http://vocab.getty.edu/ontology"/>
  </rdf:Description>
  <rdf:Description rdf:about="http://vocab.getty.edu/term/kind/SiteName">
    <skos:scopeNote>Used in TGN only</skos:scopeNote>
    <skos:prefLabel>Site Name</skos:prefLabel>
    <rdf:type rdf:resource="http://www.w3.org/2004/02/skos/core#Concept"/>
    <dct:description>Used in TGN only.
Example: "Flavia Solva", a deserted settlement and archaeological site (TGN)</dct:description>
    <skos:notation>S</skos:notation>
    <skos:inScheme rdf:resource="http://vocab.getty.edu/term/kind/"/>
    <skos:example>"Flavia Solva", a deserted settlement and archaeological site (TGN)</skos:example>
  </rdf:Description>
  <rdf:Description rdf:about="http://vocab.getty.edu/ontology#Hierarchy">
    <skos:broader rdf:resource="http://vocab.getty.edu/ontology#Subject"/>
    <rdfs:subClassOf rdf:resource="http://vocab.getty.edu/ontology#Subject"/>
    <rdf:type rdf:resource="http://www.w3.org/2002/07/owl#Class"/>
    <rdfs:subClassOf rdf:resource="http://purl.org/iso25964/skos-thes#ThesaurusArray"/>
    <dct:description>Top of a hierarchy. Used in AAT only. Not used for indexing or cataloguing.
Example: Containers (Hierarchy Name) (AAT)</dct:description>
    <rdfs:isDefinedBy rdf:resource="http://vocab.getty.edu/ontology"/>
    <skos:example>Containers (Hierarchy Name) (AAT)</skos:example>
    <rdfs:comment>Top of a hierarchy. Used in AAT only. Not used for indexing or cataloguing</rdfs:comment>
    <skos:scopeNote>Top of a hierarchy. Used in AAT only. Not used for indexing or cataloguing.
Example: Containers (Hierarchy Name) (AAT)</skos:scopeNote>
    <rdfs:label>Hierarchy</rdfs:label>
    <skos:definition>Top of a hierarchy. Used in AAT only. Not used for indexing or cataloguing</skos:definition>
    <skos:prefLabel>Hierarchy</skos:prefLabel>
  </rdf:Description>
  <rdf:Description rdf:about="http://vocab.getty.edu/term/POS/">
    <rdf:type rdf:resource="http://www.w3.org/2004/02/skos/core#ConceptScheme"/>
    <skos:scopeNote>Part of Speech concept scheme</skos:scopeNote>
    <rdfs:label>Part of Speech concept scheme</rdfs:label>
    <dct:description>Part of Speech concept scheme</dct:description>
    <skos:prefLabel>Part of Speech concept scheme</skos:prefLabel>
    <rdfs:isDefinedBy rdf:resource="http://vocab.getty.edu/ontology"/>
  </rdf:Description>
  <rdf:Description rdf:nodeID="N52cd7acc51f54260bfe30b76ba441dc7">
    <rdf:rest rdf:nodeID="N7c0ee6a758e646b284267328dc00c97c"/>
    <rdf:first rdf:resource="http://vocab.getty.edu/ontology#broaderPartitiveExtended"/>
  </rdf:Description>
  <rdf:Description rdf:about="http://vocab.getty.edu/term/kind/BirthName">
    <skos:notation>BN</skos:notation>
    <rdf:type rdf:resource="http://www.w3.org/2004/02/skos/core#Concept"/>
    <skos:inScheme rdf:resource="http://vocab.getty.edu/term/kind/"/>
    <skos:example>TODO</skos:example>
    <dct:description>Birth Name of an ULAN agent.
Example: TODO</dct:description>
    <skos:scopeNote>Birth Name of an ULAN agent</skos:scopeNote>
    <skos:prefLabel>Birth Name</skos:prefLabel>
  </rdf:Description>
  <rdf:Description rdf:about="http://vocab.getty.edu/ontology#ulan1307_assistant_of">
    <skos:scopeNote>person - assistant of - person.&#13;
Example: Bernard Castelli was assistant of Pablo Picasso</skos:scopeNote>
    <skos:example>Bernard Castelli was assistant of Pablo Picasso</skos:example>
    <rdfs:isDefinedBy rdf:resource="http://vocab.getty.edu/ontology"/>
    <rdf:type rdf:resource="http://www.w3.org/2002/07/owl#ObjectProperty"/>
    <skos:prefLabel>ulan1307_assistant_of</skos:prefLabel>
    <dc:title>assistant of - person</dc:title>
    <rdfs:isDefinedBy rdf:resource="http://vocab.getty.edu/ulan/"/>
    <rdfs:range rdf:resource="http://www.w3.org/2004/02/skos/core#Concept"/>
    <owl:inverseOf rdf:resource="http://vocab.getty.edu/ontology#ulan1308_assisted_by"/>
    <rdfs:subPropertyOf rdf:resource="http://www.w3.org/2004/02/skos/core#related"/>
    <rdfs:domain rdf:resource="http://www.w3.org/2004/02/skos/core#Concept"/>
    <dct:description>person - assistant of - person.&#13;
Example: Bernard Castelli was assistant of Pablo Picasso</dct:description>
    <dc:identifier>1307</dc:identifier>
  </rdf:Description>
  <rdf:Description rdf:about="http://vocab.getty.edu/ontology#ulan2696_leader_of">
    <owl:inverseOf rdf:resource="http://vocab.getty.edu/ontology#ulan2697_leader_was"/>
    <dc:title>leader of - institution</dc:title>
    <dct:description>person - leader of - institution.&#13;
Example: Rush Harrison Kress was the leader of Samuel H. Kress Foundation</dct:description>
    <dc:identifier>2696</dc:identifier>
    <rdfs:range rdf:resource="http://www.w3.org/2004/02/skos/core#Concept"/>
    <rdfs:domain rdf:resource="http://www.w3.org/2004/02/skos/core#Concept"/>
    <skos:scopeNote>person - leader of - institution.&#13;
Example: Rush Harrison Kress was the leader of Samuel H. Kress Foundation</skos:scopeNote>
    <rdfs:subPropertyOf rdf:resource="http://www.w3.org/2004/02/skos/core#related"/>
    <skos:prefLabel>ulan2696_leader_of</skos:prefLabel>
    <rdfs:isDefinedBy rdf:resource="http://vocab.getty.edu/ulan/"/>
    <rdf:type rdf:resource="http://www.w3.org/2002/07/owl#ObjectProperty"/>
    <skos:example>Rush Harrison Kress was the leader of Samuel H. Kress Foundation</skos:example>
    <rdfs:isDefinedBy rdf:resource="http://vocab.getty.edu/ontology"/>
  </rdf:Description>
  <rdf:Description rdf:about="http://vocab.getty.edu/ontology#aat2802_exemplified_by">
    <dc:identifier>2802</dc:identifier>
    <skos:example>petrolium jelly is exemplified by Vaseline (TM)</skos:example>
    <owl:inverseOf rdf:resource="http://vocab.getty.edu/ontology#aat2803_example_of"/>
    <skos:scopeNote>material - [is] exemplified by - brand name.&#13;
Example: petrolium jelly is exemplified by Vaseline (TM); polytetrafluoroethyelene is exemplified by Teflon (TM)</skos:scopeNote>
    <rdfs:isDefinedBy rdf:resource="http://vocab.getty.edu/ontology"/>
    <dct:description>material - [is] exemplified by - brand name.&#13;
Example: petrolium jelly is exemplified by Vaseline (TM); polytetrafluoroethyelene is exemplified by Teflon (TM)</dct:description>
    <rdfs:range rdf:resource="http://www.w3.org/2004/02/skos/core#Concept"/>
    <rdfs:subPropertyOf rdf:resource="http://www.w3.org/2004/02/skos/core#related"/>
    <skos:example>polytetrafluoroethyelene is exemplified by Teflon (TM)</skos:example>
    <rdf:type rdf:resource="http://www.w3.org/2002/07/owl#ObjectProperty"/>
    <dc:title>exemplified by - brand name</dc:title>
    <skos:prefLabel>aat2802_exemplified_by</skos:prefLabel>
    <rdfs:domain rdf:resource="http://www.w3.org/2004/02/skos/core#Concept"/>
    <rdfs:isDefinedBy rdf:resource="http://vocab.getty.edu/aat/"/>
  </rdf:Description>
  <rdf:Description rdf:about="http://vocab.getty.edu/ontology#ulan1511_child_of">
    <skos:scopeNote>person - child of - person.&#13;
Example: Rembrandt van Rijn is the child of Neeltgen Willemsdr van Zuydtbroeck</skos:scopeNote>
    <rdf:type rdf:resource="http://www.w3.org/2002/07/owl#ObjectProperty"/>
    <dc:title>child of - person</dc:title>
    <dct:description>person - child of - person.&#13;
Example: Rembrandt van Rijn is the child of Neeltgen Willemsdr van Zuydtbroeck</dct:description>
    <rdfs:domain rdf:resource="http://www.w3.org/2004/02/skos/core#Concept"/>
    <rdfs:range rdf:resource="http://www.w3.org/2004/02/skos/core#Concept"/>
    <owl:inverseOf rdf:resource="http://vocab.getty.edu/ontology#ulan1512_parent_of"/>
    <rdfs:isDefinedBy rdf:resource="http://vocab.getty.edu/ulan/"/>
    <skos:prefLabel>ulan1511_child_of</skos:prefLabel>
    <skos:example>Rembrandt van Rijn is the child of Neeltgen Willemsdr van Zuydtbroeck</skos:example>
    <dc:identifier>1511</dc:identifier>
    <rdfs:subPropertyOf rdf:resource="http://www.w3.org/2004/02/skos/core#related"/>
    <rdfs:isDefinedBy rdf:resource="http://vocab.getty.edu/ontology"/>
  </rdf:Description>
  <rdf:Description rdf:about="http://vocab.getty.edu/term/kind/ISOalpha3">
    <skos:prefLabel>ISO alpha-3 code</skos:prefLabel>
    <skos:notation>ISO3L</skos:notation>
    <rdf:type rdf:resource="http://www.w3.org/2004/02/skos/core#Concept"/>
    <skos:scopeNote>ISO 3166-1 alpha-3 country code. Used in TGN</skos:scopeNote>
    <dct:description>ISO 3166-1 alpha-3 country code. Used in TGN.
Example: "ATA" for Antarctica</dct:description>
    <skos:example>"ATA" for Antarctica</skos:example>
    <skos:inScheme rdf:resource="http://vocab.getty.edu/term/kind/"/>
  </rdf:Description>
  <rdf:Description rdf:about="http://vocab.getty.edu/ontology#tgn3202_capital_is">
    <dc:title>capital is - city</dc:title>
    <rdfs:domain rdf:resource="http://www.w3.org/2004/02/skos/core#Concept"/>
    <rdfs:range rdf:resource="http://www.w3.org/2004/02/skos/core#Concept"/>
    <rdfs:isDefinedBy rdf:resource="http://vocab.getty.edu/tgn/"/>
    <rdfs:isDefinedBy rdf:resource="http://vocab.getty.edu/ontology"/>
    <skos:scopeNote>nation - capital is - city.&#13;
Example: London was the capital of Maxima Caesariensis from 296 to 800 CE</skos:scopeNote>
    <rdf:type rdf:resource="http://www.w3.org/2002/07/owl#ObjectProperty"/>
    <dc:identifier>3202</dc:identifier>
    <rdfs:subPropertyOf rdf:resource="http://www.w3.org/2004/02/skos/core#related"/>
    <skos:example>London was the capital of Maxima Caesariensis from 296 to 800 CE</skos:example>
    <skos:prefLabel>tgn3202_capital_is</skos:prefLabel>
    <dct:description>nation - capital is - city.&#13;
Example: London was the capital of Maxima Caesariensis from 296 to 800 CE</dct:description>
  </rdf:Description>
  <rdf:Description rdf:about="http://vocab.getty.edu/ontology#ulan1321_school_of">
    <owl:inverseOf rdf:resource="http://vocab.getty.edu/ontology#ulan1322_school_was"/>
    <rdfs:subPropertyOf rdf:resource="http://www.w3.org/2004/02/skos/core#related"/>
    <rdfs:domain rdf:resource="http://www.w3.org/2004/02/skos/core#Concept"/>
    <rdfs:range rdf:resource="http://www.w3.org/2004/02/skos/core#Concept"/>
    <dct:description>person - school of - firm/group.&#13;
Example: The school of Pierre Saalburg was the Architectural Association. School of Architecture</dct:description>
    <rdf:type rdf:resource="http://www.w3.org/2002/07/owl#ObjectProperty"/>
    <skos:prefLabel>ulan1321_school_of</skos:prefLabel>
    <rdfs:isDefinedBy rdf:resource="http://vocab.getty.edu/ontology"/>
    <dc:identifier>1321</dc:identifier>
    <skos:scopeNote>person - school of - firm/group.&#13;
Example: The school of Pierre Saalburg was the Architectural Association. School of Architecture</skos:scopeNote>
    <skos:example>The school of Pierre Saalburg was the Architectural Association. School of Architecture</skos:example>
    <dc:title>school of - firm/group</dc:title>
    <rdfs:isDefinedBy rdf:resource="http://vocab.getty.edu/ulan/"/>
  </rdf:Description>
  <rdf:Description rdf:about="http://vocab.getty.edu/historic/localUse">
    <skos:example>500051176 Abinetti (ULAN) is an unknown artist mentioned in documentation of lot 209 of an auction held 29 Jan 1824 in London</skos:example>
    <skos:notation>LU</skos:notation>
    <dct:description>Used locally for Unidentified Named People mentioned in some document (ULAN only).
Example: 500051176 Abinetti (ULAN) is an unknown artist mentioned in documentation of lot 209 of an auction held 29 Jan 1824 in London</dct:description>
    <skos:scopeNote>Used locally for Unidentified Named People mentioned in some document (ULAN only)</skos:scopeNote>
    <rdf:type rdf:resource="http://www.w3.org/2004/02/skos/core#Concept"/>
    <skos:prefLabel>Local Use</skos:prefLabel>
    <skos:inScheme rdf:resource="http://vocab.getty.edu/historic/"/>
  </rdf:Description>
  <rdf:Description rdf:about="http://vocab.getty.edu/ontology#ulan1217_employee_of">
    <dc:title>employee of - person</dc:title>
    <rdf:type rdf:resource="http://www.w3.org/2002/07/owl#ObjectProperty"/>
    <owl:inverseOf rdf:resource="http://vocab.getty.edu/ontology#ulan1218_employee_was"/>
    <rdfs:isDefinedBy rdf:resource="http://vocab.getty.edu/ontology"/>
    <skos:scopeNote>person/firm - employee of - person.&#13;
Example: Employee of Christopher Wren was Jean Tijou</skos:scopeNote>
    <rdfs:range rdf:resource="http://www.w3.org/2004/02/skos/core#Concept"/>
    <rdfs:subPropertyOf rdf:resource="http://www.w3.org/2004/02/skos/core#related"/>
    <rdfs:domain rdf:resource="http://www.w3.org/2004/02/skos/core#Concept"/>
    <skos:example>Employee of Christopher Wren was Jean Tijou</skos:example>
    <dct:description>person/firm - employee of - person.&#13;
Example: Employee of Christopher Wren was Jean Tijou</dct:description>
    <rdfs:isDefinedBy rdf:resource="http://vocab.getty.edu/ulan/"/>
    <dc:identifier>1217</dc:identifier>
    <skos:prefLabel>ulan1217_employee_of</skos:prefLabel>
  </rdf:Description>
  <rdf:Description rdf:nodeID="N8eab80e9df0a4f29aa7d04c3bd66fd47">
    <rdf:rest rdf:nodeID="Nb94f42dcb520415381be684e6f7568e7"/>
    <rdf:first rdf:resource="http://vocab.getty.edu/ontology#broaderPartitiveExtended"/>
  </rdf:Description>
  <rdf:Description rdf:about="http://vocab.getty.edu/ontology#aat2552_reflected_in-produces">
    <dct:description>style/period/culture/[religion/ideology] - [is] reflected in/produces - things.&#13;
Example: Nasca [culture] produces/is reflected in Nasca lines; Judaism produces/is reflected in Judaica</dct:description>
    <skos:example>Judaism produces/is reflected in Judaica</skos:example>
    <dc:title>reflected in/produces - things</dc:title>
    <rdfs:range rdf:resource="http://www.w3.org/2004/02/skos/core#Concept"/>
    <rdfs:isDefinedBy rdf:resource="http://vocab.getty.edu/aat/"/>
    <rdfs:domain rdf:resource="http://www.w3.org/2004/02/skos/core#Concept"/>
    <rdfs:isDefinedBy rdf:resource="http://vocab.getty.edu/ontology"/>
    <skos:scopeNote>style/period/culture/[religion/ideology] - [is] reflected in/produces - things.&#13;
Example: Nasca [culture] produces/is reflected in Nasca lines; Judaism produces/is reflected in Judaica</skos:scopeNote>
    <rdf:type rdf:resource="http://www.w3.org/2002/07/owl#ObjectProperty"/>
    <dc:identifier>2552</dc:identifier>
    <skos:example>Nasca [culture] produces/is reflected in Nasca lines</skos:example>
    <rdfs:subPropertyOf rdf:resource="http://www.w3.org/2004/02/skos/core#related"/>
    <skos:prefLabel>aat2552_reflected_in-produces</skos:prefLabel>
  </rdf:Description>
  <rdf:Description rdf:about="http://vocab.getty.edu/term/POS/SingularNoun">
    <rdf:type rdf:resource="http://www.w3.org/2004/02/skos/core#Concept"/>
    <skos:inScheme rdf:resource="http://vocab.getty.edu/term/POS/"/>
    <skos:prefLabel>Singular Noun</skos:prefLabel>
    <skos:example>"filigrane" is the French singular for "watermark"</skos:example>
    <dct:description>A term that is singular (the same word may be plural in another language).
Example: "filigrane" is the French singular for "watermark"</dct:description>
    <skos:notation>SN</skos:notation>
    <skos:scopeNote>A term that is singular (the same word may be plural in another language)</skos:scopeNote>
  </rdf:Description>
  <rdf:Description rdf:about="http://vocab.getty.edu/term/flag/Vernacular">
    <skos:scopeNote>Term is the vernacular for a certain place</skos:scopeNote>
    <skos:prefLabel>Vernacular</skos:prefLabel>
    <skos:inScheme rdf:resource="http://vocab.getty.edu/term/flag/"/>
    <rdf:type rdf:resource="http://www.w3.org/2004/02/skos/core#Concept"/>
    <skos:example>"kachoga" is the Vernacular for 300266169 "bird-and-flower paintings" (AAT). "Firenze" is the vernacular in Italian (TGN)</skos:example>
    <skos:notation>V</skos:notation>
    <dct:description>Term is the vernacular for a certain place.
Example: "kachoga" is the Vernacular for 300266169 "bird-and-flower paintings" (AAT). "Firenze" is the vernacular in Italian (TGN)</dct:description>
  </rdf:Description>
  <rdf:Description rdf:about="http://vocab.getty.edu/ontology#ulan2677_teacher_was">
    <dct:description>institution - teacher was - person.&#13;
Example: A teacher at Black Mountain College was Willem De Kooning</dct:description>
    <rdfs:isDefinedBy rdf:resource="http://vocab.getty.edu/ulan/"/>
    <dc:title>teacher was - person</dc:title>
    <rdfs:subPropertyOf rdf:resource="http://www.w3.org/2004/02/skos/core#related"/>
    <skos:prefLabel>ulan2677_teacher_was</skos:prefLabel>
    <skos:example>A teacher at Black Mountain College was Willem De Kooning</skos:example>
    <rdfs:domain rdf:resource="http://www.w3.org/2004/02/skos/core#Concept"/>
    <rdf:type rdf:resource="http://www.w3.org/2002/07/owl#ObjectProperty"/>
    <rdfs:isDefinedBy rdf:resource="http://vocab.getty.edu/ontology"/>
    <dc:identifier>2677</dc:identifier>
    <rdfs:range rdf:resource="http://www.w3.org/2004/02/skos/core#Concept"/>
    <skos:scopeNote>institution - teacher was - person.&#13;
Example: A teacher at Black Mountain College was Willem De Kooning</skos:scopeNote>
  </rdf:Description>
  <rdf:Description rdf:about="http://vocab.getty.edu/ontology#sourceNonPreferred">
    <rdfs:comment>Source for which the term is Non-preferred. Range is bibo:Document or bibo:DocumentPart</rdfs:comment>
    <skos:example>"Panderma" is non-preferred in Webster's New Geographical Dictionary (1988)</skos:example>
    <skos:definition>Source for which the term is Non-preferred. Range is bibo:Document or bibo:DocumentPart</skos:definition>
    <rdf:type rdf:resource="http://www.w3.org/2002/07/owl#ObjectProperty"/>
    <dct:description>Source for which the term is Non-preferred. Range is bibo:Document or bibo:DocumentPart.
Example: "Panderma" is non-preferred in Webster's New Geographical Dictionary (1988)</dct:description>
    <rdfs:range rdf:resource="http://purl.org/ontology/bibo/Document"/>
    <rdfs:isDefinedBy rdf:resource="http://vocab.getty.edu/ontology"/>
    <skos:scopeNote>Source for which the term is Non-preferred. Range is bibo:Document or bibo:DocumentPart.
Example: "Panderma" is non-preferred in Webster's New Geographical Dictionary (1988)</skos:scopeNote>
    <rdfs:label>sourceNonPreferred</rdfs:label>
    <rdfs:domain rdf:resource="http://www.w3.org/2008/05/skos-xl#Label"/>
    <rdfs:subPropertyOf rdf:resource="http://purl.org/dc/terms/source"/>
    <skos:prefLabel>sourceNonPreferred</skos:prefLabel>
  </rdf:Description>
  <rdf:Description rdf:about="http://vocab.getty.edu/ontology#aat2875_characteristic_of">
    <skos:example>Celtic (language) was characteristic of Celtic (culture)</skos:example>
    <rdfs:isDefinedBy rdf:resource="http://vocab.getty.edu/ontology"/>
    <rdfs:range rdf:resource="http://www.w3.org/2004/02/skos/core#Concept"/>
    <rdfs:subPropertyOf rdf:resource="http://www.w3.org/2004/02/skos/core#related"/>
    <rdf:type rdf:resource="http://www.w3.org/2002/07/owl#ObjectProperty"/>
    <dc:title>characteristic of - style/period/culture</dc:title>
    <skos:example>Afar (language) is characteristic of Afar (culture)</skos:example>
    <skos:scopeNote>language - [is] characteristic of - style/period/culture.&#13;
Example: Afar (language) is characteristic of Afar (culture); Celtic (language) was characteristic of Celtic (culture)</skos:scopeNote>
    <dc:identifier>2875</dc:identifier>
    <skos:prefLabel>aat2875_characteristic_of</skos:prefLabel>
    <rdfs:domain rdf:resource="http://www.w3.org/2004/02/skos/core#Concept"/>
    <dct:description>language - [is] characteristic of - style/period/culture.&#13;
Example: Afar (language) is characteristic of Afar (culture); Celtic (language) was characteristic of Celtic (culture)</dct:description>
    <owl:inverseOf rdf:resource="http://vocab.getty.edu/ontology#aat2876_characterized_by"/>
    <rdfs:isDefinedBy rdf:resource="http://vocab.getty.edu/aat/"/>
  </rdf:Description>
  <rdf:Description rdf:about="http://vocab.getty.edu/ontology#Infer_broaderPreferredExtended">
    <rdf:type rdf:resource="http://www.ontotext.com/proton/protontop#PropChainRestr"/>
    <ptop:restriction rdf:resource="http://vocab.getty.edu/ontology#broaderExtended"/>
    <ptop:premise2 rdf:resource="http://vocab.getty.edu/ontology#broaderPreferred"/>
    <ptop:conclusion rdf:resource="http://vocab.getty.edu/ontology#broaderPreferredExtended"/>
    <ptop:premise1 rdf:resource="http://vocab.getty.edu/ontology#broaderPreferredExtended"/>
  </rdf:Description>
  <rdf:Description rdf:about="http://vocab.getty.edu/ontology#aat2326_create">
    <rdfs:range rdf:resource="http://www.w3.org/2004/02/skos/core#Concept"/>
    <rdfs:isDefinedBy rdf:resource="http://vocab.getty.edu/aat/"/>
    <rdfs:domain rdf:resource="http://www.w3.org/2004/02/skos/core#Concept"/>
    <dc:title>create - things</dc:title>
    <skos:scopeNote>[actors having] role - create - things.&#13;
Example: draftsmen create drawings; poets create poems</skos:scopeNote>
    <skos:example>poets create poems</skos:example>
    <rdf:type rdf:resource="http://www.w3.org/2002/07/owl#ObjectProperty"/>
    <rdfs:isDefinedBy rdf:resource="http://vocab.getty.edu/ontology"/>
    <skos:prefLabel>aat2326_create</skos:prefLabel>
    <rdfs:subPropertyOf rdf:resource="http://www.w3.org/2004/02/skos/core#related"/>
    <dc:identifier>2326</dc:identifier>
    <dct:description>[actors having] role - create - things.&#13;
Example: draftsmen create drawings; poets create poems</dct:description>
    <skos:example>draftsmen create drawings</skos:example>
  </rdf:Description>
  <rdf:Description rdf:about="http://vocab.getty.edu/ontology#ulan2582_administered_by">
    <rdf:type rdf:resource="http://www.w3.org/2002/07/owl#ObjectProperty"/>
    <rdfs:isDefinedBy rdf:resource="http://vocab.getty.edu/ontology"/>
    <skos:example>Societe nationale des chemins de fer Francais. Agence des gares was administered by Georges Mathieu</skos:example>
    <dc:title>administered by - person</dc:title>
    <rdfs:isDefinedBy rdf:resource="http://vocab.getty.edu/ulan/"/>
    <rdfs:domain rdf:resource="http://www.w3.org/2004/02/skos/core#Concept"/>
    <rdfs:range rdf:resource="http://www.w3.org/2004/02/skos/core#Concept"/>
    <dct:description>institution - administered by - person.&#13;
Example: Societe nationale des chemins de fer Francais. Agence des gares was administered by Georges Mathieu</dct:description>
    <rdfs:subPropertyOf rdf:resource="http://www.w3.org/2004/02/skos/core#related"/>
    <skos:prefLabel>ulan2582_administered_by</skos:prefLabel>
    <skos:scopeNote>institution - administered by - person.&#13;
Example: Societe nationale des chemins de fer Francais. Agence des gares was administered by Georges Mathieu</skos:scopeNote>
    <dc:identifier>2582</dc:identifier>
  </rdf:Description>
  <rdf:Description rdf:about="http://vocab.getty.edu/term/kind/FIPSCode">
    <dct:description>FIPS region code. Used in TGN.
Example: "MX21" for Puebla, Mexico</dct:description>
    <skos:scopeNote>FIPS region code. Used in TGN</skos:scopeNote>
    <skos:notation>FIPS</skos:notation>
    <skos:inScheme rdf:resource="http://vocab.getty.edu/term/kind/"/>
    <skos:example>"MX21" for Puebla, Mexico</skos:example>
    <rdf:type rdf:resource="http://www.w3.org/2004/02/skos/core#Concept"/>
    <skos:prefLabel>FIPS Code</skos:prefLabel>
  </rdf:Description>
  <rdf:Description rdf:about="http://vocab.getty.edu/term/display/Display">
    <skos:scopeNote>Use in displays where natural order is appropriate</skos:scopeNote>
    <skos:prefLabel>Use for Display</skos:prefLabel>
    <rdf:type rdf:resource="http://www.w3.org/2004/02/skos/core#Concept"/>
    <skos:notation>D</skos:notation>
    <dct:description>Use in displays where natural order is appropriate</dct:description>
    <skos:inScheme rdf:resource="http://vocab.getty.edu/term/display/"/>
    <skos:notation>Y</skos:notation>
  </rdf:Description>
  <rdf:Description rdf:about="http://vocab.getty.edu/term/kind/ISOnumeric2">
    <skos:scopeNote>May be used in TGN, but no code of this kind is present</skos:scopeNote>
    <skos:inScheme rdf:resource="http://vocab.getty.edu/term/kind/"/>
    <skos:notation>ISO2N</skos:notation>
    <rdf:type rdf:resource="http://www.w3.org/2004/02/skos/core#Concept"/>
    <dct:description>May be used in TGN, but no code of this kind is present</dct:description>
    <skos:prefLabel>ISO numeric-2 code</skos:prefLabel>
  </rdf:Description>
  <rdf:Description rdf:about="http://vocab.getty.edu/term/kind/JargonOrSlang">
    <skos:inScheme rdf:resource="http://vocab.getty.edu/term/kind/"/>
    <skos:notation>J</skos:notation>
    <skos:prefLabel>Jargon or Slang</skos:prefLabel>
    <skos:scopeNote>Slang or jargon term. Used in AAT only</skos:scopeNote>
    <skos:example>"fool's gold" is slang for "pyrite"</skos:example>
    <rdf:type rdf:resource="http://www.w3.org/2004/02/skos/core#Concept"/>
    <dct:description>Slang or jargon term. Used in AAT only.
Example: "fool's gold" is slang for "pyrite"</dct:description>
  </rdf:Description>
  <rdf:Description rdf:about="http://vocab.getty.edu/term/kind/">
    <skos:scopeNote>Term Kind concept scheme</skos:scopeNote>
    <rdfs:isDefinedBy rdf:resource="http://vocab.getty.edu/ontology"/>
    <rdfs:label>Term Kind concept scheme</rdfs:label>
    <rdf:type rdf:resource="http://www.w3.org/2004/02/skos/core#ConceptScheme"/>
    <skos:prefLabel>Term Kind concept scheme</skos:prefLabel>
    <dct:description>Term Kind concept scheme</dct:description>
  </rdf:Description>
  <rdf:Description rdf:about="http://vocab.getty.edu/ontology#ulan1544_significant_other_of">
    <rdfs:domain rdf:resource="http://www.w3.org/2004/02/skos/core#Concept"/>
    <rdfs:isDefinedBy rdf:resource="http://vocab.getty.edu/ulan/"/>
    <rdfs:subPropertyOf rdf:resource="http://www.w3.org/2004/02/skos/core#related"/>
    <rdf:type rdf:resource="http://www.w3.org/2002/07/owl#SymmetricProperty"/>
    <skos:prefLabel>ulan1544_significant_other_of</skos:prefLabel>
    <rdf:type rdf:resource="http://www.w3.org/2002/07/owl#ObjectProperty"/>
    <rdfs:isDefinedBy rdf:resource="http://vocab.getty.edu/ontology"/>
    <dct:description>person - significant other of - person.&#13;
Example: Jeanne Hebuterne was the significant other of Amedeo Modigliani</dct:description>
    <dc:title>significant other of - person</dc:title>
    <dc:identifier>1544</dc:identifier>
    <rdfs:range rdf:resource="http://www.w3.org/2004/02/skos/core#Concept"/>
    <skos:example>Jeanne Hebuterne was the significant other of Amedeo Modigliani</skos:example>
    <skos:scopeNote>person - significant other of - person.&#13;
Example: Jeanne Hebuterne was the significant other of Amedeo Modigliani</skos:scopeNote>
  </rdf:Description>
  <rdf:Description rdf:about="http://vocab.getty.edu/ontology#aat2424_produced_by">
    <dct:description>material - [is] produced by - activity/event/process.&#13;
Example: wire is produced by wiredrawing; paper is produced by papermaking</dct:description>
    <rdf:type rdf:resource="http://www.w3.org/2002/07/owl#ObjectProperty"/>
    <rdfs:isDefinedBy rdf:resource="http://vocab.getty.edu/ontology"/>
    <skos:example>wire is produced by wiredrawing</skos:example>
    <rdfs:domain rdf:resource="http://www.w3.org/2004/02/skos/core#Concept"/>
    <rdfs:subPropertyOf rdf:resource="http://www.w3.org/2004/02/skos/core#related"/>
    <rdfs:range rdf:resource="http://www.w3.org/2004/02/skos/core#Concept"/>
    <skos:scopeNote>material - [is] produced by - activity/event/process.&#13;
Example: wire is produced by wiredrawing; paper is produced by papermaking</skos:scopeNote>
    <dc:identifier>2424</dc:identifier>
    <owl:inverseOf rdf:resource="http://vocab.getty.edu/ontology#aat2425_produces"/>
    <skos:prefLabel>aat2424_produced_by</skos:prefLabel>
    <dc:title>produced by - activity/event/process</dc:title>
    <rdfs:isDefinedBy rdf:resource="http://vocab.getty.edu/aat/"/>
    <skos:example>paper is produced by papermaking</skos:example>
  </rdf:Description>
  <rdf:Description rdf:about="http://vocab.getty.edu/ontology#ulan1513_grandchild_of">
    <skos:example>Eric Lloyd Wright is the grandchild of Frank Lloyd Wright</skos:example>
    <rdfs:subPropertyOf rdf:resource="http://www.w3.org/2004/02/skos/core#related"/>
    <owl:inverseOf rdf:resource="http://vocab.getty.edu/ontology#ulan1514_gandparent_of"/>
    <rdfs:isDefinedBy rdf:resource="http://vocab.getty.edu/ontology"/>
    <skos:scopeNote>person - grandchild of - person.&#13;
Example: Eric Lloyd Wright is the grandchild of Frank Lloyd Wright</skos:scopeNote>
    <rdf:type rdf:resource="http://www.w3.org/2002/07/owl#ObjectProperty"/>
    <skos:prefLabel>ulan1513_grandchild_of</skos:prefLabel>
    <rdfs:range rdf:resource="http://www.w3.org/2004/02/skos/core#Concept"/>
    <rdfs:domain rdf:resource="http://www.w3.org/2004/02/skos/core#Concept"/>
    <dct:description>person - grandchild of - person.&#13;
Example: Eric Lloyd Wright is the grandchild of Frank Lloyd Wright</dct:description>
    <rdfs:isDefinedBy rdf:resource="http://vocab.getty.edu/ulan/"/>
    <dc:title>grandchild of - person</dc:title>
    <dc:identifier>1513</dc:identifier>
  </rdf:Description>
  <rdf:Description rdf:about="http://vocab.getty.edu/ontology#displayOrder">
    <rdfs:range rdf:resource="http://www.w3.org/2001/XMLSchema#positiveInteger"/>
    <dct:description>Display order of subject or term amongst its siblings.
If all are 1 then use alphabetical. Domain is gvp:Subject or skosxl:Label</dct:description>
    <rdfs:comment>Display order of subject or term amongst its siblings.
If all are 1 then use alphabetical. Domain is gvp:Subject or skosxl:Label</rdfs:comment>
    <skos:definition>Display order of subject or term amongst its siblings.
If all are 1 then use alphabetical. Domain is gvp:Subject or skosxl:Label</skos:definition>
    <rdfs:isDefinedBy rdf:resource="http://vocab.getty.edu/ontology"/>
    <skos:scopeNote>Display order of subject or term amongst its siblings.
If all are 1 then use alphabetical. Domain is gvp:Subject or skosxl:Label</skos:scopeNote>
    <rdf:type rdf:resource="http://www.w3.org/2002/07/owl#DatatypeProperty"/>
    <skos:prefLabel>displayOrder</skos:prefLabel>
    <rdfs:label>displayOrder</rdfs:label>
  </rdf:Description>
  <rdf:Description rdf:about="http://vocab.getty.edu/ontology#ulan2781_dedicatee_of">
    <owl:inverseOf rdf:resource="http://vocab.getty.edu/ontology#ulan2782_dedicated_to"/>
    <rdfs:domain rdf:resource="http://www.w3.org/2004/02/skos/core#Concept"/>
    <rdfs:range rdf:resource="http://www.w3.org/2004/02/skos/core#Concept"/>
    <dct:description>person - dedicatee of - institution.&#13;
Example: Auguste Rodin is the dedicatee of The Rodin Museum in Philadelphia</dct:description>
    <dc:identifier>2781</dc:identifier>
    <rdf:type rdf:resource="http://www.w3.org/2002/07/owl#ObjectProperty"/>
    <rdfs:isDefinedBy rdf:resource="http://vocab.getty.edu/ontology"/>
    <skos:prefLabel>ulan2781_dedicatee_of</skos:prefLabel>
    <skos:example>Auguste Rodin is the dedicatee of The Rodin Museum in Philadelphia</skos:example>
    <rdfs:subPropertyOf rdf:resource="http://www.w3.org/2004/02/skos/core#related"/>
    <skos:scopeNote>person - dedicatee of - institution.&#13;
Example: Auguste Rodin is the dedicatee of The Rodin Museum in Philadelphia</skos:scopeNote>
    <rdfs:isDefinedBy rdf:resource="http://vocab.getty.edu/ulan/"/>
    <dc:title>dedicatee of - institution</dc:title>
  </rdf:Description>
  <rdf:Description rdf:about="http://vocab.getty.edu/ontology#ulan1223_crowned_by">
    <owl:inverseOf rdf:resource="http://vocab.getty.edu/ontology#ulan1224_crowned"/>
    <rdfs:range rdf:resource="http://www.w3.org/2004/02/skos/core#Concept"/>
    <rdfs:isDefinedBy rdf:resource="http://vocab.getty.edu/ulan/"/>
    <rdfs:subPropertyOf rdf:resource="http://www.w3.org/2004/02/skos/core#related"/>
    <dct:description>person - crowned by - person.&#13;
Example: Pope Leo III crowned Emperor Charlemagne</dct:description>
    <rdf:type rdf:resource="http://www.w3.org/2002/07/owl#ObjectProperty"/>
    <dc:title>crowned by - person</dc:title>
    <rdfs:isDefinedBy rdf:resource="http://vocab.getty.edu/ontology"/>
    <skos:example>Pope Leo III crowned Emperor Charlemagne</skos:example>
    <skos:scopeNote>person - crowned by - person.&#13;
Example: Pope Leo III crowned Emperor Charlemagne</skos:scopeNote>
    <dc:identifier>1223</dc:identifier>
    <rdfs:domain rdf:resource="http://www.w3.org/2004/02/skos/core#Concept"/>
    <skos:prefLabel>ulan1223_crowned_by</skos:prefLabel>
  </rdf:Description>
  <rdf:Description rdf:about="http://vocab.getty.edu/ontology#aat2900_miscellaneous_relationship">
    <rdfs:isDefinedBy rdf:resource="http://vocab.getty.edu/ontology"/>
    <rdfs:isDefinedBy rdf:resource="http://vocab.getty.edu/aat/"/>
    <rdfs:domain rdf:resource="http://www.w3.org/2004/02/skos/core#Concept"/>
    <rdfs:range rdf:resource="http://www.w3.org/2004/02/skos/core#Concept"/>
    <skos:example>Conditions and Effects has miscellaneous relationship with Processes and Techniques</skos:example>
    <skos:scopeNote>any - [has] miscellaneous relationship [to] - any.&#13;
Example: Conditions and Effects has miscellaneous relationship with Processes and Techniques</skos:scopeNote>
    <skos:prefLabel>aat2900_miscellaneous_relationship</skos:prefLabel>
    <dc:identifier>2900</dc:identifier>
    <dc:title>miscellaneous relationship - any</dc:title>
    <rdfs:subPropertyOf rdf:resource="http://www.w3.org/2004/02/skos/core#related"/>
    <dct:description>any - [has] miscellaneous relationship [to] - any.&#13;
Example: Conditions and Effects has miscellaneous relationship with Processes and Techniques</dct:description>
    <rdf:type rdf:resource="http://www.w3.org/2002/07/owl#ObjectProperty"/>
    <rdf:type rdf:resource="http://www.w3.org/2002/07/owl#SymmetricProperty"/>
  </rdf:Description>
  <rdf:Description rdf:about="http://vocab.getty.edu/ontology#ulan2583_chairman_of">
    <dc:title>chairman of - institution</dc:title>
    <rdfs:domain rdf:resource="http://www.w3.org/2004/02/skos/core#Concept"/>
    <rdfs:range rdf:resource="http://www.w3.org/2004/02/skos/core#Concept"/>
    <rdfs:subPropertyOf rdf:resource="http://www.w3.org/2004/02/skos/core#related"/>
    <skos:prefLabel>ulan2583_chairman_of</skos:prefLabel>
    <rdfs:isDefinedBy rdf:resource="http://vocab.getty.edu/ulan/"/>
    <owl:inverseOf rdf:resource="http://vocab.getty.edu/ontology#ulan2584_chaired_by"/>
    <rdf:type rdf:resource="http://www.w3.org/2002/07/owl#ObjectProperty"/>
    <skos:scopeNote>person - chairman of - institution</skos:scopeNote>
    <rdfs:isDefinedBy rdf:resource="http://vocab.getty.edu/ontology"/>
    <dc:identifier>2583</dc:identifier>
    <dct:description>person - chairman of - institution</dct:description>
  </rdf:Description>
  <rdf:Description rdf:nodeID="N7c0ee6a758e646b284267328dc00c97c">
    <rdf:first rdf:resource="http://vocab.getty.edu/ontology#broaderPartitive"/>
    <rdf:rest rdf:resource="http://www.w3.org/1999/02/22-rdf-syntax-ns#nil"/>
  </rdf:Description>
  <rdf:Description rdf:about="http://vocab.getty.edu/ontology#Facet">
    <skos:definition>One of the major divisions of a vocabulary</skos:definition>
    <skos:prefLabel>Facet</skos:prefLabel>
    <rdf:type rdf:resource="http://www.w3.org/2002/07/owl#Class"/>
    <rdfs:subClassOf rdf:resource="http://vocab.getty.edu/ontology#Subject"/>
    <skos:scopeNote>One of the major divisions of a vocabulary.
Example: Objects Facet (AAT), World (TGN), Artists (ULAN)</skos:scopeNote>
    <skos:broader rdf:resource="http://vocab.getty.edu/ontology#Subject"/>
    <rdfs:label>Facet</rdfs:label>
    <rdfs:isDefinedBy rdf:resource="http://vocab.getty.edu/ontology"/>
    <dct:description>One of the major divisions of a vocabulary.
Example: Objects Facet (AAT), World (TGN), Artists (ULAN)</dct:description>
    <rdfs:comment>One of the major divisions of a vocabulary</rdfs:comment>
    <skos:example>Objects Facet (AAT), World (TGN), Artists (ULAN)</skos:example>
    <rdfs:subClassOf rdf:resource="http://purl.org/iso25964/skos-thes#ThesaurusArray"/>
  </rdf:Description>
  <rdf:Description rdf:about="http://vocab.getty.edu/ontology#ulan2674_professor_at">
    <rdfs:isDefinedBy rdf:resource="http://vocab.getty.edu/ontology"/>
    <rdfs:range rdf:resource="http://www.w3.org/2004/02/skos/core#Concept"/>
    <rdfs:domain rdf:resource="http://www.w3.org/2004/02/skos/core#Concept"/>
    <skos:example>Paul Klee was a professor at Bauhaus</skos:example>
    <dct:description>person - professor at - institution.&#13;
Example: Paul Klee was a professor at Bauhaus</dct:description>
    <rdfs:subPropertyOf rdf:resource="http://www.w3.org/2004/02/skos/core#related"/>
    <rdf:type rdf:resource="http://www.w3.org/2002/07/owl#ObjectProperty"/>
    <skos:prefLabel>ulan2674_professor_at</skos:prefLabel>
    <rdfs:isDefinedBy rdf:resource="http://vocab.getty.edu/ulan/"/>
    <dc:title>professor at - institution</dc:title>
    <dc:identifier>2674</dc:identifier>
    <owl:inverseOf rdf:resource="http://vocab.getty.edu/ontology#ulan2675_professor_was"/>
    <skos:scopeNote>person - professor at - institution.&#13;
Example: Paul Klee was a professor at Bauhaus</skos:scopeNote>
  </rdf:Description>
  <rdf:Description rdf:about="http://vocab.getty.edu/ontology#aat2336_has_associates">
    <rdfs:isDefinedBy rdf:resource="http://vocab.getty.edu/ontology"/>
    <rdfs:isDefinedBy rdf:resource="http://vocab.getty.edu/aat/"/>
    <rdfs:domain rdf:resource="http://www.w3.org/2004/02/skos/core#Concept"/>
    <rdfs:range rdf:resource="http://www.w3.org/2004/02/skos/core#Concept"/>
    <skos:scopeNote>style/period/culture/[relgion] - has associates - [actors having] role.&#13;
Example: Abstract (fine arts style) has associates abstract artists; Roman Catholicism has associates popes</skos:scopeNote>
    <skos:prefLabel>aat2336_has_associates</skos:prefLabel>
    <skos:example>Roman Catholicism has associates popes</skos:example>
    <dc:identifier>2336</dc:identifier>
    <rdfs:subPropertyOf rdf:resource="http://www.w3.org/2004/02/skos/core#related"/>
    <dct:description>style/period/culture/[relgion] - has associates - [actors having] role.&#13;
Example: Abstract (fine arts style) has associates abstract artists; Roman Catholicism has associates popes</dct:description>
    <dc:title>has associates - role</dc:title>
    <rdf:type rdf:resource="http://www.w3.org/2002/07/owl#ObjectProperty"/>
    <skos:example>Abstract (fine arts style) has associates abstract artists</skos:example>
  </rdf:Description>
  <rdf:Description rdf:about="http://vocab.getty.edu/term/kind/Pseudonym">
    <skos:prefLabel>Pseudonym</skos:prefLabel>
    <skos:scopeNote>Used in TGN and ULAN</skos:scopeNote>
    <rdf:type rdf:resource="http://www.w3.org/2004/02/skos/core#Concept"/>
    <skos:example>"Frisco" is nickname for San Francisco (TGN)</skos:example>
    <skos:notation>P</skos:notation>
    <dct:description>Used in TGN and ULAN.
Example: "Frisco" is nickname for San Francisco (TGN)</dct:description>
    <skos:inScheme rdf:resource="http://vocab.getty.edu/term/kind/"/>
  </rdf:Description>
  <rdf:Description rdf:about="http://vocab.getty.edu/ontology#ulan1213_court_artist_to">
    <rdf:type rdf:resource="http://www.w3.org/2002/07/owl#ObjectProperty"/>
    <dc:title>court artist to - person</dc:title>
    <rdfs:isDefinedBy rdf:resource="http://vocab.getty.edu/ulan/"/>
    <skos:scopeNote>person - court artist to - person.&#13;
Example: Court artist to Gonzaga Vincenzo I, Duke of Mantua was Peter Paul Rubens; court artist to Charles IV, King of Spain was Francisco de Goya</skos:scopeNote>
    <skos:prefLabel>ulan1213_court_artist_to</skos:prefLabel>
    <owl:inverseOf rdf:resource="http://vocab.getty.edu/ontology#ulan1214_court_artist_was"/>
    <rdfs:subPropertyOf rdf:resource="http://www.w3.org/2004/02/skos/core#related"/>
    <dc:identifier>1213</dc:identifier>
    <rdfs:domain rdf:resource="http://www.w3.org/2004/02/skos/core#Concept"/>
    <rdfs:range rdf:resource="http://www.w3.org/2004/02/skos/core#Concept"/>
    <dct:description>person - court artist to - person.&#13;
Example: Court artist to Gonzaga Vincenzo I, Duke of Mantua was Peter Paul Rubens; court artist to Charles IV, King of Spain was Francisco de Goya</dct:description>
    <skos:example>court artist to Charles IV, King of Spain was Francisco de Goya</skos:example>
    <rdfs:isDefinedBy rdf:resource="http://vocab.getty.edu/ontology"/>
    <skos:example>Court artist to Gonzaga Vincenzo I, Duke of Mantua was Peter Paul Rubens</skos:example>
  </rdf:Description>
  <rdf:Description rdf:about="http://vocab.getty.edu/term/POS/Adjectival">
    <skos:scopeNote>This term may be combined with others in post-coordinated compound terms</skos:scopeNote>
    <skos:prefLabel>Adjectival</skos:prefLabel>
    <skos:inScheme rdf:resource="http://vocab.getty.edu/term/POS/"/>
    <skos:notation>A</skos:notation>
    <rdf:type rdf:resource="http://www.w3.org/2004/02/skos/core#Concept"/>
    <skos:example>"Renaissance" (as in "Renaissance cathedral"), "painter's" (as in "painter's smock")</skos:example>
    <dct:description>This term may be combined with others in post-coordinated compound terms.
Example: "Renaissance" (as in "Renaissance cathedral"), "painter's" (as in "painter's smock")</dct:description>
  </rdf:Description>
  <rdf:Description rdf:nodeID="Nb94f42dcb520415381be684e6f7568e7">
    <rdf:rest rdf:resource="http://www.w3.org/1999/02/22-rdf-syntax-ns#nil"/>
    <rdf:first rdf:resource="http://vocab.getty.edu/ontology#broaderGeneric"/>
  </rdf:Description>
  <rdf:Description rdf:about="http://vocab.getty.edu/ontology#ulan1590_possibly_related_to">
    <skos:prefLabel>ulan1590_possibly_related_to</skos:prefLabel>
    <skos:scopeNote>person - possibly related to (familial relationship) - person.&#13;
Example: A familial relationship between Ramon Destorrents, the younger and Ramon Destorrents, the elder is possible</skos:scopeNote>
    <rdf:type rdf:resource="http://www.w3.org/2002/07/owl#SymmetricProperty"/>
    <dct:description>person - possibly related to (familial relationship) - person.&#13;
Example: A familial relationship between Ramon Destorrents, the younger and Ramon Destorrents, the elder is possible</dct:description>
    <dc:identifier>1590</dc:identifier>
    <rdfs:isDefinedBy rdf:resource="http://vocab.getty.edu/ulan/"/>
    <rdfs:subPropertyOf rdf:resource="http://www.w3.org/2004/02/skos/core#related"/>
    <rdfs:range rdf:resource="http://www.w3.org/2004/02/skos/core#Concept"/>
    <rdfs:domain rdf:resource="http://www.w3.org/2004/02/skos/core#Concept"/>
    <skos:example>A familial relationship between Ramon Destorrents, the younger and Ramon Destorrents, the elder is possible</skos:example>
    <rdf:type rdf:resource="http://www.w3.org/2002/07/owl#ObjectProperty"/>
    <rdfs:isDefinedBy rdf:resource="http://vocab.getty.edu/ontology"/>
    <dc:title>possibly related to - person</dc:title>
  </rdf:Description>
  <rdf:Description rdf:about="http://vocab.getty.edu/ontology#tgn3101_near-adjacent_to">
    <dct:description>any - near/adjacent to - any.&#13;
Example: Saint Paul (Minnesota, USA), is linked to its 'Twin City' Minneapolis (Hennepin county, Minnesota, USA)</dct:description>
    <rdf:type rdf:resource="http://www.w3.org/2002/07/owl#SymmetricProperty"/>
    <skos:prefLabel>tgn3101_near-adjacent_to</skos:prefLabel>
    <skos:example>Saint Paul (Minnesota, USA), is linked to its 'Twin City' Minneapolis (Hennepin county, Minnesota, USA)</skos:example>
    <dc:title>near/adjacent to - any</dc:title>
    <rdfs:isDefinedBy rdf:resource="http://vocab.getty.edu/ontology"/>
    <rdfs:subPropertyOf rdf:resource="http://www.w3.org/2004/02/skos/core#related"/>
    <rdfs:domain rdf:resource="http://www.w3.org/2004/02/skos/core#Concept"/>
    <rdfs:range rdf:resource="http://www.w3.org/2004/02/skos/core#Concept"/>
    <rdf:type rdf:resource="http://www.w3.org/2002/07/owl#ObjectProperty"/>
    <dc:identifier>3101</dc:identifier>
    <rdfs:isDefinedBy rdf:resource="http://vocab.getty.edu/tgn/"/>
    <skos:scopeNote>any - near/adjacent to - any.&#13;
Example: Saint Paul (Minnesota, USA), is linked to its 'Twin City' Minneapolis (Hennepin county, Minnesota, USA)</skos:scopeNote>
  </rdf:Description>
  <rdf:Description rdf:about="http://vocab.getty.edu/ontology#aat2409_takes_place_in">
    <skos:scopeNote>field of study/discipline - takes place in - locus/setting.&#13;
Example: education takes place in schools (buildings); medicine (discipline) takes place in hospitals (buildings)</skos:scopeNote>
    <dc:title>takes place in - locus/setting</dc:title>
    <skos:example>education takes place in schools (buildings)</skos:example>
    <dc:identifier>2409</dc:identifier>
    <rdfs:range rdf:resource="http://www.w3.org/2004/02/skos/core#Concept"/>
    <rdfs:domain rdf:resource="http://www.w3.org/2004/02/skos/core#Concept"/>
    <rdfs:isDefinedBy rdf:resource="http://vocab.getty.edu/ontology"/>
    <skos:prefLabel>aat2409_takes_place_in</skos:prefLabel>
    <rdfs:subPropertyOf rdf:resource="http://www.w3.org/2004/02/skos/core#related"/>
    <rdf:type rdf:resource="http://www.w3.org/2002/07/owl#ObjectProperty"/>
    <dct:description>field of study/discipline - takes place in - locus/setting.&#13;
Example: education takes place in schools (buildings); medicine (discipline) takes place in hospitals (buildings)</dct:description>
    <skos:example>medicine (discipline) takes place in hospitals (buildings)</skos:example>
    <rdfs:isDefinedBy rdf:resource="http://vocab.getty.edu/aat/"/>
  </rdf:Description>
  <rdf:Description rdf:about="http://vocab.getty.edu/ontology#ulan1543_consort_was">
    <rdfs:isDefinedBy rdf:resource="http://vocab.getty.edu/ulan/"/>
    <dc:identifier>1543</dc:identifier>
    <rdfs:subPropertyOf rdf:resource="http://www.w3.org/2004/02/skos/core#related"/>
    <dc:title>consort was - person</dc:title>
    <skos:prefLabel>ulan1543_consort_was</skos:prefLabel>
    <skos:scopeNote>person - consort was - person.&#13;
Example: Augustus, Emperor of Rome's consort was Empress Livia</skos:scopeNote>
    <dct:description>person - consort was - person.&#13;
Example: Augustus, Emperor of Rome's consort was Empress Livia</dct:description>
    <rdfs:range rdf:resource="http://www.w3.org/2004/02/skos/core#Concept"/>
    <rdfs:domain rdf:resource="http://www.w3.org/2004/02/skos/core#Concept"/>
    <rdf:type rdf:resource="http://www.w3.org/2002/07/owl#ObjectProperty"/>
    <skos:example>Augustus, Emperor of Rome's consort was Empress Livia</skos:example>
    <rdfs:isDefinedBy rdf:resource="http://vocab.getty.edu/ontology"/>
  </rdf:Description>
  <rdf:Description rdf:about="http://vocab.getty.edu/ontology#prefLabelGVP">
    <rdfs:range rdf:resource="http://www.w3.org/2008/05/skos-xl#Label"/>
    <rdfs:comment>Term preferred by the Getty Vocabulary Program. The language is usually English. Applicable to AAT, ULAN, TGN. Used with skosxl:prefLabel</rdfs:comment>
    <rdf:type rdf:resource="http://www.w3.org/2002/07/owl#ObjectProperty"/>
    <skos:scopeNote>Term preferred by the Getty Vocabulary Program. The language is usually English. Applicable to AAT, ULAN, TGN. Used with skosxl:prefLabel</skos:scopeNote>
    <skos:prefLabel>prefLabelGVP</skos:prefLabel>
    <rdfs:domain rdf:resource="http://vocab.getty.edu/ontology#Subject"/>
    <dct:description>Term preferred by the Getty Vocabulary Program. The language is usually English. Applicable to AAT, ULAN, TGN. Used with skosxl:prefLabel</dct:description>
    <skos:definition>Term preferred by the Getty Vocabulary Program. The language is usually English. Applicable to AAT, ULAN, TGN. Used with skosxl:prefLabel</skos:definition>
    <rdfs:isDefinedBy rdf:resource="http://vocab.getty.edu/ontology"/>
    <rdfs:label>prefLabelGVP</rdfs:label>
  </rdf:Description>
  <rdf:Description rdf:about="http://vocab.getty.edu/ontology#ulan1318_member_was">
    <rdfs:subPropertyOf rdf:resource="http://www.w3.org/2004/02/skos/core#related"/>
    <skos:example>The National Gallery of Art was/is a member of the Foundation of Documentation of Architecture</skos:example>
    <dct:description>person/firm/group - member was - firm/group.&#13;
Example: The National Gallery of Art was/is a member of the Foundation of Documentation of Architecture</dct:description>
    <dc:title>member was - firm/group</dc:title>
    <dc:identifier>1318</dc:identifier>
    <rdfs:range rdf:resource="http://www.w3.org/2004/02/skos/core#Concept"/>
    <skos:scopeNote>person/firm/group - member was - firm/group.&#13;
Example: The National Gallery of Art was/is a member of the Foundation of Documentation of Architecture</skos:scopeNote>
    <rdfs:isDefinedBy rdf:resource="http://vocab.getty.edu/ontology"/>
    <skos:prefLabel>ulan1318_member_was</skos:prefLabel>
    <rdf:type rdf:resource="http://www.w3.org/2002/07/owl#ObjectProperty"/>
    <rdfs:isDefinedBy rdf:resource="http://vocab.getty.edu/ulan/"/>
    <rdfs:domain rdf:resource="http://www.w3.org/2004/02/skos/core#Concept"/>
  </rdf:Description>
  <rdf:Description rdf:about="http://vocab.getty.edu/ontology#ulan2676_teacher_at">
    <dc:title>teacher at - institution</dc:title>
    <skos:prefLabel>ulan2676_teacher_at</skos:prefLabel>
    <rdfs:isDefinedBy rdf:resource="http://vocab.getty.edu/ulan/"/>
    <rdfs:range rdf:resource="http://www.w3.org/2004/02/skos/core#Concept"/>
    <owl:inverseOf rdf:resource="http://vocab.getty.edu/ontology#ulan2677_teacher_was"/>
    <rdfs:subPropertyOf rdf:resource="http://www.w3.org/2004/02/skos/core#related"/>
    <dct:description>person - teacher at - institution.&#13;
Example: Willem De Kooning was a teacher at Black Mountain College</dct:description>
    <dc:identifier>2676</dc:identifier>
    <rdf:type rdf:resource="http://www.w3.org/2002/07/owl#ObjectProperty"/>
    <skos:example>Willem De Kooning was a teacher at Black Mountain College</skos:example>
    <rdfs:isDefinedBy rdf:resource="http://vocab.getty.edu/ontology"/>
    <skos:scopeNote>person - teacher at - institution.&#13;
Example: Willem De Kooning was a teacher at Black Mountain College</skos:scopeNote>
    <rdfs:domain rdf:resource="http://www.w3.org/2004/02/skos/core#Concept"/>
  </rdf:Description>
  <rdf:Description rdf:about="http://vocab.getty.edu/ontology#tgn3317_member_of">
    <skos:example>Belgium is a member of the European Union since 1958</skos:example>
    <rdfs:domain rdf:resource="http://www.w3.org/2004/02/skos/core#Concept"/>
    <rdfs:range rdf:resource="http://www.w3.org/2004/02/skos/core#Concept"/>
    <rdfs:subPropertyOf rdf:resource="http://www.w3.org/2004/02/skos/core#related"/>
    <rdfs:isDefinedBy rdf:resource="http://vocab.getty.edu/ontology"/>
    <dc:identifier>3317</dc:identifier>
    <owl:inverseOf rdf:resource="http://vocab.getty.edu/ontology#tgn3318_member_is"/>
    <rdf:type rdf:resource="http://www.w3.org/2002/07/owl#ObjectProperty"/>
    <dct:description>nation - member of - union.&#13;
Example: Austria is a member of the European Union since 1915; Belgium is a member of the European Union since 1958</dct:description>
    <skos:example>Austria is a member of the European Union since 1915</skos:example>
    <rdfs:isDefinedBy rdf:resource="http://vocab.getty.edu/tgn/"/>
    <dc:title>member of - union</dc:title>
    <skos:prefLabel>tgn3317_member_of</skos:prefLabel>
    <skos:scopeNote>nation - member of - union.&#13;
Example: Austria is a member of the European Union since 1915; Belgium is a member of the European Union since 1958</skos:scopeNote>
  </rdf:Description>
  <rdf:Description rdf:about="http://vocab.getty.edu/ontology#ulan1301_colleague_of">
    <dc:title>colleague of - person</dc:title>
    <skos:example>Titian was a colleague of Maria Giovanni Verdizotti</skos:example>
    <rdfs:isDefinedBy rdf:resource="http://vocab.getty.edu/ulan/"/>
    <rdfs:domain rdf:resource="http://www.w3.org/2004/02/skos/core#Concept"/>
    <dc:identifier>1301</dc:identifier>
    <rdfs:range rdf:resource="http://www.w3.org/2004/02/skos/core#Concept"/>
    <rdf:type rdf:resource="http://www.w3.org/2002/07/owl#SymmetricProperty"/>
    <rdfs:isDefinedBy rdf:resource="http://vocab.getty.edu/ontology"/>
    <rdfs:subPropertyOf rdf:resource="http://www.w3.org/2004/02/skos/core#related"/>
    <dct:description>person - colleague of - person.&#13;
Example: Titian was a colleague of Maria Giovanni Verdizotti</dct:description>
    <rdf:type rdf:resource="http://www.w3.org/2002/07/owl#ObjectProperty"/>
    <skos:prefLabel>ulan1301_colleague_of</skos:prefLabel>
    <skos:scopeNote>person - colleague of - person.&#13;
Example: Titian was a colleague of Maria Giovanni Verdizotti</skos:scopeNote>
  </rdf:Description>
  <rdf:Description rdf:about="http://vocab.getty.edu/ontology#ulan2577_patron_was">
    <rdfs:range rdf:resource="http://www.w3.org/2004/02/skos/core#Concept"/>
    <rdfs:domain rdf:resource="http://www.w3.org/2004/02/skos/core#Concept"/>
    <rdfs:isDefinedBy rdf:resource="http://vocab.getty.edu/ontology"/>
    <rdfs:subPropertyOf rdf:resource="http://www.w3.org/2004/02/skos/core#related"/>
    <rdf:type rdf:resource="http://www.w3.org/2002/07/owl#ObjectProperty"/>
    <rdfs:isDefinedBy rdf:resource="http://vocab.getty.edu/ulan/"/>
    <dct:description>person - patron was - person.&#13;
Example: James Caulfiel, Earl of Charlemont was the patron of William Chambers</dct:description>
    <skos:prefLabel>ulan2577_patron_was</skos:prefLabel>
    <dc:title>patron was - person</dc:title>
    <dc:identifier>2577</dc:identifier>
    <skos:example>James Caulfiel, Earl of Charlemont was the patron of William Chambers</skos:example>
    <skos:scopeNote>person - patron was - person.&#13;
Example: James Caulfiel, Earl of Charlemont was the patron of William Chambers</skos:scopeNote>
  </rdf:Description>
  <rdf:Description rdf:about="http://vocab.getty.edu/ontology#ulan2578_trustee_of">
    <rdfs:isDefinedBy rdf:resource="http://vocab.getty.edu/ulan/"/>
    <rdfs:domain rdf:resource="http://www.w3.org/2004/02/skos/core#Concept"/>
    <dc:title>trustee of - institution</dc:title>
    <rdfs:range rdf:resource="http://www.w3.org/2004/02/skos/core#Concept"/>
    <skos:prefLabel>ulan2578_trustee_of</skos:prefLabel>
    <dc:identifier>2578</dc:identifier>
    <dct:description>person - trustee of - institution.&#13;
Example: George Douglas Haig was a trustee of the National Galleries of Scotland</dct:description>
    <skos:example>George Douglas Haig was a trustee of the National Galleries of Scotland</skos:example>
    <owl:inverseOf rdf:resource="http://vocab.getty.edu/ontology#ulan2579_trustee_was"/>
    <skos:scopeNote>person - trustee of - institution.&#13;
Example: George Douglas Haig was a trustee of the National Galleries of Scotland</skos:scopeNote>
    <rdfs:isDefinedBy rdf:resource="http://vocab.getty.edu/ontology"/>
    <rdfs:subPropertyOf rdf:resource="http://www.w3.org/2004/02/skos/core#related"/>
    <rdf:type rdf:resource="http://www.w3.org/2002/07/owl#ObjectProperty"/>
  </rdf:Description>
  <rdf:Description rdf:about="http://vocab.getty.edu/ontology#ulan1211_artist_to">
    <skos:scopeNote>person - artist to - person.&#13;
Example: Artist to Louis XIV, King of France was Charles-Pierre Coustou</skos:scopeNote>
    <owl:inverseOf rdf:resource="http://vocab.getty.edu/ontology#ulan1212_artist_was"/>
    <rdf:type rdf:resource="http://www.w3.org/2002/07/owl#ObjectProperty"/>
    <skos:prefLabel>ulan1211_artist_to</skos:prefLabel>
    <rdfs:range rdf:resource="http://www.w3.org/2004/02/skos/core#Concept"/>
    <rdfs:domain rdf:resource="http://www.w3.org/2004/02/skos/core#Concept"/>
    <dct:description>person - artist to - person.&#13;
Example: Artist to Louis XIV, King of France was Charles-Pierre Coustou</dct:description>
    <dc:identifier>1211</dc:identifier>
    <rdfs:isDefinedBy rdf:resource="http://vocab.getty.edu/ulan/"/>
    <dc:title>artist to - person</dc:title>
    <rdfs:subPropertyOf rdf:resource="http://www.w3.org/2004/02/skos/core#related"/>
    <rdfs:isDefinedBy rdf:resource="http://vocab.getty.edu/ontology"/>
    <skos:example>Artist to Louis XIV, King of France was Charles-Pierre Coustou</skos:example>
  </rdf:Description>
  <rdf:Description rdf:about="http://vocab.getty.edu/ontology#contributorAlternatePreferred">
    <rdfs:label>contributorAlternatePreferred</rdfs:label>
    <rdfs:range rdf:resource="http://xmlns.com/foaf/0.1/Agent"/>
    <rdfs:subPropertyOf rdf:resource="http://purl.org/dc/terms/contributor"/>
    <skos:definition>Contributor for which the term is Alternate Preferred. Range is foaf:Agent</skos:definition>
    <rdfs:comment>Contributor for which the term is Alternate Preferred. Range is foaf:Agent</rdfs:comment>
    <rdfs:domain rdf:resource="http://www.w3.org/2008/05/skos-xl#Label"/>
    <skos:prefLabel>contributorAlternatePreferred</skos:prefLabel>
    <dct:description>Contributor for which the term is Alternate Preferred. Range is foaf:Agent</dct:description>
    <rdf:type rdf:resource="http://www.w3.org/2002/07/owl#ObjectProperty"/>
    <rdfs:isDefinedBy rdf:resource="http://vocab.getty.edu/ontology"/>
    <skos:scopeNote>Contributor for which the term is Alternate Preferred. Range is foaf:Agent</skos:scopeNote>
  </rdf:Description>
  <rdf:Description rdf:about="http://vocab.getty.edu/ontology#ulan2840_performer_with">
    <rdfs:isDefinedBy rdf:resource="http://vocab.getty.edu/ulan/"/>
    <skos:prefLabel>ulan2840_performer_with</skos:prefLabel>
    <dct:description>person - performer with - group</dct:description>
    <rdfs:subPropertyOf rdf:resource="http://www.w3.org/2004/02/skos/core#related"/>
    <rdfs:isDefinedBy rdf:resource="http://vocab.getty.edu/ontology"/>
    <dc:title>performer with - group</dc:title>
    <rdfs:range rdf:resource="http://www.w3.org/2004/02/skos/core#Concept"/>
    <rdf:type rdf:resource="http://www.w3.org/2002/07/owl#ObjectProperty"/>
    <skos:scopeNote>person - performer with - group</skos:scopeNote>
    <rdfs:domain rdf:resource="http://www.w3.org/2004/02/skos/core#Concept"/>
    <dc:identifier>2840</dc:identifier>
    <owl:inverseOf rdf:resource="http://vocab.getty.edu/ontology#ulan2841_performer_was"/>
  </rdf:Description>
  <rdf:Description rdf:about="http://vocab.getty.edu/ontology#ulan1310_advised_by">
    <rdfs:subPropertyOf rdf:resource="http://www.w3.org/2004/02/skos/core#related"/>
    <dc:title>advised by - person</dc:title>
    <dct:description>person - advised by - person.&#13;
Example: Henry VIII, King of England was advised by Thomas Cromwell, Earl of Essex</dct:description>
    <skos:example>Henry VIII, King of England was advised by Thomas Cromwell, Earl of Essex</skos:example>
    <rdfs:isDefinedBy rdf:resource="http://vocab.getty.edu/ulan/"/>
    <skos:prefLabel>ulan1310_advised_by</skos:prefLabel>
    <rdfs:range rdf:resource="http://www.w3.org/2004/02/skos/core#Concept"/>
    <dc:identifier>1310</dc:identifier>
    <rdfs:domain rdf:resource="http://www.w3.org/2004/02/skos/core#Concept"/>
    <skos:scopeNote>person - advised by - person.&#13;
Example: Henry VIII, King of England was advised by Thomas Cromwell, Earl of Essex</skos:scopeNote>
    <rdf:type rdf:resource="http://www.w3.org/2002/07/owl#ObjectProperty"/>
    <rdfs:isDefinedBy rdf:resource="http://vocab.getty.edu/ontology"/>
  </rdf:Description>
  <rdf:Description rdf:about="http://vocab.getty.edu/ontology#aat2295_located_in">
    <skos:example>mountains are located in mountain ranges</skos:example>
    <skos:scopeNote>locus/setting - [is] located in - locus/setting.&#13;
Example: national capitals are located in nations; mountains are located in mountain ranges</skos:scopeNote>
    <rdfs:isDefinedBy rdf:resource="http://vocab.getty.edu/aat/"/>
    <skos:example>national capitals are located in nations</skos:example>
    <dc:title>located in - locus/setting</dc:title>
    <rdfs:isDefinedBy rdf:resource="http://vocab.getty.edu/ontology"/>
    <rdfs:domain rdf:resource="http://www.w3.org/2004/02/skos/core#Concept"/>
    <rdfs:range rdf:resource="http://www.w3.org/2004/02/skos/core#Concept"/>
    <skos:prefLabel>aat2295_located_in</skos:prefLabel>
    <rdf:type rdf:resource="http://www.w3.org/2002/07/owl#ObjectProperty"/>
    <dc:identifier>2295</dc:identifier>
    <dct:description>locus/setting - [is] located in - locus/setting.&#13;
Example: national capitals are located in nations; mountains are located in mountain ranges</dct:description>
    <rdfs:subPropertyOf rdf:resource="http://www.w3.org/2004/02/skos/core#related"/>
  </rdf:Description>
  <rdf:Description rdf:about="http://vocab.getty.edu/ontology#Infer_skosBroader_PropChainType2">
    <ptop:conclusion rdf:resource="http://www.w3.org/2004/02/skos/core#broader"/>
    <ptop:premise2 rdf:resource="http://vocab.getty.edu/ontology#broader"/>
    <rdf:type rdf:resource="http://www.ontotext.com/proton/protontop#PropChainType2"/>
    <ptop:premise1 rdf:resource="http://vocab.getty.edu/ontology#broaderNonConcept"/>
    <ptop:type2 rdf:resource="http://www.w3.org/2004/02/skos/core#Concept"/>
  </rdf:Description>
  <rdf:Description rdf:about="http://vocab.getty.edu/ontology#aat2848_involved_in">
    <rdfs:isDefinedBy rdf:resource="http://vocab.getty.edu/aat/"/>
    <rdfs:isDefinedBy rdf:resource="http://vocab.getty.edu/ontology"/>
    <dc:identifier>2848</dc:identifier>
    <rdf:type rdf:resource="http://www.w3.org/2002/07/owl#ObjectProperty"/>
    <skos:prefLabel>aat2848_involved_in</skos:prefLabel>
    <rdfs:domain rdf:resource="http://www.w3.org/2004/02/skos/core#Concept"/>
    <rdfs:subPropertyOf rdf:resource="http://www.w3.org/2004/02/skos/core#related"/>
    <rdfs:range rdf:resource="http://www.w3.org/2004/02/skos/core#Concept"/>
    <skos:scopeNote>genus/species - is involved in - activity/event.&#13;
Example: bulls (animals) are involved in bullfighting; Equus caballus (species) is involved in polo(field sport)</skos:scopeNote>
    <skos:example>bulls (animals) are involved in bullfighting</skos:example>
    <owl:inverseOf rdf:resource="http://vocab.getty.edu/ontology#aat2849_involves"/>
    <dct:description>genus/species - is involved in - activity/event.&#13;
Example: bulls (animals) are involved in bullfighting; Equus caballus (species) is involved in polo(field sport)</dct:description>
    <dc:title>involved in - activity/event</dc:title>
    <skos:example>Equus caballus (species) is involved in polo(field sport)</skos:example>
  </rdf:Description>
  <rdf:Description rdf:about="http://vocab.getty.edu/ontology#Infer_broaderNonConcept_TypeRestr">
    <ptop:premise rdf:resource="http://vocab.getty.edu/ontology#broader"/>
    <rdf:type rdf:resource="http://www.ontotext.com/proton/protontop#TypeRestr"/>
    <ptop:type1 rdf:resource="http://www.w3.org/2004/02/skos/core#Concept"/>
    <ptop:type2 rdf:resource="http://vocab.getty.edu/ontology#GuideTerm"/>
    <ptop:conclusion rdf:resource="http://vocab.getty.edu/ontology#broaderNonConcept"/>
  </rdf:Description>
  <rdf:Description rdf:about="http://vocab.getty.edu/ontology#aat2435_context_for">
    <rdfs:range rdf:resource="http://www.w3.org/2004/02/skos/core#Concept"/>
    <skos:scopeNote>activity/event/process - [is] contextualized in - thing.&#13;
Example: funerals are the context for funeral books; Christmas is the context for Christmas trees</skos:scopeNote>
    <skos:example>Christmas is the context for Christmas trees</skos:example>
    <skos:example>funerals are the context for funeral books</skos:example>
    <dc:title>context for - things</dc:title>
    <rdfs:isDefinedBy rdf:resource="http://vocab.getty.edu/aat/"/>
    <skos:prefLabel>aat2435_context_for</skos:prefLabel>
    <rdf:type rdf:resource="http://www.w3.org/2002/07/owl#ObjectProperty"/>
    <rdfs:isDefinedBy rdf:resource="http://vocab.getty.edu/ontology"/>
    <dct:description>activity/event/process - [is] contextualized in - thing.&#13;
Example: funerals are the context for funeral books; Christmas is the context for Christmas trees</dct:description>
    <rdfs:domain rdf:resource="http://www.w3.org/2004/02/skos/core#Concept"/>
    <rdfs:subPropertyOf rdf:resource="http://www.w3.org/2004/02/skos/core#related"/>
    <dc:identifier>2435</dc:identifier>
  </rdf:Description>
  <rdf:Description rdf:about="http://vocab.getty.edu/ontology#aat2812_followed">
    <dct:description>style/period/culture/[religion/ideology] - followed  - style/period/culture/[religion/ideology].&#13;
Example: Abstract Impressionism followed Impressionist; Micoquian followed Acheulian</dct:description>
    <dc:title>followed - style/period/culture</dc:title>
    <skos:prefLabel>aat2812_followed</skos:prefLabel>
    <rdfs:range rdf:resource="http://www.w3.org/2004/02/skos/core#Concept"/>
    <rdfs:domain rdf:resource="http://www.w3.org/2004/02/skos/core#Concept"/>
    <skos:scopeNote>style/period/culture/[religion/ideology] - followed  - style/period/culture/[religion/ideology].&#13;
Example: Abstract Impressionism followed Impressionist; Micoquian followed Acheulian</skos:scopeNote>
    <rdfs:isDefinedBy rdf:resource="http://vocab.getty.edu/aat/"/>
    <dc:identifier>2812</dc:identifier>
    <rdfs:isDefinedBy rdf:resource="http://vocab.getty.edu/ontology"/>
    <skos:example>Abstract Impressionism followed Impressionist</skos:example>
    <skos:example>Micoquian followed Acheulian</skos:example>
    <rdfs:subPropertyOf rdf:resource="http://www.w3.org/2004/02/skos/core#related"/>
    <rdf:type rdf:resource="http://www.w3.org/2002/07/owl#ObjectProperty"/>
  </rdf:Description>
  <rdf:Description rdf:about="http://vocab.getty.edu/term/type/">
    <skos:scopeNote>Term Type concept scheme</skos:scopeNote>
    <rdfs:label>Term Type concept scheme</rdfs:label>
    <rdf:type rdf:resource="http://www.w3.org/2004/02/skos/core#ConceptScheme"/>
    <dct:description>Term Type concept scheme</dct:description>
    <rdfs:isDefinedBy rdf:resource="http://vocab.getty.edu/ontology"/>
    <skos:prefLabel>Term Type concept scheme</skos:prefLabel>
  </rdf:Description>
  <rdf:Description rdf:about="http://vocab.getty.edu/ontology#tgn3301_ally_of">
    <rdfs:isDefinedBy rdf:resource="http://vocab.getty.edu/tgn/"/>
    <rdf:type rdf:resource="http://www.w3.org/2002/07/owl#SymmetricProperty"/>
    <rdfs:domain rdf:resource="http://www.w3.org/2004/02/skos/core#Concept"/>
    <rdfs:range rdf:resource="http://www.w3.org/2004/02/skos/core#Concept"/>
    <dc:title>ally of - nation</dc:title>
    <dct:description>nation - ally of - nation.&#13;
Example: Siena, Arezzo, Pisa, and Pistoia were Ghibeline allies during the 13th and 14th centuries.</dct:description>
    <dc:identifier>3301</dc:identifier>
    <skos:example>Siena, Arezzo, Pisa, and Pistoia were Ghibeline allies during the 13th and 14th centuries.</skos:example>
    <rdfs:subPropertyOf rdf:resource="http://www.w3.org/2004/02/skos/core#related"/>
    <rdfs:isDefinedBy rdf:resource="http://vocab.getty.edu/ontology"/>
    <skos:prefLabel>tgn3301_ally_of</skos:prefLabel>
    <skos:scopeNote>nation - ally of - nation.&#13;
Example: Siena, Arezzo, Pisa, and Pistoia were Ghibeline allies during the 13th and 14th centuries.</skos:scopeNote>
    <rdf:type rdf:resource="http://www.w3.org/2002/07/owl#ObjectProperty"/>
  </rdf:Description>
  <rdf:Description rdf:about="http://vocab.getty.edu/ontology#aat2208_locus-setting_for">
    <rdfs:range rdf:resource="http://www.w3.org/2004/02/skos/core#Concept"/>
    <rdf:type rdf:resource="http://www.w3.org/2002/07/owl#ObjectProperty"/>
    <skos:prefLabel>aat2208_locus-setting_for</skos:prefLabel>
    <skos:example>glassworks (buildings) are the locus/setting for glassware</skos:example>
    <dc:title>locus/setting for - things</dc:title>
    <dct:description>locus/setting - [is] locus/setting for - things.&#13;
Example: glassworks (buildings) are the locus/setting for glassware; caves are the locus/setting for cave paintings</dct:description>
    <rdfs:subPropertyOf rdf:resource="http://www.w3.org/2004/02/skos/core#related"/>
    <rdfs:isDefinedBy rdf:resource="http://vocab.getty.edu/aat/"/>
    <owl:inverseOf rdf:resource="http://vocab.getty.edu/ontology#aat2209_used-located_in"/>
    <skos:scopeNote>locus/setting - [is] locus/setting for - things.&#13;
Example: glassworks (buildings) are the locus/setting for glassware; caves are the locus/setting for cave paintings</skos:scopeNote>
    <dc:identifier>2208</dc:identifier>
    <rdfs:domain rdf:resource="http://www.w3.org/2004/02/skos/core#Concept"/>
    <skos:example>caves are the locus/setting for cave paintings</skos:example>
    <rdfs:isDefinedBy rdf:resource="http://vocab.getty.edu/ontology"/>
  </rdf:Description>
  <rdf:Description rdf:about="http://vocab.getty.edu/ontology#Infer_isoBroaderInstantial">
    <ptop:premise rdf:resource="http://vocab.getty.edu/ontology#broaderInstantialExtended"/>
    <ptop:restriction rdf:resource="http://www.w3.org/2004/02/skos/core#broader"/>
    <rdf:type rdf:resource="http://www.ontotext.com/proton/protontop#PropRestr"/>
    <ptop:conclusion rdf:resource="http://purl.org/iso25964/skos-thes#broaderInstantial"/>
  </rdf:Description>
  <rdf:Description rdf:about="http://vocab.getty.edu/ontology#aat2601_possessed_by-existing_in">
    <skos:prefLabel>aat2601_possessed_by-existing_in</skos:prefLabel>
    <rdf:type rdf:resource="http://www.w3.org/2002/07/owl#ObjectProperty"/>
    <rdfs:isDefinedBy rdf:resource="http://vocab.getty.edu/ontology"/>
    <dc:title>possessed by/existing in - role</dc:title>
    <dc:identifier>2601</dc:identifier>
    <rdfs:range rdf:resource="http://www.w3.org/2004/02/skos/core#Concept"/>
    <rdfs:subPropertyOf rdf:resource="http://www.w3.org/2004/02/skos/core#related"/>
    <rdfs:domain rdf:resource="http://www.w3.org/2004/02/skos/core#Concept"/>
    <skos:scopeNote>attributes /associated concepts - [is] possessed by/existing in - role [of actors].&#13;
Example: adulthood is possessed by/existing in adults; nomadism is possessed by/existing in nomads</skos:scopeNote>
    <skos:example>adulthood is possessed by/existing in adults</skos:example>
    <owl:inverseOf rdf:resource="http://vocab.getty.edu/ontology#aat2602_possess-exist_in"/>
    <skos:example>nomadism is possessed by/existing in nomads</skos:example>
    <rdfs:isDefinedBy rdf:resource="http://vocab.getty.edu/aat/"/>
    <dct:description>attributes /associated concepts - [is] possessed by/existing in - role [of actors].&#13;
Example: adulthood is possessed by/existing in adults; nomadism is possessed by/existing in nomads</dct:description>
  </rdf:Description>
  <rdf:Description rdf:about="http://vocab.getty.edu/ontology#aat2817_derived-made_from">
    <dc:title>derived/made from - material</dc:title>
    <skos:prefLabel>aat2817_derived-made_from</skos:prefLabel>
    <rdfs:isDefinedBy rdf:resource="http://vocab.getty.edu/ontology"/>
    <owl:inverseOf rdf:resource="http://vocab.getty.edu/ontology#aat2818_source_for"/>
    <dct:description>material - [is] derived/made from - material.&#13;
Example: gypsum is derived/made from from anhydrite; wood board is derived/made from timber (lumber)</dct:description>
    <rdfs:subPropertyOf rdf:resource="http://www.w3.org/2004/02/skos/core#related"/>
    <rdf:type rdf:resource="http://www.w3.org/2002/07/owl#ObjectProperty"/>
    <rdfs:domain rdf:resource="http://www.w3.org/2004/02/skos/core#Concept"/>
    <skos:example>gypsum is derived/made from from anhydrite</skos:example>
    <dc:identifier>2817</dc:identifier>
    <rdfs:range rdf:resource="http://www.w3.org/2004/02/skos/core#Concept"/>
    <skos:example>wood board is derived/made from timber (lumber)</skos:example>
    <rdfs:isDefinedBy rdf:resource="http://vocab.getty.edu/aat/"/>
    <skos:scopeNote>material - [is] derived/made from - material.&#13;
Example: gypsum is derived/made from from anhydrite; wood board is derived/made from timber (lumber)</skos:scopeNote>
  </rdf:Description>
  <rdf:Description rdf:about="http://vocab.getty.edu/ontology#aat2822_basis_of">
    <skos:example>curves (geometric figures) are the basis of curved [form attribute]</skos:example>
    <skos:example>plummets are the basis of pencils</skos:example>
    <rdfs:subPropertyOf rdf:resource="http://www.w3.org/2004/02/skos/core#related"/>
    <skos:prefLabel>aat2822_basis_of</skos:prefLabel>
    <rdf:type rdf:resource="http://www.w3.org/2002/07/owl#ObjectProperty"/>
    <dc:identifier>2822</dc:identifier>
    <rdfs:isDefinedBy rdf:resource="http://vocab.getty.edu/ontology"/>
    <rdfs:isDefinedBy rdf:resource="http://vocab.getty.edu/aat/"/>
    <skos:example>Gothic (Medieval) is the basis of Neo-Gothic</skos:example>
    <skos:scopeNote>any - [is] basis of - any.&#13;
Example: Gothic (Medieval) is the basis of Neo-Gothic; curves (geometric figures) are the basis of curved [form attribute]; plummets are the basis of pencils</skos:scopeNote>
    <rdfs:domain rdf:resource="http://www.w3.org/2004/02/skos/core#Concept"/>
    <rdfs:range rdf:resource="http://www.w3.org/2004/02/skos/core#Concept"/>
    <dc:title>basis of - any</dc:title>
    <dct:description>any - [is] basis of - any.&#13;
Example: Gothic (Medieval) is the basis of Neo-Gothic; curves (geometric figures) are the basis of curved [form attribute]; plummets are the basis of pencils</dct:description>
  </rdf:Description>
  <rdf:Description rdf:about="http://vocab.getty.edu/ontology#UnknownPersonConcept">
    <skos:example>500355202 Unknown Bulgarian (modern) (ULAN)</skos:example>
    <skos:definition>Unknown person representing a nationality/culture (the Unknown People by Culture facet)</skos:definition>
    <rdfs:isDefinedBy rdf:resource="http://vocab.getty.edu/ontology"/>
    <rdfs:subClassOf rdf:resource="http://vocab.getty.edu/ontology#Subject"/>
    <dct:description>Unknown person representing a nationality/culture (the Unknown People by Culture facet).
Example: 500355202 Unknown Bulgarian (modern) (ULAN)</dct:description>
    <skos:scopeNote>Unknown person representing a nationality/culture (the Unknown People by Culture facet).
Example: 500355202 Unknown Bulgarian (modern) (ULAN)</skos:scopeNote>
    <skos:broader rdf:resource="http://vocab.getty.edu/ontology#Subject"/>
    <rdfs:label>UnknownPersonConcept</rdfs:label>
    <rdf:type rdf:resource="http://www.w3.org/2002/07/owl#Class"/>
    <rdfs:subClassOf rdf:resource="http://www.w3.org/2004/02/skos/core#Concept"/>
    <rdfs:comment>Unknown person representing a nationality/culture (the Unknown People by Culture facet)</rdfs:comment>
    <skos:prefLabel>UnknownPersonConcept</skos:prefLabel>
  </rdf:Description>
  <rdf:Description rdf:about="http://vocab.getty.edu/ontology#PhysAdminPlaceConcept">
    <skos:example>6003090 Kiik-Koba (TGN)</skos:example>
    <rdfs:comment>Place that is both administrative and physical. Rarely used. Used in TGN only</rdfs:comment>
    <skos:prefLabel>PhysAdminPlaceConcept</skos:prefLabel>
    <skos:definition>Place that is both administrative and physical. Rarely used. Used in TGN only</skos:definition>
    <rdfs:isDefinedBy rdf:resource="http://vocab.getty.edu/ontology"/>
    <skos:scopeNote>Place that is both administrative and physical. Rarely used. Used in TGN only.
Example: 6003090 Kiik-Koba (TGN)</skos:scopeNote>
    <rdfs:subClassOf rdf:resource="http://vocab.getty.edu/ontology#Subject"/>
    <dct:description>Place that is both administrative and physical. Rarely used. Used in TGN only.
Example: 6003090 Kiik-Koba (TGN)</dct:description>
    <rdfs:label>PhysAdminPlaceConcept</rdfs:label>
    <skos:broader rdf:resource="http://vocab.getty.edu/ontology#Subject"/>
    <rdf:type rdf:resource="http://www.w3.org/2002/07/owl#Class"/>
    <rdfs:subClassOf rdf:resource="http://www.w3.org/2004/02/skos/core#Concept"/>
  </rdf:Description>
  <rdf:Description rdf:about="http://vocab.getty.edu/ontology#aat2801_conjuncted_with">
    <dct:description>things - [are] conjuncted with - things.&#13;
Example: cups are conjuncted with saucers; dining tables are conjuncted with dining chairs</dct:description>
    <rdfs:domain rdf:resource="http://www.w3.org/2004/02/skos/core#Concept"/>
    <rdfs:range rdf:resource="http://www.w3.org/2004/02/skos/core#Concept"/>
    <dc:identifier>2801</dc:identifier>
    <skos:example>cups are conjuncted with saucers</skos:example>
    <rdfs:isDefinedBy rdf:resource="http://vocab.getty.edu/aat/"/>
    <rdf:type rdf:resource="http://www.w3.org/2002/07/owl#ObjectProperty"/>
    <dc:title>conjuncted with - things</dc:title>
    <skos:example>dining tables are conjuncted with dining chairs</skos:example>
    <rdfs:isDefinedBy rdf:resource="http://vocab.getty.edu/ontology"/>
    <skos:scopeNote>things - [are] conjuncted with - things.&#13;
Example: cups are conjuncted with saucers; dining tables are conjuncted with dining chairs</skos:scopeNote>
    <rdf:type rdf:resource="http://www.w3.org/2002/07/owl#SymmetricProperty"/>
    <skos:prefLabel>aat2801_conjuncted_with</skos:prefLabel>
    <rdfs:subPropertyOf rdf:resource="http://www.w3.org/2004/02/skos/core#related"/>
  </rdf:Description>
  <rdf:Description rdf:about="http://vocab.getty.edu/term/kind/Neologism">
    <skos:notation>N</skos:notation>
    <skos:prefLabel>Neologism</skos:prefLabel>
    <rdf:type rdf:resource="http://www.w3.org/2004/02/skos/core#Concept"/>
    <skos:example>"folksonomy", "podcasting"</skos:example>
    <skos:scopeNote>Term that is new to the language, generally having been coined due to new technology. Used in AAT only.</skos:scopeNote>
    <skos:inScheme rdf:resource="http://vocab.getty.edu/term/kind/"/>
    <dct:description>Term that is new to the language, generally having been coined due to new technology. Used in AAT only..
Example: "folksonomy", "podcasting"</dct:description>
  </rdf:Description>
  <rdf:Description rdf:about="http://vocab.getty.edu/term/kind/ISOalpha2">
    <rdf:type rdf:resource="http://www.w3.org/2004/02/skos/core#Concept"/>
    <skos:prefLabel>ISO alpha-2 code</skos:prefLabel>
    <skos:scopeNote>ISO 3166-1 alpha-2 country code. Used in TGN</skos:scopeNote>
    <dct:description>ISO 3166-1 alpha-2 country code. Used in TGN.
Example: "AQ" for Antarctica</dct:description>
    <skos:notation>ISO2L</skos:notation>
    <skos:inScheme rdf:resource="http://vocab.getty.edu/term/kind/"/>
    <skos:example>"AQ" for Antarctica</skos:example>
  </rdf:Description>
  <rdf:Description rdf:about="http://vocab.getty.edu/ontology#tgn3104_is_location_of">
    <dc:identifier>3104</dc:identifier>
    <skos:scopeNote>place - is location of - place.&#13;
Example: tgn:7031416 Silk Road is location of tgn:7018835 Palmyra</skos:scopeNote>
    <rdf:type rdf:resource="http://www.w3.org/2002/07/owl#ObjectProperty"/>
    <rdfs:domain rdf:resource="http://www.w3.org/2004/02/skos/core#Concept"/>
    <skos:example>tgn:7031416 Silk Road is location of tgn:7018835 Palmyra</skos:example>
    <dct:description>place - is location of - place.&#13;
Example: tgn:7031416 Silk Road is location of tgn:7018835 Palmyra</dct:description>
    <dc:title>is location of - place</dc:title>
    <rdfs:isDefinedBy rdf:resource="http://vocab.getty.edu/ontology"/>
    <rdfs:isDefinedBy rdf:resource="http://vocab.getty.edu/tgn/"/>
    <skos:prefLabel>tgn3104_is_location_of</skos:prefLabel>
    <rdfs:subPropertyOf rdf:resource="http://www.w3.org/2004/02/skos/core#related"/>
    <rdfs:range rdf:resource="http://www.w3.org/2004/02/skos/core#Concept"/>
  </rdf:Description>
  <rdf:Description rdf:about="http://vocab.getty.edu/term/POS/VerbalNounGerund">
    <rdf:type rdf:resource="http://www.w3.org/2004/02/skos/core#Concept"/>
    <skos:notation>VN</skos:notation>
    <dct:description>Term is a verbal noun or gerund.
Example: polishing</dct:description>
    <skos:inScheme rdf:resource="http://vocab.getty.edu/term/POS/"/>
    <skos:example>polishing</skos:example>
    <skos:scopeNote>Term is a verbal noun or gerund</skos:scopeNote>
    <skos:prefLabel>Verbal Noun/Gerund</skos:prefLabel>
  </rdf:Description>
  <rdf:Description rdf:about="http://vocab.getty.edu/ontology#estStart">
    <rdf:type rdf:resource="http://www.w3.org/2002/07/owl#DatatypeProperty"/>
    <dct:description>Estimated start date of term, relation, type assignment, event, biography</dct:description>
    <rdfs:isDefinedBy rdf:resource="http://vocab.getty.edu/ontology"/>
    <rdfs:label>estStart</rdfs:label>
    <skos:prefLabel>estStart</skos:prefLabel>
    <rdfs:comment>Estimated start date of term, relation, type assignment, event, biography</rdfs:comment>
    <skos:definition>Estimated start date of term, relation, type assignment, event, biography</skos:definition>
    <skos:scopeNote>Estimated start date of term, relation, type assignment, event, biography</skos:scopeNote>
  </rdf:Description>
  <rdf:Description rdf:about="http://vocab.getty.edu/ontology#aat2321_used_by">
    <dct:description>things/equipment - [are] used by - [actors having] role.&#13;
Example: violoncellos are used by violoncellists; surveying instruments are used by surveyors</dct:description>
    <rdfs:range rdf:resource="http://www.w3.org/2004/02/skos/core#Concept"/>
    <rdfs:domain rdf:resource="http://www.w3.org/2004/02/skos/core#Concept"/>
    <rdfs:isDefinedBy rdf:resource="http://vocab.getty.edu/aat/"/>
    <dc:title>used by - role</dc:title>
    <skos:prefLabel>aat2321_used_by</skos:prefLabel>
    <rdf:type rdf:resource="http://www.w3.org/2002/07/owl#ObjectProperty"/>
    <skos:example>surveying instruments are used by surveyors</skos:example>
    <rdfs:isDefinedBy rdf:resource="http://vocab.getty.edu/ontology"/>
    <dc:identifier>2321</dc:identifier>
    <skos:scopeNote>things/equipment - [are] used by - [actors having] role.&#13;
Example: violoncellos are used by violoncellists; surveying instruments are used by surveyors</skos:scopeNote>
    <rdfs:subPropertyOf rdf:resource="http://www.w3.org/2004/02/skos/core#related"/>
    <owl:inverseOf rdf:resource="http://vocab.getty.edu/ontology#aat2322_use"/>
    <skos:example>violoncellos are used by violoncellists</skos:example>
  </rdf:Description>
  <rdf:Description rdf:about="http://www.getty.edu/research/">
    <foaf:name>Getty Research Institute</foaf:name>
    <rdf:type rdf:resource="http://xmlns.com/foaf/0.1/Organization"/>
    <skos:prefLabel>Getty Research Institute</skos:prefLabel>
    <rdfs:label>Getty Research Institute</rdfs:label>
  </rdf:Description>
  <rdf:Description rdf:about="http://vocab.getty.edu/ontology#aat2205_causes-is_required">
    <rdf:type rdf:resource="http://www.w3.org/2002/07/owl#ObjectProperty"/>
    <skos:example>on-demand printing causes/is required for on-demand publishing</skos:example>
    <skos:scopeNote>activity/event/[process/function] - causes/is required for - activity/event/[process/function].&#13;
Example: on-demand printing causes/is required for on-demand publishing;  preserving causes/is required for preservation</skos:scopeNote>
    <rdfs:subPropertyOf rdf:resource="http://www.w3.org/2004/02/skos/core#related"/>
    <skos:prefLabel>aat2205_causes-is_required</skos:prefLabel>
    <rdfs:range rdf:resource="http://www.w3.org/2004/02/skos/core#Concept"/>
    <rdfs:isDefinedBy rdf:resource="http://vocab.getty.edu/aat/"/>
    <dc:identifier>2205</dc:identifier>
    <rdfs:domain rdf:resource="http://www.w3.org/2004/02/skos/core#Concept"/>
    <dc:title>causes/is required - activity/event</dc:title>
    <rdfs:isDefinedBy rdf:resource="http://vocab.getty.edu/ontology"/>
    <owl:inverseOf rdf:resource="http://vocab.getty.edu/ontology#aat2206_caused_by-requires"/>
    <dct:description>activity/event/[process/function] - causes/is required for - activity/event/[process/function].&#13;
Example: on-demand printing causes/is required for on-demand publishing;  preserving causes/is required for preservation</dct:description>
    <skos:example>preserving causes/is required for preservation</skos:example>
  </rdf:Description>
  <rdf:Description rdf:about="http://vocab.getty.edu/ontology#aat2846_locus-setting_for">
    <skos:example>vineyards are the locus/setting of Vitaceae (family)</skos:example>
    <dct:description>locus/setting - [is] locus/setting for - genus/species.&#13;
Example: elephant houses are the locus/setting for Elephantidae(family); vineyards are the locus/setting of Vitaceae (family)</dct:description>
    <dc:identifier>2846</dc:identifier>
    <rdfs:subPropertyOf rdf:resource="http://www.w3.org/2004/02/skos/core#related"/>
    <skos:example>elephant houses are the locus/setting for Elephantidae(family)</skos:example>
    <rdfs:isDefinedBy rdf:resource="http://vocab.getty.edu/ontology"/>
    <dc:title>locus/setting for - genus/species</dc:title>
    <rdf:type rdf:resource="http://www.w3.org/2002/07/owl#ObjectProperty"/>
    <rdfs:isDefinedBy rdf:resource="http://vocab.getty.edu/aat/"/>
    <skos:prefLabel>aat2846_locus-setting_for</skos:prefLabel>
    <skos:scopeNote>locus/setting - [is] locus/setting for - genus/species.&#13;
Example: elephant houses are the locus/setting for Elephantidae(family); vineyards are the locus/setting of Vitaceae (family)</skos:scopeNote>
    <rdfs:range rdf:resource="http://www.w3.org/2004/02/skos/core#Concept"/>
    <rdfs:domain rdf:resource="http://www.w3.org/2004/02/skos/core#Concept"/>
  </rdf:Description>
  <rdf:Description rdf:about="http://vocab.getty.edu/term/kind/FullTerm">
    <rdf:type rdf:resource="http://www.w3.org/2004/02/skos/core#Concept"/>
    <dct:description>Full-form term. Used when the descriptor is a shorter form, or the subject also includes an Abbreviation. Used in AAT only.
Example: "Extensible Markup Language" is the full term for "XML" (which is preferred)</dct:description>
    <skos:scopeNote>Full-form term. Used when the descriptor is a shorter form, or the subject also includes an Abbreviation. Used in AAT only</skos:scopeNote>
    <skos:inScheme rdf:resource="http://vocab.getty.edu/term/kind/"/>
    <skos:notation>F</skos:notation>
    <skos:example>"Extensible Markup Language" is the full term for "XML" (which is preferred)</skos:example>
    <skos:prefLabel>Full term</skos:prefLabel>
  </rdf:Description>
  <rdf:Description rdf:about="http://vocab.getty.edu/term/display/Indexing">
    <skos:notation>I</skos:notation>
    <dct:description>Use in indexes or permuted lists where inverted order is appropriate</dct:description>
    <skos:prefLabel>Use in Indexes/lists</skos:prefLabel>
    <skos:scopeNote>Use in indexes or permuted lists where inverted order is appropriate</skos:scopeNote>
    <skos:inScheme rdf:resource="http://vocab.getty.edu/term/display/"/>
    <rdf:type rdf:resource="http://www.w3.org/2004/02/skos/core#Concept"/>
  </rdf:Description>
  <rdf:Description rdf:about="http://vocab.getty.edu/ontology#ulan2778_owner_of">
    <rdfs:isDefinedBy rdf:resource="http://vocab.getty.edu/ulan/"/>
    <dct:description>firm - owner of - person.&#13;
Example: Walter Scott Lenox was the owner of Lenox China Co.</dct:description>
    <dc:identifier>2778</dc:identifier>
    <rdf:type rdf:resource="http://www.w3.org/2002/07/owl#ObjectProperty"/>
    <rdfs:isDefinedBy rdf:resource="http://vocab.getty.edu/ontology"/>
    <dc:title>owner of - person</dc:title>
    <rdfs:range rdf:resource="http://www.w3.org/2004/02/skos/core#Concept"/>
    <owl:inverseOf rdf:resource="http://vocab.getty.edu/ontology#ulan2779_owned_by"/>
    <skos:example>Walter Scott Lenox was the owner of Lenox China Co.</skos:example>
    <skos:prefLabel>ulan2778_owner_of</skos:prefLabel>
    <rdfs:domain rdf:resource="http://www.w3.org/2004/02/skos/core#Concept"/>
    <skos:scopeNote>firm - owner of - person.&#13;
Example: Walter Scott Lenox was the owner of Lenox China Co.</skos:scopeNote>
    <rdfs:subPropertyOf rdf:resource="http://www.w3.org/2004/02/skos/core#related"/>
  </rdf:Description>
  <rdf:Description rdf:about="http://vocab.getty.edu/ontology#ulan1316_principal_was">
    <skos:example>Orazio Fontana was principal in Fontana Workshop</skos:example>
    <rdfs:isDefinedBy rdf:resource="http://vocab.getty.edu/ontology"/>
    <skos:prefLabel>ulan1316_principal_was</skos:prefLabel>
    <rdf:type rdf:resource="http://www.w3.org/2002/07/owl#ObjectProperty"/>
    <rdfs:isDefinedBy rdf:resource="http://vocab.getty.edu/ulan/"/>
    <dct:description>firm - principal was - person.&#13;
Example: Orazio Fontana was principal in Fontana Workshop</dct:description>
    <rdfs:domain rdf:resource="http://www.w3.org/2004/02/skos/core#Concept"/>
    <rdfs:range rdf:resource="http://www.w3.org/2004/02/skos/core#Concept"/>
    <rdfs:subPropertyOf rdf:resource="http://www.w3.org/2004/02/skos/core#related"/>
    <dc:title>principal was - person</dc:title>
    <dc:identifier>1316</dc:identifier>
    <skos:scopeNote>firm - principal was - person.&#13;
Example: Orazio Fontana was principal in Fontana Workshop</skos:scopeNote>
  </rdf:Description>
  <rdf:Description rdf:about="http://vocab.getty.edu/ontology#ulan2651_publisher_of">
    <skos:scopeNote>firm - publisher of - person.&#13;
Example: Negretti and Zambra was the publisher of Pierre Joseph Rossier</skos:scopeNote>
    <skos:example>Negretti and Zambra was the publisher of Pierre Joseph Rossier</skos:example>
    <skos:prefLabel>ulan2651_publisher_of</skos:prefLabel>
    <rdfs:isDefinedBy rdf:resource="http://vocab.getty.edu/ulan/"/>
    <rdfs:subPropertyOf rdf:resource="http://www.w3.org/2004/02/skos/core#related"/>
    <rdfs:domain rdf:resource="http://www.w3.org/2004/02/skos/core#Concept"/>
    <dct:description>firm - publisher of - person.&#13;
Example: Negretti and Zambra was the publisher of Pierre Joseph Rossier</dct:description>
    <rdfs:range rdf:resource="http://www.w3.org/2004/02/skos/core#Concept"/>
    <dc:title>publisher of - person</dc:title>
    <rdf:type rdf:resource="http://www.w3.org/2002/07/owl#ObjectProperty"/>
    <rdfs:isDefinedBy rdf:resource="http://vocab.getty.edu/ontology"/>
    <dc:identifier>2651</dc:identifier>
  </rdf:Description>
  <rdf:Description rdf:about="http://vocab.getty.edu/ontology#aat2554_reflects">
    <dc:identifier>2554</dc:identifier>
    <dc:title>reflects - style/period/culture</dc:title>
    <skos:prefLabel>aat2554_reflects</skos:prefLabel>
    <rdfs:domain rdf:resource="http://www.w3.org/2004/02/skos/core#Concept"/>
    <rdfs:range rdf:resource="http://www.w3.org/2004/02/skos/core#Concept"/>
    <rdfs:isDefinedBy rdf:resource="http://vocab.getty.edu/aat/"/>
    <owl:inverseOf rdf:resource="http://vocab.getty.edu/ontology#aat2555_reflected_in"/>
    <skos:scopeNote>activity/event - reflects - style/period/culture /[religion/ideology].&#13;
Example: dhokra (casting technique) reflects Dhokra (culture); red-figure vase painting reflects Red-figure [style]</skos:scopeNote>
    <skos:example>dhokra (casting technique) reflects Dhokra (culture)</skos:example>
    <skos:example>red-figure vase painting reflects Red-figure [style]</skos:example>
    <rdfs:isDefinedBy rdf:resource="http://vocab.getty.edu/ontology"/>
    <dct:description>activity/event - reflects - style/period/culture /[religion/ideology].&#13;
Example: dhokra (casting technique) reflects Dhokra (culture); red-figure vase painting reflects Red-figure [style]</dct:description>
    <rdfs:subPropertyOf rdf:resource="http://www.w3.org/2004/02/skos/core#related"/>
    <rdf:type rdf:resource="http://www.w3.org/2002/07/owl#ObjectProperty"/>
  </rdf:Description>
  <rdf:Description rdf:about="http://vocab.getty.edu/ontology#eventPreferred">
    <rdfs:range rdf:resource="http://purl.org/vocab/bio/0.1/Event"/>
    <skos:definition>Preferred life event of an ULAN agent. Domain is schema:Person/Organization, range is bio:Event</skos:definition>
    <rdfs:subPropertyOf rdf:resource="http://purl.org/vocab/bio/0.1/event"/>
    <skos:prefLabel>eventPreferred</skos:prefLabel>
    <skos:scopeNote>Preferred life event of an ULAN agent. Domain is schema:Person/Organization, range is bio:Event</skos:scopeNote>
    <rdf:type rdf:resource="http://www.w3.org/2002/07/owl#ObjectProperty"/>
    <rdfs:label>eventPreferred</rdfs:label>
    <rdfs:isDefinedBy rdf:resource="http://vocab.getty.edu/ontology"/>
    <rdfs:comment>Preferred life event of an ULAN agent. Domain is schema:Person/Organization, range is bio:Event</rdfs:comment>
    <dct:description>Preferred life event of an ULAN agent. Domain is schema:Person/Organization, range is bio:Event</dct:description>
  </rdf:Description>
  <rdf:Description rdf:about="http://vocab.getty.edu/ontology#Infer_broaderNonConcept_PropChainType2">
    <ptop:premise2 rdf:resource="http://vocab.getty.edu/ontology#broader"/>
    <rdf:type rdf:resource="http://www.ontotext.com/proton/protontop#PropChainType2"/>
    <ptop:premise1 rdf:resource="http://vocab.getty.edu/ontology#broaderNonConcept"/>
    <ptop:type2 rdf:resource="http://vocab.getty.edu/ontology#GuideTerm"/>
    <ptop:conclusion rdf:resource="http://vocab.getty.edu/ontology#broaderNonConcept"/>
  </rdf:Description>
  <rdf:Description rdf:about="http://vocab.getty.edu/term/flag/LoanTerm">
    <skos:inScheme rdf:resource="http://vocab.getty.edu/term/flag/"/>
    <skos:notation>L</skos:notation>
    <skos:scopeNote>Term borrowed from another language that has become naturalized in American English</skos:scopeNote>
    <dct:description>Term borrowed from another language that has become naturalized in American English.
Example: papier mache</dct:description>
    <rdf:type rdf:resource="http://www.w3.org/2004/02/skos/core#Concept"/>
    <skos:prefLabel>Loan Term</skos:prefLabel>
    <skos:example>papier mache</skos:example>
  </rdf:Description>
  <rdf:Description rdf:about="http://vocab.getty.edu/ontology#aat2882_reflect">
    <skos:prefLabel>aat2882_reflect</skos:prefLabel>
    <rdfs:domain rdf:resource="http://www.w3.org/2004/02/skos/core#Concept"/>
    <rdfs:isDefinedBy rdf:resource="http://vocab.getty.edu/ontology"/>
    <dc:identifier>2882</dc:identifier>
    <rdfs:range rdf:resource="http://www.w3.org/2004/02/skos/core#Concept"/>
    <rdfs:subPropertyOf rdf:resource="http://www.w3.org/2004/02/skos/core#related"/>
    <rdf:type rdf:resource="http://www.w3.org/2002/07/owl#ObjectProperty"/>
    <dc:title>reflect - language</dc:title>
    <dct:description>things - reflect - language.&#13;
Example: Greek alphabet reflects Greek (language); Vedas reflect Sanskrit</dct:description>
    <skos:example>Vedas reflect Sanskrit</skos:example>
    <rdfs:isDefinedBy rdf:resource="http://vocab.getty.edu/aat/"/>
    <skos:example>Greek alphabet reflects Greek (language)</skos:example>
    <skos:scopeNote>things - reflect - language.&#13;
Example: Greek alphabet reflects Greek (language); Vedas reflect Sanskrit</skos:scopeNote>
  </rdf:Description>
  <rdf:Description rdf:about="http://vocab.getty.edu/ontology#termKind">
    <skos:scopeNote>Term Kind</skos:scopeNote>
    <rdfs:domain rdf:resource="http://www.w3.org/2008/05/skos-xl#Label"/>
    <rdfs:label>termKind</rdfs:label>
    <rdfs:range rdf:resource="http://www.w3.org/2004/02/skos/core#Concept"/>
    <skos:prefLabel>termKind</skos:prefLabel>
    <rdf:type rdf:resource="http://www.w3.org/2002/07/owl#ObjectProperty"/>
    <rdfs:isDefinedBy rdf:resource="http://vocab.getty.edu/ontology"/>
    <dct:description>Term Kind</dct:description>
  </rdf:Description>
  <rdf:Description rdf:about="http://vocab.getty.edu/ontology#ulan1007_distinguished_from">
    <skos:example>The Noguchi Museum is distinguished form Isamu Noguchi Garden Museum Japan</skos:example>
    <rdfs:isDefinedBy rdf:resource="http://vocab.getty.edu/ulan/"/>
    <rdf:type rdf:resource="http://www.w3.org/2002/07/owl#SymmetricProperty"/>
    <skos:prefLabel>ulan1007_distinguished_from</skos:prefLabel>
    <dct:description>any - distinguished from - any.&#13;
Example: Laura Theresa Alma-Tadema is distinguished from Lawrence Alma-Tadema; The Noguchi Museum is distinguished form Isamu Noguchi Garden Museum Japan</dct:description>
    <skos:example>Laura Theresa Alma-Tadema is distinguished from Lawrence Alma-Tadema</skos:example>
    <dc:title>distinguished from - any</dc:title>
    <rdf:type rdf:resource="http://www.w3.org/2002/07/owl#ObjectProperty"/>
    <rdfs:domain rdf:resource="http://www.w3.org/2004/02/skos/core#Concept"/>
    <dc:identifier>1007</dc:identifier>
    <rdfs:isDefinedBy rdf:resource="http://vocab.getty.edu/ontology"/>
    <rdfs:range rdf:resource="http://www.w3.org/2004/02/skos/core#Concept"/>
    <rdfs:subPropertyOf rdf:resource="http://www.w3.org/2004/02/skos/core#related"/>
    <skos:scopeNote>any - distinguished from - any.&#13;
Example: Laura Theresa Alma-Tadema is distinguished from Lawrence Alma-Tadema; The Noguchi Museum is distinguished form Isamu Noguchi Garden Museum Japan</skos:scopeNote>
  </rdf:Description>
  <rdf:Description rdf:about="http://vocab.getty.edu/ontology#aat2895_example_of">
    <skos:scopeNote>brand name - [is] example of - activity/event/[process/function].&#13;
Example: Papersave Process (TM) is example of deacidification [process/function]</skos:scopeNote>
    <skos:example>Papersave Process (TM) is example of deacidification [process/function]</skos:example>
    <dct:description>brand name - [is] example of - activity/event/[process/function].&#13;
Example: Papersave Process (TM) is example of deacidification [process/function]</dct:description>
    <rdfs:subPropertyOf rdf:resource="http://www.w3.org/2004/02/skos/core#related"/>
    <skos:prefLabel>aat2895_example_of</skos:prefLabel>
    <rdf:type rdf:resource="http://www.w3.org/2002/07/owl#ObjectProperty"/>
    <dc:title>example of - activity/event</dc:title>
    <rdfs:isDefinedBy rdf:resource="http://vocab.getty.edu/ontology"/>
    <rdfs:range rdf:resource="http://www.w3.org/2004/02/skos/core#Concept"/>
    <rdfs:isDefinedBy rdf:resource="http://vocab.getty.edu/aat/"/>
    <rdfs:domain rdf:resource="http://www.w3.org/2004/02/skos/core#Concept"/>
    <dc:identifier>2895</dc:identifier>
  </rdf:Description>
  <rdf:Description rdf:about="http://vocab.getty.edu/ontology#agentTypeNonPreferred">
    <rdfs:domain rdf:resource="http://vocab.getty.edu/ontology#Subject"/>
    <rdfs:range rdf:resource="http://vocab.getty.edu/ontology#Subject"/>
    <rdfs:comment>A secondary type of a ULAN Person or Corporate body. Domain is ULAN concept, range is AAT concept</rdfs:comment>
    <skos:example>Non-preferred types of "Albrecht Duerer Workshop" (ULAN) include "printmakers" and painters" (AAT)</skos:example>
    <dct:description>A secondary type of a ULAN Person or Corporate body. Domain is ULAN concept, range is AAT concept.
Example: Non-preferred types of "Albrecht Duerer Workshop" (ULAN) include "printmakers" and painters" (AAT)</dct:description>
    <rdfs:isDefinedBy rdf:resource="http://vocab.getty.edu/ontology"/>
    <rdfs:label>agentTypeNonPreferred</rdfs:label>
    <rdf:type rdf:resource="http://www.w3.org/2002/07/owl#ObjectProperty"/>
    <rdfs:subPropertyOf rdf:resource="http://vocab.getty.edu/ontology#agentType"/>
    <skos:scopeNote>A secondary type of a ULAN Person or Corporate body. Domain is ULAN concept, range is AAT concept.
Example: Non-preferred types of "Albrecht Duerer Workshop" (ULAN) include "printmakers" and painters" (AAT)</skos:scopeNote>
    <skos:definition>A secondary type of a ULAN Person or Corporate body. Domain is ULAN concept, range is AAT concept</skos:definition>
    <skos:prefLabel>agentTypeNonPreferred</skos:prefLabel>
  </rdf:Description>
  <rdf:Description rdf:about="http://vocab.getty.edu/ontology#Infer_skosBroader_TypeRestr">
    <ptop:type1 rdf:resource="http://www.w3.org/2004/02/skos/core#Concept"/>
    <rdf:type rdf:resource="http://www.ontotext.com/proton/protontop#TypeRestr"/>
    <ptop:premise rdf:resource="http://vocab.getty.edu/ontology#broader"/>
    <ptop:type2 rdf:resource="http://www.w3.org/2004/02/skos/core#Concept"/>
    <ptop:conclusion rdf:resource="http://www.w3.org/2004/02/skos/core#broader"/>
  </rdf:Description>
  <rdf:Description rdf:about="http://vocab.getty.edu/ontology#agentType">
    <rdfs:domain rdf:resource="http://vocab.getty.edu/ontology#Subject"/>
    <rdfs:range rdf:resource="http://vocab.getty.edu/ontology#Subject"/>
    <skos:scopeNote>Type of a ULAN PersonConcept or GroupConcept. Domain is ULAN concept, range is AAT concept</skos:scopeNote>
    <skos:definition>Type of a ULAN PersonConcept or GroupConcept. Domain is ULAN concept, range is AAT concept</skos:definition>
    <rdfs:comment>Type of a ULAN PersonConcept or GroupConcept. Domain is ULAN concept, range is AAT concept</rdfs:comment>
    <rdf:type rdf:resource="http://www.w3.org/2002/07/owl#ObjectProperty"/>
    <rdfs:isDefinedBy rdf:resource="http://vocab.getty.edu/ontology"/>
    <skos:prefLabel>agentType</skos:prefLabel>
    <dct:description>Type of a ULAN PersonConcept or GroupConcept. Domain is ULAN concept, range is AAT concept</dct:description>
    <rdfs:label>agentType</rdfs:label>
  </rdf:Description>
  <rdf:Description rdf:about="http://vocab.getty.edu/ontology#Infer_isoBroaderGeneric">
    <ptop:premise rdf:resource="http://vocab.getty.edu/ontology#broaderGenericExtended"/>
    <ptop:conclusion rdf:resource="http://purl.org/iso25964/skos-thes#broaderGeneric"/>
    <rdf:type rdf:resource="http://www.ontotext.com/proton/protontop#PropRestr"/>
    <ptop:restriction rdf:resource="http://www.w3.org/2004/02/skos/core#broader"/>
  </rdf:Description>
  <rdf:Description rdf:about="http://vocab.getty.edu/ontology#termPOS">
    <rdfs:domain rdf:resource="http://www.w3.org/2008/05/skos-xl#Label"/>
    <rdf:type rdf:resource="http://www.w3.org/2002/07/owl#ObjectProperty"/>
    <rdfs:label>termPOS</rdfs:label>
    <dct:description>Part of Speech</dct:description>
    <rdfs:isDefinedBy rdf:resource="http://vocab.getty.edu/ontology"/>
    <skos:prefLabel>termPOS</skos:prefLabel>
    <rdfs:range rdf:resource="http://www.w3.org/2004/02/skos/core#Concept"/>
    <skos:scopeNote>Part of Speech</skos:scopeNote>
  </rdf:Description>
  <rdf:Description rdf:about="http://vocab.getty.edu/ontology#aat2604_possessed_by-existing_in">
    <dc:title>possessed by/existing in - things</dc:title>
    <rdfs:domain rdf:resource="http://www.w3.org/2004/02/skos/core#Concept"/>
    <rdfs:range rdf:resource="http://www.w3.org/2004/02/skos/core#Concept"/>
    <rdfs:isDefinedBy rdf:resource="http://vocab.getty.edu/aat/"/>
    <dct:description>attributes /associated concepts - [is] possessed by/existing in - things.&#13;
Example: boudoir (photograph size) is possessed by/existing in boudoir photographs; ruined [condition] is possessed by/existing in ruins</dct:description>
    <rdf:type rdf:resource="http://www.w3.org/2002/07/owl#ObjectProperty"/>
    <rdfs:isDefinedBy rdf:resource="http://vocab.getty.edu/ontology"/>
    <skos:example>ruined [condition] is possessed by/existing in ruins</skos:example>
    <rdfs:subPropertyOf rdf:resource="http://www.w3.org/2004/02/skos/core#related"/>
    <skos:example>boudoir (photograph size) is possessed by/existing in boudoir photographs</skos:example>
    <owl:inverseOf rdf:resource="http://vocab.getty.edu/ontology#aat2605_possess-exist_in"/>
    <skos:scopeNote>attributes /associated concepts - [is] possessed by/existing in - things.&#13;
Example: boudoir (photograph size) is possessed by/existing in boudoir photographs; ruined [condition] is possessed by/existing in ruins</skos:scopeNote>
    <dc:identifier>2604</dc:identifier>
    <skos:prefLabel>aat2604_possessed_by-existing_in</skos:prefLabel>
  </rdf:Description>
  <rdf:Description rdf:about="http://vocab.getty.edu/term/kind/CommonTerm">
    <skos:notation>C</skos:notation>
    <rdf:type rdf:resource="http://www.w3.org/2004/02/skos/core#Concept"/>
    <skos:scopeNote>Preferred common language term. Used for subjects that also include a Scientific term. Used in AAT only</skos:scopeNote>
    <skos:prefLabel>Common term</skos:prefLabel>
    <dct:description>Preferred common language term. Used for subjects that also include a Scientific term. Used in AAT only.
Example: "frankincense" (species) is common term for "Boswellia sacra" (species)</dct:description>
    <skos:example>"frankincense" (species) is common term for "Boswellia sacra" (species)</skos:example>
    <skos:inScheme rdf:resource="http://vocab.getty.edu/term/kind/"/>
  </rdf:Description>
  <rdf:Description rdf:about="http://vocab.getty.edu/term/POS/PastParticiple">
    <skos:scopeNote>Rarely used but if at all, is most likely to apply in Attributes and Properties</skos:scopeNote>
    <skos:notation>PP</skos:notation>
    <dct:description>Rarely used but if at all, is most likely to apply in Attributes and Properties.
Example: hand-painted</dct:description>
    <skos:inScheme rdf:resource="http://vocab.getty.edu/term/POS/"/>
    <skos:prefLabel>Past Participle</skos:prefLabel>
    <skos:example>hand-painted</skos:example>
    <rdf:type rdf:resource="http://www.w3.org/2004/02/skos/core#Concept"/>
  </rdf:Description>
  <rdf:Description rdf:about="http://vocab.getty.edu/ontology#ulan2779_owned_by">
    <rdfs:isDefinedBy rdf:resource="http://vocab.getty.edu/ulan/"/>
    <skos:example>Walter Scott Lenox was owned by Lenox China Co.</skos:example>
    <skos:prefLabel>ulan2779_owned_by</skos:prefLabel>
    <dct:description>person - owned by - firm.&#13;
Example: Walter Scott Lenox was owned by Lenox China Co.</dct:description>
    <rdfs:range rdf:resource="http://www.w3.org/2004/02/skos/core#Concept"/>
    <rdfs:domain rdf:resource="http://www.w3.org/2004/02/skos/core#Concept"/>
    <skos:scopeNote>person - owned by - firm.&#13;
Example: Walter Scott Lenox was owned by Lenox China Co.</skos:scopeNote>
    <rdfs:isDefinedBy rdf:resource="http://vocab.getty.edu/ontology"/>
    <dc:title>owned by - firm</dc:title>
    <dc:identifier>2779</dc:identifier>
    <rdfs:subPropertyOf rdf:resource="http://www.w3.org/2004/02/skos/core#related"/>
    <rdf:type rdf:resource="http://www.w3.org/2002/07/owl#ObjectProperty"/>
  </rdf:Description>
  <rdf:Description rdf:about="http://vocab.getty.edu/ontology#AdminPlaceConcept">
    <skos:scopeNote>Place defined by administrative boundaries and conditions, including inhabited places, nations, and empires. Used in TGN only.
Example: Burgundy region in France (TGN)</skos:scopeNote>
    <rdfs:isDefinedBy rdf:resource="http://vocab.getty.edu/ontology"/>
    <rdfs:comment>Place defined by administrative boundaries and conditions, including inhabited places, nations, and empires. Used in TGN only</rdfs:comment>
    <skos:example>Burgundy region in France (TGN)</skos:example>
    <skos:definition>Place defined by administrative boundaries and conditions, including inhabited places, nations, and empires. Used in TGN only</skos:definition>
    <rdfs:subClassOf rdf:resource="http://www.w3.org/2004/02/skos/core#Concept"/>
    <rdfs:label>AdminPlaceConcept</rdfs:label>
    <skos:prefLabel>AdminPlaceConcept</skos:prefLabel>
    <dct:description>Place defined by administrative boundaries and conditions, including inhabited places, nations, and empires. Used in TGN only.
Example: Burgundy region in France (TGN)</dct:description>
    <rdf:type rdf:resource="http://www.w3.org/2002/07/owl#Class"/>
    <rdfs:subClassOf rdf:resource="http://vocab.getty.edu/ontology#Subject"/>
    <skos:broader rdf:resource="http://www.w3.org/2004/02/skos/core#Concept"/>
  </rdf:Description>
  <rdf:Description rdf:about="http://vocab.getty.edu/ontology#aat2222_are_acted_upon">
    <rdfs:subPropertyOf rdf:resource="http://www.w3.org/2004/02/skos/core#related"/>
    <skos:example>Equus caballus(species) is acted upon by jockeys</skos:example>
    <dc:identifier>2222</dc:identifier>
    <rdfs:range rdf:resource="http://www.w3.org/2004/02/skos/core#Concept"/>
    <rdfs:isDefinedBy rdf:resource="http://vocab.getty.edu/aat/"/>
    <dct:description>genus/species - is acted upon [by] - [actors having] role.&#13;
Example: Equus caballus(species) is acted upon by jockeys; Acer saccharum(species) is acted upon by tappers</dct:description>
    <skos:scopeNote>genus/species - is acted upon [by] - [actors having] role.&#13;
Example: Equus caballus(species) is acted upon by jockeys; Acer saccharum(species) is acted upon by tappers</skos:scopeNote>
    <rdfs:isDefinedBy rdf:resource="http://vocab.getty.edu/ontology"/>
    <dc:title>are acted upon - role</dc:title>
    <skos:prefLabel>aat2222_are_acted_upon</skos:prefLabel>
    <rdf:type rdf:resource="http://www.w3.org/2002/07/owl#ObjectProperty"/>
    <skos:example>Acer saccharum(species) is acted upon by tappers</skos:example>
    <rdfs:domain rdf:resource="http://www.w3.org/2004/02/skos/core#Concept"/>
  </rdf:Description>
  <rdf:Description rdf:about="http://vocab.getty.edu/ontology#ulan2579_trustee_was">
    <rdf:type rdf:resource="http://www.w3.org/2002/07/owl#ObjectProperty"/>
    <skos:prefLabel>ulan2579_trustee_was</skos:prefLabel>
    <skos:scopeNote>institution - trustee was - person.&#13;
Example: National Galleries of Scotland trustee was George Douglas Haig</skos:scopeNote>
    <rdfs:domain rdf:resource="http://www.w3.org/2004/02/skos/core#Concept"/>
    <rdfs:range rdf:resource="http://www.w3.org/2004/02/skos/core#Concept"/>
    <skos:example>National Galleries of Scotland trustee was George Douglas Haig</skos:example>
    <dc:title>trustee was - person</dc:title>
    <rdfs:isDefinedBy rdf:resource="http://vocab.getty.edu/ulan/"/>
    <dct:description>institution - trustee was - person.&#13;
Example: National Galleries of Scotland trustee was George Douglas Haig</dct:description>
    <rdfs:subPropertyOf rdf:resource="http://www.w3.org/2004/02/skos/core#related"/>
    <rdfs:isDefinedBy rdf:resource="http://vocab.getty.edu/ontology"/>
    <dc:identifier>2579</dc:identifier>
  </rdf:Description>
  <rdf:Description rdf:about="http://vocab.getty.edu/ontology#broaderNonConcept">
    <rdf:type rdf:resource="http://www.w3.org/2002/07/owl#ObjectProperty"/>
    <rdfs:label>broaderNonConcept</rdfs:label>
    <dct:description>Chain of gvp:broader from Concept to GuideTerms, without intervening Concept</dct:description>
    <rdfs:range rdf:resource="http://vocab.getty.edu/ontology#GuideTerm"/>
    <rdfs:comment>Chain of gvp:broader from Concept to GuideTerms, without intervening Concept</rdfs:comment>
    <skos:prefLabel>broaderNonConcept</skos:prefLabel>
    <skos:scopeNote>Chain of gvp:broader from Concept to GuideTerms, without intervening Concept</skos:scopeNote>
    <skos:definition>Chain of gvp:broader from Concept to GuideTerms, without intervening Concept</skos:definition>
    <rdfs:domain rdf:resource="http://www.w3.org/2004/02/skos/core#Concept"/>
    <rdfs:isDefinedBy rdf:resource="http://vocab.getty.edu/ontology"/>
  </rdf:Description>
  <rdf:Description rdf:about="http://vocab.getty.edu/term/flag/LiteralTranslation">
    <dct:description>Literal translation of a name.  Defined for ULAN, but currently there are no examples of this</dct:description>
    <skos:notation>T</skos:notation>
    <skos:prefLabel>Literal Translation</skos:prefLabel>
    <skos:scopeNote>Literal translation of a name.  Defined for ULAN, but currently there are no examples of this</skos:scopeNote>
    <skos:inScheme rdf:resource="http://vocab.getty.edu/term/flag/"/>
    <rdf:type rdf:resource="http://www.w3.org/2004/02/skos/core#Concept"/>
  </rdf:Description>
  <rdf:Description rdf:about="http://vocab.getty.edu/term/kind/Code">
    <skos:inScheme rdf:resource="http://vocab.getty.edu/term/kind/"/>
    <skos:scopeNote>Code, similar to Abbreviation</skos:scopeNote>
    <skos:prefLabel>Code</skos:prefLabel>
    <skos:notation>79000</skos:notation>
    <rdf:type rdf:resource="http://www.w3.org/2004/02/skos/core#Concept"/>
    <dct:description>Code, similar to Abbreviation.
Example: "sq yds", "m2"</dct:description>
    <skos:example>"sq yds", "m2"</skos:example>
  </rdf:Description>
  <rdf:Description rdf:about="http://vocab.getty.edu/ontology#aat2806_provide_context">
    <skos:example>books provide context for chapters</skos:example>
    <dct:description>[larger] things - provide context [for] - [smaller] things.&#13;
Example: altarpieces provide context for predellas; books provide context for chapters</dct:description>
    <rdf:type rdf:resource="http://www.w3.org/2002/07/owl#ObjectProperty"/>
    <dc:identifier>2806</dc:identifier>
    <dc:title>provide context - things</dc:title>
    <rdfs:isDefinedBy rdf:resource="http://vocab.getty.edu/aat/"/>
    <rdfs:domain rdf:resource="http://www.w3.org/2004/02/skos/core#Concept"/>
    <skos:example>altarpieces provide context for predellas</skos:example>
    <rdfs:range rdf:resource="http://www.w3.org/2004/02/skos/core#Concept"/>
    <skos:scopeNote>[larger] things - provide context [for] - [smaller] things.&#13;
Example: altarpieces provide context for predellas; books provide context for chapters</skos:scopeNote>
    <rdfs:subPropertyOf rdf:resource="http://www.w3.org/2004/02/skos/core#related"/>
    <rdfs:isDefinedBy rdf:resource="http://vocab.getty.edu/ontology"/>
    <skos:prefLabel>aat2806_provide_context</skos:prefLabel>
  </rdf:Description>
  <rdf:Description rdf:about="http://vocab.getty.edu/ontology#aat2294_locus-setting_for">
    <rdfs:domain rdf:resource="http://www.w3.org/2004/02/skos/core#Concept"/>
    <rdf:type rdf:resource="http://www.w3.org/2002/07/owl#ObjectProperty"/>
    <dct:description>locus/setting - [is] locus setting for - locus/setting.&#13;
Example: nations are the locus/setting for national capitals; mountain ranges are the locus/setting for mountains</dct:description>
    <rdfs:isDefinedBy rdf:resource="http://vocab.getty.edu/aat/"/>
    <dc:identifier>2294</dc:identifier>
    <skos:prefLabel>aat2294_locus-setting_for</skos:prefLabel>
    <skos:scopeNote>locus/setting - [is] locus setting for - locus/setting.&#13;
Example: nations are the locus/setting for national capitals; mountain ranges are the locus/setting for mountains</skos:scopeNote>
    <skos:example>mountain ranges are the locus/setting for mountains</skos:example>
    <rdfs:range rdf:resource="http://www.w3.org/2004/02/skos/core#Concept"/>
    <dc:title>locus/setting for - locus/setting</dc:title>
    <owl:inverseOf rdf:resource="http://vocab.getty.edu/ontology#aat2295_located_in"/>
    <rdfs:subPropertyOf rdf:resource="http://www.w3.org/2004/02/skos/core#related"/>
    <rdfs:isDefinedBy rdf:resource="http://vocab.getty.edu/ontology"/>
    <skos:example>nations are the locus/setting for national capitals</skos:example>
  </rdf:Description>
  <rdf:Description rdf:about="http://vocab.getty.edu/ontology#aat2555_reflected_in">
    <dc:title>reflected in - activity/event</dc:title>
    <rdf:type rdf:resource="http://www.w3.org/2002/07/owl#ObjectProperty"/>
    <dct:description>style/period/culture /[religion/ideology] - [is] reflected in activity/event.&#13;
Example: Dhokra (culture) is reflected in dhokra (casting technique); Red-figure [style] is reflected in red-figure vase painting</dct:description>
    <dc:identifier>2555</dc:identifier>
    <skos:example>Dhokra (culture) is reflected in dhokra (casting technique)</skos:example>
    <rdfs:isDefinedBy rdf:resource="http://vocab.getty.edu/aat/"/>
    <rdfs:range rdf:resource="http://www.w3.org/2004/02/skos/core#Concept"/>
    <rdfs:domain rdf:resource="http://www.w3.org/2004/02/skos/core#Concept"/>
    <skos:scopeNote>style/period/culture /[religion/ideology] - [is] reflected in activity/event.&#13;
Example: Dhokra (culture) is reflected in dhokra (casting technique); Red-figure [style] is reflected in red-figure vase painting</skos:scopeNote>
    <skos:prefLabel>aat2555_reflected_in</skos:prefLabel>
    <rdfs:subPropertyOf rdf:resource="http://www.w3.org/2004/02/skos/core#related"/>
    <rdfs:isDefinedBy rdf:resource="http://vocab.getty.edu/ontology"/>
    <skos:example>Red-figure [style] is reflected in red-figure vase painting</skos:example>
  </rdf:Description>
  <rdf:Description rdf:about="http://vocab.getty.edu/ontology#aat2328_involved_with">
    <skos:prefLabel>aat2328_involved_with</skos:prefLabel>
    <skos:example>sitters are involved with portraits</skos:example>
    <rdfs:range rdf:resource="http://www.w3.org/2004/02/skos/core#Concept"/>
    <rdfs:domain rdf:resource="http://www.w3.org/2004/02/skos/core#Concept"/>
    <skos:scopeNote>[actors having] role - [are] involved in- things.&#13;
Example: sitters are involved with portraits; actors (performing artists) are involved with motion pictures (visual works)</skos:scopeNote>
    <dc:identifier>2328</dc:identifier>
    <rdf:type rdf:resource="http://www.w3.org/2002/07/owl#ObjectProperty"/>
    <rdfs:isDefinedBy rdf:resource="http://vocab.getty.edu/aat/"/>
    <rdfs:isDefinedBy rdf:resource="http://vocab.getty.edu/ontology"/>
    <skos:example>actors (performing artists) are involved with motion pictures (visual works)</skos:example>
    <dct:description>[actors having] role - [are] involved in- things.&#13;
Example: sitters are involved with portraits; actors (performing artists) are involved with motion pictures (visual works)</dct:description>
    <owl:inverseOf rdf:resource="http://vocab.getty.edu/ontology#aat2329_involves"/>
    <dc:title>involved with - things</dc:title>
    <rdfs:subPropertyOf rdf:resource="http://www.w3.org/2004/02/skos/core#related"/>
  </rdf:Description>
  <rdf:Description rdf:about="http://vocab.getty.edu/ontology#aat2505_locus-setting_for">
    <dc:title>locus/setting for - material</dc:title>
    <skos:scopeNote>locus/setting - [is] locus/setting for - material.&#13;
Example: volcanoes are locus/setting for  tephra; brickworks (factories) are locus/setting for brick (clay product)</skos:scopeNote>
    <rdfs:domain rdf:resource="http://www.w3.org/2004/02/skos/core#Concept"/>
    <rdfs:range rdf:resource="http://www.w3.org/2004/02/skos/core#Concept"/>
    <rdfs:subPropertyOf rdf:resource="http://www.w3.org/2004/02/skos/core#related"/>
    <dct:description>locus/setting - [is] locus/setting for - material.&#13;
Example: volcanoes are locus/setting for  tephra; brickworks (factories) are locus/setting for brick (clay product)</dct:description>
    <skos:prefLabel>aat2505_locus-setting_for</skos:prefLabel>
    <rdf:type rdf:resource="http://www.w3.org/2002/07/owl#ObjectProperty"/>
    <rdfs:isDefinedBy rdf:resource="http://vocab.getty.edu/ontology"/>
    <skos:example>brickworks (factories) are locus/setting for brick (clay product)</skos:example>
    <rdfs:isDefinedBy rdf:resource="http://vocab.getty.edu/aat/"/>
    <dc:identifier>2505</dc:identifier>
    <skos:example>volcanoes are locus/setting for  tephra</skos:example>
  </rdf:Description>
  <rdf:Description rdf:about="http://vocab.getty.edu/ontology#ulan1557_step-sibling_of">
    <skos:scopeNote>person - step-sibling of - person.&#13;
Example: W. L. Wyllie and Lionel Percy Smythe are step-siblings</skos:scopeNote>
    <rdfs:subPropertyOf rdf:resource="http://www.w3.org/2004/02/skos/core#related"/>
    <dc:identifier>1557</dc:identifier>
    <rdf:type rdf:resource="http://www.w3.org/2002/07/owl#SymmetricProperty"/>
    <skos:prefLabel>ulan1557_step-sibling_of</skos:prefLabel>
    <rdfs:range rdf:resource="http://www.w3.org/2004/02/skos/core#Concept"/>
    <dc:title>step-sibling of - person</dc:title>
    <dct:description>person - step-sibling of - person.&#13;
Example: W. L. Wyllie and Lionel Percy Smythe are step-siblings</dct:description>
    <skos:example>W. L. Wyllie and Lionel Percy Smythe are step-siblings</skos:example>
    <rdf:type rdf:resource="http://www.w3.org/2002/07/owl#ObjectProperty"/>
    <rdfs:isDefinedBy rdf:resource="http://vocab.getty.edu/ontology"/>
    <rdfs:isDefinedBy rdf:resource="http://vocab.getty.edu/ulan/"/>
    <rdfs:domain rdf:resource="http://www.w3.org/2004/02/skos/core#Concept"/>
  </rdf:Description>
  <rdf:Description rdf:about="http://vocab.getty.edu/ontology#broaderGenericExtended">
    <rdfs:isDefinedBy rdf:resource="http://vocab.getty.edu/ontology"/>
    <skos:prefLabel>broaderGenericExtended</skos:prefLabel>
    <rdfs:domain rdf:resource="http://vocab.getty.edu/ontology#Subject"/>
    <rdfs:range rdf:resource="http://vocab.getty.edu/ontology#Subject"/>
    <rdfs:label>broaderGenericExtended</rdfs:label>
    <skos:example>&lt;anvils and anvil accessories&gt; BTG &lt;forging and metal-shaping tools&gt; BTG &lt;forging and metal-shaping equipment&gt;,
so &lt;anvils and anvil accessories&gt; BTGE &lt;forging and metal-shaping equipment&gt;</skos:example>
    <rdfs:comment>Ancestors (Generic). Meaningful closure of gvp:broaderGeneric. Infers iso:broaderGeneric for pairs of directly related skos:Concepts</rdfs:comment>
    <skos:definition>Ancestors (Generic). Meaningful closure of gvp:broaderGeneric. Infers iso:broaderGeneric for pairs of directly related skos:Concepts</skos:definition>
    <skos:scopeNote>Ancestors (Generic). Meaningful closure of gvp:broaderGeneric. Infers iso:broaderGeneric for pairs of directly related skos:Concepts.
Example: &lt;anvils and anvil accessories&gt; BTG &lt;forging and metal-shaping tools&gt; BTG &lt;forging and metal-shaping equipment&gt;,
so &lt;anvils and anvil accessories&gt; BTGE &lt;forging and metal-shaping equipment&gt;</skos:scopeNote>
    <owl:propertyChainAxiom rdf:nodeID="Nc8f3b7a936da4ce0ad4f9bb8fc5ead4e"/>
    <rdf:type rdf:resource="http://www.w3.org/2002/07/owl#ObjectProperty"/>
    <dct:description>Ancestors (Generic). Meaningful closure of gvp:broaderGeneric. Infers iso:broaderGeneric for pairs of directly related skos:Concepts.
Example: &lt;anvils and anvil accessories&gt; BTG &lt;forging and metal-shaping tools&gt; BTG &lt;forging and metal-shaping equipment&gt;,
so &lt;anvils and anvil accessories&gt; BTGE &lt;forging and metal-shaping equipment&gt;</dct:description>
    <rdfs:subPropertyOf rdf:resource="http://vocab.getty.edu/ontology#broaderExtended"/>
  </rdf:Description>
  <rdf:Description rdf:about="http://vocab.getty.edu/term/type/Descriptor">
    <skos:inScheme rdf:resource="http://vocab.getty.edu/term/type/"/>
    <dct:description>Main term. Getty usually uses the plural.
Example: "manuscripts" (English)</dct:description>
    <skos:scopeNote>Main term. Getty usually uses the plural</skos:scopeNote>
    <skos:notation>D</skos:notation>
    <skos:example>"manuscripts" (English)</skos:example>
    <rdf:type rdf:resource="http://www.w3.org/2004/02/skos/core#Concept"/>
    <skos:prefLabel>Descriptor</skos:prefLabel>
  </rdf:Description>
  <rdf:Description rdf:about="http://vocab.getty.edu/ontology#ulan1102_student_of">
    <dc:title>student of - person</dc:title>
    <rdfs:domain rdf:resource="http://www.w3.org/2004/02/skos/core#Concept"/>
    <rdfs:range rdf:resource="http://www.w3.org/2004/02/skos/core#Concept"/>
    <dc:identifier>1102</dc:identifier>
    <rdf:type rdf:resource="http://www.w3.org/2002/07/owl#ObjectProperty"/>
    <skos:scopeNote>person - student of - person.&#13;
Example: Pierre Subleyras was the student of Rivalz, Antoine</skos:scopeNote>
    <rdfs:isDefinedBy rdf:resource="http://vocab.getty.edu/ontology"/>
    <rdfs:subPropertyOf rdf:resource="http://www.w3.org/2004/02/skos/core#related"/>
    <skos:prefLabel>ulan1102_student_of</skos:prefLabel>
    <rdfs:isDefinedBy rdf:resource="http://vocab.getty.edu/ulan/"/>
    <skos:example>Pierre Subleyras was the student of Rivalz, Antoine</skos:example>
    <dct:description>person - student of - person.&#13;
Example: Pierre Subleyras was the student of Rivalz, Antoine</dct:description>
  </rdf:Description>
  <rdf:Description rdf:about="http://vocab.getty.edu/ontology#Subject">
    <rdf:type rdf:resource="http://www.w3.org/2002/07/owl#Class"/>
    <dct:description>Node in a GVP vocabulary hierarchy. 
May be Facet, GuideTerm, Hierarchy, Concept, AdminPlaceConcept, PhysPlaceConcept, PhysAdminPlaceConcept, or ObsoleteSubject.
Implemented as skos:Concept or iso:ThesaurusArray and skos:Collection</dct:description>
    <rdfs:comment>Node in a GVP vocabulary hierarchy. 
May be Facet, GuideTerm, Hierarchy, Concept, AdminPlaceConcept, PhysPlaceConcept, PhysAdminPlaceConcept, or ObsoleteSubject.
Implemented as skos:Concept or iso:ThesaurusArray and skos:Collection</rdfs:comment>
    <rdfs:label>Subject</rdfs:label>
    <skos:scopeNote>Node in a GVP vocabulary hierarchy. 
May be Facet, GuideTerm, Hierarchy, Concept, AdminPlaceConcept, PhysPlaceConcept, PhysAdminPlaceConcept, or ObsoleteSubject.
Implemented as skos:Concept or iso:ThesaurusArray and skos:Collection</skos:scopeNote>
    <skos:prefLabel>Subject</skos:prefLabel>
    <skos:definition>Node in a GVP vocabulary hierarchy. 
May be Facet, GuideTerm, Hierarchy, Concept, AdminPlaceConcept, PhysPlaceConcept, PhysAdminPlaceConcept, or ObsoleteSubject.
Implemented as skos:Concept or iso:ThesaurusArray and skos:Collection</skos:definition>
    <rdfs:isDefinedBy rdf:resource="http://vocab.getty.edu/ontology"/>
  </rdf:Description>
  <rdf:Description rdf:about="http://vocab.getty.edu/term/POS/Noun">
    <rdf:type rdf:resource="http://www.w3.org/2004/02/skos/core#Concept"/>
    <skos:notation>N</skos:notation>
    <skos:inScheme rdf:resource="http://vocab.getty.edu/term/POS/"/>
    <skos:scopeNote>Term is a noun but we are uncertain if it is plural or singular</skos:scopeNote>
    <dct:description>Term is a noun but we are uncertain if it is plural or singular.
Example: Panthera leo</dct:description>
    <skos:prefLabel>Noun</skos:prefLabel>
    <skos:example>Panthera leo</skos:example>
  </rdf:Description>
  <rdf:Description rdf:about="http://vocab.getty.edu/ontology#contributorNonPreferred">
    <rdfs:isDefinedBy rdf:resource="http://vocab.getty.edu/ontology"/>
    <dct:description>Contributor for which the term is Non-preferred. Range is foaf:Agent.
Example: "Lycra" is non-preferred term for WHS</dct:description>
    <rdf:type rdf:resource="http://www.w3.org/2002/07/owl#ObjectProperty"/>
    <rdfs:domain rdf:resource="http://www.w3.org/2008/05/skos-xl#Label"/>
    <skos:prefLabel>contributorNonPreferred</skos:prefLabel>
    <skos:definition>Contributor for which the term is Non-preferred. Range is foaf:Agent</skos:definition>
    <rdfs:comment>Contributor for which the term is Non-preferred. Range is foaf:Agent</rdfs:comment>
    <skos:example>"Lycra" is non-preferred term for WHS</skos:example>
    <rdfs:subPropertyOf rdf:resource="http://purl.org/dc/terms/contributor"/>
    <skos:scopeNote>Contributor for which the term is Non-preferred. Range is foaf:Agent.
Example: "Lycra" is non-preferred term for WHS</skos:scopeNote>
    <rdfs:range rdf:resource="http://xmlns.com/foaf/0.1/Agent"/>
    <rdfs:label>contributorNonPreferred</rdfs:label>
  </rdf:Description>
  <rdf:Description rdf:about="http://vocab.getty.edu/ontology#PersonConcept">
    <skos:prefLabel>PersonConcept</skos:prefLabel>
    <skos:definition>A single individual. Usually people engaged in the design or creation of art or architecture ("Artists"); but may also include donors, patrons, rulers, sitters, art historians, etc ("Non-Artists")</skos:definition>
    <rdfs:comment>A single individual. Usually people engaged in the design or creation of art or architecture ("Artists"); but may also include donors, patrons, rulers, sitters, art historians, etc ("Non-Artists")</rdfs:comment>
    <dct:description>A single individual. Usually people engaged in the design or creation of art or architecture ("Artists"); but may also include donors, patrons, rulers, sitters, art historians, etc ("Non-Artists").
Example: 500115493 Duerer, Albrecht (ULAN)</dct:description>
    <rdf:type rdf:resource="http://www.w3.org/2002/07/owl#Class"/>
    <rdfs:isDefinedBy rdf:resource="http://vocab.getty.edu/ontology"/>
    <rdfs:subClassOf rdf:resource="http://vocab.getty.edu/ontology#Subject"/>
    <rdfs:label>PersonConcept</rdfs:label>
    <rdfs:subClassOf rdf:resource="http://www.w3.org/2004/02/skos/core#Concept"/>
    <skos:broader rdf:resource="http://vocab.getty.edu/ontology#Subject"/>
    <skos:example>500115493 Duerer, Albrecht (ULAN)</skos:example>
    <skos:scopeNote>A single individual. Usually people engaged in the design or creation of art or architecture ("Artists"); but may also include donors, patrons, rulers, sitters, art historians, etc ("Non-Artists").
Example: 500115493 Duerer, Albrecht (ULAN)</skos:scopeNote>
  </rdf:Description>
  <rdf:Description rdf:about="http://vocab.getty.edu/ontology#aat2419_used_for">
    <rdf:type rdf:resource="http://www.w3.org/2002/07/owl#ObjectProperty"/>
    <rdfs:isDefinedBy rdf:resource="http://vocab.getty.edu/aat/"/>
    <rdfs:range rdf:resource="http://www.w3.org/2004/02/skos/core#Concept"/>
    <rdfs:domain rdf:resource="http://www.w3.org/2004/02/skos/core#Concept"/>
    <dct:description>things/[equipment] - [are] used for - field [of study]/discipline.&#13;
Example: astronomical instruments are used for astronomy; divination objects are used for divination [discipline]</dct:description>
    <dc:identifier>2419</dc:identifier>
    <skos:scopeNote>things/[equipment] - [are] used for - field [of study]/discipline.&#13;
Example: astronomical instruments are used for astronomy; divination objects are used for divination [discipline]</skos:scopeNote>
    <skos:example>astronomical instruments are used for astronomy</skos:example>
    <rdfs:subPropertyOf rdf:resource="http://www.w3.org/2004/02/skos/core#related"/>
    <rdfs:isDefinedBy rdf:resource="http://vocab.getty.edu/ontology"/>
    <dc:title>used for - field/discipline</dc:title>
    <skos:prefLabel>aat2419_used_for</skos:prefLabel>
    <skos:example>divination objects are used for divination [discipline]</skos:example>
  </rdf:Description>
  <rdf:Description rdf:about="http://vocab.getty.edu/ontology#aat2834_decendant_of">
    <skos:example>donkeys are the descendents of Equus asinus</skos:example>
    <skos:scopeNote>genus/species - is decendant of -  genus/species.&#13;
Example: Canis familiaris is the descendant of Canis lupus; donkeys are the descendents of Equus asinus</skos:scopeNote>
    <dct:description>genus/species - is decendant of -  genus/species.&#13;
Example: Canis familiaris is the descendant of Canis lupus; donkeys are the descendents of Equus asinus</dct:description>
    <rdfs:range rdf:resource="http://www.w3.org/2004/02/skos/core#Concept"/>
    <dc:identifier>2834</dc:identifier>
    <rdfs:domain rdf:resource="http://www.w3.org/2004/02/skos/core#Concept"/>
    <rdfs:subPropertyOf rdf:resource="http://www.w3.org/2004/02/skos/core#related"/>
    <skos:example>Canis familiaris is the descendant of Canis lupus</skos:example>
    <dc:title>decendant of - genus/species</dc:title>
    <rdf:type rdf:resource="http://www.w3.org/2002/07/owl#ObjectProperty"/>
    <rdfs:isDefinedBy rdf:resource="http://vocab.getty.edu/ontology"/>
    <rdfs:isDefinedBy rdf:resource="http://vocab.getty.edu/aat/"/>
    <skos:prefLabel>aat2834_decendant_of</skos:prefLabel>
  </rdf:Description>
  <rdf:Description rdf:about="http://vocab.getty.edu/ontology#tgn3001_distinguished_from">
    <dc:identifier>3001</dc:identifier>
    <dc:title>distinguished from - any</dc:title>
    <skos:scopeNote>any - distinguished from - any.&#13;
Example: The Ancient Mesopotamian Kingdom 'Assyria' is distinguished from the Roman Province of the same name</skos:scopeNote>
    <skos:prefLabel>tgn3001_distinguished_from</skos:prefLabel>
    <rdf:type rdf:resource="http://www.w3.org/2002/07/owl#SymmetricProperty"/>
    <rdfs:domain rdf:resource="http://www.w3.org/2004/02/skos/core#Concept"/>
    <rdfs:range rdf:resource="http://www.w3.org/2004/02/skos/core#Concept"/>
    <rdfs:subPropertyOf rdf:resource="http://www.w3.org/2004/02/skos/core#related"/>
    <skos:example>The Ancient Mesopotamian Kingdom 'Assyria' is distinguished from the Roman Province of the same name</skos:example>
    <rdf:type rdf:resource="http://www.w3.org/2002/07/owl#ObjectProperty"/>
    <rdfs:isDefinedBy rdf:resource="http://vocab.getty.edu/ontology"/>
    <dct:description>any - distinguished from - any.&#13;
Example: The Ancient Mesopotamian Kingdom 'Assyria' is distinguished from the Roman Province of the same name</dct:description>
    <rdfs:isDefinedBy rdf:resource="http://vocab.getty.edu/tgn/"/>
  </rdf:Description>
  <rdf:Description rdf:about="http://vocab.getty.edu/ontology#ulan2572_founder_of">
    <rdf:type rdf:resource="http://www.w3.org/2002/07/owl#ObjectProperty"/>
    <rdfs:isDefinedBy rdf:resource="http://vocab.getty.edu/ontology"/>
    <dc:title>founder of - institution</dc:title>
    <rdfs:domain rdf:resource="http://www.w3.org/2004/02/skos/core#Concept"/>
    <skos:example>Louis Comfort Tiffany was the founder of Tiffany Glass &amp; Decorating Company</skos:example>
    <rdfs:range rdf:resource="http://www.w3.org/2004/02/skos/core#Concept"/>
    <skos:prefLabel>ulan2572_founder_of</skos:prefLabel>
    <dct:description>person - founder of - institution.&#13;
Example: Louis Comfort Tiffany was the founder of Tiffany Glass &amp; Decorating Company</dct:description>
    <rdfs:isDefinedBy rdf:resource="http://vocab.getty.edu/ulan/"/>
    <rdfs:subPropertyOf rdf:resource="http://www.w3.org/2004/02/skos/core#related"/>
    <owl:inverseOf rdf:resource="http://vocab.getty.edu/ontology#ulan2573_founded_by"/>
    <skos:scopeNote>person - founder of - institution.&#13;
Example: Louis Comfort Tiffany was the founder of Tiffany Glass &amp; Decorating Company</skos:scopeNote>
    <dc:identifier>2572</dc:identifier>
  </rdf:Description>
  <rdf:Description rdf:about="http://vocab.getty.edu/ontology#aat2557_reflects">
    <rdf:type rdf:resource="http://www.w3.org/2002/07/owl#ObjectProperty"/>
    <skos:example>classics (discipline) reflects Ancient Greek [culture]</skos:example>
    <skos:scopeNote>field/discipline - reflects - style/period/culture /[religion/ideology].&#13;
Example: bugatu [dance discipline] reflects Buddhism; church history reflects Christianity; classics (discipline) reflects Ancient Greek [culture]</skos:scopeNote>
    <rdfs:isDefinedBy rdf:resource="http://vocab.getty.edu/aat/"/>
    <skos:prefLabel>aat2557_reflects</skos:prefLabel>
    <dc:identifier>2557</dc:identifier>
    <rdfs:range rdf:resource="http://www.w3.org/2004/02/skos/core#Concept"/>
    <skos:example>church history reflects Christianity</skos:example>
    <dct:description>field/discipline - reflects - style/period/culture /[religion/ideology].&#13;
Example: bugatu [dance discipline] reflects Buddhism; church history reflects Christianity; classics (discipline) reflects Ancient Greek [culture]</dct:description>
    <dc:title>reflects - style/period/culture</dc:title>
    <owl:inverseOf rdf:resource="http://vocab.getty.edu/ontology#aat2558_reflected_in"/>
    <skos:example>bugatu [dance discipline] reflects Buddhism</skos:example>
    <rdfs:isDefinedBy rdf:resource="http://vocab.getty.edu/ontology"/>
    <rdfs:subPropertyOf rdf:resource="http://www.w3.org/2004/02/skos/core#related"/>
    <rdfs:domain rdf:resource="http://www.w3.org/2004/02/skos/core#Concept"/>
  </rdf:Description>
  <rdf:Description rdf:about="http://vocab.getty.edu/historic/currentAndHistoric">
    <skos:inScheme rdf:resource="http://vocab.getty.edu/historic/"/>
    <skos:scopeNote>Valid/used both in the past and currently</skos:scopeNote>
    <dct:description>Valid/used both in the past and currently.
Example: Saint Petersburg (TGN)</dct:description>
    <skos:example>Saint Petersburg (TGN)</skos:example>
    <skos:notation>B</skos:notation>
    <skos:prefLabel>Both Current and Historic</skos:prefLabel>
    <rdf:type rdf:resource="http://www.w3.org/2004/02/skos/core#Concept"/>
  </rdf:Description>
  <rdf:Description rdf:about="http://vocab.getty.edu/ontology#tgn3612_administrative_entity_for">
    <skos:scopeNote>place - administrative entity for - place.&#13;
Example: Ortonovo (Massa-Carra province, Tuscany, Italy) is the administrative entity for Luni (La Spezia province, Liguria, Italy)</skos:scopeNote>
    <rdfs:subPropertyOf rdf:resource="http://www.w3.org/2004/02/skos/core#related"/>
    <skos:example>Ortonovo (Massa-Carra province, Tuscany, Italy) is the administrative entity for Luni (La Spezia province, Liguria, Italy)</skos:example>
    <dc:title>administrative entity for - place</dc:title>
    <dct:description>place - administrative entity for - place.&#13;
Example: Ortonovo (Massa-Carra province, Tuscany, Italy) is the administrative entity for Luni (La Spezia province, Liguria, Italy)</dct:description>
    <rdfs:isDefinedBy rdf:resource="http://vocab.getty.edu/tgn/"/>
    <rdf:type rdf:resource="http://www.w3.org/2002/07/owl#ObjectProperty"/>
    <skos:prefLabel>tgn3612_administrative_entity_for</skos:prefLabel>
    <rdfs:isDefinedBy rdf:resource="http://vocab.getty.edu/ontology"/>
    <rdfs:domain rdf:resource="http://www.w3.org/2004/02/skos/core#Concept"/>
    <rdfs:range rdf:resource="http://www.w3.org/2004/02/skos/core#Concept"/>
    <dc:identifier>3612</dc:identifier>
  </rdf:Description>
  <rdf:Description rdf:about="http://vocab.getty.edu/ontology#ulan1218_employee_was">
    <rdf:type rdf:resource="http://www.w3.org/2002/07/owl#ObjectProperty"/>
    <skos:scopeNote>person - employee was - person/firm.&#13;
Example: Jean Tijou was an employee of Christopher Wren</skos:scopeNote>
    <rdfs:isDefinedBy rdf:resource="http://vocab.getty.edu/ontology"/>
    <rdfs:isDefinedBy rdf:resource="http://vocab.getty.edu/ulan/"/>
    <rdfs:range rdf:resource="http://www.w3.org/2004/02/skos/core#Concept"/>
    <rdfs:domain rdf:resource="http://www.w3.org/2004/02/skos/core#Concept"/>
    <dc:identifier>1218</dc:identifier>
    <rdfs:subPropertyOf rdf:resource="http://www.w3.org/2004/02/skos/core#related"/>
    <skos:example>Jean Tijou was an employee of Christopher Wren</skos:example>
    <dct:description>person - employee was - person/firm.&#13;
Example: Jean Tijou was an employee of Christopher Wren</dct:description>
    <skos:prefLabel>ulan1218_employee_was</skos:prefLabel>
    <dc:title>employee was - person/firm</dc:title>
  </rdf:Description>
  <rdf:Description rdf:nodeID="N35cd4461e8ba4403b72ec8a74ddcd3cd">
    <rdf:rest rdf:resource="http://www.w3.org/1999/02/22-rdf-syntax-ns#nil"/>
    <rdf:first rdf:resource="http://vocab.getty.edu/ontology#broaderGeneric"/>
  </rdf:Description>
  <rdf:Description rdf:about="http://vocab.getty.edu/aat/300189557">
    <skos:exactMatch rdf:resource="http://www.wikidata.org/entity/Q6581072"/>
    <skos:exactMatch rdf:resource="http://rdaregistry.info/termList/gender/1001"/>
  </rdf:Description>
  <rdf:Description rdf:about="http://vocab.getty.edu/ontology#Biography">
    <skos:definition>Biography of a ULAN agent (schema:Person|Organization). Depending on the agent, has these fields:
- schema:description: one-line-biography
- gvp:estStart
- schema:birthPlace | foundationLocation, pointing to TGN
- gvp:estEnd
- schema:deathPlace | dissolutionLocation, pointing to TGN
- schema:gender, pointing to AAT (male, female, other)
- dct:contributor
The fields of the preferred biogrpahy are also available in the agent.</skos:definition>
    <rdfs:isDefinedBy rdf:resource="http://vocab.getty.edu/ontology"/>
    <rdfs:comment>Biography of a ULAN agent (schema:Person|Organization). Depending on the agent, has these fields:
- schema:description: one-line-biography
- gvp:estStart
- schema:birthPlace | foundationLocation, pointing to TGN
- gvp:estEnd
- schema:deathPlace | dissolutionLocation, pointing to TGN
- schema:gender, pointing to AAT (male, female, other)
- dct:contributor
The fields of the preferred biogrpahy are also available in the agent.</rdfs:comment>
    <rdf:type rdf:resource="http://www.w3.org/2002/07/owl#Class"/>
  </rdf:Description>
  <rdf:Description rdf:about="http://www.w3.org/2004/02/skos/core#prefLabel">
    <owl:propertyChainAxiom rdf:nodeID="N42b7ac9239fa49009ec882f6ded18b8e"/>
  </rdf:Description>
  <rdf:Description rdf:nodeID="N1a416c3537d746a48699cfdbe39976a5">
    <rdf:rest rdf:nodeID="Nb50df4c21fce4564aeac401e52e57f93"/>
    <rdf:first rdf:resource="http://www.w3.org/2008/05/skos-xl#hiddenLabel"/>
  </rdf:Description>
  <rdf:Description rdf:about="http://vocab.getty.edu/ontology#biographyPreferred">
    <rdfs:label>biographyPreferred</rdfs:label>
    <dct:description>Preferred biography of an ULAN agent. Domain is schema:Person/Organization, range is gvp:Biography. The biography fields are also directly available in the Person/Organization</dct:description>
    <rdfs:range rdf:resource="http://vocab.getty.edu/ontology#Biography"/>
    <rdfs:isDefinedBy rdf:resource="http://vocab.getty.edu/ontology"/>
    <rdfs:subPropertyOf rdf:resource="http://vocab.getty.edu/ontology#biography"/>
    <skos:prefLabel>biographyPreferred</skos:prefLabel>
    <rdf:type rdf:resource="http://www.w3.org/2002/07/owl#ObjectProperty"/>
    <skos:scopeNote>Preferred biography of an ULAN agent. Domain is schema:Person/Organization, range is gvp:Biography. The biography fields are also directly available in the Person/Organization</skos:scopeNote>
    <rdfs:comment>Preferred biography of an ULAN agent. Domain is schema:Person/Organization, range is gvp:Biography. The biography fields are also directly available in the Person/Organization</rdfs:comment>
    <skos:definition>Preferred biography of an ULAN agent. Domain is schema:Person/Organization, range is gvp:Biography. The biography fields are also directly available in the Person/Organization</skos:definition>
  </rdf:Description>
  <rdf:Description rdf:about="http://vocab.getty.edu/ontology#ulan1332_worker_was">
    <dc:identifier>1332</dc:identifier>
    <rdfs:domain rdf:resource="http://www.w3.org/2004/02/skos/core#Concept"/>
    <rdfs:range rdf:resource="http://www.w3.org/2004/02/skos/core#Concept"/>
    <rdfs:subPropertyOf rdf:resource="http://www.w3.org/2004/02/skos/core#related"/>
    <rdfs:isDefinedBy rdf:resource="http://vocab.getty.edu/ontology"/>
    <rdf:type rdf:resource="http://www.w3.org/2002/07/owl#ObjectProperty"/>
    <dc:title>worker was - any</dc:title>
    <skos:scopeNote>person - worker was - any.&#13;
Example: Workers for the Carracci family included Scarsellino and Domenichino</skos:scopeNote>
    <skos:example>Workers for the Carracci family included Scarsellino and Domenichino</skos:example>
    <skos:prefLabel>ulan1332_worker_was</skos:prefLabel>
    <rdfs:isDefinedBy rdf:resource="http://vocab.getty.edu/ulan/"/>
    <dct:description>person - worker was - any.&#13;
Example: Workers for the Carracci family included Scarsellino and Domenichino</dct:description>
  </rdf:Description>
  <rdf:Description rdf:about="http://vocab.getty.edu/ontology#ScopeNote">
    <rdfs:isDefinedBy rdf:resource="http://vocab.getty.edu/ontology"/>
    <dct:description>Defines a GVP subject or provides usage information. Has fields:
- dc:identifier: numeric ID, also used in the URL.
- rdf:value: the note itself (as per SKOS Primer: 4.2 Advanced Documentation Features) with language tag
- dct:language: matches the language tag
- gvp:displayOrder, order of this note amongst others
- gvp:historicFlag, vp:estStart, gvp:estEnd, rdfs:comment: Historic Information about applicability
- dct:source or subproperties thereof 
- dct:contributor or subproperties thereof</dct:description>
    <skos:definition>Defines a GVP subject or provides usage information. Has fields:
- dc:identifier: numeric ID, also used in the URL.
- rdf:value: the note itself (as per SKOS Primer: 4.2 Advanced Documentation Features) with language tag
- dct:language: matches the language tag
- gvp:displayOrder, order of this note amongst others
- gvp:historicFlag, gvp:estStart, gvp:estEnd, rdfs:comment: Historic Information about applicability
- dct:source or subproperties thereof 
- dct:contributor or subproperties thereof</skos:definition>
    <rdf:type rdf:resource="http://www.w3.org/2002/07/owl#Class"/>
    <skos:scopeNote>Defines a GVP subject or provides usage information. Has fields:
- dc:identifier: numeric ID, also used in the URL.
- rdf:value: the note itself (as per SKOS Primer: 4.2 Advanced Documentation Features) with language tag
- dct:language: matches the language tag
- gvp:displayOrder, order of this note amongst others
- gvp:historicFlag, vp:estStart, gvp:estEnd, rdfs:comment: Historic Information about applicability
- dct:source or subproperties thereof 
- dct:contributor or subproperties thereof</skos:scopeNote>
    <rdfs:comment>Defines a GVP subject or provides usage information. Has fields:
- dc:identifier: numeric ID, also used in the URL.
- rdf:value: the note itself (as per SKOS Primer: 4.2 Advanced Documentation Features) with language tag
- dct:language: matches the language tag
- gvp:displayOrder, order of this note amongst others
- gvp:historicFlag, gvp:estStart, gvp:estEnd, rdfs:comment: Historic Information about applicability
- dct:source or subproperties thereof 
- dct:contributor or subproperties thereof</rdfs:comment>
  </rdf:Description>
  <rdf:Description rdf:about="http://vocab.getty.edu/term/type/UsedForTerm">
    <skos:inScheme rdf:resource="http://vocab.getty.edu/term/type/"/>
    <skos:notation>UF</skos:notation>
    <rdf:type rdf:resource="http://www.w3.org/2004/02/skos/core#Concept"/>
    <skos:scopeNote>A synonym</skos:scopeNote>
    <skos:prefLabel>Used for Term</skos:prefLabel>
    <dct:description>A synonym.
Example: "handschriften" (Dutch) instead of "manuscripten"</dct:description>
    <skos:example>"handschriften" (Dutch) instead of "manuscripten"</skos:example>
  </rdf:Description>
  <rdf:Description rdf:about="http://purl.org/dc/terms/isReplacedBy">
    <owl:inverseOf rdf:resource="http://purl.org/dc/terms/replaces"/>
  </rdf:Description>
  <rdf:Description rdf:about="http://vocab.getty.edu/ontology#broaderPreferredExtended">
    <skos:example>Mt Athos has preferred ancestor places (BTPE) World, Europe, Greece, Macedonia, Pangaíon Óros regional division;
and prefererd place type (BTIE) inhabited place</skos:example>
    <skos:prefLabel>broaderPreferredExtended</skos:prefLabel>
    <dct:description>Preferred Ancestors. Meaningful closure of gvp:broaderPreferred. Needed to display the hierarchy.
Example: Mt Athos has preferred ancestor places (BTPE) World, Europe, Greece, Macedonia, Pangaíon Óros regional division;
and prefererd place type (BTIE) inhabited place</dct:description>
    <skos:definition>Preferred Ancestors. Meaningful closure of gvp:broaderPreferred. Needed to display the hierarchy</skos:definition>
    <rdfs:label>broaderPreferredExtended</rdfs:label>
    <rdf:type rdf:resource="http://www.w3.org/2002/07/owl#ObjectProperty"/>
    <rdfs:isDefinedBy rdf:resource="http://vocab.getty.edu/ontology"/>
    <rdfs:comment>Preferred Ancestors. Meaningful closure of gvp:broaderPreferred. Needed to display the hierarchy</rdfs:comment>
    <rdfs:range rdf:resource="http://vocab.getty.edu/ontology#Subject"/>
    <skos:scopeNote>Preferred Ancestors. Meaningful closure of gvp:broaderPreferred. Needed to display the hierarchy.
Example: Mt Athos has preferred ancestor places (BTPE) World, Europe, Greece, Macedonia, Pangaíon Óros regional division;
and prefererd place type (BTIE) inhabited place</skos:scopeNote>
    <rdfs:domain rdf:resource="http://vocab.getty.edu/ontology#Subject"/>
  </rdf:Description>
  <rdf:Description rdf:about="http://vocab.getty.edu/term/POS/BothSingularAndPlural">
    <skos:inScheme rdf:resource="http://vocab.getty.edu/term/POS/"/>
    <skos:scopeNote>A term that is used for both the singular and plural in the same language</skos:scopeNote>
    <skos:example>"chassis" is both singular and plural in French</skos:example>
    <skos:prefLabel>Both Singular and Plural</skos:prefLabel>
    <rdf:type rdf:resource="http://www.w3.org/2004/02/skos/core#Concept"/>
    <skos:notation>B</skos:notation>
    <dct:description>A term that is used for both the singular and plural in the same language.
Example: "chassis" is both singular and plural in French</dct:description>
  </rdf:Description>
  <rdf:Description rdf:nodeID="N4d85f5c68de741c3b712aa69558e7a7b">
    <rdf:rest rdf:resource="http://www.w3.org/1999/02/22-rdf-syntax-ns#nil"/>
    <rdf:first rdf:resource="http://vocab.getty.edu/ontology#broaderPartitiveExtended"/>
  </rdf:Description>
  <rdf:Description rdf:about="http://vocab.getty.edu/term/display/">
    <rdfs:label>Term Display concept scheme</rdfs:label>
    <dct:description>Term Display concept scheme</dct:description>
    <skos:prefLabel>Term Display concept scheme</skos:prefLabel>
    <skos:scopeNote>Term Display concept scheme</skos:scopeNote>
    <rdfs:isDefinedBy rdf:resource="http://vocab.getty.edu/ontology"/>
    <rdf:type rdf:resource="http://www.w3.org/2004/02/skos/core#ConceptScheme"/>
  </rdf:Description>
  <rdf:Description rdf:about="http://vocab.getty.edu/ontology#aat2504_used-located_in">
    <rdfs:domain rdf:resource="http://www.w3.org/2004/02/skos/core#Concept"/>
    <owl:inverseOf rdf:resource="http://vocab.getty.edu/ontology#aat2505_locus-setting_for"/>
    <skos:example>tephra is used/located in [at] volcanoes</skos:example>
    <rdfs:isDefinedBy rdf:resource="http://vocab.getty.edu/ontology"/>
    <rdfs:subPropertyOf rdf:resource="http://www.w3.org/2004/02/skos/core#related"/>
    <skos:scopeNote>material - [is] used/located in - locus/setting.&#13;
Example: tephra is used/located in [at] volcanoes; brick (clay product) is used/located in brickworks (factories)</skos:scopeNote>
    <rdf:type rdf:resource="http://www.w3.org/2002/07/owl#ObjectProperty"/>
    <dc:title>used/located in - locus/setting</dc:title>
    <skos:prefLabel>aat2504_used-located_in</skos:prefLabel>
    <skos:example>brick (clay product) is used/located in brickworks (factories)</skos:example>
    <rdfs:isDefinedBy rdf:resource="http://vocab.getty.edu/aat/"/>
    <rdfs:range rdf:resource="http://www.w3.org/2004/02/skos/core#Concept"/>
    <dc:identifier>2504</dc:identifier>
    <dct:description>material - [is] used/located in - locus/setting.&#13;
Example: tephra is used/located in [at] volcanoes; brick (clay product) is used/located in brickworks (factories)</dct:description>
  </rdf:Description>
  <rdf:Description rdf:nodeID="N9c386dc021084c29bfcaa74d6d7c1db7">
    <rdf:first rdf:resource="http://vocab.getty.edu/ontology#broaderGeneric"/>
    <rdf:rest rdf:nodeID="N4d85f5c68de741c3b712aa69558e7a7b"/>
  </rdf:Description>
  <rdf:Description rdf:about="http://vocab.getty.edu/ontology#termType">
    <rdfs:isDefinedBy rdf:resource="http://vocab.getty.edu/ontology"/>
    <rdfs:label>termType</rdfs:label>
    <dct:description>Term Type</dct:description>
    <rdf:type rdf:resource="http://www.w3.org/2002/07/owl#ObjectProperty"/>
    <rdfs:domain rdf:resource="http://www.w3.org/2008/05/skos-xl#Label"/>
    <rdfs:range rdf:resource="http://www.w3.org/2004/02/skos/core#Concept"/>
    <skos:prefLabel>termType</skos:prefLabel>
    <skos:scopeNote>Term Type</skos:scopeNote>
  </rdf:Description>
  <rdf:Description rdf:about="http://vocab.getty.edu/ontology#nationalityNonPreferred">
    <rdfs:subPropertyOf rdf:resource="http://schema.org/nationality"/>
    <rdfs:isDefinedBy rdf:resource="http://vocab.getty.edu/ontology"/>
    <rdfs:label>nationalityNonPreferred</rdfs:label>
    <dct:description>Non-preferred nationality/culture/race/ethnicity/religion/sexual orientation of an ULAN agent. Domain is schema:Person/Organization, range is AAT concept</dct:description>
    <skos:prefLabel>nationalityNonPreferred</skos:prefLabel>
    <rdf:type rdf:resource="http://www.w3.org/2002/07/owl#ObjectProperty"/>
    <skos:definition>Non-preferred nationality/culture/race/ethnicity/religion/sexual orientation of an ULAN agent. Domain is schema:Person/Organization, range is AAT concept</skos:definition>
    <rdfs:comment>Non-preferred nationality/culture/race/ethnicity/religion/sexual orientation of an ULAN agent. Domain is schema:Person/Organization, range is AAT concept</rdfs:comment>
    <skos:scopeNote>Non-preferred nationality/culture/race/ethnicity/religion/sexual orientation of an ULAN agent. Domain is schema:Person/Organization, range is AAT concept</skos:scopeNote>
    <rdfs:range rdf:resource="http://vocab.getty.edu/ontology#Subject"/>
  </rdf:Description>
  <rdf:Description rdf:about="http://vocab.getty.edu/term/type/AlternateDescriptor">
    <skos:prefLabel>Alternate Descriptor</skos:prefLabel>
    <rdf:type rdf:resource="http://www.w3.org/2004/02/skos/core#Concept"/>
    <skos:inScheme rdf:resource="http://vocab.getty.edu/term/type/"/>
    <dct:description>A lexical variant, eg singular.
Example: "manuscript" (English) instead of "manuscripts"</dct:description>
    <skos:example>"manuscript" (English) instead of "manuscripts"</skos:example>
    <skos:scopeNote>A lexical variant, eg singular</skos:scopeNote>
    <skos:notation>AD</skos:notation>
  </rdf:Description>
  <rdf:Description rdf:nodeID="Nd22a60620bea4ea7ad721eadcab0dd92">
    <rdf:rest rdf:resource="http://www.w3.org/1999/02/22-rdf-syntax-ns#nil"/>
    <rdf:first rdf:resource="http://www.w3.org/2008/05/skos-xl#literalForm"/>
  </rdf:Description>
  <rdf:Description rdf:nodeID="Nb50df4c21fce4564aeac401e52e57f93">
    <rdf:rest rdf:resource="http://www.w3.org/1999/02/22-rdf-syntax-ns#nil"/>
    <rdf:first rdf:resource="http://www.w3.org/2008/05/skos-xl#literalForm"/>
  </rdf:Description>
  <rdf:Description rdf:nodeID="Nc8f3b7a936da4ce0ad4f9bb8fc5ead4e">
    <rdf:first rdf:resource="http://vocab.getty.edu/ontology#broaderGenericExtended"/>
    <rdf:rest rdf:nodeID="N35cd4461e8ba4403b72ec8a74ddcd3cd"/>
  </rdf:Description>
  <rdf:Description rdf:about="http://vocab.getty.edu/term/kind/ChemicalName">
    <skos:notation>CN</skos:notation>
    <dct:description>Term is the chemical name for the descriptor. Used in AAT only.
Example: "sodium tetraborate decahydrate" is chemical name for "borax"</dct:description>
    <skos:prefLabel>Chemical Name</skos:prefLabel>
    <rdf:type rdf:resource="http://www.w3.org/2004/02/skos/core#Concept"/>
    <skos:inScheme rdf:resource="http://vocab.getty.edu/term/kind/"/>
    <skos:example>"sodium tetraborate decahydrate" is chemical name for "borax"</skos:example>
    <skos:scopeNote>Term is the chemical name for the descriptor. Used in AAT only</skos:scopeNote>
  </rdf:Description>
  <rdf:Description rdf:about="http://vocab.getty.edu/term/kind/ISOnumeric3">
    <dct:description>ISO 3166-1 numeric country code as "ISOnnn" (though ISO specifies only "nnn"). Used in TGN only.
Example: "ISO414" for Kuwait</dct:description>
    <rdf:type rdf:resource="http://www.w3.org/2004/02/skos/core#Concept"/>
    <skos:notation>ISO3N</skos:notation>
    <skos:prefLabel>ISO numeric-3 code</skos:prefLabel>
    <skos:example>"ISO414" for Kuwait</skos:example>
    <skos:inScheme rdf:resource="http://vocab.getty.edu/term/kind/"/>
    <skos:scopeNote>ISO 3166-1 numeric country code as "ISOnnn" (though ISO specifies only "nnn"). Used in TGN only</skos:scopeNote>
  </rdf:Description>
  <rdf:Description rdf:about="http://vocab.getty.edu/ontology#nationalityPreferred">
    <rdfs:range rdf:resource="http://vocab.getty.edu/ontology#Subject"/>
    <skos:scopeNote>Preferred nationality/culture/race/ethnicity/religion/sexual orientation of an ULAN agent. Domain is schema:Person/Organization, range is AAT concept</skos:scopeNote>
    <rdfs:subPropertyOf rdf:resource="http://schema.org/nationality"/>
    <rdfs:comment>Preferred nationality/culture/race/ethnicity/religion/sexual orientation of an ULAN agent. Domain is schema:Person/Organization, range is AAT concept</rdfs:comment>
    <rdfs:label>nationalityPreferred</rdfs:label>
    <rdf:type rdf:resource="http://www.w3.org/2002/07/owl#ObjectProperty"/>
    <skos:definition>Preferred nationality/culture/race/ethnicity/religion/sexual orientation of an ULAN agent. Domain is schema:Person/Organization, range is AAT concept</skos:definition>
    <rdfs:isDefinedBy rdf:resource="http://vocab.getty.edu/ontology"/>
    <skos:prefLabel>nationalityPreferred</skos:prefLabel>
    <dct:description>Preferred nationality/culture/race/ethnicity/religion/sexual orientation of an ULAN agent. Domain is schema:Person/Organization, range is AAT concept</dct:description>
  </rdf:Description>
  <rdf:Description rdf:nodeID="N42b7ac9239fa49009ec882f6ded18b8e">
    <rdf:first rdf:resource="http://www.w3.org/2008/05/skos-xl#prefLabel"/>
    <rdf:rest rdf:nodeID="Nb968b6a3c4c044e0a4f4e6044cd09dc3"/>
  </rdf:Description>
  <rdf:Description rdf:about="http://vocab.getty.edu/term/kind/FullName">
    <rdf:type rdf:resource="http://www.w3.org/2004/02/skos/core#Concept"/>
    <skos:notation>FN</skos:notation>
    <dct:description>Full Name of an ULAN agent.
Example: TODO</dct:description>
    <skos:inScheme rdf:resource="http://vocab.getty.edu/term/kind/"/>
    <skos:scopeNote>Full Name of an ULAN agent</skos:scopeNote>
    <skos:example>TODO</skos:example>
    <skos:prefLabel>Full Name</skos:prefLabel>
  </rdf:Description>
  <rdf:Description rdf:about="http://vocab.getty.edu/aat/300189559">
    <skos:exactMatch rdf:resource="http://rdaregistry.info/termList/gender/1002"/>
    <skos:exactMatch rdf:resource="http://www.wikidata.org/entity/Q6581097"/>
  </rdf:Description>
  <rdf:Description rdf:about="http://vocab.getty.edu/ontology#ulan2693_president_was">
    <skos:prefLabel>ulan2693_president_was</skos:prefLabel>
    <rdfs:domain rdf:resource="http://www.w3.org/2004/02/skos/core#Concept"/>
    <rdfs:range rdf:resource="http://www.w3.org/2004/02/skos/core#Concept"/>
    <rdfs:isDefinedBy rdf:resource="http://vocab.getty.edu/ulan/"/>
    <skos:scopeNote>institution - president was - person.&#13;
Example: A president of National Gallery of Art was David K. E. Bruce</skos:scopeNote>
    <skos:example>A president of National Gallery of Art was David K. E. Bruce</skos:example>
    <rdfs:subPropertyOf rdf:resource="http://www.w3.org/2004/02/skos/core#related"/>
    <rdfs:isDefinedBy rdf:resource="http://vocab.getty.edu/ontology"/>
    <dc:title>president was - person</dc:title>
    <rdf:type rdf:resource="http://www.w3.org/2002/07/owl#ObjectProperty"/>
    <dct:description>institution - president was - person.&#13;
Example: A president of National Gallery of Art was David K. E. Bruce</dct:description>
    <dc:identifier>2693</dc:identifier>
  </rdf:Description>
  <rdf:Description rdf:about="http://www.w3.org/2004/02/skos/core#altLabel">
    <owl:propertyChainAxiom rdf:nodeID="Na0ee3bfeca0a443a8478a44519eef76e"/>
  </rdf:Description>
  <rdf:Description rdf:nodeID="N44c4d2cbe9fe489fbe561b09d3239654">
    <rdf:first rdf:resource="http://vocab.getty.edu/ontology#broaderInstantialExtended"/>
    <rdf:rest rdf:nodeID="N4f8191fc73ed4f37845b7445e638cdee"/>
  </rdf:Description>
  <rdf:Description rdf:nodeID="N4f8191fc73ed4f37845b7445e638cdee">
    <rdf:first rdf:resource="http://vocab.getty.edu/ontology#broaderGeneric"/>
    <rdf:rest rdf:resource="http://www.w3.org/1999/02/22-rdf-syntax-ns#nil"/>
  </rdf:Description>
  <rdf:Description rdf:nodeID="Na0ee3bfeca0a443a8478a44519eef76e">
    <rdf:rest rdf:nodeID="Nd22a60620bea4ea7ad721eadcab0dd92"/>
    <rdf:first rdf:resource="http://www.w3.org/2008/05/skos-xl#altLabel"/>
  </rdf:Description>
  <rdf:Description rdf:about="http://www.ontotext.com">
    <rdfs:label>Ontotext Corp</rdfs:label>
    <foaf:name>Ontotext Corp</foaf:name>
    <rdf:type rdf:resource="http://xmlns.com/foaf/0.1/Organization"/>
    <skos:prefLabel>Ontotext Corp</skos:prefLabel>
  </rdf:Description>
  <rdf:Description rdf:nodeID="Nb968b6a3c4c044e0a4f4e6044cd09dc3">
    <rdf:rest rdf:resource="http://www.w3.org/1999/02/22-rdf-syntax-ns#nil"/>
    <rdf:first rdf:resource="http://www.w3.org/2008/05/skos-xl#literalForm"/>
  </rdf:Description>
  <rdf:Description rdf:about="http://www.w3.org/2004/02/skos/core#hiddenLabel">
    <owl:propertyChainAxiom rdf:nodeID="N1a416c3537d746a48699cfdbe39976a5"/>
  </rdf:Description>
</rdf:RDF>
